@prefix : <https://w3id.org/emmo/domain/electrochemistry#> .
@prefix dcterms: <http://purl.org/dc/terms/> .
@prefix emmo: <https://w3id.org/emmo#> .
@prefix foaf: <http://xmlns.com/foaf/0.1/> .
@prefix owl: <http://www.w3.org/2002/07/owl#> .
@prefix rdfs: <http://www.w3.org/2000/01/rdf-schema#> .
@prefix skos: <http://www.w3.org/2004/02/skos/core#> .
@prefix xsd: <http://www.w3.org/2001/XMLSchema#> .

dcterms:abstract a owl:AnnotationProperty .

dcterms:license a owl:AnnotationProperty .

dcterms:references a owl:AnnotationProperty .

dcterms:source a owl:AnnotationProperty .

skos:prefLabel a owl:AnnotationProperty .

skos:scopeNote a owl:AnnotationProperty ;
    rdfs:comment "a note that helps to clarify the meaning and/or the use of a concept"@en ;
    emmo:EMMO_967080e5_2f42_4eb2_a3a9_c58143e835f9 "a note that helps to clarify the meaning and/or the use of a concept"@en .

foaf:name a owl:AnnotationProperty .

emmo:EMMO_0fa6566e_500f_4d24_baa9_b2b22c9a0b72 a owl:AnnotationProperty ;
    rdfs:label "warning"@en ;
    rdfs:comment "q critical alert about potential dangers, system failures, or serious misuse of a concept."@en ;
    rdfs:subPropertyOf skos:note ;
    skos:prefLabel "warning"@en ;
    emmo:EMMO_967080e5_2f42_4eb2_a3a9_c58143e835f9 "q critical alert about potential dangers, system failures, or serious misuse of a concept."@en .

emmo:EMMO_1744d51d_0dac_4f48_8b50_fde6c7c2ab39 rdfs:subClassOf :electrochemistry_14d93129_d94d_42ff_a6f2_e8fca36ffec4 .

emmo:EMMO_32214c66_8bce_40f5_b22d_5059f6cf571b a owl:AnnotationProperty ;
    rdfs:label "error"@en ;
    rdfs:comment "marks an error or incorrect usage"@en ;
    rdfs:subPropertyOf skos:note ;
    skos:prefLabel "error"@en ;
    emmo:EMMO_967080e5_2f42_4eb2_a3a9_c58143e835f9 "marks an error or incorrect usage"@en .

emmo:EMMO_4c8480cf_56de_41da_8699_f12a9033313a a owl:AnnotationProperty ;
    rdfs:label "important"@en ;
    rdfs:comment "highlights crucial points users must be aware of"@en ;
    rdfs:subPropertyOf skos:note ;
    skos:prefLabel "important"@en ;
    emmo:EMMO_967080e5_2f42_4eb2_a3a9_c58143e835f9 "highlights crucial points users must be aware of"@en .

emmo:EMMO_50c298c2_55a2_4068_b3ac_4e948c33181f a owl:AnnotationProperty .

emmo:EMMO_5c78b424_087b_4e31_8c91_6422f1be1e86 owl:equivalentClass :electrochemistry_9c657fdc_b9d3_4964_907c_f9a6e8c5f52b .

emmo:EMMO_5f7abc2a_5b50_41c3_8def_c8ba7c3b083e a owl:AnnotationProperty ;
    rdfs:label "tip"@en ;
    rdfs:comment "a best practice or helpful suggestion related to the concept."@en ;
    rdfs:subPropertyOf skos:note ;
    skos:prefLabel "tip"@en ;
    emmo:EMMO_967080e5_2f42_4eb2_a3a9_c58143e835f9 "a best practice or helpful suggestion related to the concept."@en .

emmo:EMMO_709ee08d_76b1_4fee_be22_925412ac313b a owl:AnnotationProperty ;
    rdfs:label "admonition"@en ;
    rdfs:comment "a customized callout for information not covered by default note types"@en ;
    rdfs:subPropertyOf skos:note ;
    skos:prefLabel "admonition"@en ;
    emmo:EMMO_967080e5_2f42_4eb2_a3a9_c58143e835f9 "a customized callout for information not covered by default note types"@en .

emmo:EMMO_931a725b_926d_4f60_8955_61fe17fce98b rdfs:subClassOf :electrochemistry_37b24a94_cae0_4d7a_9519_9f7692dec607 ;
    skos:altLabel "MassDiffusivity"@en ;
    emmo:EMMO_26bf1bef_d192_4da6_b0eb_d2209698fb54 "https://www.wikidata.org/wiki/Q604008"@en ;
    emmo:EMMO_c84c6752_6d64_48cc_9500_e54a3c34898d "https://en.wikipedia.org/wiki/Mass_diffusivity"@en .

emmo:EMMO_95317324_4b53_4665_a087_82c3a2a0540b a owl:AnnotationProperty ;
    rdfs:label "danger"@en ;
    rdfs:comment "indicates a serious risk, often safety-related"@en ;
    rdfs:subPropertyOf skos:note ;
    skos:prefLabel "danger"@en ;
    emmo:EMMO_967080e5_2f42_4eb2_a3a9_c58143e835f9 "indicates a serious risk, often safety-related"@en .

emmo:EMMO_b6730304_cabc_4104_b415_14218466445c a owl:AnnotationProperty ;
    rdfs:label "caution"@en ;
    rdfs:comment "a moderate-level advisory about possible pitfalls, errors, or inefficiencies"@en ;
    rdfs:subPropertyOf skos:note ;
    skos:prefLabel "caution"@en ;
    emmo:EMMO_967080e5_2f42_4eb2_a3a9_c58143e835f9 "a moderate-level advisory about possible pitfalls, errors, or inefficiencies"@en .

emmo:EMMO_cc65321f_1964_4f16_aea3_2a8edf2f3394 a owl:AnnotationProperty ;
    rdfs:label "typicalUnit"@en ;
    rdfs:comment "links a quantity to the typical unit(s) that are commonly used"@en ;
    rdfs:subPropertyOf emmo:EMMO_58e7c821_4af0_4394_89f7_a9649735f4d2 ;
    skos:prefLabel "typicalUnit"@en ;
    emmo:EMMO_967080e5_2f42_4eb2_a3a9_c58143e835f9 "links a quantity to the typical unit(s) that are commonly used"@en .

emmo:EMMO_e6e7277a_1d40_4be5_a3a9_afd3da53d937 rdfs:subClassOf :electrochemistry_25dabdc2_68bf_4a38_8cbe_11be017358bc ;
    :electrochemistry_0a5b99ee_995b_4899_a79b_925a4086da37 "['Parameterisation','Electrolyte','Conductivity [S.m-1]']"@en ;
    :electrochemistry_1b718841_5d72_4071_bb71_fc4a754f5e30 "['electrolyte','ionic_conductivity','value']"@en .

:electrochemistry_0089729b_5890_4c15_aa09_1244d41f8626 a owl:Class ;
    rdfs:label "ImaginaryElectricImpedance"@en ;
    rdfs:comment "the imaginary part of the complex electric impedance"@en ;
    rdfs:subClassOf emmo:EMMO_79a02de5_b884_4eab_bc18_f67997d597a2 ;
    skos:prefLabel "ImaginaryElectricImpedance"@en ;
    emmo:EMMO_967080e5_2f42_4eb2_a3a9_c58143e835f9 "the imaginary part of the complex electric impedance"@en .

:electrochemistry_02d2d1d1_241c_429b_b4e7_31f2c3dc4835 a owl:Class ;
    rdfs:label "D95ParticleSize"@en ;
    rdfs:comment "a statistical measure used in particle size distribution analysis, indicating the particle diameter below which 95% of the sample's particles fall."@en ;
    rdfs:subClassOf emmo:EMMO_c1c8ac3c_8a1c_4777_8e0b_14c1f9f9b0c6 ;
    skos:prefLabel "D95ParticleSize"@en ;
    emmo:EMMO_967080e5_2f42_4eb2_a3a9_c58143e835f9 "a statistical measure used in particle size distribution analysis, indicating the particle diameter below which 95% of the sample's particles fall."@en .

:electrochemistry_05012606_b93d_4016_bbc7_8a927efdf723 a owl:Class ;
    rdfs:label "NPRatio"@en ;
    rdfs:comment "quotient of the capacity of the negative electrode and the capacity of the positive electrode in a cell"@en ;
    rdfs:subClassOf emmo:EMMO_faab3f84_e475_4a46_af9c_7d249f0b9aef,
        :electrochemistry_aecc6094_c6a5_4a36_a825_8a497a2ae112 ;
    skos:altLabel "ACRatio"@en,
        "AToCRatio"@en,
        "NToPRatio"@en ;
    skos:prefLabel "NPRatio"@en ;
    emmo:EMMO_967080e5_2f42_4eb2_a3a9_c58143e835f9 "quotient of the capacity of the negative electrode and the capacity of the positive electrode in a cell"@en .

:electrochemistry_08833ed2_6324_411a_b34b_fe64c44cd5ef a owl:Class ;
    rdfs:label "ConstantCurrentDischargingCapacity"@en ;
    rdfs:comment "the capacity obtained during constant current discharging of an electrochemical device"@en ;
    rdfs:subClassOf :electrochemistry_0141b5c2_9f15_46f4_82e6_92a104faa476 ;
    skos:altLabel "ConstantCurrentDischargeCapacity" ;
    skos:hiddenLabel "DC-Cap"@en,
        "DC-Cap/mAh"@en ;
    skos:prefLabel "ConstantCurrentDischargingCapacity"@en ;
    emmo:EMMO_967080e5_2f42_4eb2_a3a9_c58143e835f9 "the capacity obtained during constant current discharging of an electrochemical device"@en ;
    emmo:EMMO_cc65321f_1964_4f16_aea3_2a8edf2f3394 emmo:AmpereHour,
        emmo:MilliAmpereHour .

:electrochemistry_08b6d07a_0f6c_4932_afbd_fb6b699164ae a owl:Class ;
    rdfs:label "LowerCRateLimit"@en ;
    rdfs:comment "the lower value for C-Rate that is used to indicate a change in an electrochemical measurement process"@en ;
    rdfs:subClassOf :electrochemistry_b395a244_3a75_4737_be38_981bfa1277fe,
        :electrochemistry_e1fd84eb_acdb_4b2c_b90c_e899d552a3ee ;
    skos:prefLabel "LowerCRateLimit"@en ;
    emmo:EMMO_967080e5_2f42_4eb2_a3a9_c58143e835f9 "the lower value for C-Rate that is used to indicate a change in an electrochemical measurement process"@en .

:electrochemistry_097ea615_c209_4edd_a1a1_5eea71d98fe8 a owl:AnnotationProperty ;
    rdfs:label "maccorLabel"@en ;
    rdfs:comment "the label of a term used in resources from Maccor"@en ;
    rdfs:subPropertyOf skos:hiddenLabel ;
    skos:prefLabel "maccorLabel"@en ;
    emmo:EMMO_967080e5_2f42_4eb2_a3a9_c58143e835f9 "the label of a term used in resources from Maccor"@en .

:electrochemistry_098f98dc_e015_4dbd_b358_a7ac3b3ecff3 a owl:Class ;
    rdfs:label "InitialChargeCarrierConcentrationInElectrolyte"@en ;
    rdfs:comment "the initial amount concentration of lithium in an electrolyte"@en ;
    rdfs:subClassOf emmo:EMMO_d5be1faf_0c56_4f5a_9b78_581e6dee949f ;
    skos:prefLabel "InitialChargeCarrierConcentrationInElectrolyte"@en ;
    emmo:EMMO_967080e5_2f42_4eb2_a3a9_c58143e835f9 "the initial amount concentration of lithium in an electrolyte"@en ;
    emmo:EMMO_c7b62dd7_063a_4c2a_8504_42f7264ba83f "this is a very specific term with a narrow conceptualization, used mostly as an anchor term for supporting interoperability; a more general term is suitable in most cases."@en ;
    :electrochemistry_0a5b99ee_995b_4899_a79b_925a4086da37 "['Parameterisation','Electrolyte','Initial concentration [mol.m-3]']"@en ;
    :electrochemistry_1b718841_5d72_4071_bb71_fc4a754f5e30 "['electrolyte','initial_concentration','value']"@en .

:electrochemistry_09e64707_a17d_4405_84cc_ee9d91ed32ef a owl:Class ;
    rdfs:label "VoltageChangeLimit"@en ;
    rdfs:comment "a control limit placed on the rate of change of the cell voltage, dV/dt."@en ;
    rdfs:subClassOf [ a owl:Restriction ;
            owl:onProperty emmo:EMMO_bed1d005_b04e_4a90_94cf_02bc678a8569 ;
            owl:someValuesFrom emmo:EMMO_6837b106_7220_4ec6_b7c9_d549d6163672 ],
        :electrochemistry_c5047d29_4e68_43ee_8355_3e8f05dc70a5,
        :electrochemistry_f6f45881_9bf1_4cf5_988b_de79dab718ef ;
    skos:altLabel "dV/dt"@en ;
    skos:prefLabel "VoltageChangeLimit"@en ;
    emmo:EMMO_967080e5_2f42_4eb2_a3a9_c58143e835f9 "a control limit placed on the rate of change of the cell voltage, dV/dt."@en .

:electrochemistry_0a1e73c5_e91b_4365_88d4_1e1f476bf776 a owl:Class ;
    rdfs:label "PositiveElectrodeActiveMaterialVolumetricSurfaceArea"@en ;
    rdfs:comment "this is a very specific term with a narrow conceptualization, used mostly as an anchor term for supporting interoperability; a more general term is suitable in most cases."@en ;
    rdfs:subClassOf :electrochemistry_a5571263_f153_448f_84a3_cd18092cf8fa ;
    skos:prefLabel "PositiveElectrodeActiveMaterialVolumetricSurfaceArea"@en ;
    emmo:EMMO_967080e5_2f42_4eb2_a3a9_c58143e835f9 "this is a very specific term with a narrow conceptualization, used mostly as an anchor term for supporting interoperability; a more general term is suitable in most cases."@en ;
    :electrochemistry_0a5b99ee_995b_4899_a79b_925a4086da37 "['Parameterisation','Positive electrode','Surface area per unit volume [m-1]']"@en .

:electrochemistry_0a5b99ee_995b_4899_a79b_925a4086da37 a owl:AnnotationProperty ;
    rdfs:label "bpxKey"@en ;
    rdfs:subPropertyOf rdfs:label ;
    skos:prefLabel "bpxKey"@en .

:electrochemistry_0bf1ed19_2fc9_4e6d_87ec_62015985a9a6 a owl:Class ;
    rdfs:label "StepSignalVoltage"@en ;
    rdfs:comment "the magnitude of the voltage step in step voltammetry and related techniques"@en ;
    rdfs:subClassOf [ a owl:Restriction ;
            owl:onProperty emmo:EMMO_bed1d005_b04e_4a90_94cf_02bc678a8569 ;
            owl:someValuesFrom emmo:EMMO_2e7e5796_4a80_4d73_bb84_f31138446c0c ],
        :electrochemistry_c5047d29_4e68_43ee_8355_3e8f05dc70a5 ;
    skos:prefLabel "StepSignalVoltage"@en ;
    emmo:EMMO_967080e5_2f42_4eb2_a3a9_c58143e835f9 "the magnitude of the voltage step in step voltammetry and related techniques"@en .

:electrochemistry_0c9655c6_6b0b_4819_a219_f286ad196fa9 a owl:Class ;
    rdfs:label "InternalConductance"@en ;
    rdfs:comment "inverse of internal resistance"@en,
        "the internal conductance of an electrochemical device"@en ;
    rdfs:subClassOf emmo:EMMO_ffb73b1e_5786_43e4_a964_cb32ac7affb7,
        :electrochemistry_4a450a27_b84a_4c70_a3a9_15ec30e2f30b ;
    skos:prefLabel "InternalConductance"@en ;
    emmo:EMMO_967080e5_2f42_4eb2_a3a9_c58143e835f9 "the internal conductance of an electrochemical device"@en .

:electrochemistry_0ddfd57a_d338_4690_be45_b26884ed6302 a owl:Class ;
    rdfs:label "MinimumStorageTemperature"@en ;
    rdfs:comment "the miniumum temperature at which an electrochemical device shall be stored"@en ;
    rdfs:subClassOf :electrochemistry_4747c51d_86ab_4684_a4fb_b05f5c405ea3 ;
    skos:prefLabel "MinimumStorageTemperature"@en ;
    emmo:EMMO_967080e5_2f42_4eb2_a3a9_c58143e835f9 "the miniumum temperature at which an electrochemical device shall be stored"@en .

:electrochemistry_0e2f4fe6_570a_4d13_81e9_de1d4f9987af a owl:Class ;
    rdfs:label "NegativeElectrodeActiveMaterialOpenCircuitVoltage"@en ;
    rdfs:comment "this is a very specific term with a narrow conceptualization, used mostly as an anchor term for supporting interoperability; a more general term is suitable in most cases."@en ;
    rdfs:subClassOf :electrochemistry_9c657fdc_b9d3_4964_907c_f9a6e8c5f52b ;
    skos:prefLabel "NegativeElectrodeActiveMaterialOpenCircuitVoltage"@en ;
    emmo:EMMO_967080e5_2f42_4eb2_a3a9_c58143e835f9 "this is a very specific term with a narrow conceptualization, used mostly as an anchor term for supporting interoperability; a more general term is suitable in most cases."@en ;
    :electrochemistry_0a5b99ee_995b_4899_a79b_925a4086da37 "['Parameterisation','Negative electrode','OCP [V]']"@en ;
    :electrochemistry_1b718841_5d72_4071_bb71_fc4a754f5e30 "['negative_electrode','active_materials',0,'OCP','value']"@en .

:electrochemistry_0ea21f71_d1bd_4714_a260_b991e6d4bcf7 a owl:Class ;
    rdfs:label "DeviceDensity"@en ;
    rdfs:comment "the overall density of an electrochemical device, calculated as the quotient of the total mass and the total volume"@en ;
    rdfs:subClassOf emmo:EMMO_06448f64_8db6_4304_8b2c_e785dba82044 ;
    skos:prefLabel "DeviceDensity"@en ;
    emmo:EMMO_967080e5_2f42_4eb2_a3a9_c58143e835f9 "the overall density of an electrochemical device, calculated as the quotient of the total mass and the total volume"@en ;
    :electrochemistry_0a5b99ee_995b_4899_a79b_925a4086da37 "['Parameterisation','Cell','Density [kg.m-3]']"@en ;
    :electrochemistry_1b718841_5d72_4071_bb71_fc4a754f5e30 "['properties','density','value']"@en .

:electrochemistry_0ea4d188_9701_4699_a5ca_812a98a9afa7 a owl:Class ;
    rdfs:label "MaximumStorageTemperature"@en ;
    rdfs:comment "the maximum temperature at which an electrochemical device shall be stored"@en ;
    rdfs:subClassOf :electrochemistry_cc519a19_b8d5_4e3f_b893_3a884888ad79 ;
    skos:prefLabel "MaximumStorageTemperature"@en ;
    emmo:EMMO_967080e5_2f42_4eb2_a3a9_c58143e835f9 "the maximum temperature at which an electrochemical device shall be stored"@en .

:electrochemistry_0ed0362e_b7ae_482c_a7d0_2ca2eebda648 a owl:Class ;
    rdfs:label "D30ParticleSize"@en ;
    rdfs:comment "a statistical measure used in particle size distribution analysis, indicating the particle diameter below which 30% of the sample's particles fall."@en ;
    rdfs:subClassOf emmo:EMMO_c1c8ac3c_8a1c_4777_8e0b_14c1f9f9b0c6 ;
    skos:prefLabel "D30ParticleSize"@en ;
    emmo:EMMO_967080e5_2f42_4eb2_a3a9_c58143e835f9 "a statistical measure used in particle size distribution analysis, indicating the particle diameter below which 30% of the sample's particles fall."@en .

:electrochemistry_0f986d97_445f_4075_a5ce_ddde598a47a9 a owl:Class ;
    rdfs:label "TotalEnergy"@en ;
    rdfs:comment "the total amount of energy that has passed through an electrochemical device"@en ;
    rdfs:subClassOf :electrochemistry_46376e5d_9627_4514_9881_9e62083625c3 ;
    skos:prefLabel "TotalEnergy"@en ;
    emmo:EMMO_967080e5_2f42_4eb2_a3a9_c58143e835f9 "the total amount of energy that has passed through an electrochemical device"@en .

:electrochemistry_10104499_6580_4867_9c5d_b9882c89c2f7 a owl:Class ;
    rdfs:label "DifferentialCapacity"@en ;
    rdfs:comment "the derivative of the capacity of an electrochemical device with respect to the terminal voltage"@en ;
    rdfs:subClassOf :electrochemistry_aecc6094_c6a5_4a36_a825_8a497a2ae112 ;
    skos:altLabel "dQ/dV"@en ;
    skos:prefLabel "DifferentialCapacity"@en ;
    emmo:EMMO_967080e5_2f42_4eb2_a3a9_c58143e835f9 "the derivative of the capacity of an electrochemical device with respect to the terminal voltage"@en ;
    :electrochemistry_811aafc3_0c6d_470e_b67e_ff5c82992609 "dQ/dV(mAh/V)"@en .

:electrochemistry_10eb778d_da60_4832_a355_4ee74baea650 a owl:Class ;
    rdfs:label "AmplitudeOfAlternatingCurrent"@en ;
    rdfs:comment "half the peak-to-peak amplitude of a sinusoidal alternating current"@en ;
    rdfs:subClassOf emmo:EMMO_c995ae70_3b84_4ebb_bcfc_69e6a281bb88,
        :electrochemistry_c5047d29_4e68_43ee_8355_3e8f05dc70a5 ;
    skos:prefLabel "AmplitudeOfAlternatingCurrent"@en ;
    emmo:EMMO_967080e5_2f42_4eb2_a3a9_c58143e835f9 "half the peak-to-peak amplitude of a sinusoidal alternating current"@en ;
    emmo:EMMO_fe015383_afb3_44a6_ae86_043628697aa2 "https://doi.org/10.1351/goldbook.A00310" .

:electrochemistry_129926b6_fc30_441d_b359_29b44c988514 a owl:Class ;
    rdfs:label "ElectrochemicalWindow"@en ;
    rdfs:comment "The electrode electric potential range between which the substance is neither oxidized nor reduced."@en ;
    rdfs:subClassOf emmo:EMMO_4f2d3939_91b1_4001_b8ab_7d19074bf845,
        :electrochemistry_2d896559_eee3_447c_9759_87c854a4266a ;
    skos:altLabel "ElectrochemicalStabilityWindow"@en ;
    skos:prefLabel "ElectrochemicalWindow"@en ;
    emmo:EMMO_26bf1bef_d192_4da6_b0eb_d2209698fb54 "https://www.wikidata.org/wiki/Q759643" ;
    emmo:EMMO_967080e5_2f42_4eb2_a3a9_c58143e835f9 "The electrode electric potential range between which the substance is neither oxidized nor reduced."@en ;
    emmo:EMMO_c84c6752_6d64_48cc_9500_e54a3c34898d "https://en.wikipedia.org/wiki/Electrochemical_window"@en .

:electrochemistry_1acab8af_9798_45df_a64b_a7030c57a4de a owl:Class ;
    rdfs:label "DepthOfDischarge"@en ;
    rdfs:comment "the ratio of the discharged capacity to the rated capacity of an electrochemical device"@en ;
    rdfs:subClassOf emmo:EMMO_faab3f84_e475_4a46_af9c_7d249f0b9aef,
        :electrochemistry_aecc6094_c6a5_4a36_a825_8a497a2ae112 ;
    skos:altLabel "DoD"@en ;
    skos:prefLabel "DepthOfDischarge"@en ;
    emmo:EMMO_967080e5_2f42_4eb2_a3a9_c58143e835f9 "the ratio of the discharged capacity to the rated capacity of an electrochemical device"@en ;
    emmo:EMMO_c84c6752_6d64_48cc_9500_e54a3c34898d "https://en.wikipedia.org/wiki/Depth_of_discharge" .

:electrochemistry_1b2a7137_64d4_483a_8437_dcb3bedcb6da a owl:Class ;
    rdfs:label "MaximumPulseChargingCurrent"@en ;
    rdfs:comment "the maximum current approved for pulse charge of an electrochemical device"@en ;
    rdfs:subClassOf :electrochemistry_74de2c33_84fc_4c2f_afe1_56d169149114 ;
    skos:altLabel "MaximumPulseChargeCurrent"@en ;
    skos:prefLabel "MaximumPulseChargingCurrent"@en ;
    emmo:EMMO_967080e5_2f42_4eb2_a3a9_c58143e835f9 "the maximum current approved for pulse charge of an electrochemical device"@en .

:electrochemistry_1b717a20_17e3_4480_8c60_c4ae94058f05 a owl:AnnotationProperty ;
    rdfs:label "batteryArchiveLabel"@en ;
    rdfs:comment "the label of a term used in resources from Battery Archive"@en ;
    rdfs:subPropertyOf skos:hiddenLabel ;
    skos:prefLabel "batteryArchiveLabel"@en ;
    emmo:EMMO_967080e5_2f42_4eb2_a3a9_c58143e835f9 "the label of a term used in resources from Battery Archive"@en .

:electrochemistry_1b718841_5d72_4071_bb71_fc4a754f5e30 a owl:AnnotationProperty ;
    rdfs:label "cidemodKey"@en ;
    rdfs:subPropertyOf rdfs:label ;
    skos:prefLabel "cidemodKey"@en .

:electrochemistry_1be95f7c_7381_4d60_a4fb_25b3db63be97 a owl:Class ;
    rdfs:label "D65ParticleSize"@en ;
    rdfs:comment "a statistical measure used in particle size distribution analysis, indicating the particle diameter below which 10% of the sample's particles fall."@en ;
    rdfs:subClassOf emmo:EMMO_c1c8ac3c_8a1c_4777_8e0b_14c1f9f9b0c6 ;
    skos:prefLabel "D65ParticleSize"@en ;
    emmo:EMMO_967080e5_2f42_4eb2_a3a9_c58143e835f9 "a statistical measure used in particle size distribution analysis, indicating the particle diameter below which 10% of the sample's particles fall."@en .

:electrochemistry_1cdeedbf_7f9a_4e1f_a297_204a6e16b718 a owl:Class ;
    rdfs:label "MaximumStorageEnergy"@en ;
    rdfs:comment "the maximum amount of energy that can be reversible stored within an electrochemical device, component, or material - operated at an infinitely low rate - based on its chemical composition and design"@en ;
    rdfs:subClassOf :electrochemistry_da215d1a_196a_465f_9de8_89f6fbb76982 ;
    skos:prefLabel "MaximumStorageEnergy"@en ;
    emmo:EMMO_967080e5_2f42_4eb2_a3a9_c58143e835f9 "the maximum amount of energy that can be reversible stored within an electrochemical device, component, or material - operated at an infinitely low rate - based on its chemical composition and design"@en .

:electrochemistry_1eeb0e2a_229a_43f1_b197_348d475067ff a owl:Class ;
    rdfs:label "ActiveMassLoading"@en ;
    rdfs:comment "the mass of active material per unit area"@en ;
    rdfs:subClassOf :electrochemistry_c955c089_6ee1_41a2_95fc_d534c5cfd3d5 ;
    skos:prefLabel "ActiveMassLoading"@en ;
    emmo:EMMO_967080e5_2f42_4eb2_a3a9_c58143e835f9 "the mass of active material per unit area"@en .

:electrochemistry_21da0fe9_9fb6_4840_a12f_fbcc1ba84fb3 a owl:Class ;
    rdfs:label "NegativeElectrodeActiveMaterialGuestStoichiometricCoefficientAtSOC0"@en ;
    rdfs:comment "this is a very specific term with a narrow conceptualization, used mostly as an anchor term for supporting interoperability; a more general term is suitable in most cases."@en ;
    rdfs:subClassOf :electrochemistry_f22bd1ec_faca_4335_92a5_a1687154c622 ;
    skos:prefLabel "NegativeElectrodeActiveMaterialGuestStoichiometricCoefficientAtSOC0"@en ;
    emmo:EMMO_967080e5_2f42_4eb2_a3a9_c58143e835f9 "this is a very specific term with a narrow conceptualization, used mostly as an anchor term for supporting interoperability; a more general term is suitable in most cases."@en ;
    :electrochemistry_0a5b99ee_995b_4899_a79b_925a4086da37 "['Parameterisation','Negative electrode','Minimum stoichiometry']"@en ;
    :electrochemistry_1b718841_5d72_4071_bb71_fc4a754f5e30 "['negative_electrode','active_materials',0,'stoichiometry0','value']"@en .

:electrochemistry_2678a656_4a27_4706_8dde_b0a93e9b92fa a owl:Class ;
    rdfs:label "RestingTime"@en ;
    rdfs:comment "the duration during which an electrochemical device is kept at open-circuit conditions"@en ;
    rdfs:subClassOf emmo:EMMO_0adabf6f_7404_44cb_9f65_32d83d8101a3,
        :electrochemistry_c5047d29_4e68_43ee_8355_3e8f05dc70a5 ;
    skos:altLabel "RestingDuration"@en ;
    skos:prefLabel "RestingTime"@en ;
    emmo:EMMO_967080e5_2f42_4eb2_a3a9_c58143e835f9 "the duration during which an electrochemical device is kept at open-circuit conditions"@en .

:electrochemistry_27b3799c_250c_4332_8b71_7992c4a7bb05 a owl:Class ;
    rdfs:label "TestTime"@en ;
    rdfs:comment "time of a measurement relative to the start of the test (t = 0)"@en ;
    rdfs:subClassOf emmo:EMMO_d4f7d378_5e3b_468a_baa1_a7e98358cda7,
        :electrochemistry_aecc6094_c6a5_4a36_a825_8a497a2ae112 ;
    skos:altLabel "RunTime"@en ;
    skos:hiddenLabel "TestTime/Sec"@en,
        "time/s"@en ;
    skos:prefLabel "TestTime"@en ;
    emmo:EMMO_967080e5_2f42_4eb2_a3a9_c58143e835f9 "time of a measurement relative to the start of the test (t = 0)"@en ;
    :electrochemistry_097ea615_c209_4edd_a1a1_5eea71d98fe8 "test (sec)"@en ;
    :electrochemistry_1b717a20_17e3_4480_8c60_c4ae94058f05 "Test_Time (s)"@en ;
    :electrochemistry_811aafc3_0c6d_470e_b67e_ff5c82992609 "Time(h:min:s.ms)"@en ;
    :electrochemistry_8377c1f7_2b09_4632_9a4d_bb318438adbb "time_s"@en ;
    :electrochemistry_a07dd85b_d0df_4d5d_8b0c_14d20ea3fe45 "test_time"@en ;
    :electrochemistry_ea9f4dba_8ca2_419e_9cdf_ce54e9ebbd46 "Run Time (h)"@en .

:electrochemistry_2a1de79f_e927_45a2_9619_3799a0d61e9b a owl:Class ;
    rdfs:label "MinimumDischargingTemperature"@en ;
    rdfs:comment "the minimum allowable temperature of an electrochemical device during a discharging process"@en ;
    rdfs:subClassOf :electrochemistry_4747c51d_86ab_4684_a4fb_b05f5c405ea3 ;
    skos:prefLabel "MinimumDischargingTemperature"@en ;
    emmo:EMMO_967080e5_2f42_4eb2_a3a9_c58143e835f9 "the minimum allowable temperature of an electrochemical device during a discharging process"@en .

:electrochemistry_2ab7af60_da58_4243_b3bc_cbb2155cac53 a owl:Class ;
    rdfs:label "ChargingEnergy"@en ;
    rdfs:comment "energy delivered by a deviced under some specific charge conditions"@en ;
    rdfs:subClassOf :electrochemistry_46376e5d_9627_4514_9881_9e62083625c3 ;
    skos:altLabel "ChargeEnergy" ;
    skos:hiddenLabel "Energy charge/W.h"@en,
        "EnergyC"@en,
        "EnergyC/mWh"@en,
        "WH-IN"@en ;
    skos:prefLabel "ChargingEnergy"@en ;
    emmo:EMMO_967080e5_2f42_4eb2_a3a9_c58143e835f9 "energy delivered by a deviced under some specific charge conditions"@en ;
    :electrochemistry_097ea615_c209_4edd_a1a1_5eea71d98fe8 "wf chg e"@en ;
    :electrochemistry_1b717a20_17e3_4480_8c60_c4ae94058f05 "Charge_Energy (Wh)"@en ;
    :electrochemistry_69022178_77b8_4669_97e2_351d45356e5a "Energy charge/W.h"@en ;
    :electrochemistry_811aafc3_0c6d_470e_b67e_ff5c82992609 "Engy_Chg(mWh)"@en ;
    :electrochemistry_a07dd85b_d0df_4d5d_8b0c_14d20ea3fe45 "charge_energy"@en .

:electrochemistry_2c0e66c8_d58d_44b2_b0ce_ba55194bd505 a owl:Class ;
    rdfs:label "WeightPercent"@en ;
    rdfs:comment "the percentage quantity relating the weight of a constituent to the total weight"@en ;
    rdfs:subClassOf :electrochemistry_cf386c1e_e62b_43ef_9b0e_e5e58935d63f ;
    skos:prefLabel "WeightPercent"@en ;
    emmo:EMMO_967080e5_2f42_4eb2_a3a9_c58143e835f9 "the percentage quantity relating the weight of a constituent to the total weight"@en .

:electrochemistry_2c4c2626_7db5_440c_a65e_95ed2986ee01 a owl:Class ;
    rdfs:label "InitialCondition"@en ;
    rdfs:comment "the initial value of a property at the start of a simulation or experiment"@en ;
    rdfs:subClassOf :electrochemistry_33e6986c_b35a_4cae_9a94_acb23248065c ;
    skos:prefLabel "InitialCondition"@en ;
    emmo:EMMO_967080e5_2f42_4eb2_a3a9_c58143e835f9 "the initial value of a property at the start of a simulation or experiment"@en .

:electrochemistry_2cfea66b_756d_4642_986f_9a41abbd7034 a owl:Class ;
    rdfs:label "InactiveMassLoading"@en ;
    rdfs:comment "the mass of inactive material per unit area"@en ;
    rdfs:subClassOf :electrochemistry_c955c089_6ee1_41a2_95fc_d534c5cfd3d5 ;
    skos:prefLabel "InactiveMassLoading"@en ;
    emmo:EMMO_967080e5_2f42_4eb2_a3a9_c58143e835f9 "the mass of inactive material per unit area"@en .

:electrochemistry_2d58b059_2ef0_418e_9337_13aa2de4b07f a owl:Class ;
    rdfs:label "StepType"@en ;
    rdfs:comment "a description (usually an integer, string, or alpha numeric code) describing the nature of a step in an electrochemical test protocol"@en ;
    rdfs:subClassOf :electrochemistry_aecc6094_c6a5_4a36_a825_8a497a2ae112 ;
    skos:altLabel "State"@en ;
    skos:prefLabel "StepType"@en ;
    emmo:EMMO_967080e5_2f42_4eb2_a3a9_c58143e835f9 "a description (usually an integer, string, or alpha numeric code) describing the nature of a step in an electrochemical test protocol"@en ;
    :electrochemistry_097ea615_c209_4edd_a1a1_5eea71d98fe8 "state"@en ;
    :electrochemistry_ea9f4dba_8ca2_419e_9cdf_ce54e9ebbd46 "Step Type"@en .

:electrochemistry_2e2d92f4_9fd5_4965_b15a_30b43c68e3e5 a owl:Class ;
    rdfs:label "D5ParticleSize"@en ;
    rdfs:comment "a statistical measure used in particle size distribution analysis, indicating the particle diameter below which 5% of the sample's particles fall."@en ;
    rdfs:subClassOf emmo:EMMO_c1c8ac3c_8a1c_4777_8e0b_14c1f9f9b0c6 ;
    skos:prefLabel "D5ParticleSize"@en ;
    emmo:EMMO_967080e5_2f42_4eb2_a3a9_c58143e835f9 "a statistical measure used in particle size distribution analysis, indicating the particle diameter below which 5% of the sample's particles fall."@en .

:electrochemistry_31a74e23_bb07_41d0_bb8f_1d8cca157503 a owl:Class ;
    rdfs:label "ChargingEnergyDensity"@en ;
    rdfs:comment "the energy density of a device obtained during a charging process"@en ;
    rdfs:subClassOf :electrochemistry_4aa1b96e_44a0_4b1a_a0ac_723d0223d80b ;
    skos:prefLabel "ChargingEnergyDensity"@en ;
    emmo:EMMO_967080e5_2f42_4eb2_a3a9_c58143e835f9 "the energy density of a device obtained during a charging process"@en .

:electrochemistry_372c89d0_adab_4585_9662_33c912acef23 a owl:Class ;
    rdfs:label "TheoreticalCapacity"@en ;
    rdfs:comment "the amount of electric charge that can be stored in a material, component, or device, under infinitely low current, and derived from first principles"@en ;
    rdfs:subClassOf :electrochemistry_9b3b4668_0795_4a35_9965_2af383497a26 ;
    skos:prefLabel "TheoreticalCapacity"@en ;
    emmo:EMMO_967080e5_2f42_4eb2_a3a9_c58143e835f9 "the amount of electric charge that can be stored in a material, component, or device, under infinitely low current, and derived from first principles"@en ;
    emmo:EMMO_b6730304_cabc_4104_b415_14218466445c "The value of the practically achieve able capacity is often much lower than the theoretical value."@en ;
    emmo:EMMO_cc65321f_1964_4f16_aea3_2a8edf2f3394 emmo:AmpereHour,
        emmo:Coulomb,
        emmo:MilliAmpereHour .

:electrochemistry_37c38b7e_9ded_481a_85fd_a467f1ee2b9f a owl:Class ;
    rdfs:label "ConstantCurrentChargingCapacity"@en ;
    rdfs:comment "the capacity obtained during constant current charging of an electrochemical device"@en ;
    rdfs:seeAlso :electrochemistry_0cc8f231_0ce5_467e_9c76_29b2c80349ad,
        :electrochemistry_a7a4614f_2426_46f3_8475_cda4a9fabfce ;
    rdfs:subClassOf :electrochemistry_10763eb0_dbc9_4d34_bd1a_7b8996590d45 ;
    skos:altLabel "ConstantCurrentChargeCapacity" ;
    skos:hiddenLabel "CC-Cap"@en,
        "CC-Cap/mAh"@en ;
    skos:prefLabel "ConstantCurrentChargingCapacity"@en ;
    skos:scopeNote "Constant current charging capacity is often used to assess device performance and state-of-health. In a CC-CV charging process, if this value is significantly lower than the rated capacity under the same conditions, it may indicate underlying limitations. A decline over multiple cycles can be a sign of degradation."@en ;
    emmo:EMMO_967080e5_2f42_4eb2_a3a9_c58143e835f9 "the capacity obtained during constant current charging of an electrochemical device"@en ;
    emmo:EMMO_cc65321f_1964_4f16_aea3_2a8edf2f3394 emmo:AmpereHour,
        emmo:MilliAmpereHour .

:electrochemistry_398c6427_320d_4df7_bd09_55931eed4922 a owl:Class ;
    rdfs:label "AmperePerAmpereHour"@en ;
    rdfs:comment "the unit for C-Rate in electrochemistry and related domains"@en ;
    rdfs:subClassOf :electrochemistry_67930f7b_ad4c_4b21_9b2e_a000e5c153ae ;
    skos:prefLabel "AmperePerAmpereHour"@en ;
    emmo:EMMO_967080e5_2f42_4eb2_a3a9_c58143e835f9 "the unit for C-Rate in electrochemistry and related domains"@en .

:electrochemistry_39a44af0_0e1a_4859_b550_bdabad64386e a owl:Class ;
    rdfs:label "AmbientThermodynamicTemperature"@en ;
    rdfs:comment "the ambient thermodynamic temperature"@en ;
    rdfs:subClassOf emmo:EMMO_affe07e4_e9bc_4852_86c6_69e26182a17f ;
    skos:prefLabel "AmbientThermodynamicTemperature"@en ;
    emmo:EMMO_967080e5_2f42_4eb2_a3a9_c58143e835f9 "the ambient thermodynamic temperature"@en .

:electrochemistry_39d8a6ee_cd55_4855_8b5b_d42bef95ac78 a owl:Class ;
    rdfs:label "MaximumContinuousChargingCurrent"@en ;
    rdfs:comment "the maximum current approved for continuous charge for a given electrochemical device"@en ;
    rdfs:subClassOf :electrochemistry_74de2c33_84fc_4c2f_afe1_56d169149114 ;
    skos:altLabel "MaximumContinuousChargeCurrent"@en ;
    skos:prefLabel "MaximumContinuousChargingCurrent"@en ;
    emmo:EMMO_967080e5_2f42_4eb2_a3a9_c58143e835f9 "the maximum current approved for continuous charge for a given electrochemical device"@en .

:electrochemistry_3cfdfc10_a5cb_4e3e_b1a1_281010d1465c a owl:Class ;
    rdfs:label "D50ParticleSize"@en ;
    rdfs:comment "a statistical measure used in particle size distribution analysis, indicating the particle diameter below which 50% of the sample's particles fall."@en,
        "in particle size distribution measurements, the mass-median-diameter, considered to be the average particle size by mass"@en ;
    rdfs:subClassOf emmo:EMMO_c1c8ac3c_8a1c_4777_8e0b_14c1f9f9b0c6,
        :electrochemistry_aecc6094_c6a5_4a36_a825_8a497a2ae112 ;
    skos:altLabel "MassMedianDiameter"@en ;
    skos:prefLabel "D50ParticleSize"@en ;
    emmo:EMMO_967080e5_2f42_4eb2_a3a9_c58143e835f9 "a statistical measure used in particle size distribution analysis, indicating the particle diameter below which 50% of the sample's particles fall."@en .

:electrochemistry_3dac5115_6337_40a6_a2ab_317087fe3b45 a owl:Class ;
    rdfs:label "UpperCurrentLimit"@en ;
    rdfs:comment "the upper bounding limit on the current used in the definition of an electrochemical testing protocol"@en ;
    rdfs:subClassOf :electrochemistry_74de2c33_84fc_4c2f_afe1_56d169149114 ;
    skos:prefLabel "UpperCurrentLimit"@en ;
    emmo:EMMO_967080e5_2f42_4eb2_a3a9_c58143e835f9 "the upper bounding limit on the current used in the definition of an electrochemical testing protocol"@en .

:electrochemistry_3e54f9e3_a31d_4821_9bfb_ef953a42c35b a owl:Class ;
    rdfs:label "MaximumPulseDischargingCurrent"@en ;
    rdfs:comment "the maximum current approved for pulse discharge of an electrochemical device"@en ;
    rdfs:subClassOf :electrochemistry_346519a4_006c_496d_8f36_74e38814ed2d,
        :electrochemistry_74de2c33_84fc_4c2f_afe1_56d169149114 ;
    skos:altLabel "MaximumPulseDischargeCurrent"@en ;
    skos:prefLabel "MaximumPulseDischargingCurrent"@en ;
    emmo:EMMO_967080e5_2f42_4eb2_a3a9_c58143e835f9 "the maximum current approved for pulse discharge of an electrochemical device"@en .

:electrochemistry_404126e0_cb1b_44e4_98dc_2474185767a1 a owl:Class ;
    rdfs:label "PositiveElectrodeReactionRateConstant"@en ;
    rdfs:comment "this is a very specific term with a narrow conceptualization, used mostly as an anchor term for supporting interoperability; a more general term is suitable in most cases."@en ;
    rdfs:subClassOf :electrochemistry_0335e3f6_d1d8_4daa_8376_a9285f1bc9f1 ;
    skos:prefLabel "PositiveElectrodeReactionRateConstant"@en ;
    emmo:EMMO_967080e5_2f42_4eb2_a3a9_c58143e835f9 "this is a very specific term with a narrow conceptualization, used mostly as an anchor term for supporting interoperability; a more general term is suitable in most cases."@en ;
    :electrochemistry_0a5b99ee_995b_4899_a79b_925a4086da37 "['Parameterisation','Positive electrode','Reaction rate constant [mol.m-2.s-1]']"@en ;
    :electrochemistry_1b718841_5d72_4071_bb71_fc4a754f5e30 "['positive_electrode','active_materials',0,'kinetic_constant','value']"@en .

:electrochemistry_43f77743_1af6_4a0f_9cc6_285c2a450549 a owl:Class ;
    rdfs:label "PositiveElectrodeElectronicConductivity"@en ;
    rdfs:comment "this is a very specific term with a narrow conceptualization, used mostly as an anchor term for supporting interoperability; a more general term is suitable in most cases."@en ;
    rdfs:subClassOf :electrochemistry_ce74d2dc_d496_4116_b2fb_3e83d88bc744 ;
    skos:prefLabel "PositiveElectrodeElectronicConductivity"@en ;
    emmo:EMMO_967080e5_2f42_4eb2_a3a9_c58143e835f9 "this is a very specific term with a narrow conceptualization, used mostly as an anchor term for supporting interoperability; a more general term is suitable in most cases."@en ;
    :electrochemistry_0a5b99ee_995b_4899_a79b_925a4086da37 "['Parameterisation','Positive electrode','Conductivity [S.m-1]']"@en ;
    :electrochemistry_1b718841_5d72_4071_bb71_fc4a754f5e30 "['positive_electrode','electronic_conductivity','value']"@en .

:electrochemistry_44a67eb4_52e8_433c_aef7_a928c2b9906c a owl:Class ;
    rdfs:label "TerminationQuantity"@en ;
    rdfs:comment "a quantity that is used to express the termination criteria for an electrochemical process"@en ;
    rdfs:subClassOf :electrochemistry_c5047d29_4e68_43ee_8355_3e8f05dc70a5 ;
    skos:prefLabel "TerminationQuantity"@en ;
    emmo:EMMO_967080e5_2f42_4eb2_a3a9_c58143e835f9 "a quantity that is used to express the termination criteria for an electrochemical process"@en .

:electrochemistry_457aed58_6e7e_42d5_9d78_b424c8d60aa3 a owl:Class ;
    rdfs:label "DischargingConstantCurrentPercentage"@en ;
    rdfs:comment "the percentage of the total discharge capacity that is obtained during a constant current discharge process"@en ;
    rdfs:subClassOf emmo:EMMO_faab3f84_e475_4a46_af9c_7d249f0b9aef ;
    skos:altLabel "ConstantCurrentDischargePercentage"@en ;
    skos:hiddenLabel "DC-Per"@en,
        "DC-Per/%"@en ;
    skos:prefLabel "DischargingConstantCurrentPercentage"@en ;
    emmo:EMMO_967080e5_2f42_4eb2_a3a9_c58143e835f9 "the percentage of the total discharge capacity that is obtained during a constant current discharge process"@en .

:electrochemistry_463950b9_fd8d_48de_a52d_b29cab026391 a owl:Class ;
    rdfs:label "DeviceTemperature"@en ;
    rdfs:comment "the temperature of an electrochemical device"@en ;
    rdfs:subClassOf emmo:EMMO_66bc9029_f473_45ff_bab9_c3509ff37a22 ;
    skos:prefLabel "DeviceTemperature"@en ;
    emmo:EMMO_967080e5_2f42_4eb2_a3a9_c58143e835f9 "the temperature of an electrochemical device"@en ;
    :electrochemistry_1b717a20_17e3_4480_8c60_c4ae94058f05 "Cell_Temperature (C)"@en .

:electrochemistry_47288277_4aed_447e_b659_0c975d031406 a owl:Class ;
    rdfs:label "SeparatorThickness"@en ;
    rdfs:comment "the thickness of a separator"@en ;
    rdfs:subClassOf emmo:EMMO_43003c86_9d15_433b_9789_ee2940920656 ;
    skos:prefLabel "SeparatorThickness"@en ;
    emmo:EMMO_967080e5_2f42_4eb2_a3a9_c58143e835f9 "the thickness of a separator"@en ;
    :electrochemistry_0a5b99ee_995b_4899_a79b_925a4086da37 "['Parameterisation','Separator','Thickness [m]']"@en ;
    :electrochemistry_1b718841_5d72_4071_bb71_fc4a754f5e30 "['separator','thickness','value']"@en .

:electrochemistry_482173dc_7779_4f12_982c_b19f2cda2dac a owl:Class ;
    rdfs:label "NumberOfCellsConnectedInParallel"@en ;
    rdfs:comment "the number of electrochemical cells connected in parallel"@en ;
    rdfs:subClassOf emmo:EMMO_41efdf5d_0c9c_4ea0_bb65_f8236e663be5,
        :electrochemistry_aecc6094_c6a5_4a36_a825_8a497a2ae112 ;
    skos:prefLabel "NumberOfCellsConnectedInParallel"@en ;
    emmo:EMMO_967080e5_2f42_4eb2_a3a9_c58143e835f9 "the number of electrochemical cells connected in parallel"@en .

:electrochemistry_4882cf2f_aab7_4a3a_a103_7f56b55fbed3 a owl:Class ;
    rdfs:label "ChargingSpecificCapacity"@en ;
    rdfs:comment "quotient of the capacity of a cell or battery [ or electrode or active material ] obtained during a charge process by its mass."@en ;
    rdfs:subClassOf :electrochemistry_1e3dc60d_dd6b_47d6_8161_70004fc5ee30 ;
    skos:altLabel "SpecificChargeCapacity"@en ;
    skos:hiddenLabel "SpeCapC"@en,
        "SpeCapC/mAh/g"@en ;
    skos:prefLabel "ChargingSpecificCapacity"@en ;
    emmo:EMMO_967080e5_2f42_4eb2_a3a9_c58143e835f9 "quotient of the capacity of a cell or battery [ or electrode or active material ] obtained during a charge process by its mass."@en .

:electrochemistry_4a30ff40_3ffa_4a08_9134_36dbe718bee1 a owl:Class ;
    rdfs:label "TotalDuration"@en ;
    rdfs:comment "the total duration of a test"@en ;
    rdfs:subClassOf emmo:EMMO_0adabf6f_7404_44cb_9f65_32d83d8101a3 ;
    skos:prefLabel "TotalDuration"@en ;
    emmo:EMMO_967080e5_2f42_4eb2_a3a9_c58143e835f9 "the total duration of a test"@en .

:electrochemistry_4a354510_4dc2_4803_8845_f4024a1a7260 a owl:Class ;
    rdfs:label "MaximumChargingTemperature"@en ;
    rdfs:comment "the maximum allowable temperature of an electrochemical device during a charging process"@en ;
    rdfs:subClassOf :electrochemistry_cc519a19_b8d5_4e3f_b893_3a884888ad79 ;
    skos:prefLabel "MaximumChargingTemperature"@en ;
    emmo:EMMO_967080e5_2f42_4eb2_a3a9_c58143e835f9 "the maximum allowable temperature of an electrochemical device during a charging process"@en .

:electrochemistry_4b18c3f9_df10_4259_adb4_cd10842ff0be a owl:Class ;
    rdfs:label "DropTimeInPolarography"@en ;
    rdfs:comment "the time that elapses between the instants at which two successive drops of liquid metal are detached from the tip of the capillary."@en ;
    rdfs:subClassOf emmo:EMMO_0adabf6f_7404_44cb_9f65_32d83d8101a3,
        :electrochemistry_aecc6094_c6a5_4a36_a825_8a497a2ae112 ;
    skos:prefLabel "DropTimeInPolarography"@en ;
    emmo:EMMO_967080e5_2f42_4eb2_a3a9_c58143e835f9 "the time that elapses between the instants at which two successive drops of liquid metal are detached from the tip of the capillary."@en ;
    emmo:EMMO_fe015383_afb3_44a6_ae86_043628697aa2 "https://doi.org/10.1351/goldbook.D01862"@en .

:electrochemistry_4c274506_af5b_4ef1_8217_829ffd459f28 a owl:Class ;
    rdfs:label "ChargeCarrierDiffusivityInElectrolyte"@en ;
    rdfs:comment "the diffusivity of lithium in an electrolyte"@en ;
    rdfs:subClassOf :electrochemistry_37b24a94_cae0_4d7a_9519_9f7692dec607 ;
    skos:prefLabel "ChargeCarrierDiffusivityInElectrolyte"@en ;
    emmo:EMMO_967080e5_2f42_4eb2_a3a9_c58143e835f9 "the diffusivity of lithium in an electrolyte"@en ;
    emmo:EMMO_c7b62dd7_063a_4c2a_8504_42f7264ba83f "this is a very specific term with a narrow conceptualization, used mostly as an anchor term for supporting interoperability; a more general term is suitable in most cases."@en ;
    :electrochemistry_0a5b99ee_995b_4899_a79b_925a4086da37 "['Parameterisation','Electrolyte','Diffusivity [m2.s-1]']"@en ;
    :electrochemistry_1b718841_5d72_4071_bb71_fc4a754f5e30 "['electrolyte','diffusion_constant','value']"@en .

:electrochemistry_4d2b102b_3515_4591_b079_69232c44f9dc a owl:Class ;
    rdfs:label "PulseVoltage"@en ;
    rdfs:comment "The magnitude of a voltage pulse applied to an electrochemical cell during pulsed amperometry and related techniques."@en ;
    rdfs:subClassOf :electrochemistry_4ebe2ef1_eea8_4b10_822d_7a68215bd24d,
        :electrochemistry_c5047d29_4e68_43ee_8355_3e8f05dc70a5 ;
    skos:altLabel "MagnitudeOfPotentialPulse"@en,
        "PulseMagnitudePotential"@en ;
    skos:prefLabel "PulseVoltage"@en ;
    emmo:EMMO_967080e5_2f42_4eb2_a3a9_c58143e835f9 "The magnitude of a voltage pulse applied to an electrochemical cell during pulsed amperometry and related techniques."@en .

:electrochemistry_4d69edda_d2fa_40b0_9c1e_52e08debf578 a owl:Class ;
    rdfs:label "ActivationEnergyOfGuestDiffusivityInPositiveElectrodeActiveMaterial"@en ;
    rdfs:comment "the activation energy barrier in an Arrhenius expression for the diffusivity of lithium in the positive electrode"@en ;
    rdfs:subClassOf :electrochemistry_d7f8cab9_b035_4ecd_be63_292672572526 ;
    skos:prefLabel "ActivationEnergyOfGuestDiffusivityInPositiveElectrodeActiveMaterial"@en ;
    emmo:EMMO_967080e5_2f42_4eb2_a3a9_c58143e835f9 "the activation energy barrier in an Arrhenius expression for the diffusivity of lithium in the positive electrode"@en ;
    emmo:EMMO_c7b62dd7_063a_4c2a_8504_42f7264ba83f "this is a very specific term with a narrow conceptualization, used mostly as an anchor term for supporting interoperability; a more general term is suitable in most cases."@en ;
    :electrochemistry_0a5b99ee_995b_4899_a79b_925a4086da37 "['Parameterisation','Positive electrode','Diffusivity activation energy [J.mol-1]']"@en ;
    :electrochemistry_1b718841_5d72_4071_bb71_fc4a754f5e30 "['positive_electrode','active_materials',0,'diffusion_constant','arrhenius','activation_energy']"@en .

:electrochemistry_4f14e153_cffb_42bd_9a7f_ae40d51ad2cd a owl:Class ;
    rdfs:label "DischargingEnergyDensity"@en ;
    rdfs:comment "the energy density of a device obtained during a discharging process."@en ;
    rdfs:subClassOf :electrochemistry_4aa1b96e_44a0_4b1a_a0ac_723d0223d80b ;
    skos:prefLabel "DischargingEnergyDensity"@en ;
    emmo:EMMO_967080e5_2f42_4eb2_a3a9_c58143e835f9 "the energy density of a device obtained during a discharging process."@en .

:electrochemistry_50247e71_75fe_4986_959e_fd06c6be98db a owl:Class ;
    rdfs:label "GuestDiffusivityInNegativeElectrodeActiveMaterial"@en ;
    rdfs:comment "the diffusivity of lithium in the negative electrode"@en ;
    rdfs:subClassOf :electrochemistry_37b24a94_cae0_4d7a_9519_9f7692dec607 ;
    skos:prefLabel "GuestDiffusivityInNegativeElectrodeActiveMaterial"@en ;
    emmo:EMMO_967080e5_2f42_4eb2_a3a9_c58143e835f9 "the diffusivity of lithium in the negative electrode"@en ;
    emmo:EMMO_c7b62dd7_063a_4c2a_8504_42f7264ba83f "this is a very specific term with a narrow conceptualization, used mostly as an anchor term for supporting interoperability; a more general term is suitable in most cases."@en ;
    :electrochemistry_0a5b99ee_995b_4899_a79b_925a4086da37 "['Parameterisation','Negative electrode','Diffusivity [m2.s-1]']"@en ;
    :electrochemistry_1b718841_5d72_4071_bb71_fc4a754f5e30 "['negative_electrode','active_materials',0,'diffusion_constant','value']"@en .

:electrochemistry_520995f8_ec9c_4b3c_bb64_2cd691947379 a owl:Class ;
    rdfs:label "CalenderedDensity"@en ;
    rdfs:comment "density after calendering"@en ;
    rdfs:subClassOf emmo:EMMO_06448f64_8db6_4304_8b2c_e785dba82044,
        :electrochemistry_aecc6094_c6a5_4a36_a825_8a497a2ae112 ;
    skos:prefLabel "CalenderedDensity"@en ;
    emmo:EMMO_967080e5_2f42_4eb2_a3a9_c58143e835f9 "density after calendering"@en .

:electrochemistry_52ab4fdd_f945_4541_9ce6_cd6fd3a05861 a owl:Class ;
    rdfs:label "PositiveElectrodeActiveMaterialOpenCircuitVoltage"@en ;
    rdfs:comment "this is a very specific term with a narrow conceptualization, used mostly as an anchor term for supporting interoperability; a more general term is suitable in most cases."@en ;
    rdfs:subClassOf :electrochemistry_9c657fdc_b9d3_4964_907c_f9a6e8c5f52b ;
    skos:prefLabel "PositiveElectrodeActiveMaterialOpenCircuitVoltage"@en ;
    emmo:EMMO_967080e5_2f42_4eb2_a3a9_c58143e835f9 "this is a very specific term with a narrow conceptualization, used mostly as an anchor term for supporting interoperability; a more general term is suitable in most cases."@en ;
    :electrochemistry_0a5b99ee_995b_4899_a79b_925a4086da37 "['Parameterisation','Positive electrode','OCP [V]']"@en ;
    :electrochemistry_1b718841_5d72_4071_bb71_fc4a754f5e30 "['positive_electrode','active_materials',0,'OCP','value']"@en .

:electrochemistry_56b9cd1f_5397_4385_9292_30d93d9e7a05 a owl:Class ;
    rdfs:label "PostiveElectrodeActivationEnergyOfReaction"@en ;
    rdfs:comment "the activation energy barrier in an Arrhenius expression for the positive electrode charge transfer reaction"@en ;
    rdfs:subClassOf :electrochemistry_d7f8cab9_b035_4ecd_be63_292672572526 ;
    skos:prefLabel "PostiveElectrodeActivationEnergyOfReaction"@en ;
    emmo:EMMO_967080e5_2f42_4eb2_a3a9_c58143e835f9 "the activation energy barrier in an Arrhenius expression for the positive electrode charge transfer reaction"@en ;
    :electrochemistry_0a5b99ee_995b_4899_a79b_925a4086da37 "['Parameterisation','Positive electrode','Reaction rate constant activation energy [J.mol-1]']"@en .

:electrochemistry_56de36fe_e8e1_486c_8d29_061ac8d28c13 a owl:Class ;
    rdfs:label "ActivationEnergyOfChargeCarrierDiffusivityInElectrolyte"@en ;
    rdfs:comment "the activation energy barrier in an Arrhenius expression for the diffusivity of lithium in an electrolyte"@en ;
    rdfs:subClassOf :electrochemistry_d7f8cab9_b035_4ecd_be63_292672572526 ;
    skos:prefLabel "ActivationEnergyOfChargeCarrierDiffusivityInElectrolyte"@en ;
    emmo:EMMO_967080e5_2f42_4eb2_a3a9_c58143e835f9 "the activation energy barrier in an Arrhenius expression for the diffusivity of lithium in an electrolyte"@en ;
    emmo:EMMO_c7b62dd7_063a_4c2a_8504_42f7264ba83f "this is a very specific term with a narrow conceptualization, used mostly as an anchor term for supporting interoperability; a more general term is suitable in most cases."@en ;
    :electrochemistry_0a5b99ee_995b_4899_a79b_925a4086da37 "['Parameterisation','Electrolyte','Diffusivity activation energy [J.mol-1]']"@en ;
    :electrochemistry_1b718841_5d72_4071_bb71_fc4a754f5e30 "['electrolyte','diffusion_constant','arrhenius','activation_energy']"@en .

:electrochemistry_5766a819_c319_48ba_ab9a_ce3bd8fedee8 a owl:Class ;
    rdfs:label "CycleIndex"@en ;
    rdfs:comment "the number of charge-discharge cycles that an electrochemical device has experienced"@en ;
    rdfs:subClassOf emmo:EMMO_ba882f34_0d71_4e4f_9d92_0c076c633a2c,
        :electrochemistry_aecc6094_c6a5_4a36_a825_8a497a2ae112 ;
    skos:altLabel "Cycle"@en,
        "CycleNumber"@en ;
    skos:hiddenLabel "Cycle-Index"@en,
        "CycleNo"@en ;
    skos:prefLabel "CycleIndex"@en ;
    emmo:EMMO_967080e5_2f42_4eb2_a3a9_c58143e835f9 "the number of charge-discharge cycles that an electrochemical device has experienced"@en ;
    :electrochemistry_097ea615_c209_4edd_a1a1_5eea71d98fe8 "cyc#"@en ;
    :electrochemistry_1b717a20_17e3_4480_8c60_c4ae94058f05 "Cycle_Index"@en ;
    :electrochemistry_69022178_77b8_4669_97e2_351d45356e5a "cycle number"@en ;
    :electrochemistry_811aafc3_0c6d_470e_b67e_ff5c82992609 "Cycle ID"@en ;
    :electrochemistry_8377c1f7_2b09_4632_9a4d_bb318438adbb "cycle_count"@en ;
    :electrochemistry_a07dd85b_d0df_4d5d_8b0c_14d20ea3fe45 "cycle_index"@en ;
    :electrochemistry_ea9f4dba_8ca2_419e_9cdf_ce54e9ebbd46 "Cycle Number"@en .

:electrochemistry_58400817_3282_46e5_942e_3a1538631403 a owl:Class ;
    rdfs:label "PositiveElectrodeActiveMaterialParticleRadius"@en ;
    rdfs:comment "this is a very specific term with a narrow conceptualization, used mostly as an anchor term for supporting interoperability; a more general term is suitable in most cases."@en ;
    rdfs:subClassOf :electrochemistry_b92e382f_5109_4f60_ab5e_c89d340419a9 ;
    skos:prefLabel "PositiveElectrodeActiveMaterialParticleRadius"@en ;
    emmo:EMMO_967080e5_2f42_4eb2_a3a9_c58143e835f9 "this is a very specific term with a narrow conceptualization, used mostly as an anchor term for supporting interoperability; a more general term is suitable in most cases."@en ;
    :electrochemistry_0a5b99ee_995b_4899_a79b_925a4086da37 "['Parameterisation','Positive electrode','Particle radius [m]']"@en ;
    :electrochemistry_1b718841_5d72_4071_bb71_fc4a754f5e30 "['positive_electrode','active_materials',0,'particle_radius','value']"@en .

:electrochemistry_5973f91a_fa6b_49c9_ba46_3ecc1c2253d2 a owl:Class ;
    rdfs:label "InstantaneousPower"@en ;
    rdfs:comment "for a two-terminal element or a two-terminal circuit with terminals A and B, product of the voltage uAB between the terminals and the electric current i in the element or circuit"@en ;
    rdfs:subClassOf emmo:EMMO_09b9021b_f97b_43eb_b83d_0a764b472bc2 ;
    skos:prefLabel "InstantaneousPower"@en ;
    emmo:EMMO_50c298c2_55a2_4068_b3ac_4e948c33181f "https://www.electropedia.org/iev/iev.nsf/display?openform&ievref=131-11-30"@en ;
    emmo:EMMO_967080e5_2f42_4eb2_a3a9_c58143e835f9 "for a two-terminal element or a two-terminal circuit with terminals A and B, product of the voltage uAB between the terminals and the electric current i in the element or circuit"@en ;
    :electrochemistry_811aafc3_0c6d_470e_b67e_ff5c82992609 "Power(mW)"@en ;
    :electrochemistry_8377c1f7_2b09_4632_9a4d_bb318438adbb "cell_power_w"@en .

:electrochemistry_5cb403c4_4f28_46cb_81c4_21c5c47ef14a a owl:Class ;
    rdfs:label "NegativeElectrodeCoatingPorosity"@en ;
    rdfs:comment "this is a very specific term with a narrow conceptualization, used mostly as an anchor term for supporting interoperability; a more general term is suitable in most cases."@en ;
    rdfs:subClassOf emmo:EMMO_3a6578ac_aee0_43b9_9bc6_1eb208c8c9a9 ;
    skos:prefLabel "NegativeElectrodeCoatingPorosity"@en ;
    emmo:EMMO_967080e5_2f42_4eb2_a3a9_c58143e835f9 "this is a very specific term with a narrow conceptualization, used mostly as an anchor term for supporting interoperability; a more general term is suitable in most cases."@en ;
    :electrochemistry_0a5b99ee_995b_4899_a79b_925a4086da37 "['Parameterisation','Negative electrode','Porosity']"@en ;
    :electrochemistry_1b718841_5d72_4071_bb71_fc4a754f5e30 "['negative_electrode','porosity','value']"@en .

:electrochemistry_5ce6a328_713c_4383_ad63_26c902c30e34 a owl:Class ;
    rdfs:label "TappedDensity"@en ;
    rdfs:comment "the density of a powdered or granular material when it is subjected to tapping or mechanical vibration"@en ;
    rdfs:subClassOf emmo:EMMO_06448f64_8db6_4304_8b2c_e785dba82044 ;
    skos:altLabel "TapDensity"@en ;
    skos:prefLabel "TappedDensity"@en ;
    emmo:EMMO_967080e5_2f42_4eb2_a3a9_c58143e835f9 "the density of a powdered or granular material when it is subjected to tapping or mechanical vibration"@en .

:electrochemistry_5e4490b8_c1dd_4e00_980b_c484e1bf4904 a owl:Class ;
    rdfs:label "ChargingSpecificEnergy"@en ;
    rdfs:comment "the specific energy of an electrochemical device obtained during a charge process"@en ;
    rdfs:subClassOf emmo:EMMO_e218c625_6a39_47a9_8d08_a2ef41c152a9 ;
    skos:altLabel "SpecificEnergyCharge" ;
    skos:hiddenLabel "SpeEnergyC"@en,
        "SpeEnergyC/mWh/g"@en ;
    skos:prefLabel "ChargingSpecificEnergy"@en ;
    emmo:EMMO_967080e5_2f42_4eb2_a3a9_c58143e835f9 "the specific energy of an electrochemical device obtained during a charge process"@en .

:electrochemistry_62e03250_8987_497b_85d5_1399aca9a0aa a owl:Class ;
    rdfs:label "D20ParticleSize"@en ;
    rdfs:comment "a statistical measure used in particle size distribution analysis, indicating the particle diameter below which 20% of the sample's particles fall."@en ;
    rdfs:subClassOf emmo:EMMO_c1c8ac3c_8a1c_4777_8e0b_14c1f9f9b0c6 ;
    skos:prefLabel "D20ParticleSize"@en ;
    emmo:EMMO_967080e5_2f42_4eb2_a3a9_c58143e835f9 "a statistical measure used in particle size distribution analysis, indicating the particle diameter below which 20% of the sample's particles fall."@en .

:electrochemistry_62f5beeb_6d1e_442a_8048_3ebe08882964 a owl:Class ;
    rdfs:label "PositiveElectrodeCoatingThickness"@en ;
    rdfs:comment "thickness of the positive electrode coating"@en ;
    rdfs:subClassOf :electrochemistry_3b938708_e7e4_4ac0_a959_9c04306302e7 ;
    skos:prefLabel "PositiveElectrodeCoatingThickness"@en ;
    emmo:EMMO_967080e5_2f42_4eb2_a3a9_c58143e835f9 "thickness of the positive electrode coating"@en ;
    emmo:EMMO_c7b62dd7_063a_4c2a_8504_42f7264ba83f "this is a very specific term with a narrow conceptualization, used mostly as an anchor term for supporting interoperability; a more general term is suitable in most cases."@en ;
    :electrochemistry_0a5b99ee_995b_4899_a79b_925a4086da37 "['Parameterisation','Positive electrode','Thickness [m]']"@en ;
    :electrochemistry_1b718841_5d72_4071_bb71_fc4a754f5e30 "['positive_electrode','thickness','value']"@en .

:electrochemistry_6516ed26_9661_4d81_8c6d_15d2384d17c0 a owl:Class ;
    rdfs:label "CurrentChangeRate"@en ;
    rdfs:comment "the first order time rate of change of electric current"@en ;
    rdfs:subClassOf :electrochemistry_aecc6094_c6a5_4a36_a825_8a497a2ae112 ;
    skos:prefLabel "CurrentChangeRate"@en ;
    emmo:EMMO_967080e5_2f42_4eb2_a3a9_c58143e835f9 "the first order time rate of change of electric current"@en ;
    :electrochemistry_ea9f4dba_8ca2_419e_9cdf_ce54e9ebbd46 "dIdt (V/h)"@en .

:electrochemistry_666f0b69_9c74_49a3_80b3_96a188332462 a owl:Class ;
    rdfs:label "UpperFrequencyLimit"@en ;
    rdfs:comment "the higher end of the interval of frequencies tested in impedimetry and related techniques"@en ;
    rdfs:subClassOf emmo:EMMO_852b4ab8_fc29_4749_a8c7_b92d4fca7d5a,
        :electrochemistry_c5047d29_4e68_43ee_8355_3e8f05dc70a5 ;
    skos:prefLabel "UpperFrequencyLimit"@en ;
    emmo:EMMO_967080e5_2f42_4eb2_a3a9_c58143e835f9 "the higher end of the interval of frequencies tested in impedimetry and related techniques"@en .

:electrochemistry_6769536b_5320_4b48_a2d8_ac285ec635a8 a owl:Class ;
    rdfs:label "StepSignalCurrent"@en ;
    rdfs:comment "the magnitude of the current step in chronopotentiometry and related techniques"@en ;
    rdfs:subClassOf emmo:EMMO_c995ae70_3b84_4ebb_bcfc_69e6a281bb88,
        :electrochemistry_c5047d29_4e68_43ee_8355_3e8f05dc70a5 ;
    skos:prefLabel "StepSignalCurrent"@en ;
    emmo:EMMO_967080e5_2f42_4eb2_a3a9_c58143e835f9 "the magnitude of the current step in chronopotentiometry and related techniques"@en .

:electrochemistry_69022178_77b8_4669_97e2_351d45356e5a a owl:AnnotationProperty ;
    rdfs:label "biologicLabel"@en ;
    rdfs:comment "the label of a term used in resources from Biologic"@en ;
    rdfs:subPropertyOf skos:hiddenLabel ;
    skos:prefLabel "biologicLabel"@en ;
    emmo:EMMO_967080e5_2f42_4eb2_a3a9_c58143e835f9 "the label of a term used in resources from Biologic"@en .

:electrochemistry_6d981c04_3ace_4f1b_b0f8_770776cceb6f a owl:Class ;
    rdfs:label "TotalNumberOfCycles"@en ;
    rdfs:comment "the total number of cycles carried out on a specific device under a given set of conditions"@en ;
    rdfs:subClassOf emmo:EMMO_ba882f34_0d71_4e4f_9d92_0c076c633a2c,
        :electrochemistry_aecc6094_c6a5_4a36_a825_8a497a2ae112 ;
    skos:prefLabel "TotalNumberOfCycles"@en ;
    emmo:EMMO_967080e5_2f42_4eb2_a3a9_c58143e835f9 "the total number of cycles carried out on a specific device under a given set of conditions"@en .

:electrochemistry_6dcd5baf_58cd_43f5_a692_51508e036c88 a owl:Class ;
    rdfs:label "UpperVoltageLimit"@en ;
    rdfs:comment "maximum voltage limit at which an applied excitation is altered or terminated"@en ;
    rdfs:subClassOf :electrochemistry_5ebeea80_af22_456b_9087_78c2a8465c58 ;
    skos:altLabel "EndOfChargeVoltage"@en,
        "UpperCutoffVoltage"@en ;
    skos:prefLabel "UpperVoltageLimit"@en ;
    emmo:EMMO_50c298c2_55a2_4068_b3ac_4e948c33181f "https://www.electropedia.org/iev/iev.nsf/display?openform&ievref=482-05-55" ;
    emmo:EMMO_967080e5_2f42_4eb2_a3a9_c58143e835f9 "maximum voltage limit at which an applied excitation is altered or terminated"@en ;
    emmo:EMMO_c7b62dd7_063a_4c2a_8504_42f7264ba83f "term used in the context of primary and secondary cells and batteries"@en .

:electrochemistry_7104c722_d5a5_4bff_ba2f_37e229bb6cce a owl:AnnotationProperty ;
    rdfs:label "includeDocs"@en ;
    rdfs:range xsd:boolean ;
    rdfs:subPropertyOf rdfs:comment ;
    skos:prefLabel "includeDocs"@en .

:electrochemistry_71f10616_15eb_4dc4_bc8d_ffaac3838af2 a owl:Class ;
    rdfs:label "CurrentChangeLimit"@en ;
    rdfs:comment "the limit on the value of the time change of the electric current"@en ;
    rdfs:subClassOf :electrochemistry_c5047d29_4e68_43ee_8355_3e8f05dc70a5 ;
    skos:prefLabel "CurrentChangeLimit"@en ;
    emmo:EMMO_967080e5_2f42_4eb2_a3a9_c58143e835f9 "the limit on the value of the time change of the electric current"@en .

:electrochemistry_73f169de_d189_4d7c_893f_a2549771825c a owl:Class ;
    rdfs:label "RecoveredCapacity"@en ;
    rdfs:comment "the capacity that can be obtained from an electrochemical device after it has been subjected to some specified conditions, then recharged and discharged according to a recommended protocol"@en ;
    rdfs:subClassOf :electrochemistry_9b3b4668_0795_4a35_9965_2af383497a26 ;
    skos:altLabel "RecoveryCapacity"@en ;
    skos:prefLabel "RecoveredCapacity"@en ;
    emmo:EMMO_967080e5_2f42_4eb2_a3a9_c58143e835f9 "the capacity that can be obtained from an electrochemical device after it has been subjected to some specified conditions, then recharged and discharged according to a recommended protocol"@en ;
    emmo:EMMO_cc65321f_1964_4f16_aea3_2a8edf2f3394 emmo:AmpereHour,
        emmo:MilliAmpereHour .

:electrochemistry_7481c4c9_c247_4248_a045_a1077230acba a owl:Class ;
    rdfs:label "PositiveElectrodeCoatingPorosity"@en ;
    rdfs:comment "this is a very specific term with a narrow conceptualization, used mostly as an anchor term for supporting interoperability; a more general term is suitable in most cases."@en ;
    rdfs:subClassOf emmo:EMMO_3a6578ac_aee0_43b9_9bc6_1eb208c8c9a9 ;
    skos:prefLabel "PositiveElectrodeCoatingPorosity"@en ;
    emmo:EMMO_967080e5_2f42_4eb2_a3a9_c58143e835f9 "this is a very specific term with a narrow conceptualization, used mostly as an anchor term for supporting interoperability; a more general term is suitable in most cases."@en ;
    :electrochemistry_0a5b99ee_995b_4899_a79b_925a4086da37 "['Parameterisation','Positive electrode','Porosity']"@en ;
    :electrochemistry_1b718841_5d72_4071_bb71_fc4a754f5e30 "['positive_electrode','porosity','value']"@en .

:electrochemistry_762ba55f_9b56_4c31_865f_cff2e7d0a94b a owl:Class ;
    rdfs:label "PulseMagnitude"@en ;
    rdfs:comment "a single value, for instance a mean, root mean square or peak value characterizing the aggregate instantaneous values of a unidirectional pulse with respect to the common initial and final value"@en ;
    rdfs:subClassOf emmo:EMMO_dd4a7f3e_ef56_466c_ac1a_d2716b5f87ec ;
    skos:prefLabel "PulseMagnitude"@en ;
    emmo:EMMO_50c298c2_55a2_4068_b3ac_4e948c33181f "https://www.electropedia.org/iev/iev.nsf/display?openform&ievref=702-03-03" ;
    emmo:EMMO_967080e5_2f42_4eb2_a3a9_c58143e835f9 "a single value, for instance a mean, root mean square or peak value characterizing the aggregate instantaneous values of a unidirectional pulse with respect to the common initial and final value"@en .

:electrochemistry_77f9d496_555e_4ae2_ae80_f297ef8335ca a owl:Class ;
    rdfs:label "FaradayConstant"@en ;
    rdfs:comment "fundamental physical constant representing molar elementary charge"@en ;
    rdfs:subClassOf emmo:EMMO_f2ca6dd0_0e5f_4392_a92d_cafdae6cfc95,
        :electrochemistry_aecc6094_c6a5_4a36_a825_8a497a2ae112 ;
    skos:prefLabel "FaradayConstant"@en ;
    emmo:EMMO_26bf1bef_d192_4da6_b0eb_d2209698fb54 "https://www.wikidata.org/wiki/Q192819" ;
    emmo:EMMO_967080e5_2f42_4eb2_a3a9_c58143e835f9 "fundamental physical constant representing molar elementary charge"@en ;
    emmo:EMMO_c84c6752_6d64_48cc_9500_e54a3c34898d "https://en.wikipedia.org/wiki/Faraday_constant"@en ;
    emmo:EMMO_fe015383_afb3_44a6_ae86_043628697aa2 "https://doi.org/10.1351/goldbook.F02325"@en .

:electrochemistry_79551e01_4bc6_4292_916e_08fe28a84600 a owl:Class ;
    rdfs:label "ChargingCurrent"@en ;
    rdfs:comment "electric current applied to an electrochemical device during a charging process"@en ;
    rdfs:subClassOf :electrochemistry_637ee9c4_4b3f_4d3a_975b_c0572dfe53ce,
        :electrochemistry_aecc6094_c6a5_4a36_a825_8a497a2ae112 ;
    owl:disjointWith :electrochemistry_e4d666ee_d637_45cd_a904_dc33941ead4f ;
    skos:prefLabel "ChargingCurrent"@en ;
    emmo:EMMO_967080e5_2f42_4eb2_a3a9_c58143e835f9 "electric current applied to an electrochemical device during a charging process"@en .

:electrochemistry_79a9e1be_35b0_4c3c_8087_b5f967ca0e87 a owl:Class ;
    rdfs:label "ChargingVoltage"@en ;
    rdfs:comment "voltage between the terminals of a cell or battery when being charged"@en ;
    rdfs:subClassOf :electrochemistry_4ebe2ef1_eea8_4b10_822d_7a68215bd24d ;
    skos:prefLabel "ChargingVoltage"@en ;
    emmo:EMMO_967080e5_2f42_4eb2_a3a9_c58143e835f9 "voltage between the terminals of a cell or battery when being charged"@en .

:electrochemistry_7db845e7_0e5b_47d4_b954_2a2b8e85deea a owl:Class ;
    rdfs:label "LowerCurrentLimit"@en ;
    rdfs:comment "the lower bounding limit on the current used in the definition of an electrochemical testing protocol"@en ;
    rdfs:subClassOf :electrochemistry_74de2c33_84fc_4c2f_afe1_56d169149114 ;
    skos:prefLabel "LowerCurrentLimit"@en ;
    emmo:EMMO_967080e5_2f42_4eb2_a3a9_c58143e835f9 "the lower bounding limit on the current used in the definition of an electrochemical testing protocol"@en .

:electrochemistry_7f073272_8925_4344_995c_a5a6dd1fcde6 a owl:Class ;
    rdfs:label "ChargingConstantCurrentPercentage"@en ;
    rdfs:comment "the percentage of the total charge capacity that is obtained during a constant current charge process"@en ;
    rdfs:subClassOf emmo:EMMO_faab3f84_e475_4a46_af9c_7d249f0b9aef ;
    skos:altLabel "ConstantCurrentChargePercentage"@en ;
    skos:hiddenLabel "CC-Per"@en,
        "CC-Per/%"@en ;
    skos:prefLabel "ChargingConstantCurrentPercentage"@en ;
    emmo:EMMO_967080e5_2f42_4eb2_a3a9_c58143e835f9 "the percentage of the total charge capacity that is obtained during a constant current charge process"@en .

:electrochemistry_7f17f6bb_c1f9_4f4a_bfdf_d8974443d07b a owl:Class ;
    rdfs:label "D25ParticleSize"@en ;
    rdfs:comment "a statistical measure used in particle size distribution analysis, indicating the particle diameter below which 25% of the sample's particles fall."@en ;
    rdfs:subClassOf emmo:EMMO_c1c8ac3c_8a1c_4777_8e0b_14c1f9f9b0c6 ;
    skos:prefLabel "D25ParticleSize"@en ;
    emmo:EMMO_967080e5_2f42_4eb2_a3a9_c58143e835f9 "a statistical measure used in particle size distribution analysis, indicating the particle diameter below which 25% of the sample's particles fall."@en .

:electrochemistry_7f381c19_cf07_47a8_ab10_0b14d46901e8 a owl:Class ;
    rdfs:label "SurfaceAreaPerVolume"@en ;
    rdfs:comment "the quotient of the surface area of some object and its total volume"@en ;
    rdfs:subClassOf emmo:EMMO_2946d40b_24a1_47fa_8176_e3f79bb45064 ;
    skos:prefLabel "SurfaceAreaPerVolume"@en ;
    emmo:EMMO_967080e5_2f42_4eb2_a3a9_c58143e835f9 "the quotient of the surface area of some object and its total volume"@en .

:electrochemistry_7fe804b8_6126_4132_be8f_b4985d61b1f6 a owl:Class ;
    rdfs:label "MolarElectrochemicalPotential"@en ;
    rdfs:comment "Of a substance in a specified phase, the partial molar Gibbs energy of the substance at the specified electric potential."@en,
        "electrochemical potential per mole."@en ;
    rdfs:subClassOf [ a owl:Restriction ;
            owl:onProperty emmo:EMMO_bed1d005_b04e_4a90_94cf_02bc678a8569 ;
            owl:someValuesFrom emmo:EMMO_0972cb08_48bd_4524_ac03_8a2e7f30f02f ],
        emmo:EMMO_2946d40b_24a1_47fa_8176_e3f79bb45064,
        :electrochemistry_2d896559_eee3_447c_9759_87c854a4266a ;
    skos:prefLabel "MolarElectrochemicalPotential"@en ;
    emmo:EMMO_967080e5_2f42_4eb2_a3a9_c58143e835f9 "electrochemical potential per mole."@en ;
    emmo:EMMO_fe015383_afb3_44a6_ae86_043628697aa2 "https://goldbook.iupac.org/terms/view/E01945" .

:electrochemistry_80920875_62ac_4e29_b970_ec4316e76aa5 a owl:Class ;
    rdfs:label "PositiveElectrodeActiveMaterialGuestStoichiometricCoefficientAtSOC0"@en ;
    rdfs:comment "this is a very specific term with a narrow conceptualization, used mostly as an anchor term for supporting interoperability; a more general term is suitable in most cases."@en ;
    rdfs:subClassOf :electrochemistry_f22bd1ec_faca_4335_92a5_a1687154c622 ;
    skos:prefLabel "PositiveElectrodeActiveMaterialGuestStoichiometricCoefficientAtSOC0"@en ;
    emmo:EMMO_967080e5_2f42_4eb2_a3a9_c58143e835f9 "this is a very specific term with a narrow conceptualization, used mostly as an anchor term for supporting interoperability; a more general term is suitable in most cases."@en ;
    :electrochemistry_0a5b99ee_995b_4899_a79b_925a4086da37 "['Parameterisation','Positive electrode','Minimum stoichiometry']"@en ;
    :electrochemistry_1b718841_5d72_4071_bb71_fc4a754f5e30 "['positive_electrode','active_materials',0,'stoichiometry0','value']"@en .

:electrochemistry_80ca00f8_c891_4493_87a2_7d39b9d1e098 a owl:Class ;
    rdfs:label "StepTime"@en ;
    rdfs:comment "time of a measurement relative to the start of the step (t = 0)"@en ;
    rdfs:subClassOf emmo:EMMO_d4f7d378_5e3b_468a_baa1_a7e98358cda7,
        :electrochemistry_aecc6094_c6a5_4a36_a825_8a497a2ae112 ;
    skos:hiddenLabel "StepTime/Sec"@en ;
    skos:prefLabel "StepTime"@en ;
    emmo:EMMO_967080e5_2f42_4eb2_a3a9_c58143e835f9 "time of a measurement relative to the start of the step (t = 0)"@en ;
    :electrochemistry_097ea615_c209_4edd_a1a1_5eea71d98fe8 "step (sec)"@en ;
    :electrochemistry_a07dd85b_d0df_4d5d_8b0c_14d20ea3fe45 "step_time"@en ;
    :electrochemistry_ea9f4dba_8ca2_419e_9cdf_ce54e9ebbd46 "Step Time (h)"@en .

:electrochemistry_811aafc3_0c6d_470e_b67e_ff5c82992609 a owl:AnnotationProperty ;
    rdfs:label "newareLabel"@en ;
    rdfs:comment "the label of a term used in resources from Neware"@en ;
    rdfs:subPropertyOf skos:hiddenLabel ;
    skos:prefLabel "newareLabel"@en ;
    emmo:EMMO_967080e5_2f42_4eb2_a3a9_c58143e835f9 "the label of a term used in resources from Neware"@en .

:electrochemistry_8177eae6_1631_430d_99f2_942669bcb784 a owl:Class ;
    rdfs:label "IonConcentration"@en ;
    rdfs:comment "the amount concentration of some ionic species in a given volume of solution"@en ;
    rdfs:subClassOf emmo:EMMO_d5be1faf_0c56_4f5a_9b78_581e6dee949f,
        :electrochemistry_2d896559_eee3_447c_9759_87c854a4266a ;
    skos:prefLabel "IonConcentration"@en ;
    emmo:EMMO_50c298c2_55a2_4068_b3ac_4e948c33181f "https://www.electropedia.org/iev/iev.nsf/display?openform&ievref=114-01-16" ;
    emmo:EMMO_967080e5_2f42_4eb2_a3a9_c58143e835f9 "the amount concentration of some ionic species in a given volume of solution"@en .

:electrochemistry_8377c1f7_2b09_4632_9a4d_bb318438adbb a owl:AnnotationProperty ;
    rdfs:label "indigoLabel"@en ;
    rdfs:comment "the label of a term used in resources from Indigo"@en ;
    rdfs:subPropertyOf skos:hiddenLabel ;
    skos:prefLabel "indigoLabel"@en ;
    emmo:EMMO_967080e5_2f42_4eb2_a3a9_c58143e835f9 "the label of a term used in resources from Indigo"@en .

:electrochemistry_838a927f_775e_4c6d_8e39_7865548608c2 a owl:Class ;
    rdfs:label "Record"@en ;
    rdfs:comment "an entry in a dataset, typically consisting of one line."@en ;
    rdfs:subClassOf :electrochemistry_aecc6094_c6a5_4a36_a825_8a497a2ae112 ;
    skos:hiddenLabel "Rec#"@en ;
    skos:prefLabel "Record"@en ;
    emmo:EMMO_967080e5_2f42_4eb2_a3a9_c58143e835f9 "an entry in a dataset, typically consisting of one line."@en .

:electrochemistry_8541f8b7_c55e_452d_b3f8_db29dcb2a61d a owl:Class ;
    rdfs:label "TotalMassLoading"@en ;
    rdfs:comment "the mass of all material (active and inactive) per unit area"@en ;
    rdfs:subClassOf :electrochemistry_c955c089_6ee1_41a2_95fc_d534c5cfd3d5 ;
    skos:prefLabel "TotalMassLoading"@en ;
    emmo:EMMO_967080e5_2f42_4eb2_a3a9_c58143e835f9 "the mass of all material (active and inactive) per unit area"@en .

:electrochemistry_85e39686_9658_4c74_bb91_a935704c174a a owl:Class ;
    rdfs:label "StepDuration"@en ;
    rdfs:comment "the duration between two consecutive steps in a staircase signal"@en ;
    rdfs:subClassOf emmo:EMMO_0adabf6f_7404_44cb_9f65_32d83d8101a3,
        :electrochemistry_c5047d29_4e68_43ee_8355_3e8f05dc70a5 ;
    skos:prefLabel "StepDuration"@en ;
    emmo:EMMO_967080e5_2f42_4eb2_a3a9_c58143e835f9 "the duration between two consecutive steps in a staircase signal"@en ;
    emmo:EMMO_c7b62dd7_063a_4c2a_8504_42f7264ba83f "Typically, the duration is defined between the onset of one step and the onset of the next step."@en .

:electrochemistry_86324806_4263_4d80_b5af_1a7be844ab5b a owl:Class ;
    rdfs:label "MinimumStoichiometricCoefficient"@en ;
    rdfs:comment "The minimum allowed value for stoichiometric coefficient for an entity in a chemical substance"@en ;
    rdfs:subClassOf :electrochemistry_f0667139_6428_4e3d_ac0d_08c1dd7f36ea ;
    skos:prefLabel "MinimumStoichiometricCoefficient"@en ;
    emmo:EMMO_967080e5_2f42_4eb2_a3a9_c58143e835f9 "The minimum allowed value for stoichiometric coefficient for an entity in a chemical substance"@en .

:electrochemistry_86af4487_33c1_4562_a00b_3a8252ffe378 a owl:Class ;
    rdfs:label "ActivationEnergyOfGuestDiffusivityInNegativeElectrodeActiveMaterial"@en ;
    rdfs:comment "the activation energy barrier in an Arrhenius expression for the diffusivity of lithium in the negative electrode"@en ;
    rdfs:subClassOf :electrochemistry_d7f8cab9_b035_4ecd_be63_292672572526 ;
    skos:prefLabel "ActivationEnergyOfGuestDiffusivityInNegativeElectrodeActiveMaterial"@en ;
    emmo:EMMO_967080e5_2f42_4eb2_a3a9_c58143e835f9 "the activation energy barrier in an Arrhenius expression for the diffusivity of lithium in the negative electrode"@en ;
    emmo:EMMO_c7b62dd7_063a_4c2a_8504_42f7264ba83f "this is a very specific term with a narrow conceptualization, used mostly as an anchor term for supporting interoperability; a more general term is suitable in most cases."@en ;
    :electrochemistry_0a5b99ee_995b_4899_a79b_925a4086da37 "['Parameterisation','Negative electrode','Diffusivity activation energy [J.mol-1]']"@en ;
    :electrochemistry_1b718841_5d72_4071_bb71_fc4a754f5e30 "['negative_electrode','active_materials',0,'diffusion_constant','arrhenius','activation_energy']"@en .

:electrochemistry_8768c8f4_eaa8_4670_a3a0_91524e59a7f6 a owl:Class ;
    rdfs:label "D60ParticleSize"@en ;
    rdfs:comment "a statistical measure used in particle size distribution analysis, indicating the particle diameter below which 60% of the sample's particles fall."@en ;
    rdfs:subClassOf emmo:EMMO_c1c8ac3c_8a1c_4777_8e0b_14c1f9f9b0c6 ;
    skos:prefLabel "D60ParticleSize"@en ;
    emmo:EMMO_967080e5_2f42_4eb2_a3a9_c58143e835f9 "a statistical measure used in particle size distribution analysis, indicating the particle diameter below which 60% of the sample's particles fall."@en .

:electrochemistry_884650fd_6cc6_4ec6_8264_c18fbe6b90ee a owl:Class ;
    rdfs:label "DischargingSpecificCapacity"@en ;
    rdfs:comment "quotient of the capacity of a cell or battery [ or electrode or active material ] obtained during a discharge process by its mass."@en ;
    rdfs:subClassOf :electrochemistry_1e3dc60d_dd6b_47d6_8161_70004fc5ee30 ;
    skos:altLabel "SpecificDischargeCapacity"@en ;
    skos:hiddenLabel "SpeCapD"@en,
        "SpeCapD/mAh/g"@en ;
    skos:prefLabel "DischargingSpecificCapacity"@en ;
    emmo:EMMO_967080e5_2f42_4eb2_a3a9_c58143e835f9 "quotient of the capacity of a cell or battery [ or electrode or active material ] obtained during a discharge process by its mass."@en .

:electrochemistry_88dd2bce_fb17_4705_905d_892681812290 a owl:Class ;
    rdfs:label "NumberOfIterations"@en ;
    rdfs:comment "the number of times an iterative process should occur"@en ;
    rdfs:subClassOf emmo:EMMO_ba882f34_0d71_4e4f_9d92_0c076c633a2c ;
    skos:prefLabel "NumberOfIterations"@en ;
    emmo:EMMO_967080e5_2f42_4eb2_a3a9_c58143e835f9 "the number of times an iterative process should occur"@en .

:electrochemistry_8b2aaa50_bbe1_45da_8778_8898326246a2 a owl:Class ;
    rdfs:label "StateOfCharge"@en ;
    rdfs:comment "the ratio of the charged capacity to the rated capacity of an electrochemical device"@en ;
    rdfs:subClassOf emmo:EMMO_faab3f84_e475_4a46_af9c_7d249f0b9aef,
        :electrochemistry_aecc6094_c6a5_4a36_a825_8a497a2ae112 ;
    skos:altLabel "SoC"@en ;
    skos:prefLabel "StateOfCharge"@en ;
    emmo:EMMO_967080e5_2f42_4eb2_a3a9_c58143e835f9 "the ratio of the charged capacity to the rated capacity of an electrochemical device"@en ;
    emmo:EMMO_c84c6752_6d64_48cc_9500_e54a3c34898d "https://en.wikipedia.org/wiki/State_of_charge" .

:electrochemistry_8c16cb12_41c1_43bd_9e7c_2eea7b06a1f0 a owl:Class ;
    rdfs:label "ActivationEnergyOfElectrolyteConductivity"@en ;
    rdfs:comment "the activation energy barrier in an Arrhenius expression for the ionic conductivity of an electrolyte"@en ;
    rdfs:subClassOf :electrochemistry_d7f8cab9_b035_4ecd_be63_292672572526 ;
    skos:prefLabel "ActivationEnergyOfElectrolyteConductivity"@en ;
    emmo:EMMO_967080e5_2f42_4eb2_a3a9_c58143e835f9 "the activation energy barrier in an Arrhenius expression for the ionic conductivity of an electrolyte"@en ;
    :electrochemistry_0a5b99ee_995b_4899_a79b_925a4086da37 "['Parameterisation','Electrolyte','Conductivity activation energy [J.mol-1]']"@en ;
    :electrochemistry_1b718841_5d72_4071_bb71_fc4a754f5e30 "['electrolyte','ionic_conductivity','arrhenius','activation_energy']"@en .

:electrochemistry_8c336ae9_1818_4b08_a660_4bb83b28351f a owl:Class ;
    rdfs:label "NegativeElectrodeActiveMaterialGuestStoichiometricCoefficientAtSOC100"@en ;
    rdfs:comment "this is a very specific term with a narrow conceptualization, used mostly as an anchor term for supporting interoperability; a more general term is suitable in most cases."@en ;
    rdfs:subClassOf :electrochemistry_38ab058e_3912_48c2_a7eb_76d25d000820 ;
    skos:prefLabel "NegativeElectrodeActiveMaterialGuestStoichiometricCoefficientAtSOC100"@en ;
    emmo:EMMO_967080e5_2f42_4eb2_a3a9_c58143e835f9 "this is a very specific term with a narrow conceptualization, used mostly as an anchor term for supporting interoperability; a more general term is suitable in most cases."@en ;
    :electrochemistry_0a5b99ee_995b_4899_a79b_925a4086da37 "['Parameterisation','Negative electrode','Maximum stoichiometry']"@en ;
    :electrochemistry_1b718841_5d72_4071_bb71_fc4a754f5e30 "['negative_electrode','active_materials',0,'stoichiometry1','value']"@en .

:electrochemistry_8e943e12_ecc0_4093_899e_7226be6be7f2 a owl:Class ;
    rdfs:label "D90ParticleSize"@en ;
    rdfs:comment "a statistical measure used in particle size distribution analysis, indicating the particle diameter below which 90% of the sample's particles fall."@en ;
    rdfs:subClassOf emmo:EMMO_c1c8ac3c_8a1c_4777_8e0b_14c1f9f9b0c6 ;
    skos:prefLabel "D90ParticleSize"@en ;
    emmo:EMMO_967080e5_2f42_4eb2_a3a9_c58143e835f9 "a statistical measure used in particle size distribution analysis, indicating the particle diameter below which 90% of the sample's particles fall."@en .

:electrochemistry_8f4b90ef_fea4_47c9_99f5_a9b3290a505d a owl:Class ;
    rdfs:label "ElectrochemicalStabilityLimit"@en ;
    rdfs:comment "electric potential at which a material undergoes an oxidation or reduction decomposition"@en ;
    rdfs:subClassOf emmo:EMMO_4f2d3939_91b1_4001_b8ab_7d19074bf845,
        :electrochemistry_2d896559_eee3_447c_9759_87c854a4266a ;
    skos:prefLabel "ElectrochemicalStabilityLimit"@en ;
    emmo:EMMO_967080e5_2f42_4eb2_a3a9_c58143e835f9 "electric potential at which a material undergoes an oxidation or reduction decomposition"@en .

:electrochemistry_92fc0dba_6f11_4019_a8cb_db2a5b1634f5 a owl:Class ;
    rdfs:label "D15ParticleSize"@en ;
    rdfs:comment "a statistical measure used in particle size distribution analysis, indicating the particle diameter below which 15% of the sample's particles fall."@en ;
    rdfs:subClassOf emmo:EMMO_c1c8ac3c_8a1c_4777_8e0b_14c1f9f9b0c6 ;
    skos:prefLabel "D15ParticleSize"@en ;
    emmo:EMMO_967080e5_2f42_4eb2_a3a9_c58143e835f9 "a statistical measure used in particle size distribution analysis, indicating the particle diameter below which 15% of the sample's particles fall."@en .

:electrochemistry_93f000d8_efc1_4364_896c_c9ebc4c7ce3a a owl:Class ;
    rdfs:label "ChargingPRate"@en ;
    rdfs:comment "an indicator of the electric power at which an electrochemical device is charged"@en ;
    rdfs:subClassOf :electrochemistry_c4120ce7_f1ff_4917_b59e_002454a65040 ;
    skos:prefLabel "ChargingPRate"@en ;
    emmo:EMMO_967080e5_2f42_4eb2_a3a9_c58143e835f9 "an indicator of the electric power at which an electrochemical device is charged"@en .

:electrochemistry_95ef8c3c_62fe_467f_b5d4_dd0cd18a7ea8 a owl:Class ;
    rdfs:label "MaximumStoichiometricCoefficient"@en ;
    rdfs:comment "The maximum allowed value for stoichiometric coefficient for an entity in a chemical substance"@en ;
    rdfs:subClassOf :electrochemistry_f0667139_6428_4e3d_ac0d_08c1dd7f36ea ;
    skos:prefLabel "MaximumStoichiometricCoefficient"@en ;
    emmo:EMMO_967080e5_2f42_4eb2_a3a9_c58143e835f9 "The maximum allowed value for stoichiometric coefficient for an entity in a chemical substance"@en .

:electrochemistry_97bc06e6_6141_47ec_9e81_fd9e6a5b07c7 a owl:Class ;
    rdfs:label "D80ParticleSize"@en ;
    rdfs:comment "a statistical measure used in particle size distribution analysis, indicating the particle diameter below which 10% of the sample's particles fall."@en ;
    rdfs:subClassOf emmo:EMMO_c1c8ac3c_8a1c_4777_8e0b_14c1f9f9b0c6 ;
    skos:prefLabel "D80ParticleSize"@en ;
    emmo:EMMO_967080e5_2f42_4eb2_a3a9_c58143e835f9 "a statistical measure used in particle size distribution analysis, indicating the particle diameter below which 10% of the sample's particles fall."@en .

:electrochemistry_99041897_5c08_40ed_9118_3e77e9b0e191 a owl:Class ;
    rdfs:label "PositiveElectrodeActiveMaterialGuestStoichiometricCoefficientAtSOC100"@en ;
    rdfs:comment "this is a very specific term with a narrow conceptualization, used mostly as an anchor term for supporting interoperability; a more general term is suitable in most cases."@en ;
    rdfs:subClassOf :electrochemistry_38ab058e_3912_48c2_a7eb_76d25d000820 ;
    skos:prefLabel "PositiveElectrodeActiveMaterialGuestStoichiometricCoefficientAtSOC100"@en ;
    emmo:EMMO_967080e5_2f42_4eb2_a3a9_c58143e835f9 "this is a very specific term with a narrow conceptualization, used mostly as an anchor term for supporting interoperability; a more general term is suitable in most cases."@en ;
    :electrochemistry_0a5b99ee_995b_4899_a79b_925a4086da37 "['Parameterisation','Positive electrode','Maximum stoichiometry']"@en ;
    :electrochemistry_1b718841_5d72_4071_bb71_fc4a754f5e30 "['positive_electrode','active_materials',0,'stoichiometry1','value']"@en .

:electrochemistry_9c9b80a4_a00b_4b91_8e17_3a7831f2bf2f a owl:Class ;
    rdfs:label "InititalThermodynamicTemperature"@en ;
    rdfs:comment "the thermodynamic temperature at some point in time designated to be the initial state"@en ;
    rdfs:subClassOf emmo:EMMO_affe07e4_e9bc_4852_86c6_69e26182a17f ;
    skos:prefLabel "InititalThermodynamicTemperature"@en ;
    emmo:EMMO_967080e5_2f42_4eb2_a3a9_c58143e835f9 "the thermodynamic temperature at some point in time designated to be the initial state"@en .

:electrochemistry_9cba2158_26ba_4dd7_b082_ba66dbb960c7 a owl:Class ;
    rdfs:label "DeviceLumpedSpecificHeatCapacity"@en ;
    rdfs:comment "the lumped specific heat capacity of an electrochemical device"@en ;
    rdfs:subClassOf emmo:EMMO_b4f4ed28_d24c_4a00_9583_62ab839abeca ;
    skos:prefLabel "DeviceLumpedSpecificHeatCapacity"@en ;
    emmo:EMMO_967080e5_2f42_4eb2_a3a9_c58143e835f9 "the lumped specific heat capacity of an electrochemical device"@en ;
    :electrochemistry_0a5b99ee_995b_4899_a79b_925a4086da37 "['Parameterisation','Cell','Specific heat capacity [J.K-1.kg-1]']"@en ;
    :electrochemistry_1b718841_5d72_4071_bb71_fc4a754f5e30 "['properties','specific_heat','value']"@en .

:electrochemistry_9cf8e627_a3d2_4f86_9bdc_e0e77996acde a owl:Class ;
    rdfs:label "D75ParticleSize"@en ;
    rdfs:comment "a statistical measure used in particle size distribution analysis, indicating the particle diameter below which 10% of the sample's particles fall."@en ;
    rdfs:subClassOf emmo:EMMO_c1c8ac3c_8a1c_4777_8e0b_14c1f9f9b0c6 ;
    skos:prefLabel "D75ParticleSize"@en ;
    emmo:EMMO_967080e5_2f42_4eb2_a3a9_c58143e835f9 "a statistical measure used in particle size distribution analysis, indicating the particle diameter below which 10% of the sample's particles fall."@en .

:electrochemistry_9d558b56_d3b8_429a_a4e2_d2ffab895e42 a owl:Class ;
    rdfs:label "PositiveElectrodeEntropicChangeCoefficient"@en ;
    rdfs:comment "this is a very specific term with a narrow conceptualization, used mostly as an anchor term for supporting interoperability; a more general term is suitable in most cases."@en ;
    rdfs:subClassOf :electrochemistry_3bb5ae23_59fa_4bc7_9495_803eb6719f28 ;
    skos:prefLabel "PositiveElectrodeEntropicChangeCoefficient"@en ;
    emmo:EMMO_967080e5_2f42_4eb2_a3a9_c58143e835f9 "this is a very specific term with a narrow conceptualization, used mostly as an anchor term for supporting interoperability; a more general term is suitable in most cases."@en ;
    :electrochemistry_0a5b99ee_995b_4899_a79b_925a4086da37 "['Parameterisation','Positive electrode','Entropic change coefficient [V.K-1]']"@en ;
    :electrochemistry_1b718841_5d72_4071_bb71_fc4a754f5e30 "['positive_electrode','active_materials',0,'entropy_coefficient','value']"@en .

:electrochemistry_9d57962c_e150_4e64_962b_8fd6a92c9234 a owl:Class ;
    rdfs:label "DischargingSpecificEnergy"@en ;
    rdfs:comment "the specific energy of an electrochemical device obtained during a discharge process"@en ;
    rdfs:subClassOf emmo:EMMO_e218c625_6a39_47a9_8d08_a2ef41c152a9 ;
    skos:altLabel "SpecificEnergyDischarge" ;
    skos:hiddenLabel "SpeEnergyD"@en,
        "SpeEnergyD/mWh/g"@en ;
    skos:prefLabel "DischargingSpecificEnergy"@en ;
    emmo:EMMO_967080e5_2f42_4eb2_a3a9_c58143e835f9 "the specific energy of an electrochemical device obtained during a discharge process"@en .

:electrochemistry_9d60c4ab_d9ac_4dda_af0c_c64059326916 a owl:Class ;
    rdfs:label "D45ParticleSize"@en ;
    rdfs:comment "a statistical measure used in particle size distribution analysis, indicating the particle diameter below which 45% of the sample's particles fall."@en ;
    rdfs:subClassOf emmo:EMMO_c1c8ac3c_8a1c_4777_8e0b_14c1f9f9b0c6 ;
    skos:prefLabel "D45ParticleSize"@en ;
    emmo:EMMO_967080e5_2f42_4eb2_a3a9_c58143e835f9 "a statistical measure used in particle size distribution analysis, indicating the particle diameter below which 45% of the sample's particles fall."@en .

:electrochemistry_9d6a52ed_a53d_4327_a391_f173677a4b1d a owl:Class ;
    rdfs:label "NumberOfCellsConnectedInSeries"@en ;
    rdfs:comment "the number of electrochemical cells connected in series"@en ;
    rdfs:subClassOf emmo:EMMO_41efdf5d_0c9c_4ea0_bb65_f8236e663be5,
        :electrochemistry_aecc6094_c6a5_4a36_a825_8a497a2ae112 ;
    skos:prefLabel "NumberOfCellsConnectedInSeries"@en ;
    emmo:EMMO_967080e5_2f42_4eb2_a3a9_c58143e835f9 "the number of electrochemical cells connected in series"@en .

:electrochemistry_a07dd85b_d0df_4d5d_8b0c_14d20ea3fe45 a owl:AnnotationProperty ;
    rdfs:label "arbinLabel"@en ;
    rdfs:comment "the label of a term used in resources from Arbin"@en ;
    rdfs:subPropertyOf skos:hiddenLabel ;
    skos:prefLabel "arbinLabel"@en ;
    emmo:EMMO_967080e5_2f42_4eb2_a3a9_c58143e835f9 "the label of a term used in resources from Arbin"@en .

:electrochemistry_a17ee4e0_c81a_4a64_9ecb_9c6fa022cf4d a owl:Class ;
    rdfs:label "LimitingMolarConductivity"@en ;
    rdfs:comment "molar conductivity at infinite dilution"@en ;
    rdfs:seeAlso "Kohlrausch's Law"@en,
        "Nernst-Einstein Equation"@en ;
    rdfs:subClassOf emmo:EMMO_9e955e04_2977_457e_a91a_bc6a541c9a9e,
        :electrochemistry_4a450a27_b84a_4c70_a3a9_15ec30e2f30b ;
    skos:prefLabel "LimitingMolarConductivity"@en ;
    emmo:EMMO_967080e5_2f42_4eb2_a3a9_c58143e835f9 "molar conductivity at infinite dilution"@en ;
    emmo:EMMO_c84c6752_6d64_48cc_9500_e54a3c34898d "https://en.wikipedia.org/wiki/Molar_conductivity#Variation_of_molar_conductivity_with_dilution"@en .

:electrochemistry_a4858e4d_dd3b_48ce_97ba_3eeb8571b633 a owl:Class ;
    rdfs:label "SeparatorPorosity"@en ;
    rdfs:comment "the porosity of a separator"@en ;
    rdfs:subClassOf emmo:EMMO_3a6578ac_aee0_43b9_9bc6_1eb208c8c9a9 ;
    skos:prefLabel "SeparatorPorosity"@en ;
    emmo:EMMO_967080e5_2f42_4eb2_a3a9_c58143e835f9 "the porosity of a separator"@en ;
    :electrochemistry_0a5b99ee_995b_4899_a79b_925a4086da37 "['Parameterisation','Separator','Porosity']"@en ;
    :electrochemistry_1b718841_5d72_4071_bb71_fc4a754f5e30 "['separator','porosity','value']"@en .

:electrochemistry_a5e00e3a_736c_4200_8d04_ed222fe07037 a owl:Class ;
    rdfs:label "NumberOfFiniteVolumeCellsInZ"@en ;
    rdfs:comment "number of discrete finite volume cells in a grid or sub-grid in the Z-direction"@en ;
    rdfs:subClassOf :electrochemistry_47608fd0_cc0d_457e_9141_051935029e3a ;
    skos:prefLabel "NumberOfFiniteVolumeCellsInZ"@en ;
    emmo:EMMO_967080e5_2f42_4eb2_a3a9_c58143e835f9 "number of discrete finite volume cells in a grid or sub-grid in the Z-direction"@en .

:electrochemistry_a7eb870c_4ef7_4ccd_85e8_4b7b726d7a2a a owl:Class ;
    rdfs:label "PowerDensity" ;
    rdfs:comment "the quotient of the power of an energy-storage device or system and its volume"@en ;
    rdfs:subClassOf :electrochemistry_02eb0465_4f94_453c_8c1f_5ddf80134634 ;
    skos:altLabel "VolumetricPowerDensity"@en ;
    skos:prefLabel "PowerDensity" ;
    emmo:EMMO_967080e5_2f42_4eb2_a3a9_c58143e835f9 "the quotient of the power of an energy-storage device or system and its volume"@en .

:electrochemistry_a9873707_8103_4bb4_9e51_83db1e89b1bd a owl:Class ;
    rdfs:label "MiniumumConcentration"@en ;
    rdfs:comment "the minimum amount concentration of a species in a phase, either imposed or naturally occuring"@en ;
    rdfs:subClassOf :electrochemistry_5eae657f_5914_4252_85c6_3fc772dea113 ;
    skos:prefLabel "MiniumumConcentration"@en ;
    emmo:EMMO_967080e5_2f42_4eb2_a3a9_c58143e835f9 "the minimum amount concentration of a species in a phase, either imposed or naturally occuring"@en .

:electrochemistry_abd08921_6f3b_4a48_811e_7685c58aec0b a owl:Class ;
    rdfs:label "AmbientCelsiusTemperature"@en ;
    rdfs:comment "the celsius temperature of the ambient environment"@en ;
    rdfs:subClassOf emmo:EMMO_66bc9029_f473_45ff_bab9_c3509ff37a22 ;
    skos:prefLabel "AmbientCelsiusTemperature"@en ;
    emmo:EMMO_967080e5_2f42_4eb2_a3a9_c58143e835f9 "the celsius temperature of the ambient environment"@en ;
    :electrochemistry_1b717a20_17e3_4480_8c60_c4ae94058f05 "Environmental_Temperature (C)"@en .

:electrochemistry_abf986d2_90d5_4746_b42b_89dc7cc1bf0f a owl:Class ;
    rdfs:label "RealElectricImpedance"@en ;
    rdfs:comment "the imaginary part of the complex electric impedance"@en ;
    rdfs:subClassOf emmo:EMMO_79a02de5_b884_4eab_bc18_f67997d597a2 ;
    skos:altLabel "ACResistance"@en ;
    skos:prefLabel "RealElectricImpedance"@en ;
    emmo:EMMO_26bf1bef_d192_4da6_b0eb_d2209698fb54 "https://www.wikidata.org/wiki/Q1048490"@en ;
    emmo:EMMO_967080e5_2f42_4eb2_a3a9_c58143e835f9 "the imaginary part of the complex electric impedance"@en .

:electrochemistry_ae108db7_8765_4329_9908_059277dee586 a owl:Class ;
    rdfs:label "StepCapacity"@en ;
    rdfs:comment "the amount of charge that has passed through an electrochemical device within the time interval of a given testing step"@en ;
    rdfs:subClassOf :electrochemistry_791c1915_a791_4450_acd8_7f94764743b5 ;
    skos:prefLabel "StepCapacity"@en ;
    emmo:EMMO_967080e5_2f42_4eb2_a3a9_c58143e835f9 "the amount of charge that has passed through an electrochemical device within the time interval of a given testing step"@en .

:electrochemistry_ae782b14_88ce_4cdd_9418_12aca00be937 a owl:Class ;
    rdfs:label "CycleLife"@en ;
    rdfs:comment "a typical end-of-life criterion in the battery domain is 80% of the initial capacity of the device"@en,
        "the maximum number of cycles achieved in an electrochemical device before reaching some end-of-life criterion"@en ;
    rdfs:subClassOf emmo:EMMO_ba882f34_0d71_4e4f_9d92_0c076c633a2c,
        :electrochemistry_02eb0465_4f94_453c_8c1f_5ddf80134634 ;
    skos:altLabel "ElectrochemicalCycleLife"@en ;
    skos:prefLabel "CycleLife"@en ;
    emmo:EMMO_967080e5_2f42_4eb2_a3a9_c58143e835f9 "the maximum number of cycles achieved in an electrochemical device before reaching some end-of-life criterion"@en .

:electrochemistry_b095e977_dbc2_4a9e_9930_6af0dab089f1 a owl:Class ;
    rdfs:label "D55ParticleSize"@en ;
    rdfs:comment "a statistical measure used in particle size distribution analysis, indicating the particle diameter below which 55% of the sample's particles fall."@en ;
    rdfs:subClassOf emmo:EMMO_c1c8ac3c_8a1c_4777_8e0b_14c1f9f9b0c6 ;
    skos:prefLabel "D55ParticleSize"@en ;
    emmo:EMMO_967080e5_2f42_4eb2_a3a9_c58143e835f9 "a statistical measure used in particle size distribution analysis, indicating the particle diameter below which 55% of the sample's particles fall."@en .

:electrochemistry_b4184e46_c53c_47cc_9bfc_186fd77836a5 a owl:Class ;
    rdfs:label "DeviceVolume"@en ;
    rdfs:comment "the total volume of an electrochemical device, determined by its external dimensions"@en ;
    rdfs:subClassOf emmo:EMMO_f1a51559_aa3d_43a0_9327_918039f0dfed ;
    skos:prefLabel "DeviceVolume"@en ;
    emmo:EMMO_967080e5_2f42_4eb2_a3a9_c58143e835f9 "the total volume of an electrochemical device, determined by its external dimensions"@en ;
    :electrochemistry_0a5b99ee_995b_4899_a79b_925a4086da37 "['Parameterisation','Cell','Volume [m3]']"@en ;
    :electrochemistry_1b718841_5d72_4071_bb71_fc4a754f5e30 "['properties','volume','value']"@en .

:electrochemistry_b66d6553_6136_4754_902a_707e414210c2 a owl:Class ;
    rdfs:label "LowerFrequencyLimit"@en ;
    rdfs:comment "the lower end of the interval of frequencies tested in impedimetry and related techniques"@en ;
    rdfs:subClassOf emmo:EMMO_852b4ab8_fc29_4749_a8c7_b92d4fca7d5a,
        :electrochemistry_c5047d29_4e68_43ee_8355_3e8f05dc70a5 ;
    skos:prefLabel "LowerFrequencyLimit"@en ;
    emmo:EMMO_967080e5_2f42_4eb2_a3a9_c58143e835f9 "the lower end of the interval of frequencies tested in impedimetry and related techniques"@en .

:electrochemistry_b6f33044_1892_41a4_ae89_8683d4225f8d a owl:Class ;
    rdfs:label "DischargingPRate"@en ;
    rdfs:comment "an indicator of the electric power at which an electrochemical device is discharged"@en ;
    rdfs:subClassOf :electrochemistry_c4120ce7_f1ff_4917_b59e_002454a65040 ;
    skos:prefLabel "DischargingPRate"@en ;
    emmo:EMMO_967080e5_2f42_4eb2_a3a9_c58143e835f9 "an indicator of the electric power at which an electrochemical device is discharged"@en .

:electrochemistry_b83c6435_6edf_470e_9725_538a853e08f7 a owl:Class ;
    rdfs:label "D10ParticleSize"@en ;
    rdfs:comment "a statistical measure used in particle size distribution analysis, indicating the particle diameter below which 10% of the sample's particles fall."@en ;
    rdfs:subClassOf emmo:EMMO_c1c8ac3c_8a1c_4777_8e0b_14c1f9f9b0c6 ;
    skos:prefLabel "D10ParticleSize"@en ;
    emmo:EMMO_967080e5_2f42_4eb2_a3a9_c58143e835f9 "a statistical measure used in particle size distribution analysis, indicating the particle diameter below which 10% of the sample's particles fall."@en .

:electrochemistry_b8d4042d_329a_450f_9088_2fc0e16a8667 a owl:Class ;
    rdfs:label "RetainedCapacity"@en ;
    rdfs:comment "the capacity that an electrochemical device can deliver after being stored under some specified conditions"@en ;
    rdfs:subClassOf :electrochemistry_9b3b4668_0795_4a35_9965_2af383497a26 ;
    skos:prefLabel "RetainedCapacity"@en ;
    emmo:EMMO_967080e5_2f42_4eb2_a3a9_c58143e835f9 "the capacity that an electrochemical device can deliver after being stored under some specified conditions"@en ;
    emmo:EMMO_cc65321f_1964_4f16_aea3_2a8edf2f3394 emmo:AmpereHour,
        emmo:MilliAmpereHour .

:electrochemistry_b90b1ad7_b9a8_44df_ad45_bfd25aac2e49 a owl:Class ;
    rdfs:label "MinimumChargingTemperature"@en ;
    rdfs:comment "the minimum allowable temperature of an electrochemical device during a charging process"@en ;
    rdfs:subClassOf :electrochemistry_4747c51d_86ab_4684_a4fb_b05f5c405ea3 ;
    skos:prefLabel "MinimumChargingTemperature"@en ;
    emmo:EMMO_967080e5_2f42_4eb2_a3a9_c58143e835f9 "the minimum allowable temperature of an electrochemical device during a charging process"@en .

:electrochemistry_ba7ac581_0e13_4815_b888_013c378932f5 a owl:Class ;
    rdfs:label "MaximumContinuousDischargingCurrent"@en ;
    rdfs:comment "the maximum current approved for continuous discharge for a given electrochemical device"@en ;
    rdfs:subClassOf :electrochemistry_74de2c33_84fc_4c2f_afe1_56d169149114 ;
    skos:altLabel "MaximumContinuousDischargeCurrent"@en ;
    skos:prefLabel "MaximumContinuousDischargingCurrent"@en ;
    emmo:EMMO_967080e5_2f42_4eb2_a3a9_c58143e835f9 "the maximum current approved for continuous discharge for a given electrochemical device"@en .

:electrochemistry_be3da3e2_58a9_4e58_adc2_7336d312717c a owl:Class ;
    rdfs:label "NegativeElectrodeElectronicConductivity"@en ;
    rdfs:comment "the electronic conductivity of the negative electrode"@en ;
    rdfs:subClassOf :electrochemistry_ce74d2dc_d496_4116_b2fb_3e83d88bc744 ;
    skos:prefLabel "NegativeElectrodeElectronicConductivity"@en ;
    emmo:EMMO_967080e5_2f42_4eb2_a3a9_c58143e835f9 "the electronic conductivity of the negative electrode"@en ;
    emmo:EMMO_c7b62dd7_063a_4c2a_8504_42f7264ba83f "this is a very specific term with a narrow conceptualization, used mostly as an anchor term for supporting interoperability; a more general term is suitable in most cases."@en ;
    :electrochemistry_0a5b99ee_995b_4899_a79b_925a4086da37 "['Parameterisation','Negative electrode','Conductivity [S.m-1]']"@en ;
    :electrochemistry_1b718841_5d72_4071_bb71_fc4a754f5e30 "['negative_electrode','electronic_conductivity','value']"@en .

:electrochemistry_bfe553c2_a63e_49b6_a209_0855dfc39724 a owl:Class ;
    rdfs:label "NegativeElectrodeActiveMaterialParticleRadius"@en ;
    rdfs:comment "this is a very specific term with a narrow conceptualization, used mostly as an anchor term for supporting interoperability; a more general term is suitable in most cases."@en ;
    rdfs:subClassOf :electrochemistry_b92e382f_5109_4f60_ab5e_c89d340419a9 ;
    skos:prefLabel "NegativeElectrodeActiveMaterialParticleRadius"@en ;
    emmo:EMMO_967080e5_2f42_4eb2_a3a9_c58143e835f9 "this is a very specific term with a narrow conceptualization, used mostly as an anchor term for supporting interoperability; a more general term is suitable in most cases."@en ;
    :electrochemistry_0a5b99ee_995b_4899_a79b_925a4086da37 "['Parameterisation','Negative electrode','Particle radius [m]']"@en ;
    :electrochemistry_1b718841_5d72_4071_bb71_fc4a754f5e30 "['negative_electrode','active_materials',0,'particle_radius','value']"@en .

:electrochemistry_c1c1288c_97c1_4f1f_8f42_6dfd34d028fd a owl:Class ;
    rdfs:label "D35ParticleSize"@en ;
    rdfs:comment "a statistical measure used in particle size distribution analysis, indicating the particle diameter below which 35% of the sample's particles fall."@en ;
    rdfs:subClassOf emmo:EMMO_c1c8ac3c_8a1c_4777_8e0b_14c1f9f9b0c6 ;
    skos:prefLabel "D35ParticleSize"@en ;
    emmo:EMMO_967080e5_2f42_4eb2_a3a9_c58143e835f9 "a statistical measure used in particle size distribution analysis, indicating the particle diameter below which 35% of the sample's particles fall."@en .

:electrochemistry_c2a85d02_c6b4_42df_b5ed_a9904ec34a5c a owl:Class ;
    rdfs:label "NumberOfFiniteVolumeCellsInY"@en ;
    rdfs:comment "number of discrete finite volume cells in a grid or sub-grid in the Y-direction"@en ;
    rdfs:subClassOf :electrochemistry_47608fd0_cc0d_457e_9141_051935029e3a ;
    skos:prefLabel "NumberOfFiniteVolumeCellsInY"@en ;
    emmo:EMMO_967080e5_2f42_4eb2_a3a9_c58143e835f9 "number of discrete finite volume cells in a grid or sub-grid in the Y-direction"@en .

:electrochemistry_c5dcb1a2_f2cf_421a_b8ae_47a88a61fce3 a owl:Class ;
    rdfs:label "NegativeElectrodeReactionRateConstant"@en ;
    rdfs:comment "this is a very specific term with a narrow conceptualization, used mostly as an anchor term for supporting interoperability; a more general term is suitable in most cases."@en ;
    rdfs:subClassOf :electrochemistry_0335e3f6_d1d8_4daa_8376_a9285f1bc9f1 ;
    skos:prefLabel "NegativeElectrodeReactionRateConstant"@en ;
    emmo:EMMO_967080e5_2f42_4eb2_a3a9_c58143e835f9 "this is a very specific term with a narrow conceptualization, used mostly as an anchor term for supporting interoperability; a more general term is suitable in most cases."@en ;
    :electrochemistry_0a5b99ee_995b_4899_a79b_925a4086da37 "['Parameterisation','Negative electrode','Reaction rate constant [mol.m-2.s-1]']"@en ;
    :electrochemistry_1b718841_5d72_4071_bb71_fc4a754f5e30 "['negative_electrode','active_materials',0,'kinetic_constant','value']"@en .

:electrochemistry_c5f9b91e_a770_4e9b_837e_fa2a76019111 a owl:Class ;
    rdfs:label "NegativeElectrodeActiveMaterialVolumetricSurfaceArea"@en ;
    rdfs:comment "this is a very specific term with a narrow conceptualization, used mostly as an anchor term for supporting interoperability; a more general term is suitable in most cases."@en ;
    rdfs:subClassOf :electrochemistry_a5571263_f153_448f_84a3_cd18092cf8fa ;
    skos:prefLabel "NegativeElectrodeActiveMaterialVolumetricSurfaceArea"@en ;
    emmo:EMMO_967080e5_2f42_4eb2_a3a9_c58143e835f9 "this is a very specific term with a narrow conceptualization, used mostly as an anchor term for supporting interoperability; a more general term is suitable in most cases."@en ;
    :electrochemistry_0a5b99ee_995b_4899_a79b_925a4086da37 "['Parameterisation','Negative electrode','Surface area per unit volume [m-1]']"@en .

:electrochemistry_c69a9d55_823f_4113_a305_ebc89dde7de3 a owl:Class ;
    rdfs:label "PositiveElectrodeActiveMaterialMaximumGuestConcentration"@en ;
    rdfs:comment "maximum concentration of lithium in the positive electrode"@en ;
    rdfs:subClassOf :electrochemistry_47287d09_6108_45ca_ac65_8b9451b1065e ;
    skos:prefLabel "PositiveElectrodeActiveMaterialMaximumGuestConcentration"@en ;
    emmo:EMMO_967080e5_2f42_4eb2_a3a9_c58143e835f9 "maximum concentration of lithium in the positive electrode"@en ;
    emmo:EMMO_c7b62dd7_063a_4c2a_8504_42f7264ba83f "this is a very specific term with a narrow conceptualization, used mostly as an anchor term for supporting interoperability; a more general term is suitable in most cases."@en ;
    :electrochemistry_0a5b99ee_995b_4899_a79b_925a4086da37 "['Parameterisation','Positive electrode','Maximum concentration [mol.m-3]']"@en ;
    :electrochemistry_1b718841_5d72_4071_bb71_fc4a754f5e30 "['positive_electrode','active_materials',0,'maximum_concentration','value']"@en .

:electrochemistry_c762a928_5a74_46fd_9929_4ac2d7a3a8d7 a owl:Class ;
    rdfs:label "SpecificPower"@en ;
    rdfs:comment "the quotient of the power of an energy-storage device or system and its mass"@en ;
    rdfs:subClassOf :electrochemistry_02eb0465_4f94_453c_8c1f_5ddf80134634 ;
    skos:prefLabel "SpecificPower"@en ;
    emmo:EMMO_967080e5_2f42_4eb2_a3a9_c58143e835f9 "the quotient of the power of an energy-storage device or system and its mass"@en .

:electrochemistry_c8abaf09_300a_4008_a42a_2f4a3953ca7a a owl:Class ;
    rdfs:label "D40ParticleSize"@en ;
    rdfs:comment "a statistical measure used in particle size distribution analysis, indicating the particle diameter below which 40% of the sample's particles fall."@en ;
    rdfs:subClassOf emmo:EMMO_c1c8ac3c_8a1c_4777_8e0b_14c1f9f9b0c6 ;
    skos:prefLabel "D40ParticleSize"@en ;
    emmo:EMMO_967080e5_2f42_4eb2_a3a9_c58143e835f9 "a statistical measure used in particle size distribution analysis, indicating the particle diameter below which 40% of the sample's particles fall."@en .

:electrochemistry_ca36cbf3_1fed_4b88_9177_b4e16ad00cf7 a owl:Class ;
    rdfs:label "DischargingEnergy"@en ;
    rdfs:comment "energy delivered by a deviced under some specific discharge conditions"@en ;
    rdfs:subClassOf :electrochemistry_46376e5d_9627_4514_9881_9e62083625c3 ;
    skos:altLabel "DischargeEnergy" ;
    skos:hiddenLabel "Energy discharge/W.h"@en,
        "EnergyD"@en,
        "EnergyD/mWh"@en,
        "WH-OUT"@en ;
    skos:prefLabel "DischargingEnergy"@en ;
    emmo:EMMO_967080e5_2f42_4eb2_a3a9_c58143e835f9 "energy delivered by a deviced under some specific discharge conditions"@en ;
    :electrochemistry_097ea615_c209_4edd_a1a1_5eea71d98fe8 "wf dis e"@en ;
    :electrochemistry_1b717a20_17e3_4480_8c60_c4ae94058f05 "Discharge_Energy (Wh)"@en ;
    :electrochemistry_69022178_77b8_4669_97e2_351d45356e5a "Energy discharge/W.h"@en ;
    :electrochemistry_811aafc3_0c6d_470e_b67e_ff5c82992609 "Engy_DChg(mWh)"@en ;
    :electrochemistry_a07dd85b_d0df_4d5d_8b0c_14d20ea3fe45 "discharge_energy"@en .

:electrochemistry_ccde24bb_790a_40ca_a06e_cea156a61031 a owl:Class ;
    rdfs:label "ExchangeCurrent"@en ;
    rdfs:comment "For an electrode at equilibrium at which only one reaction is significant i = 0. When more than one reaction is significant at a given electrode, subscripts to i0 may be used to distinguish exchange currents. i is not usually zero when only one of these reactions is at equilibrium."@en,
        "i0 = ia = - ic"@en,
        "the common value (i0) of the anodic and cathodic partial currents when the reaction is at equilibrium"@en ;
    rdfs:subClassOf emmo:EMMO_c995ae70_3b84_4ebb_bcfc_69e6a281bb88,
        :electrochemistry_21745019_2830_4395_bca7_15ddfd266673 ;
    skos:prefLabel "ExchangeCurrent"@en ;
    emmo:EMMO_967080e5_2f42_4eb2_a3a9_c58143e835f9 "the common value (i0) of the anodic and cathodic partial currents when the reaction is at equilibrium"@en ;
    emmo:EMMO_fe015383_afb3_44a6_ae86_043628697aa2 "https://goldbook.iupac.org/terms/view/E02238" .

:electrochemistry_ccde4e5f_ace4_41d1_b4d8_cbd63e6376e6 a owl:Class ;
    rdfs:label "DeviceSurfaceArea"@en ;
    rdfs:comment "the external surface area of an electrochemical device"@en ;
    rdfs:subClassOf :electrochemistry_05cf26ef_782a_4f66_a196_7004dd973f8e ;
    skos:prefLabel "DeviceSurfaceArea"@en ;
    emmo:EMMO_967080e5_2f42_4eb2_a3a9_c58143e835f9 "the external surface area of an electrochemical device"@en ;
    :electrochemistry_0a5b99ee_995b_4899_a79b_925a4086da37 "['Parameterisation','Parameterisation','Cell','External surface area [m2]']"@en ;
    :electrochemistry_1b718841_5d72_4071_bb71_fc4a754f5e30 "['properties','external_surface_area','value']"@en .

:electrochemistry_cdc91ec0_9fc5_4551_bbd9_6824c2920124 a owl:Class ;
    rdfs:label "NegativeElectrodeCoatingThickness"@en ;
    rdfs:comment "thickness of the negative electrode coating"@en ;
    rdfs:subClassOf :electrochemistry_3b938708_e7e4_4ac0_a959_9c04306302e7 ;
    skos:prefLabel "NegativeElectrodeCoatingThickness"@en ;
    emmo:EMMO_967080e5_2f42_4eb2_a3a9_c58143e835f9 "thickness of the negative electrode coating"@en ;
    emmo:EMMO_c7b62dd7_063a_4c2a_8504_42f7264ba83f "this is a very specific term with a narrow conceptualization, used mostly as an anchor term for supporting interoperability; a more general term is suitable in most cases."@en ;
    :electrochemistry_0a5b99ee_995b_4899_a79b_925a4086da37 "['Parameterisation','Negative electrode','Thickness [m]']"@en ;
    :electrochemistry_1b718841_5d72_4071_bb71_fc4a754f5e30 "['negative_electrode','thickness','value']"@en .

:electrochemistry_cf54e7c1_f359_4715_b61d_0350b890d597 a owl:Class ;
    rdfs:label "SpecificSurfaceArea"@en ;
    rdfs:comment "total surface of a solid per mass"@en ;
    rdfs:subClassOf [ a owl:Restriction ;
            owl:onProperty emmo:EMMO_bed1d005_b04e_4a90_94cf_02bc678a8569 ;
            owl:someValuesFrom emmo:EMMO_4817e479_e401_437e_a49b_54540b93d2a1 ],
        :electrochemistry_aecc6094_c6a5_4a36_a825_8a497a2ae112 ;
    skos:prefLabel "SpecificSurfaceArea"@en ;
    emmo:EMMO_26bf1bef_d192_4da6_b0eb_d2209698fb54 "https://www.wikidata.org/wiki/Q622205" ;
    emmo:EMMO_50c298c2_55a2_4068_b3ac_4e948c33181f "https://www.electropedia.org/iev/iev.nsf/display?openform&ievref=485-02-10" ;
    emmo:EMMO_967080e5_2f42_4eb2_a3a9_c58143e835f9 "total surface of a solid per mass"@en ;
    emmo:EMMO_c84c6752_6d64_48cc_9500_e54a3c34898d "https://en.wikipedia.org/wiki/Specific_surface_area"@en .

:electrochemistry_d5dc0c1d_0926_4268_89f0_4519a326eabc a owl:Class ;
    rdfs:label "MaximumDischargingPulseDuration"@en ;
    rdfs:comment "the maximum duration of a pulse discharge for a given electrochemical device"@en ;
    rdfs:subClassOf :electrochemistry_3cd0e74e_292c_48ed_a831_4cb8753d9a56 ;
    skos:prefLabel "MaximumDischargingPulseDuration"@en ;
    emmo:EMMO_967080e5_2f42_4eb2_a3a9_c58143e835f9 "the maximum duration of a pulse discharge for a given electrochemical device"@en .

:electrochemistry_d78b696d_9832_4352_a264_28a2ea7d82e4 a owl:Class ;
    rdfs:label "StepIndex"@en ;
    rdfs:comment "the currently running step number in the procedure"@en ;
    rdfs:subClassOf emmo:EMMO_ba882f34_0d71_4e4f_9d92_0c076c633a2c,
        :electrochemistry_aecc6094_c6a5_4a36_a825_8a497a2ae112 ;
    skos:altLabel "StepNumber"@en ;
    skos:hiddenLabel "Step"@en ;
    skos:prefLabel "StepIndex"@en ;
    emmo:EMMO_967080e5_2f42_4eb2_a3a9_c58143e835f9 "the currently running step number in the procedure"@en ;
    :electrochemistry_097ea615_c209_4edd_a1a1_5eea71d98fe8 "step"@en ;
    :electrochemistry_811aafc3_0c6d_470e_b67e_ff5c82992609 "Step ID"@en ;
    :electrochemistry_a07dd85b_d0df_4d5d_8b0c_14d20ea3fe45 "step_index"@en ;
    :electrochemistry_ea9f4dba_8ca2_419e_9cdf_ce54e9ebbd46 "Step Number"@en .

:electrochemistry_db37b358_b2f0_4e06_b6ae_8c56c8fbb6ba a owl:Class ;
    rdfs:label "VolumePercent"@en ;
    rdfs:comment "the ratio of a constituent volume to the total volume"@en ;
    rdfs:subClassOf :electrochemistry_cf386c1e_e62b_43ef_9b0e_e5e58935d63f ;
    skos:prefLabel "VolumePercent"@en ;
    emmo:EMMO_967080e5_2f42_4eb2_a3a9_c58143e835f9 "the ratio of a constituent volume to the total volume"@en .

:electrochemistry_db40df7e_1aa5_49a7_85cb_2aa2c1c70489 a owl:Class ;
    rdfs:label "ReferenceThermodynamicTemperature"@en ;
    rdfs:comment "the thermodynamic temperature that is the reference for a calculation"@en ;
    rdfs:subClassOf emmo:EMMO_affe07e4_e9bc_4852_86c6_69e26182a17f ;
    skos:prefLabel "ReferenceThermodynamicTemperature"@en ;
    emmo:EMMO_967080e5_2f42_4eb2_a3a9_c58143e835f9 "the thermodynamic temperature that is the reference for a calculation"@en .

:electrochemistry_de612af2_a029_4a02_8090_4a75ab13271d a owl:Class ;
    rdfs:label "MaximumDischargingTemperature"@en ;
    rdfs:comment "the maximum allowable temperature of an electrochemical device during a discharging process"@en ;
    rdfs:subClassOf :electrochemistry_cc519a19_b8d5_4e3f_b893_3a884888ad79 ;
    skos:prefLabel "MaximumDischargingTemperature"@en ;
    emmo:EMMO_967080e5_2f42_4eb2_a3a9_c58143e835f9 "the maximum allowable temperature of an electrochemical device during a discharging process"@en .

:electrochemistry_df9e9d49_12fa_4794_b482_e0dcd2a7bb66 a owl:Class ;
    rdfs:label "TotalCapacity"@en ;
    rdfs:comment "the total amount of electric charge that has passed through an electrochemical device within a defined time interval"@en ;
    rdfs:subClassOf :electrochemistry_791c1915_a791_4450_acd8_7f94764743b5 ;
    skos:prefLabel "TotalCapacity"@en ;
    emmo:EMMO_967080e5_2f42_4eb2_a3a9_c58143e835f9 "the total amount of electric charge that has passed through an electrochemical device within a defined time interval"@en .

:electrochemistry_e03f6800_92c5_4218_bb6d_1c919abaa063 a owl:Class ;
    rdfs:label "D70ParticleSize"@en ;
    rdfs:comment "a statistical measure used in particle size distribution analysis, indicating the particle diameter below which 10% of the sample's particles fall."@en ;
    rdfs:subClassOf emmo:EMMO_c1c8ac3c_8a1c_4777_8e0b_14c1f9f9b0c6 ;
    skos:prefLabel "D70ParticleSize"@en ;
    emmo:EMMO_967080e5_2f42_4eb2_a3a9_c58143e835f9 "a statistical measure used in particle size distribution analysis, indicating the particle diameter below which 10% of the sample's particles fall."@en .

:electrochemistry_e2514bf9_d012_4990_b68b_6f37443f18f6 a owl:Class ;
    rdfs:label "ReactionRate"@en ;
    rdfs:comment "rate at which a chemical reaction takes place"@en ;
    rdfs:subClassOf :electrochemistry_21745019_2830_4395_bca7_15ddfd266673 ;
    skos:prefLabel "ReactionRate"@en ;
    emmo:EMMO_26bf1bef_d192_4da6_b0eb_d2209698fb54 "https://www.wikidata.org/wiki/Q3394849" ;
    emmo:EMMO_50c298c2_55a2_4068_b3ac_4e948c33181f "https://www.electropedia.org/iev/iev.nsf/display?openform&ievref=114-02-02" ;
    emmo:EMMO_967080e5_2f42_4eb2_a3a9_c58143e835f9 "rate at which a chemical reaction takes place"@en ;
    emmo:EMMO_c84c6752_6d64_48cc_9500_e54a3c34898d "https://en.wikipedia.org/wiki/Reaction_rate"@en .

:electrochemistry_e3e78df2_d568_4ab7_8c0d_d3a2ee3ae282 a owl:Class ;
    rdfs:label "ChargeCarrierTransportNumber"@en ;
    rdfs:comment "transport number of lithium ion in electrolyte"@en ;
    rdfs:subClassOf emmo:EMMO_d97b27cb_61a4_4568_a38b_4edd4f224acc ;
    skos:prefLabel "ChargeCarrierTransportNumber"@en ;
    emmo:EMMO_967080e5_2f42_4eb2_a3a9_c58143e835f9 "transport number of lithium ion in electrolyte"@en ;
    emmo:EMMO_c7b62dd7_063a_4c2a_8504_42f7264ba83f "this is a very specific term with a narrow conceptualization, used mostly as an anchor term for supporting interoperability; a more general term is suitable in most cases."@en ;
    :electrochemistry_0a5b99ee_995b_4899_a79b_925a4086da37 "['Parameterisation','Electrolyte','Cation transference number']"@en ;
    :electrochemistry_1b718841_5d72_4071_bb71_fc4a754f5e30 "['electrolyte','transference_number','value']"@en .

:electrochemistry_e59188bb_ce66_49f6_84aa_ecb98e76941e a owl:Class ;
    rdfs:label "GuestDiffusivityInPositiveElectrodeActiveMaterial"@en ;
    rdfs:comment "the diffusivity of lithium in the positive electrode"@en ;
    rdfs:subClassOf :electrochemistry_37b24a94_cae0_4d7a_9519_9f7692dec607 ;
    skos:prefLabel "GuestDiffusivityInPositiveElectrodeActiveMaterial"@en ;
    emmo:EMMO_967080e5_2f42_4eb2_a3a9_c58143e835f9 "the diffusivity of lithium in the positive electrode"@en ;
    emmo:EMMO_c7b62dd7_063a_4c2a_8504_42f7264ba83f "this is a very specific term with a narrow conceptualization, used mostly as an anchor term for supporting interoperability; a more general term is suitable in most cases."@en ;
    :electrochemistry_0a5b99ee_995b_4899_a79b_925a4086da37 "['Parameterisation','Positive electrode','Diffusivity [m2.s-1]']"@en ;
    :electrochemistry_1b718841_5d72_4071_bb71_fc4a754f5e30 "['positive_electrode','active_materials',0,'diffusion_constant','value']"@en .

:electrochemistry_e5e86474_8623_48ea_a1cf_502bdb10aa14 a owl:AnnotationProperty ;
    rdfs:label "battmoKey"@en ;
    rdfs:subPropertyOf rdfs:label ;
    skos:prefLabel "battmoKey"@en .

:electrochemistry_e73586eb_8475_4879_a43e_087c702ea6bf a owl:Class ;
    rdfs:label "NumberOfFiniteVolumeCellsInX"@en ;
    rdfs:comment "number of discrete finite volume cells in a grid or sub-grid in the X-direction"@en ;
    rdfs:subClassOf :electrochemistry_47608fd0_cc0d_457e_9141_051935029e3a ;
    skos:prefLabel "NumberOfFiniteVolumeCellsInX"@en ;
    emmo:EMMO_967080e5_2f42_4eb2_a3a9_c58143e835f9 "number of discrete finite volume cells in a grid or sub-grid in the X-direction"@en .

:electrochemistry_e808a26a_5812_49e9_894c_b793c7fe0c38 a owl:Class ;
    rdfs:label "NegativeElectrodeActiveMaterialMaximumGuestConcentration"@en ;
    rdfs:comment "maximum concentration of lithium in the negative electrode"@en ;
    rdfs:subClassOf :electrochemistry_47287d09_6108_45ca_ac65_8b9451b1065e ;
    skos:prefLabel "NegativeElectrodeActiveMaterialMaximumGuestConcentration"@en ;
    emmo:EMMO_967080e5_2f42_4eb2_a3a9_c58143e835f9 "maximum concentration of lithium in the negative electrode"@en ;
    emmo:EMMO_c7b62dd7_063a_4c2a_8504_42f7264ba83f "this is a very specific term with a narrow conceptualization, used mostly as an anchor term for supporting interoperability; a more general term is suitable in most cases."@en ;
    :electrochemistry_0a5b99ee_995b_4899_a79b_925a4086da37 "['Parameterisation','Negative electrode','Maximum concentration [mol.m-3]']"@en ;
    :electrochemistry_1b718841_5d72_4071_bb71_fc4a754f5e30 "['negative_electrode','active_materials',0,'maximum_concentration','value']"@en .

:electrochemistry_e9fd9ef9_adfe_46cb_b2f9_4558468a25e7 a owl:Class ;
    rdfs:label "ExchangeCurrentDensity"@en ;
    rdfs:comment "defined by j0 = i0/A, where i0 is the exchange current of the electrode reaction and A is usually taken as the geometric area of the electrode"@en ;
    rdfs:subClassOf emmo:EMMO_7c8007b0_58a7_4486_bf1c_4772852caca0,
        :electrochemistry_21745019_2830_4395_bca7_15ddfd266673 ;
    skos:altLabel "MeanExchangeCurrentDensity"@en ;
    skos:prefLabel "ExchangeCurrentDensity"@en ;
    emmo:EMMO_967080e5_2f42_4eb2_a3a9_c58143e835f9 "defined by j0 = i0/A, where i0 is the exchange current of the electrode reaction and A is usually taken as the geometric area of the electrode"@en ;
    emmo:EMMO_c84c6752_6d64_48cc_9500_e54a3c34898d "https://en.wikipedia.org/wiki/Exchange_current_density" ;
    emmo:EMMO_fe015383_afb3_44a6_ae86_043628697aa2 "https://goldbook.iupac.org/terms/view/M03777" .

:electrochemistry_ea9f4dba_8ca2_419e_9cdf_ce54e9ebbd46 a owl:AnnotationProperty ;
    rdfs:label "novonixLabel"@en ;
    rdfs:comment "the label of a term used in resources from Novonix"@en ;
    rdfs:subPropertyOf skos:hiddenLabel ;
    skos:prefLabel "novonixLabel"@en ;
    emmo:EMMO_967080e5_2f42_4eb2_a3a9_c58143e835f9 "the label of a term used in resources from Novonix"@en .

:electrochemistry_eac57b09_5cc9_41d7_b2c8_40218d7fd47c a owl:Class ;
    rdfs:label "NegativeElectrodeEntropicChangeCoefficient"@en ;
    rdfs:comment "this is a very specific term with a narrow conceptualization, used mostly as an anchor term for supporting interoperability; a more general term is suitable in most cases."@en ;
    rdfs:subClassOf :electrochemistry_3bb5ae23_59fa_4bc7_9495_803eb6719f28 ;
    skos:prefLabel "NegativeElectrodeEntropicChangeCoefficient"@en ;
    emmo:EMMO_967080e5_2f42_4eb2_a3a9_c58143e835f9 "this is a very specific term with a narrow conceptualization, used mostly as an anchor term for supporting interoperability; a more general term is suitable in most cases."@en ;
    :electrochemistry_0a5b99ee_995b_4899_a79b_925a4086da37 "['Parameterisation','Negative electrode','Entropic change coefficient [V.K-1]']"@en ;
    :electrochemistry_1b718841_5d72_4071_bb71_fc4a754f5e30 "['negative_electrode','active_materials',0,'entropy_coefficient','value']"@en .

:electrochemistry_f046d602_22ea_4f9b_9101_319f510d39f0 a owl:Class ;
    rdfs:label "CurrentScanRate"@en ;
    rdfs:comment "The rate of change of an applied current with time."@en ;
    rdfs:subClassOf :electrochemistry_637ee9c4_4b3f_4d3a_975b_c0572dfe53ce,
        :electrochemistry_c5047d29_4e68_43ee_8355_3e8f05dc70a5 ;
    skos:prefLabel "CurrentScanRate"@en ;
    emmo:EMMO_967080e5_2f42_4eb2_a3a9_c58143e835f9 "The rate of change of an applied current with time."@en ;
    emmo:EMMO_c7b62dd7_063a_4c2a_8504_42f7264ba83f "Used in linear potentiometry and related techniques, where a linearly-changing current is imposed to a cell to measure its voltage response."@en .

:electrochemistry_f2f36f22_3738_49dd_b43b_7469db6675df a owl:Class ;
    rdfs:label "BoundaryCondition"@en ;
    rdfs:comment "a property whose value is controlled on some surface or domain"@en ;
    rdfs:subClassOf :electrochemistry_33e6986c_b35a_4cae_9a94_acb23248065c ;
    skos:prefLabel "BoundaryCondition"@en ;
    emmo:EMMO_967080e5_2f42_4eb2_a3a9_c58143e835f9 "a property whose value is controlled on some surface or domain"@en .

:electrochemistry_f3172070_a72c_40db_8cc7_85c76ae97be5 a owl:Class ;
    rdfs:label "C"@en ;
    rdfs:comment "the unit for C-Rate in electrochemistry and related domains"@en ;
    rdfs:subClassOf :electrochemistry_67930f7b_ad4c_4b21_9b2e_a000e5c153ae ;
    skos:prefLabel "C"@en ;
    emmo:EMMO_967080e5_2f42_4eb2_a3a9_c58143e835f9 "the unit for C-Rate in electrochemistry and related domains"@en .

:electrochemistry_f9e1c862_c510_4b11_9141_bc91045df817 a owl:Class ;
    rdfs:label "CalenderedCoatingThickness"@en ;
    rdfs:comment "thickness of the coating after a calendering process"@en ;
    rdfs:subClassOf :electrochemistry_3b938708_e7e4_4ac0_a959_9c04306302e7 ;
    skos:prefLabel "CalenderedCoatingThickness"@en ;
    emmo:EMMO_967080e5_2f42_4eb2_a3a9_c58143e835f9 "thickness of the coating after a calendering process"@en .

:electrochemistry_fbaa2d5e_b8f7_4a2f_9497_41c3698eb0ff a owl:Class ;
    rdfs:label "D85ParticleSize"@en ;
    rdfs:comment "a statistical measure used in particle size distribution analysis, indicating the particle diameter below which 10% of the sample's particles fall."@en ;
    rdfs:subClassOf emmo:EMMO_c1c8ac3c_8a1c_4777_8e0b_14c1f9f9b0c6 ;
    skos:prefLabel "D85ParticleSize"@en ;
    emmo:EMMO_967080e5_2f42_4eb2_a3a9_c58143e835f9 "a statistical measure used in particle size distribution analysis, indicating the particle diameter below which 10% of the sample's particles fall."@en .

:electrochemistry_fda9539d_5232_471c_8945_b9a8ec7247fe a owl:Class ;
    rdfs:label "NegativeElectrodeActivationEnergyOfReaction"@en ;
    rdfs:comment "this is a very specific term with a narrow conceptualization, used mostly as an anchor term for supporting interoperability; a more general term is suitable in most cases."@en ;
    rdfs:subClassOf :electrochemistry_d7f8cab9_b035_4ecd_be63_292672572526 ;
    skos:prefLabel "NegativeElectrodeActivationEnergyOfReaction"@en ;
    emmo:EMMO_967080e5_2f42_4eb2_a3a9_c58143e835f9 "this is a very specific term with a narrow conceptualization, used mostly as an anchor term for supporting interoperability; a more general term is suitable in most cases."@en ;
    :electrochemistry_0a5b99ee_995b_4899_a79b_925a4086da37 "['Parameterisation','Negative electrode','Reaction rate constant activation energy [J.mol-1]']"@en .

<https://w3id.org/emmo/domain/electrochemistry/reference/electrochemistry-quantities> a owl:Ontology ;
    dcterms:abstract "This electrochemical quantities ontology is a domain of the Elementary Multiperspective Materials Ontology (EMMO). It is a specialized framework designed to represent and organize knowledge about electrochemical quantities. It is designed to integrate with the electrochemistry domain ontology or other ontologies from the EMMO ecosystem. The main focus of this ontology is to provide machine-readable descriptions of common electrochemical quantities, linking both to the larger descriptions of physical quantities in EMMO as well as other sources of information like the IEC, QUDT, Wikidata, etc. It should be used to support linked data generation in the electrochemistry domain."@en ;
    dcterms:contributor <https://orcid.org/0000-0001-8869-3718>,
        <https://orcid.org/0000-0002-1560-809X>,
        <https://orcid.org/0000-0002-2547-155X> ;
    dcterms:creator <https://orcid.org/0000-0002-8758-6109>,
        <https://orcid.org/0000-0003-2954-1233> ;
    dcterms:license "https://creativecommons.org/licenses/by/4.0/legalcode" ;
    owl:imports <https://w3id.org/emmo/1.0.0/disciplines/isq> ;
    owl:versionIRI <https://w3id.org/emmo/domain/electrochemistry/0.28.4-beta/reference/electrochemistry-quantities> ;
    owl:versionInfo "0.28.4-beta" .

<https://orcid.org/0000-0001-8869-3718> a owl:NamedIndividual,
        foaf:Person ;
    rdfs:label "Francesca Lonstad Bleken" ;
    rdfs:comment "" ;
    skos:prefLabel "Francesca Lonstad Bleken" ;
    foaf:name "Francesca Lonstad Bleken" .

<https://orcid.org/0000-0002-1560-809X> a owl:NamedIndividual,
        foaf:Person ;
    rdfs:label "Jesper Friis" ;
    rdfs:comment "" ;
    skos:prefLabel "Jesper Friis" ;
    foaf:name "Jesper Friis" .

<https://orcid.org/0000-0002-2547-155X> a owl:NamedIndividual,
        foaf:Person ;
    rdfs:label "Casper Welzel Andersen" ;
    rdfs:comment "" ;
    skos:prefLabel "Casper Welzel Andersen" ;
    foaf:name "Casper Welzel Andersen" .

<https://orcid.org/0000-0002-8758-6109> a owl:NamedIndividual,
        foaf:Person ;
    rdfs:label "Simon Clark" ;
    rdfs:comment "" ;
    skos:prefLabel "Simon Clark" ;
    foaf:name "Simon Clark" .

<https://orcid.org/0000-0003-2954-1233> a owl:NamedIndividual,
        foaf:Person ;
    rdfs:label "Eibar Flores" ;
    rdfs:comment "" ;
    skos:prefLabel "Eibar Flores" ;
    foaf:name "Eibar Flores" .

emmo:EMMO_b432d2d5_25f4_4165_99c5_5935a7763c1a a owl:AnnotationProperty .

:electrochemistry_0141b5c2_9f15_46f4_82e6_92a104faa476 a owl:Class ;
    rdfs:label "DischargingCapacity"@en ;
    rdfs:comment "electric charge which an energy storage device can deliver under specified discharging conditions"@en ;
    rdfs:subClassOf :electrochemistry_791c1915_a791_4450_acd8_7f94764743b5 ;
    skos:altLabel "DischargeCapacity" ;
    skos:hiddenLabel "AH-OUT"@en,
        "CapD"@en,
        "CapD/mAh"@en,
        "Q discharge/mA.h"@en ;
    skos:prefLabel "DischargingCapacity"@en ;
    emmo:EMMO_50c298c2_55a2_4068_b3ac_4e948c33181f "https://www.electropedia.org/iev/iev.nsf/display?openform&ievref=482-03-14" ;
    emmo:EMMO_967080e5_2f42_4eb2_a3a9_c58143e835f9 "electric charge which an energy storage device can deliver under specified discharging conditions"@en ;
    emmo:EMMO_cc65321f_1964_4f16_aea3_2a8edf2f3394 emmo:AmpereHour,
        emmo:MilliAmpereHour ;
    :electrochemistry_097ea615_c209_4edd_a1a1_5eea71d98fe8 "wf dis cap"@en ;
    :electrochemistry_1b717a20_17e3_4480_8c60_c4ae94058f05 "Discharge_Capacity (Ah)"@en ;
    :electrochemistry_69022178_77b8_4669_97e2_351d45356e5a "Q discharge/mA.h"@en ;
    :electrochemistry_811aafc3_0c6d_470e_b67e_ff5c82992609 "Capacitance_DChg(mAh)"@en ;
    :electrochemistry_a07dd85b_d0df_4d5d_8b0c_14d20ea3fe45 "discharge_capacity"@en .

:electrochemistry_03a6ce70_5085_4683_bb4e_fc3c18f7143a a owl:Class ;
    rdfs:label "OhmicOverpotential"@en ;
    rdfs:comment "part of the electrode polarization arising from an electric current through an ohmic resistance within the electrode or the electrolyte"@en ;
    rdfs:subClassOf :electrochemistry_1cd1d777_e67b_47eb_81f1_edac35d9f2c6 ;
    skos:altLabel "OhmicOvervoltage"@en,
        "OhmicPolarization"@en ;
    skos:prefLabel "OhmicOverpotential"@en ;
    emmo:EMMO_50c298c2_55a2_4068_b3ac_4e948c33181f "https://www.electropedia.org/iev/iev.nsf/display?openform&ievref=482-03-09" ;
    emmo:EMMO_967080e5_2f42_4eb2_a3a9_c58143e835f9 "part of the electrode polarization arising from an electric current through an ohmic resistance within the electrode or the electrolyte"@en .

:electrochemistry_07e219c3_890f_488f_bd96_bee8e445d764 a owl:Class ;
    rdfs:label "ResidualCurrent"@en ;
    rdfs:comment "Electric current that flows, at a particular value of the applied potential, in the absence of the substance whose electrode behaviour is being investigated, i.e. a \"blank\" solution."@en,
        "I_{r}"@en,
        "The residual (or background) current may be subtracted from the total current to calculate the net faradaic current."@en ;
    rdfs:subClassOf emmo:EMMO_c995ae70_3b84_4ebb_bcfc_69e6a281bb88,
        :electrochemistry_aecc6094_c6a5_4a36_a825_8a497a2ae112 ;
    skos:altLabel "BackgroundCurrent"@en ;
    skos:prefLabel "ResidualCurrent"@en ;
    emmo:EMMO_967080e5_2f42_4eb2_a3a9_c58143e835f9 "Electric current that flows, at a particular value of the applied potential, in the absence of the substance whose electrode behaviour is being investigated, i.e. a \"blank\" solution."@en ;
    emmo:EMMO_fe015383_afb3_44a6_ae86_043628697aa2 "https://goldbook.iupac.org/terms/view/R05311"@en .

:electrochemistry_0853b072_3b80_4864_8147_24ce35407ade a owl:Class ;
    rdfs:label "CathodicOverpotential"@en ;
    rdfs:comment "electrode polarization associated with an electrochemical reduction reaction"@en ;
    rdfs:subClassOf :electrochemistry_f4fadc4e_ca7d_4e4e_89cf_eacf45b4041e ;
    skos:altLabel "CathodicPolarization"@en ;
    skos:prefLabel "CathodicOverpotential"@en ;
    emmo:EMMO_50c298c2_55a2_4068_b3ac_4e948c33181f "https://www.electropedia.org/iev/iev.nsf/display?openform&ievref=482-03-07" ;
    emmo:EMMO_967080e5_2f42_4eb2_a3a9_c58143e835f9 "electrode polarization associated with an electrochemical reduction reaction"@en .

:electrochemistry_10763eb0_dbc9_4d34_bd1a_7b8996590d45 a owl:Class ;
    rdfs:label "ChargingCapacity"@en ;
    rdfs:comment "electric charge which an energy storage device can deliver under specified charging conditions"@en ;
    rdfs:subClassOf :electrochemistry_791c1915_a791_4450_acd8_7f94764743b5 ;
    skos:altLabel "ChargeCapacity" ;
    skos:hiddenLabel "AH-IN"@en,
        "CapC"@en,
        "CapC/mAh"@en,
        "Q charge/mA.h"@en ;
    skos:prefLabel "ChargingCapacity"@en ;
    emmo:EMMO_967080e5_2f42_4eb2_a3a9_c58143e835f9 "electric charge which an energy storage device can deliver under specified charging conditions"@en ;
    emmo:EMMO_cc65321f_1964_4f16_aea3_2a8edf2f3394 emmo:AmpereHour,
        emmo:MilliAmpereHour ;
    :electrochemistry_097ea615_c209_4edd_a1a1_5eea71d98fe8 "wf chg cap"@en ;
    :electrochemistry_1b717a20_17e3_4480_8c60_c4ae94058f05 "Charge_Capacity (Ah)"@en ;
    :electrochemistry_69022178_77b8_4669_97e2_351d45356e5a "Q charge/mA.h"@en ;
    :electrochemistry_811aafc3_0c6d_470e_b67e_ff5c82992609 "Capacitance_Chg(mAh)"@en ;
    :electrochemistry_a07dd85b_d0df_4d5d_8b0c_14d20ea3fe45 "charge_capacity"@en .

:electrochemistry_136744ff_0563_4df7_aa03_4219d70392a0 a owl:Class ;
    rdfs:label "PotentiometricSelectivityCoefficient"@en ;
    rdfs:comment "The selectivity coefficient is determined by means of the potential difference of the ion- selective electrode in mixed solutions of the primary ion, A, and interfering ion, B (Fixed Interference Method) or, less desirably, in separate solutions of A and B (Separate Solution Method). The activities of the primary ion, A, and the interfering ion, B, at which K is determined should always be specified, as the value of K is defined by a modified Nikolsky-Eisenman equation. The smaller the value of K , the A,B greater the electrode’s preference for the primary ion, A."@en,
        "parameter defining the ability of an ion-selective electrode to distinguish a particular ion, i.e., a primary ion A from an interfering ion B"@en ;
    rdfs:subClassOf :electrochemistry_aecc6094_c6a5_4a36_a825_8a497a2ae112 ;
    skos:altLabel "SelectivityCoefficient"@en,
        "SelectivityConstant"@en,
        "SelectivityFactor"@en ;
    skos:prefLabel "PotentiometricSelectivityCoefficient"@en ;
    emmo:EMMO_967080e5_2f42_4eb2_a3a9_c58143e835f9 "parameter defining the ability of an ion-selective electrode to distinguish a particular ion, i.e., a primary ion A from an interfering ion B"@en ;
    emmo:EMMO_fe015383_afb3_44a6_ae86_043628697aa2 "https://doi.org/10.1351/goldbook.P04791"@en .

:electrochemistry_14577b99_a8a9_4358_9bc5_ab8c401dd34b a owl:Class ;
    rdfs:label "NetFaradaicCurrent"@en ;
    rdfs:comment "I"@en,
        "algebraic sum of faradaic currents flowing through an electrode"@en ;
    rdfs:subClassOf :electrochemistry_2a2f59b7_aa16_40aa_9c8b_0de8a2720456 ;
    skos:prefLabel "NetFaradaicCurrent"@en ;
    emmo:EMMO_967080e5_2f42_4eb2_a3a9_c58143e835f9 "algebraic sum of faradaic currents flowing through an electrode"@en .

:electrochemistry_14d93129_d94d_42ff_a6f2_e8fca36ffec4 a owl:Class ;
    rdfs:label "EffectivePorousMediaQuantity"@en ;
    rdfs:comment "a physical quantity that is adjusted to consider the effects of porous media structure"@en ;
    rdfs:subClassOf emmo:EMMO_79751276_b2d0_4e2f_bbd4_99d412f43d55 ;
    skos:prefLabel "EffectivePorousMediaQuantity"@en ;
    emmo:EMMO_967080e5_2f42_4eb2_a3a9_c58143e835f9 "a physical quantity that is adjusted to consider the effects of porous media structure"@en .

:electrochemistry_16a5de33_a2ca_4563_80d4_6caeb08d97ca a owl:Class ;
    rdfs:label "Polarity"@en ;
    rdfs:comment "nominal property of an electrode, having values negative or positive according to the sign of the electrode potential, or neutral when the electrode potential is zero."@en ;
    rdfs:subClassOf :electrochemistry_900e357f_2ee3_425a_a0b6_322661117787 ;
    skos:prefLabel "Polarity"@en ;
    emmo:EMMO_50c298c2_55a2_4068_b3ac_4e948c33181f "https://www.electropedia.org/iev/iev.nsf/display?openform&ievref=114-02-14" ;
    emmo:EMMO_967080e5_2f42_4eb2_a3a9_c58143e835f9 "nominal property of an electrode, having values negative or positive according to the sign of the electrode potential, or neutral when the electrode potential is zero."@en .

:electrochemistry_1900143f_cbc0_415f_9057_9382022a7bfe a owl:Class ;
    rdfs:label "RotatingDiskSpeed"@en ;
    rdfs:comment "rotational frequency of a rotating component in a rotating disk electrode"@en ;
    rdfs:subClassOf emmo:EMMO_3789d3c5_77f4_456e_b7ed_40e670f47e52,
        :electrochemistry_c5047d29_4e68_43ee_8355_3e8f05dc70a5 ;
    skos:prefLabel "RotatingDiskSpeed"@en ;
    emmo:EMMO_967080e5_2f42_4eb2_a3a9_c58143e835f9 "rotational frequency of a rotating component in a rotating disk electrode"@en ;
    emmo:EMMO_c7b62dd7_063a_4c2a_8504_42f7264ba83f "The rotating component can be the main rotating disk or a secondary ring as used in rotating ring disk electrodes."@en .

:electrochemistry_214d925c_76c4_4f69_9afc_056a1ea82fc6 a owl:Class ;
    rdfs:label "AdsorptionCurrent"@en ;
    rdfs:comment "I_{ads}"@en,
        "The terms “adsorption current” and “limiting adsorption current” should not be applied to faradaic cur- rents that have been increased or decreased by adding a non-electroactive surfactant to a solution con- taining an electroactive substance, nor to currents resulting from the effect of adsorption or desorption on double-layer currents."@en,
        "electric current that accompanies the adsorption of a species"@en ;
    rdfs:subClassOf emmo:EMMO_c995ae70_3b84_4ebb_bcfc_69e6a281bb88,
        :electrochemistry_aecc6094_c6a5_4a36_a825_8a497a2ae112 ;
    skos:prefLabel "AdsorptionCurrent"@en ;
    emmo:EMMO_967080e5_2f42_4eb2_a3a9_c58143e835f9 "electric current that accompanies the adsorption of a species"@en ;
    emmo:EMMO_fe015383_afb3_44a6_ae86_043628697aa2 "https://goldbook.iupac.org/terms/view/A00159"@en .

:electrochemistry_22cec04f_c7f3_4ff8_a34b_e512379c9dcb a owl:Class ;
    rdfs:label "MigrationCurrent"@en ;
    rdfs:comment "I_{m}"@en,
        "The sign convention regarding current is such that the migration current is positive for the oxida- tion of a cation or the reduction of an anion and is negative for the reduction of a cation or for the oxidation of an anion. Hence, the migration current may either increase or decrease the total current observed. The migration current approaches zero as the transport number of the electroactive sub- stance is decreased by increasing the concentration of supporting electrolyte, and hence the conduc- tivity of the solution."@en,
        "component of electric current due to transport of ions in the electric field between the electrodes"@en ;
    rdfs:subClassOf emmo:EMMO_c995ae70_3b84_4ebb_bcfc_69e6a281bb88,
        :electrochemistry_4a450a27_b84a_4c70_a3a9_15ec30e2f30b ;
    skos:prefLabel "MigrationCurrent"@en ;
    emmo:EMMO_967080e5_2f42_4eb2_a3a9_c58143e835f9 "component of electric current due to transport of ions in the electric field between the electrodes"@en ;
    emmo:EMMO_fe015383_afb3_44a6_ae86_043628697aa2 "https://goldbook.iupac.org/terms/view/M03921"@en .

:electrochemistry_25dabdc2_68bf_4a38_8cbe_11be017358bc a owl:Class ;
    rdfs:label "IonicConductivity"@en ;
    rdfs:comment "a measure of a substance's tendency towards ionic conduction"@en ;
    rdfs:subClassOf emmo:EMMO_cde4368c_1d4d_4c94_8548_604749523c6d,
        :electrochemistry_4a450a27_b84a_4c70_a3a9_15ec30e2f30b ;
    owl:disjointWith :electrochemistry_ce74d2dc_d496_4116_b2fb_3e83d88bc744 ;
    skos:prefLabel "IonicConductivity"@en ;
    emmo:EMMO_26bf1bef_d192_4da6_b0eb_d2209698fb54 "https://www.wikidata.org/wiki/Q6063658" ;
    emmo:EMMO_967080e5_2f42_4eb2_a3a9_c58143e835f9 "a measure of a substance's tendency towards ionic conduction"@en ;
    emmo:EMMO_c84c6752_6d64_48cc_9500_e54a3c34898d "https://en.wikipedia.org/wiki/Ionic_conductivity_(solid_state)"@en ;
    emmo:EMMO_fe015383_afb3_44a6_ae86_043628697aa2 "https://doi.org/10.1351/goldbook.I03175"@en .

:electrochemistry_264f40d1_17c9_4bc7_9c47_5cfb18132278 a owl:Class ;
    rdfs:label "PotentialScanRate"@en ;
    rdfs:comment "the rate of change of applied potential with time"@en ;
    rdfs:subClassOf [ a owl:Restriction ;
            owl:onProperty emmo:EMMO_bed1d005_b04e_4a90_94cf_02bc678a8569 ;
            owl:someValuesFrom emmo:EMMO_6837b106_7220_4ec6_b7c9_d549d6163672 ],
        emmo:EMMO_2946d40b_24a1_47fa_8176_e3f79bb45064,
        :electrochemistry_c5047d29_4e68_43ee_8355_3e8f05dc70a5 ;
    skos:altLabel "PotentialSweepRate"@en,
        "ScanRate"@en,
        "SweepRate"@en ;
    skos:prefLabel "PotentialScanRate"@en ;
    emmo:EMMO_967080e5_2f42_4eb2_a3a9_c58143e835f9 "the rate of change of applied potential with time"@en .

:electrochemistry_265bb4d6_5eec_40f6_a3fa_59b3bd08e9af a owl:Class ;
    rdfs:label "CellPolarisationPotential"@en ;
    rdfs:comment "sum of the absolute values of the potential differences resulting from anodic and cathodic polarizations of an electrochemical cell"@en ;
    rdfs:subClassOf :electrochemistry_4ebe2ef1_eea8_4b10_822d_7a68215bd24d ;
    skos:altLabel "CellPolarizationPotential"@en ;
    skos:prefLabel "CellPolarisationPotential"@en ;
    emmo:EMMO_50c298c2_55a2_4068_b3ac_4e948c33181f "https://www.electropedia.org/iev/iev.nsf/display?openform&ievref=114-03-12" ;
    emmo:EMMO_967080e5_2f42_4eb2_a3a9_c58143e835f9 "sum of the absolute values of the potential differences resulting from anodic and cathodic polarizations of an electrochemical cell"@en .

:electrochemistry_269ddd97_1437_4545_b272_0df75a12c68a a owl:Class ;
    rdfs:label "BaselineCellVoltage"@en ;
    rdfs:comment "In electrochemical measurements, the voltage of an electrochemical cell to which a voltage signal is superimposed."@en ;
    rdfs:seeAlso "ElectrochemicalImpedanceSpectroscopy" ;
    rdfs:subClassOf :electrochemistry_4ebe2ef1_eea8_4b10_822d_7a68215bd24d,
        :electrochemistry_c5047d29_4e68_43ee_8355_3e8f05dc70a5 ;
    skos:prefLabel "BaselineCellVoltage"@en ;
    emmo:EMMO_967080e5_2f42_4eb2_a3a9_c58143e835f9 "In electrochemical measurements, the voltage of an electrochemical cell to which a voltage signal is superimposed."@en ;
    emmo:EMMO_b432d2d5_25f4_4165_99c5_5935a7763c1a "in EIS, an alternating voltage signal is superimposed to a baseline voltage, which can be the open circuit potential or a fixed cell voltage"@en .

:electrochemistry_2705525b_7512_48bf_825b_f2d0409bede4 a owl:Class ;
    rdfs:label "QuarterTransitionTimePotential"@en ;
    rdfs:comment "In practice, appropriate correction for the double-layer charging current is needed."@en,
        "electric potential of the indicator electrode, in chronopotentiometry at constant current, at the instant when the time that has elapsed since the application of current is equal to one-fourth of the transition time"@en ;
    rdfs:subClassOf [ a owl:Restriction ;
            owl:onProperty emmo:EMMO_bed1d005_b04e_4a90_94cf_02bc678a8569 ;
            owl:someValuesFrom emmo:EMMO_2e7e5796_4a80_4d73_bb84_f31138446c0c ],
        :electrochemistry_aecc6094_c6a5_4a36_a825_8a497a2ae112 ;
    skos:prefLabel "QuarterTransitionTimePotential"@en ;
    emmo:EMMO_967080e5_2f42_4eb2_a3a9_c58143e835f9 "electric potential of the indicator electrode, in chronopotentiometry at constant current, at the instant when the time that has elapsed since the application of current is equal to one-fourth of the transition time"@en .

:electrochemistry_2ae53fc6_d44d_41c9_acaf_c5606e6a981d a owl:Class ;
    rdfs:label "HalfWavePotential"@en ;
    rdfs:comment "E1/2 is used in techniques providing a sigmoidal wave-shaped current including DC voltammetry/polarography, normal pulse voltammetry, hydrodynamic voltammetry, and tast polarography."@en,
        "For quasi-reversible and irreversible electrode reactions, the value of E1/2 is also affected by the rate constant of the charge transfer reaction, the difference being greater than that caused by different diffusion coefficients."@en,
        "The quarter-wave potential, Ep/4, the three-quarter-wave potential, Ep3/4 , etc., may be similarly defined."@en,
        "electric potential of a steady-state voltammetric working electrode at the point, on the rising part of the voltammetric wave, where the current is equal to one-half of the limiting current"@en ;
    rdfs:subClassOf emmo:EMMO_4f2d3939_91b1_4001_b8ab_7d19074bf845,
        :electrochemistry_aecc6094_c6a5_4a36_a825_8a497a2ae112 ;
    skos:prefLabel "HalfWavePotential"@en ;
    emmo:EMMO_967080e5_2f42_4eb2_a3a9_c58143e835f9 "electric potential of a steady-state voltammetric working electrode at the point, on the rising part of the voltammetric wave, where the current is equal to one-half of the limiting current"@en ;
    emmo:EMMO_fe015383_afb3_44a6_ae86_043628697aa2 "https://doi.org/10.1351/goldbook.H02722"@en .

:electrochemistry_327eb3e1_f74a_4076_96de_5a2e3f63cb65 a owl:Class ;
    rdfs:label "SquareWaveCurrent"@en ;
    rdfs:comment "I_{SW}"@en,
        "The component may be faradaic (if the analyte is electroactive) or non-faradaic (if the analyte is surface-active). The simultaneous occurrence of both effects is quite common."@en,
        "component of an electric current that is associated with the presence of an analyate in square-wave voltammetry"@en ;
    rdfs:subClassOf emmo:EMMO_c995ae70_3b84_4ebb_bcfc_69e6a281bb88,
        :electrochemistry_aecc6094_c6a5_4a36_a825_8a497a2ae112 ;
    skos:prefLabel "SquareWaveCurrent"@en ;
    emmo:EMMO_967080e5_2f42_4eb2_a3a9_c58143e835f9 "component of an electric current that is associated with the presence of an analyate in square-wave voltammetry"@en ;
    emmo:EMMO_fe015383_afb3_44a6_ae86_043628697aa2 "https://goldbook.iupac.org/terms/view/S05897"@en .

:electrochemistry_346519a4_006c_496d_8f36_74e38814ed2d a owl:Class ;
    rdfs:label "PulseCurrent"@en ;
    rdfs:comment "the magnitude of a current pulse applied to an electrochemical cell during pulsed potentiometry and related techniques"@en ;
    rdfs:subClassOf emmo:EMMO_c995ae70_3b84_4ebb_bcfc_69e6a281bb88,
        :electrochemistry_c5047d29_4e68_43ee_8355_3e8f05dc70a5 ;
    skos:altLabel "MagnitudeOfCurrentPulse"@en,
        "PulseMagnitudeCurrent"@en ;
    skos:prefLabel "PulseCurrent"@en ;
    emmo:EMMO_967080e5_2f42_4eb2_a3a9_c58143e835f9 "the magnitude of a current pulse applied to an electrochemical cell during pulsed potentiometry and related techniques"@en .

:electrochemistry_382b10dc_83aa_4e77_a1d5_1edd06fd1e05 a owl:Class ;
    rdfs:label "PeakCurrent"@en ;
    rdfs:comment "I_{p}"@en,
        "Since the concentration of an electroactive substance at the electrode-solution interface decreases mono- tonically, the faradaic current due to its electrooxidation or electroreduction increases monotonically with time because of the increasing concentration gradient of the electroactive substance, the concentra- tion of which remains constant in the bulk. The maximum current value is passed when the transport rate of electroactive substance to the electrode-solution interface starts to be lower than the rate at which it is removed by reaction at the electrode. The result of these two competing processes leads to the peak- shaped I-E dependence."@en,
        "in dynamic voltammetric techniques, the maximum value of the faradaic current attained by varying the applied potential in the current-potential or I-E curve"@en ;
    rdfs:subClassOf emmo:EMMO_c995ae70_3b84_4ebb_bcfc_69e6a281bb88,
        :electrochemistry_aecc6094_c6a5_4a36_a825_8a497a2ae112 ;
    skos:prefLabel "PeakCurrent"@en ;
    emmo:EMMO_967080e5_2f42_4eb2_a3a9_c58143e835f9 "in dynamic voltammetric techniques, the maximum value of the faradaic current attained by varying the applied potential in the current-potential or I-E curve"@en ;
    emmo:EMMO_b432d2d5_25f4_4165_99c5_5935a7763c1a "Typical examples of imposed potential programmes in dynamic voltammetric techniques resulting in peak-shaped responses are linear-scan voltammetry, cyclic voltammetry, ac voltammetry, differential pulse voltammetry, square-wave voltammetry, stripping voltammetry, and derivative techniques."@en ;
    emmo:EMMO_fe015383_afb3_44a6_ae86_043628697aa2 "https://goldbook.iupac.org/terms/view/P04457"@en .

:electrochemistry_49efb72a_f8e6_4f50_acac_975302200d47 a owl:Class ;
    rdfs:label "ChargeRetention"@en ;
    rdfs:comment "ability of a cell or battery to retain capacity on open circuit under specified conditions."@en ;
    rdfs:seeAlso "SelfDischarge"@en ;
    rdfs:subClassOf :electrochemistry_900e357f_2ee3_425a_a0b6_322661117787 ;
    skos:altLabel "CapacityRetention"@en ;
    skos:prefLabel "ChargeRetention"@en ;
    emmo:EMMO_50c298c2_55a2_4068_b3ac_4e948c33181f "https://www.electropedia.org/iev/iev.nsf/display?openform&ievref=482-03-35" ;
    emmo:EMMO_967080e5_2f42_4eb2_a3a9_c58143e835f9 "ability of a cell or battery to retain capacity on open circuit under specified conditions."@en .

:electrochemistry_50674621_09ae_4f03_8ee9_3997b88c8b2a a owl:Class ;
    rdfs:label "FinishingCRate"@en ;
    rdfs:comment "[an indicator of the] electric current at which a battery is charged towards the end of charge"@en,
        "the quantity CRate is not used for energy-decoupled batteries like Redox Flox batteries"@en ;
    rdfs:subClassOf :electrochemistry_e1fd84eb_acdb_4b2c_b90c_e899d552a3ee ;
    skos:altLabel "FinishingChargeRate"@en ;
    skos:prefLabel "FinishingCRate"@en ;
    emmo:EMMO_50c298c2_55a2_4068_b3ac_4e948c33181f "https://www.electropedia.org/iev/iev.nsf/display?openform&ievref=482-05-46" ;
    emmo:EMMO_967080e5_2f42_4eb2_a3a9_c58143e835f9 "[an indicator of the] electric current at which a battery is charged towards the end of charge"@en .

:electrochemistry_526bf81a_0572_49ff_a8cc_85efc343c1c2 a owl:Class ;
    rdfs:label "ResidualActiveMass"@en ;
    rdfs:comment "charged active material remaining in a cell following a discharge to a specified end-of-discharge voltage."@en ;
    rdfs:subClassOf [ a owl:Restriction ;
            owl:onProperty emmo:EMMO_bed1d005_b04e_4a90_94cf_02bc678a8569 ;
            owl:someValuesFrom emmo:EMMO_77e9dc31_5b19_463e_b000_44c6e79f98aa ],
        :electrochemistry_aecc6094_c6a5_4a36_a825_8a497a2ae112 ;
    skos:prefLabel "ResidualActiveMass"@en ;
    emmo:EMMO_50c298c2_55a2_4068_b3ac_4e948c33181f "https://www.electropedia.org/iev/iev.nsf/display?openform&ievref=482-03-37"@en ;
    emmo:EMMO_967080e5_2f42_4eb2_a3a9_c58143e835f9 "charged active material remaining in a cell following a discharge to a specified end-of-discharge voltage."@en .

:electrochemistry_52ac73c7_763c_4fda_93cd_a2db9dfc2dab a owl:Class ;
    rdfs:label "SamplingInterval"@en ;
    rdfs:comment "time interval during which the current is measured in pulse voltammetry"@en ;
    rdfs:subClassOf emmo:EMMO_0adabf6f_7404_44cb_9f65_32d83d8101a3,
        :electrochemistry_c5047d29_4e68_43ee_8355_3e8f05dc70a5 ;
    skos:prefLabel "SamplingInterval"@en ;
    emmo:EMMO_967080e5_2f42_4eb2_a3a9_c58143e835f9 "time interval during which the current is measured in pulse voltammetry"@en ;
    emmo:EMMO_fe015383_afb3_44a6_ae86_043628697aa2 "https://doi.org/10.1351/goldbook.S05465"@en .

:electrochemistry_534dd59c_904c_45d9_8550_ae9d2eb6bbc9 a owl:Class ;
    rdfs:label "LowerVoltageLimit" ;
    rdfs:comment "minimum voltage limit at which an applied excitation is altered or terminated"@en,
        "specified voltage of a battery at which the battery discharge is terminated."@en ;
    rdfs:subClassOf :electrochemistry_5ebeea80_af22_456b_9087_78c2a8465c58 ;
    skos:altLabel "CutOffVoltage"@en,
        "DischargeCutoffVoltage"@en,
        "EndOfDischargeVoltage"@en,
        "EndPointVoltage"@en,
        "EndVoltage"@en,
        "FinalVoltage"@en,
        "LowerCutoffVoltage"@en ;
    skos:prefLabel "LowerVoltageLimit" ;
    emmo:EMMO_50c298c2_55a2_4068_b3ac_4e948c33181f "https://www.electropedia.org/iev/iev.nsf/display?openform&ievref=482-03-30" ;
    emmo:EMMO_967080e5_2f42_4eb2_a3a9_c58143e835f9 "minimum voltage limit at which an applied excitation is altered or terminated"@en .

:electrochemistry_565c0b10_70fe_441a_b76a_b9a8e08ca7b7 a owl:Class ;
    rdfs:label "AnodicOverpotential"@en ;
    rdfs:comment "electrode polarization associated with an electrochemical oxidation reaction"@en ;
    rdfs:subClassOf :electrochemistry_f4fadc4e_ca7d_4e4e_89cf_eacf45b4041e ;
    skos:altLabel "AnodicPolarization"@en ;
    skos:prefLabel "AnodicOverpotential"@en ;
    emmo:EMMO_50c298c2_55a2_4068_b3ac_4e948c33181f "https://www.electropedia.org/iev/iev.nsf/display?openform&ievref=482-03-06" ;
    emmo:EMMO_967080e5_2f42_4eb2_a3a9_c58143e835f9 "electrode polarization associated with an electrochemical oxidation reaction"@en .

:electrochemistry_5696453c_9da7_41e2_bbda_603c1b90a8fc a owl:Class ;
    rdfs:label "CoulombicEfficiency"@en ;
    rdfs:comment "fraction of the electric current passing through an electrochemical cell which accomplishes the desired chemical reaction"@en ;
    rdfs:subClassOf emmo:EMMO_faab3f84_e475_4a46_af9c_7d249f0b9aef,
        :electrochemistry_02eb0465_4f94_453c_8c1f_5ddf80134634 ;
    skos:altLabel "CoulombEfficiency"@en,
        "CurrentEfficiency"@en,
        "FaradayEfficiency"@en ;
    skos:hiddenLabel "CoulombEfficiency/%"@en ;
    skos:prefLabel "CoulombicEfficiency"@en ;
    emmo:EMMO_50c298c2_55a2_4068_b3ac_4e948c33181f "https://www.electropedia.org/iev/iev.nsf/display?openform&ievref=114-03-07" ;
    emmo:EMMO_967080e5_2f42_4eb2_a3a9_c58143e835f9 "fraction of the electric current passing through an electrochemical cell which accomplishes the desired chemical reaction"@en .

:electrochemistry_5c34b3b5_c9c4_477d_809a_3f682f995aa9 a owl:Class ;
    rdfs:label "BruggemanCoefficient"@en ;
    rdfs:comment "quantity that is used to estimate effective transport coefficients in porous media"@en,
        "valid in situations where the insulating phase is present in a low volume fraction and represented by random, isotropic spheres"@en ;
    rdfs:subClassOf emmo:EMMO_ba882f34_0d71_4e4f_9d92_0c076c633a2c ;
    skos:prefLabel "BruggemanCoefficient"@en ;
    emmo:EMMO_967080e5_2f42_4eb2_a3a9_c58143e835f9 "quantity that is used to estimate effective transport coefficients in porous media"@en .

:electrochemistry_5fb7a03f_d6dd_47ee_9317_0629681c7d00 a owl:Class ;
    rdfs:label "DiffusionLimitedCurrent"@en ;
    rdfs:comment "I_{d,lim}"@en,
        "diffusion current of the potential-independent value that is approached as the rate of the charge-transfer process is increased by varying the applied potential, being greater than the rate of mass transport controlled by diffusion"@en ;
    rdfs:subClassOf :electrochemistry_17626b8e_dfce_4d3a_ae6c_5a7215d43a90 ;
    skos:altLabel "LimitingDiffusionCurrent"@en ;
    skos:prefLabel "DiffusionLimitedCurrent"@en ;
    emmo:EMMO_967080e5_2f42_4eb2_a3a9_c58143e835f9 "diffusion current of the potential-independent value that is approached as the rate of the charge-transfer process is increased by varying the applied potential, being greater than the rate of mass transport controlled by diffusion"@en ;
    emmo:EMMO_fe015383_afb3_44a6_ae86_043628697aa2 "https://goldbook.iupac.org/terms/view/L03534"@en .

:electrochemistry_601ff226_59b9_460b_90f5_2593450d96fa a owl:Class ;
    rdfs:label "MembranePotential"@en ;
    rdfs:comment "electric potential difference between two solutions separated by an ion-selective membrane in the absence of any electric current flowing through the membrane"@en ;
    rdfs:subClassOf emmo:EMMO_4f2d3939_91b1_4001_b8ab_7d19074bf845,
        :electrochemistry_2d896559_eee3_447c_9759_87c854a4266a ;
    skos:altLabel "DonnanPotential"@en,
        "MembraneElectromotiveForce"@en ;
    skos:prefLabel "MembranePotential"@en ;
    emmo:EMMO_967080e5_2f42_4eb2_a3a9_c58143e835f9 "electric potential difference between two solutions separated by an ion-selective membrane in the absence of any electric current flowing through the membrane"@en ;
    emmo:EMMO_fe015383_afb3_44a6_ae86_043628697aa2 "https://doi.org/10.1351/goldbook.M03825"@en .

:electrochemistry_60741c58_a10d_4aa6_bb68_0066a6ff8e30 a owl:Class ;
    rdfs:label "SurfaceOverpotential"@en ;
    rdfs:comment "A positive surface overpotential produces a positive (anodic) current."@en,
        "The driving force for an electrochemcial charge-transfer reaction."@en,
        "The potential of a working electrode relative to a reference electrode of the same kinds placed in the solution adjacent to the surface of the working electrode (just outside the double layer)."@en,
        "\\eta_s = \\phi_{electrode} - \\phi_{solution} - E_{eq}"@en ;
    rdfs:subClassOf [ a owl:Restriction ;
            owl:onProperty emmo:EMMO_b2282816_b7a3_44c6_b2cb_3feff1ceb7fe ;
            owl:someValuesFrom :electrochemistry_d91940f0_c8b6_4505_9b68_6bf6cfc5c544 ],
        :electrochemistry_1cd1d777_e67b_47eb_81f1_edac35d9f2c6 ;
    skos:altLabel "SurfacePolarization"@en ;
    skos:prefLabel "SurfaceOverpotential"@en ;
    emmo:EMMO_967080e5_2f42_4eb2_a3a9_c58143e835f9 "The potential of a working electrode relative to a reference electrode of the same kinds placed in the solution adjacent to the surface of the working electrode (just outside the double layer)."@en .

:electrochemistry_639b844a_e801_436b_985d_28926129ead6 a owl:Class ;
    rdfs:label "NominalVoltage"@en ;
    rdfs:comment "suitable approximate value of the voltage used to designate or identify a cell, a battery or an electrochemical system"@en ;
    rdfs:subClassOf emmo:EMMO_17b031fb_4695_49b6_bb69_189ec63df3ee ;
    skos:prefLabel "NominalVoltage"@en ;
    skos:scopeNote "Nominal voltage is the standardized voltage value assigned to a battery cell or module based on typical operating conditions. It serves as a reference point for battery specifications but does not represent the actual voltage during operation. Actual cell voltage may vary due to factors such as state-of-charge, temperature, and load conditions."@en ;
    emmo:EMMO_50c298c2_55a2_4068_b3ac_4e948c33181f "https://www.electropedia.org/iev/iev.nsf/display?openform&ievref=482-03-31"@en ;
    emmo:EMMO_967080e5_2f42_4eb2_a3a9_c58143e835f9 "suitable approximate value of the voltage used to designate or identify a cell, a battery or an electrochemical system"@en ;
    emmo:EMMO_b6730304_cabc_4104_b415_14218466445c "Nominal voltage may not accurately reflect voltage under extreme loads or temperatures—always check manufacturer specifications."@en .

:electrochemistry_63a8f9d2_0cf6_484d_b996_2e5c3f0a3c73 a owl:Class ;
    rdfs:label "ElectrodeCoverageDensity"@en ;
    rdfs:comment "The total coverage may be distinguished from coverage that is electrochemically reactive or accessible on some given timescale."@en,
        "amount of a chemical modifier at an electrode surface per unit area"@en ;
    rdfs:subClassOf [ a owl:Restriction ;
            owl:onProperty emmo:EMMO_bed1d005_b04e_4a90_94cf_02bc678a8569 ;
            owl:someValuesFrom emmo:EMMO_183f6fac_8543_44e0_bd59_434aa7054f4c ],
        emmo:EMMO_2946d40b_24a1_47fa_8176_e3f79bb45064,
        :electrochemistry_aecc6094_c6a5_4a36_a825_8a497a2ae112 ;
    skos:altLabel "ElectrodeCoverage"@en ;
    skos:prefLabel "ElectrodeCoverageDensity"@en ;
    emmo:EMMO_967080e5_2f42_4eb2_a3a9_c58143e835f9 "amount of a chemical modifier at an electrode surface per unit area"@en .

:electrochemistry_68059d94_4c21_4065_b329_07faeebc7e87 a owl:Class ;
    rdfs:label "SignalReferencePotential"@en ;
    rdfs:comment "Alternating potential signals such as the ones applied in Electrochemical Impedance Spectroscopy are superimposed to a reference potential, which can be an applied potential or the open circuit potential."@en,
        "Potential to which the magnitude of an excitation signal is compared to."@en ;
    rdfs:subClassOf [ a owl:Restriction ;
            owl:onProperty emmo:EMMO_bed1d005_b04e_4a90_94cf_02bc678a8569 ;
            owl:someValuesFrom emmo:EMMO_2e7e5796_4a80_4d73_bb84_f31138446c0c ],
        :electrochemistry_c5047d29_4e68_43ee_8355_3e8f05dc70a5 ;
    skos:altLabel "BaselinePotential"@en ;
    skos:prefLabel "SignalReferencePotential"@en ;
    emmo:EMMO_967080e5_2f42_4eb2_a3a9_c58143e835f9 "Potential to which the magnitude of an excitation signal is compared to."@en .

:electrochemistry_74861991_7da2_4e0f_b6c1_b16713f538bf a owl:Class ;
    rdfs:label "InitialDischargingVoltage"@en ;
    rdfs:comment "discharge voltage of a cell or battery at the beginning of the discharge immediately after any transients have subsided"@en ;
    rdfs:subClassOf :electrochemistry_c7b26177_21bf_4787_b656_8e78edf27f88 ;
    skos:altLabel "InitialDischargeVoltage",
        "InitialClosedCircuitVoltage"@en ;
    skos:prefLabel "InitialDischargingVoltage"@en ;
    emmo:EMMO_50c298c2_55a2_4068_b3ac_4e948c33181f "https://www.electropedia.org/iev/iev.nsf/display?openform&ievref=482-03-29"@en ;
    emmo:EMMO_967080e5_2f42_4eb2_a3a9_c58143e835f9 "discharge voltage of a cell or battery at the beginning of the discharge immediately after any transients have subsided"@en .

:electrochemistry_76e7e556_f47e_47e2_b2ef_67aeed09c63e a owl:Class ;
    rdfs:label "CurrentDensityLimit"@en ;
    rdfs:comment "maximum electric current density that can be achieved for an electrode reaction at a given concentration of a electrochemically active material in the presence of a large excess of supporting electrolyte"@en ;
    rdfs:subClassOf emmo:EMMO_7c8007b0_58a7_4486_bf1c_4772852caca0,
        :electrochemistry_02eb0465_4f94_453c_8c1f_5ddf80134634 ;
    skos:prefLabel "CurrentDensityLimit"@en ;
    emmo:EMMO_50c298c2_55a2_4068_b3ac_4e948c33181f "https://www.electropedia.org/iev/iev.nsf/display?openform&ievref=114-03-13" ;
    emmo:EMMO_967080e5_2f42_4eb2_a3a9_c58143e835f9 "maximum electric current density that can be achieved for an electrode reaction at a given concentration of a electrochemically active material in the presence of a large excess of supporting electrolyte"@en .

:electrochemistry_79198264_cdf5_4fc3_8bcf_e5140a52547a a owl:Class ;
    rdfs:label "EnergyEfficiency"@en ;
    rdfs:comment "ratio of the electric energy provided from a secondary battery [ or electrochemical device ] during discharge to the electric energy supplied to the battery during the preceding charge"@en ;
    rdfs:subClassOf emmo:EMMO_faab3f84_e475_4a46_af9c_7d249f0b9aef,
        :electrochemistry_02eb0465_4f94_453c_8c1f_5ddf80134634 ;
    skos:altLabel "RoundTripEfficiency"@en ;
    skos:hiddenLabel "EnergyEfficiency/%"@en ;
    skos:prefLabel "EnergyEfficiency"@en ;
    emmo:EMMO_50c298c2_55a2_4068_b3ac_4e948c33181f "https://www.electropedia.org/iev/iev.nsf/display?openform&ievref=482-05-53" ;
    emmo:EMMO_967080e5_2f42_4eb2_a3a9_c58143e835f9 "ratio of the electric energy provided from a secondary battery [ or electrochemical device ] during discharge to the electric energy supplied to the battery during the preceding charge"@en .

:electrochemistry_7fa406b0_512a_4d59_9e0c_5d8aba0103ae a owl:Class ;
    rdfs:label "ActivationOverpotential"@en ;
    rdfs:comment "part of the electrode polarization arising from a charge-transfer step of the electrode reaction"@en ;
    rdfs:subClassOf :electrochemistry_1cd1d777_e67b_47eb_81f1_edac35d9f2c6 ;
    skos:altLabel "ActivationPolarization"@en ;
    skos:prefLabel "ActivationOverpotential"@en ;
    emmo:EMMO_50c298c2_55a2_4068_b3ac_4e948c33181f "https://www.electropedia.org/iev/iev.nsf/display?openform&ievref=482-03-05"@en ;
    emmo:EMMO_967080e5_2f42_4eb2_a3a9_c58143e835f9 "part of the electrode polarization arising from a charge-transfer step of the electrode reaction"@en .

:electrochemistry_83928dce_9746_4452_a9f9_da4366a20ca4 a owl:Class ;
    rdfs:label "ElectrolyteContainment"@en ;
    rdfs:comment "ability of a cell or battery to contain its electrolyte under specified mechanical and environmental conditions"@en ;
    rdfs:subClassOf :electrochemistry_900e357f_2ee3_425a_a0b6_322661117787 ;
    skos:prefLabel "ElectrolyteContainment"@en ;
    emmo:EMMO_50c298c2_55a2_4068_b3ac_4e948c33181f "https://www.electropedia.org/iev/iev.nsf/display?openform&ievref=482-02-31" ;
    emmo:EMMO_967080e5_2f42_4eb2_a3a9_c58143e835f9 "ability of a cell or battery to contain its electrolyte under specified mechanical and environmental conditions"@en .

:electrochemistry_83fbc038_0c2e_4d04_91d7_cdf30f8a5535 a owl:Class ;
    rdfs:label "Prismatic"@en ;
    rdfs:comment "[a sign that] qualifies a cell or a battery having the shape of a parallelepiped whose faces are rectangular"@en ;
    rdfs:subClassOf :electrochemistry_900e357f_2ee3_425a_a0b6_322661117787 ;
    skos:prefLabel "Prismatic"@en ;
    emmo:EMMO_50c298c2_55a2_4068_b3ac_4e948c33181f "https://www.electropedia.org/iev/iev.nsf/display?openform&ievref=482-02-38" ;
    emmo:EMMO_967080e5_2f42_4eb2_a3a9_c58143e835f9 "[a sign that] qualifies a cell or a battery having the shape of a parallelepiped whose faces are rectangular"@en .

:electrochemistry_8430be19_6cae_4a15_a570_3c15d0d190eb a owl:Class ;
    rdfs:label "PercentUnit"@en ;
    rdfs:comment "unit of percentage"@en ;
    rdfs:subClassOf emmo:EMMO_c2f5ee66_579c_44c6_a2e9_fa2eaa9fa4da ;
    skos:prefLabel "PercentUnit"@en ;
    emmo:EMMO_967080e5_2f42_4eb2_a3a9_c58143e835f9 "unit of percentage"@en .

:electrochemistry_8de9735b_374a_4a0f_b29f_71a50794cf94 a owl:Class ;
    rdfs:label "CrystalizationOverpotential"@en ;
    rdfs:comment "part of the electrode polarization arising from crystal nucleation and growth phenomena"@en ;
    rdfs:subClassOf :electrochemistry_f4fadc4e_ca7d_4e4e_89cf_eacf45b4041e ;
    skos:altLabel "CrystalizationPolarization"@en ;
    skos:prefLabel "CrystalizationOverpotential"@en ;
    emmo:EMMO_50c298c2_55a2_4068_b3ac_4e948c33181f "https://www.electropedia.org/iev/iev.nsf/display?openform&ievref=482-03-04" ;
    emmo:EMMO_967080e5_2f42_4eb2_a3a9_c58143e835f9 "part of the electrode polarization arising from crystal nucleation and growth phenomena"@en .

:electrochemistry_8f3ab19f_ce22_424e_a9bf_d5cedb815374 a owl:Class ;
    rdfs:label "TemperatureCoefficientOfTheCapacity"@en ;
    rdfs:comment "quotient of the change in capacity of a cell by the corresponding change in temperature."@en ;
    rdfs:subClassOf :electrochemistry_aecc6094_c6a5_4a36_a825_8a497a2ae112 ;
    skos:prefLabel "TemperatureCoefficientOfTheCapacity"@en ;
    emmo:EMMO_50c298c2_55a2_4068_b3ac_4e948c33181f "https://www.electropedia.org/iev/iev.nsf/display?openform&ievref=482-03-18" ;
    emmo:EMMO_967080e5_2f42_4eb2_a3a9_c58143e835f9 "quotient of the change in capacity of a cell by the corresponding change in temperature."@en .

:electrochemistry_98b6e9d7_d5df_46a5_87dd_79642b8b2e4b a owl:Class ;
    rdfs:label "KineticCurrent"@en ;
    rdfs:comment "The kinetic current is partially or entirely controlled by the rate of the chemical reaction. This reaction may be heterogeneous, occurring at an electrode-solution interface (surface reaction), or it may be homo- geneous, occurring at some distance from the interface (bulk reaction)."@en,
        "faradaic current of an electroactive substance B formed by a prior chemical reaction from another substance Y that is no electroactive at the potential at which B is electrochemically transformed"@en ;
    rdfs:subClassOf :electrochemistry_2a2f59b7_aa16_40aa_9c8b_0de8a2720456 ;
    skos:prefLabel "KineticCurrent"@en ;
    emmo:EMMO_967080e5_2f42_4eb2_a3a9_c58143e835f9 "faradaic current of an electroactive substance B formed by a prior chemical reaction from another substance Y that is no electroactive at the potential at which B is electrochemically transformed"@en ;
    emmo:EMMO_fe015383_afb3_44a6_ae86_043628697aa2 "https://goldbook.iupac.org/terms/view/K03399"@en .

:electrochemistry_9bf40017_3f58_4030_ada7_cb37a3dfda2d a owl:Class ;
    rdfs:label "InternalResistance"@en ;
    rdfs:comment "According to to Thévenin's theorem can any linear electric curcuit be replaced with a voltage source in series with an impedance. This impedance is for historical reasons termed \"internal resistance\"."@en,
        "For batteries, it the internal resistance the resistance of the cell."@en,
        "impedance of a linear circuit's Thévenin representation"@en ;
    rdfs:subClassOf emmo:EMMO_e88f75d6_9a17_4cfc_bdf7_43d7cea5a9a1,
        :electrochemistry_02eb0465_4f94_453c_8c1f_5ddf80134634 ;
    skos:prefLabel "InternalResistance"@en ;
    emmo:EMMO_26bf1bef_d192_4da6_b0eb_d2209698fb54 "https://www.wikidata.org/wiki/Q2527701" ;
    emmo:EMMO_50c298c2_55a2_4068_b3ac_4e948c33181f "https://www.electropedia.org/iev/iev.nsf/display?openform&ievref=485-15-04" ;
    emmo:EMMO_967080e5_2f42_4eb2_a3a9_c58143e835f9 "impedance of a linear circuit's Thévenin representation"@en ;
    emmo:EMMO_c84c6752_6d64_48cc_9500_e54a3c34898d "https://en.wikipedia.org/wiki/Internal_resistance"@en ;
    :electrochemistry_097ea615_c209_4edd_a1a1_5eea71d98fe8 "dcir/ohms"@en ;
    :electrochemistry_811aafc3_0c6d_470e_b67e_ff5c82992609 "DCIR(O)"@en ;
    :electrochemistry_a07dd85b_d0df_4d5d_8b0c_14d20ea3fe45 "internal_resistance"@en .

:electrochemistry_a56fc557_9dea_42e6_b936_e9d62dcaf84f a owl:Class ;
    rdfs:label "DoubleLayerCurrent"@en ;
    rdfs:comment "non-faradaic current associated with the charging of the electrical double layer at the electrode-solution interface"@en ;
    rdfs:subClassOf emmo:EMMO_c995ae70_3b84_4ebb_bcfc_69e6a281bb88,
        :electrochemistry_aecc6094_c6a5_4a36_a825_8a497a2ae112 ;
    skos:prefLabel "DoubleLayerCurrent"@en ;
    emmo:EMMO_967080e5_2f42_4eb2_a3a9_c58143e835f9 "non-faradaic current associated with the charging of the electrical double layer at the electrode-solution interface"@en ;
    emmo:EMMO_fe015383_afb3_44a6_ae86_043628697aa2 "https://goldbook.iupac.org/terms/view/D01847"@en .

:electrochemistry_a5962e05_466d_46a4_8951_bea59d7326e5 a owl:Class ;
    rdfs:label "ChargeEfficiency"@en ;
    rdfs:comment "ratio of the electric charge discharged from a secondary battery to the electric charge provided during the preceding charge"@en ;
    rdfs:subClassOf emmo:EMMO_faab3f84_e475_4a46_af9c_7d249f0b9aef,
        :electrochemistry_02eb0465_4f94_453c_8c1f_5ddf80134634 ;
    skos:prefLabel "ChargeEfficiency"@en ;
    emmo:EMMO_50c298c2_55a2_4068_b3ac_4e948c33181f "https://www.electropedia.org/iev/iev.nsf/display?openform&ievref=482-05-39"@en ;
    emmo:EMMO_967080e5_2f42_4eb2_a3a9_c58143e835f9 "ratio of the electric charge discharged from a secondary battery to the electric charge provided during the preceding charge"@en .

:electrochemistry_a82e16c3_b766_482f_be94_b8e9af37f6fc a owl:Class ;
    rdfs:label "ElectrodeRealSurfaceArea"@en ;
    rdfs:comment "A_{real}",
        "surface area of an electrode that takes into account non-idealities of the interface (roughness, porosity, etc.) and can be measured by a variety of electrochemical methods"@en,
        "the electroactive area is the area calculated from experiments with model electroactive species and may be different from the real surface area in cases where not all of the surface is electrochemically active or accessible"@en ;
    rdfs:subClassOf :electrochemistry_47ab1dad_cc09_4fd8_af23_acb36fb680dd ;
    skos:prefLabel "ElectrodeRealSurfaceArea"@en ;
    emmo:EMMO_967080e5_2f42_4eb2_a3a9_c58143e835f9 "surface area of an electrode that takes into account non-idealities of the interface (roughness, porosity, etc.) and can be measured by a variety of electrochemical methods"@en .

:electrochemistry_abfadc99_6e43_4d37_9b04_7fc5b0f327ae a owl:Class ;
    rdfs:label "NumberOfElectronsTransferred"@en ;
    rdfs:comment "Symbol n is commonly used when there is no risk of confusion with an amount of substance."@en,
        "The apparent number of electrons transferred, z_{app} , represents the experimentally measured number of electrons transferred between an electrode and one electroactive substance species, whose identity must be specified. When the electrooxidation or electroreduction of a substance B is accompanied by chemical processes, such as the catalyzed or induced reduction of a second substance, or a side reaction that consumes B or an intermediate, the value of z_{app} will differ from that of z."@en,
        "number of electrons transferred in a charge transfer reaction between an electrode and a single entity (ion, radical-ion, or molecule) of an electroactive substance, whose identity must be specified"@en ;
    rdfs:subClassOf emmo:EMMO_ba882f34_0d71_4e4f_9d92_0c076c633a2c,
        :electrochemistry_21745019_2830_4395_bca7_15ddfd266673 ;
    skos:altLabel "ChargeNumber"@en,
        "ElectronNumberOfAnElectrochemicalReaction"@en ;
    skos:prefLabel "NumberOfElectronsTransferred"@en ;
    emmo:EMMO_967080e5_2f42_4eb2_a3a9_c58143e835f9 "number of electrons transferred in a charge transfer reaction between an electrode and a single entity (ion, radical-ion, or molecule) of an electroactive substance, whose identity must be specified"@en ;
    emmo:EMMO_fe015383_afb3_44a6_ae86_043628697aa2 "https://goldbook.iupac.org/terms/view/C00995" .

:electrochemistry_ae9882de_d6a2_4525_a84f_80947c10f1cb a owl:Class ;
    rdfs:label "TransitionTime"@en ;
    rdfs:comment "In experimental practice, the latter is often taken to be the moment when the rate of varia- tion of the potential of the indicator electrode attains a maximum value."@en,
        "in chronopotentiometry and related techniques, the duration between the application of current and when the concentration of an electroactive substance at the electrode-solution interface becomes indistinguishable from zero"@en ;
    rdfs:subClassOf :electrochemistry_aecc6094_c6a5_4a36_a825_8a497a2ae112 ;
    skos:prefLabel "TransitionTime"@en ;
    emmo:EMMO_967080e5_2f42_4eb2_a3a9_c58143e835f9 "in chronopotentiometry and related techniques, the duration between the application of current and when the concentration of an electroactive substance at the electrode-solution interface becomes indistinguishable from zero"@en ;
    emmo:EMMO_fe015383_afb3_44a6_ae86_043628697aa2 "https://doi.org/10.1351/goldbook.T06472"@en .

:electrochemistry_b21de1ef_6c15_4d63_b320_c9b96fbf186f a owl:Class ;
    rdfs:label "FormalElectrodePotential"@en ;
    rdfs:comment "E^{\\circ '}"@en,
        "E_{eq} = E^{\\circ '} - (R*T / (z*F)) * \\sum_i{\\nu_i * ln(c_i/c^{circ})}"@en,
        "It is E°′ which is calculated in electrochemical experiments when the concentrations of the various species are known, but their activities are not. Its value depends on the composi- tion of the electrolyte solution. The argument of ln is dimensionless, while the concentration ci is normalized through division by the standard concentration, usually c° = 1 mol dm^{−3} for soluble species."@en,
        "equilibrium electrode potential under conditions of unit concentration of species involved in the electrode reaction"@en ;
    rdfs:subClassOf :electrochemistry_d91940f0_c8b6_4505_9b68_6bf6cfc5c544 ;
    skos:altLabel "FormalPotential"@en ;
    skos:prefLabel "FormalElectrodePotential"@en ;
    emmo:EMMO_967080e5_2f42_4eb2_a3a9_c58143e835f9 "equilibrium electrode potential under conditions of unit concentration of species involved in the electrode reaction"@en .

:electrochemistry_bad1b6f4_1b26_40e2_b552_6d53873e3973 a owl:Class ;
    rdfs:label "ElectrochemicallyActiveSurfaceArea"@en ;
    rdfs:comment "the area of the electrode material that is accessible to the electrolyte that is used for charge transfer and/or storage"@en ;
    rdfs:subClassOf :electrochemistry_47ab1dad_cc09_4fd8_af23_acb36fb680dd ;
    skos:altLabel "EASA"@en,
        "ECSA"@en,
        "ElectrochemicalActiveSurfaceArea"@en ;
    skos:prefLabel "ElectrochemicallyActiveSurfaceArea"@en ;
    emmo:EMMO_50c298c2_55a2_4068_b3ac_4e948c33181f "https://www.electropedia.org/iev/iev.nsf/display?openform&ievref=485-02-09" ;
    emmo:EMMO_967080e5_2f42_4eb2_a3a9_c58143e835f9 "the area of the electrode material that is accessible to the electrolyte that is used for charge transfer and/or storage"@en .

:electrochemistry_bcb33f7e_5573_4bc2_b636_4ea313a9dd3a a owl:Class ;
    rdfs:label "AreicCapacity"@en ;
    rdfs:comment "Can also be applied to electrodes."@en,
        "quotient of the capacity of a battery cell or battery by its plane area."@en ;
    rdfs:subClassOf emmo:EMMO_2946d40b_24a1_47fa_8176_e3f79bb45064,
        :electrochemistry_02eb0465_4f94_453c_8c1f_5ddf80134634 ;
    skos:altLabel "ArealCapacity"@en ;
    skos:prefLabel "AreicCapacity"@en ;
    emmo:EMMO_50c298c2_55a2_4068_b3ac_4e948c33181f "https://www.electropedia.org/iev/iev.nsf/display?openform&ievref=482-03-20" ;
    emmo:EMMO_967080e5_2f42_4eb2_a3a9_c58143e835f9 "quotient of the capacity of a battery cell or battery by its plane area."@en .

:electrochemistry_c39b2498_783e_48e1_9814_6164bd99823c a owl:Class ;
    rdfs:label "WorkingPotentialRange"@en ;
    rdfs:comment "Because the working potential range is a function of a specific electrode/electrolyte system, only approximate ranges can be given for generic systems."@en,
        "The working potential range is usually limited by the stability of the electrolyte, itself affected by the catalytic properties of the electrode, or by the stability of the electrode."@en,
        "range of electrode potentials of a given working electrode in a given electrolyte, where the electric current from reactions of the electrode or electrolyte is negligible compared with the current from reactions of the system under investigation"@en ;
    rdfs:subClassOf emmo:EMMO_4f2d3939_91b1_4001_b8ab_7d19074bf845,
        :electrochemistry_aecc6094_c6a5_4a36_a825_8a497a2ae112 ;
    skos:prefLabel "WorkingPotentialRange"@en ;
    emmo:EMMO_967080e5_2f42_4eb2_a3a9_c58143e835f9 "range of electrode potentials of a given working electrode in a given electrolyte, where the electric current from reactions of the electrode or electrolyte is negligible compared with the current from reactions of the system under investigation"@en .

:electrochemistry_c4d551db_db17_4c33_92e6_aec71638afbc a owl:Class ;
    rdfs:label "HalfPeakPotential"@en ;
    rdfs:comment "The quarter-peak potential, Ep/4, the three-quarter-peak potential, Ep3/4, etc., may be similarly defined."@en,
        "This term is used in techniques providing peak-shaped responses (linear scan voltammetry, cyclic voltammetry, AC voltammetry, differential pulse voltammetry, square-wave voltam- metry, stripping voltammetry, and derivative techniques)."@en,
        "for dynamic voltammetric techniques, the electric potential of the working electrode at which the current is equal to one-half of the peak current"@en ;
    rdfs:subClassOf emmo:EMMO_4f2d3939_91b1_4001_b8ab_7d19074bf845,
        :electrochemistry_aecc6094_c6a5_4a36_a825_8a497a2ae112 ;
    skos:prefLabel "HalfPeakPotential"@en ;
    emmo:EMMO_967080e5_2f42_4eb2_a3a9_c58143e835f9 "for dynamic voltammetric techniques, the electric potential of the working electrode at which the current is equal to one-half of the peak current"@en ;
    emmo:EMMO_fe015383_afb3_44a6_ae86_043628697aa2 "https://doi.org/10.1351/goldbook.H02720"@en .

:electrochemistry_c55bcb85_b7b8_4e67_8a78_9a42fe25b6cf a owl:Class ;
    rdfs:label "CatalyticCurrent"@en ;
    rdfs:comment "I_{cat}"@en,
        "In either of the two following situations, the current increase is termed a catalytic current: (i) The scheme below generates a catalytic or regenerative current: B±e→ B′, B' + A → B (ii) The presence at the electrode-solution interface of a substance, which may be added or generated by an electrochemical reaction, decreases the overpotential for the electrochemical reaction of B. In either case, the magnitude of the catalytic current depends on the applied potential. If the current observed with a mixture of A and B is lower than the sum of the separate currents, the term non-additive current should be used."@en,
        "faradaic current measured in a solution containing two electroactive substances, A and B, that exceeds the sum of the faradaic currents that would be obtained for A and B separately under the same experimental conditions"@en ;
    rdfs:subClassOf :electrochemistry_2a2f59b7_aa16_40aa_9c8b_0de8a2720456 ;
    skos:prefLabel "CatalyticCurrent"@en ;
    emmo:EMMO_967080e5_2f42_4eb2_a3a9_c58143e835f9 "faradaic current measured in a solution containing two electroactive substances, A and B, that exceeds the sum of the faradaic currents that would be obtained for A and B separately under the same experimental conditions"@en ;
    emmo:EMMO_fe015383_afb3_44a6_ae86_043628697aa2 "https://doi.org/10.1351/goldbook.C00889"@en .

:electrochemistry_d47985f1_6bd7_4c4f_894f_13a6cab38bb5 a owl:Class ;
    rdfs:label "ResidualCapacity"@en ;
    rdfs:comment "electric charge capacity remaining in a cell or battery following a discharge, operation or storage under specific test conditions"@en ;
    rdfs:subClassOf :electrochemistry_791c1915_a791_4450_acd8_7f94764743b5 ;
    skos:prefLabel "ResidualCapacity"@en ;
    emmo:EMMO_50c298c2_55a2_4068_b3ac_4e948c33181f "https://www.electropedia.org/iev/iev.nsf/display?openform&ievref=482-03-16" ;
    emmo:EMMO_967080e5_2f42_4eb2_a3a9_c58143e835f9 "electric charge capacity remaining in a cell or battery following a discharge, operation or storage under specific test conditions"@en .

:electrochemistry_d5ac8868_d318_4065_aa23_72140ae888ae a owl:Class ;
    rdfs:label "LimitingCurrent"@en ;
    rdfs:comment "A limiting current is reached when the overpotential is sufficiently large that the faradaic current is deter- mined solely by the ability to supply electroactive species by mass transport. A limiting current is there- fore independent of applied potential over a corresponding finite potential range. A limiting current may have the character of an adsorption, catalytic, diffusion, or kinetic current, and may include a migration current."@en,
        "faradaic current that is approached as the rate of the charge-transfer process is increased by varying the applied potential, being greater than the rate of mass transport controlled by diffusion"@en ;
    rdfs:subClassOf :electrochemistry_2a2f59b7_aa16_40aa_9c8b_0de8a2720456 ;
    skos:prefLabel "LimitingCurrent"@en ;
    emmo:EMMO_967080e5_2f42_4eb2_a3a9_c58143e835f9 "faradaic current that is approached as the rate of the charge-transfer process is increased by varying the applied potential, being greater than the rate of mass transport controlled by diffusion"@en ;
    emmo:EMMO_fe015383_afb3_44a6_ae86_043628697aa2 "https://goldbook.iupac.org/terms/view/L03532"@en .

:electrochemistry_da215d1a_196a_465f_9de8_89f6fbb76982 a owl:Class ;
    rdfs:label "RatedEnergy"@en ;
    rdfs:comment "the amount of energy that an electrochemical device can store under some specific conditions"@en ;
    rdfs:subClassOf :electrochemistry_46376e5d_9627_4514_9881_9e62083625c3 ;
    skos:prefLabel "RatedEnergy"@en ;
    emmo:EMMO_967080e5_2f42_4eb2_a3a9_c58143e835f9 "the amount of energy that an electrochemical device can store under some specific conditions"@en .

:electrochemistry_e38f11d0_a16f_4fe8_8ec5_3fe4493b7759 a owl:Class ;
    rdfs:label "DiffuseLayerPotential"@en ;
    rdfs:comment "electric potential difference between the rigid layer and the diffuse layer of a double layer"@en ;
    rdfs:subClassOf emmo:EMMO_4f2d3939_91b1_4001_b8ab_7d19074bf845,
        :electrochemistry_aecc6094_c6a5_4a36_a825_8a497a2ae112 ;
    skos:prefLabel "DiffuseLayerPotential"@en ;
    emmo:EMMO_50c298c2_55a2_4068_b3ac_4e948c33181f "https://www.electropedia.org/iev/iev.nsf/display?openform&ievref=114-02-20" ;
    emmo:EMMO_967080e5_2f42_4eb2_a3a9_c58143e835f9 "electric potential difference between the rigid layer and the diffuse layer of a double layer"@en .

:electrochemistry_e4a221e0_afc9_4464_91d4_e0c8ecdf79e8 a owl:Class ;
    rdfs:label "PeakPotential"@en ;
    rdfs:comment "This term is used in dynamic voltammetric techniques providing a peak-shaped current response (linear-sweep voltammetry, triangular-wave voltammetry, cyclic voltammetry, AC voltammetry, differential pulse voltammetry, square-wave voltammetry, stripping voltamme- try and derivative techniques)."@en,
        "electrode potential of the working electrode at which the peak current is attained"@en ;
    rdfs:subClassOf [ a owl:Restriction ;
            owl:onProperty emmo:EMMO_bed1d005_b04e_4a90_94cf_02bc678a8569 ;
            owl:someValuesFrom emmo:EMMO_2e7e5796_4a80_4d73_bb84_f31138446c0c ],
        :electrochemistry_aecc6094_c6a5_4a36_a825_8a497a2ae112 ;
    skos:prefLabel "PeakPotential"@en ;
    emmo:EMMO_967080e5_2f42_4eb2_a3a9_c58143e835f9 "electrode potential of the working electrode at which the peak current is attained"@en ;
    emmo:EMMO_fe015383_afb3_44a6_ae86_043628697aa2 "https://doi.org/10.1351/goldbook.P04464"@en .

:electrochemistry_e6b63190_acac_4e78_9cba_fb2b10bbe910 a owl:Class ;
    rdfs:label "VolumetricCapacity"@en ;
    rdfs:comment "quotient of the capacity of a cell or battery by its volume."@en ;
    rdfs:subClassOf :electrochemistry_aecc6094_c6a5_4a36_a825_8a497a2ae112 ;
    skos:altLabel "VolumetricChargeCapacity"@en,
        "VolumetricElectricChargeCapacity"@en ;
    skos:prefLabel "VolumetricCapacity"@en ;
    emmo:EMMO_50c298c2_55a2_4068_b3ac_4e948c33181f "https://www.electropedia.org/iev/iev.nsf/display?openform&ievref=482-03-17" ;
    emmo:EMMO_967080e5_2f42_4eb2_a3a9_c58143e835f9 "quotient of the capacity of a cell or battery by its volume."@en .

:electrochemistry_e8ec76bf_2a60_4982_8cde_02dfbd2e626f a owl:Class ;
    rdfs:label "ShelfLife"@en ;
    rdfs:comment "duration, under specific conditions, at the end of which a battery [ or electrochemical device ] has retained the ability to perform a specified function"@en ;
    rdfs:subClassOf :electrochemistry_02eb0465_4f94_453c_8c1f_5ddf80134634 ;
    skos:altLabel "StorageLife"@en ;
    skos:prefLabel "ShelfLife"@en ;
    emmo:EMMO_50c298c2_55a2_4068_b3ac_4e948c33181f "https://www.electropedia.org/iev/iev.nsf/display?openform&ievref=482-03-47" ;
    emmo:EMMO_967080e5_2f42_4eb2_a3a9_c58143e835f9 "duration, under specific conditions, at the end of which a battery [ or electrochemical device ] has retained the ability to perform a specified function"@en .

:electrochemistry_ecb6dfdf_bd3d_4339_8a1c_d32abbef30ba a owl:Class ;
    rdfs:label "SamplingTime"@en ;
    rdfs:comment "duration of the sampling interval in pulse voltammetry"@en ;
    rdfs:subClassOf emmo:EMMO_0adabf6f_7404_44cb_9f65_32d83d8101a3,
        :electrochemistry_c5047d29_4e68_43ee_8355_3e8f05dc70a5 ;
    skos:prefLabel "SamplingTime"@en ;
    emmo:EMMO_967080e5_2f42_4eb2_a3a9_c58143e835f9 "duration of the sampling interval in pulse voltammetry"@en ;
    emmo:EMMO_fe015383_afb3_44a6_ae86_043628697aa2 "https://doi.org/10.1351/goldbook.S05467"@en .

:electrochemistry_f591a444_89d6_4093_836d_7d53895edce4 a owl:Class ;
    rdfs:label "AmplitudeOfAlternatingVoltage"@en ;
    rdfs:comment "For Electrochemical Impedance Spectroscopy, the Peak Potential Amplitude is usually small, (normally 5 to 10 mV)."@en,
        "half of the peak-to-peak amplitude of a periodic voltage perturbation within a single time period, with respect to a reference potential value"@en ;
    rdfs:subClassOf emmo:EMMO_4f2d3939_91b1_4001_b8ab_7d19074bf845,
        :electrochemistry_c5047d29_4e68_43ee_8355_3e8f05dc70a5 ;
    skos:prefLabel "AmplitudeOfAlternatingVoltage"@en ;
    emmo:EMMO_967080e5_2f42_4eb2_a3a9_c58143e835f9 "half of the peak-to-peak amplitude of a periodic voltage perturbation within a single time period, with respect to a reference potential value"@en ;
    emmo:EMMO_c7b62dd7_063a_4c2a_8504_42f7264ba83f "This term should denote half of the peak-to-peak amplitude. Peak-to-peak and r.m.s. amplitudes should be so specified."@en ;
    emmo:EMMO_fe015383_afb3_44a6_ae86_043628697aa2 "https://doi.org/10.1351/goldbook.A00311" .

:electrochemistry_f6f45881_9bf1_4cf5_988b_de79dab718ef a owl:Class ;
    rdfs:label "VoltageChangeRate"@en ;
    rdfs:comment "the first order time rate of change of voltage"@en ;
    rdfs:subClassOf [ a owl:Restriction ;
            owl:onProperty emmo:EMMO_bed1d005_b04e_4a90_94cf_02bc678a8569 ;
            owl:someValuesFrom emmo:EMMO_6837b106_7220_4ec6_b7c9_d549d6163672 ],
        :electrochemistry_aecc6094_c6a5_4a36_a825_8a497a2ae112 ;
    skos:altLabel "dV/dt" ;
    skos:prefLabel "VoltageChangeRate"@en ;
    emmo:EMMO_967080e5_2f42_4eb2_a3a9_c58143e835f9 "the first order time rate of change of voltage"@en ;
    :electrochemistry_a07dd85b_d0df_4d5d_8b0c_14d20ea3fe45 "dv/dt"@en ;
    :electrochemistry_ea9f4dba_8ca2_419e_9cdf_ce54e9ebbd46 "dVdt (I/h)"@en .

:electrochemistry_fa7790d6_07bb_4b0f_9965_55966828f5f3 a owl:Class ;
    rdfs:label "ElectrodeGeometricSurfaceArea"@en ;
    rdfs:comment "A_{geom}"@en,
        "the interfacial area, determined on the assumption that the interface is truly flat (2-dimensional) and calculated using the geometric data of the involved surfaces"@en ;
    rdfs:subClassOf :electrochemistry_47ab1dad_cc09_4fd8_af23_acb36fb680dd ;
    skos:prefLabel "ElectrodeGeometricSurfaceArea"@en ;
    emmo:EMMO_967080e5_2f42_4eb2_a3a9_c58143e835f9 "the interfacial area, determined on the assumption that the interface is truly flat (2-dimensional) and calculated using the geometric data of the involved surfaces"@en .

:electrochemistry_ff7797ed_9ef7_40d0_872b_2c215cd54578 a owl:Class ;
    rdfs:label "IsopotentialPoint"@en ;
    rdfs:comment "The specification of the ISE and outer reference electrode must be described."@en,
        "When an isothermal cell is used with identical internal and external reference electrodes, the isopotential point is the activity of sensed ions for which zero net membrane potential difference is measured, e.g., sensed ion activity is the same in the inner and outer (test) solution. Slopes of calibration plots for different cell temperatures are different, but inter- sect at a common activity point. Cells with temperature gradients are not recommended."@en,
        "electric potential of an ion-selective electrode (ISE) and activity of an analyte ion at which the potential of the ISE is independent of temperature"@en ;
    rdfs:subClassOf emmo:EMMO_4f2d3939_91b1_4001_b8ab_7d19074bf845,
        :electrochemistry_aecc6094_c6a5_4a36_a825_8a497a2ae112 ;
    skos:prefLabel "IsopotentialPoint"@en ;
    emmo:EMMO_967080e5_2f42_4eb2_a3a9_c58143e835f9 "electric potential of an ion-selective electrode (ISE) and activity of an analyte ion at which the potential of the ISE is independent of temperature"@en ;
    emmo:EMMO_fe015383_afb3_44a6_ae86_043628697aa2 "https://doi.org/10.1351/goldbook.I03304"@en .

emmo:EMMO_79a02de5_b884_4eab_bc18_f67997d597a2 :electrochemistry_097ea615_c209_4edd_a1a1_5eea71d98fe8 "acimp/ohms"@en .

emmo:EMMO_e218c625_6a39_47a9_8d08_a2ef41c152a9 rdfs:subClassOf :electrochemistry_02eb0465_4f94_453c_8c1f_5ddf80134634 ;
    skos:altLabel "GravimetricEnergyDensity"@en ;
    :electrochemistry_811aafc3_0c6d_470e_b67e_ff5c82992609 "CmpEng(mWh/g)"@en .

:electrochemistry_0335e3f6_d1d8_4daa_8376_a9285f1bc9f1 a owl:Class ;
    rdfs:label "ReactionRateConstant"@en ;
    rdfs:comment "a proportionality constant which quantifies the rate and direction of a chemical reaction by relating it with the concentration of reactants"@en ;
    rdfs:subClassOf emmo:EMMO_2946d40b_24a1_47fa_8176_e3f79bb45064,
        :electrochemistry_21745019_2830_4395_bca7_15ddfd266673 ;
    skos:prefLabel "ReactionRateConstant"@en ;
    emmo:EMMO_26bf1bef_d192_4da6_b0eb_d2209698fb54 "https://www.wikidata.org/wiki/Q658700" ;
    emmo:EMMO_967080e5_2f42_4eb2_a3a9_c58143e835f9 "a proportionality constant which quantifies the rate and direction of a chemical reaction by relating it with the concentration of reactants"@en ;
    emmo:EMMO_c84c6752_6d64_48cc_9500_e54a3c34898d "https://en.wikipedia.org/wiki/Reaction_rate_constant"@en .

:electrochemistry_05cf26ef_782a_4f66_a196_7004dd973f8e a owl:Class ;
    rdfs:label "SurfaceArea"@en ;
    rdfs:comment "a measure of the total area that the surface of a solid object occupies"@en ;
    rdfs:subClassOf emmo:EMMO_96f39f77_44dc_491b_8fa7_30d887fe0890,
        :electrochemistry_aecc6094_c6a5_4a36_a825_8a497a2ae112 ;
    skos:prefLabel "SurfaceArea"@en ;
    emmo:EMMO_26bf1bef_d192_4da6_b0eb_d2209698fb54 "https://www.wikidata.org/wiki/Q1379273" ;
    emmo:EMMO_6dd685dd_1895_46e4_b227_be9f7d643c25 "https://dbpedia.org/page/Surface_area"@en ;
    emmo:EMMO_967080e5_2f42_4eb2_a3a9_c58143e835f9 "a measure of the total area that the surface of a solid object occupies"@en ;
    emmo:EMMO_c84c6752_6d64_48cc_9500_e54a3c34898d "https://en.wikipedia.org/wiki/Surface_area"@en .

:electrochemistry_1422cde1_929e_46b6_b0dc_1010eebc5dfd a owl:Class ;
    rdfs:label "ElectrochemicalPotential"@en ;
    rdfs:comment "in quantum mechanical terms, electrochemical potential is defined as the energy level of the electron orbitals in the species that have a 50 percent probability of occupancy"@en,
        "the chemical potential of an ion in the presence of an electric potential"@en ;
    rdfs:subClassOf [ a owl:Restriction ;
            owl:onProperty emmo:EMMO_bed1d005_b04e_4a90_94cf_02bc678a8569 ;
            owl:someValuesFrom emmo:EMMO_f6070071_d054_4b17_9d2d_f446f7147d0f ],
        emmo:EMMO_2946d40b_24a1_47fa_8176_e3f79bb45064,
        :electrochemistry_2d896559_eee3_447c_9759_87c854a4266a ;
    skos:prefLabel "ElectrochemicalPotential"@en ;
    emmo:EMMO_26bf1bef_d192_4da6_b0eb_d2209698fb54 "https://www.wikidata.org/wiki/Q62525" ;
    emmo:EMMO_967080e5_2f42_4eb2_a3a9_c58143e835f9 "the chemical potential of an ion in the presence of an electric potential"@en ;
    emmo:EMMO_c84c6752_6d64_48cc_9500_e54a3c34898d "https://en.wikipedia.org/wiki/Electrochemical_potential"@en ;
    emmo:EMMO_fe015383_afb3_44a6_ae86_043628697aa2 "https://goldbook.iupac.org/terms/view/E01945" .

:electrochemistry_17626b8e_dfce_4d3a_ae6c_5a7215d43a90 a owl:Class ;
    rdfs:label "DiffusionCurrent"@en ;
    rdfs:comment "Diffusion current is governed by Fick’s Laws of diffusion. It is the principle on which many electroana- lytical methods are based, because the current is proportional to the bulk concentration of the diffusing species. I_{d} = z*F*A*D*\\grad(c)_{x=0}, where z is the electron number of an electrochemical reaction, F the Faraday constant, A the electrode surface area, D the diffusion coefficient of electroactive substance, and (∂c/∂x)x=0 the gradient of the amount concentration at the electrode surface position x = 0."@en,
        "I_{d}"@en,
        "faradaic current that is controlled by the rate at which electroactive species diffuse toward (or away from) and electrode-solution interface."@en ;
    rdfs:subClassOf :electrochemistry_2a2f59b7_aa16_40aa_9c8b_0de8a2720456 ;
    skos:prefLabel "DiffusionCurrent"@en ;
    emmo:EMMO_26bf1bef_d192_4da6_b0eb_d2209698fb54 "https://www.wikidata.org/wiki/Q1224527" ;
    emmo:EMMO_967080e5_2f42_4eb2_a3a9_c58143e835f9 "faradaic current that is controlled by the rate at which electroactive species diffuse toward (or away from) and electrode-solution interface."@en ;
    emmo:EMMO_c84c6752_6d64_48cc_9500_e54a3c34898d "https://en.wikipedia.org/wiki/Diffusion_current"@en ;
    emmo:EMMO_fe015383_afb3_44a6_ae86_043628697aa2 "https://goldbook.iupac.org/terms/view/D01722"@en .

:electrochemistry_1a104474_c326_4a29_ac26_26a05ac8f72c a owl:Class ;
    rdfs:label "ResponseTimeAtAnISE"@en ;
    rdfs:comment "Buck and Lindner suggest a slope of 0.6 mV min-1 ."@en,
        "Duration between the time when an ion-selective electrode and an external reference electrode (the two completing the ion-selective electrode cell) are brought into contact with a sample solution (or the time at which the activity of the ion of interest in solution is changed) and the first time at which the slope of the cell potential vs. time plot (ΔE/Δt) becomes equal to a limiting value selected on the basis of the experimental conditions and/or requirements concerning accuracy."@en,
        "Previously defined response times t95 (corresponding to the 95% change of the potential span) and t* (to 1 mV from the steady value) require prior knowledge of steady-state E values that may not be available. These descriptive quantities underestimate practical response times of ion-selective electrodes in clinical applications where the total span may be narrower than 10 mV. The response time expressed in terms of ΔE/Δt (i.e., rate of cell potential variation with time) seems to be the best choice among non-ideal options. It can be related to t95 and t* through mathematical models, provided that the long-time potential- determining processes are identified."@en ;
    rdfs:subClassOf [ a owl:Restriction ;
            owl:onProperty emmo:EMMO_bed1d005_b04e_4a90_94cf_02bc678a8569 ;
            owl:someValuesFrom emmo:EMMO_02e894c3_b793_4197_b120_3442e08f58d1 ],
        :electrochemistry_aecc6094_c6a5_4a36_a825_8a497a2ae112 ;
    skos:prefLabel "ResponseTimeAtAnISE"@en ;
    emmo:EMMO_967080e5_2f42_4eb2_a3a9_c58143e835f9 "Duration between the time when an ion-selective electrode and an external reference electrode (the two completing the ion-selective electrode cell) are brought into contact with a sample solution (or the time at which the activity of the ion of interest in solution is changed) and the first time at which the slope of the cell potential vs. time plot (ΔE/Δt) becomes equal to a limiting value selected on the basis of the experimental conditions and/or requirements concerning accuracy."@en .

:electrochemistry_25e20915_c35d_4bee_ad31_736235a79780 a owl:Class ;
    rdfs:label "DischargingCRate"@en ;
    rdfs:comment "[an indicator of the] electric current at which a battery is discharged"@en,
        "the discharge rate is calculated as the rated capacity divided by the corresponding discharge time which results in an electric current"@en,
        "the quantity DRate is not used for energy-decoupled batteries like Redox Flox batteries"@en ;
    rdfs:seeAlso "CRate"@en ;
    rdfs:subClassOf emmo:EMMO_faab3f84_e475_4a46_af9c_7d249f0b9aef,
        :electrochemistry_e1fd84eb_acdb_4b2c_b90c_e899d552a3ee ;
    skos:altLabel "DRate"@en,
        "DischargeRate"@en ;
    skos:prefLabel "DischargingCRate"@en ;
    emmo:EMMO_50c298c2_55a2_4068_b3ac_4e948c33181f "https://www.electropedia.org/iev/iev.nsf/display?openform&ievref=482-03-25" ;
    emmo:EMMO_967080e5_2f42_4eb2_a3a9_c58143e835f9 "[an indicator of the] electric current at which a battery is discharged"@en .

:electrochemistry_33e6986c_b35a_4cae_9a94_acb23248065c a owl:Class ;
    rdfs:label "ControlProperty"@en ;
    rdfs:comment "a target quantity in a control system"@en ;
    rdfs:subClassOf emmo:EMMO_dd4a7f3e_ef56_466c_ac1a_d2716b5f87ec ;
    skos:altLabel "ControlledQuantity"@en,
        "SetQuantity"@en ;
    skos:prefLabel "ControlProperty"@en ;
    emmo:EMMO_967080e5_2f42_4eb2_a3a9_c58143e835f9 "a target quantity in a control system"@en .

:electrochemistry_38ab058e_3912_48c2_a7eb_76d25d000820 a owl:Class ;
    rdfs:label "StoichiometricCoefficientAtSOC100"@en ;
    rdfs:comment "the stoichiometric coefficient for a reactive entity in a chemical substance that corresponds to a cell-level state-of-charge of 100%"@en ;
    rdfs:subClassOf :electrochemistry_f0667139_6428_4e3d_ac0d_08c1dd7f36ea ;
    skos:prefLabel "StoichiometricCoefficientAtSOC100"@en ;
    emmo:EMMO_967080e5_2f42_4eb2_a3a9_c58143e835f9 "the stoichiometric coefficient for a reactive entity in a chemical substance that corresponds to a cell-level state-of-charge of 100%"@en .

:electrochemistry_3cd0e74e_292c_48ed_a831_4cb8753d9a56 a owl:Class ;
    rdfs:label "PulseDuration"@en ;
    rdfs:comment "The pulse duration includes the sampling interval."@en,
        "time interval during which the excitation signal deviates from the base line in normal pulse voltamme- try, differential pulse voltammetry, and related techniques"@en ;
    rdfs:subClassOf emmo:EMMO_0adabf6f_7404_44cb_9f65_32d83d8101a3,
        :electrochemistry_c5047d29_4e68_43ee_8355_3e8f05dc70a5 ;
    skos:prefLabel "PulseDuration"@en ;
    emmo:EMMO_967080e5_2f42_4eb2_a3a9_c58143e835f9 "time interval during which the excitation signal deviates from the base line in normal pulse voltamme- try, differential pulse voltammetry, and related techniques"@en ;
    emmo:EMMO_fe015383_afb3_44a6_ae86_043628697aa2 "https://doi.org/10.1351/goldbook.P04947"@en .

:electrochemistry_47287d09_6108_45ca_ac65_8b9451b1065e a owl:Class ;
    rdfs:label "MaximumConcentration"@en ;
    rdfs:comment "the maximum amount concentration of a species in a phase, either imposed or naturally occurring"@en ;
    rdfs:subClassOf :electrochemistry_5eae657f_5914_4252_85c6_3fc772dea113 ;
    skos:prefLabel "MaximumConcentration"@en ;
    emmo:EMMO_967080e5_2f42_4eb2_a3a9_c58143e835f9 "the maximum amount concentration of a species in a phase, either imposed or naturally occurring"@en .

:electrochemistry_4aa1b96e_44a0_4b1a_a0ac_723d0223d80b a owl:Class ;
    rdfs:label "EnergyDensity"@en ;
    rdfs:comment "the quotient of the energy of an energy-storage device or system and its volume"@en ;
    rdfs:subClassOf [ a owl:Restriction ;
            owl:onProperty emmo:EMMO_bed1d005_b04e_4a90_94cf_02bc678a8569 ;
            owl:someValuesFrom emmo:EMMO_53bd0c90_41c3_46e2_8779_cd2a80f7e18b ],
        emmo:EMMO_602397bd_e302_42a6_be33_fe67ea81933a,
        :electrochemistry_02eb0465_4f94_453c_8c1f_5ddf80134634 ;
    skos:altLabel "EnergyDensityOfStorage"@en,
        "VolumetricEnergyDensity"@en ;
    skos:prefLabel "EnergyDensity"@en ;
    emmo:EMMO_50c298c2_55a2_4068_b3ac_4e948c33181f "https://www.electropedia.org/iev/iev.nsf/display?openform&ievref=482-03-22" ;
    emmo:EMMO_967080e5_2f42_4eb2_a3a9_c58143e835f9 "the quotient of the energy of an energy-storage device or system and its volume"@en .

:electrochemistry_5eae657f_5914_4252_85c6_3fc772dea113 a owl:Class ;
    rdfs:label "ConcentrationLimit"@en ;
    rdfs:comment "limit on the amount concentration of a species in a phase, either imposed or naturally occurring"@en ;
    rdfs:subClassOf emmo:EMMO_d5be1faf_0c56_4f5a_9b78_581e6dee949f,
        :electrochemistry_b395a244_3a75_4737_be38_981bfa1277fe ;
    skos:prefLabel "ConcentrationLimit"@en ;
    emmo:EMMO_967080e5_2f42_4eb2_a3a9_c58143e835f9 "limit on the amount concentration of a species in a phase, either imposed or naturally occurring"@en .

:electrochemistry_5ebeea80_af22_456b_9087_78c2a8465c58 a owl:Class ;
    rdfs:label "VoltageLimit"@en ;
    rdfs:comment "limit on the voltage of an electrical system"@en ;
    rdfs:subClassOf emmo:EMMO_17b031fb_4695_49b6_bb69_189ec63df3ee,
        :electrochemistry_b395a244_3a75_4737_be38_981bfa1277fe ;
    skos:prefLabel "VoltageLimit"@en ;
    emmo:EMMO_967080e5_2f42_4eb2_a3a9_c58143e835f9 "limit on the voltage of an electrical system"@en ;
    emmo:EMMO_cc65321f_1964_4f16_aea3_2a8edf2f3394 emmo:Volt .

:electrochemistry_75c28dc8_3d7d_4b6e_861e_6c8b1ad7d644 a owl:Class ;
    rdfs:label "ShortCircuitCurrent"@en ;
    rdfs:comment "maximum current which should be delivered by a cell or battery into an external circuit with zero electric resistance, or an external circuit which depresses the cell or battery voltage to approximately zero volt"@en,
        "zero electric resistance is a hypothetical condition and in practice the short-circuit current is the peak current flowing in a circuit of very low resistance compared to the internal resistance of the battery"@en ;
    rdfs:subClassOf :electrochemistry_637ee9c4_4b3f_4d3a_975b_c0572dfe53ce ;
    skos:prefLabel "ShortCircuitCurrent"@en ;
    emmo:EMMO_50c298c2_55a2_4068_b3ac_4e948c33181f "https://www.electropedia.org/iev/iev.nsf/display?openform&ievref=482-03-26" ;
    emmo:EMMO_967080e5_2f42_4eb2_a3a9_c58143e835f9 "maximum current which should be delivered by a cell or battery into an external circuit with zero electric resistance, or an external circuit which depresses the cell or battery voltage to approximately zero volt"@en .

:electrochemistry_7fc10197_41d9_4c1e_a107_928f03eb2d36 a owl:Class ;
    rdfs:label "StandardElectrodePotential"@en ;
    rdfs:comment "E° is related to the standard Gibbs Energy of the electrode reaction, ΔrG° or ΔrG , written as a reduction with respect to that of the standard hydrogen electrode (SHE) E° = −ΔrG°/zF."@en,
        "The standard electrode potential of an electrochemical reaction is the standard potential of a hypothetical cell in which the electrode (half cell) at the left of the cell diagram is the standard hydrogen electrode (SHE) and the electrode at the right is the electrode in question. See also line representation of electrochemical cells."@en,
        "equilibrium electrode potential of an electrode under standard conditions"@en,
        "equilibrium electrode potential referenced to the standard hydrogen electrode."@en ;
    rdfs:subClassOf :electrochemistry_d91940f0_c8b6_4505_9b68_6bf6cfc5c544 ;
    skos:altLabel "StandardPotential"@en ;
    skos:prefLabel "StandardElectrodePotential"@en ;
    emmo:EMMO_50c298c2_55a2_4068_b3ac_4e948c33181f "https://www.electropedia.org/iev/iev.nsf/display?openform&ievref=114-02-13" ;
    emmo:EMMO_6dd685dd_1895_46e4_b227_be9f7d643c25 "https://dbpedia.org/page/Standard_electrode_potential" ;
    emmo:EMMO_967080e5_2f42_4eb2_a3a9_c58143e835f9 "equilibrium electrode potential of an electrode under standard conditions"@en ;
    emmo:EMMO_fe015383_afb3_44a6_ae86_043628697aa2 "https://goldbook.iupac.org/terms/view/S05912"@en .

:electrochemistry_82fce40c_434d_4640_a3d2_e26379b6acae a owl:Class ;
    rdfs:label "TemperatureLimit"@en ;
    rdfs:comment "limit on the temperature of a system"@en ;
    rdfs:subClassOf emmo:EMMO_66bc9029_f473_45ff_bab9_c3509ff37a22,
        :electrochemistry_b395a244_3a75_4737_be38_981bfa1277fe ;
    skos:prefLabel "TemperatureLimit"@en ;
    emmo:EMMO_967080e5_2f42_4eb2_a3a9_c58143e835f9 "limit on the temperature of a system"@en .

:electrochemistry_8abde9d0_84f6_4b4f_a87e_86028a397100 a owl:Class ;
    rdfs:label "NominalCapacity"@en ;
    rdfs:comment "the rated capacity that is representative of the typical value associated with a cell as stated by the manufacturer"@en ;
    rdfs:seeAlso :electrochemistry_a7a4614f_2426_46f3_8475_cda4a9fabfce,
        :electrochemistry_b7781ebc_90a7_4f19_997f_aed28dee1b01,
        :electrochemistry_d3c0078e_c1d3_461e_873d_e5c3adf441c5 ;
    rdfs:subClassOf :electrochemistry_9b3b4668_0795_4a35_9965_2af383497a26 ;
    skos:prefLabel "NominalCapacity"@en ;
    skos:scopeNote "The value for 'nominal capacity' is provided by manufacturers as an indication of the expected performance of the device under a set of defined nominal conditions. It serves as a benchmark for comparing different devices."@en ;
    emmo:EMMO_5f7abc2a_5b50_41c3_8def_c8ba7c3b083e "To ensure meaningful comparisons, nominal capacity values should always be evaluated under matching test conditions."@en ;
    emmo:EMMO_967080e5_2f42_4eb2_a3a9_c58143e835f9 "the rated capacity that is representative of the typical value associated with a cell as stated by the manufacturer"@en ;
    emmo:EMMO_b6730304_cabc_4104_b415_14218466445c "While nominal capacity provides a useful reference, actual capacity depends on various factors, including temperature, rate, and state-of-health."@en ;
    emmo:EMMO_cc65321f_1964_4f16_aea3_2a8edf2f3394 emmo:AmpereHour,
        emmo:MilliAmpereHour .

:electrochemistry_9ed7210c_c4fa_467b_822d_ba12f885bdf4 a owl:Class ;
    rdfs:label "ConcentrationOverpotential"@en ;
    rdfs:comment "The concentration overpotential of an electrode reaction at a given electrode current density (c.d.) is basically the difference in equilibrium potentials across the diffusion layer. More precisely, it is the potential of a reference electrode (of the same electrode reaction as the working electrode ) with the interfacial concentrations which establish themselves at c.d., relative to the potential of a similar reference electrode with the concentrations of the bulk solution. From such a measured potential difference, with c.d. flowing, one needs to subtract the ohmic potential drop prevailing between the two electrodes."@en,
        "part of the electrode polarization arising from concentration gradients of electrode reactants and products."@en ;
    rdfs:subClassOf :electrochemistry_1cd1d777_e67b_47eb_81f1_edac35d9f2c6 ;
    skos:altLabel "ConcentrationPolarization"@en,
        "MassTransferOverpotential"@en,
        "MassTransferPolarization"@en ;
    skos:prefLabel "ConcentrationOverpotential"@en ;
    emmo:EMMO_50c298c2_55a2_4068_b3ac_4e948c33181f "https://www.electropedia.org/iev/iev.nsf/display?openform&ievref=482-03-08"@en ;
    emmo:EMMO_967080e5_2f42_4eb2_a3a9_c58143e835f9 "The concentration overpotential of an electrode reaction at a given electrode current density (c.d.) is basically the difference in equilibrium potentials across the diffusion layer. More precisely, it is the potential of a reference electrode (of the same electrode reaction as the working electrode ) with the interfacial concentrations which establish themselves at c.d., relative to the potential of a similar reference electrode with the concentrations of the bulk solution. From such a measured potential difference, with c.d. flowing, one needs to subtract the ohmic potential drop prevailing between the two electrodes."@en ;
    emmo:EMMO_c84c6752_6d64_48cc_9500_e54a3c34898d "https://en.wikipedia.org/wiki/Overpotential#Concentration_overpotential"@en ;
    emmo:EMMO_fe015383_afb3_44a6_ae86_043628697aa2 "https://goldbook.iupac.org/terms/view/C01230" .

:electrochemistry_a24f8581_a5a4_41a4_bb45_d0fdd5c0d810 a owl:Class ;
    rdfs:label "InstantaneousCurrent"@en ;
    rdfs:comment "I_{t}"@en,
        "The instantaneous current is usually time-dependent and may have the character of an adsorption current, catalytic current, diffusion current, double-layer current, or kinetic current, and may include a migration current. A plot of the dependence of instantaneous current on time is commonly called an “I-t curve”."@en,
        "value of an electric current at an instant in time"@en ;
    rdfs:subClassOf emmo:EMMO_c995ae70_3b84_4ebb_bcfc_69e6a281bb88,
        :electrochemistry_aecc6094_c6a5_4a36_a825_8a497a2ae112 ;
    skos:prefLabel "InstantaneousCurrent"@en ;
    emmo:EMMO_26bf1bef_d192_4da6_b0eb_d2209698fb54 "https://www.wikidata.org/wiki/Q108057717" ;
    emmo:EMMO_967080e5_2f42_4eb2_a3a9_c58143e835f9 "value of an electric current at an instant in time"@en ;
    emmo:EMMO_fe015383_afb3_44a6_ae86_043628697aa2 "https://goldbook.iupac.org/terms/view/I03062"@en .

:electrochemistry_a4dfa5c1_55a9_4285_b71d_90cf6613ca31 a owl:Class ;
    rdfs:label "ChargeTransferCoefficient"@en ;
    rdfs:comment "The cathodic transfer coefficient αc is defined as –(RT/nF)(dlnkc /dE), where kc is the electroreduction rate constant, E is the applied potential, and R, T, and F have their usual significance. This definition is equivalent to the other, -(RT/nF)(dln|jc |/dE), where jc is the cathodic current density corrected for any changes in the reactant concentration at the electrode surface with respect to its bulk value."@en,
        "the fraction of the electrostatic potential energy affecting the reduction rate in an electrode reaction, with the remaining fraction affecting the corresponding oxidation rate"@en ;
    rdfs:subClassOf emmo:EMMO_faab3f84_e475_4a46_af9c_7d249f0b9aef,
        :electrochemistry_21745019_2830_4395_bca7_15ddfd266673 ;
    skos:prefLabel "ChargeTransferCoefficient"@en ;
    emmo:EMMO_967080e5_2f42_4eb2_a3a9_c58143e835f9 "the fraction of the electrostatic potential energy affecting the reduction rate in an electrode reaction, with the remaining fraction affecting the corresponding oxidation rate"@en ;
    emmo:EMMO_c84c6752_6d64_48cc_9500_e54a3c34898d "https://en.wikipedia.org/wiki/Charge_transfer_coefficient" .

:electrochemistry_a5571263_f153_448f_84a3_cd18092cf8fa a owl:Class ;
    rdfs:label "VolumetricSurfaceArea"@en ;
    rdfs:comment "ratio of the surface area of a solid object to the volume of the object"@en ;
    rdfs:subClassOf :electrochemistry_aecc6094_c6a5_4a36_a825_8a497a2ae112 ;
    skos:altLabel "SurfaceAreaToVolumeRatio"@en ;
    skos:prefLabel "VolumetricSurfaceArea"@en ;
    emmo:EMMO_26bf1bef_d192_4da6_b0eb_d2209698fb54 "https://www.wikidata.org/wiki/Q766786" ;
    emmo:EMMO_967080e5_2f42_4eb2_a3a9_c58143e835f9 "ratio of the surface area of a solid object to the volume of the object"@en ;
    emmo:EMMO_c84c6752_6d64_48cc_9500_e54a3c34898d "https://en.wikipedia.org/wiki/Surface-area-to-volume_ratio"@en .

:electrochemistry_a7dc73e2_d4aa_4dfc_8b4d_cb611f1501fb a owl:Class ;
    rdfs:label "ChargingCRate"@en ;
    rdfs:comment "[an indicator of the] electric current at which a secondary cell or battery is charged"@en ;
    rdfs:subClassOf :electrochemistry_e1fd84eb_acdb_4b2c_b90c_e899d552a3ee ;
    skos:prefLabel "ChargingCRate"@en ;
    emmo:EMMO_50c298c2_55a2_4068_b3ac_4e948c33181f "https://www.electropedia.org/iev/iev.nsf/display?openform&ievref=482-05-45"@en ;
    emmo:EMMO_967080e5_2f42_4eb2_a3a9_c58143e835f9 "[an indicator of the] electric current at which a secondary cell or battery is charged"@en ;
    emmo:EMMO_c7b62dd7_063a_4c2a_8504_42f7264ba83f "the charge rate is expressed as the reference current It = Cr/n where Cr is the rated capacity declared by the manufacturer and n is the time base in hours for which the rated capacity is declared"@en .

:electrochemistry_b7781ebc_90a7_4f19_997f_aed28dee1b01 a owl:Class ;
    rdfs:label "MaximumCapacity"@en ;
    rdfs:comment "the maximum amount of electric charge that can be reversible stored within an electrochemical device"@en ;
    rdfs:seeAlso :electrochemistry_8abde9d0_84f6_4b4f_a87e_86028a397100,
        :electrochemistry_a7a4614f_2426_46f3_8475_cda4a9fabfce,
        :electrochemistry_d3c0078e_c1d3_461e_873d_e5c3adf441c5 ;
    rdfs:subClassOf :electrochemistry_9b3b4668_0795_4a35_9965_2af383497a26,
        :electrochemistry_aecc6094_c6a5_4a36_a825_8a497a2ae112 ;
    skos:altLabel "MaximumStorageCapacity"@en ;
    skos:prefLabel "MaximumCapacity"@en ;
    skos:scopeNote "Manufacturers define the value for 'maximum capacity' as the upper performance limit that a device in a batch will typically achieve. The maximum capacity is larger than the nominal capacity, and acts as an indicator of the spread in performacne in a given batch of devices."@en ;
    emmo:EMMO_967080e5_2f42_4eb2_a3a9_c58143e835f9 "the maximum amount of electric charge that can be reversible stored within an electrochemical device"@en ;
    emmo:EMMO_b6730304_cabc_4104_b415_14218466445c "For real applications, the maximum capacity is affected by environmental conditions, rate of operation, and state-of-heath and can deviate from the reported value."@en ;
    emmo:EMMO_cc65321f_1964_4f16_aea3_2a8edf2f3394 emmo:AmpereHour,
        emmo:MilliAmpereHour .

:electrochemistry_b92e382f_5109_4f60_ab5e_c89d340419a9 a owl:Class ;
    rdfs:label "ParticleRadius"@en ;
    rdfs:comment "radius of a particle"@en ;
    rdfs:subClassOf emmo:EMMO_32dcd601_47c7_4028_b7fa_5e972ae57f12,
        :electrochemistry_aecc6094_c6a5_4a36_a825_8a497a2ae112 ;
    skos:prefLabel "ParticleRadius"@en ;
    emmo:EMMO_967080e5_2f42_4eb2_a3a9_c58143e835f9 "radius of a particle"@en .

:electrochemistry_c4120ce7_f1ff_4917_b59e_002454a65040 a owl:Class ;
    rdfs:label "PRate"@en ;
    rdfs:comment "an indicator of the electric power at which an electrochemical device is operated"@en ;
    rdfs:subClassOf emmo:EMMO_faab3f84_e475_4a46_af9c_7d249f0b9aef,
        :electrochemistry_aecc6094_c6a5_4a36_a825_8a497a2ae112 ;
    skos:prefLabel "PRate"@en ;
    emmo:EMMO_967080e5_2f42_4eb2_a3a9_c58143e835f9 "an indicator of the electric power at which an electrochemical device is operated"@en .

:electrochemistry_c7b26177_21bf_4787_b656_8e78edf27f88 a owl:Class ;
    rdfs:label "DischargingVoltage"@en ;
    dcterms:source "https://www.electropedia.org/iev/iev.nsf/display?openform&ievref=482-03-28"@en ;
    rdfs:comment "voltage between the terminals of a cell or battery when being discharged"@en ;
    rdfs:subClassOf :electrochemistry_4ebe2ef1_eea8_4b10_822d_7a68215bd24d ;
    skos:altLabel "DischargeVoltage",
        "ClosedCircuitVoltage"@en ;
    skos:prefLabel "DischargingVoltage"@en ;
    emmo:EMMO_967080e5_2f42_4eb2_a3a9_c58143e835f9 "voltage between the terminals of a cell or battery when being discharged"@en .

:electrochemistry_cf386c1e_e62b_43ef_9b0e_e5e58935d63f a owl:Class ;
    rdfs:label "PercentQuantity"@en ;
    rdfs:comment "a quantity that is expressed as a percentage"@en ;
    rdfs:subClassOf [ a owl:Restriction ;
            owl:onProperty emmo:EMMO_67fc0a36_8dcb_4ffa_9a43_31074efa3296 ;
            owl:someValuesFrom :electrochemistry_8430be19_6cae_4a15_a570_3c15d0d190eb ],
        emmo:EMMO_faab3f84_e475_4a46_af9c_7d249f0b9aef ;
    skos:prefLabel "PercentQuantity"@en ;
    emmo:EMMO_967080e5_2f42_4eb2_a3a9_c58143e835f9 "a quantity that is expressed as a percentage"@en .

:electrochemistry_d3c0078e_c1d3_461e_873d_e5c3adf441c5 a owl:Class ;
    rdfs:label "MinimumCapacity"@en ;
    rdfs:comment "the minimum acceptable threshold value for the rated capacity of an electrochemical device, as stated by the manufacturer."@en ;
    rdfs:seeAlso :electrochemistry_8abde9d0_84f6_4b4f_a87e_86028a397100,
        :electrochemistry_a7a4614f_2426_46f3_8475_cda4a9fabfce,
        :electrochemistry_b7781ebc_90a7_4f19_997f_aed28dee1b01 ;
    rdfs:subClassOf :electrochemistry_9b3b4668_0795_4a35_9965_2af383497a26 ;
    skos:altLabel "MiniumumAcceptedCapacity"@en ;
    skos:prefLabel "MinimumCapacity"@en ;
    skos:scopeNote "Manufacturers define the value for 'minimum capacity' as the lower performance limit, ensuring that every device meets a minimum standard. In practice, minimum capacity is often about 95-97% of the nominal capacity, acting as a guaranteed lower bound rather than an exact measurement."@en ;
    emmo:EMMO_967080e5_2f42_4eb2_a3a9_c58143e835f9 "the minimum acceptable threshold value for the rated capacity of an electrochemical device, as stated by the manufacturer."@en ;
    emmo:EMMO_b6730304_cabc_4104_b415_14218466445c "For real applications, the achieveable minimum capacity is affected by environmental conditions, rate of operation, and state-of-heath and can deviate from the reported value."@en ;
    emmo:EMMO_cc65321f_1964_4f16_aea3_2a8edf2f3394 emmo:AmpereHour,
        emmo:MilliAmpereHour .

:electrochemistry_e4d666ee_d637_45cd_a904_dc33941ead4f a owl:Class ;
    rdfs:label "DischargingCurrent"@en ;
    rdfs:comment "electric current delivered by a battery during its discharge"@en ;
    rdfs:subClassOf :electrochemistry_637ee9c4_4b3f_4d3a_975b_c0572dfe53ce,
        :electrochemistry_aecc6094_c6a5_4a36_a825_8a497a2ae112 ;
    skos:prefLabel "DischargingCurrent"@en ;
    emmo:EMMO_50c298c2_55a2_4068_b3ac_4e948c33181f "https://www.electropedia.org/iev/iev.nsf/display?openform&ievref=482-03-24"@en ;
    emmo:EMMO_967080e5_2f42_4eb2_a3a9_c58143e835f9 "electric current delivered by a battery during its discharge"@en .

:electrochemistry_f22bd1ec_faca_4335_92a5_a1687154c622 a owl:Class ;
    rdfs:label "StoichiometricCoefficientAtSOC0"@en ;
    rdfs:comment "the stoichiometric coefficient for a reactive entity in a chemical substance that corresponds to a cell-level state-of-charge of 0%"@en ;
    rdfs:subClassOf :electrochemistry_f0667139_6428_4e3d_ac0d_08c1dd7f36ea ;
    skos:prefLabel "StoichiometricCoefficientAtSOC0"@en ;
    emmo:EMMO_967080e5_2f42_4eb2_a3a9_c58143e835f9 "the stoichiometric coefficient for a reactive entity in a chemical substance that corresponds to a cell-level state-of-charge of 0%"@en .

:electrochemistry_f94678d6_1386_48fc_8e54_024921924401 a owl:Class ;
    rdfs:label "InternalApparentResistance"@en ;
    rdfs:comment "internal apparent resistance is expressed in ohms"@en,
        "quotient of change of voltage of a battery by the corresponding change in discharge current under specified conditions."@en ;
    rdfs:subClassOf :electrochemistry_9bf40017_3f58_4030_ada7_cb37a3dfda2d ;
    skos:prefLabel "InternalApparentResistance"@en ;
    emmo:EMMO_50c298c2_55a2_4068_b3ac_4e948c33181f "https://www.electropedia.org/iev/iev.nsf/display?openform&ievref=482-03-36" ;
    emmo:EMMO_967080e5_2f42_4eb2_a3a9_c58143e835f9 "quotient of change of voltage of a battery by the corresponding change in discharge current under specified conditions."@en .

:electrochemistry_1e3dc60d_dd6b_47d6_8161_70004fc5ee30 a owl:Class ;
    rdfs:label "SpecificCapacity"@en ;
    rdfs:comment "Can also be applied to electrodes."@en,
        "quotient of the capacity of a cell or battery [ or electrode or active material ] by its mass."@en ;
    rdfs:subClassOf [ a owl:Restriction ;
            owl:onProperty emmo:EMMO_bed1d005_b04e_4a90_94cf_02bc678a8569 ;
            owl:someValuesFrom emmo:EMMO_4dbe2b16_3e84_4049_898d_eb89bcc925a2 ],
        emmo:EMMO_2946d40b_24a1_47fa_8176_e3f79bb45064,
        :electrochemistry_02eb0465_4f94_453c_8c1f_5ddf80134634 ;
    skos:altLabel "GravimetricCapacity"@en,
        "SpecificChargeCapacity"@en,
        "SpecificElectricChargeCapacity"@en ;
    skos:prefLabel "SpecificCapacity"@en ;
    emmo:EMMO_50c298c2_55a2_4068_b3ac_4e948c33181f "https://www.electropedia.org/iev/iev.nsf/display?openform&ievref=482-03-19" ;
    emmo:EMMO_967080e5_2f42_4eb2_a3a9_c58143e835f9 "quotient of the capacity of a cell or battery [ or electrode or active material ] by its mass."@en ;
    :electrochemistry_811aafc3_0c6d_470e_b67e_ff5c82992609 "Capacity Density(mAh/g)"@en .

:electrochemistry_3b938708_e7e4_4ac0_a959_9c04306302e7 a owl:Class ;
    rdfs:label "CoatingThickness"@en ;
    rdfs:comment "thickness of the coating before any additional treatment is applied"@en ;
    rdfs:subClassOf emmo:EMMO_43003c86_9d15_433b_9789_ee2940920656,
        :electrochemistry_aecc6094_c6a5_4a36_a825_8a497a2ae112 ;
    skos:prefLabel "CoatingThickness"@en ;
    emmo:EMMO_967080e5_2f42_4eb2_a3a9_c58143e835f9 "thickness of the coating before any additional treatment is applied"@en .

:electrochemistry_3bb5ae23_59fa_4bc7_9495_803eb6719f28 a owl:Class ;
    rdfs:label "TemperatureCoefficientOfTheOpenCircuitVoltage"@en ;
    rdfs:comment "quotient of change in open-circuit voltage of a cell or battery by the corresponding change in temperature."@en ;
    rdfs:subClassOf :electrochemistry_aecc6094_c6a5_4a36_a825_8a497a2ae112 ;
    skos:prefLabel "TemperatureCoefficientOfTheOpenCircuitVoltage"@en ;
    emmo:EMMO_50c298c2_55a2_4068_b3ac_4e948c33181f "https://www.electropedia.org/iev/iev.nsf/display?openform&ievref=482-03-33" ;
    emmo:EMMO_967080e5_2f42_4eb2_a3a9_c58143e835f9 "quotient of change in open-circuit voltage of a cell or battery by the corresponding change in temperature."@en .

:electrochemistry_4747c51d_86ab_4684_a4fb_b05f5c405ea3 a owl:Class ;
    rdfs:label "MiniumumTemperature"@en ;
    rdfs:comment "the minimum allowable temperature"@en ;
    rdfs:subClassOf :electrochemistry_82fce40c_434d_4640_a3d2_e26379b6acae ;
    skos:prefLabel "MiniumumTemperature"@en ;
    emmo:EMMO_967080e5_2f42_4eb2_a3a9_c58143e835f9 "the minimum allowable temperature"@en ;
    :electrochemistry_811aafc3_0c6d_470e_b67e_ff5c82992609 "Min-T(C)"@en .

:electrochemistry_47608fd0_cc0d_457e_9141_051935029e3a a owl:Class ;
    rdfs:label "NumberOfFiniteVolumeCells"@en ;
    rdfs:comment "number of discrete finite volume cells in a grid or sub-grid"@en ;
    rdfs:subClassOf emmo:EMMO_41efdf5d_0c9c_4ea0_bb65_f8236e663be5 ;
    skos:prefLabel "NumberOfFiniteVolumeCells"@en ;
    emmo:EMMO_967080e5_2f42_4eb2_a3a9_c58143e835f9 "number of discrete finite volume cells in a grid or sub-grid"@en .

:electrochemistry_67930f7b_ad4c_4b21_9b2e_a000e5c153ae a owl:Class ;
    rdfs:label "CRateUnit"@en ;
    rdfs:comment "the class of units for describing the C-Rate in electrochemistry and related domains"@en ;
    rdfs:subClassOf [ a owl:Restriction ;
            owl:hasValue "T-1 L0 M0 I0 Θ0 N0 J0" ;
            owl:onProperty emmo:EMMO_19d925d0_2cf1_40e5_a391_1a99d68409c9 ],
        emmo:EMMO_9895a1b4_f0a5_4167_ac5e_97db40b8bfcc ;
    skos:prefLabel "CRateUnit"@en ;
    emmo:EMMO_967080e5_2f42_4eb2_a3a9_c58143e835f9 "the class of units for describing the C-Rate in electrochemistry and related domains"@en .

:electrochemistry_c955c089_6ee1_41a2_95fc_d534c5cfd3d5 a owl:Class ;
    rdfs:label "MassLoading"@en ;
    rdfs:comment "mass of a material per unit area"@en ;
    rdfs:subClassOf emmo:EMMO_afea89af_ef16_4bdb_99d5_f3b2f4c85a6c,
        :electrochemistry_aecc6094_c6a5_4a36_a825_8a497a2ae112 ;
    skos:prefLabel "MassLoading"@en ;
    emmo:EMMO_967080e5_2f42_4eb2_a3a9_c58143e835f9 "mass of a material per unit area"@en .

:electrochemistry_cc519a19_b8d5_4e3f_b893_3a884888ad79 a owl:Class ;
    rdfs:label "MaximumTemperature"@en ;
    rdfs:comment "the maximum allowable temperature"@en ;
    rdfs:subClassOf :electrochemistry_82fce40c_434d_4640_a3d2_e26379b6acae ;
    skos:prefLabel "MaximumTemperature"@en ;
    emmo:EMMO_967080e5_2f42_4eb2_a3a9_c58143e835f9 "the maximum allowable temperature"@en ;
    :electrochemistry_811aafc3_0c6d_470e_b67e_ff5c82992609 "Max-T(C)"@en .

:electrochemistry_ce74d2dc_d496_4116_b2fb_3e83d88bc744 a owl:Class ;
    rdfs:label "ElectronicConductivity"@en ;
    rdfs:comment "measure of a substance's tendency towards electronic conduction"@en ;
    rdfs:subClassOf emmo:EMMO_cde4368c_1d4d_4c94_8548_604749523c6d,
        :electrochemistry_aecc6094_c6a5_4a36_a825_8a497a2ae112 ;
    skos:prefLabel "ElectronicConductivity"@en ;
    emmo:EMMO_967080e5_2f42_4eb2_a3a9_c58143e835f9 "measure of a substance's tendency towards electronic conduction"@en .

:electrochemistry_f509645f_eb27_470e_9112_7ab828ed40d3 a owl:Class ;
    rdfs:label "ElectrodePotential"@en ;
    rdfs:comment "E, U"@en,
        "The absolute value of the electrode potential cannot be measured, so E is always reported relative to the potential of a reference electrode, e.g. that of a standard hydrogen electrode (SHE)."@en,
        "cell source voltage when the electrodes of the electrochemical cell are a reference electrode and the electrode in question."@en,
        "electric potential at an electrode, reported as the difference in potential relative to a reference electrode"@en ;
    rdfs:subClassOf emmo:EMMO_4f2d3939_91b1_4001_b8ab_7d19074bf845,
        :electrochemistry_aecc6094_c6a5_4a36_a825_8a497a2ae112 ;
    skos:prefLabel "ElectrodePotential"@en ;
    emmo:EMMO_50c298c2_55a2_4068_b3ac_4e948c33181f "https://www.electropedia.org/iev/iev.nsf/display?openform&ievref=114-02-11" ;
    emmo:EMMO_967080e5_2f42_4eb2_a3a9_c58143e835f9 "electric potential at an electrode, reported as the difference in potential relative to a reference electrode"@en ;
    emmo:EMMO_c84c6752_6d64_48cc_9500_e54a3c34898d "https://en.wikipedia.org/wiki/Electrode_potential" ;
    emmo:EMMO_fe015383_afb3_44a6_ae86_043628697aa2 "https://goldbook.iupac.org/terms/view/E01956" .

emmo:EMMO_17b031fb_4695_49b6_bb69_189ec63df3ee skos:scopeNote "Voltage represents the difference in electric potential between two points in an electric circuit. In electrochemistry, it refers to the potential difference between the electrodes of a battery or electrochemical cell. Voltage influences the driving force of redox reactions and determines energy output in batteries, fuel cells, and electrolysis processes. It is commonly measured in volts (V)."@en ;
    emmo:EMMO_b6730304_cabc_4104_b415_14218466445c "Voltage is often used interchangeably with electric potential, but technically, voltage refers to a potential difference between two points."@en .

:electrochemistry_37b24a94_cae0_4d7a_9519_9f7692dec607 a owl:Class ;
    rdfs:label "Diffusivity"@en ;
    rdfs:comment "a measure of the rate at which particles or heat or fluids spread"@en,
        "not to be confused with MassDiffusivity (i.e., DiffusionCoefficient)"@en ;
    rdfs:subClassOf emmo:EMMO_2946d40b_24a1_47fa_8176_e3f79bb45064 ;
    skos:prefLabel "Diffusivity"@en ;
    emmo:EMMO_967080e5_2f42_4eb2_a3a9_c58143e835f9 "a measure of the rate at which particles or heat or fluids spread"@en .

:electrochemistry_46376e5d_9627_4514_9881_9e62083625c3 a owl:Class ;
    rdfs:label "StoredEnergy"@en ;
    rdfs:comment "amount of energy that is passed to or from an energy storage device under specified conditions"@en ;
    rdfs:subClassOf emmo:EMMO_31ec09ba_1713_42cb_83c7_b38bf6f9ced2,
        :electrochemistry_02eb0465_4f94_453c_8c1f_5ddf80134634 ;
    skos:altLabel "BatteryEnergy"@en,
        "EnergyStorageCapability"@en ;
    skos:hiddenLabel "Energy/mWh"@en,
        "Watt-hr"@en,
        "mWatt-hr"@en ;
    skos:prefLabel "StoredEnergy"@en ;
    emmo:EMMO_50c298c2_55a2_4068_b3ac_4e948c33181f "https://www.electropedia.org/iev/iev.nsf/display?openform&ievref=482-03-21"@en ;
    emmo:EMMO_967080e5_2f42_4eb2_a3a9_c58143e835f9 "amount of energy that is passed to or from an energy storage device under specified conditions"@en ;
    :electrochemistry_097ea615_c209_4edd_a1a1_5eea71d98fe8 "watt-hr"@en ;
    :electrochemistry_811aafc3_0c6d_470e_b67e_ff5c82992609 "Energy(mWh)"@en ;
    :electrochemistry_8377c1f7_2b09_4632_9a4d_bb318438adbb "cell_energy_j"@en ;
    :electrochemistry_ea9f4dba_8ca2_419e_9cdf_ce54e9ebbd46 "Energy (Wh)"@en .

:electrochemistry_47ab1dad_cc09_4fd8_af23_acb36fb680dd a owl:Class ;
    rdfs:label "ElectrodeSurfaceArea"@en ;
    rdfs:comment "A"@en,
        "The geometric area, A_{geom} , is the interfacial area, determined on the assumption that the interface is truly flat (2-dimensional) and calculated using the geometric data of the involved surfaces. The real (true) area, A_{real}, takes into account non-idealities of the interface (roughness, porosity, etc.) and can be measured by a variety of electrochemical methods. The electroactive area is the area calculated from experiments with model electroactive species and may be different from the real surface area in cases where not all of the surface is electrochemically active or accessible."@en,
        "area of electrode - solution interface."@en ;
    rdfs:subClassOf :electrochemistry_05cf26ef_782a_4f66_a196_7004dd973f8e,
        :electrochemistry_aecc6094_c6a5_4a36_a825_8a497a2ae112 ;
    skos:prefLabel "ElectrodeSurfaceArea"@en ;
    emmo:EMMO_967080e5_2f42_4eb2_a3a9_c58143e835f9 "area of electrode - solution interface."@en .

:electrochemistry_4a450a27_b84a_4c70_a3a9_15ec30e2f30b a owl:Class ;
    rdfs:label "ElectrochemicalTransportQuantity"@en ;
    rdfs:comment "an electrochemical quantity related to the transport of mass, charge, or energy."@en ;
    rdfs:subClassOf :electrochemistry_aecc6094_c6a5_4a36_a825_8a497a2ae112 ;
    skos:prefLabel "ElectrochemicalTransportQuantity"@en ;
    emmo:EMMO_967080e5_2f42_4eb2_a3a9_c58143e835f9 "an electrochemical quantity related to the transport of mass, charge, or energy."@en .

:electrochemistry_637ee9c4_4b3f_4d3a_975b_c0572dfe53ce a owl:Class ;
    rdfs:label "CellCurrent"@en ;
    rdfs:comment "electric current flowing to or from an electrochemical cell or device"@en ;
    rdfs:subClassOf :electrochemistry_a24f8581_a5a4_41a4_bb45_d0fdd5c0d810 ;
    skos:hiddenLabel "<I>/mA"@en,
        "Amps"@en,
        "Current/mA"@en,
        "mAmps"@en ;
    skos:prefLabel "CellCurrent"@en ;
    emmo:EMMO_967080e5_2f42_4eb2_a3a9_c58143e835f9 "electric current flowing to or from an electrochemical cell or device"@en ;
    :electrochemistry_097ea615_c209_4edd_a1a1_5eea71d98fe8 "amps"@en ;
    :electrochemistry_1b717a20_17e3_4480_8c60_c4ae94058f05 "Current (A)"@en ;
    :electrochemistry_69022178_77b8_4669_97e2_351d45356e5a "I/mA"@en ;
    :electrochemistry_811aafc3_0c6d_470e_b67e_ff5c82992609 "Current(mA)"@en ;
    :electrochemistry_8377c1f7_2b09_4632_9a4d_bb318438adbb "cell_current_a"@en ;
    :electrochemistry_a07dd85b_d0df_4d5d_8b0c_14d20ea3fe45 "current"@en ;
    :electrochemistry_ea9f4dba_8ca2_419e_9cdf_ce54e9ebbd46 "Current (A)"@en .

:electrochemistry_900e357f_2ee3_425a_a0b6_322661117787 a owl:Class ;
    rdfs:label "ElectrochemicalProperty"@en ;
    rdfs:comment "a property that is typical in the electrochemistry domain"@en ;
    rdfs:subClassOf emmo:EMMO_909415d1_7c43_4d5e_bbeb_7e1910159f66 ;
    skos:prefLabel "ElectrochemicalProperty"@en ;
    emmo:EMMO_967080e5_2f42_4eb2_a3a9_c58143e835f9 "a property that is typical in the electrochemistry domain"@en .

:electrochemistry_a7a4614f_2426_46f3_8475_cda4a9fabfce a owl:Class ;
    rdfs:label "StateOfHealth"@en ;
    rdfs:comment "An indication of the health of an electrochemical device"@en ;
    rdfs:subClassOf :electrochemistry_aecc6094_c6a5_4a36_a825_8a497a2ae112 ;
    skos:prefLabel "StateOfHealth"@en ;
    emmo:EMMO_967080e5_2f42_4eb2_a3a9_c58143e835f9 "An indication of the health of an electrochemical device"@en .

:electrochemistry_f0667139_6428_4e3d_ac0d_08c1dd7f36ea a owl:Class ;
    rdfs:label "StoichiometricCoefficient"@en ;
    rdfs:comment "the absolute value of the stoichiometric number"@en ;
    rdfs:subClassOf emmo:EMMO_ba882f34_0d71_4e4f_9d92_0c076c633a2c ;
    skos:prefLabel "StoichiometricCoefficient"@en ;
    emmo:EMMO_26bf1bef_d192_4da6_b0eb_d2209698fb54 "https://www.wikidata.org/wiki/Q118455387"@en ;
    emmo:EMMO_967080e5_2f42_4eb2_a3a9_c58143e835f9 "the absolute value of the stoichiometric number"@en ;
    emmo:EMMO_c84c6752_6d64_48cc_9500_e54a3c34898d "https://en.wikipedia.org/wiki/Stoichiometry#Stoichiometric_coefficient_and_stoichiometric_number"@en .

:electrochemistry_f4fadc4e_ca7d_4e4e_89cf_eacf45b4041e a owl:Class ;
    rdfs:label "ReactionOverpotential"@en ;
    rdfs:comment "part of the electrode polarization arising from a chemical reaction impeding the electrode reaction"@en ;
    rdfs:subClassOf :electrochemistry_1cd1d777_e67b_47eb_81f1_edac35d9f2c6 ;
    skos:altLabel "ReactionOvervoltage"@en,
        "ReactionPolarization"@en ;
    skos:prefLabel "ReactionOverpotential"@en ;
    emmo:EMMO_50c298c2_55a2_4068_b3ac_4e948c33181f "https://www.electropedia.org/iev/iev.nsf/display?openform&ievref=482-03-10"@en ;
    emmo:EMMO_967080e5_2f42_4eb2_a3a9_c58143e835f9 "part of the electrode polarization arising from a chemical reaction impeding the electrode reaction"@en .

foaf:Person a owl:Class ;
    rdfs:label "Person"@en ;
    skos:prefLabel "Person"@en .

:electrochemistry_b395a244_3a75_4737_be38_981bfa1277fe a owl:Class ;
    rdfs:label "LimitQuantity"@en ;
    rdfs:comment "a limit quantity in a control system"@en ;
    rdfs:subClassOf :electrochemistry_c5047d29_4e68_43ee_8355_3e8f05dc70a5 ;
    skos:prefLabel "LimitQuantity"@en ;
    emmo:EMMO_967080e5_2f42_4eb2_a3a9_c58143e835f9 "a limit quantity in a control system"@en .

:electrochemistry_d91940f0_c8b6_4505_9b68_6bf6cfc5c544 a owl:Class ;
    rdfs:label "EquilibriumElectrodePotential"@en ;
    rdfs:comment "Eeq is related to the standard electrode potential by the Nernst equation."@en,
        "Temperature and activities of relevant species must be specified."@en,
        "electrode potential when the electrode reaction is in equilibrium."@en,
        "potential of an electrode when no electric current flows through the cell and all local charge transfer equilibria across phase boundaries that are represented in the cell diagram (except at possible electrolyte-electrolyte junctions) and local chemical equilibria are established"@en ;
    rdfs:subClassOf :electrochemistry_9c657fdc_b9d3_4964_907c_f9a6e8c5f52b,
        :electrochemistry_f509645f_eb27_470e_9112_7ab828ed40d3 ;
    skos:altLabel "EquilibriumPotential"@en,
        "NernstPotential"@en,
        "ReversiblePotential"@en ;
    skos:prefLabel "EquilibriumElectrodePotential"@en ;
    emmo:EMMO_50c298c2_55a2_4068_b3ac_4e948c33181f "https://www.electropedia.org/iev/iev.nsf/display?openform&ievref=114-02-12" ;
    emmo:EMMO_967080e5_2f42_4eb2_a3a9_c58143e835f9 "potential of an electrode when no electric current flows through the cell and all local charge transfer equilibria across phase boundaries that are represented in the cell diagram (except at possible electrolyte-electrolyte junctions) and local chemical equilibria are established"@en ;
    emmo:EMMO_c84c6752_6d64_48cc_9500_e54a3c34898d "https://en.wikipedia.org/wiki/Reversal_potential"@en .

:electrochemistry_e1fd84eb_acdb_4b2c_b90c_e899d552a3ee a owl:Class ;
    rdfs:label "CRate"@en ;
    rdfs:comment "[an indicator of the] electric current at which a secondary cell or battery is charged"@en,
        "the quantity CRate is not used for energy-decoupled batteries like Redox Flox batteries"@en ;
    rdfs:subClassOf [ a owl:Restriction ;
            owl:onProperty emmo:EMMO_bed1d005_b04e_4a90_94cf_02bc678a8569 ;
            owl:someValuesFrom :electrochemistry_67930f7b_ad4c_4b21_9b2e_a000e5c153ae ],
        emmo:EMMO_faab3f84_e475_4a46_af9c_7d249f0b9aef,
        :electrochemistry_aecc6094_c6a5_4a36_a825_8a497a2ae112 ;
    skos:altLabel "CapacityRate"@en ;
    skos:prefLabel "CRate"@en ;
    emmo:EMMO_967080e5_2f42_4eb2_a3a9_c58143e835f9 "[an indicator of the] electric current at which a secondary cell or battery is charged"@en .

:electrochemistry_21745019_2830_4395_bca7_15ddfd266673 a owl:Class ;
    rdfs:label "ElectrochemicalKineticQuantity"@en ;
    rdfs:comment "a quantity that relates to the kinetics of a reaction."@en ;
    rdfs:subClassOf :electrochemistry_aecc6094_c6a5_4a36_a825_8a497a2ae112 ;
    skos:prefLabel "ElectrochemicalKineticQuantity"@en ;
    emmo:EMMO_967080e5_2f42_4eb2_a3a9_c58143e835f9 "a quantity that relates to the kinetics of a reaction."@en .

:electrochemistry_2a2f59b7_aa16_40aa_9c8b_0de8a2720456 a owl:Class ;
    rdfs:label "FaradaicCurrent"@en ;
    rdfs:comment "Current that is produced by other processes, for example by diffusion of charged species, is termed ‘non- faradaic current’."@en,
        "I_f"@en,
        "electric current that results from the electrooxidation or electroreduction of an electroactive substance"@en ;
    rdfs:subClassOf emmo:EMMO_c995ae70_3b84_4ebb_bcfc_69e6a281bb88,
        :electrochemistry_aecc6094_c6a5_4a36_a825_8a497a2ae112 ;
    skos:prefLabel "FaradaicCurrent"@en ;
    emmo:EMMO_26bf1bef_d192_4da6_b0eb_d2209698fb54 "https://www.wikidata.org/wiki/Q5434687" ;
    emmo:EMMO_6dd685dd_1895_46e4_b227_be9f7d643c25 "https://dbpedia.org/page/Faradaic_current"@en ;
    emmo:EMMO_967080e5_2f42_4eb2_a3a9_c58143e835f9 "electric current that results from the electrooxidation or electroreduction of an electroactive substance"@en ;
    emmo:EMMO_c84c6752_6d64_48cc_9500_e54a3c34898d "https://en.wikipedia.org/wiki/Faradaic_current"@en ;
    emmo:EMMO_fe015383_afb3_44a6_ae86_043628697aa2 "https://goldbook.iupac.org/terms/view/F02321"@en .

:electrochemistry_74de2c33_84fc_4c2f_afe1_56d169149114 a owl:Class ;
    rdfs:label "CurrentLimit"@en ;
    rdfs:comment "limit on the electric current of an electrical system"@en ;
    rdfs:subClassOf emmo:EMMO_c995ae70_3b84_4ebb_bcfc_69e6a281bb88,
        :electrochemistry_b395a244_3a75_4737_be38_981bfa1277fe ;
    skos:prefLabel "CurrentLimit"@en ;
    emmo:EMMO_967080e5_2f42_4eb2_a3a9_c58143e835f9 "limit on the electric current of an electrical system"@en .

:electrochemistry_d7f8cab9_b035_4ecd_be63_292672572526 a owl:Class ;
    rdfs:label "ActivationEnergy"@en ;
    rdfs:comment "the activation energy in an arrhenius formulation"@en ;
    rdfs:subClassOf emmo:EMMO_f675294e_6f30_4b1d_a68e_a74e59f3b2fc ;
    skos:altLabel "ArrheniusActivationEnergy"@en ;
    skos:prefLabel "ActivationEnergy"@en ;
    emmo:EMMO_26bf1bef_d192_4da6_b0eb_d2209698fb54 "https://www.wikidata.org/wiki/Q190474"@en ;
    emmo:EMMO_967080e5_2f42_4eb2_a3a9_c58143e835f9 "the activation energy in an arrhenius formulation"@en ;
    emmo:EMMO_c84c6752_6d64_48cc_9500_e54a3c34898d "https://en.wikipedia.org/wiki/Activation_energy"@en ;
    emmo:EMMO_fe015383_afb3_44a6_ae86_043628697aa2 "https://doi.org/10.1351/goldbook.A00102"@en .

skos:note a owl:AnnotationProperty ;
    rdfs:comment "a general annotation that provides extra context, clarifications, or useful background information"@en ;
    emmo:EMMO_967080e5_2f42_4eb2_a3a9_c58143e835f9 "a general annotation that provides extra context, clarifications, or useful background information"@en .

:electrochemistry_1cd1d777_e67b_47eb_81f1_edac35d9f2c6 a owl:Class ;
    rdfs:label "Overpotential"@en ;
    rdfs:comment "difference between the electrode potential with current flow, and the electrode potential without current flow, i.e. the equilibrium potential"@en,
        "electrode potential (E) minus the equilibrium electrode potential (Eeq) of an electrochemical reaction"@en,
        "overpotential is positive for oxidation reactions and negative for reduction reactions"@en ;
    rdfs:subClassOf emmo:EMMO_4f2d3939_91b1_4001_b8ab_7d19074bf845,
        :electrochemistry_aecc6094_c6a5_4a36_a825_8a497a2ae112 ;
    skos:altLabel "ElectrodePolarization"@en,
        "Overvoltage"@en,
        "PolarizationPotential"@en ;
    skos:note "Overpotential is often divided into different contributions: activation overpotential, ohmic overpotential, and concentration overpotential."@en ;
    skos:prefLabel "Overpotential"@en ;
    skos:scopeNote "Overpotential is the extra voltage required to drive an electrochemical reaction beyond its thermodynamic equilibrium potential. It arises due to kinetic barriers such as activation energy, mass transport limitations, and charge transfer resistance. Overpotential is a key factor in battery efficiency, electrolysis, and corrosion studies, as it affects reaction rates and energy losses."@en ;
    emmo:EMMO_50c298c2_55a2_4068_b3ac_4e948c33181f "https://www.electropedia.org/iev/iev.nsf/display?openform&ievref=482-03-02" ;
    emmo:EMMO_967080e5_2f42_4eb2_a3a9_c58143e835f9 "electrode potential (E) minus the equilibrium electrode potential (Eeq) of an electrochemical reaction"@en ;
    emmo:EMMO_c84c6752_6d64_48cc_9500_e54a3c34898d "https://en.wikipedia.org/wiki/Overpotential"@en ;
    emmo:EMMO_fe015383_afb3_44a6_ae86_043628697aa2 "https://goldbook.iupac.org/terms/view/O04358" .

:electrochemistry_2d896559_eee3_447c_9759_87c854a4266a a owl:Class ;
    rdfs:label "ElectrochemicalThermodynamicQuantity"@en ;
    rdfs:comment "an electrochemical quantity describing concepts from thermodynamics"@en ;
    rdfs:subClassOf :electrochemistry_aecc6094_c6a5_4a36_a825_8a497a2ae112 ;
    skos:prefLabel "ElectrochemicalThermodynamicQuantity"@en ;
    emmo:EMMO_967080e5_2f42_4eb2_a3a9_c58143e835f9 "an electrochemical quantity describing concepts from thermodynamics"@en .

:electrochemistry_791c1915_a791_4450_acd8_7f94764743b5 a owl:Class ;
    rdfs:label "Capacity"@en ;
    rdfs:comment "electric charge which an energy storage device can deliver under specified conditions"@en,
        "the SI unit for electric charge is the coulomb (1 C = 1 A·s) but in practice, capacity is usually expressed in ampere hours (A·h)"@en ;
    rdfs:subClassOf emmo:EMMO_1604f495_328a_4f28_9962_f4cc210739dd,
        emmo:EMMO_2946d40b_24a1_47fa_8176_e3f79bb45064,
        :electrochemistry_aecc6094_c6a5_4a36_a825_8a497a2ae112 ;
    skos:altLabel "ChargeCapacity"@en,
        "ElectricChargeCapacity"@en,
        "StorageCapacity"@en ;
    skos:hiddenLabel "AH"@en,
        "Amp-hr"@en,
        "Capacity/mAh"@en,
        "mAmp-hr"@en ;
    skos:prefLabel "Capacity"@en ;
    emmo:EMMO_967080e5_2f42_4eb2_a3a9_c58143e835f9 "electric charge which an energy storage device can deliver under specified conditions"@en ;
    emmo:EMMO_cc65321f_1964_4f16_aea3_2a8edf2f3394 emmo:AmpereHour,
        emmo:MilliAmpereHour ;
    :electrochemistry_097ea615_c209_4edd_a1a1_5eea71d98fe8 "amp-hr"@en ;
    :electrochemistry_811aafc3_0c6d_470e_b67e_ff5c82992609 "Capacity(mAh)"@en ;
    :electrochemistry_8377c1f7_2b09_4632_9a4d_bb318438adbb "cell_coulomb_count_c"@en ;
    :electrochemistry_ea9f4dba_8ca2_419e_9cdf_ce54e9ebbd46 "Capacity (Ah)"@en .

:electrochemistry_9b3b4668_0795_4a35_9965_2af383497a26 a owl:Class ;
    rdfs:label "RatedCapacity"@en ;
    rdfs:comment "capacity value of a battery [or electrode or electrochemical device] determined under specified conditions and declared by the manufacturer"@en ;
    rdfs:seeAlso "https://w3id.org/emmo/domain/electrochemistry#electrochemistry_5ebeea80_af22_456b_9087_78c2a8465c58",
        "https://w3id.org/emmo/domain/electrochemistry#electrochemistry_e1fd84eb_acdb_4b2c_b90c_e899d552a3ee" ;
    rdfs:subClassOf :electrochemistry_791c1915_a791_4450_acd8_7f94764743b5 ;
    skos:prefLabel "RatedCapacity"@en ;
    skos:scopeNote "The term 'rated capacity' is used by manufacturers to specify the energy storage capability of a product under some controlled test conditions. The value is often determined during a constant current load until the a voltage limit is reached, under controlled temperature conditions. The 'rated capacity' helps to compare performance across different devices and provides a bisis for performing system engineering calculations. It can also be used as a basis for calculating other terms like the C-Rate, state-of-charge, and state-of-health of the device. The rated capacity at beginning of life serves as a reference for capacity-fade analysis during long-term cycling."@en ;
    emmo:EMMO_50c298c2_55a2_4068_b3ac_4e948c33181f "https://www.electropedia.org/iev/iev.nsf/display?openform&ievref=482-03-15"@en ;
    emmo:EMMO_5f7abc2a_5b50_41c3_8def_c8ba7c3b083e "The value of rated capacity should be reported together with information on the conditions under which it was determined (e.g. voltage limits, applied current, temperature)."@en ;
    emmo:EMMO_967080e5_2f42_4eb2_a3a9_c58143e835f9 "capacity value of a battery [or electrode or electrochemical device] determined under specified conditions and declared by the manufacturer"@en ;
    emmo:EMMO_b6730304_cabc_4104_b415_14218466445c "The value for rated capacity does not necessarily represent the actual capacity in real-world usage, as factors like temperature, rate, and state-of-health affect the effective capacity."@en ;
    emmo:EMMO_cc65321f_1964_4f16_aea3_2a8edf2f3394 "https://w3id.org/emmo#AmpereHour"^^xsd:anyURI,
        "https://w3id.org/emmo#MilliAmpereHour" .

:electrochemistry_9c657fdc_b9d3_4964_907c_f9a6e8c5f52b a owl:Class ;
    rdfs:label "OpenCircuitVoltage"@en ;
    rdfs:comment "voltage of a cell or battery when the discharge current is zero.",
        "In the case of a reversible electrode system, the OCP is also referred to as the equilibrium electrode potential. Otherwise, it is called the rest potential, or the corrosion potential, depending on the system being studied."@en,
        "electrode potential of working electrode relative to the reference electrode when no potential or electric current is being applied to the electrochemical cell"@en ;
    rdfs:subClassOf :electrochemistry_2d896559_eee3_447c_9759_87c854a4266a,
        :electrochemistry_4ebe2ef1_eea8_4b10_822d_7a68215bd24d ;
    skos:altLabel "OCP"@en,
        "OCV"@en,
        "OpenCircuitPotential"@en ;
    skos:prefLabel "OpenCircuitVoltage"@en ;
    emmo:EMMO_26bf1bef_d192_4da6_b0eb_d2209698fb54 "https://www.wikidata.org/wiki/Q1812203" ;
    emmo:EMMO_50c298c2_55a2_4068_b3ac_4e948c33181f "https://www.electropedia.org/iev/iev.nsf/display?openform&ievref=482-03-32" ;
    emmo:EMMO_967080e5_2f42_4eb2_a3a9_c58143e835f9 "electrode potential of working electrode relative to the reference electrode when no potential or electric current is being applied to the electrochemical cell"@en ;
    emmo:EMMO_c84c6752_6d64_48cc_9500_e54a3c34898d "https://en.wikipedia.org/wiki/Open-circuit_voltage"@en .

:electrochemistry_4ebe2ef1_eea8_4b10_822d_7a68215bd24d a owl:Class ;
    rdfs:label "CellVoltage"@en ;
    rdfs:comment "difference of electric potentials measured between identical metallic leads to two electrodes of an electrochemical cell"@en,
        "voltage between the terminals of an electrochemical cell"@en ;
    rdfs:seeAlso emmo:EMMO_17b031fb_4695_49b6_bb69_189ec63df3ee,
        emmo:EMMO_4f2d3939_91b1_4001_b8ab_7d19074bf845 ;
    rdfs:subClassOf emmo:EMMO_17b031fb_4695_49b6_bb69_189ec63df3ee,
        :electrochemistry_aecc6094_c6a5_4a36_a825_8a497a2ae112 ;
    skos:altLabel "AppliedPotential"@en ;
    skos:hiddenLabel "Ecell/V"@en,
        "Voltage/V"@en,
        "Volts"@en ;
    skos:note "Cell voltage fluctuates based on factors such as applied current, internal resistance, temperature, and composition."@en ;
    skos:prefLabel "CellVoltage"@en ;
    skos:scopeNote "Cell voltage represents the instantaneous electrical potential difference between the positive and negative electrodes of an electrochemical cell. It is a key parameter for monitoring battery performance, estimating state-of-charge, and diagnosing potential failures."@en ;
    emmo:EMMO_50c298c2_55a2_4068_b3ac_4e948c33181f "https://www.electropedia.org/iev/iev.nsf/display?openform&ievref=114-03-10" ;
    emmo:EMMO_967080e5_2f42_4eb2_a3a9_c58143e835f9 "voltage between the terminals of an electrochemical cell"@en ;
    emmo:EMMO_fe015383_afb3_44a6_ae86_043628697aa2 "https://doi.org/10.1351/goldbook.A00424"@en ;
    :electrochemistry_097ea615_c209_4edd_a1a1_5eea71d98fe8 "volts"@en ;
    :electrochemistry_1b717a20_17e3_4480_8c60_c4ae94058f05 "Voltage (V)"@en ;
    :electrochemistry_69022178_77b8_4669_97e2_351d45356e5a "Ecell/V"@en ;
    :electrochemistry_811aafc3_0c6d_470e_b67e_ff5c82992609 "Voltage(V)"@en ;
    :electrochemistry_8377c1f7_2b09_4632_9a4d_bb318438adbb "cell_voltage_v"@en ;
    :electrochemistry_a07dd85b_d0df_4d5d_8b0c_14d20ea3fe45 "voltage"@en ;
    :electrochemistry_ea9f4dba_8ca2_419e_9cdf_ce54e9ebbd46 "Potential (V)"@en .

emmo:EMMO_4f2d3939_91b1_4001_b8ab_7d19074bf845 skos:scopeNote "Electric potential is the amount of electric potential energy per unit charge at a specific point in an electric field. In electrochemistry, it helps describe the energy state of an electrode relative to a reference electrode. It is a fundamental concept in electrode reactions, influencing redox potential and determining the driving force behind electrochemical processes. Electric potential is commonly measured in volts (V) and is essential for understanding electrode kinetics, corrosion processes, and electrochemical equilibrium."@en ;
    emmo:EMMO_5f7abc2a_5b50_41c3_8def_c8ba7c3b083e "Use a well-defined reference electrode (e.g., Standard Hydrogen Electrode, Ag/AgCl) when measuring electric potential to ensure consistency and comparability."@en ;
    emmo:EMMO_b6730304_cabc_4104_b415_14218466445c "Electric potential differs from voltage; voltage is the difference in electric potential between two points."@en ;
    :electrochemistry_7104c722_d5a5_4bff_ba2f_37e229bb6cce true .

:electrochemistry_02eb0465_4f94_453c_8c1f_5ddf80134634 a owl:Class ;
    rdfs:label "ElectrochemicalPerformanceQuantity"@en ;
    rdfs:comment "a quantity that indicates the performance of an electrochemical device"@en ;
    rdfs:subClassOf :electrochemistry_aecc6094_c6a5_4a36_a825_8a497a2ae112 ;
    skos:prefLabel "ElectrochemicalPerformanceQuantity"@en ;
    emmo:EMMO_967080e5_2f42_4eb2_a3a9_c58143e835f9 "a quantity that indicates the performance of an electrochemical device"@en .

:electrochemistry_c5047d29_4e68_43ee_8355_3e8f05dc70a5 a owl:Class ;
    rdfs:label "ElectrochemicalControlQuantity"@en ;
    rdfs:comment "quantities that control electroanalytical techniques"@en ;
    rdfs:subClassOf :electrochemistry_aecc6094_c6a5_4a36_a825_8a497a2ae112 ;
    skos:prefLabel "ElectrochemicalControlQuantity"@en ;
    emmo:EMMO_967080e5_2f42_4eb2_a3a9_c58143e835f9 "quantities that control electroanalytical techniques"@en .

:electrochemistry_aecc6094_c6a5_4a36_a825_8a497a2ae112 a owl:Class ;
    rdfs:label "ElectrochemicalQuantity"@en ;
    rdfs:comment "Physical quantities defined within the domain of electrochemistry."@en ;
    rdfs:subClassOf emmo:EMMO_79751276_b2d0_4e2f_bbd4_99d412f43d55,
        emmo:EMMO_faab3f84_e475_4a46_af9c_7d249f0b9aef ;
    skos:prefLabel "ElectrochemicalQuantity"@en ;
    emmo:EMMO_967080e5_2f42_4eb2_a3a9_c58143e835f9 "Physical quantities defined within the domain of electrochemistry."@en .

[] a owl:Axiom ;
    dcterms:source "International Electrotechnical Commission (IEC), IEC 60050 - International Electrotechnical Vocabulary, retrieved from: https://www.electropedia.org" ;
    owl:annotatedProperty emmo:EMMO_967080e5_2f42_4eb2_a3a9_c58143e835f9 ;
    owl:annotatedSource :electrochemistry_03a6ce70_5085_4683_bb4e_fc3c18f7143a ;
    owl:annotatedTarget "part of the electrode polarization arising from an electric current through an ohmic resistance within the electrode or the electrolyte"@en .

[] a owl:Axiom ;
    dcterms:source "J. M. Pingarrón et al., Terminology of electrochemical methods of analysis (IUPAC Recommendations 2019), Pure and Applied Chemistry, 4, 92, 2020, 641-694. https://doi.org/10.1515/pac-2018-0109" ;
    owl:annotatedProperty emmo:EMMO_967080e5_2f42_4eb2_a3a9_c58143e835f9 ;
    owl:annotatedSource :electrochemistry_14577b99_a8a9_4358_9bc5_ab8c401dd34b ;
    owl:annotatedTarget "algebraic sum of faradaic currents flowing through an electrode"@en .

[] a owl:Axiom ;
    dcterms:source "International Electrotechnical Commission (IEC), IEC 60050 - International Electrotechnical Vocabulary, retrieved from: https://www.electropedia.org" ;
    owl:annotatedProperty emmo:EMMO_967080e5_2f42_4eb2_a3a9_c58143e835f9 ;
    owl:annotatedSource :electrochemistry_d47985f1_6bd7_4c4f_894f_13a6cab38bb5 ;
    owl:annotatedTarget "electric charge capacity remaining in a cell or battery following a discharge, operation or storage under specific test conditions"@en .

[] a owl:Axiom ;
    dcterms:source "J. M. Pingarrón et al., Terminology of electrochemical methods of analysis (IUPAC Recommendations 2019), Pure and Applied Chemistry, 4, 92, 2020, 641-694. https://doi.org/10.1515/pac-2018-0109" ;
    owl:annotatedProperty emmo:EMMO_967080e5_2f42_4eb2_a3a9_c58143e835f9 ;
    owl:annotatedSource :electrochemistry_d5ac8868_d318_4065_aa23_72140ae888ae ;
    owl:annotatedTarget "faradaic current that is approached as the rate of the charge-transfer process is increased by varying the applied potential, being greater than the rate of mass transport controlled by diffusion"@en .

[] a owl:Axiom ;
    dcterms:source "International Electrotechnical Commission (IEC), IEC 60050 - International Electrotechnical Vocabulary, retrieved from: https://www.electropedia.org" ;
    owl:annotatedProperty rdfs:comment ;
    owl:annotatedSource :electrochemistry_d91940f0_c8b6_4505_9b68_6bf6cfc5c544 ;
    owl:annotatedTarget "electrode potential when the electrode reaction is in equilibrium."@en .

[] a owl:Axiom ;
    dcterms:source "J. M. Pingarrón et al., Terminology of electrochemical methods of analysis (IUPAC Recommendations 2019), Pure and Applied Chemistry, 4, 92, 2020, 641-694. https://doi.org/10.1515/pac-2018-0109" ;
    owl:annotatedProperty emmo:EMMO_967080e5_2f42_4eb2_a3a9_c58143e835f9 ;
    owl:annotatedSource :electrochemistry_d91940f0_c8b6_4505_9b68_6bf6cfc5c544 ;
    owl:annotatedTarget "potential of an electrode when no electric current flows through the cell and all local charge transfer equilibria across phase boundaries that are represented in the cell diagram (except at possible electrolyte-electrolyte junctions) and local chemical equilibria are established"@en .

[] a owl:Axiom ;
    dcterms:source "International Electrotechnical Commission (IEC), IEC 60050 - International Electrotechnical Vocabulary, retrieved from: https://www.electropedia.org" ;
    owl:annotatedProperty emmo:EMMO_967080e5_2f42_4eb2_a3a9_c58143e835f9 ;
    owl:annotatedSource :electrochemistry_e1fd84eb_acdb_4b2c_b90c_e899d552a3ee ;
    owl:annotatedTarget "[an indicator of the] electric current at which a secondary cell or battery is charged"@en .

[] a owl:Axiom ;
    dcterms:source "International Electrotechnical Commission (IEC), IEC 60050 - International Electrotechnical Vocabulary, retrieved from: https://www.electropedia.org" ;
    owl:annotatedProperty emmo:EMMO_967080e5_2f42_4eb2_a3a9_c58143e835f9 ;
    owl:annotatedSource :electrochemistry_e38f11d0_a16f_4fe8_8ec5_3fe4493b7759 ;
    owl:annotatedTarget "electric potential difference between the rigid layer and the diffuse layer of a double layer"@en .

[] a owl:Axiom ;
    dcterms:source "J. M. Pingarrón et al., Terminology of electrochemical methods of analysis (IUPAC Recommendations 2019), Pure and Applied Chemistry, 4, 92, 2020, 641-694. https://doi.org/10.1515/pac-2018-0109." ;
    owl:annotatedProperty emmo:EMMO_967080e5_2f42_4eb2_a3a9_c58143e835f9 ;
    owl:annotatedSource :electrochemistry_e4a221e0_afc9_4464_91d4_e0c8ecdf79e8 ;
    owl:annotatedTarget "electrode potential of the working electrode at which the peak current is attained"@en .

[] a owl:Axiom ;
    dcterms:source "International Electrotechnical Commission (IEC), IEC 60050 - International Electrotechnical Vocabulary, retrieved from: https://www.electropedia.org" ;
    owl:annotatedProperty emmo:EMMO_967080e5_2f42_4eb2_a3a9_c58143e835f9 ;
    owl:annotatedSource :electrochemistry_e4d666ee_d637_45cd_a904_dc33941ead4f ;
    owl:annotatedTarget "electric current delivered by a battery during its discharge"@en .

[] a owl:Axiom ;
    dcterms:source "International Electrotechnical Commission (IEC), IEC 60050 - International Electrotechnical Vocabulary, retrieved from: https://www.electropedia.org" ;
    owl:annotatedProperty emmo:EMMO_967080e5_2f42_4eb2_a3a9_c58143e835f9 ;
    owl:annotatedSource :electrochemistry_16a5de33_a2ca_4563_80d4_6caeb08d97ca ;
    owl:annotatedTarget "nominal property of an electrode, having values negative or positive according to the sign of the electrode potential, or neutral when the electrode potential is zero."@en .

[] a owl:Axiom ;
    dcterms:source "International Electrotechnical Commission (IEC), IEC 60050 - International Electrotechnical Vocabulary, retrieved from: https://www.electropedia.org" ;
    owl:annotatedProperty emmo:EMMO_967080e5_2f42_4eb2_a3a9_c58143e835f9 ;
    owl:annotatedSource :electrochemistry_e6b63190_acac_4e78_9cba_fb2b10bbe910 ;
    owl:annotatedTarget "quotient of the capacity of a cell or battery by its volume."@en .

[] a owl:Axiom ;
    dcterms:source "International Electrotechnical Commission (IEC), IEC 60050 - International Electrotechnical Vocabulary, retrieved from: https://www.electropedia.org" ;
    owl:annotatedProperty emmo:EMMO_967080e5_2f42_4eb2_a3a9_c58143e835f9 ;
    owl:annotatedSource :electrochemistry_e8ec76bf_2a60_4982_8cde_02dfbd2e626f ;
    owl:annotatedTarget "duration, under specific conditions, at the end of which a battery [ or electrochemical device ] has retained the ability to perform a specified function"@en .

[] a owl:Axiom ;
    dcterms:source "J. M. Pingarrón et al., Terminology of electrochemical methods of analysis (IUPAC Recommendations 2019), Pure and Applied Chemistry, 4, 92, 2020, 641-694. https://doi.org/10.1515/pac-2018-0109" ;
    owl:annotatedProperty emmo:EMMO_967080e5_2f42_4eb2_a3a9_c58143e835f9 ;
    owl:annotatedSource :electrochemistry_ecb6dfdf_bd3d_4339_8a1c_d32abbef30ba ;
    owl:annotatedTarget "duration of the sampling interval in pulse voltammetry"@en .

[] a owl:Axiom ;
    dcterms:source "International Electrotechnical Commission (IEC), IEC 60050 - International Electrotechnical Vocabulary, retrieved from: https://www.electropedia.org" ;
    owl:annotatedProperty emmo:EMMO_967080e5_2f42_4eb2_a3a9_c58143e835f9 ;
    owl:annotatedSource :electrochemistry_f4fadc4e_ca7d_4e4e_89cf_eacf45b4041e ;
    owl:annotatedTarget "part of the electrode polarization arising from a chemical reaction impeding the electrode reaction"@en .

[] a owl:Axiom ;
    dcterms:source "International Electrotechnical Commission (IEC), IEC 60050 - International Electrotechnical Vocabulary, retrieved from: https://www.electropedia.org" ;
    owl:annotatedProperty rdfs:comment ;
    owl:annotatedSource :electrochemistry_f509645f_eb27_470e_9112_7ab828ed40d3 ;
    owl:annotatedTarget "cell source voltage when the electrodes of the electrochemical cell are a reference electrode and the electrode in question."@en .

[] a owl:Axiom ;
    dcterms:source "J. M. Pingarrón et al., Terminology of electrochemical methods of analysis (IUPAC Recommendations 2019), Pure and Applied Chemistry, 4, 92, 2020, 641-694. https://doi.org/10.1515/pac-2018-0109" ;
    owl:annotatedProperty emmo:EMMO_967080e5_2f42_4eb2_a3a9_c58143e835f9 ;
    owl:annotatedSource :electrochemistry_f509645f_eb27_470e_9112_7ab828ed40d3 ;
    owl:annotatedTarget "electric potential at an electrode, reported as the difference in potential relative to a reference electrode"@en .

[] a owl:Axiom ;
    dcterms:source "PINGARRÓN, José M., et al. Terminology of electrochemical methods of analysis (IUPAC Recommendations 2019). Pure and Applied Chemistry, 2020, 92.4: 641-694." ;
    owl:annotatedProperty rdfs:comment ;
    owl:annotatedSource :electrochemistry_f591a444_89d6_4093_836d_7d53895edce4 ;
    owl:annotatedTarget "For Electrochemical Impedance Spectroscopy, the Peak Potential Amplitude is usually small, (normally 5 to 10 mV)."@en .

[] a owl:Axiom ;
    dcterms:source "International Electrotechnical Commission (IEC), IEC 60050 - International Electrotechnical Vocabulary, retrieved from: https://www.electropedia.org" ;
    owl:annotatedProperty rdfs:comment ;
    owl:annotatedSource :electrochemistry_f94678d6_1386_48fc_8e54_024921924401 ;
    owl:annotatedTarget "internal apparent resistance is expressed in ohms"@en .

[] a owl:Axiom ;
    dcterms:source "International Electrotechnical Commission (IEC), IEC 60050 - International Electrotechnical Vocabulary, retrieved from: https://www.electropedia.org" ;
    owl:annotatedProperty emmo:EMMO_967080e5_2f42_4eb2_a3a9_c58143e835f9 ;
    owl:annotatedSource :electrochemistry_f94678d6_1386_48fc_8e54_024921924401 ;
    owl:annotatedTarget "quotient of change of voltage of a battery by the corresponding change in discharge current under specified conditions."@en .

[] a owl:Axiom ;
    dcterms:source "J. M. Pingarrón et al., Terminology of electrochemical methods of analysis (IUPAC Recommendations 2019), Pure and Applied Chemistry, 4, 92, 2020, 641-694. https://doi.org/10.1515/pac-2018-0109" ;
    owl:annotatedProperty emmo:EMMO_967080e5_2f42_4eb2_a3a9_c58143e835f9 ;
    owl:annotatedSource :electrochemistry_17626b8e_dfce_4d3a_ae6c_5a7215d43a90 ;
    owl:annotatedTarget "faradaic current that is controlled by the rate at which electroactive species diffuse toward (or away from) and electrode-solution interface."@en .

[] a owl:Axiom ;
    dcterms:source "J. M. Pingarrón et al., Terminology of electrochemical methods of analysis (IUPAC Recommendations 2019), Pure and Applied Chemistry, 4, 92, 2020, 641-694. https://doi.org/10.1515/pac-2018-0109" ;
    owl:annotatedProperty emmo:EMMO_967080e5_2f42_4eb2_a3a9_c58143e835f9 ;
    owl:annotatedSource :electrochemistry_fa7790d6_07bb_4b0f_9965_55966828f5f3 ;
    owl:annotatedTarget "the interfacial area, determined on the assumption that the interface is truly flat (2-dimensional) and calculated using the geometric data of the involved surfaces"@en .

[] a owl:Axiom ;
    dcterms:source "J. M. Pingarrón et al., Terminology of electrochemical methods of analysis (IUPAC Recommendations 2019), Pure and Applied Chemistry, 4, 92, 2020, 641-694. https://doi.org/10.1515/pac-2018-0109" ;
    owl:annotatedProperty emmo:EMMO_967080e5_2f42_4eb2_a3a9_c58143e835f9 ;
    owl:annotatedSource :electrochemistry_ff7797ed_9ef7_40d0_872b_2c215cd54578 ;
    owl:annotatedTarget "electric potential of an ion-selective electrode (ISE) and activity of an analyte ion at which the potential of the ISE is independent of temperature"@en .

[] a owl:Axiom ;
    dcterms:source "J. M. Pingarrón et al., Terminology of electrochemical methods of analysis (IUPAC Recommendations 2019), Pure and Applied Chemistry, 4, 92, 2020, 641-694. https://doi.org/10.1515/pac-2018-0109" ;
    owl:annotatedProperty emmo:EMMO_967080e5_2f42_4eb2_a3a9_c58143e835f9 ;
    owl:annotatedSource :electrochemistry_1900143f_cbc0_415f_9057_9382022a7bfe ;
    owl:annotatedTarget "rotational frequency of a rotating component in a rotating disk electrode"@en .

[] a owl:Axiom ;
    dcterms:source "Buck, Richard P., and Erno Lindner. \"Recommendations for nomenclature of ionselective electrodes (IUPAC Recommendations 1994).\" Pure and Applied Chemistry 66.12 (1994): 2527-2536. DOI: 10.1351/pac199466122527" ;
    owl:annotatedProperty rdfs:comment ;
    owl:annotatedSource :electrochemistry_1a104474_c326_4a29_ac26_26a05ac8f72c ;
    owl:annotatedTarget "Buck and Lindner suggest a slope of 0.6 mV min-1 ."@en .

[] a owl:Axiom ;
    dcterms:source "J. M. Pingarrón et al., Terminology of electrochemical methods of analysis (IUPAC Recommendations 2019), Pure and Applied Chemistry, 4, 92, 2020, 641-694. https://doi.org/10.1515/pac-2018-0109" ;
    owl:annotatedProperty emmo:EMMO_967080e5_2f42_4eb2_a3a9_c58143e835f9 ;
    owl:annotatedSource :electrochemistry_1a104474_c326_4a29_ac26_26a05ac8f72c ;
    owl:annotatedTarget "Duration between the time when an ion-selective electrode and an external reference electrode (the two completing the ion-selective electrode cell) are brought into contact with a sample solution (or the time at which the activity of the ion of interest in solution is changed) and the first time at which the slope of the cell potential vs. time plot (ΔE/Δt) becomes equal to a limiting value selected on the basis of the experimental conditions and/or requirements concerning accuracy."@en .

[] a owl:Axiom ;
    dcterms:source "International Electrotechnical Commission (IEC), IEC 60050 - International Electrotechnical Vocabulary, retrieved from: https://www.electropedia.org" ;
    owl:annotatedProperty rdfs:comment ;
    owl:annotatedSource :electrochemistry_1cd1d777_e67b_47eb_81f1_edac35d9f2c6 ;
    owl:annotatedTarget "difference between the electrode potential with current flow, and the electrode potential without current flow, i.e. the equilibrium potential"@en .

[] a owl:Axiom ;
    dcterms:source "J. M. Pingarrón et al., Terminology of electrochemical methods of analysis (IUPAC Recommendations 2019), Pure and Applied Chemistry, 4, 92, 2020, 641-694. https://doi.org/10.1515/pac-2018-0109" ;
    owl:annotatedProperty emmo:EMMO_967080e5_2f42_4eb2_a3a9_c58143e835f9 ;
    owl:annotatedSource :electrochemistry_1cd1d777_e67b_47eb_81f1_edac35d9f2c6 ;
    owl:annotatedTarget "electrode potential (E) minus the equilibrium electrode potential (Eeq) of an electrochemical reaction"@en .

[] a owl:Axiom ;
    dcterms:source "International Electrotechnical Commission (IEC), IEC 60050 - International Electrotechnical Vocabulary, retrieved from: https://www.electropedia.org" ;
    owl:annotatedProperty emmo:EMMO_967080e5_2f42_4eb2_a3a9_c58143e835f9 ;
    owl:annotatedSource :electrochemistry_07e219c3_890f_488f_bd96_bee8e445d764 ;
    owl:annotatedTarget "Electric current that flows, at a particular value of the applied potential, in the absence of the substance whose electrode behaviour is being investigated, i.e. a \"blank\" solution."@en .

[] a owl:Axiom ;
    dcterms:source "International Electrotechnical Commission (IEC), IEC 60050 - International Electrotechnical Vocabulary, retrieved from: https://www.electropedia.org" ;
    owl:annotatedProperty emmo:EMMO_967080e5_2f42_4eb2_a3a9_c58143e835f9 ;
    owl:annotatedSource :electrochemistry_1e3dc60d_dd6b_47d6_8161_70004fc5ee30 ;
    owl:annotatedTarget "quotient of the capacity of a cell or battery [ or electrode or active material ] by its mass."@en .

[] a owl:Axiom ;
    dcterms:source "J. M. Pingarrón et al., Terminology of electrochemical methods of analysis (IUPAC Recommendations 2019), Pure and Applied Chemistry, 4, 92, 2020, 641-694. https://doi.org/10.1515/pac-2018-0109" ;
    owl:annotatedProperty emmo:EMMO_967080e5_2f42_4eb2_a3a9_c58143e835f9 ;
    owl:annotatedSource :electrochemistry_214d925c_76c4_4f69_9afc_056a1ea82fc6 ;
    owl:annotatedTarget "electric current that accompanies the adsorption of a species"@en .

[] a owl:Axiom ;
    dcterms:source "J. M. Pingarrón et al., Terminology of electrochemical methods of analysis (IUPAC Recommendations 2019), Pure and Applied Chemistry, 4, 92, 2020, 641-694. https://doi.org/10.1515/pac-2018-0109" ;
    owl:annotatedProperty emmo:EMMO_967080e5_2f42_4eb2_a3a9_c58143e835f9 ;
    owl:annotatedSource :electrochemistry_22cec04f_c7f3_4ff8_a34b_e512379c9dcb ;
    owl:annotatedTarget "component of electric current due to transport of ions in the electric field between the electrodes"@en .

[] a owl:Axiom ;
    dcterms:source "International Electrotechnical Commission (IEC), IEC 60050 - International Electrotechnical Vocabulary, retrieved from: https://www.electropedia.org" ;
    owl:annotatedProperty rdfs:comment ;
    owl:annotatedSource :electrochemistry_25e20915_c35d_4bee_ad31_736235a79780 ;
    owl:annotatedTarget "the discharge rate is calculated as the rated capacity divided by the corresponding discharge time which results in an electric current"@en .

[] a owl:Axiom ;
    dcterms:source "International Electrotechnical Commission (IEC), IEC 60050 - International Electrotechnical Vocabulary, retrieved from: https://www.electropedia.org" ;
    owl:annotatedProperty emmo:EMMO_967080e5_2f42_4eb2_a3a9_c58143e835f9 ;
    owl:annotatedSource :electrochemistry_25e20915_c35d_4bee_ad31_736235a79780 ;
    owl:annotatedTarget "[an indicator of the] electric current at which a battery is discharged"@en .

[] a owl:Axiom ;
    dcterms:source "J. M. Pingarrón et al., Terminology of electrochemical methods of analysis (IUPAC Recommendations 2019), Pure and Applied Chemistry, 4, 92, 2020, 641-694. https://doi.org/10.1515/pac-2018-0109" ;
    owl:annotatedProperty emmo:EMMO_967080e5_2f42_4eb2_a3a9_c58143e835f9 ;
    owl:annotatedSource :electrochemistry_264f40d1_17c9_4bc7_9c47_5cfb18132278 ;
    owl:annotatedTarget "the rate of change of applied potential with time"@en .

[] a owl:Axiom ;
    dcterms:source "International Electrotechnical Commission (IEC), IEC 60050 - International Electrotechnical Vocabulary, retrieved from: https://www.electropedia.org" ;
    owl:annotatedProperty emmo:EMMO_967080e5_2f42_4eb2_a3a9_c58143e835f9 ;
    owl:annotatedSource :electrochemistry_265bb4d6_5eec_40f6_a3fa_59b3bd08e9af ;
    owl:annotatedTarget "sum of the absolute values of the potential differences resulting from anodic and cathodic polarizations of an electrochemical cell"@en .

[] a owl:Axiom ;
    dcterms:source "J. M. Pingarrón et al., Terminology of electrochemical methods of analysis (IUPAC Recommendations 2019), Pure and Applied Chemistry, 4, 92, 2020, 641-694. https://doi.org/10.1515/pac-2018-0109" ;
    owl:annotatedProperty emmo:EMMO_b432d2d5_25f4_4165_99c5_5935a7763c1a ;
    owl:annotatedSource :electrochemistry_269ddd97_1437_4545_b272_0df75a12c68a ;
    owl:annotatedTarget "in EIS, an alternating voltage signal is superimposed to a baseline voltage, which can be the open circuit potential or a fixed cell voltage"@en .

[] a owl:Axiom ;
    dcterms:source "International Electrotechnical Commission (IEC), IEC 60050 - International Electrotechnical Vocabulary, retrieved from: https://www.electropedia.org" ;
    owl:annotatedProperty emmo:EMMO_967080e5_2f42_4eb2_a3a9_c58143e835f9 ;
    owl:annotatedSource :electrochemistry_0853b072_3b80_4864_8147_24ce35407ade ;
    owl:annotatedTarget "electrode polarization associated with an electrochemical reduction reaction"@en .

[] a owl:Axiom ;
    dcterms:source "J. M. Pingarrón et al., Terminology of electrochemical methods of analysis (IUPAC Recommendations 2019), Pure and Applied Chemistry, 4, 92, 2020, 641-694. https://doi.org/10.1515/pac-2018-0109." ;
    owl:annotatedProperty emmo:EMMO_967080e5_2f42_4eb2_a3a9_c58143e835f9 ;
    owl:annotatedSource :electrochemistry_2705525b_7512_48bf_825b_f2d0409bede4 ;
    owl:annotatedTarget "electric potential of the indicator electrode, in chronopotentiometry at constant current, at the instant when the time that has elapsed since the application of current is equal to one-fourth of the transition time"@en .

[] a owl:Axiom ;
    dcterms:source "J. M. Pingarrón et al., Terminology of electrochemical methods of analysis (IUPAC Recommendations 2019), Pure and Applied Chemistry, 4, 92, 2020, 641-694. https://doi.org/10.1515/pac-2018-0109" ;
    owl:annotatedProperty emmo:EMMO_967080e5_2f42_4eb2_a3a9_c58143e835f9 ;
    owl:annotatedSource :electrochemistry_2a2f59b7_aa16_40aa_9c8b_0de8a2720456 ;
    owl:annotatedTarget "electric current that results from the electrooxidation or electroreduction of an electroactive substance"@en .

[] a owl:Axiom ;
    dcterms:source "J. M. Pingarrón et al., Terminology of electrochemical methods of analysis (IUPAC Recommendations 2019), Pure and Applied Chemistry, 4, 92, 2020, 641-694. https://doi.org/10.1515/pac-2018-0109" ;
    owl:annotatedProperty emmo:EMMO_967080e5_2f42_4eb2_a3a9_c58143e835f9 ;
    owl:annotatedSource :electrochemistry_2ae53fc6_d44d_41c9_acaf_c5606e6a981d ;
    owl:annotatedTarget "electric potential of a steady-state voltammetric working electrode at the point, on the rising part of the voltammetric wave, where the current is equal to one-half of the limiting current"@en .

[] a owl:Axiom ;
    dcterms:source "International Electrotechnical Commission (IEC), IEC 60050 - International Electrotechnical Vocabulary, retrieved from: https://www.electropedia.org" ;
    owl:annotatedProperty emmo:EMMO_967080e5_2f42_4eb2_a3a9_c58143e835f9 ;
    owl:annotatedSource :electrochemistry_327eb3e1_f74a_4076_96de_5a2e3f63cb65 ;
    owl:annotatedTarget "component of an electric current that is associated with the presence of an analyate in square-wave voltammetry"@en .

[] a owl:Axiom ;
    dcterms:source "J. M. Pingarrón et al., Terminology of electrochemical methods of analysis (IUPAC Recommendations 2019), Pure and Applied Chemistry, 4, 92, 2020, 641-694. https://doi.org/10.1515/pac-2018-0109" ;
    owl:annotatedProperty emmo:EMMO_967080e5_2f42_4eb2_a3a9_c58143e835f9 ;
    owl:annotatedSource :electrochemistry_382b10dc_83aa_4e77_a1d5_1edd06fd1e05 ;
    owl:annotatedTarget "in dynamic voltammetric techniques, the maximum value of the faradaic current attained by varying the applied potential in the current-potential or I-E curve"@en .

[] a owl:Axiom ;
    dcterms:source "International Electrotechnical Commission (IEC), IEC 60050 - International Electrotechnical Vocabulary, retrieved from: https://www.electropedia.org" ;
    owl:annotatedProperty emmo:EMMO_967080e5_2f42_4eb2_a3a9_c58143e835f9 ;
    owl:annotatedSource :electrochemistry_3bb5ae23_59fa_4bc7_9495_803eb6719f28 ;
    owl:annotatedTarget "quotient of change in open-circuit voltage of a cell or battery by the corresponding change in temperature."@en .

[] a owl:Axiom ;
    dcterms:source "J. M. Pingarrón et al., Terminology of electrochemical methods of analysis (IUPAC Recommendations 2019), Pure and Applied Chemistry, 4, 92, 2020, 641-694. https://doi.org/10.1515/pac-2018-0109." ;
    owl:annotatedProperty emmo:EMMO_967080e5_2f42_4eb2_a3a9_c58143e835f9 ;
    owl:annotatedSource :electrochemistry_3cd0e74e_292c_48ed_a831_4cb8753d9a56 ;
    owl:annotatedTarget "time interval during which the excitation signal deviates from the base line in normal pulse voltamme- try, differential pulse voltammetry, and related techniques"@en .

[] a owl:Axiom ;
    dcterms:source "J. M. Pingarrón et al., Terminology of electrochemical methods of analysis (IUPAC Recommendations 2019), Pure and Applied Chemistry, 4, 92, 2020, 641-694. https://doi.org/10.1515/pac-2018-0109" ;
    owl:annotatedProperty emmo:EMMO_967080e5_2f42_4eb2_a3a9_c58143e835f9 ;
    owl:annotatedSource :electrochemistry_47ab1dad_cc09_4fd8_af23_acb36fb680dd ;
    owl:annotatedTarget "area of electrode - solution interface."@en .

[] a owl:Axiom ;
    dcterms:source "International Electrotechnical Commission (IEC), IEC 60050 - International Electrotechnical Vocabulary, retrieved from: https://www.electropedia.org" ;
    owl:annotatedProperty emmo:EMMO_967080e5_2f42_4eb2_a3a9_c58143e835f9 ;
    owl:annotatedSource :electrochemistry_49efb72a_f8e6_4f50_acac_975302200d47 ;
    owl:annotatedTarget "ability of a cell or battery to retain capacity on open circuit under specified conditions."@en .

[] a owl:Axiom ;
    dcterms:source "J. M. Pingarrón et al., Terminology of electrochemical methods of analysis (IUPAC Recommendations 2019), Pure and Applied Chemistry, 4, 92, 2020, 641-694. https://doi.org/10.1515/pac-2018-0109" ;
    owl:annotatedProperty rdfs:comment ;
    owl:annotatedSource :electrochemistry_4ebe2ef1_eea8_4b10_822d_7a68215bd24d ;
    owl:annotatedTarget "difference of electric potentials measured between identical metallic leads to two electrodes of an electrochemical cell"@en .

[] a owl:Axiom ;
    dcterms:source "International Electrotechnical Commission (IEC), IEC 60050 - International Electrotechnical Vocabulary, retrieved from: https://www.electropedia.org" ;
    owl:annotatedProperty emmo:EMMO_967080e5_2f42_4eb2_a3a9_c58143e835f9 ;
    owl:annotatedSource :electrochemistry_4ebe2ef1_eea8_4b10_822d_7a68215bd24d ;
    owl:annotatedTarget "voltage between the terminals of an electrochemical cell"@en .

[] a owl:Axiom ;
    dcterms:source "International Electrotechnical Commission (IEC), IEC 60050 - International Electrotechnical Vocabulary, retrieved from: https://www.electropedia.org" ;
    owl:annotatedProperty emmo:EMMO_967080e5_2f42_4eb2_a3a9_c58143e835f9 ;
    owl:annotatedSource :electrochemistry_50674621_09ae_4f03_8ee9_3997b88c8b2a ;
    owl:annotatedTarget "[an indicator of the] electric current at which a battery is charged towards the end of charge"@en .

[] a owl:Axiom ;
    dcterms:source "International Electrotechnical Commission (IEC), IEC 60050 - International Electrotechnical Vocabulary, retrieved from: https://www.electropedia.org" ;
    owl:annotatedProperty emmo:EMMO_967080e5_2f42_4eb2_a3a9_c58143e835f9 ;
    owl:annotatedSource :electrochemistry_526bf81a_0572_49ff_a8cc_85efc343c1c2 ;
    owl:annotatedTarget "charged active material remaining in a cell following a discharge to a specified end-of-discharge voltage."@en .

[] a owl:Axiom ;
    dcterms:source "J. M. Pingarrón et al., Terminology of electrochemical methods of analysis (IUPAC Recommendations 2019), Pure and Applied Chemistry, 4, 92, 2020, 641-694. https://doi.org/10.1515/pac-2018-0109" ;
    owl:annotatedProperty emmo:EMMO_967080e5_2f42_4eb2_a3a9_c58143e835f9 ;
    owl:annotatedSource :electrochemistry_52ac73c7_763c_4fda_93cd_a2db9dfc2dab ;
    owl:annotatedTarget "time interval during which the current is measured in pulse voltammetry"@en .

[] a owl:Axiom ;
    dcterms:source "International Electrotechnical Commission (IEC), IEC 60050 - International Electrotechnical Vocabulary, retrieved from: https://www.electropedia.org" ;
    owl:annotatedProperty rdfs:comment ;
    owl:annotatedSource :electrochemistry_534dd59c_904c_45d9_8550_ae9d2eb6bbc9 ;
    owl:annotatedTarget "specified voltage of a battery at which the battery discharge is terminated."@en .

[] a owl:Axiom ;
    dcterms:source "International Electrotechnical Commission (IEC), IEC 60050 - International Electrotechnical Vocabulary, retrieved from: https://www.electropedia.org" ;
    owl:annotatedProperty emmo:EMMO_967080e5_2f42_4eb2_a3a9_c58143e835f9 ;
    owl:annotatedSource :electrochemistry_565c0b10_70fe_441a_b76a_b9a8e08ca7b7 ;
    owl:annotatedTarget "electrode polarization associated with an electrochemical oxidation reaction"@en .

[] a owl:Axiom ;
    dcterms:source "International Electrotechnical Commission (IEC), IEC 60050 - International Electrotechnical Vocabulary, retrieved from: https://www.electropedia.org" ;
    owl:annotatedProperty emmo:EMMO_967080e5_2f42_4eb2_a3a9_c58143e835f9 ;
    owl:annotatedSource :electrochemistry_5696453c_9da7_41e2_bbda_603c1b90a8fc ;
    owl:annotatedTarget "fraction of the electric current passing through an electrochemical cell which accomplishes the desired chemical reaction"@en .

[] a owl:Axiom ;
    dcterms:source "https://doi.org/10.1016/j.coche.2016.02.006" ;
    owl:annotatedProperty rdfs:comment ;
    owl:annotatedSource :electrochemistry_5c34b3b5_c9c4_477d_809a_3f682f995aa9 ;
    owl:annotatedTarget "valid in situations where the insulating phase is present in a low volume fraction and represented by random, isotropic spheres"@en .

[] a owl:Axiom ;
    dcterms:source "J. M. Pingarrón et al., Terminology of electrochemical methods of analysis (IUPAC Recommendations 2019), Pure and Applied Chemistry, 4, 92, 2020, 641-694. https://doi.org/10.1515/pac-2018-0109" ;
    owl:annotatedProperty emmo:EMMO_967080e5_2f42_4eb2_a3a9_c58143e835f9 ;
    owl:annotatedSource :electrochemistry_5fb7a03f_d6dd_47ee_9317_0629681c7d00 ;
    owl:annotatedTarget "diffusion current of the potential-independent value that is approached as the rate of the charge-transfer process is increased by varying the applied potential, being greater than the rate of mass transport controlled by diffusion"@en .

[] a owl:Axiom ;
    dcterms:source "J. M. Pingarrón et al., Terminology of electrochemical methods of analysis (IUPAC Recommendations 2019), Pure and Applied Chemistry, 4, 92, 2020, 641-694. https://doi.org/10.1515/pac-2018-0109" ;
    owl:annotatedProperty emmo:EMMO_967080e5_2f42_4eb2_a3a9_c58143e835f9 ;
    owl:annotatedSource :electrochemistry_601ff226_59b9_460b_90f5_2593450d96fa ;
    owl:annotatedTarget "electric potential difference between two solutions separated by an ion-selective membrane in the absence of any electric current flowing through the membrane"@en .

[] a owl:Axiom ;
    dcterms:references "J. Newman and K. E. Thmoas-Alyea, Electrochemical Systems, 3rd ed. Hoboken, New Jersey: John Wiley & Sons, 2004." ;
    owl:annotatedProperty emmo:EMMO_967080e5_2f42_4eb2_a3a9_c58143e835f9 ;
    owl:annotatedSource :electrochemistry_60741c58_a10d_4aa6_bb68_0066a6ff8e30 ;
    owl:annotatedTarget "The potential of a working electrode relative to a reference electrode of the same kinds placed in the solution adjacent to the surface of the working electrode (just outside the double layer)."@en .

[] a owl:Axiom ;
    dcterms:source "International Electrotechnical Commission (IEC), IEC 60050 - International Electrotechnical Vocabulary, retrieved from: https://www.electropedia.org" ;
    owl:annotatedProperty emmo:EMMO_967080e5_2f42_4eb2_a3a9_c58143e835f9 ;
    owl:annotatedSource :electrochemistry_639b844a_e801_436b_985d_28926129ead6 ;
    owl:annotatedTarget "suitable approximate value of the voltage used to designate or identify a cell, a battery or an electrochemical system"@en .

[] a owl:Axiom ;
    dcterms:source "J. M. Pingarrón et al., Terminology of electrochemical methods of analysis (IUPAC Recommendations 2019), Pure and Applied Chemistry, 4, 92, 2020, 641-694. https://doi.org/10.1515/pac-2018-0109" ;
    owl:annotatedProperty emmo:EMMO_967080e5_2f42_4eb2_a3a9_c58143e835f9 ;
    owl:annotatedSource :electrochemistry_63a8f9d2_0cf6_484d_b996_2e5c3f0a3c73 ;
    owl:annotatedTarget "amount of a chemical modifier at an electrode surface per unit area"@en .

[] a owl:Axiom ;
    dcterms:source "PINGARRÓN, José M., et al. Terminology of electrochemical methods of analysis (IUPAC Recommendations 2019). Pure and Applied Chemistry, 2020, 92.4: 641-694." ;
    owl:annotatedProperty rdfs:comment ;
    owl:annotatedSource :electrochemistry_68059d94_4c21_4065_b329_07faeebc7e87 ;
    owl:annotatedTarget "Alternating potential signals such as the ones applied in Electrochemical Impedance Spectroscopy are superimposed to a reference potential, which can be an applied potential or the open circuit potential."@en .

[] a owl:Axiom ;
    dcterms:source "J. M. Pingarrón et al., Terminology of electrochemical methods of analysis (IUPAC Recommendations 2019), Pure and Applied Chemistry, 4, 92, 2020, 641-694. https://doi.org/10.1515/pac-2018-0109." ;
    owl:annotatedProperty emmo:EMMO_967080e5_2f42_4eb2_a3a9_c58143e835f9 ;
    owl:annotatedSource :electrochemistry_136744ff_0563_4df7_aa03_4219d70392a0 ;
    owl:annotatedTarget "parameter defining the ability of an ion-selective electrode to distinguish a particular ion, i.e., a primary ion A from an interfering ion B"@en .

[] a owl:Axiom ;
    dcterms:source "International Electrotechnical Commission (IEC), IEC 60050 - International Electrotechnical Vocabulary, retrieved from: https://www.electropedia.org" ;
    owl:annotatedProperty emmo:EMMO_967080e5_2f42_4eb2_a3a9_c58143e835f9 ;
    owl:annotatedSource :electrochemistry_74861991_7da2_4e0f_b6c1_b16713f538bf ;
    owl:annotatedTarget "discharge voltage of a cell or battery at the beginning of the discharge immediately after any transients have subsided"@en .

[] a owl:Axiom ;
    dcterms:source "International Electrotechnical Commission (IEC), IEC 60050 - International Electrotechnical Vocabulary, retrieved from: https://www.electropedia.org" ;
    owl:annotatedProperty rdfs:comment ;
    owl:annotatedSource :electrochemistry_75c28dc8_3d7d_4b6e_861e_6c8b1ad7d644 ;
    owl:annotatedTarget "zero electric resistance is a hypothetical condition and in practice the short-circuit current is the peak current flowing in a circuit of very low resistance compared to the internal resistance of the battery"@en .

[] a owl:Axiom ;
    dcterms:source "International Electrotechnical Commission (IEC), IEC 60050 - International Electrotechnical Vocabulary, retrieved from: https://www.electropedia.org" ;
    owl:annotatedProperty emmo:EMMO_967080e5_2f42_4eb2_a3a9_c58143e835f9 ;
    owl:annotatedSource :electrochemistry_75c28dc8_3d7d_4b6e_861e_6c8b1ad7d644 ;
    owl:annotatedTarget "maximum current which should be delivered by a cell or battery into an external circuit with zero electric resistance, or an external circuit which depresses the cell or battery voltage to approximately zero volt"@en .

[] a owl:Axiom ;
    dcterms:source "International Electrotechnical Commission (IEC), IEC 60050 - International Electrotechnical Vocabulary, retrieved from: https://www.electropedia.org" ;
    owl:annotatedProperty emmo:EMMO_967080e5_2f42_4eb2_a3a9_c58143e835f9 ;
    owl:annotatedSource :electrochemistry_76e7e556_f47e_47e2_b2ef_67aeed09c63e ;
    owl:annotatedTarget "maximum electric current density that can be achieved for an electrode reaction at a given concentration of a electrochemically active material in the presence of a large excess of supporting electrolyte"@en .

[] a owl:Axiom ;
    dcterms:source "International Electrotechnical Commission (IEC), IEC 60050 - International Electrotechnical Vocabulary, retrieved from: https://www.electropedia.org" ;
    owl:annotatedProperty emmo:EMMO_967080e5_2f42_4eb2_a3a9_c58143e835f9 ;
    owl:annotatedSource :electrochemistry_79198264_cdf5_4fc3_8bcf_e5140a52547a ;
    owl:annotatedTarget "ratio of the electric energy provided from a secondary battery [ or electrochemical device ] during discharge to the electric energy supplied to the battery during the preceding charge"@en .

[] a owl:Axiom ;
    dcterms:source "International Electrotechnical Commission (IEC), IEC 60050 - International Electrotechnical Vocabulary, retrieved from: https://www.electropedia.org" ;
    owl:annotatedProperty rdfs:comment ;
    owl:annotatedSource :electrochemistry_791c1915_a791_4450_acd8_7f94764743b5 ;
    owl:annotatedTarget "the SI unit for electric charge is the coulomb (1 C = 1 A·s) but in practice, capacity is usually expressed in ampere hours (A·h)"@en .

[] a owl:Axiom ;
    dcterms:source "International Electrotechnical Commission (IEC), IEC 60050 - International Electrotechnical Vocabulary, retrieved from: https://www.electropedia.org" ;
    owl:annotatedProperty emmo:EMMO_967080e5_2f42_4eb2_a3a9_c58143e835f9 ;
    owl:annotatedSource :electrochemistry_7fa406b0_512a_4d59_9e0c_5d8aba0103ae ;
    owl:annotatedTarget "part of the electrode polarization arising from a charge-transfer step of the electrode reaction"@en .

[] a owl:Axiom ;
    dcterms:source "International Electrotechnical Commission (IEC), IEC 60050 - International Electrotechnical Vocabulary, retrieved from: https://www.electropedia.org" ;
    owl:annotatedProperty rdfs:comment ;
    owl:annotatedSource :electrochemistry_7fc10197_41d9_4c1e_a107_928f03eb2d36 ;
    owl:annotatedTarget "equilibrium electrode potential referenced to the standard hydrogen electrode."@en .

[] a owl:Axiom ;
    dcterms:source "J. M. Pingarrón et al., Terminology of electrochemical methods of analysis (IUPAC Recommendations 2019), Pure and Applied Chemistry, 4, 92, 2020, 641-694. https://doi.org/10.1515/pac-2018-0109" ;
    owl:annotatedProperty emmo:EMMO_967080e5_2f42_4eb2_a3a9_c58143e835f9 ;
    owl:annotatedSource :electrochemistry_7fc10197_41d9_4c1e_a107_928f03eb2d36 ;
    owl:annotatedTarget "equilibrium electrode potential of an electrode under standard conditions"@en .

[] a owl:Axiom ;
    dcterms:source "International Electrotechnical Commission (IEC), IEC 60050 - International Electrotechnical Vocabulary, retrieved from: https://www.electropedia.org" ;
    owl:annotatedProperty emmo:EMMO_967080e5_2f42_4eb2_a3a9_c58143e835f9 ;
    owl:annotatedSource :electrochemistry_83928dce_9746_4452_a9f9_da4366a20ca4 ;
    owl:annotatedTarget "ability of a cell or battery to contain its electrolyte under specified mechanical and environmental conditions"@en .

[] a owl:Axiom ;
    dcterms:source "International Electrotechnical Commission (IEC), IEC 60050 - International Electrotechnical Vocabulary, retrieved from: https://www.electropedia.org" ;
    owl:annotatedProperty emmo:EMMO_967080e5_2f42_4eb2_a3a9_c58143e835f9 ;
    owl:annotatedSource :electrochemistry_83fbc038_0c2e_4d04_91d7_cdf30f8a5535 ;
    owl:annotatedTarget "[a sign that] qualifies a cell or a battery having the shape of a parallelepiped whose faces are rectangular"@en .

[] a owl:Axiom ;
    dcterms:source "International Electrotechnical Commission (IEC), IEC 60050 - International Electrotechnical Vocabulary, retrieved from: https://www.electropedia.org" ;
    owl:annotatedProperty emmo:EMMO_967080e5_2f42_4eb2_a3a9_c58143e835f9 ;
    owl:annotatedSource :electrochemistry_8de9735b_374a_4a0f_b29f_71a50794cf94 ;
    owl:annotatedTarget "part of the electrode polarization arising from crystal nucleation and growth phenomena"@en .

[] a owl:Axiom ;
    dcterms:source "International Electrotechnical Commission (IEC), IEC 60050 - International Electrotechnical Vocabulary, retrieved from: https://www.electropedia.org" ;
    owl:annotatedProperty emmo:EMMO_967080e5_2f42_4eb2_a3a9_c58143e835f9 ;
    owl:annotatedSource :electrochemistry_8f3ab19f_ce22_424e_a9bf_d5cedb815374 ;
    owl:annotatedTarget "quotient of the change in capacity of a cell by the corresponding change in temperature."@en .

[] a owl:Axiom ;
    dcterms:source "J. M. Pingarrón et al., Terminology of electrochemical methods of analysis (IUPAC Recommendations 2019), Pure and Applied Chemistry, 4, 92, 2020, 641-694. https://doi.org/10.1515/pac-2018-0109" ;
    owl:annotatedProperty emmo:EMMO_967080e5_2f42_4eb2_a3a9_c58143e835f9 ;
    owl:annotatedSource :electrochemistry_98b6e9d7_d5df_46a5_87dd_79642b8b2e4b ;
    owl:annotatedTarget "faradaic current of an electroactive substance B formed by a prior chemical reaction from another substance Y that is no electroactive at the potential at which B is electrochemically transformed"@en .

[] a owl:Axiom ;
    dcterms:source "International Electrotechnical Commission (IEC), IEC 60050 - International Electrotechnical Vocabulary, retrieved from: https://www.electropedia.org" ;
    owl:annotatedProperty emmo:EMMO_967080e5_2f42_4eb2_a3a9_c58143e835f9 ;
    owl:annotatedSource :electrochemistry_9b3b4668_0795_4a35_9965_2af383497a26 ;
    owl:annotatedTarget "capacity value of a battery [or electrode or electrochemical device] determined under specified conditions and declared by the manufacturer"@en .

[] a owl:Axiom ;
    dcterms:source "J. M. Pingarrón et al., Terminology of electrochemical methods of analysis (IUPAC Recommendations 2019), Pure and Applied Chemistry, 4, 92, 2020, 641-694. https://doi.org/10.1515/pac-2018-0109" ;
    owl:annotatedProperty rdfs:comment ;
    owl:annotatedSource :electrochemistry_9c657fdc_b9d3_4964_907c_f9a6e8c5f52b ;
    owl:annotatedTarget "In the case of a reversible electrode system, the OCP is also referred to as the equilibrium electrode potential. Otherwise, it is called the rest potential, or the corrosion potential, depending on the system being studied."@en .

[] a owl:Axiom ;
    dcterms:source "International Electrotechnical Commission (IEC), IEC 60050 - International Electrotechnical Vocabulary, retrieved from: https://www.electropedia.org" ;
    owl:annotatedProperty rdfs:comment ;
    owl:annotatedSource :electrochemistry_9c657fdc_b9d3_4964_907c_f9a6e8c5f52b ;
    owl:annotatedTarget "voltage of a cell or battery when the discharge current is zero." .

[] a owl:Axiom ;
    dcterms:source "J. M. Pingarrón et al., Terminology of electrochemical methods of analysis (IUPAC Recommendations 2019), Pure and Applied Chemistry, 4, 92, 2020, 641-694. https://doi.org/10.1515/pac-2018-0109" ;
    owl:annotatedProperty emmo:EMMO_967080e5_2f42_4eb2_a3a9_c58143e835f9 ;
    owl:annotatedSource :electrochemistry_9c657fdc_b9d3_4964_907c_f9a6e8c5f52b ;
    owl:annotatedTarget "electrode potential of working electrode relative to the reference electrode when no potential or electric current is being applied to the electrochemical cell"@en .

[] a owl:Axiom ;
    dcterms:source "International Electrotechnical Commission (IEC), IEC 60050 - International Electrotechnical Vocabulary, retrieved from: https://www.electropedia.org" ;
    owl:annotatedProperty rdfs:comment ;
    owl:annotatedSource :electrochemistry_9ed7210c_c4fa_467b_822d_ba12f885bdf4 ;
    owl:annotatedTarget "part of the electrode polarization arising from concentration gradients of electrode reactants and products."@en .

[] a owl:Axiom ;
    dcterms:source "J. Newman and K. E. Thmoas-Alyea, Electrochemical Systems, 3rd ed. Hoboken, New Jersey: John Wiley & Sons, 2004." ;
    owl:annotatedProperty rdfs:comment ;
    owl:annotatedSource :electrochemistry_1422cde1_929e_46b6_b0dc_1010eebc5dfd ;
    owl:annotatedTarget "in quantum mechanical terms, electrochemical potential is defined as the energy level of the electron orbitals in the species that have a 50 percent probability of occupancy"@en .

[] a owl:Axiom ;
    dcterms:source "IUPAC. Compendium of Chemical Terminology, 2nd ed. (the \"Gold Book\"). Compiled by A. D. McNaught and A. Wilkinson. Blackwell Scientific Publications, Oxford (1997). Online version (2019-) created by S. J. Chalk. ISBN 0-9678550-9-8. https://doi.org/10.1351/goldbook." ;
    owl:annotatedProperty emmo:EMMO_967080e5_2f42_4eb2_a3a9_c58143e835f9 ;
    owl:annotatedSource :electrochemistry_9ed7210c_c4fa_467b_822d_ba12f885bdf4 ;
    owl:annotatedTarget "The concentration overpotential of an electrode reaction at a given electrode current density (c.d.) is basically the difference in equilibrium potentials across the diffusion layer. More precisely, it is the potential of a reference electrode (of the same electrode reaction as the working electrode ) with the interfacial concentrations which establish themselves at c.d., relative to the potential of a similar reference electrode with the concentrations of the bulk solution. From such a measured potential difference, with c.d. flowing, one needs to subtract the ohmic potential drop prevailing between the two electrodes."@en .

[] a owl:Axiom ;
    dcterms:source "J. M. Pingarrón et al., Terminology of electrochemical methods of analysis (IUPAC Recommendations 2019), Pure and Applied Chemistry, 4, 92, 2020, 641-694. https://doi.org/10.1515/pac-2018-0109" ;
    owl:annotatedProperty emmo:EMMO_967080e5_2f42_4eb2_a3a9_c58143e835f9 ;
    owl:annotatedSource :electrochemistry_a24f8581_a5a4_41a4_bb45_d0fdd5c0d810 ;
    owl:annotatedTarget "value of an electric current at an instant in time"@en .

[] a owl:Axiom ;
    dcterms:source "R. Guidelli et al., “Defining the transfer coefficient in electrochemistry: An assessment (IUPAC Technical Report),” Pure Appl. Chem., vol. 86, no. 2, pp. 245–258, 2014. https://doi.org/10.1515/pac-2014-5026" ;
    owl:annotatedProperty rdfs:comment ;
    owl:annotatedSource :electrochemistry_a4dfa5c1_55a9_4285_b71d_90cf6613ca31 ;
    owl:annotatedTarget "The cathodic transfer coefficient αc is defined as –(RT/nF)(dlnkc /dE), where kc is the electroreduction rate constant, E is the applied potential, and R, T, and F have their usual significance. This definition is equivalent to the other, -(RT/nF)(dln|jc |/dE), where jc is the cathodic current density corrected for any changes in the reactant concentration at the electrode surface with respect to its bulk value."@en .

[] a owl:Axiom ;
    dcterms:source "R. Guidelli et al., “Defining the transfer coefficient in electrochemistry: An assessment (IUPAC Technical Report),” Pure Appl. Chem., vol. 86, no. 2, pp. 245–258, 2014. https://doi.org/10.1515/pac-2014-5026" ;
    owl:annotatedProperty emmo:EMMO_967080e5_2f42_4eb2_a3a9_c58143e835f9 ;
    owl:annotatedSource :electrochemistry_a4dfa5c1_55a9_4285_b71d_90cf6613ca31 ;
    owl:annotatedTarget "the fraction of the electrostatic potential energy affecting the reduction rate in an electrode reaction, with the remaining fraction affecting the corresponding oxidation rate"@en .

[] a owl:Axiom ;
    dcterms:source "J. M. Pingarrón et al., Terminology of electrochemical methods of analysis (IUPAC Recommendations 2019), Pure and Applied Chemistry, 4, 92, 2020, 641-694. https://doi.org/10.1515/pac-2018-0109" ;
    owl:annotatedProperty emmo:EMMO_967080e5_2f42_4eb2_a3a9_c58143e835f9 ;
    owl:annotatedSource :electrochemistry_a56fc557_9dea_42e6_b936_e9d62dcaf84f ;
    owl:annotatedTarget "non-faradaic current associated with the charging of the electrical double layer at the electrode-solution interface"@en .

[] a owl:Axiom ;
    dcterms:source "International Electrotechnical Commission (IEC), IEC 60050 - International Electrotechnical Vocabulary, retrieved from: https://www.electropedia.org" ;
    owl:annotatedProperty emmo:EMMO_967080e5_2f42_4eb2_a3a9_c58143e835f9 ;
    owl:annotatedSource :electrochemistry_a5962e05_466d_46a4_8951_bea59d7326e5 ;
    owl:annotatedTarget "ratio of the electric charge discharged from a secondary battery to the electric charge provided during the preceding charge"@en .

[] a owl:Axiom ;
    dcterms:source "International Electrotechnical Commission (IEC), IEC 60050 - International Electrotechnical Vocabulary, retrieved from: https://www.electropedia.org" ;
    owl:annotatedProperty emmo:EMMO_967080e5_2f42_4eb2_a3a9_c58143e835f9 ;
    owl:annotatedSource :electrochemistry_a7dc73e2_d4aa_4dfc_8b4d_cb611f1501fb ;
    owl:annotatedTarget "[an indicator of the] electric current at which a secondary cell or battery is charged"@en .

[] a owl:Axiom ;
    dcterms:source "International Electrotechnical Commission (IEC), IEC 60050 - International Electrotechnical Vocabulary, retrieved from: https://www.electropedia.org" ;
    owl:annotatedProperty emmo:EMMO_c7b62dd7_063a_4c2a_8504_42f7264ba83f ;
    owl:annotatedSource :electrochemistry_a7dc73e2_d4aa_4dfc_8b4d_cb611f1501fb ;
    owl:annotatedTarget "the charge rate is expressed as the reference current It = Cr/n where Cr is the rated capacity declared by the manufacturer and n is the time base in hours for which the rated capacity is declared"@en .

[] a owl:Axiom ;
    dcterms:source "J. M. Pingarrón et al., Terminology of electrochemical methods of analysis (IUPAC Recommendations 2019), Pure and Applied Chemistry, 4, 92, 2020, 641-694. https://doi.org/10.1515/pac-2018-0109" ;
    owl:annotatedProperty emmo:EMMO_967080e5_2f42_4eb2_a3a9_c58143e835f9 ;
    owl:annotatedSource :electrochemistry_a82e16c3_b766_482f_be94_b8e9af37f6fc ;
    owl:annotatedTarget "surface area of an electrode that takes into account non-idealities of the interface (roughness, porosity, etc.) and can be measured by a variety of electrochemical methods"@en .

[] a owl:Axiom ;
    dcterms:source "J. M. Pingarrón et al., Terminology of electrochemical methods of analysis (IUPAC Recommendations 2019), Pure and Applied Chemistry, 4, 92, 2020, 641-694. https://doi.org/10.1515/pac-2018-0109" ;
    owl:annotatedProperty emmo:EMMO_967080e5_2f42_4eb2_a3a9_c58143e835f9 ;
    owl:annotatedSource :electrochemistry_abfadc99_6e43_4d37_9b04_7fc5b0f327ae ;
    owl:annotatedTarget "number of electrons transferred in a charge transfer reaction between an electrode and a single entity (ion, radical-ion, or molecule) of an electroactive substance, whose identity must be specified"@en .

[] a owl:Axiom ;
    dcterms:source "Atkins and DePaula, Aktins' Physical Chemistry, 8th ed., p.952" ;
    owl:annotatedProperty emmo:EMMO_967080e5_2f42_4eb2_a3a9_c58143e835f9 ;
    owl:annotatedSource :electrochemistry_1422cde1_929e_46b6_b0dc_1010eebc5dfd ;
    owl:annotatedTarget "the chemical potential of an ion in the presence of an electric potential"@en .

[] a owl:Axiom ;
    dcterms:source "J. M. Pingarrón et al., Terminology of electrochemical methods of analysis (IUPAC Recommendations 2019), Pure and Applied Chemistry, 4, 92, 2020, 641-694. https://doi.org/10.1515/pac-2018-0109" ;
    owl:annotatedProperty emmo:EMMO_967080e5_2f42_4eb2_a3a9_c58143e835f9 ;
    owl:annotatedSource :electrochemistry_ae9882de_d6a2_4525_a84f_80947c10f1cb ;
    owl:annotatedTarget "in chronopotentiometry and related techniques, the duration between the application of current and when the concentration of an electroactive substance at the electrode-solution interface becomes indistinguishable from zero"@en .

[] a owl:Axiom ;
    dcterms:source "J. M. Pingarrón et al., Terminology of electrochemical methods of analysis (IUPAC Recommendations 2019), Pure and Applied Chemistry, 4, 92, 2020, 641-694. https://doi.org/10.1515/pac-2018-0109" ;
    owl:annotatedProperty emmo:EMMO_967080e5_2f42_4eb2_a3a9_c58143e835f9 ;
    owl:annotatedSource :electrochemistry_b21de1ef_6c15_4d63_b320_c9b96fbf186f ;
    owl:annotatedTarget "equilibrium electrode potential under conditions of unit concentration of species involved in the electrode reaction"@en .

[] a owl:Axiom ;
    dcterms:source "International Electrotechnical Commission (IEC), IEC 60050 - International Electrotechnical Vocabulary, retrieved from: https://www.electropedia.org" ;
    owl:annotatedProperty emmo:EMMO_967080e5_2f42_4eb2_a3a9_c58143e835f9 ;
    owl:annotatedSource :electrochemistry_bad1b6f4_1b26_40e2_b552_6d53873e3973 ;
    owl:annotatedTarget "the area of the electrode material that is accessible to the electrolyte that is used for charge transfer and/or storage"@en .

[] a owl:Axiom ;
    dcterms:source "International Electrotechnical Commission (IEC), IEC 60050 - International Electrotechnical Vocabulary, retrieved from: https://www.electropedia.org" ;
    owl:annotatedProperty emmo:EMMO_967080e5_2f42_4eb2_a3a9_c58143e835f9 ;
    owl:annotatedSource :electrochemistry_bcb33f7e_5573_4bc2_b636_4ea313a9dd3a ;
    owl:annotatedTarget "quotient of the capacity of a battery cell or battery by its plane area."@en .

[] a owl:Axiom ;
    dcterms:source "J. M. Pingarrón et al., Terminology of electrochemical methods of analysis (IUPAC Recommendations 2019), Pure and Applied Chemistry, 4, 92, 2020, 641-694. https://doi.org/10.1515/pac-2018-0109" ;
    owl:annotatedProperty emmo:EMMO_967080e5_2f42_4eb2_a3a9_c58143e835f9 ;
    owl:annotatedSource :electrochemistry_c39b2498_783e_48e1_9814_6164bd99823c ;
    owl:annotatedTarget "range of electrode potentials of a given working electrode in a given electrolyte, where the electric current from reactions of the electrode or electrolyte is negligible compared with the current from reactions of the system under investigation"@en .

[] a owl:Axiom ;
    dcterms:source "J. M. Pingarrón et al., Terminology of electrochemical methods of analysis (IUPAC Recommendations 2019), Pure and Applied Chemistry, 4, 92, 2020, 641-694. https://doi.org/10.1515/pac-2018-0109" ;
    owl:annotatedProperty emmo:EMMO_967080e5_2f42_4eb2_a3a9_c58143e835f9 ;
    owl:annotatedSource :electrochemistry_c4d551db_db17_4c33_92e6_aec71638afbc ;
    owl:annotatedTarget "for dynamic voltammetric techniques, the electric potential of the working electrode at which the current is equal to one-half of the peak current"@en .

[] a owl:Axiom ;
    dcterms:source "J. M. Pingarrón et al., Terminology of electrochemical methods of analysis (IUPAC Recommendations 2019), Pure and Applied Chemistry, 4, 92, 2020, 641-694. https://doi.org/10.1515/pac-2018-0109" ;
    owl:annotatedProperty emmo:EMMO_967080e5_2f42_4eb2_a3a9_c58143e835f9 ;
    owl:annotatedSource :electrochemistry_c55bcb85_b7b8_4e67_8a78_9a42fe25b6cf ;
    owl:annotatedTarget "faradaic current measured in a solution containing two electroactive substances, A and B, that exceeds the sum of the faradaic currents that would be obtained for A and B separately under the same experimental conditions"@en .

[] a owl:Axiom ;
    dcterms:source "International Electrotechnical Commission (IEC), IEC 60050 - International Electrotechnical Vocabulary, retrieved from: https://www.electropedia.org" ;
    owl:annotatedProperty emmo:EMMO_967080e5_2f42_4eb2_a3a9_c58143e835f9 ;
    owl:annotatedSource :electrochemistry_c7b26177_21bf_4787_b656_8e78edf27f88 ;
    owl:annotatedTarget "voltage between the terminals of a cell or battery when being discharged"@en .

