@prefix : <https://w3id.org/emmo/domain/electrochemistry#> .
@prefix bibo: <http://purl.org/ontology/bibo/> .
@prefix chems: <https://w3id.org/emmo/domain/chemical-substance#> .
@prefix dcterms: <http://purl.org/dc/terms/> .
@prefix emmo: <https://w3id.org/emmo#> .
@prefix foaf: <http://xmlns.com/foaf/0.1/> .
@prefix owl: <http://www.w3.org/2002/07/owl#> .
@prefix rdfs: <http://www.w3.org/2000/01/rdf-schema#> .
@prefix schema: <https://schema.org/> .
@prefix skos: <http://www.w3.org/2004/02/skos/core#> .
@prefix vann: <http://purl.org/vocab/vann/> .
@prefix xsd: <http://www.w3.org/2001/XMLSchema#> .

skos:related a owl:AnnotationProperty .

schema:additionalName a owl:AnnotationProperty .

schema:familyName a owl:AnnotationProperty .

schema:givenName a owl:AnnotationProperty .

schema:name a owl:AnnotationProperty .

emmo:EMMO_4207e895_8b83_4318_996a_72cfb32acd94 rdfs:subClassOf [ a owl:Restriction ;
            owl:onProperty emmo:EMMO_e1097637_70d2_4895_973f_2396f04fa204 ;
            owl:someValuesFrom emmo:EMMO_06448f64_8db6_4304_8b2c_e785dba82044 ],
        [ a owl:Restriction ;
            owl:onProperty emmo:EMMO_e1097637_70d2_4895_973f_2396f04fa204 ;
            owl:someValuesFrom emmo:EMMO_8dd40ec6_2c5a_43f3_bf64_cadcd447a1c1 ],
        [ a owl:Restriction ;
            owl:onProperty emmo:EMMO_e1097637_70d2_4895_973f_2396f04fa204 ;
            owl:someValuesFrom emmo:EMMO_b4f4ed28_d24c_4a00_9583_62ab839abeca ],
        [ a owl:Restriction ;
            owl:onProperty emmo:EMMO_e1097637_70d2_4895_973f_2396f04fa204 ;
            owl:someValuesFrom :electrochemistry_ce74d2dc_d496_4116_b2fb_3e83d88bc744 ] .

emmo:EMMO_472a0ca2_58bf_4618_b561_6fe68bd9fd49 rdfs:subClassOf [ a owl:Restriction ;
            owl:onProperty emmo:EMMO_08bd340b_9d49_4d60_8ac5_b89f2f442169 ;
            owl:someValuesFrom emmo:EMMO_b7bcff25_ffc3_474e_9ab5_01b1664bd4ba ] .

emmo:EMMO_82fc8506_1f84_4add_9683_abea077bd1e3 rdfs:subClassOf [ a owl:Restriction ;
            owl:onProperty emmo:EMMO_e1097637_70d2_4895_973f_2396f04fa204 ;
            owl:someValuesFrom emmo:EMMO_ed4af7ae_63a2_497e_bb88_2309619ea405 ],
        [ a owl:Restriction ;
            owl:onProperty emmo:EMMO_e1097637_70d2_4895_973f_2396f04fa204 ;
            owl:someValuesFrom emmo:EMMO_f1a51559_aa3d_43a0_9327_918039f0dfed ] .

emmo:EMMO_ec2c8ac8_98c5_4c74_b85b_ff8e8ca6655c rdfs:subClassOf [ a owl:Restriction ;
            owl:onProperty emmo:EMMO_dba27ca1_33c9_4443_a912_1519ce4c39ec ;
            owl:someValuesFrom emmo:EMMO_bc37743c_37c4_4ec7_9d58_d1aae5567352 ] .

:electrochemistry_027d437e_3bbf_4eda_940b_e509f8d2b993 a owl:Class ;
    rdfs:label "R416"@en ;
    rdfs:comment "a coin case with a nominal diameter of 4.8 mm and a height of 1.6 mm"@en ;
    rdfs:subClassOf :electrochemistry_3979cd56_6256_414d_966c_7f723bf71e37 ;
    skos:prefLabel "R416"@en ;
    emmo:EMMO_967080e5_2f42_4eb2_a3a9_c58143e835f9 "a coin case with a nominal diameter of 4.8 mm and a height of 1.6 mm"@en .

:electrochemistry_028069a2_4e03_409e_8af2_4c8df32b5c5e a owl:Class ;
    rdfs:label "R754"@en ;
    rdfs:comment "a coin case with a nominal diameter of 7.9 mm and a height of 5.4 mm"@en ;
    rdfs:subClassOf :electrochemistry_3979cd56_6256_414d_966c_7f723bf71e37 ;
    skos:altLabel "R48" ;
    skos:prefLabel "R754"@en ;
    emmo:EMMO_967080e5_2f42_4eb2_a3a9_c58143e835f9 "a coin case with a nominal diameter of 7.9 mm and a height of 5.4 mm"@en .

:electrochemistry_0689e6fc_cda7_4e04_b1eb_41459a0a4736 a owl:Class ;
    rdfs:label "R2325"@en ;
    rdfs:comment "a coin cell case with a nominal diameter of 23.0 mm and a height of 2.5 mm"@en ;
    rdfs:subClassOf :electrochemistry_3979cd56_6256_414d_966c_7f723bf71e37 ;
    skos:altLabel "R23/3"@en ;
    skos:prefLabel "R2325"@en ;
    emmo:EMMO_967080e5_2f42_4eb2_a3a9_c58143e835f9 "a coin cell case with a nominal diameter of 23.0 mm and a height of 2.5 mm"@en .

:electrochemistry_06db7d9e_d224_4360_b926_734f0349d396 a owl:Class ;
    rdfs:label "R726" ;
    rdfs:comment "a coin case with a nominal diameter of 7.9 mm and a height of 2.6 mm"@en ;
    rdfs:subClassOf :electrochemistry_3979cd56_6256_414d_966c_7f723bf71e37 ;
    skos:altLabel "R59" ;
    skos:prefLabel "R726" ;
    emmo:EMMO_967080e5_2f42_4eb2_a3a9_c58143e835f9 "a coin case with a nominal diameter of 7.9 mm and a height of 2.6 mm"@en .

:electrochemistry_098690e3_9010_437e_8042_cee1656efa9b a owl:Class ;
    rdfs:label "LithiumNickelManganeseCobaltOxideLithiumCobaltOxideElectrode"@en ;
    rdfs:comment "an electrode with blended lithium nickel manganese cobalt oxide (NMC) and lithium cobalt oxide (LCO) active materials"@en ;
    rdfs:subClassOf [ a owl:Restriction ;
            owl:onProperty :electrochemistry_860aa941_5ff9_4452_8a16_7856fad07bee ;
            owl:someValuesFrom chems:substance_3ac62305_acd6_4312_9e31_4f824bd2530d ],
        [ a owl:Restriction ;
            owl:onProperty :electrochemistry_860aa941_5ff9_4452_8a16_7856fad07bee ;
            owl:someValuesFrom chems:substance_4c62d334_a124_40b3_9fd1_fe713d01a6af ],
        :electrochemistry_4839708a_3864_47eb_b719_373ff8874c61 ;
    owl:deprecated true ;
    skos:altLabel "NMCLCOElectrode"@en ;
    skos:prefLabel "LithiumNickelManganeseCobaltOxideLithiumCobaltOxideElectrode"@en ;
    emmo:EMMO_967080e5_2f42_4eb2_a3a9_c58143e835f9 "an electrode with blended lithium nickel manganese cobalt oxide (NMC) and lithium cobalt oxide (LCO) active materials"@en .

:electrochemistry_0a5038d4_24af_4ea8_8d56_a156faeb98e2 a owl:Class ;
    rdfs:label "R521" ;
    rdfs:comment "a coin case with a nominal diameter of 5.8 mm and a height of 2.1 mm"@en ;
    rdfs:subClassOf :electrochemistry_3979cd56_6256_414d_966c_7f723bf71e37 ;
    skos:altLabel "R63" ;
    skos:prefLabel "R521" ;
    emmo:EMMO_967080e5_2f42_4eb2_a3a9_c58143e835f9 "a coin case with a nominal diameter of 5.8 mm and a height of 2.1 mm"@en .

:electrochemistry_0ac306fd_e98b_4af9_8cd6_5ed34f7f7d8a a owl:ObjectProperty ;
    rdfs:label "hasAnolyte"@en ;
    rdfs:comment "relates a system to the portion of the electrolyte that is in contact with the anode"@en ;
    rdfs:range :electrochemistry_fb0d9eef_92af_4628_8814_e065ca255d59 ;
    rdfs:subPropertyOf :electrochemistry_3bd08946_4e81_455d_9fca_dc7a5ead9315 ;
    skos:prefLabel "hasAnolyte"@en ;
    emmo:EMMO_967080e5_2f42_4eb2_a3a9_c58143e835f9 "relates a system to the portion of the electrolyte that is in contact with the anode"@en .

:electrochemistry_0afe79ed_dc0d_4b3e_88fa_ae0c7b1e88b5 a owl:Class ;
    rdfs:label "PotassiumBasedElectrode"@en ;
    rdfs:comment "an electrode in which the primary active material consists of potassium or potassium compounds"@en ;
    rdfs:subClassOf :electrochemistry_9a823d64_9d10_4a29_9cbd_9bbdad7985bc ;
    skos:prefLabel "PotassiumBasedElectrode"@en ;
    emmo:EMMO_967080e5_2f42_4eb2_a3a9_c58143e835f9 "an electrode in which the primary active material consists of potassium or potassium compounds"@en .

:electrochemistry_0c09df01_b251_4f75_b6e3_2578ba1a10c9 a owl:Class ;
    rdfs:label "R736" ;
    rdfs:comment "a coin case with a nominal diameter of 7.9 mm and a height of 3.6 mm"@en ;
    rdfs:subClassOf :electrochemistry_3979cd56_6256_414d_966c_7f723bf71e37 ;
    skos:altLabel "R41" ;
    skos:prefLabel "R736" ;
    emmo:EMMO_967080e5_2f42_4eb2_a3a9_c58143e835f9 "a coin case with a nominal diameter of 7.9 mm and a height of 3.6 mm"@en .

:electrochemistry_0d9ba00d_04bc_4bdc_85af_3380694f6f68 a owl:Class ;
    rdfs:label "ReversibleHydrogenElectrode"@en ;
    rdfs:comment "a practical hydrogen electrode whose potential depends on the pH of the solution"@en ;
    rdfs:subClassOf :electrochemistry_7729c34e_1ae9_403d_b933_1765885e7f29 ;
    skos:prefLabel "ReversibleHydrogenElectrode"@en ;
    emmo:EMMO_26bf1bef_d192_4da6_b0eb_d2209698fb54 "https://www.wikidata.org/wiki/Q900576" ;
    emmo:EMMO_967080e5_2f42_4eb2_a3a9_c58143e835f9 "a practical hydrogen electrode whose potential depends on the pH of the solution"@en ;
    emmo:EMMO_c84c6752_6d64_48cc_9500_e54a3c34898d "https://en.wikipedia.org/wiki/Reversible_hydrogen_electrode"@en .

:electrochemistry_0e366263_fded_4509_bddd_392d839013e4 a owl:Class ;
    rdfs:label "P21148128" ;
    rdfs:comment "a prismatic case with a nominal length of 21 mm, width of 148 mm, and height of 128 mm"@en ;
    rdfs:subClassOf :electrochemistry_43cd6e14_dd43_41b5_b5b4_344d53841603 ;
    skos:altLabel "P21/148/128" ;
    skos:prefLabel "P21148128" ;
    emmo:EMMO_967080e5_2f42_4eb2_a3a9_c58143e835f9 "a prismatic case with a nominal length of 21 mm, width of 148 mm, and height of 128 mm"@en .

:electrochemistry_103c9e6c_9c26_430a_9fb9_f4f041e970b0 a owl:Class ;
    rdfs:label "SodiumMetatitanateElectrode"@en ;
    rdfs:comment "electrode in which the active material is sodium metatitanate"@en ;
    rdfs:subClassOf :electrochemistry_9c557caa_61e2_4fa9_a517_4bad01a68122,
        :electrochemistry_e4b6cb36_4dac_49e3_871d_40bcfca943a5 ;
    owl:deprecated true ;
    skos:prefLabel "SodiumMetatitanateElectrode"@en ;
    emmo:EMMO_967080e5_2f42_4eb2_a3a9_c58143e835f9 "electrode in which the active material is sodium metatitanate"@en .

:electrochemistry_10a91aba_da41_4309_a926_ddc0f285c2c1 a owl:Class ;
    rdfs:label "RutheniumOxideElectrode"@en ;
    rdfs:comment "electrode in which the active material is ruthenium oxide"@en ;
    rdfs:subClassOf :electrochemistry_e4b6cb36_4dac_49e3_871d_40bcfca943a5 ;
    owl:deprecated true ;
    skos:altLabel "RuO2Electrode"@en ;
    skos:prefLabel "RutheniumOxideElectrode"@en ;
    emmo:EMMO_967080e5_2f42_4eb2_a3a9_c58143e835f9 "electrode in which the active material is ruthenium oxide"@en .

:electrochemistry_11579b47_cbf8_45ac_aed3_343ea533b346 a owl:Class ;
    rdfs:label "R2330" ;
    rdfs:comment "a coin case with a nominal diameter of 23.0 mm and a height of 3.0 mm"@en ;
    rdfs:subClassOf :electrochemistry_3979cd56_6256_414d_966c_7f723bf71e37 ;
    skos:prefLabel "R2330" ;
    emmo:EMMO_967080e5_2f42_4eb2_a3a9_c58143e835f9 "a coin case with a nominal diameter of 23.0 mm and a height of 3.0 mm"@en .

:electrochemistry_11a774f3_d20a_4741_bd81_cae53230bd0c a owl:Class ;
    rdfs:label "ProtonInsertionElectrode"@en ;
    rdfs:comment "an insertion electrode in which the guest molecule is a proton (hydrogen)"@en ;
    rdfs:subClassOf :electrochemistry_757eae08_4d43_42d4_8b4e_8a0bfd2f9a1c ;
    owl:deprecated true ;
    skos:prefLabel "ProtonInsertionElectrode"@en ;
    emmo:EMMO_967080e5_2f42_4eb2_a3a9_c58143e835f9 "an insertion electrode in which the guest molecule is a proton (hydrogen)"@en .

:electrochemistry_11e9f765_4fea_456b_bd8e_4624b9c752ae a owl:Class ;
    rdfs:label "R2430" ;
    rdfs:comment "a coin case with a nominal diameter of 24.5 mm and a height of 3.0 mm"@en ;
    rdfs:subClassOf :electrochemistry_3979cd56_6256_414d_966c_7f723bf71e37 ;
    skos:prefLabel "R2430" ;
    emmo:EMMO_967080e5_2f42_4eb2_a3a9_c58143e835f9 "a coin case with a nominal diameter of 24.5 mm and a height of 3.0 mm"@en .

:electrochemistry_14377ecb_5ead_431e_831e_159d622bd0ea a owl:Class ;
    rdfs:label "RectangularElectrode"@en ;
    rdfs:comment "an electrode in the shape of a rectangle"@en ;
    rdfs:subClassOf [ a owl:Restriction ;
            owl:onProperty emmo:EMMO_e1097637_70d2_4895_973f_2396f04fa204 ;
            owl:someValuesFrom emmo:EMMO_cd2cd0de_e0cc_4ef1_b27e_2e88db027bac ],
        [ a owl:Restriction ;
            owl:onProperty emmo:EMMO_e1097637_70d2_4895_973f_2396f04fa204 ;
            owl:someValuesFrom emmo:EMMO_e4de48b1_dabb_4490_ac2b_040f926c64f0 ],
        :electrochemistry_0f007072_a8dd_4798_b865_1bf9363be627 ;
    skos:prefLabel "RectangularElectrode"@en ;
    emmo:EMMO_967080e5_2f42_4eb2_a3a9_c58143e835f9 "an electrode in the shape of a rectangle"@en .

:electrochemistry_15ec346a_6d3c_4161_95e1_9cf889965f85 a owl:Class ;
    rdfs:label "R621" ;
    rdfs:comment "a coin case with a nominal diameter of 6.8 mm and a height of 2.1 mm"@en ;
    rdfs:subClassOf :electrochemistry_3979cd56_6256_414d_966c_7f723bf71e37 ;
    skos:altLabel "R60" ;
    skos:prefLabel "R621" ;
    emmo:EMMO_967080e5_2f42_4eb2_a3a9_c58143e835f9 "a coin case with a nominal diameter of 6.8 mm and a height of 2.1 mm"@en .

:electrochemistry_169fb6e4_cbed_4b00_ace0_8731123a35b4 a owl:Class ;
    rdfs:label "R38138" ;
    rdfs:comment "a cylindrical case with a nominal diameter of 38 mm and height of 138 mm"@en ;
    rdfs:subClassOf :electrochemistry_b1cf9fee_2164_4f95_8204_90f717373a8a ;
    skos:altLabel "R38/138" ;
    skos:prefLabel "R38138" ;
    emmo:EMMO_967080e5_2f42_4eb2_a3a9_c58143e835f9 "a cylindrical case with a nominal diameter of 38 mm and height of 138 mm"@en .

:electrochemistry_1afa2c7e_6ddd_4a9b_9623_40975131a304 a owl:Class ;
    rdfs:label "R46800" ;
    rdfs:comment "a cylindrical case with a nominal diameter of 46 mm and height of 80 mm"@en ;
    rdfs:subClassOf :electrochemistry_b1cf9fee_2164_4f95_8204_90f717373a8a ;
    skos:altLabel "R46/80",
        "R4680" ;
    skos:prefLabel "R46800" ;
    emmo:EMMO_967080e5_2f42_4eb2_a3a9_c58143e835f9 "a cylindrical case with a nominal diameter of 46 mm and height of 80 mm"@en .

:electrochemistry_1c0c8f43_7349_4646_94e3_c36727c5c2e3 a owl:Class ;
    rdfs:label "Seawater"@en ;
    rdfs:comment "a naturally occuring solution of salts (mostly NaCl) dissolved in water"@en ;
    rdfs:subClassOf :electrochemistry_dc205ac2_314e_415c_a2b6_b12e8359d54c ;
    skos:prefLabel "Seawater"@en ;
    emmo:EMMO_967080e5_2f42_4eb2_a3a9_c58143e835f9 "a naturally occuring solution of salts (mostly NaCl) dissolved in water"@en .

:electrochemistry_1c530688_ee63_4683_b38f_80cce7ca75c1 a owl:Class ;
    rdfs:label "CarbonFelt"@en ;
    rdfs:comment "a non-woven mat of randomly oriented carbon fibers, providing excellent thermal insulation, chemical resistance, and high surface area for various industrial and electrochemical applications"@en ;
    rdfs:subClassOf emmo:EMMO_ec7464a9_d99d_45f8_965b_4e9230ea8356 ;
    skos:prefLabel "CarbonFelt"@en ;
    emmo:EMMO_967080e5_2f42_4eb2_a3a9_c58143e835f9 "a non-woven mat of randomly oriented carbon fibers, providing excellent thermal insulation, chemical resistance, and high surface area for various industrial and electrochemical applications"@en .

:electrochemistry_1c6cef85_811f_45d0_a0fd_2bc2d9369ea4 a owl:Class ;
    rdfs:label "AluminiumInsertionElectrode"@en ;
    rdfs:comment "an insertion electrode in which the guest molecule is aluminium"@en ;
    rdfs:subClassOf :electrochemistry_757eae08_4d43_42d4_8b4e_8a0bfd2f9a1c ;
    owl:deprecated true ;
    skos:prefLabel "AluminiumInsertionElectrode"@en ;
    emmo:EMMO_967080e5_2f42_4eb2_a3a9_c58143e835f9 "an insertion electrode in which the guest molecule is aluminium"@en .

:electrochemistry_1d0f15cb_d6b5_4c27_89ca_fe78adc1ce5b a owl:Class ;
    rdfs:label "LithiumIronPhosphateElectrode"@en ;
    rdfs:comment "electrode in which the active material is lithium iron phosphate"@en ;
    rdfs:subClassOf [ a owl:Restriction ;
            owl:onProperty :electrochemistry_860aa941_5ff9_4452_8a16_7856fad07bee ;
            owl:someValuesFrom chems:substance_aa8e9cc4_5f66_4307_b1c8_26fac7653a90 ],
        :electrochemistry_d54f6aac_7cd2_4d52_9bca_2f19bb1eaec4,
        :electrochemistry_e4b6cb36_4dac_49e3_871d_40bcfca943a5 ;
    owl:deprecated true ;
    skos:altLabel "LFPElectrode"@en ;
    skos:prefLabel "LithiumIronPhosphateElectrode"@en ;
    emmo:EMMO_967080e5_2f42_4eb2_a3a9_c58143e835f9 "electrode in which the active material is lithium iron phosphate"@en .

:electrochemistry_1d5377a7_9f2b_4fdf_958a_7eeadce158d6 a owl:Class ;
    rdfs:label "Foil"@en ;
    rdfs:comment "a sheet of material in which the thickness is much smaller than the length and width"@en ;
    rdfs:subClassOf emmo:EMMO_ec7464a9_d99d_45f8_965b_4e9230ea8356 ;
    skos:prefLabel "Foil"@en ;
    emmo:EMMO_967080e5_2f42_4eb2_a3a9_c58143e835f9 "a sheet of material in which the thickness is much smaller than the length and width"@en .

:electrochemistry_21eef598_0799_4cb1_b2d5_6e072a8579a3 a owl:Class ;
    rdfs:label "R1136" ;
    rdfs:comment "a coin case with a nominal diameter of 11.6 mm and a height of 3.6 mm"@en ;
    rdfs:subClassOf :electrochemistry_3979cd56_6256_414d_966c_7f723bf71e37 ;
    skos:altLabel "R42" ;
    skos:prefLabel "R1136" ;
    emmo:EMMO_967080e5_2f42_4eb2_a3a9_c58143e835f9 "a coin case with a nominal diameter of 11.6 mm and a height of 3.6 mm"@en .

:electrochemistry_23b30468_be7b_45a9_bc11_a8219bc3ab8b a owl:Class ;
    rdfs:label "LeclancheElectrolyte"@en ;
    rdfs:comment "an aqueous mixture of ammonium chloride and zinc chloride"@en ;
    rdfs:subClassOf :electrochemistry_dc205ac2_314e_415c_a2b6_b12e8359d54c ;
    skos:prefLabel "LeclancheElectrolyte"@en ;
    emmo:EMMO_967080e5_2f42_4eb2_a3a9_c58143e835f9 "an aqueous mixture of ammonium chloride and zinc chloride"@en .

:electrochemistry_245c9442_ca1d_4070_a624_182b92d30b10 a owl:Class ;
    rdfs:label "ZincInsertionElectrode"@en ;
    rdfs:comment "an insertion electrode in which the guest molecule is zinc"@en ;
    rdfs:subClassOf :electrochemistry_757eae08_4d43_42d4_8b4e_8a0bfd2f9a1c ;
    owl:deprecated true ;
    skos:prefLabel "ZincInsertionElectrode"@en ;
    emmo:EMMO_967080e5_2f42_4eb2_a3a9_c58143e835f9 "an insertion electrode in which the guest molecule is zinc"@en .

:electrochemistry_2522cbd8_5382_457f_b9b5_775860f83357 a owl:Class ;
    rdfs:label "Coin"@en ;
    rdfs:comment "a form factor describing a coin cell, which is a cylindrical cell where the height is less than the diameter"@en ;
    rdfs:subClassOf :electrochemistry_1586ef26_6d30_49e3_ae32_b4c9fc181941 ;
    skos:prefLabel "Coin"@en ;
    emmo:EMMO_967080e5_2f42_4eb2_a3a9_c58143e835f9 "a form factor describing a coin cell, which is a cylindrical cell where the height is less than the diameter"@en .

:electrochemistry_26a0dc36_8171_4a84_88dd_0f5dd7cb2d20 a owl:Class ;
    rdfs:label "PotassiumHydroxideSolution"@en ;
    rdfs:comment "a solution of potassium hydroxide (KOH) dissolved in water (H2O)"@en ;
    rdfs:subClassOf :electrochemistry_615cff2a_be95_4e65_9471_98db23f4c878 ;
    owl:deprecated true ;
    skos:altLabel "AqueousPotassiumHydroxideSolution"@en,
        "KOHSolution"@en ;
    skos:prefLabel "PotassiumHydroxideSolution"@en ;
    emmo:EMMO_967080e5_2f42_4eb2_a3a9_c58143e835f9 "a solution of potassium hydroxide (KOH) dissolved in water (H2O)"@en .

:electrochemistry_27f95593_47f1_4494_b6bb_ac0733df185d a owl:Class ;
    rdfs:label "P12103310" ;
    rdfs:comment "a prismatic case with a nominal length of 12 mm, width of 103 mm, and height of 310 mm"@en ;
    rdfs:subClassOf :electrochemistry_43cd6e14_dd43_41b5_b5b4_344d53841603 ;
    skos:altLabel "P12/103/310" ;
    skos:prefLabel "P12103310" ;
    emmo:EMMO_967080e5_2f42_4eb2_a3a9_c58143e835f9 "a prismatic case with a nominal length of 12 mm, width of 103 mm, and height of 310 mm"@en .

:electrochemistry_289da03d_606a_4668_a195_e81627bc80b7 a owl:Class ;
    rdfs:label "P1865140" ;
    rdfs:comment "a prismatic case with a nominal length of 18 mm, width of 65 mm, and height of 140 mm"@en ;
    rdfs:subClassOf :electrochemistry_43cd6e14_dd43_41b5_b5b4_344d53841603 ;
    skos:altLabel "P18/65/140" ;
    skos:prefLabel "P1865140" ;
    emmo:EMMO_967080e5_2f42_4eb2_a3a9_c58143e835f9 "a prismatic case with a nominal length of 18 mm, width of 65 mm, and height of 140 mm"@en .

:electrochemistry_296b95b0_c4cb_45db_a8ca_f638379870c4 a owl:Class ;
    rdfs:label "R1220" ;
    rdfs:comment "a coin case with a nominal diameter of 12.5 mm and a height of 2.0 mm"@en ;
    rdfs:subClassOf :electrochemistry_3979cd56_6256_414d_966c_7f723bf71e37 ;
    skos:prefLabel "R1220" ;
    emmo:EMMO_967080e5_2f42_4eb2_a3a9_c58143e835f9 "a coin case with a nominal diameter of 12.5 mm and a height of 2.0 mm"@en .

:electrochemistry_2a177462_ff01_4b83_ab9f_032e93c9ec69 a owl:Class ;
    rdfs:label "MagnesiumBasedElectrode"@en ;
    rdfs:comment "an electrode in which the primary active material consists of magnesium or magnesium compounds"@en ;
    rdfs:subClassOf :electrochemistry_9a823d64_9d10_4a29_9cbd_9bbdad7985bc ;
    skos:prefLabel "MagnesiumBasedElectrode"@en ;
    emmo:EMMO_967080e5_2f42_4eb2_a3a9_c58143e835f9 "an electrode in which the primary active material consists of magnesium or magnesium compounds"@en .

:electrochemistry_2c63d7f4_09ba_4ca9_baa2_a1da899bf477 a owl:Class ;
    rdfs:label "P45173225" ;
    rdfs:comment "a prismatic case with a nominal length of 45 mm, width of 173 mm, and height of 225 mm"@en ;
    rdfs:subClassOf :electrochemistry_43cd6e14_dd43_41b5_b5b4_344d53841603 ;
    skos:altLabel "BEV4",
        "P45/173/225" ;
    skos:prefLabel "P45173225" ;
    emmo:EMMO_967080e5_2f42_4eb2_a3a9_c58143e835f9 "a prismatic case with a nominal length of 45 mm, width of 173 mm, and height of 225 mm"@en .

:electrochemistry_2fd5964b_0c65_4413_8b8c_849639e6d1e7 a owl:Class ;
    rdfs:label "SiliconOxideGraphiteElectrode"@en ;
    rdfs:comment "an electrode with blended silicon oxide and graphite active materials"@en ;
    rdfs:subClassOf [ a owl:Restriction ;
            owl:onProperty :electrochemistry_860aa941_5ff9_4452_8a16_7856fad07bee ;
            owl:someValuesFrom chems:substance_d53259a7_0d9c_48b9_a6c1_4418169df303 ],
        :electrochemistry_5186239a_2af7_4dbf_92ca_22e8e583c528 ;
    owl:deprecated true ;
    skos:prefLabel "SiliconOxideGraphiteElectrode"@en ;
    emmo:EMMO_967080e5_2f42_4eb2_a3a9_c58143e835f9 "an electrode with blended silicon oxide and graphite active materials"@en .

:electrochemistry_30c8fb1b_3c75_49f5_9395_c15dfaf71b12 a owl:Class ;
    rdfs:label "R2016" ;
    rdfs:comment "a coin case with a nominal diameter of 20.0 mm and a height of 1.6 mm"@en ;
    rdfs:subClassOf :electrochemistry_3979cd56_6256_414d_966c_7f723bf71e37 ;
    skos:prefLabel "R2016" ;
    emmo:EMMO_967080e5_2f42_4eb2_a3a9_c58143e835f9 "a coin case with a nominal diameter of 20.0 mm and a height of 1.6 mm"@en ;
    emmo:EMMO_c7b62dd7_063a_4c2a_8504_42f7264ba83f "often used in wrist watches"@en .

:electrochemistry_31b38a1b_5873_454c_ba99_00491497fb43 a owl:Class ;
    rdfs:label "ExpandedMesh"@en ;
    rdfs:comment "a sheet that has been slit and stretched to form a network of diamond-shaped openings, providing structural strength and high surface area for applications like filtration and reinforcement"@en ;
    rdfs:subClassOf emmo:EMMO_ec7464a9_d99d_45f8_965b_4e9230ea8356 ;
    skos:prefLabel "ExpandedMesh"@en ;
    emmo:EMMO_967080e5_2f42_4eb2_a3a9_c58143e835f9 "a sheet that has been slit and stretched to form a network of diamond-shaped openings, providing structural strength and high surface area for applications like filtration and reinforcement"@en .

:electrochemistry_31b7ac6a_b1eb_45e7_a075_b6063080c949 a owl:Class ;
    rdfs:label "R1121" ;
    rdfs:comment "a coin case with a nominal diameter of 11.6 mm and a height of 2.1 mm"@en ;
    rdfs:subClassOf :electrochemistry_3979cd56_6256_414d_966c_7f723bf71e37 ;
    skos:altLabel "R55" ;
    skos:prefLabel "R1121" ;
    emmo:EMMO_967080e5_2f42_4eb2_a3a9_c58143e835f9 "a coin case with a nominal diameter of 11.6 mm and a height of 2.1 mm"@en .

:electrochemistry_3279f575_1c62_4bf2_a6e8_de4c7ff36f8e a owl:Class ;
    rdfs:label "R721" ;
    rdfs:comment "a coin case with a nominal diameter of 7.9 mm and a height of 2.1 mm"@en ;
    rdfs:subClassOf :electrochemistry_3979cd56_6256_414d_966c_7f723bf71e37 ;
    skos:altLabel "R58" ;
    skos:prefLabel "R721" ;
    emmo:EMMO_967080e5_2f42_4eb2_a3a9_c58143e835f9 "a coin case with a nominal diameter of 7.9 mm and a height of 2.1 mm"@en .

:electrochemistry_334b3acd_e35d_4d5a_b8b5_6d13cbebbc57 a owl:Class ;
    rdfs:label "SulfuricAcidSolution"@en ;
    rdfs:comment "a solution of sulfuric acid (H2SO4) dissolved in water (H2O)"@en ;
    rdfs:subClassOf :electrochemistry_6592d8cc_4ce4_42ca_b010_6bfc4a8444d2 ;
    owl:deprecated true ;
    skos:prefLabel "SulfuricAcidSolution"@en ;
    emmo:EMMO_967080e5_2f42_4eb2_a3a9_c58143e835f9 "a solution of sulfuric acid (H2SO4) dissolved in water (H2O)"@en .

:electrochemistry_339e1ba1_2006_4f22_aac4_3ce75edf1088 a owl:Class ;
    rdfs:label "FluorineDopedTinOxideElectrode"@en ;
    rdfs:comment "electrode in which the active material is tin oxide doped with fluorine"@en ;
    rdfs:subClassOf [ a owl:Restriction ;
            owl:onProperty :electrochemistry_860aa941_5ff9_4452_8a16_7856fad07bee ;
            owl:someValuesFrom chems:substance_db74b6b7_09fc_40db_a7d5_6eb86b69192a ],
        :electrochemistry_e4b6cb36_4dac_49e3_871d_40bcfca943a5 ;
    owl:deprecated true ;
    skos:altLabel "FTOElectrode"@en ;
    skos:prefLabel "FluorineDopedTinOxideElectrode"@en ;
    emmo:EMMO_967080e5_2f42_4eb2_a3a9_c58143e835f9 "electrode in which the active material is tin oxide doped with fluorine"@en .

:electrochemistry_344ed3a6_481a_499f_afef_631f1cece9ef a owl:Class ;
    rdfs:label "NickelOxideHydroxideElectrode"@en ;
    rdfs:comment "an electrode in which the primary active material consists of nickel oxide hydroxide or nickel oxide hydroxide compounds."@en ;
    rdfs:subClassOf [ a owl:Restriction ;
            owl:onProperty :electrochemistry_860aa941_5ff9_4452_8a16_7856fad07bee ;
            owl:someValuesFrom chems:substance_7dc738d6_74f2_489e_ae84_a6dbdf627f2e ],
        :electrochemistry_0d2aaaf4_1a8a_4a32_abd8_7d0fdf0ae9d2,
        :electrochemistry_e4b6cb36_4dac_49e3_871d_40bcfca943a5 ;
    skos:altLabel "NiOOHElectrode"@en,
        "NickelOxyhydroxideElectrode"@en ;
    skos:prefLabel "NickelOxideHydroxideElectrode"@en ;
    emmo:EMMO_967080e5_2f42_4eb2_a3a9_c58143e835f9 "an electrode in which the primary active material consists of nickel oxide hydroxide or nickel oxide hydroxide compounds."@en ;
    emmo:EMMO_c7b62dd7_063a_4c2a_8504_42f7264ba83f "the combination with zinc metal and an alkali metal hydoxide electrolyte is designated using IEC electrochemical system letter code Z"@en .

:electrochemistry_34cb7ea7_2436_46e0_806e_a3c7835ae228 a owl:Class ;
    rdfs:label "R716" ;
    rdfs:comment "a coin case with a nominal diameter of 7.9 mm and a height of 1.65 mm"@en ;
    rdfs:subClassOf :electrochemistry_3979cd56_6256_414d_966c_7f723bf71e37 ;
    skos:altLabel "R67" ;
    skos:prefLabel "R716" ;
    emmo:EMMO_967080e5_2f42_4eb2_a3a9_c58143e835f9 "a coin case with a nominal diameter of 7.9 mm and a height of 1.65 mm"@en .

:electrochemistry_36444184_1100_4271_869f_7f2d983aaecb a owl:Class ;
    rdfs:label "P45173115" ;
    rdfs:comment "a prismatic case with a nominal length of 45 mm, width of 173 mm, and height of 115 mm"@en ;
    rdfs:subClassOf :electrochemistry_43cd6e14_dd43_41b5_b5b4_344d53841603 ;
    skos:altLabel "BEV2",
        "P45/173/115" ;
    skos:prefLabel "P45173115" ;
    emmo:EMMO_967080e5_2f42_4eb2_a3a9_c58143e835f9 "a prismatic case with a nominal length of 45 mm, width of 173 mm, and height of 115 mm"@en .

:electrochemistry_36e05f2f_d279_4816_b5ae_6bb4cef02736 a owl:Class ;
    rdfs:label "R1216" ;
    rdfs:comment "a coin case with a nominal diameter of 12.5 mm and a height of 1.6 mm"@en ;
    rdfs:subClassOf :electrochemistry_3979cd56_6256_414d_966c_7f723bf71e37 ;
    skos:prefLabel "R1216" ;
    emmo:EMMO_967080e5_2f42_4eb2_a3a9_c58143e835f9 "a coin case with a nominal diameter of 12.5 mm and a height of 1.6 mm"@en .

:electrochemistry_37504d4d_2aff_4f7f_9f46_a24e258028e8 a owl:Class ;
    rdfs:label "P29135214" ;
    rdfs:comment "a prismatic case with a nominal length of 29 mm, width of 135 mm, and height of 214 mm"@en ;
    rdfs:subClassOf :electrochemistry_43cd6e14_dd43_41b5_b5b4_344d53841603 ;
    skos:altLabel "P29/135/214" ;
    skos:prefLabel "P29135214" ;
    emmo:EMMO_967080e5_2f42_4eb2_a3a9_c58143e835f9 "a prismatic case with a nominal length of 29 mm, width of 135 mm, and height of 214 mm"@en .

:electrochemistry_38755e67_9d3b_4a82_bd8d_ef40a70379c1 a owl:Class ;
    rdfs:label "AnolyteTank"@en ;
    rdfs:comment "a tank for holding anolyte"@en ;
    rdfs:subClassOf emmo:EMMO_f76884f7_964e_488e_9bb7_1b2453e9e817 ;
    skos:prefLabel "AnolyteTank"@en ;
    emmo:EMMO_967080e5_2f42_4eb2_a3a9_c58143e835f9 "a tank for holding anolyte"@en ;
    emmo:EMMO_c7b62dd7_063a_4c2a_8504_42f7264ba83f "usually used in a flow cell system"@en .

:electrochemistry_387e1e59_e511_4acb_b5ec_fa7360ec7557 a owl:Class ;
    rdfs:label "R927"@en ;
    rdfs:comment "a coin case with a nominal diameter of 9.5 mm and a height of 2.7 mm"@en ;
    rdfs:subClassOf :electrochemistry_3979cd56_6256_414d_966c_7f723bf71e37 ;
    skos:prefLabel "R927"@en ;
    emmo:EMMO_967080e5_2f42_4eb2_a3a9_c58143e835f9 "a coin case with a nominal diameter of 9.5 mm and a height of 2.7 mm"@en .

:electrochemistry_399b10cd_8a2e_47be_96b8_295890bd2460 a owl:Class ;
    rdfs:label "RhodiumBasedElectrode"@en ;
    rdfs:comment "an electrode in which the primary active material consists of rhodium or rhodium compounds"@en ;
    rdfs:subClassOf :electrochemistry_9a823d64_9d10_4a29_9cbd_9bbdad7985bc ;
    skos:prefLabel "RhodiumBasedElectrode"@en ;
    emmo:EMMO_967080e5_2f42_4eb2_a3a9_c58143e835f9 "an electrode in which the primary active material consists of rhodium or rhodium compounds"@en .

:electrochemistry_39c6f5a0_5dc8_4112_b432_b9fece568ca2 a owl:Class ;
    rdfs:label "R1130" ;
    rdfs:comment "a coin case with a nominal diameter of 11.5 mm and a height of 3.0 mm"@en ;
    rdfs:subClassOf :electrochemistry_3979cd56_6256_414d_966c_7f723bf71e37 ;
    skos:prefLabel "R1130" ;
    emmo:EMMO_967080e5_2f42_4eb2_a3a9_c58143e835f9 "a coin case with a nominal diameter of 11.5 mm and a height of 3.0 mm"@en .

:electrochemistry_3a69a00e_235a_4948_b369_8ac20116c85e a owl:Class ;
    rdfs:label "WovenMesh"@en ;
    rdfs:comment "a fabric-like structure created by interweaving wires or fibres in an over-under pattern, commonly used for filtration, screening, and reinforcement due to its high strength and durability"@en ;
    rdfs:subClassOf emmo:EMMO_ec7464a9_d99d_45f8_965b_4e9230ea8356 ;
    skos:prefLabel "WovenMesh"@en ;
    emmo:EMMO_967080e5_2f42_4eb2_a3a9_c58143e835f9 "a fabric-like structure created by interweaving wires or fibres in an over-under pattern, commonly used for filtration, screening, and reinforcement due to its high strength and durability"@en .

:electrochemistry_3b048a62_8591_4bf1_8fac_3d647beb9323 a owl:Class ;
    rdfs:label "R21700" ;
    rdfs:comment "a cylindrical case with a nominal diameter of 21 mm and height of 70 mm"@en ;
    rdfs:subClassOf :electrochemistry_b1cf9fee_2164_4f95_8204_90f717373a8a ;
    skos:altLabel "R21/70",
        "R2170" ;
    skos:prefLabel "R21700" ;
    emmo:EMMO_967080e5_2f42_4eb2_a3a9_c58143e835f9 "a cylindrical case with a nominal diameter of 21 mm and height of 70 mm"@en .

:electrochemistry_3b714a22_4212_4f4f_b578_140c357b18de a owl:Class ;
    rdfs:label "P2117385" ;
    rdfs:comment "a prismatic case with a nominal length of 21 mm, width of 173 mm, and height of 85 mm"@en ;
    rdfs:subClassOf :electrochemistry_43cd6e14_dd43_41b5_b5b4_344d53841603 ;
    skos:altLabel "P21/173/85",
        "PHEV1" ;
    skos:prefLabel "P2117385" ;
    emmo:EMMO_967080e5_2f42_4eb2_a3a9_c58143e835f9 "a prismatic case with a nominal length of 21 mm, width of 173 mm, and height of 85 mm"@en .

:electrochemistry_3d2f9945_2319_4a08_899b_6a5ffabd4925 a owl:Class ;
    rdfs:label "R18650" ;
    rdfs:comment "a cylindrical case with a nominal diameter of 18 mm and height of 65 mm"@en ;
    rdfs:subClassOf :electrochemistry_b1cf9fee_2164_4f95_8204_90f717373a8a ;
    skos:altLabel "R18/65",
        "R1865" ;
    skos:prefLabel "R18650" ;
    emmo:EMMO_967080e5_2f42_4eb2_a3a9_c58143e835f9 "a cylindrical case with a nominal diameter of 18 mm and height of 65 mm"@en .

:electrochemistry_3e6a7d5f_3700_46b3_b1b8_f34e37e6f931 a owl:Class ;
    rdfs:label "IridiumBasedElectrode"@en ;
    rdfs:comment "an electrode in which the primary active material consists of iridium or iridium compounds"@en ;
    rdfs:subClassOf :electrochemistry_9a823d64_9d10_4a29_9cbd_9bbdad7985bc ;
    skos:prefLabel "IridiumBasedElectrode"@en ;
    emmo:EMMO_967080e5_2f42_4eb2_a3a9_c58143e835f9 "an electrode in which the primary active material consists of iridium or iridium compounds"@en .

:electrochemistry_3f67016b_32b9_4419_a3f8_a5ffb5e92538 a owl:Class ;
    rdfs:label "AmmoniumChlorideSolution"@en ;
    rdfs:comment "a solution of ammonium chloride (NH4Cl) dissolved in water (H2O)"@en ;
    rdfs:subClassOf :electrochemistry_dc205ac2_314e_415c_a2b6_b12e8359d54c ;
    skos:altLabel "AqueousAmmoniumChlorideSolution"@en ;
    skos:prefLabel "AmmoniumChlorideSolution"@en ;
    emmo:EMMO_967080e5_2f42_4eb2_a3a9_c58143e835f9 "a solution of ammonium chloride (NH4Cl) dissolved in water (H2O)"@en .

:electrochemistry_3fdc81d5_eef3_4408_a6e4_3c51c5b1c8dc a owl:Class ;
    rdfs:label "TungstenOxideElectrode"@en ;
    rdfs:comment "electrode in which the active material is tungsten oxide"@en ;
    rdfs:subClassOf :electrochemistry_e4b6cb36_4dac_49e3_871d_40bcfca943a5 ;
    owl:deprecated true ;
    skos:altLabel "WO3Electrode"@en ;
    skos:prefLabel "TungstenOxideElectrode"@en ;
    emmo:EMMO_967080e5_2f42_4eb2_a3a9_c58143e835f9 "electrode in which the active material is tungsten oxide"@en .

:electrochemistry_400cb3e0_27b5_4d9a_be80_f86ad2757763 a owl:Class ;
    rdfs:label "R2050" ;
    rdfs:comment "a coin case with a nominal diameter of 20.0 mm and a height of 5.0 mm"@en ;
    rdfs:subClassOf :electrochemistry_3979cd56_6256_414d_966c_7f723bf71e37 ;
    skos:prefLabel "R2050" ;
    emmo:EMMO_967080e5_2f42_4eb2_a3a9_c58143e835f9 "a coin case with a nominal diameter of 20.0 mm and a height of 5.0 mm"@en .

:electrochemistry_402598d9_0eea_405d_b0d0_3b8b79deba6f a owl:Class ;
    rdfs:label "InterphaseGrowth"@en ;
    rdfs:comment "the process through which the size of an interphase increases over time"@en ;
    rdfs:subClassOf [ a owl:Restriction ;
            owl:onProperty emmo:EMMO_ae2d1a96_bfa1_409a_a7d2_03d69e8a125a ;
            owl:someValuesFrom :electrochemistry_0f007072_a8dd_4798_b865_1bf9363be627 ],
        :electrochemistry_19abaccd_43be_4048_965c_e4fb63c5951b ;
    skos:example "solid electrolyte interphase (SEI) growth"@en ;
    skos:prefLabel "InterphaseGrowth"@en ;
    emmo:EMMO_967080e5_2f42_4eb2_a3a9_c58143e835f9 "the process through which the size of an interphase increases over time"@en .

:electrochemistry_4143b1c2_2d21_419e_af45_247d4c78ce7e a owl:Class ;
    rdfs:label "SiliconOxideElectrode"@en ;
    rdfs:comment "electrode in which the active material is silicon oxide"@en ;
    rdfs:subClassOf :electrochemistry_e4b6cb36_4dac_49e3_871d_40bcfca943a5 ;
    owl:deprecated true ;
    skos:prefLabel "SiliconOxideElectrode"@en ;
    emmo:EMMO_967080e5_2f42_4eb2_a3a9_c58143e835f9 "electrode in which the active material is silicon oxide"@en .

:electrochemistry_418c59bd_dc9d_438b_bc7c_494fbd1bb4f8 a owl:Class ;
    rdfs:label "SingleCoatedElectrode"@en ;
    rdfs:comment "an electrode that is coated on only one side of the current collector"@en ;
    rdfs:subClassOf :electrochemistry_92147e31_d015_4889_a092_04fbab033f15 ;
    skos:prefLabel "SingleCoatedElectrode"@en ;
    emmo:EMMO_157fdf31_6387_42be_8e72_10530519214a "https://raw.githubusercontent.com/emmo-repo/domain-electrochemistry/dev/docs/assets/img/fig/png/SingleCoatedElectrode.png" ;
    emmo:EMMO_967080e5_2f42_4eb2_a3a9_c58143e835f9 "an electrode that is coated on only one side of the current collector"@en .

:electrochemistry_41ab11ec_af9f_401d_b80d_474c1dc86cd6 a owl:Class ;
    rdfs:label "P4014895" ;
    rdfs:comment "a prismatic case with a nominal length of 40 mm, width of 148 mm, and height of 95 mm"@en ;
    rdfs:subClassOf :electrochemistry_43cd6e14_dd43_41b5_b5b4_344d53841603 ;
    skos:altLabel "P40/148/95" ;
    skos:prefLabel "P4014895" ;
    emmo:EMMO_967080e5_2f42_4eb2_a3a9_c58143e835f9 "a prismatic case with a nominal length of 40 mm, width of 148 mm, and height of 95 mm"@en .

:electrochemistry_41ddf723_245f_4ce8_b9b1_7d9b3b9eea7d a owl:Class ;
    rdfs:label "LithiumNickelManganeseOxideElectrode"@en ;
    rdfs:comment "electrode in which the active material is lithium nickel manganese oxide"@en ;
    rdfs:subClassOf [ a owl:Restriction ;
            owl:onProperty :electrochemistry_860aa941_5ff9_4452_8a16_7856fad07bee ;
            owl:someValuesFrom chems:substance_f3e7979a_e3ef_450a_8762_7d8778afe478 ],
        :electrochemistry_0d2aaaf4_1a8a_4a32_abd8_7d0fdf0ae9d2,
        :electrochemistry_e4b6cb36_4dac_49e3_871d_40bcfca943a5 ;
    owl:deprecated true ;
    skos:altLabel "LNMOElectrode"@en ;
    skos:prefLabel "LithiumNickelManganeseOxideElectrode"@en ;
    emmo:EMMO_967080e5_2f42_4eb2_a3a9_c58143e835f9 "electrode in which the active material is lithium nickel manganese oxide"@en .

:electrochemistry_424bf750_7df5_49b5_ba73_ba74397a166b a owl:Class ;
    rdfs:label "ZincElectrode"@en ;
    rdfs:comment "an electrode in which the main active material is zinc metal"@en ;
    rdfs:subClassOf [ a owl:Restriction ;
            owl:onProperty :electrochemistry_860aa941_5ff9_4452_8a16_7856fad07bee ;
            owl:someValuesFrom chems:substance_9bd78e1c_a4dc_41b6_8013_adb51df1ffdc ],
        :electrochemistry_5adb91e0_ffe1_41f3_b779_c6966f65fb0e,
        :electrochemistry_d0a26dc2_fde9_4a11_ac26_7c18499d28a5 ;
    skos:prefLabel "ZincElectrode"@en ;
    emmo:EMMO_967080e5_2f42_4eb2_a3a9_c58143e835f9 "an electrode in which the main active material is zinc metal"@en ;
    emmo:EMMO_c7b62dd7_063a_4c2a_8504_42f7264ba83f "the combination with manganese dioxide and an alkali metal hydoxide electrolyte is designated using IEC electrochemical system letter code L"@en,
        "the combination with nickel oxide hydroxide and an alkali metal hydoxide electrolyte is designated using IEC electrochemical system letter code Z"@en,
        "the combination with oxygen and an alkali metal hydoxide electrolyte is designated using IEC electrochemical system letter code P"@en,
        "the combination with oxygen and an ammonium chloride zinc chloride electrolyte is designated using IEC electrochemical system letter code A"@en,
        "the combination with silver oxide and an alkali metal hydoxide electrolyte is designated using IEC electrochemical system letter code S"@en .

:electrochemistry_46ac0fd3_2b8e_40aa_bf5d_19cf1dd39052 a owl:Class ;
    rdfs:label "StrontiumBasedElectrode"@en ;
    rdfs:comment "an electrode in which the primary active material consists of strontium or strontium compounds"@en ;
    rdfs:subClassOf :electrochemistry_9a823d64_9d10_4a29_9cbd_9bbdad7985bc ;
    skos:prefLabel "StrontiumBasedElectrode"@en ;
    emmo:EMMO_967080e5_2f42_4eb2_a3a9_c58143e835f9 "an electrode in which the primary active material consists of strontium or strontium compounds"@en .

:electrochemistry_48e380c3_0441_4761_a80f_3e448cb2f0ba a owl:Class ;
    rdfs:label "LithiumNickelMananeseCobaltOxideLithiumManganeseOxideElectrode"@en ;
    rdfs:comment "an electrode with blended lithium nickel manganese cobalt oxide (NMC) and lithium manganese oxide (LMO) active materials"@en ;
    rdfs:subClassOf [ a owl:Restriction ;
            owl:onProperty :electrochemistry_860aa941_5ff9_4452_8a16_7856fad07bee ;
            owl:someValuesFrom chems:substance_3ac62305_acd6_4312_9e31_4f824bd2530d ],
        [ a owl:Restriction ;
            owl:onProperty :electrochemistry_860aa941_5ff9_4452_8a16_7856fad07bee ;
            owl:someValuesFrom chems:substance_e8fafdc8_6cd3_4dd0_9630_10ca8e3f1827 ],
        :electrochemistry_4839708a_3864_47eb_b719_373ff8874c61 ;
    owl:deprecated true ;
    skos:altLabel "NMCLMOElectrode"@en ;
    skos:prefLabel "LithiumNickelMananeseCobaltOxideLithiumManganeseOxideElectrode"@en ;
    emmo:EMMO_967080e5_2f42_4eb2_a3a9_c58143e835f9 "an electrode with blended lithium nickel manganese cobalt oxide (NMC) and lithium manganese oxide (LMO) active materials"@en .

:electrochemistry_4977521c_0438_4659_bc81_1c77fae836bb a owl:Class ;
    rdfs:label "ThionylChlorideElectrode"@en ;
    rdfs:comment "an electrode in which the primary active material consists of thionyl chloride"@en ;
    rdfs:subClassOf :electrochemistry_88d2d4bc_4244_4419_a260_ad099a62d580 ;
    skos:prefLabel "ThionylChlorideElectrode"@en ;
    emmo:EMMO_967080e5_2f42_4eb2_a3a9_c58143e835f9 "an electrode in which the primary active material consists of thionyl chloride"@en ;
    emmo:EMMO_c7b62dd7_063a_4c2a_8504_42f7264ba83f "the combination with lithium metal and non-aqueous in-organic electrolyte is designated using IEC electrochemical system letter code E"@en .

:electrochemistry_4a13e538_4c08_4ba9_8ebc_98a866208e01 a owl:Class ;
    rdfs:label "SodiumNickelPhosphateElectrode"@en ;
    rdfs:comment "electrode in which the active material is sodium nickel phosphate"@en ;
    rdfs:subClassOf [ a owl:Restriction ;
            owl:onProperty :electrochemistry_860aa941_5ff9_4452_8a16_7856fad07bee ;
            owl:someValuesFrom chems:substance_97439fbb_155f_433d_9edd_d510cd491f24 ],
        :electrochemistry_0d2aaaf4_1a8a_4a32_abd8_7d0fdf0ae9d2,
        :electrochemistry_e4b6cb36_4dac_49e3_871d_40bcfca943a5 ;
    owl:deprecated true ;
    skos:prefLabel "SodiumNickelPhosphateElectrode"@en ;
    emmo:EMMO_967080e5_2f42_4eb2_a3a9_c58143e835f9 "electrode in which the active material is sodium nickel phosphate"@en .

:electrochemistry_4bdd6359_1422_4c50_ac0c_5d8042dd65fc a owl:Class ;
    rdfs:label "BockrisDevanathanMuellerModel"@en ;
    rdfs:comment "a model for the double layer that includes the action of the solvent on the surface"@en ;
    rdfs:subClassOf :electrochemistry_ac9723d1_bac0_4109_874e_32849de9299b ;
    skos:altLabel "BDM"@en ;
    skos:prefLabel "BockrisDevanathanMuellerModel"@en ;
    emmo:EMMO_967080e5_2f42_4eb2_a3a9_c58143e835f9 "a model for the double layer that includes the action of the solvent on the surface"@en ;
    emmo:EMMO_c7b62dd7_063a_4c2a_8504_42f7264ba83f "proposed by John Bockris, M. A. V. Devanathan, and Klaus Mueller in 1963"@en .

:electrochemistry_4c3ee364_829b_41a4_b895_ca4a041efb2a a owl:Class ;
    rdfs:label "LithiumInsertionElectrode"@en ;
    rdfs:comment "an insertion electrode in which the guest molecule is lithium"@en ;
    rdfs:subClassOf :electrochemistry_757eae08_4d43_42d4_8b4e_8a0bfd2f9a1c ;
    owl:deprecated true ;
    skos:prefLabel "LithiumInsertionElectrode"@en ;
    emmo:EMMO_967080e5_2f42_4eb2_a3a9_c58143e835f9 "an insertion electrode in which the guest molecule is lithium"@en .

:electrochemistry_4ca551d2_2969_4c18_96ce_db99831ed0af a owl:Class ;
    rdfs:label "P1212085" ;
    rdfs:comment "a prismatic case with a nominal length of 12 mm, width of 120 mm, and height of 85 mm"@en ;
    rdfs:subClassOf :electrochemistry_43cd6e14_dd43_41b5_b5b4_344d53841603 ;
    skos:altLabel "P12/120/85" ;
    skos:prefLabel "P1212085" ;
    emmo:EMMO_967080e5_2f42_4eb2_a3a9_c58143e835f9 "a prismatic case with a nominal length of 12 mm, width of 120 mm, and height of 85 mm"@en .

:electrochemistry_4edb47d6_107c_40a2_be7c_6b26e9d296da a owl:Class ;
    rdfs:label "SodiumManganeseHexacyanoferrateElectrode"@en ;
    rdfs:comment "electrode in which the active material is sodium manganese hexacyanoferrate"@en ;
    rdfs:subClassOf :electrochemistry_b1ac8d0c_a215_4e60_82b0_38272eff5131,
        :electrochemistry_e4b6cb36_4dac_49e3_871d_40bcfca943a5 ;
    owl:deprecated true ;
    skos:prefLabel "SodiumManganeseHexacyanoferrateElectrode"@en ;
    emmo:EMMO_967080e5_2f42_4eb2_a3a9_c58143e835f9 "electrode in which the active material is sodium manganese hexacyanoferrate"@en .

:electrochemistry_4f2348dd_d9ea_4448_af8c_a4a38f3d04b4 a owl:Class ;
    rdfs:label "CalciumBasedElectrode"@en ;
    rdfs:comment "an electrode in which the primary active material consists of calcium or calcium compounds"@en ;
    rdfs:subClassOf :electrochemistry_9a823d64_9d10_4a29_9cbd_9bbdad7985bc ;
    skos:prefLabel "CalciumBasedElectrode"@en ;
    emmo:EMMO_967080e5_2f42_4eb2_a3a9_c58143e835f9 "an electrode in which the primary active material consists of calcium or calcium compounds"@en .

:electrochemistry_502a98a3_ce47_421f_8e0a_016ed171c900 a owl:Class ;
    rdfs:label "SodiumIronPhosphateElectrode"@en ;
    rdfs:comment "electrode in which the active material is sodium iron phosphate"@en ;
    rdfs:subClassOf [ a owl:Restriction ;
            owl:onProperty :electrochemistry_860aa941_5ff9_4452_8a16_7856fad07bee ;
            owl:someValuesFrom chems:substance_c5582dae_ccff_4fbe_adaa_078091054640 ],
        :electrochemistry_d54f6aac_7cd2_4d52_9bca_2f19bb1eaec4,
        :electrochemistry_e4b6cb36_4dac_49e3_871d_40bcfca943a5 ;
    owl:deprecated true ;
    skos:prefLabel "SodiumIronPhosphateElectrode"@en ;
    emmo:EMMO_967080e5_2f42_4eb2_a3a9_c58143e835f9 "electrode in which the active material is sodium iron phosphate"@en .

:electrochemistry_50d9652c_6b68_457c_bd72_f89a8e549bcf a owl:Class ;
    rdfs:label "P2714898" ;
    rdfs:comment "a prismatic case with a nominal length of 27 mm, width of 148 mm, and height of 98 mm"@en ;
    rdfs:subClassOf :electrochemistry_43cd6e14_dd43_41b5_b5b4_344d53841603 ;
    skos:altLabel "P27/148/98" ;
    skos:prefLabel "P2714898" ;
    emmo:EMMO_967080e5_2f42_4eb2_a3a9_c58143e835f9 "a prismatic case with a nominal length of 27 mm, width of 148 mm, and height of 98 mm"@en .

:electrochemistry_510e4061_c4fa_49aa_a052_23ad56098eda a owl:Class ;
    rdfs:label "ChromiumBasedElectrode"@en ;
    rdfs:comment "an electrode in which the primary active material consists of chromium or chromium compounds"@en ;
    rdfs:subClassOf :electrochemistry_9a823d64_9d10_4a29_9cbd_9bbdad7985bc ;
    skos:prefLabel "ChromiumBasedElectrode"@en ;
    emmo:EMMO_967080e5_2f42_4eb2_a3a9_c58143e835f9 "an electrode in which the primary active material consists of chromium or chromium compounds"@en .

:electrochemistry_554286d4_1f46_44c0_bebc_4ddae00dbce1 a owl:Class ;
    rdfs:label "ElectrolyteAdditive"@en ;
    rdfs:comment "A substance added to an electrolyte to alter its properties"@en ;
    rdfs:subClassOf :electrochemistry_0a399f3f_b873_41f5_be1f_9b6df75cc30a ;
    skos:prefLabel "ElectrolyteAdditive"@en ;
    emmo:EMMO_967080e5_2f42_4eb2_a3a9_c58143e835f9 "A substance added to an electrolyte to alter its properties"@en .

:electrochemistry_55775b50_b9d9_4d68_8cb5_38fcd7b9b54d a owl:Class ;
    rdfs:label "LithiumElectrode"@en ;
    rdfs:comment "an electrode in which the active material is lithium metal" ;
    rdfs:subClassOf [ a owl:Restriction ;
            owl:onProperty :electrochemistry_860aa941_5ff9_4452_8a16_7856fad07bee ;
            owl:someValuesFrom chems:substance_c109ca45_08c7_4436_a818_a9c575785e2f ],
        :electrochemistry_47346d85_b9be_4480_8993_6307b1c58fcd ;
    skos:prefLabel "LithiumElectrode"@en ;
    emmo:EMMO_967080e5_2f42_4eb2_a3a9_c58143e835f9 "an electrode in which the active material is lithium metal" .

:electrochemistry_56177336_3ae5_48cb_93ca_a8c73216ea73 a owl:Class ;
    rdfs:label "R40108" ;
    rdfs:comment "a cylindrical case with a nominal diameter of 40 mm and height of 108 mm"@en ;
    rdfs:subClassOf :electrochemistry_b1cf9fee_2164_4f95_8204_90f717373a8a ;
    skos:altLabel "R40/108" ;
    skos:prefLabel "R40108" ;
    emmo:EMMO_967080e5_2f42_4eb2_a3a9_c58143e835f9 "a cylindrical case with a nominal diameter of 40 mm and height of 108 mm"@en .

:electrochemistry_564d31be_91cb_4a8f_8369_2a55f1180499 a owl:Class ;
    rdfs:label "OrganicElectrolyte"@en ;
    rdfs:comment "an electrolyte solution with an organic solvent"@en ;
    rdfs:subClassOf :electrochemistry_fa22874b_76a9_4043_8b8f_6086c88746de ;
    skos:prefLabel "OrganicElectrolyte"@en ;
    emmo:EMMO_967080e5_2f42_4eb2_a3a9_c58143e835f9 "an electrolyte solution with an organic solvent"@en .

:electrochemistry_56def0d5_fe57_40d7_85e3_97872fa2a3e1 a owl:Class ;
    rdfs:label "P1714891" ;
    rdfs:comment "a prismatic case with a nominal length of 17 mm, width of 148 mm, and height of 91 mm"@en ;
    rdfs:subClassOf :electrochemistry_43cd6e14_dd43_41b5_b5b4_344d53841603 ;
    skos:altLabel "P17/148/91",
        "PHEV2" ;
    skos:prefLabel "P1714891" ;
    emmo:EMMO_967080e5_2f42_4eb2_a3a9_c58143e835f9 "a prismatic case with a nominal length of 17 mm, width of 148 mm, and height of 91 mm"@en .

:electrochemistry_56f85b19_1384_4e88_b130_cb8e7984db83 a owl:Class ;
    rdfs:label "DoubleCoatedElectrode"@en ;
    rdfs:comment "an electrode that is coated on both sides of the current collector"@en ;
    rdfs:subClassOf :electrochemistry_92147e31_d015_4889_a092_04fbab033f15 ;
    skos:prefLabel "DoubleCoatedElectrode"@en ;
    emmo:EMMO_157fdf31_6387_42be_8e72_10530519214a "https://raw.githubusercontent.com/emmo-repo/domain-electrochemistry/dev/docs/assets/img/fig/png/DoubleCoatedElectrode.png" ;
    emmo:EMMO_967080e5_2f42_4eb2_a3a9_c58143e835f9 "an electrode that is coated on both sides of the current collector"@en .

:electrochemistry_573be62a_5aae_4984_9a51_7c50845493df a owl:Class ;
    rdfs:label "CardonDioxideElectrode"@en ;
    rdfs:comment "a gas diffusion electrode in which the active material is carbon dioxide (CO2)"@en ;
    rdfs:subClassOf :electrochemistry_bbb1d95b_72d1_44f6_b07e_a3d7d41ac215 ;
    skos:prefLabel "CardonDioxideElectrode"@en ;
    emmo:EMMO_967080e5_2f42_4eb2_a3a9_c58143e835f9 "a gas diffusion electrode in which the active material is carbon dioxide (CO2)"@en .

:electrochemistry_58413d4e_2885_459e_ac06_8d45e661cf91 a owl:Class ;
    rdfs:label "PorousSeparator"@en ;
    rdfs:comment "a separator with a porosity greater than 0"@en ;
    rdfs:subClassOf :electrochemistry_331e6cca_f260_4bf8_af55_35304fe1bbe0 ;
    owl:deprecated true ;
    skos:prefLabel "PorousSeparator"@en ;
    emmo:EMMO_967080e5_2f42_4eb2_a3a9_c58143e835f9 "a separator with a porosity greater than 0"@en .

:electrochemistry_598ae3d0_76e9_429c_a0e1_8694525cb574 a owl:Class ;
    rdfs:label "KohlrauschsLaw"@en ;
    rdfs:comment "For any electrolyte A_xB_y, the limiting molar conductivity is expressed as x times the limiting molar conductivity of A^{y+} and y times the limiting molar conductivity of B^{x-}."@en ;
    rdfs:subClassOf emmo:EMMO_f19ff3b4_6bfe_4c41_a2b2_9affd39c140b ;
    skos:prefLabel "KohlrauschsLaw"@en ;
    emmo:EMMO_26bf1bef_d192_4da6_b0eb_d2209698fb54 "https://www.wikidata.org/wiki/Q3258329" ;
    emmo:EMMO_967080e5_2f42_4eb2_a3a9_c58143e835f9 "For any electrolyte A_xB_y, the limiting molar conductivity is expressed as x times the limiting molar conductivity of A^{y+} and y times the limiting molar conductivity of B^{x-}."@en ;
    emmo:EMMO_c7b62dd7_063a_4c2a_8504_42f7264ba83f "proposed by Friedrich Kohlrausch between 1875-1879"@en,
        "valid for dilute solutions"@en ;
    emmo:EMMO_c84c6752_6d64_48cc_9500_e54a3c34898d "https://en.wikipedia.org/wiki/Molar_conductivity#Kohlrausch's_law_of_independent_migration_of_ions"@en .

:electrochemistry_5a7a3028_db9e_4045_ab68_054c6afc91fc a owl:Class ;
    rdfs:label "LawOfMassAction"@en ;
    rdfs:comment "the rate of the chemical reaction is directly proportional to the product of the activities or concentrations of the reactants"@en ;
    rdfs:subClassOf emmo:EMMO_9c32fd69_f480_4130_83b3_fb25d9face14 ;
    skos:prefLabel "LawOfMassAction"@en ;
    emmo:EMMO_26bf1bef_d192_4da6_b0eb_d2209698fb54 "https://www.wikidata.org/wiki/Q899494" ;
    emmo:EMMO_967080e5_2f42_4eb2_a3a9_c58143e835f9 "the rate of the chemical reaction is directly proportional to the product of the activities or concentrations of the reactants"@en ;
    emmo:EMMO_c84c6752_6d64_48cc_9500_e54a3c34898d "https://en.wikipedia.org/wiki/Law_of_mass_action"@en .

:electrochemistry_5c0fdc09_166e_40a6_ad74_be66f0db51bc a owl:Class ;
    rdfs:label "CarbonMonofluorideElectrode"@en ;
    rdfs:comment "electrode in which the active material is carbon monofluoride"@en ;
    rdfs:subClassOf [ a owl:Restriction ;
            owl:onProperty :electrochemistry_860aa941_5ff9_4452_8a16_7856fad07bee ;
            owl:someValuesFrom chems:substance_9da78aea_d436_40e2_a68f_c3dee32b825e ],
        :electrochemistry_9a823d64_9d10_4a29_9cbd_9bbdad7985bc,
        :electrochemistry_f2c33088_224f_4fdb_857a_7cb62e3dddca ;
    skos:prefLabel "CarbonMonofluorideElectrode"@en ;
    emmo:EMMO_967080e5_2f42_4eb2_a3a9_c58143e835f9 "electrode in which the active material is carbon monofluoride"@en ;
    emmo:EMMO_c7b62dd7_063a_4c2a_8504_42f7264ba83f "the combination with lithium metal and an organic electrolyte is designated using IEC electrochemical system letter code B"@en .

:electrochemistry_610f0bc8_557d_455b_a8ed_272d5d1813c9 a owl:Class ;
    rdfs:label "LeadBasedElectrode"@en ;
    rdfs:comment "an electrode in which the primary active material consists of lead or lead compounds"@en ;
    rdfs:subClassOf :electrochemistry_9a823d64_9d10_4a29_9cbd_9bbdad7985bc ;
    skos:prefLabel "LeadBasedElectrode"@en ;
    emmo:EMMO_967080e5_2f42_4eb2_a3a9_c58143e835f9 "an electrode in which the primary active material consists of lead or lead compounds"@en .

:electrochemistry_6164a2b0_7fd7_4059_8567_3dcce90b1dec a owl:ObjectProperty ;
    rdfs:label "hasLayer"@en ;
    rdfs:comment "relates a system or component to a layer that forms part of its structural composition, typically distinguished by its material or functional characteristics"@en ;
    rdfs:subPropertyOf emmo:EMMO_3c7f239f_e833_4a2b_98a1_c88831770c1b ;
    skos:prefLabel "hasLayer"@en ;
    emmo:EMMO_967080e5_2f42_4eb2_a3a9_c58143e835f9 "relates a system or component to a layer that forms part of its structural composition, typically distinguished by its material or functional characteristics"@en .

:electrochemistry_619c2e56_077d_4bb4_9062_65fb75763651 a owl:Class ;
    rdfs:label "P27148129" ;
    rdfs:comment "a prismatic case with a nominal length of 27 mm, width of 148 mm, and height of 129 mm"@en ;
    rdfs:subClassOf :electrochemistry_43cd6e14_dd43_41b5_b5b4_344d53841603 ;
    skos:altLabel "P27/148/129" ;
    skos:prefLabel "P27148129" ;
    emmo:EMMO_967080e5_2f42_4eb2_a3a9_c58143e835f9 "a prismatic case with a nominal length of 27 mm, width of 148 mm, and height of 129 mm"@en .

:electrochemistry_6235cc7c_2eee_432a_93af_47d7e05db007 a owl:Class ;
    rdfs:label "HardCarbonElectrode"@en ;
    rdfs:comment "electrode in which the active material is hard carbon"@en ;
    rdfs:subClassOf [ a owl:Restriction ;
            owl:onProperty :electrochemistry_860aa941_5ff9_4452_8a16_7856fad07bee ;
            owl:someValuesFrom chems:substance_5cee19d2_f916_4264_a8ed_efed13a808d2 ],
        :electrochemistry_9a823d64_9d10_4a29_9cbd_9bbdad7985bc,
        :electrochemistry_f2c33088_224f_4fdb_857a_7cb62e3dddca ;
    skos:prefLabel "HardCarbonElectrode"@en ;
    emmo:EMMO_967080e5_2f42_4eb2_a3a9_c58143e835f9 "electrode in which the active material is hard carbon"@en .

:electrochemistry_634467ad_feed_4979_adb2_877d98fe1768 a owl:Class ;
    rdfs:label "LiquidJunction"@en ;
    rdfs:comment "any junction between two electrolyte solutions of different composition."@en ;
    rdfs:subClassOf :electrochemistry_50044b99_b858_433b_a32d_23d1e1cf88b2 ;
    skos:prefLabel "LiquidJunction"@en ;
    emmo:EMMO_967080e5_2f42_4eb2_a3a9_c58143e835f9 "any junction between two electrolyte solutions of different composition."@en ;
    emmo:EMMO_c7b62dd7_063a_4c2a_8504_42f7264ba83f "Across such a junction there arises a potential difference, called the liquid junction potential."@en,
        "In the operational pH cell the junction is between the test, or pH standard, solution and the filling solution or the bridge solution of the reference electrode."@en ;
    emmo:EMMO_fe015383_afb3_44a6_ae86_043628697aa2 "https://goldbook.iupac.org/terms/view/L03584"@en .

:electrochemistry_6385e07f_f40d_46b2_b998_c439950d75cb a owl:Class ;
    rdfs:label "WaveSpring"@en ;
    rdfs:comment "a spring made of pre-hardened flat wire, formed into a wavy washer shape"@en ;
    rdfs:subClassOf :electrochemistry_872b11e1_8bb3_4a2a_af90_bbaa0055d01e ;
    skos:prefLabel "WaveSpring"@en ;
    emmo:EMMO_26bf1bef_d192_4da6_b0eb_d2209698fb54 "https://www.wikidata.org/wiki/Q11288626" ;
    emmo:EMMO_967080e5_2f42_4eb2_a3a9_c58143e835f9 "a spring made of pre-hardened flat wire, formed into a wavy washer shape"@en ;
    emmo:EMMO_c84c6752_6d64_48cc_9500_e54a3c34898d "https://en.wikipedia.org/wiki/Wave_spring"@en .

:electrochemistry_6775b232_c58a_4303_8164_137261329db6 a owl:Class ;
    rdfs:label "Prismatic"@en ;
    rdfs:comment "a form factor describing a prismatic cell, which has the shape of a rectangular prism"@en ;
    rdfs:subClassOf :electrochemistry_1586ef26_6d30_49e3_ae32_b4c9fc181941 ;
    skos:prefLabel "Prismatic"@en ;
    emmo:EMMO_967080e5_2f42_4eb2_a3a9_c58143e835f9 "a form factor describing a prismatic cell, which has the shape of a rectangular prism"@en .

:electrochemistry_68c1c36e_1548_4247_bae2_fe7102a2c4ff a owl:Class ;
    rdfs:label "R626" ;
    rdfs:comment "a coin case with a nominal diameter of 6.8 mm and a height of 2.6 mm"@en ;
    rdfs:subClassOf :electrochemistry_3979cd56_6256_414d_966c_7f723bf71e37 ;
    skos:altLabel "R66" ;
    skos:prefLabel "R626" ;
    emmo:EMMO_967080e5_2f42_4eb2_a3a9_c58143e835f9 "a coin case with a nominal diameter of 6.8 mm and a height of 2.6 mm"@en .

:electrochemistry_69e59b3d_b19d_4f8e_8b9c_84eb64307626 a owl:Class ;
    rdfs:label "R54137" ;
    rdfs:comment "a cylindrical case with a nominal diameter of 54 mm and height of 137 mm"@en ;
    rdfs:subClassOf :electrochemistry_b1cf9fee_2164_4f95_8204_90f717373a8a ;
    skos:altLabel "R54/137" ;
    skos:prefLabel "R54137" ;
    emmo:EMMO_967080e5_2f42_4eb2_a3a9_c58143e835f9 "a cylindrical case with a nominal diameter of 54 mm and height of 137 mm"@en .

:electrochemistry_6b275583_433f_46f7_aafd_ebc9409257cc a owl:Class ;
    rdfs:label "R626" ;
    rdfs:comment "a coin case with a nominal diameter of 6.8 mm and a height of 2.6 mm"@en ;
    rdfs:subClassOf :electrochemistry_3979cd56_6256_414d_966c_7f723bf71e37 ;
    skos:altLabel "R66" ;
    skos:prefLabel "R626" ;
    emmo:EMMO_967080e5_2f42_4eb2_a3a9_c58143e835f9 "a coin case with a nominal diameter of 6.8 mm and a height of 2.6 mm"@en ;
    emmo:EMMO_c7b62dd7_063a_4c2a_8504_42f7264ba83f "often used in wrist watches"@en .

:electrochemistry_6d0fe07e_a629_479c_ab24_2846f209bb0b a owl:Class ;
    rdfs:label "LithiumTitanateElectrode"@en ;
    rdfs:comment "electrode in which the active material is lithium titanate"@en ;
    rdfs:subClassOf [ a owl:Restriction ;
            owl:onProperty :electrochemistry_860aa941_5ff9_4452_8a16_7856fad07bee ;
            owl:someValuesFrom chems:substance_acdb232f_8041_4e11_8a11_5db2d2baae4d ],
        :electrochemistry_9c557caa_61e2_4fa9_a517_4bad01a68122,
        :electrochemistry_e4b6cb36_4dac_49e3_871d_40bcfca943a5 ;
    owl:deprecated true ;
    skos:altLabel "LTOElectrode"@en ;
    skos:prefLabel "LithiumTitanateElectrode"@en ;
    emmo:EMMO_967080e5_2f42_4eb2_a3a9_c58143e835f9 "electrode in which the active material is lithium titanate"@en .

:electrochemistry_6eaa3c0d_e1f3_4c6e_91a6_9b8c5a21b8cb a owl:Class ;
    rdfs:label "R40920" ;
    rdfs:comment "a cylindrical case with a nominal diameter of 40 mm and height of 92 mm"@en ;
    rdfs:subClassOf :electrochemistry_b1cf9fee_2164_4f95_8204_90f717373a8a ;
    skos:altLabel "R40/92" ;
    skos:prefLabel "R40920" ;
    emmo:EMMO_967080e5_2f42_4eb2_a3a9_c58143e835f9 "a cylindrical case with a nominal diameter of 40 mm and height of 92 mm"@en .

:electrochemistry_6ec59f99_5f26_4a7d_9b90_b52e0f8ad190 a owl:Class ;
    rdfs:label "SilverChlorideElectrode"@en ;
    rdfs:comment "A type of reference electrode based on the reaction between sliver and silver chloride."@en ;
    rdfs:subClassOf :electrochemistry_7729c34e_1ae9_403d_b933_1765885e7f29 ;
    skos:prefLabel "SilverChlorideElectrode"@en ;
    emmo:EMMO_26bf1bef_d192_4da6_b0eb_d2209698fb54 "https://www.wikidata.org/wiki/Q900939" ;
    emmo:EMMO_967080e5_2f42_4eb2_a3a9_c58143e835f9 "A type of reference electrode based on the reaction between sliver and silver chloride."@en ;
    emmo:EMMO_c84c6752_6d64_48cc_9500_e54a3c34898d "https://en.wikipedia.org/wiki/Silver_chloride_electrode"@en .

:electrochemistry_6ee40e33_ccbf_410e_a8fa_047a9eae0362 a owl:Class ;
    rdfs:label "R27660" ;
    rdfs:comment "a cylindrical case with a nominal diameter of 27 mm and height of 66 mm"@en ;
    rdfs:subClassOf :electrochemistry_b1cf9fee_2164_4f95_8204_90f717373a8a ;
    skos:altLabel "R27/66" ;
    skos:prefLabel "R27660" ;
    emmo:EMMO_967080e5_2f42_4eb2_a3a9_c58143e835f9 "a cylindrical case with a nominal diameter of 27 mm and height of 66 mm"@en .

:electrochemistry_7018bd4e_6ca1_44eb_a558_6585c0bf8547 a owl:Class ;
    rdfs:label "P2770120" ;
    rdfs:comment "a prismatic case with a nominal length of 27 mm, width of 70 mm, and height of 120 mm"@en ;
    rdfs:subClassOf :electrochemistry_43cd6e14_dd43_41b5_b5b4_344d53841603 ;
    skos:altLabel "P27/70/120" ;
    skos:prefLabel "P2770120" ;
    emmo:EMMO_967080e5_2f42_4eb2_a3a9_c58143e835f9 "a prismatic case with a nominal length of 27 mm, width of 70 mm, and height of 120 mm"@en .

:electrochemistry_713200a1_952b_49e2_90b7_deba229f6bbe a owl:Class ;
    rdfs:label "LithiumManganesePhosphateElectrode"@en ;
    rdfs:comment "electrode in which the active material is lithium manganese phosphate"@en ;
    rdfs:subClassOf :electrochemistry_468b3b63_b62a_4110_8c7e_40fffd5fdfd6,
        :electrochemistry_e4b6cb36_4dac_49e3_871d_40bcfca943a5 ;
    owl:deprecated true ;
    skos:altLabel "LMPElectrode"@en ;
    skos:prefLabel "LithiumManganesePhosphateElectrode"@en ;
    emmo:EMMO_967080e5_2f42_4eb2_a3a9_c58143e835f9 "electrode in which the active material is lithium manganese phosphate"@en .

:electrochemistry_7393f12f_e3b9_42d6_bffb_e5613f53108f a owl:Class ;
    rdfs:label "ZincChlorideSolution"@en ;
    rdfs:comment "a solution of zinc chloride (ZnCl2) dissolved in water (H2O)"@en ;
    rdfs:subClassOf :electrochemistry_dc205ac2_314e_415c_a2b6_b12e8359d54c ;
    skos:altLabel "AqueousZincChlorideSolution"@en ;
    skos:prefLabel "ZincChlorideSolution"@en ;
    emmo:EMMO_967080e5_2f42_4eb2_a3a9_c58143e835f9 "a solution of zinc chloride (ZnCl2) dissolved in water (H2O)"@en .

:electrochemistry_74459386_875c_4303_b774_60125b599d06 a owl:Class ;
    rdfs:label "PouchCase"@en ;
    rdfs:comment "a soft pouch case that is described by its length, width, and height"@en ;
    rdfs:subClassOf :electrochemistry_1aec4cc0_82d5_4042_a657_ed7fe291c3d8 ;
    skos:prefLabel "PouchCase"@en ;
    emmo:EMMO_967080e5_2f42_4eb2_a3a9_c58143e835f9 "a soft pouch case that is described by its length, width, and height"@en ;
    emmo:EMMO_c7b62dd7_063a_4c2a_8504_42f7264ba83f "often represented in cell designations by the letter P"@en .

:electrochemistry_76318e8e_c1ba_49ac_8029_a951bd9dc955 a owl:Class ;
    rdfs:label "R516" ;
    rdfs:comment "a coin case with a nominal diameter of 5.8 mm and a height of 1.6 mm"@en ;
    rdfs:subClassOf :electrochemistry_3979cd56_6256_414d_966c_7f723bf71e37 ;
    skos:altLabel "R62" ;
    skos:prefLabel "R516" ;
    emmo:EMMO_967080e5_2f42_4eb2_a3a9_c58143e835f9 "a coin case with a nominal diameter of 5.8 mm and a height of 1.6 mm"@en .

:electrochemistry_76e461aa_5948_4a68_8337_284d11e0fd7d a owl:Class ;
    rdfs:label "NickelOxideElectrode"@en ;
    rdfs:comment "electrode in which the active material is nickel oxide"@en ;
    rdfs:subClassOf [ a owl:Restriction ;
            owl:onProperty :electrochemistry_860aa941_5ff9_4452_8a16_7856fad07bee ;
            owl:someValuesFrom chems:substance_5088ad54_b37d_4ee1_a086_d6c17e644f9a ],
        :electrochemistry_0d2aaaf4_1a8a_4a32_abd8_7d0fdf0ae9d2,
        :electrochemistry_e4b6cb36_4dac_49e3_871d_40bcfca943a5 ;
    owl:deprecated true ;
    skos:altLabel "NiOElectrode"@en ;
    skos:prefLabel "NickelOxideElectrode"@en ;
    emmo:EMMO_967080e5_2f42_4eb2_a3a9_c58143e835f9 "electrode in which the active material is nickel oxide"@en .

:electrochemistry_76fe8fb2_868e_48eb_95ca_fc6acd6f5fc9 a owl:Class ;
    rdfs:label "TitaniumDioxideElectrode"@en ;
    rdfs:comment "electrode in which the active material is titanium dioxide"@en ;
    rdfs:subClassOf [ a owl:Restriction ;
            owl:onProperty :electrochemistry_860aa941_5ff9_4452_8a16_7856fad07bee ;
            owl:someValuesFrom chems:substance_d673ceb2_3045_4e2e_8cad_56f5169b542f ],
        :electrochemistry_9c557caa_61e2_4fa9_a517_4bad01a68122,
        :electrochemistry_e4b6cb36_4dac_49e3_871d_40bcfca943a5 ;
    owl:deprecated true ;
    skos:altLabel "TiO2Electrode"@en ;
    skos:prefLabel "TitaniumDioxideElectrode"@en ;
    emmo:EMMO_967080e5_2f42_4eb2_a3a9_c58143e835f9 "electrode in which the active material is titanium dioxide"@en .

:electrochemistry_780aeb7b_9eb2_4324_ba2d_1a874136b4e5 a owl:Class ;
    rdfs:label "Cylindrical"@en ;
    rdfs:comment "a form factor describing a cylindrical cell, which has the shape of a cylinder nominally described by a height and diameter"@en ;
    rdfs:subClassOf :electrochemistry_1586ef26_6d30_49e3_ae32_b4c9fc181941 ;
    skos:prefLabel "Cylindrical"@en ;
    emmo:EMMO_967080e5_2f42_4eb2_a3a9_c58143e835f9 "a form factor describing a cylindrical cell, which has the shape of a cylinder nominally described by a height and diameter"@en .

:electrochemistry_78f75a64_55b6_4243_a35e_3d279c83209b a owl:Class ;
    rdfs:label "PhosphoricAcidSolution"@en ;
    rdfs:comment "a solution of phosphoric acid (H3PO4) dissolved in water (H2O)"@en ;
    rdfs:subClassOf :electrochemistry_6592d8cc_4ce4_42ca_b010_6bfc4a8444d2 ;
    owl:deprecated true ;
    skos:prefLabel "PhosphoricAcidSolution"@en ;
    emmo:EMMO_967080e5_2f42_4eb2_a3a9_c58143e835f9 "a solution of phosphoric acid (H3PO4) dissolved in water (H2O)"@en .

:electrochemistry_79e12290_d1e5_4c41_916c_18f1e4d7fb51 a owl:Class ;
    rdfs:label "SiliconBasedElectrode"@en ;
    rdfs:comment "an electrode in which the primary active material consists of silicon or silicon compounds"@en ;
    rdfs:subClassOf :electrochemistry_9a823d64_9d10_4a29_9cbd_9bbdad7985bc ;
    skos:prefLabel "SiliconBasedElectrode"@en ;
    emmo:EMMO_967080e5_2f42_4eb2_a3a9_c58143e835f9 "an electrode in which the primary active material consists of silicon or silicon compounds"@en .

:electrochemistry_7b811780_7251_481b_a4d3_97d437955099 a owl:Class ;
    rdfs:label "CobaltBasedElectrode"@en ;
    rdfs:comment "an electrode in which the primary active material consists of cobalt or cobalt compounds"@en ;
    rdfs:subClassOf :electrochemistry_9a823d64_9d10_4a29_9cbd_9bbdad7985bc ;
    owl:deprecated true ;
    skos:prefLabel "CobaltBasedElectrode"@en ;
    emmo:EMMO_967080e5_2f42_4eb2_a3a9_c58143e835f9 "an electrode in which the primary active material consists of cobalt or cobalt compounds"@en .

:electrochemistry_7b9db6b3_36f0_4b5d_acbb_9284a9054a09 a owl:Class ;
    rdfs:label "IndiumBasedElectrode"@en ;
    rdfs:comment "an electrode in which the primary active material consists of indium or indium compounds"@en ;
    rdfs:subClassOf :electrochemistry_9a823d64_9d10_4a29_9cbd_9bbdad7985bc ;
    skos:prefLabel "IndiumBasedElectrode"@en ;
    emmo:EMMO_967080e5_2f42_4eb2_a3a9_c58143e835f9 "an electrode in which the primary active material consists of indium or indium compounds"@en .

:electrochemistry_7cc8b738_3462_4592_ba83_951a8d50fef7 a owl:Class ;
    rdfs:label "CaesiumBasedElectrode"@en ;
    rdfs:comment "an electrode in which the primary active material consists of caesium or caesium compounds"@en ;
    rdfs:subClassOf :electrochemistry_9a823d64_9d10_4a29_9cbd_9bbdad7985bc ;
    skos:prefLabel "CaesiumBasedElectrode"@en ;
    emmo:EMMO_967080e5_2f42_4eb2_a3a9_c58143e835f9 "an electrode in which the primary active material consists of caesium or caesium compounds"@en .

:electrochemistry_7cef0da2_8de3_418e_b390_cce9a5d3c129 a owl:Class ;
    rdfs:label "OpenCellFoam"@en ;
    rdfs:comment "a lightweight, porous material characterized by a network of interconnected pores, typically made from metals or polymers, which allows for high gas and liquid permeability and is used in applications such as filtration, thermal insulation, and energy absorption"@en ;
    rdfs:subClassOf emmo:EMMO_ec7464a9_d99d_45f8_965b_4e9230ea8356 ;
    skos:altLabel "ReticulatedFoam"@en ;
    skos:prefLabel "OpenCellFoam"@en ;
    emmo:EMMO_26bf1bef_d192_4da6_b0eb_d2209698fb54 "https://www.wikidata.org/wiki/Q1312510" ;
    emmo:EMMO_967080e5_2f42_4eb2_a3a9_c58143e835f9 "a lightweight, porous material characterized by a network of interconnected pores, typically made from metals or polymers, which allows for high gas and liquid permeability and is used in applications such as filtration, thermal insulation, and energy absorption"@en ;
    emmo:EMMO_c84c6752_6d64_48cc_9500_e54a3c34898d "https://en.wikipedia.org/wiki/Reticulated_foam" .

:electrochemistry_7f168ebc_4c78_459c_9a39_bddaa57e214c a owl:Class ;
    rdfs:label "GrahameModel"@en ;
    rdfs:comment "a modification of the Stern model that considers the double layer as three regions separated by the inner Helmholtz plane and the outer Helmholtz plane"@en ;
    rdfs:subClassOf :electrochemistry_ac9723d1_bac0_4109_874e_32849de9299b ;
    skos:prefLabel "GrahameModel"@en ;
    emmo:EMMO_967080e5_2f42_4eb2_a3a9_c58143e835f9 "a modification of the Stern model that considers the double layer as three regions separated by the inner Helmholtz plane and the outer Helmholtz plane"@en ;
    emmo:EMMO_c7b62dd7_063a_4c2a_8504_42f7264ba83f "proposed by D. C. Grahame in 1947"@en .

:electrochemistry_7ffe1cb6_f87e_4b4a_8ce7_c98e2a584cb1 a owl:Class ;
    rdfs:label "RutheniumBasedElectrode"@en ;
    rdfs:comment "an electrode in which the primary active material consists of ruthenium or ruthenium compounds"@en ;
    rdfs:subClassOf :electrochemistry_9a823d64_9d10_4a29_9cbd_9bbdad7985bc ;
    skos:prefLabel "RutheniumBasedElectrode"@en ;
    emmo:EMMO_967080e5_2f42_4eb2_a3a9_c58143e835f9 "an electrode in which the primary active material consists of ruthenium or ruthenium compounds"@en .

:electrochemistry_80fdbd63_9b7a_462b_a8cb_b50f5f6ab182 a owl:Class ;
    rdfs:label "LiquidGalliumElectrode"@en ;
    rdfs:comment "a liquid electrode with an active material of gallium"@en ;
    rdfs:subClassOf [ a owl:Restriction ;
            owl:onProperty :electrochemistry_860aa941_5ff9_4452_8a16_7856fad07bee ;
            owl:someValuesFrom chems:substance_73d4606c_7460_4a5c_9413_793bdf35753e ],
        :electrochemistry_9fd49892_cf6d_482e_a6c3_5f763948ec29 ;
    skos:prefLabel "LiquidGalliumElectrode"@en ;
    emmo:EMMO_967080e5_2f42_4eb2_a3a9_c58143e835f9 "a liquid electrode with an active material of gallium"@en .

:electrochemistry_8112c7ba_e58a_463b_8661_b836bb6d7c86 a owl:Class ;
    rdfs:label "P32173115" ;
    rdfs:comment "a prismatic case with a nominal length of 32 mm, width of 173 mm, and height of 115 mm"@en ;
    rdfs:subClassOf :electrochemistry_43cd6e14_dd43_41b5_b5b4_344d53841603 ;
    skos:altLabel "BEV1",
        "P32/173/115" ;
    skos:prefLabel "P32173115" ;
    emmo:EMMO_967080e5_2f42_4eb2_a3a9_c58143e835f9 "a prismatic case with a nominal length of 32 mm, width of 173 mm, and height of 115 mm"@en .

:electrochemistry_82b66bfe_ec25_417b_ba65_b631ddaaca0e a owl:Class ;
    rdfs:label "SaturatedCalomelElectrode"@en ;
    rdfs:comment "A reference electrode based on the reaction between elemental mercury and mercury(I) chloride."@en ;
    rdfs:subClassOf :electrochemistry_7729c34e_1ae9_403d_b933_1765885e7f29 ;
    skos:prefLabel "SaturatedCalomelElectrode"@en ;
    emmo:EMMO_26bf1bef_d192_4da6_b0eb_d2209698fb54 "https://www.wikidata.org/wiki/Q898591" ;
    emmo:EMMO_967080e5_2f42_4eb2_a3a9_c58143e835f9 "A reference electrode based on the reaction between elemental mercury and mercury(I) chloride."@en ;
    emmo:EMMO_c84c6752_6d64_48cc_9500_e54a3c34898d "https://en.wikipedia.org/wiki/Saturated_calomel_electrode"@en .

:electrochemistry_82c70935_0aea_454b_92bf_17fb0b488012 a owl:Class ;
    rdfs:label "ZincOxideElectrode"@en ;
    rdfs:comment "electrode in which the active material is zinc oxide"@en ;
    rdfs:subClassOf [ a owl:Restriction ;
            owl:onProperty :electrochemistry_860aa941_5ff9_4452_8a16_7856fad07bee ;
            owl:someValuesFrom chems:substance_848003a2_71ee_4967_8039_354c907ec7f4 ],
        :electrochemistry_e4b6cb36_4dac_49e3_871d_40bcfca943a5 ;
    owl:deprecated true ;
    skos:altLabel "ZnOElectrode"@en ;
    skos:prefLabel "ZincOxideElectrode"@en ;
    emmo:EMMO_967080e5_2f42_4eb2_a3a9_c58143e835f9 "electrode in which the active material is zinc oxide"@en .

:electrochemistry_82fef384_8eec_4765_b707_5397054df594 a owl:Class ;
    rdfs:label "ConductiveAdditive"@en ;
    rdfs:comment "a material added to an electrode for the purpose of increasing its electronic conductivity."@en ;
    rdfs:subClassOf :electrochemistry_0a399f3f_b873_41f5_be1f_9b6df75cc30a ;
    skos:altLabel "ElectronicallyConductiveElectrodeAdditive"@en ;
    skos:example "carbon black"@en ;
    skos:prefLabel "ConductiveAdditive"@en ;
    emmo:EMMO_967080e5_2f42_4eb2_a3a9_c58143e835f9 "a material added to an electrode for the purpose of increasing its electronic conductivity."@en .

:electrochemistry_83ee23b3_2f5c_4afa_b972_ac85e91d7306 a owl:Class ;
    rdfs:label "NormalHydrogenElectrode"@en ;
    rdfs:comment "potential of a platinum electrode in 1 M acid solution."@en ;
    rdfs:subClassOf :electrochemistry_7729c34e_1ae9_403d_b933_1765885e7f29 ;
    skos:altLabel "NHE"@en ;
    skos:prefLabel "NormalHydrogenElectrode"@en ;
    emmo:EMMO_26bf1bef_d192_4da6_b0eb_d2209698fb54 "https://www.wikidata.org/wiki/Q115694592" ;
    emmo:EMMO_967080e5_2f42_4eb2_a3a9_c58143e835f9 "potential of a platinum electrode in 1 M acid solution."@en ;
    emmo:EMMO_c7b62dd7_063a_4c2a_8504_42f7264ba83f "hydrogen gas at 1 atm pressures is bubbled through the acid solution"@en .

:electrochemistry_85c4b478_645a_459e_8431_5a9d864ca02e a owl:Class ;
    rdfs:label "CarbonCloth"@en ;
    rdfs:comment "a woven fabric made from carbon fibers, offering flexibility, high electrical conductivity, and durability, commonly used in high-performance fuel cells"@en ;
    rdfs:subClassOf emmo:EMMO_ec7464a9_d99d_45f8_965b_4e9230ea8356 ;
    skos:prefLabel "CarbonCloth"@en ;
    emmo:EMMO_967080e5_2f42_4eb2_a3a9_c58143e835f9 "a woven fabric made from carbon fibers, offering flexibility, high electrical conductivity, and durability, commonly used in high-performance fuel cells"@en .

:electrochemistry_88100e2c_0f6e_4483_afbf_30029a6702c6 a owl:Class ;
    rdfs:label "R731" ;
    rdfs:comment "a coin case with a nominal diameter of 7.9 mm and a height of 3.1 mm"@en ;
    rdfs:subClassOf :electrochemistry_3979cd56_6256_414d_966c_7f723bf71e37 ;
    skos:prefLabel "R731" ;
    emmo:EMMO_967080e5_2f42_4eb2_a3a9_c58143e835f9 "a coin case with a nominal diameter of 7.9 mm and a height of 3.1 mm"@en .

:electrochemistry_885ffc4d_2b29_42d6_8597_6fc879c21d60 a owl:Class ;
    rdfs:label "R2335" ;
    rdfs:comment "a coin case with a nominal diameter of 23.0 mm and a height of 3.5 mm"@en ;
    rdfs:subClassOf :electrochemistry_3979cd56_6256_414d_966c_7f723bf71e37 ;
    skos:prefLabel "R2335" ;
    emmo:EMMO_967080e5_2f42_4eb2_a3a9_c58143e835f9 "a coin case with a nominal diameter of 23.0 mm and a height of 3.5 mm"@en .

:electrochemistry_8968eb7a_9a65_4286_a596_c31b998df329 a owl:Class ;
    rdfs:label "SodiumIronHexacyanoferrateElectrode"@en ;
    rdfs:comment "electrode in which the active material is sodium iron hexacyanoferrate"@en ;
    rdfs:subClassOf :electrochemistry_e4b6cb36_4dac_49e3_871d_40bcfca943a5 ;
    owl:deprecated true ;
    skos:prefLabel "SodiumIronHexacyanoferrateElectrode"@en ;
    emmo:EMMO_967080e5_2f42_4eb2_a3a9_c58143e835f9 "electrode in which the active material is sodium iron hexacyanoferrate"@en .

:electrochemistry_8b40856f_1ca2_4137_9616_7fb624671909 a owl:Class ;
    rdfs:label "AirElectrode"@en ;
    rdfs:comment "a gas diffusion electrode in which the gas is air"@en ;
    rdfs:subClassOf [ a owl:Restriction ;
            owl:onProperty emmo:EMMO_dba27ca1_33c9_4443_a912_1519ce4c39ec ;
            owl:someValuesFrom :electrochemistry_a3b53904_22b1_42a9_a515_c8a3aed7e841 ],
        :electrochemistry_bbb1d95b_72d1_44f6_b07e_a3d7d41ac215 ;
    skos:prefLabel "AirElectrode"@en ;
    emmo:EMMO_967080e5_2f42_4eb2_a3a9_c58143e835f9 "a gas diffusion electrode in which the gas is air"@en ;
    emmo:EMMO_c7b62dd7_063a_4c2a_8504_42f7264ba83f "The reaction occuring in an air electrode is typically the oxygen reduction reaction (ORR)."@en .

:electrochemistry_90103be0_9096_4f98_89c7_b5db01197858 a owl:Class ;
    rdfs:label "CalciumInsertionElectrode"@en ;
    rdfs:comment "an insertion electrode in which the guest molecule is calcium"@en ;
    rdfs:subClassOf :electrochemistry_757eae08_4d43_42d4_8b4e_8a0bfd2f9a1c ;
    owl:deprecated true ;
    skos:prefLabel "CalciumInsertionElectrode"@en ;
    emmo:EMMO_967080e5_2f42_4eb2_a3a9_c58143e835f9 "an insertion electrode in which the guest molecule is calcium"@en .

:electrochemistry_9017b8b9_e21e_4961_a3c1_c0aeef3fe795 a owl:Class ;
    rdfs:label "R2020" ;
    rdfs:comment "a coin case with a nominal diameter of 20.0 mm and a height of 2.0 mm"@en ;
    rdfs:subClassOf :electrochemistry_3979cd56_6256_414d_966c_7f723bf71e37 ;
    skos:prefLabel "R2020" ;
    emmo:EMMO_967080e5_2f42_4eb2_a3a9_c58143e835f9 "a coin case with a nominal diameter of 20.0 mm and a height of 2.0 mm"@en .

:electrochemistry_9109b3f6_112b_456d_ae45_b82c271c656b a owl:Class ;
    rdfs:label "LithiumManganeseIronPhosphateElectrode"@en ;
    rdfs:comment "electrode in which the active material is lithium manganese iron phosphate"@en ;
    rdfs:subClassOf :electrochemistry_468b3b63_b62a_4110_8c7e_40fffd5fdfd6,
        :electrochemistry_e4b6cb36_4dac_49e3_871d_40bcfca943a5 ;
    owl:deprecated true ;
    skos:altLabel "LMFPElectrode"@en ;
    skos:prefLabel "LithiumManganeseIronPhosphateElectrode"@en ;
    emmo:EMMO_967080e5_2f42_4eb2_a3a9_c58143e835f9 "electrode in which the active material is lithium manganese iron phosphate"@en .

:electrochemistry_93358d9b_8976_42d0_84ae_e5a2400c3ea7 a owl:Class ;
    rdfs:label "P1312085" ;
    rdfs:comment "a prismatic case with a nominal length of 13 mm, width of 120 mm, and height of 85 mm"@en ;
    rdfs:subClassOf :electrochemistry_43cd6e14_dd43_41b5_b5b4_344d53841603 ;
    skos:altLabel "HEV1",
        "P13/120/85" ;
    skos:prefLabel "P1312085" ;
    emmo:EMMO_967080e5_2f42_4eb2_a3a9_c58143e835f9 "a prismatic case with a nominal length of 13 mm, width of 120 mm, and height of 85 mm"@en .

:electrochemistry_94209cd8_f68f_40e6_ac70_cfb97a16e593 a owl:Class ;
    rdfs:label "R512" ;
    rdfs:comment "a coin case with a nominal diameter of 5.8 mm and a height of 1.3 mm"@en ;
    rdfs:subClassOf :electrochemistry_3979cd56_6256_414d_966c_7f723bf71e37 ;
    skos:prefLabel "R512" ;
    emmo:EMMO_967080e5_2f42_4eb2_a3a9_c58143e835f9 "a coin case with a nominal diameter of 5.8 mm and a height of 1.3 mm"@en .

:electrochemistry_94497aca_52a0_48e3_9b76_157b050e35b3 a owl:Class ;
    rdfs:label "R2032" ;
    rdfs:comment "a coin case with a nominal diameter of 20.0 mm and a height of 3.2 mm"@en ;
    rdfs:subClassOf :electrochemistry_3979cd56_6256_414d_966c_7f723bf71e37 ;
    skos:prefLabel "R2032" ;
    emmo:EMMO_967080e5_2f42_4eb2_a3a9_c58143e835f9 "a coin case with a nominal diameter of 20.0 mm and a height of 3.2 mm"@en ;
    emmo:EMMO_c7b62dd7_063a_4c2a_8504_42f7264ba83f "very common case for lithim metal cells"@en .

:electrochemistry_948234f6_4095_4419_af30_00ab297a7694 a owl:Class ;
    rdfs:label "P32173225" ;
    rdfs:comment "a prismatic case with a nominal length of 32 mm, width of 173 mm, and height of 225"@en ;
    rdfs:subClassOf :electrochemistry_43cd6e14_dd43_41b5_b5b4_344d53841603 ;
    skos:altLabel "BEV3",
        "P32/173/225" ;
    skos:prefLabel "P32173225" ;
    emmo:EMMO_967080e5_2f42_4eb2_a3a9_c58143e835f9 "a prismatic case with a nominal length of 32 mm, width of 173 mm, and height of 225"@en .

:electrochemistry_952c8c3a_df21_4dd1_8d8c_380e43dc8c78 a owl:Class ;
    rdfs:label "AluminiumBasedElectrode"@en ;
    rdfs:comment "an electrode in which the primary active material consists of aluminium or aluminium compounds"@en ;
    rdfs:subClassOf :electrochemistry_9a823d64_9d10_4a29_9cbd_9bbdad7985bc ;
    skos:prefLabel "AluminiumBasedElectrode"@en ;
    emmo:EMMO_967080e5_2f42_4eb2_a3a9_c58143e835f9 "an electrode in which the primary active material consists of aluminium or aluminium compounds"@en .

:electrochemistry_95d841eb_2002_4411_9f8e_927d6c60e4b3 a owl:Class ;
    rdfs:label "R26650" ;
    rdfs:comment "a cylindrical case with a nominal diameter of 26 mm and height of 65 mm"@en ;
    rdfs:subClassOf :electrochemistry_b1cf9fee_2164_4f95_8204_90f717373a8a ;
    skos:altLabel "R26/65" ;
    skos:prefLabel "R26650" ;
    emmo:EMMO_967080e5_2f42_4eb2_a3a9_c58143e835f9 "a cylindrical case with a nominal diameter of 26 mm and height of 65 mm"@en .

:electrochemistry_98d5101e_cd11_4a0d_b856_6fcd8aad132e a owl:Class ;
    rdfs:label "BellevilleWasher"@en ;
    rdfs:comment "a type of spring, in the form of a conical washer"@en ;
    rdfs:subClassOf :electrochemistry_872b11e1_8bb3_4a2a_af90_bbaa0055d01e ;
    skos:prefLabel "BellevilleWasher"@en ;
    emmo:EMMO_26bf1bef_d192_4da6_b0eb_d2209698fb54 "https://www.wikidata.org/wiki/Q3056595"@en ;
    emmo:EMMO_967080e5_2f42_4eb2_a3a9_c58143e835f9 "a type of spring, in the form of a conical washer"@en .

:electrochemistry_99475d6c_304c_4d6b_9eca_fbc42f768be5 a owl:Class ;
    rdfs:label "R3032" ;
    rdfs:comment "a coin case with a nominal diameter of 30.0 mm and a height of 3.2 mm"@en ;
    rdfs:subClassOf :electrochemistry_3979cd56_6256_414d_966c_7f723bf71e37 ;
    skos:prefLabel "R3032" ;
    emmo:EMMO_967080e5_2f42_4eb2_a3a9_c58143e835f9 "a coin case with a nominal diameter of 30.0 mm and a height of 3.2 mm"@en .

:electrochemistry_9a23f61b_fef0_40f8_84f9_2057f90f6a95 a owl:Class ;
    rdfs:label "R932" ;
    rdfs:comment "a coin case with a nominal diameter of 9.3 mm and a height of 3.2 mm"@en ;
    rdfs:subClassOf :electrochemistry_3979cd56_6256_414d_966c_7f723bf71e37 ;
    skos:prefLabel "R932" ;
    emmo:EMMO_967080e5_2f42_4eb2_a3a9_c58143e835f9 "a coin case with a nominal diameter of 9.3 mm and a height of 3.2 mm"@en ;
    emmo:EMMO_c7b62dd7_063a_4c2a_8504_42f7264ba83f "8 of these in series are used to form an A23 battery"@en,
        "rarely used independently"@en .

:electrochemistry_9b6853e7_3412_463d_b5a9_82c14acebf7d a owl:Class ;
    rdfs:label "CatholyteTank"@en ;
    rdfs:comment "a tank for holding catholyte"@en ;
    rdfs:subClassOf emmo:EMMO_f76884f7_964e_488e_9bb7_1b2453e9e817 ;
    skos:prefLabel "CatholyteTank"@en ;
    emmo:EMMO_967080e5_2f42_4eb2_a3a9_c58143e835f9 "a tank for holding catholyte"@en ;
    emmo:EMMO_c7b62dd7_063a_4c2a_8504_42f7264ba83f "usually used in a flow cell system"@en .

:electrochemistry_9bc02662_9799_4593_906d_638a841d7352 a owl:Class ;
    rdfs:label "HelmholtzModel"@en ;
    rdfs:comment "a structural representation of the double layer that states that the accumulation of electric charge on the surface of the electrode is balanced by a layer of ions in the electrolyte"@en ;
    rdfs:subClassOf :electrochemistry_ac9723d1_bac0_4109_874e_32849de9299b ;
    skos:prefLabel "HelmholtzModel"@en ;
    emmo:EMMO_967080e5_2f42_4eb2_a3a9_c58143e835f9 "a structural representation of the double layer that states that the accumulation of electric charge on the surface of the electrode is balanced by a layer of ions in the electrolyte"@en ;
    emmo:EMMO_c7b62dd7_063a_4c2a_8504_42f7264ba83f "proposed by Hermann von Helmholtz in 1853"@en,
        "the first model for the double layer"@en .

:electrochemistry_9c0e683b_40d7_4786_b31f_910dd68b2ea8 a owl:Class ;
    rdfs:label "R2012" ;
    rdfs:comment "a coin case with a nominal diameter of 20.0 mm and a height of 1.2 mm"@en ;
    rdfs:subClassOf :electrochemistry_3979cd56_6256_414d_966c_7f723bf71e37 ;
    skos:prefLabel "R2012" ;
    emmo:EMMO_967080e5_2f42_4eb2_a3a9_c58143e835f9 "a coin case with a nominal diameter of 20.0 mm and a height of 1.2 mm"@en .

:electrochemistry_9ceffffd_b918_48c2_aad9_5db16fa6149d a owl:Class ;
    rdfs:label "R2025" ;
    rdfs:comment "a coin case with a nominal diameter of 20.0 mm and a height of 2.5 mm"@en ;
    rdfs:subClassOf :electrochemistry_3979cd56_6256_414d_966c_7f723bf71e37 ;
    skos:prefLabel "R2025" ;
    emmo:EMMO_967080e5_2f42_4eb2_a3a9_c58143e835f9 "a coin case with a nominal diameter of 20.0 mm and a height of 2.5 mm"@en ;
    emmo:EMMO_c7b62dd7_063a_4c2a_8504_42f7264ba83f "often used in wrist watches and automobile remotes"@en .

:electrochemistry_9d7e5fea_a49a_4a19_a8de_8e24c60e420c a owl:Class ;
    rdfs:label "NernstEinsteinEquation"@en ;
    rdfs:comment "an equation relating the limiting molar conductivity _m^0  to the ionic diffusion coefficients."@en ;
    rdfs:seeAlso "KohlrauschsLaw"@en ;
    rdfs:subClassOf :electrochemistry_3d805c2a_4801_440e_9e4d_0fa5585c76ae ;
    skos:prefLabel "NernstEinsteinEquation"@en ;
    emmo:EMMO_26bf1bef_d192_4da6_b0eb_d2209698fb54 "https://www.wikidata.org/wiki/Q9325636" ;
    emmo:EMMO_967080e5_2f42_4eb2_a3a9_c58143e835f9 "an equation relating the limiting molar conductivity _m^0  to the ionic diffusion coefficients."@en ;
    emmo:EMMO_c7b62dd7_063a_4c2a_8504_42f7264ba83f "\\Lambda_m^0 = (F^2/(R*T)) * (v_{+} * z_{+}^2 * D_{+} + v_{} * z_{}^2 * D_{})"@en ;
    emmo:EMMO_c84c6752_6d64_48cc_9500_e54a3c34898d "https://en.wikipedia.org/wiki/Einstein_relation_(kinetic_theory)#Nernst%E2%80%93Einstein_equation"@en .

:electrochemistry_9da958fc_f76d_4654_8a78_99b5f98c118c a owl:Class ;
    rdfs:label "ElectrochemicalHalfCell"@en ;
    rdfs:comment "a system comprising one electrode in contact with an ionic conductor."@en ;
    rdfs:subClassOf [ a owl:Restriction ;
            owl:onProperty emmo:EMMO_e1097637_70d2_4895_973f_2396f04fa204 ;
            owl:someValuesFrom :electrochemistry_7fc10197_41d9_4c1e_a107_928f03eb2d36 ],
        [ a owl:Restriction ;
            owl:onProperty :electrochemistry_3bd08946_4e81_455d_9fca_dc7a5ead9315 ;
            owl:someValuesFrom emmo:EMMO_bc37743c_37c4_4ec7_9d58_d1aae5567352 ],
        [ a owl:Restriction ;
            owl:onProperty :electrochemistry_578c41e9_ee01_4840_9c8c_04ab6e4e6241 ;
            owl:someValuesFrom :electrochemistry_0f007072_a8dd_4798_b865_1bf9363be627 ],
        emmo:EMMO_b9522e56_1fac_4766_97e6_428605fabd3e ;
    skos:altLabel "HalfCell"@en ;
    skos:note "Do not conflate a half-cell (a physical arrangement) with a half-reaction (a formal redox equation component)."@en ;
    skos:prefLabel "ElectrochemicalHalfCell"@en ;
    skos:scopeNote "A half-cell becomes operational when paired with at least one other half-cell to form an electrochemical cell; the pair allows charge balance through ionic and electronic pathways."@en ;
    emmo:EMMO_0fa6566e_500f_4d24_baa9_b2b22c9a0b72 "Do not conflate an ElectrochemicalHalfCell (the combination of one electrode and one electrolyte) with a half-cell device, which is an experimental setup used to measure the properties of an electrode relative to a reference electrode."@en ;
    emmo:EMMO_26bf1bef_d192_4da6_b0eb_d2209698fb54 "https://www.wikidata.org/wiki/Q903509" ;
    emmo:EMMO_4c8480cf_56de_41da_8699_f12a9033313a "A single half-cell cannot sustain continuous current by itself; closed-circuit operation requires a counter half-cell and an external electronic path."@en ;
    emmo:EMMO_967080e5_2f42_4eb2_a3a9_c58143e835f9 "a system comprising one electrode in contact with an ionic conductor."@en ;
    emmo:EMMO_c84c6752_6d64_48cc_9500_e54a3c34898d "https://en.wikipedia.org/wiki/Half-cell"@en .

:electrochemistry_9dc236d9_c962_4fcc_94db_911a25241472 a owl:Class ;
    rdfs:label "R19660" ;
    rdfs:comment "a cylindrical case with a nominal diameter of 19 mm and height of 66 mm"@en ;
    rdfs:subClassOf :electrochemistry_b1cf9fee_2164_4f95_8204_90f717373a8a ;
    skos:altLabel "R19/66" ;
    skos:prefLabel "R19660" ;
    emmo:EMMO_967080e5_2f42_4eb2_a3a9_c58143e835f9 "a cylindrical case with a nominal diameter of 19 mm and height of 66 mm"@en .

:electrochemistry_9e24d403_8531_416e_a9ec_d1ec5508bcb1 a owl:Class ;
    rdfs:label "SodiumCobaltPhosphateElectrode"@en ;
    rdfs:comment "electrode in which the active material is sodium cobalt phosphate"@en ;
    rdfs:subClassOf [ a owl:Restriction ;
            owl:onProperty :electrochemistry_860aa941_5ff9_4452_8a16_7856fad07bee ;
            owl:someValuesFrom chems:substance_0bdf0bb9_41fc_455d_af11_a249e24acdf6 ],
        :electrochemistry_838c115b_6bc9_4ce8_9f8d_86a6bf67742a,
        :electrochemistry_e4b6cb36_4dac_49e3_871d_40bcfca943a5 ;
    owl:deprecated true ;
    skos:prefLabel "SodiumCobaltPhosphateElectrode"@en ;
    emmo:EMMO_967080e5_2f42_4eb2_a3a9_c58143e835f9 "electrode in which the active material is sodium cobalt phosphate"@en .

:electrochemistry_a10ede13_c895_4f56_a728_b1aab512b31b a owl:Class ;
    rdfs:label "TinBasedElectrode"@en ;
    rdfs:comment "an electrode in which the primary active material consists of tin or tin compounds"@en ;
    rdfs:subClassOf :electrochemistry_9a823d64_9d10_4a29_9cbd_9bbdad7985bc ;
    skos:prefLabel "TinBasedElectrode"@en ;
    emmo:EMMO_967080e5_2f42_4eb2_a3a9_c58143e835f9 "an electrode in which the primary active material consists of tin or tin compounds"@en .

:electrochemistry_a1ec9e3c_c624_4848_af13_89a6bc54d77c a owl:Class ;
    rdfs:label "PastedPlate"@en ;
    rdfs:comment "plate in which the active material is applied as a paste to a conductive current collector"@en ;
    rdfs:subClassOf :electrochemistry_92147e31_d015_4889_a092_04fbab033f15 ;
    skos:altLabel "PastedElectrode"@en ;
    skos:prefLabel "PastedPlate"@en ;
    emmo:EMMO_50c298c2_55a2_4068_b3ac_4e948c33181f "https://www.electropedia.org/iev/iev.nsf/display?openform&ievref=482-02-03"@en ;
    emmo:EMMO_967080e5_2f42_4eb2_a3a9_c58143e835f9 "plate in which the active material is applied as a paste to a conductive current collector"@en .

:electrochemistry_a277e420_2483_44d5_a2bc_4e421dea231a a owl:Class ;
    rdfs:label "R926" ;
    rdfs:comment "a coin case with a nominal diameter of 9.5 mm and a height of 2.6 mm"@en ;
    rdfs:subClassOf :electrochemistry_3979cd56_6256_414d_966c_7f723bf71e37 ;
    skos:altLabel "R57" ;
    skos:prefLabel "R926" ;
    emmo:EMMO_967080e5_2f42_4eb2_a3a9_c58143e835f9 "a coin case with a nominal diameter of 9.5 mm and a height of 2.6 mm"@en .

:electrochemistry_a3745142_b97a_4e19_b7ed_03599f56e81d a owl:Class ;
    rdfs:label "SilverOxideElectrode"@en ;
    rdfs:comment "an electrode in which the primary active material consists of manganese dioxide or vmanganese dioxide compounds"@en ;
    rdfs:subClassOf [ a owl:Restriction ;
            owl:onProperty :electrochemistry_860aa941_5ff9_4452_8a16_7856fad07bee ;
            owl:someValuesFrom chems:substance_2a540939_3908_4f85_92f9_c46da7d4e9cb ],
        :electrochemistry_e4b6cb36_4dac_49e3_871d_40bcfca943a5 ;
    skos:prefLabel "SilverOxideElectrode"@en ;
    emmo:EMMO_967080e5_2f42_4eb2_a3a9_c58143e835f9 "an electrode in which the primary active material consists of manganese dioxide or vmanganese dioxide compounds"@en ;
    emmo:EMMO_c7b62dd7_063a_4c2a_8504_42f7264ba83f "the combination with zinc metal and an alkali metal hydoxide electrolyte is designated using IEC electrochemical system letter code S"@en .

:electrochemistry_a4e7c3d6_45bd_402a_962f_5d4b88af84ff a owl:Class ;
    rdfs:label "R2412" ;
    rdfs:comment "a coin case with a nominal diameter of 24.5 mm and a height of 1.2 mm"@en ;
    rdfs:subClassOf :electrochemistry_3979cd56_6256_414d_966c_7f723bf71e37 ;
    skos:prefLabel "R2412" ;
    emmo:EMMO_967080e5_2f42_4eb2_a3a9_c58143e835f9 "a coin case with a nominal diameter of 24.5 mm and a height of 1.2 mm"@en .

:electrochemistry_a5c1b56f_5c82_4e3b_800e_5a280331348b a owl:Class ;
    rdfs:label "P2770102" ;
    rdfs:comment "a prismatic case with a nominal length of 27 mm, width of 70 mm, and height of 102 mm"@en ;
    rdfs:subClassOf :electrochemistry_43cd6e14_dd43_41b5_b5b4_344d53841603 ;
    skos:altLabel "P27/70/102" ;
    skos:prefLabel "P2770102" ;
    emmo:EMMO_967080e5_2f42_4eb2_a3a9_c58143e835f9 "a prismatic case with a nominal length of 27 mm, width of 70 mm, and height of 102 mm"@en .

:electrochemistry_a87d4b9d_ba91_4549_aed4_508d1160c0c0 a owl:Class ;
    rdfs:label "R2477" ;
    rdfs:comment "a coin case with a nominal diameter of 24.5 mm and a height of 7.7 mm"@en ;
    rdfs:subClassOf :electrochemistry_3979cd56_6256_414d_966c_7f723bf71e37 ;
    skos:prefLabel "R2477" ;
    emmo:EMMO_967080e5_2f42_4eb2_a3a9_c58143e835f9 "a coin case with a nominal diameter of 24.5 mm and a height of 7.7 mm"@en .

:electrochemistry_a8edd38f_f8a5_41fb_9fc7_48f1866fd699 a owl:Class ;
    rdfs:label "CopperOxideElectrode"@en ;
    rdfs:comment "electrode in which the active material is cupric oxide (copper (II) oxide)"@en ;
    rdfs:subClassOf [ a owl:Restriction ;
            owl:onProperty :electrochemistry_860aa941_5ff9_4452_8a16_7856fad07bee ;
            owl:someValuesFrom chems:substance_250fa43e_1f26_4ed8_b787_91a2325a8e7b ],
        :electrochemistry_26b19a7c_59ca_4e1b_8fb9_ba061c22531e,
        :electrochemistry_e4b6cb36_4dac_49e3_871d_40bcfca943a5 ;
    skos:altLabel "CupricOxideElectrode"@en ;
    skos:prefLabel "CopperOxideElectrode"@en ;
    emmo:EMMO_967080e5_2f42_4eb2_a3a9_c58143e835f9 "electrode in which the active material is cupric oxide (copper (II) oxide)"@en ;
    emmo:EMMO_c7b62dd7_063a_4c2a_8504_42f7264ba83f "the combination with lithium metal and an organic electrolyte is designated using IEC electrochemical system letter code G"@en .

:electrochemistry_aa5ed981_c11b_4c4f_b1fd_8c432e009484 a owl:Class ;
    rdfs:label "SternModel"@en ;
    rdfs:comment "describes the double layer as divided into two parts separated by the Stern plane, located about one hydrated ion radius from the electrode surface"@en ;
    rdfs:subClassOf :electrochemistry_ac9723d1_bac0_4109_874e_32849de9299b ;
    skos:prefLabel "SternModel"@en ;
    emmo:EMMO_967080e5_2f42_4eb2_a3a9_c58143e835f9 "describes the double layer as divided into two parts separated by the Stern plane, located about one hydrated ion radius from the electrode surface"@en ;
    emmo:EMMO_c7b62dd7_063a_4c2a_8504_42f7264ba83f "proposed by Otto Stern in 1924"@en .

:electrochemistry_aaafc5d6_050a_4c51_b1ca_db5839aad4de a owl:Class ;
    rdfs:label "R2450" ;
    rdfs:comment "a coin case with a nominal diameter of 24.5 mm and a height of 5.0 mm"@en ;
    rdfs:subClassOf :electrochemistry_3979cd56_6256_414d_966c_7f723bf71e37 ;
    skos:prefLabel "R2450" ;
    emmo:EMMO_967080e5_2f42_4eb2_a3a9_c58143e835f9 "a coin case with a nominal diameter of 24.5 mm and a height of 5.0 mm"@en .

:electrochemistry_abffe8cd_14d3_4437_84e6_5dfc61b057e8 a owl:Class ;
    rdfs:label "R1142" ;
    rdfs:comment "a coin case with a nominal diameter of 11.6 mm and a height of 4.2 mm"@en ;
    rdfs:subClassOf :electrochemistry_3979cd56_6256_414d_966c_7f723bf71e37 ;
    skos:altLabel "R43" ;
    skos:prefLabel "R1142" ;
    emmo:EMMO_967080e5_2f42_4eb2_a3a9_c58143e835f9 "a coin case with a nominal diameter of 11.6 mm and a height of 4.2 mm"@en .

:electrochemistry_ad9cdad6_66e8_471e_a7c6_b79f37c20814 a owl:Class ;
    rdfs:label "R32700" ;
    rdfs:comment "a cylindrical case with a nominal diameter of 32 mm and height of 70 mm"@en ;
    rdfs:subClassOf :electrochemistry_b1cf9fee_2164_4f95_8204_90f717373a8a ;
    skos:altLabel "R32/70" ;
    skos:prefLabel "R32700" ;
    emmo:EMMO_967080e5_2f42_4eb2_a3a9_c58143e835f9 "a cylindrical case with a nominal diameter of 32 mm and height of 70 mm"@en .

:electrochemistry_addf91e1_ba8c_4a3e_b1e9_092e3e1cc2b3 a owl:Class ;
    rdfs:label "NonAqueousInorganicElectrolyte"@en ;
    rdfs:comment "an electrolyte solution that contains no water and no organic species"@en ;
    rdfs:subClassOf :electrochemistry_5f9a9411_05f9_4576_acd3_81d7d41cfe98 ;
    skos:prefLabel "NonAqueousInorganicElectrolyte"@en ;
    emmo:EMMO_967080e5_2f42_4eb2_a3a9_c58143e835f9 "an electrolyte solution that contains no water and no organic species"@en .

:electrochemistry_af751d07_f0b7_43c7_911d_cba864189b2b a owl:Class ;
    rdfs:label "Pouch"@en ;
    rdfs:comment "a form factor describing a pouch cell, which has the shape of a rectangular prism where the thickness less than the length and the width and the case material is flexible"@en ;
    rdfs:subClassOf :electrochemistry_1586ef26_6d30_49e3_ae32_b4c9fc181941 ;
    skos:prefLabel "Pouch"@en ;
    emmo:EMMO_967080e5_2f42_4eb2_a3a9_c58143e835f9 "a form factor describing a pouch cell, which has the shape of a rectangular prism where the thickness less than the length and the width and the case material is flexible"@en .

:electrochemistry_af92a3ae_e870_4676_9ae7_cda277b1e6e1 a owl:Class ;
    rdfs:label "R2354" ;
    rdfs:comment "a coin case with a nominal diameter of 23.0 mm and a height of 5.4 mm"@en ;
    rdfs:subClassOf :electrochemistry_3979cd56_6256_414d_966c_7f723bf71e37 ;
    skos:prefLabel "R2354" ;
    emmo:EMMO_967080e5_2f42_4eb2_a3a9_c58143e835f9 "a coin case with a nominal diameter of 23.0 mm and a height of 5.4 mm"@en .

:electrochemistry_afe918c7_0634_40c1_9421_78ea2fe707e3 a owl:Class ;
    rdfs:label "P2770131" ;
    rdfs:comment "a prismatic case with a nominal length of 27 mm, width of 70 mm, and height of 131 mm"@en ;
    rdfs:subClassOf :electrochemistry_43cd6e14_dd43_41b5_b5b4_344d53841603 ;
    skos:altLabel "P27/70/131" ;
    skos:prefLabel "P2770131" ;
    emmo:EMMO_967080e5_2f42_4eb2_a3a9_c58143e835f9 "a prismatic case with a nominal length of 27 mm, width of 70 mm, and height of 131 mm"@en .

:electrochemistry_b3eb8c65_5644_45e3_9e17_0be6277c7962 a owl:Class ;
    rdfs:label "LithiumNickelManganeseCobaltOxideElectrode"@en ;
    rdfs:comment "electrode in which the active material is lithium nickel manganese cobalt"@en ;
    rdfs:subClassOf [ a owl:Restriction ;
            owl:onProperty :electrochemistry_860aa941_5ff9_4452_8a16_7856fad07bee ;
            owl:someValuesFrom chems:substance_3ac62305_acd6_4312_9e31_4f824bd2530d ],
        :electrochemistry_0d2aaaf4_1a8a_4a32_abd8_7d0fdf0ae9d2,
        :electrochemistry_e4b6cb36_4dac_49e3_871d_40bcfca943a5 ;
    owl:deprecated true ;
    skos:altLabel "NMCElectrode"@en ;
    skos:prefLabel "LithiumNickelManganeseCobaltOxideElectrode"@en ;
    emmo:EMMO_967080e5_2f42_4eb2_a3a9_c58143e835f9 "electrode in which the active material is lithium nickel manganese cobalt"@en .

:electrochemistry_b442217f_02f6_4991_aadf_22d81369223c a owl:Class ;
    rdfs:label "R1131" ;
    rdfs:comment "a coin case with a nominal diameter of 11.6 mm and a height of 3.1 mm"@en ;
    rdfs:subClassOf :electrochemistry_3979cd56_6256_414d_966c_7f723bf71e37 ;
    skos:altLabel "R54" ;
    skos:prefLabel "R1131" ;
    emmo:EMMO_967080e5_2f42_4eb2_a3a9_c58143e835f9 "a coin case with a nominal diameter of 11.6 mm and a height of 3.1 mm"@en .

:electrochemistry_b525a629_a679_464f_bc5b_b49d2fc82686 a owl:Class ;
    rdfs:label "ConductivityCell"@en ;
    rdfs:comment "a device used in electrochemistry to measure the resistance of a solution to determine its conductivity"@en ;
    rdfs:subClassOf :electrochemistry_0acd0fc2_1048_4604_8e90_bf4e84bd87df ;
    skos:note "Formed, in theory, by two 1 cm2 reversible electrodes spaced 1 cm apart, providing a uniform distribution of electrical field. In practice, however, a number of other configurations are used."@en ;
    skos:prefLabel "ConductivityCell"@en ;
    emmo:EMMO_967080e5_2f42_4eb2_a3a9_c58143e835f9 "a device used in electrochemistry to measure the resistance of a solution to determine its conductivity"@en .

:electrochemistry_b56a95e6_eea5_4a58_99aa_045fd28e75d3 a owl:Class ;
    rdfs:label "R527" ;
    rdfs:comment "a coin case with a nominal diameter of 5.8 mm and a height of 2.7 mm"@en ;
    rdfs:subClassOf :electrochemistry_3979cd56_6256_414d_966c_7f723bf71e37 ;
    skos:altLabel "R64" ;
    skos:prefLabel "R527" ;
    emmo:EMMO_967080e5_2f42_4eb2_a3a9_c58143e835f9 "a coin case with a nominal diameter of 5.8 mm and a height of 2.7 mm"@en .

:electrochemistry_b5e91259_cd97_4ed6_9ab2_4b18ef68a35a a owl:Class ;
    rdfs:label "LithiumVanadiumOxideElectrode"@en ;
    rdfs:comment "electrode in which the active material is lithium vanadium oxide"@en ;
    rdfs:subClassOf :electrochemistry_0ee59786_b090_444d_a46d_505797d07ca4,
        :electrochemistry_e4b6cb36_4dac_49e3_871d_40bcfca943a5 ;
    owl:deprecated true ;
    skos:prefLabel "LithiumVanadiumOxideElectrode"@en ;
    emmo:EMMO_967080e5_2f42_4eb2_a3a9_c58143e835f9 "electrode in which the active material is lithium vanadium oxide"@en .

:electrochemistry_b62a6b15_236a_48bf_a323_ccbfc295f934 a owl:ObjectProperty ;
    rdfs:label "hasCatholyte"@en ;
    rdfs:comment "relates a system to the portion of the electrolyte that is in contact with the cathode"@en ;
    rdfs:range :electrochemistry_fb0d9eef_92af_4628_8814_e065ca255d59 ;
    rdfs:subPropertyOf :electrochemistry_3bd08946_4e81_455d_9fca_dc7a5ead9315 ;
    skos:prefLabel "hasCatholyte"@en ;
    emmo:EMMO_967080e5_2f42_4eb2_a3a9_c58143e835f9 "relates a system to the portion of the electrolyte that is in contact with the cathode"@en .

:electrochemistry_bb2faf17_b819_4876_b17f_fa82917cf85d a owl:Class ;
    rdfs:label "R712" ;
    rdfs:comment "a coin case with a nominal diameter of 7.9 mm and a height of 1.3 mm"@en ;
    rdfs:subClassOf :electrochemistry_3979cd56_6256_414d_966c_7f723bf71e37 ;
    skos:prefLabel "R712" ;
    emmo:EMMO_967080e5_2f42_4eb2_a3a9_c58143e835f9 "a coin case with a nominal diameter of 7.9 mm and a height of 1.3 mm"@en .

:electrochemistry_bb710d71_98fa_48a1_85bc_d8f1ef2200da a owl:Class ;
    rdfs:label "LithiumNickelManganeseOxideLithiumIronPhosphateElectrode"@en ;
    rdfs:comment "an electrode with blended lithium nickel manganese oxide (LNMO) and lithium iron phosphate (LFP) active materials"@en ;
    rdfs:subClassOf [ a owl:Restriction ;
            owl:onProperty :electrochemistry_860aa941_5ff9_4452_8a16_7856fad07bee ;
            owl:someValuesFrom chems:substance_aa8e9cc4_5f66_4307_b1c8_26fac7653a90 ],
        [ a owl:Restriction ;
            owl:onProperty :electrochemistry_860aa941_5ff9_4452_8a16_7856fad07bee ;
            owl:someValuesFrom chems:substance_f3e7979a_e3ef_450a_8762_7d8778afe478 ],
        :electrochemistry_4839708a_3864_47eb_b719_373ff8874c61 ;
    owl:deprecated true ;
    skos:altLabel "LNMOLFPElectrode"@en ;
    skos:prefLabel "LithiumNickelManganeseOxideLithiumIronPhosphateElectrode"@en ;
    emmo:EMMO_967080e5_2f42_4eb2_a3a9_c58143e835f9 "an electrode with blended lithium nickel manganese oxide (LNMO) and lithium iron phosphate (LFP) active materials"@en .

:electrochemistry_bba6b94e_c0d7_40bf_a9d6_413ff458397c a owl:Class ;
    rdfs:label "P20100141" ;
    rdfs:comment "a prismatic case with a nominal length of 20 mm, width of 100 mm, and height of 141 mm"@en ;
    rdfs:subClassOf :electrochemistry_43cd6e14_dd43_41b5_b5b4_344d53841603 ;
    skos:altLabel "P20/100/141" ;
    skos:prefLabel "P20100141" ;
    emmo:EMMO_967080e5_2f42_4eb2_a3a9_c58143e835f9 "a prismatic case with a nominal length of 20 mm, width of 100 mm, and height of 141 mm"@en .

:electrochemistry_bd33779c_6f40_4354_ab5d_f6c17396414d a owl:Class ;
    rdfs:label "FuelCell"@en ;
    rdfs:comment "galvanic cell that transforms chemical energy from continuously supplied reactants to electric energy by an electrochemical process."@en ;
    rdfs:subClassOf :electrochemistry_0acd0fc2_1048_4604_8e90_bf4e84bd87df ;
    skos:prefLabel "FuelCell"@en ;
    emmo:EMMO_26bf1bef_d192_4da6_b0eb_d2209698fb54 "https://www.wikidata.org/wiki/Q180253"@en ;
    emmo:EMMO_50c298c2_55a2_4068_b3ac_4e948c33181f "https://www.electropedia.org/iev/iev.nsf/display?openform&ievref=114-03-05"@en ;
    emmo:EMMO_6dd685dd_1895_46e4_b227_be9f7d643c25 "https://dbpedia.org/page/Fuel_cell"@en ;
    emmo:EMMO_967080e5_2f42_4eb2_a3a9_c58143e835f9 "galvanic cell that transforms chemical energy from continuously supplied reactants to electric energy by an electrochemical process."@en ;
    emmo:EMMO_c84c6752_6d64_48cc_9500_e54a3c34898d "https://en.wikipedia.org/wiki/Fuel_cell"@en .

:electrochemistry_c066bf32_ed62_4a11_bf4f_25fe6e8e68b5 a owl:Class ;
    rdfs:label "R32134" ;
    rdfs:comment "a cylindrical case with a nominal diameter of 32 mm and height of 134 mm"@en ;
    rdfs:subClassOf :electrochemistry_b1cf9fee_2164_4f95_8204_90f717373a8a ;
    skos:altLabel "R32/134" ;
    skos:prefLabel "R32134" ;
    emmo:EMMO_967080e5_2f42_4eb2_a3a9_c58143e835f9 "a cylindrical case with a nominal diameter of 32 mm and height of 134 mm"@en .

:electrochemistry_c17b514b_57f2_4f72_9b95_c2950dd2aa7f a owl:ObjectProperty ;
    rdfs:label "hasFormFactor"@en ;
    rdfs:domain :electrochemistry_0acd0fc2_1048_4604_8e90_bf4e84bd87df ;
    rdfs:range :electrochemistry_1586ef26_6d30_49e3_ae32_b4c9fc181941 ;
    rdfs:subPropertyOf emmo:EMMO_e1097637_70d2_4895_973f_2396f04fa204 ;
    skos:prefLabel "hasFormFactor"@en .

:electrochemistry_c183f697_8995_477c_9ccd_5c12d98e3633 a owl:Class ;
    rdfs:label "PotassiumInsertionElectrode"@en ;
    rdfs:comment "an insertion electrode in which the guest molecule is potassium"@en ;
    rdfs:subClassOf :electrochemistry_757eae08_4d43_42d4_8b4e_8a0bfd2f9a1c ;
    owl:deprecated true ;
    skos:prefLabel "PotassiumInsertionElectrode"@en ;
    emmo:EMMO_967080e5_2f42_4eb2_a3a9_c58143e835f9 "an insertion electrode in which the guest molecule is potassium"@en .

:electrochemistry_c231227b_f318_4e59_ad90_6e91072903ed a owl:Class ;
    rdfs:label "LithiumManganeseOxideElectrode"@en ;
    rdfs:comment "electrode in which the active material is lithium manganese oxide"@en ;
    rdfs:subClassOf [ a owl:Restriction ;
            owl:onProperty :electrochemistry_860aa941_5ff9_4452_8a16_7856fad07bee ;
            owl:someValuesFrom chems:substance_e8fafdc8_6cd3_4dd0_9630_10ca8e3f1827 ],
        :electrochemistry_b1ac8d0c_a215_4e60_82b0_38272eff5131,
        :electrochemistry_e4b6cb36_4dac_49e3_871d_40bcfca943a5 ;
    owl:deprecated true ;
    skos:altLabel "LMOElectrode"@en ;
    skos:prefLabel "LithiumManganeseOxideElectrode"@en ;
    emmo:EMMO_967080e5_2f42_4eb2_a3a9_c58143e835f9 "electrode in which the active material is lithium manganese oxide"@en .

:electrochemistry_c54fbb75_0528_49c0_97e0_258798a947e4 a owl:Class ;
    rdfs:label "P1212080" ;
    rdfs:comment "a prismatic case with a nominal length of 12 mm, width of 120 mm, and height of 80 mm"@en ;
    rdfs:subClassOf :electrochemistry_43cd6e14_dd43_41b5_b5b4_344d53841603 ;
    skos:altLabel "P12/120/80" ;
    skos:prefLabel "P1212080" ;
    emmo:EMMO_967080e5_2f42_4eb2_a3a9_c58143e835f9 "a prismatic case with a nominal length of 12 mm, width of 120 mm, and height of 80 mm"@en .

:electrochemistry_c5f51531_1452_4654_82e5_0505491c2c7d a owl:Class ;
    rdfs:label "SodiumTitaniumOxideElectrode"@en ;
    rdfs:comment "electrode in which the active material is sodium titanium oxide"@en ;
    rdfs:subClassOf :electrochemistry_9c557caa_61e2_4fa9_a517_4bad01a68122,
        :electrochemistry_e4b6cb36_4dac_49e3_871d_40bcfca943a5 ;
    owl:deprecated true ;
    skos:prefLabel "SodiumTitaniumOxideElectrode"@en ;
    emmo:EMMO_967080e5_2f42_4eb2_a3a9_c58143e835f9 "electrode in which the active material is sodium titanium oxide"@en .

:electrochemistry_c5fd7b61_40f1_4225_a173_5caa3c5f4773 a owl:Class ;
    rdfs:label "TungstenBasedElectrode"@en ;
    rdfs:comment "an electrode in which the primary active material consists of tungsten or tungsten compounds"@en ;
    rdfs:subClassOf :electrochemistry_9a823d64_9d10_4a29_9cbd_9bbdad7985bc ;
    skos:prefLabel "TungstenBasedElectrode"@en ;
    emmo:EMMO_967080e5_2f42_4eb2_a3a9_c58143e835f9 "an electrode in which the primary active material consists of tungsten or tungsten compounds"@en .

:electrochemistry_c63baed9_48dd_4b5c_9e8c_03011010ffb6 a owl:Class ;
    rdfs:label "IndiumTinOxideElectrode"@en ;
    rdfs:comment "electrode in which the active material is indium tin oxide"@en ;
    rdfs:subClassOf [ a owl:Restriction ;
            owl:onProperty :electrochemistry_860aa941_5ff9_4452_8a16_7856fad07bee ;
            owl:someValuesFrom chems:substance_2a87ca10_fc6a_4d61_b48c_d9790a566ee3 ],
        [ a owl:Restriction ;
            owl:onProperty :electrochemistry_860aa941_5ff9_4452_8a16_7856fad07bee ;
            owl:someValuesFrom chems:substance_db74b6b7_09fc_40db_a7d5_6eb86b69192a ],
        :electrochemistry_4839708a_3864_47eb_b719_373ff8874c61 ;
    owl:deprecated true ;
    skos:altLabel "ITO"@en ;
    skos:prefLabel "IndiumTinOxideElectrode"@en ;
    emmo:EMMO_967080e5_2f42_4eb2_a3a9_c58143e835f9 "electrode in which the active material is indium tin oxide"@en .

:electrochemistry_c6d6c0a1_a06b_437a_978f_a469d3071ca9 a owl:Class ;
    rdfs:label "PolymerElectrolyte"@en ;
    rdfs:comment "a polymer matrix capable of ion conduction"@en ;
    rdfs:subClassOf :electrochemistry_fb0d9eef_92af_4628_8814_e065ca255d59 ;
    skos:prefLabel "PolymerElectrolyte"@en ;
    emmo:EMMO_26bf1bef_d192_4da6_b0eb_d2209698fb54 "https://www.wikidata.org/wiki/Q107223477" ;
    emmo:EMMO_967080e5_2f42_4eb2_a3a9_c58143e835f9 "a polymer matrix capable of ion conduction"@en ;
    emmo:EMMO_c84c6752_6d64_48cc_9500_e54a3c34898d "https://en.wikipedia.org/wiki/Polymer_electrolytes"@en .

:electrochemistry_c830c469_60c3_4380_8382_4df13a32a1e7 a owl:ObjectProperty ;
    rdfs:label "hasConductiveAdditive"@en ;
    rdfs:comment "relates a component or mixture to an additive that is intendend to increase the conductivity of the whole."@en ;
    rdfs:range emmo:EMMO_bc37743c_37c4_4ec7_9d58_d1aae5567352 ;
    rdfs:subPropertyOf :electrochemistry_7df82c48_b599_4b02_bef0_9facc9c39410 ;
    skos:prefLabel "hasConductiveAdditive"@en ;
    emmo:EMMO_967080e5_2f42_4eb2_a3a9_c58143e835f9 "relates a component or mixture to an additive that is intendend to increase the conductivity of the whole."@en .

:electrochemistry_c831d963_629a_41ab_850f_97fb6841b739 a owl:Class ;
    rdfs:label "GraphiteElectrode"@en ;
    rdfs:comment "electrode in which the active material is graphite"@en ;
    rdfs:subClassOf [ a owl:Restriction ;
            owl:onProperty :electrochemistry_860aa941_5ff9_4452_8a16_7856fad07bee ;
            owl:someValuesFrom chems:substance_d53259a7_0d9c_48b9_a6c1_4418169df303 ],
        :electrochemistry_9a823d64_9d10_4a29_9cbd_9bbdad7985bc,
        :electrochemistry_f2c33088_224f_4fdb_857a_7cb62e3dddca ;
    skos:prefLabel "GraphiteElectrode"@en ;
    emmo:EMMO_967080e5_2f42_4eb2_a3a9_c58143e835f9 "electrode in which the active material is graphite"@en .

:electrochemistry_c84a1d8f_e405_42ba_8c80_bbe3b9c6c66a a owl:Class ;
    rdfs:label "PerforatedFoil"@en ;
    rdfs:comment "a thin sheet that has been punched with a pattern of holes, offering controlled porosity and strength for uses in filtration, sound suppression, and structural components"@en ;
    rdfs:subClassOf emmo:EMMO_ec7464a9_d99d_45f8_965b_4e9230ea8356 ;
    skos:prefLabel "PerforatedFoil"@en ;
    emmo:EMMO_967080e5_2f42_4eb2_a3a9_c58143e835f9 "a thin sheet that has been punched with a pattern of holes, offering controlled porosity and strength for uses in filtration, sound suppression, and structural components"@en .

:electrochemistry_ca0527c1_f682_4eea_aca5_f3ae66a9ddce a owl:Class ;
    rdfs:label "ElectrochemicalPseudocapacitor"@en ;
    rdfs:comment "a type of supercapacitor that uses metal oxide or conducting polymer electrodes with a high amount of electrochemical pseudocapacitance additional to the double-layer capacitance"@en ;
    rdfs:subClassOf :electrochemistry_dc6abae7_39b0_4d22_b52e_14d088a4bd5f ;
    skos:prefLabel "ElectrochemicalPseudocapacitor"@en ;
    emmo:EMMO_26bf1bef_d192_4da6_b0eb_d2209698fb54 "https://www.wikidata.org/wiki/Q7254569" ;
    emmo:EMMO_967080e5_2f42_4eb2_a3a9_c58143e835f9 "a type of supercapacitor that uses metal oxide or conducting polymer electrodes with a high amount of electrochemical pseudocapacitance additional to the double-layer capacitance"@en ;
    emmo:EMMO_c7b62dd7_063a_4c2a_8504_42f7264ba83f "stores energy electrochemically via Faradaic mechanisms"@en ;
    emmo:EMMO_c84c6752_6d64_48cc_9500_e54a3c34898d "https://en.wikipedia.org/wiki/Pseudocapacitor"@en .

:electrochemistry_ca4d9efc_70be_441e_b358_d927aa4c36c4 a owl:Class ;
    rdfs:label "ManganeseDioxideElectrode"@en ;
    rdfs:comment "an electrode in which the primary active material consists of manganese dioxide or manganese dioxide compounds."@en ;
    rdfs:subClassOf [ a owl:Restriction ;
            owl:onProperty :electrochemistry_860aa941_5ff9_4452_8a16_7856fad07bee ;
            owl:someValuesFrom chems:substance_dcdbdbed_2e20_40d1_a7a5_5761de7f0618 ],
        :electrochemistry_b1ac8d0c_a215_4e60_82b0_38272eff5131,
        :electrochemistry_e4b6cb36_4dac_49e3_871d_40bcfca943a5 ;
    skos:altLabel "MnO2Electrode"@en ;
    skos:prefLabel "ManganeseDioxideElectrode"@en ;
    emmo:EMMO_967080e5_2f42_4eb2_a3a9_c58143e835f9 "an electrode in which the primary active material consists of manganese dioxide or manganese dioxide compounds."@en ;
    emmo:EMMO_c7b62dd7_063a_4c2a_8504_42f7264ba83f "the combination with lithium metal and an organic electrolyte is designated using IEC electrochemical system letter code C"@en,
        "the combination with zinc metal and an alkali metal hydoxide electrolyte is designated using IEC electrochemical system letter code L"@en .

:electrochemistry_cab66388_3feb_4101_82bc_f4441f0b60e3 a owl:Class ;
    rdfs:label "LithiumNickelOxideElectrode"@en ;
    rdfs:comment "electrode in which the active material is lithium nickel oxide"@en ;
    rdfs:subClassOf [ a owl:Restriction ;
            owl:onProperty :electrochemistry_860aa941_5ff9_4452_8a16_7856fad07bee ;
            owl:someValuesFrom chems:substance_c28a0967_ed23_48cc_a14e_a651d75a19db ],
        :electrochemistry_0d2aaaf4_1a8a_4a32_abd8_7d0fdf0ae9d2,
        :electrochemistry_e4b6cb36_4dac_49e3_871d_40bcfca943a5 ;
    owl:deprecated true ;
    skos:altLabel "LNOElectrode"@en ;
    skos:prefLabel "LithiumNickelOxideElectrode"@en ;
    emmo:EMMO_967080e5_2f42_4eb2_a3a9_c58143e835f9 "electrode in which the active material is lithium nickel oxide"@en .

:electrochemistry_cba03815_eaa8_493d_b9e4_52856b57fde6 a owl:Class ;
    rdfs:label "IridiumOxideElectrode"@en ;
    rdfs:comment "electrode in which the active material is iridium oxide"@en ;
    rdfs:subClassOf [ a owl:Restriction ;
            owl:onProperty :electrochemistry_860aa941_5ff9_4452_8a16_7856fad07bee ;
            owl:someValuesFrom chems:substance_f7525766_90cf_43e9_8932_7cb3b14f676f ],
        :electrochemistry_e4b6cb36_4dac_49e3_871d_40bcfca943a5 ;
    owl:deprecated true ;
    skos:altLabel "IrO2Electrode"@en ;
    skos:prefLabel "IridiumOxideElectrode"@en ;
    emmo:EMMO_967080e5_2f42_4eb2_a3a9_c58143e835f9 "electrode in which the active material is iridium oxide"@en .

:electrochemistry_cc0468a2_1851_4d3d_92a6_b4059db0c056 a owl:Class ;
    rdfs:label "SodiumManganesePhosphateElectrode"@en ;
    rdfs:comment "electrode in which the active material is sodium manganese phosphate"@en ;
    rdfs:subClassOf [ a owl:Restriction ;
            owl:onProperty :electrochemistry_860aa941_5ff9_4452_8a16_7856fad07bee ;
            owl:someValuesFrom chems:substance_b01771a9_218a_4b01_b20f_4021cfa0b7d5 ],
        :electrochemistry_468b3b63_b62a_4110_8c7e_40fffd5fdfd6,
        :electrochemistry_e4b6cb36_4dac_49e3_871d_40bcfca943a5 ;
    owl:deprecated true ;
    skos:prefLabel "SodiumManganesePhosphateElectrode"@en ;
    emmo:EMMO_967080e5_2f42_4eb2_a3a9_c58143e835f9 "electrode in which the active material is sodium manganese phosphate"@en .

:electrochemistry_cc4e178c_bc1f_4502_b6c2_33f304ef6bab a owl:Class ;
    rdfs:label "IronBasedElectrode"@en ;
    rdfs:comment "an electrode in which the primary active material consists of iron or iron compounds"@en ;
    rdfs:subClassOf :electrochemistry_9a823d64_9d10_4a29_9cbd_9bbdad7985bc ;
    owl:deprecated true ;
    skos:prefLabel "IronBasedElectrode"@en ;
    emmo:EMMO_967080e5_2f42_4eb2_a3a9_c58143e835f9 "an electrode in which the primary active material consists of iron or iron compounds"@en .

:electrochemistry_cd1b7943_42ce_46bd_8588_1c3161268270 a owl:Class ;
    rdfs:label "SwagelokCase"@en ;
    rdfs:comment "a container for an electrochemical cell manufactured by the company Swagelok"@en ;
    rdfs:subClassOf :electrochemistry_1aec4cc0_82d5_4042_a657_ed7fe291c3d8 ;
    skos:prefLabel "SwagelokCase"@en ;
    emmo:EMMO_967080e5_2f42_4eb2_a3a9_c58143e835f9 "a container for an electrochemical cell manufactured by the company Swagelok"@en .

:electrochemistry_cd615729_8240_487a_a619_cc94656731f2 a owl:Class ;
    rdfs:label "CarbonPaper"@en ;
    rdfs:comment "a thin, flat material composed of compressed carbon fibers, used in fuel cells and other electrochemical devices for its high electrical conductivity and gas permeability"@en ;
    rdfs:subClassOf emmo:EMMO_ec7464a9_d99d_45f8_965b_4e9230ea8356 ;
    skos:prefLabel "CarbonPaper"@en ;
    emmo:EMMO_967080e5_2f42_4eb2_a3a9_c58143e835f9 "a thin, flat material composed of compressed carbon fibers, used in fuel cells and other electrochemical devices for its high electrical conductivity and gas permeability"@en .

:electrochemistry_ce4352a7_f0b1_4f27_9184_6deebf8bbe96 a owl:Class ;
    rdfs:label "R1511" ;
    rdfs:comment "a coin case with a nominal diameter of 15.8 mm and a height of 11.1 mm"@en ;
    rdfs:subClassOf :electrochemistry_3979cd56_6256_414d_966c_7f723bf71e37 ;
    skos:altLabel "R52" ;
    skos:prefLabel "R1511" ;
    emmo:EMMO_967080e5_2f42_4eb2_a3a9_c58143e835f9 "a coin case with a nominal diameter of 15.8 mm and a height of 11.1 mm"@en .

:electrochemistry_cf6eebea_24f6_48d2_8389_65eba0393762 a owl:Class ;
    rdfs:label "R1126" ;
    rdfs:comment "a coin case with a nominal diameter of 11.6 mm and a height of 2.6 mm"@en ;
    rdfs:subClassOf :electrochemistry_3979cd56_6256_414d_966c_7f723bf71e37 ;
    skos:altLabel "R56" ;
    skos:prefLabel "R1126" ;
    emmo:EMMO_967080e5_2f42_4eb2_a3a9_c58143e835f9 "a coin case with a nominal diameter of 11.6 mm and a height of 2.6 mm"@en .

:electrochemistry_cff80dd5_19a9_4357_8fb9_410a978153e2 a owl:Class ;
    rdfs:label "SodiumTitaniumPhosphateElectrode"@en ;
    rdfs:comment "electrode in which the active material is sodium titanium phosphate"@en ;
    rdfs:subClassOf :electrochemistry_9c557caa_61e2_4fa9_a517_4bad01a68122,
        :electrochemistry_e4b6cb36_4dac_49e3_871d_40bcfca943a5 ;
    owl:deprecated true ;
    skos:prefLabel "SodiumTitaniumPhosphateElectrode"@en ;
    emmo:EMMO_967080e5_2f42_4eb2_a3a9_c58143e835f9 "electrode in which the active material is sodium titanium phosphate"@en .

:electrochemistry_d1042a12_e4be_4992_86cb_59420ef4e05c a owl:Class ;
    rdfs:label "ChargeCarrier"@en ;
    rdfs:comment "a generic denomination of particles or quasiparticles responsible for electric charge transport."@en ;
    rdfs:subClassOf :electrochemistry_b5ea31c9_bb10_4276_980e_c3eceb1efc82 ;
    skos:example "electron, hole, ion"@en ;
    skos:prefLabel "ChargeCarrier"@en ;
    emmo:EMMO_26bf1bef_d192_4da6_b0eb_d2209698fb54 "https://www.wikidata.org/wiki/Q865807",
        "https://www.wikidata.org/wiki/Q865807"@en ;
    emmo:EMMO_967080e5_2f42_4eb2_a3a9_c58143e835f9 "a generic denomination of particles or quasiparticles responsible for electric charge transport."@en ;
    emmo:EMMO_c84c6752_6d64_48cc_9500_e54a3c34898d "https://en.wikipedia.org/wiki/Charge_carrier"@en .

:electrochemistry_d1199193_b203_4fcb_971c_ccf6332973ae a owl:Class ;
    rdfs:label "P1212081" ;
    rdfs:comment "a prismatic case with a nominal length of 12 mm, width of 120 mm, and height of 81 mm"@en ;
    rdfs:subClassOf :electrochemistry_43cd6e14_dd43_41b5_b5b4_344d53841603 ;
    skos:altLabel "HEV2",
        "P12/120/81" ;
    skos:prefLabel "P1212081" ;
    emmo:EMMO_967080e5_2f42_4eb2_a3a9_c58143e835f9 "a prismatic case with a nominal length of 12 mm, width of 120 mm, and height of 81 mm"@en .

:electrochemistry_d11b0e66_c35b_4da7_80a1_037ce89b77fb a owl:Class ;
    rdfs:label "GlassFibreSeparator"@en ;
    rdfs:comment "a separator is composed of a mass of intermeshed glass fibers."@en ;
    rdfs:subClassOf :electrochemistry_331e6cca_f260_4bf8_af55_35304fe1bbe0 ;
    skos:altLabel "FibreglassSeparator"@en ;
    skos:prefLabel "GlassFibreSeparator"@en ;
    emmo:EMMO_967080e5_2f42_4eb2_a3a9_c58143e835f9 "a separator is composed of a mass of intermeshed glass fibers."@en .

:electrochemistry_d1bf3cdd_d618_40e3_b055_a952ef632157 a owl:Class ;
    rdfs:label "P1868107" ;
    rdfs:comment "a prismatic case with a nominal length of 18 mm, width of 68 mm, and height of 107 mm"@en ;
    rdfs:subClassOf :electrochemistry_43cd6e14_dd43_41b5_b5b4_344d53841603 ;
    skos:altLabel "P18/68/107" ;
    skos:prefLabel "P1868107" ;
    emmo:EMMO_967080e5_2f42_4eb2_a3a9_c58143e835f9 "a prismatic case with a nominal length of 18 mm, width of 68 mm, and height of 107 mm"@en .

:electrochemistry_d2726dd5_69f0_4cb1_bd3c_4c48813e57e7 a owl:Class ;
    rdfs:label "IronDisulfideElectrode"@en ;
    rdfs:comment "an electrode in which the primary active material consists of iron disulfide or iron disulfide compounds."@en ;
    rdfs:subClassOf [ a owl:Restriction ;
            owl:onProperty :electrochemistry_860aa941_5ff9_4452_8a16_7856fad07bee ;
            owl:someValuesFrom chems:substance_c728b6b9_449a_45ff_b5ae_6b7968708f0d ],
        :electrochemistry_5e1136d3_df00_40f7_a4bc_8259341053a1,
        :electrochemistry_9a823d64_9d10_4a29_9cbd_9bbdad7985bc ;
    skos:prefLabel "IronDisulfideElectrode"@en ;
    emmo:EMMO_967080e5_2f42_4eb2_a3a9_c58143e835f9 "an electrode in which the primary active material consists of iron disulfide or iron disulfide compounds."@en ;
    emmo:EMMO_c7b62dd7_063a_4c2a_8504_42f7264ba83f "the combination with lithium metal and an organic electrolyte is designated using IEC electrochemical system letter code F"@en .

:electrochemistry_d48ea516_5cac_4f86_bc88_21b6276c0938 a owl:Class ;
    rdfs:label "ButlerVolmerEquation"@en ;
    rdfs:comment "a phenomenological model for electrode kinetics, describing the relation between the electrode current from an electrochemical charge-transfer reaction and the surface overpotential of the electrode"@en ;
    rdfs:subClassOf :electrochemistry_3d805c2a_4801_440e_9e4d_0fa5585c76ae ;
    skos:altLabel "ButlerVolmerApproximation"@en,
        "ErdeyGruzVolmerEquation"@en ;
    skos:prefLabel "ButlerVolmerEquation"@en ;
    emmo:EMMO_26bf1bef_d192_4da6_b0eb_d2209698fb54 "https://www.wikidata.org/wiki/Q903846" ;
    emmo:EMMO_6dd685dd_1895_46e4_b227_be9f7d643c25 "https://dbpedia.org/page/Butler%E2%80%93Volmer_equation"@en ;
    emmo:EMMO_967080e5_2f42_4eb2_a3a9_c58143e835f9 "a phenomenological model for electrode kinetics, describing the relation between the electrode current from an electrochemical charge-transfer reaction and the surface overpotential of the electrode"@en ;
    emmo:EMMO_c7b62dd7_063a_4c2a_8504_42f7264ba83f "i = i0 * (exp(alpha*n*F*eta/(R*T))  exp(-(1-alpha)*n*F*eta/(R*T)))" ;
    emmo:EMMO_c84c6752_6d64_48cc_9500_e54a3c34898d "https://en.wikipedia.org/wiki/Butler%E2%80%93Volmer_equation"@en .

:electrochemistry_d5f67a0c_ed56_479d_9b68_6003142f98b0 a owl:Class ;
    rdfs:label "R1616" ;
    rdfs:comment "a coin case with a nominal diameter of 16.0 mm and a height of 1.6 mm"@en ;
    rdfs:subClassOf :electrochemistry_3979cd56_6256_414d_966c_7f723bf71e37 ;
    skos:prefLabel "R1616" ;
    emmo:EMMO_967080e5_2f42_4eb2_a3a9_c58143e835f9 "a coin case with a nominal diameter of 16.0 mm and a height of 1.6 mm"@en .

:electrochemistry_d67a0921_15e4_4c73_804e_97b2d66452b8 a owl:Class ;
    rdfs:label "R936" ;
    rdfs:comment "a coin case with a nominal diameter of 9.5 mm and a height of 3.6 mm"@en ;
    rdfs:subClassOf :electrochemistry_3979cd56_6256_414d_966c_7f723bf71e37 ;
    skos:altLabel "R45" ;
    skos:prefLabel "R936" ;
    emmo:EMMO_967080e5_2f42_4eb2_a3a9_c58143e835f9 "a coin case with a nominal diameter of 9.5 mm and a height of 3.6 mm"@en .

:electrochemistry_d90221a0_0da7_4876_9cac_0e943e445f6f a owl:Class ;
    rdfs:label "TitaniumBasedElectrode"@en ;
    rdfs:comment "an electrode in which the primary active material consists of titanium or titanium compounds"@en ;
    rdfs:subClassOf :electrochemistry_9a823d64_9d10_4a29_9cbd_9bbdad7985bc ;
    owl:deprecated true ;
    skos:prefLabel "TitaniumBasedElectrode"@en ;
    emmo:EMMO_967080e5_2f42_4eb2_a3a9_c58143e835f9 "an electrode in which the primary active material consists of titanium or titanium compounds"@en .

:electrochemistry_d936c767_1530_419c_93f4_59e08f0d702c a owl:Class ;
    rdfs:label "SodiumInsertionElectrode"@en ;
    rdfs:comment "an insertion electrode in which the guest molecule is sodium"@en ;
    rdfs:subClassOf :electrochemistry_757eae08_4d43_42d4_8b4e_8a0bfd2f9a1c ;
    owl:deprecated true ;
    skos:prefLabel "SodiumInsertionElectrode"@en ;
    emmo:EMMO_967080e5_2f42_4eb2_a3a9_c58143e835f9 "an insertion electrode in which the guest molecule is sodium"@en .

:electrochemistry_d9888f1f_2226_4ce3_9cb3_91fd9bd1bf22 a owl:Class ;
    rdfs:label "MagnesiumInsertionElectrode"@en ;
    rdfs:comment "an insertion electrode in which the guest molecule is magnesium"@en ;
    rdfs:subClassOf :electrochemistry_757eae08_4d43_42d4_8b4e_8a0bfd2f9a1c ;
    owl:deprecated true ;
    skos:prefLabel "MagnesiumInsertionElectrode"@en ;
    emmo:EMMO_967080e5_2f42_4eb2_a3a9_c58143e835f9 "an insertion electrode in which the guest molecule is magnesium"@en .

:electrochemistry_dac5067c_e6f2_4fca_a915_5b7b918ca1c4 a owl:Class ;
    rdfs:label "R11108" ;
    rdfs:comment "a coin case with a nominal diameter of 11.6 mm and a height of 10.8 mm"@en ;
    rdfs:subClassOf :electrochemistry_3979cd56_6256_414d_966c_7f723bf71e37 ;
    skos:prefLabel "R11108" ;
    emmo:EMMO_967080e5_2f42_4eb2_a3a9_c58143e835f9 "a coin case with a nominal diameter of 11.6 mm and a height of 10.8 mm"@en .

:electrochemistry_dc019f3f_e5f3_4eeb_bab9_a845a02223a0 a owl:Class ;
    rdfs:label "R616" ;
    rdfs:comment "a coin case with a nominal diameter of 6.8 mm and a height of 1.65 mm"@en ;
    rdfs:subClassOf :electrochemistry_3979cd56_6256_414d_966c_7f723bf71e37 ;
    skos:altLabel "R65" ;
    skos:prefLabel "R616" ;
    emmo:EMMO_967080e5_2f42_4eb2_a3a9_c58143e835f9 "a coin case with a nominal diameter of 6.8 mm and a height of 1.65 mm"@en .

:electrochemistry_dd4c5ffa_6228_41d8_8a44_a40a2b22723e a owl:Class ;
    rdfs:label "CadmiumBasedElectrode"@en ;
    rdfs:comment "an electrode in which the primary active material consists of cadmium or cadmium compounds."@en ;
    rdfs:subClassOf :electrochemistry_9a823d64_9d10_4a29_9cbd_9bbdad7985bc ;
    skos:prefLabel "CadmiumBasedElectrode"@en ;
    emmo:EMMO_967080e5_2f42_4eb2_a3a9_c58143e835f9 "an electrode in which the primary active material consists of cadmium or cadmium compounds."@en .

:electrochemistry_df4dd678_9642_47c9_84dd_4bb09f369f53 a owl:Class ;
    rdfs:label "SodiumBasedElectrode"@en ;
    rdfs:comment "an electrode in which the primary active material consists of sodium or sodium compounds"@en ;
    rdfs:subClassOf :electrochemistry_9a823d64_9d10_4a29_9cbd_9bbdad7985bc ;
    skos:prefLabel "SodiumBasedElectrode"@en ;
    emmo:EMMO_967080e5_2f42_4eb2_a3a9_c58143e835f9 "an electrode in which the primary active material consists of sodium or sodium compounds"@en .

:electrochemistry_e0869e7a_36fe_4e33_9843_a5dc19fcb488 a owl:Class ;
    rdfs:label "R9" ;
    rdfs:comment "a coin case with a nominal diameter of 15.5 mm and a height of 6.0 mm"@en ;
    rdfs:subClassOf :electrochemistry_3979cd56_6256_414d_966c_7f723bf71e37 ;
    skos:prefLabel "R9" ;
    emmo:EMMO_967080e5_2f42_4eb2_a3a9_c58143e835f9 "a coin case with a nominal diameter of 15.5 mm and a height of 6.0 mm"@en .

:electrochemistry_e13b7945_65ac_476b_85ee_5cdc59f5c919 a owl:Class ;
    rdfs:label "Particle"@en ;
    rdfs:comment "a small localized object which can be described by several physical or chemical properties, such as volume, density, or mass."@en ;
    rdfs:subClassOf :electrochemistry_b5ea31c9_bb10_4276_980e_c3eceb1efc82 ;
    skos:prefLabel "Particle"@en ;
    emmo:EMMO_967080e5_2f42_4eb2_a3a9_c58143e835f9 "a small localized object which can be described by several physical or chemical properties, such as volume, density, or mass."@en ;
    emmo:EMMO_c84c6752_6d64_48cc_9500_e54a3c34898d "https://en.wikipedia.org/wiki/Particle"@en .

:electrochemistry_e2c91edd_dd01_4309_9735_6fe5280261d4 a owl:Class ;
    rdfs:label "OxygenElectrode"@en ;
    rdfs:comment "a gas diffusion electrode in which the active material is oxygen (O2)"@en ;
    rdfs:subClassOf :electrochemistry_bbb1d95b_72d1_44f6_b07e_a3d7d41ac215 ;
    skos:prefLabel "OxygenElectrode"@en ;
    emmo:EMMO_967080e5_2f42_4eb2_a3a9_c58143e835f9 "a gas diffusion electrode in which the active material is oxygen (O2)"@en ;
    emmo:EMMO_c7b62dd7_063a_4c2a_8504_42f7264ba83f "the combination with zinc metal and an alkali metal hydroxide electrolyte is designated using IEC electrochemical system letter code P"@en .

:electrochemistry_e3f6eacc_f661_404e_ac16_45d2fa1f5d89 a owl:Class ;
    rdfs:label "SpaceChargeLayer"@en ;
    rdfs:comment "an interphase formed when two materials with different chemical potentials are brought in contact with each other, and the atoms or electrons are unable to migrate to establish local charge neutrality"@en ;
    rdfs:subClassOf :electrochemistry_f78e3c87_01c6_4cc2_b047_30322262e22d ;
    skos:altLabel "DepletionLayer"@en,
        "DepletionRegion"@en,
        "DepletionZone"@en,
        "JunctionRegion"@en,
        "SpaceChargeRegion"@en ;
    skos:prefLabel "SpaceChargeLayer"@en ;
    emmo:EMMO_26bf1bef_d192_4da6_b0eb_d2209698fb54 "https://www.wikidata.org/wiki/Q288224" ;
    emmo:EMMO_50c298c2_55a2_4068_b3ac_4e948c33181f "https://www.electropedia.org/iev/iev.nsf/display?openform&ievref=521-02-82" ;
    emmo:EMMO_967080e5_2f42_4eb2_a3a9_c58143e835f9 "an interphase formed when two materials with different chemical potentials are brought in contact with each other, and the atoms or electrons are unable to migrate to establish local charge neutrality"@en ;
    emmo:EMMO_c84c6752_6d64_48cc_9500_e54a3c34898d "https://en.wikipedia.org/wiki/Depletion_region"@en .

:electrochemistry_e4d666ee_d637_45cd_a904_dc33941ead4f a owl:Class .

:electrochemistry_e73cb0b7_e2af_4c1a_b05b_503df25a8bf5 a owl:Class ;
    rdfs:label "R1025" ;
    rdfs:comment "a coin case with a nominal diameter of 10.0 mm and a height of 2.5 mm"@en ;
    rdfs:subClassOf :electrochemistry_3979cd56_6256_414d_966c_7f723bf71e37 ;
    skos:prefLabel "R1025" ;
    emmo:EMMO_967080e5_2f42_4eb2_a3a9_c58143e835f9 "a coin case with a nominal diameter of 10.0 mm and a height of 2.5 mm"@en .

:electrochemistry_e84e691a_df58_465c_9771_7a7fe2212ed5 a owl:Class ;
    rdfs:label "LithiumHydroxideSolution"@en ;
    rdfs:comment "a solution of lithium hydroxide (LiOH) dissolved in water (H2O)"@en ;
    rdfs:subClassOf :electrochemistry_615cff2a_be95_4e65_9471_98db23f4c878 ;
    owl:deprecated true ;
    skos:altLabel "AqueousLithiumHydroxideSolution"@en,
        "LiOHSolution"@en ;
    skos:prefLabel "LithiumHydroxideSolution"@en ;
    emmo:EMMO_967080e5_2f42_4eb2_a3a9_c58143e835f9 "a solution of lithium hydroxide (LiOH) dissolved in water (H2O)"@en .

:electrochemistry_e8c39ecc_29d1_4172_996e_d5b05dc88015 a owl:Class ;
    rdfs:label "SiliconGraphiteElectrode"@en ;
    rdfs:comment "an electrode with blended silicon and graphite active materials"@en ;
    rdfs:subClassOf [ a owl:Restriction ;
            owl:onProperty :electrochemistry_860aa941_5ff9_4452_8a16_7856fad07bee ;
            owl:someValuesFrom chems:substance_68c0876b_cb62_41cd_846d_95cc9d9a8733 ],
        [ a owl:Restriction ;
            owl:onProperty :electrochemistry_860aa941_5ff9_4452_8a16_7856fad07bee ;
            owl:someValuesFrom chems:substance_d53259a7_0d9c_48b9_a6c1_4418169df303 ],
        :electrochemistry_5186239a_2af7_4dbf_92ca_22e8e583c528 ;
    owl:deprecated true ;
    skos:prefLabel "SiliconGraphiteElectrode"@en ;
    emmo:EMMO_967080e5_2f42_4eb2_a3a9_c58143e835f9 "an electrode with blended silicon and graphite active materials"@en .

:electrochemistry_e8d9e091_a56d_4a24_a305_d1bac55cfce3 a owl:Class ;
    rdfs:label "SodiumManganeseOxideElectrode"@en ;
    rdfs:comment "electrode in which the active material is sodium manganese oxide"@en ;
    rdfs:subClassOf [ a owl:Restriction ;
            owl:onProperty :electrochemistry_860aa941_5ff9_4452_8a16_7856fad07bee ;
            owl:someValuesFrom chems:substance_0139937b_2724_4864_84fb_f14bcfb83538 ],
        :electrochemistry_b1ac8d0c_a215_4e60_82b0_38272eff5131,
        :electrochemistry_e4b6cb36_4dac_49e3_871d_40bcfca943a5 ;
    owl:deprecated true ;
    skos:prefLabel "SodiumManganeseOxideElectrode"@en ;
    emmo:EMMO_967080e5_2f42_4eb2_a3a9_c58143e835f9 "electrode in which the active material is sodium manganese oxide"@en .

:electrochemistry_eb09ca25_90c9_4b55_9165_76fbf7fb5a46 a owl:Class ;
    rdfs:label "BismuthBasedElectrode"@en ;
    rdfs:comment "an electrode in which the primary active material consists of bismuth or bismuth compounds."@en ;
    rdfs:subClassOf :electrochemistry_9a823d64_9d10_4a29_9cbd_9bbdad7985bc ;
    skos:prefLabel "BismuthBasedElectrode"@en ;
    emmo:EMMO_967080e5_2f42_4eb2_a3a9_c58143e835f9 "an electrode in which the primary active material consists of bismuth or bismuth compounds."@en .

:electrochemistry_eb1c9aa3_ad4f_4f2a_80f6_d6c8a8bc0d9a a owl:Class ;
    rdfs:label "R921" ;
    rdfs:comment "a coin case with a nominal diameter of 9.5 mm and a height of 2.1 mm"@en ;
    rdfs:subClassOf :electrochemistry_3979cd56_6256_414d_966c_7f723bf71e37 ;
    skos:altLabel "R69" ;
    skos:prefLabel "R921" ;
    emmo:EMMO_967080e5_2f42_4eb2_a3a9_c58143e835f9 "a coin case with a nominal diameter of 9.5 mm and a height of 2.1 mm"@en .

:electrochemistry_ebd01982_6b0c_48e7_90ef_7b7342009449 a owl:Class ;
    rdfs:label "SodiumHydroxideSolution"@en ;
    rdfs:comment "a solution of sodium hydroxide (NaOH) dissolved in water (H2O)"@en ;
    rdfs:subClassOf :electrochemistry_615cff2a_be95_4e65_9471_98db23f4c878 ;
    owl:deprecated true ;
    skos:altLabel "AqueousSodiumHydroxideSolution"@en,
        "NaOHSolution"@en ;
    skos:prefLabel "SodiumHydroxideSolution"@en ;
    emmo:EMMO_967080e5_2f42_4eb2_a3a9_c58143e835f9 "a solution of sodium hydroxide (NaOH) dissolved in water (H2O)"@en .

:electrochemistry_ebf314c7_81ad_4d77_9da4_b454520fda0e a owl:Class ;
    rdfs:label "R916" ;
    rdfs:comment "a coin case with a nominal diameter of 9.5 mm and a height of 1.6 mm"@en ;
    rdfs:subClassOf :electrochemistry_3979cd56_6256_414d_966c_7f723bf71e37 ;
    skos:altLabel "R68" ;
    skos:prefLabel "R916" ;
    emmo:EMMO_967080e5_2f42_4eb2_a3a9_c58143e835f9 "a coin case with a nominal diameter of 9.5 mm and a height of 1.6 mm"@en .

:electrochemistry_ee0278fb_932d_48cd_a20a_c1b89b29d68b a owl:Class ;
    rdfs:label "SodiumCobaltOxideElectrode"@en ;
    rdfs:comment "electrode in which the active material is sodium cobalt oxide"@en ;
    rdfs:subClassOf [ a owl:Restriction ;
            owl:onProperty :electrochemistry_860aa941_5ff9_4452_8a16_7856fad07bee ;
            owl:someValuesFrom chems:substance_cdd18f0c_e7b3_4d09_b3dd_c09fe4b1adba ],
        :electrochemistry_838c115b_6bc9_4ce8_9f8d_86a6bf67742a,
        :electrochemistry_e4b6cb36_4dac_49e3_871d_40bcfca943a5 ;
    owl:deprecated true ;
    skos:prefLabel "SodiumCobaltOxideElectrode"@en ;
    emmo:EMMO_967080e5_2f42_4eb2_a3a9_c58143e835f9 "electrode in which the active material is sodium cobalt oxide"@en .

:electrochemistry_ee479886_6805_4018_95e1_500185e44215 a owl:Class ;
    rdfs:label "Powder"@en ;
    rdfs:comment "a material comprised of many particles"@en ;
    rdfs:subClassOf [ a owl:Restriction ;
            owl:onProperty emmo:EMMO_e1097637_70d2_4895_973f_2396f04fa204 ;
            owl:someValuesFrom :electrochemistry_0ed0362e_b7ae_482c_a7d0_2ca2eebda648 ],
        [ a owl:Restriction ;
            owl:onProperty emmo:EMMO_e1097637_70d2_4895_973f_2396f04fa204 ;
            owl:someValuesFrom :electrochemistry_2e2d92f4_9fd5_4965_b15a_30b43c68e3e5 ],
        [ a owl:Restriction ;
            owl:onProperty emmo:EMMO_e1097637_70d2_4895_973f_2396f04fa204 ;
            owl:someValuesFrom :electrochemistry_5ce6a328_713c_4383_ad63_26c902c30e34 ],
        [ a owl:Restriction ;
            owl:onProperty emmo:EMMO_e1097637_70d2_4895_973f_2396f04fa204 ;
            owl:someValuesFrom :electrochemistry_62e03250_8987_497b_85d5_1399aca9a0aa ],
        [ a owl:Restriction ;
            owl:onProperty emmo:EMMO_e1097637_70d2_4895_973f_2396f04fa204 ;
            owl:someValuesFrom :electrochemistry_7f17f6bb_c1f9_4f4a_bfdf_d8974443d07b ],
        [ a owl:Restriction ;
            owl:onProperty emmo:EMMO_e1097637_70d2_4895_973f_2396f04fa204 ;
            owl:someValuesFrom :electrochemistry_92fc0dba_6f11_4019_a8cb_db2a5b1634f5 ],
        [ a owl:Restriction ;
            owl:onProperty emmo:EMMO_e1097637_70d2_4895_973f_2396f04fa204 ;
            owl:someValuesFrom :electrochemistry_b83c6435_6edf_470e_9725_538a853e08f7 ],
        emmo:EMMO_ec7464a9_d99d_45f8_965b_4e9230ea8356 ;
    skos:prefLabel "Powder"@en ;
    emmo:EMMO_967080e5_2f42_4eb2_a3a9_c58143e835f9 "a material comprised of many particles"@en .

:electrochemistry_f19d3b4f_d59b_4a92_a547_54a6f59cc9b4 a owl:Class ;
    rdfs:label "LithiumNickelCobaltAluminumOxideElectrode"@en ;
    rdfs:comment "electrode in which the active material is lithium nickel cobalt aluminium oxide"@en ;
    rdfs:subClassOf [ a owl:Restriction ;
            owl:onProperty :electrochemistry_860aa941_5ff9_4452_8a16_7856fad07bee ;
            owl:someValuesFrom chems:substance_cd17ca33_ae3d_4738_8930_547673bf6c1f ],
        :electrochemistry_0d2aaaf4_1a8a_4a32_abd8_7d0fdf0ae9d2,
        :electrochemistry_e4b6cb36_4dac_49e3_871d_40bcfca943a5 ;
    owl:deprecated true ;
    skos:altLabel "NCAElectrode"@en ;
    skos:prefLabel "LithiumNickelCobaltAluminumOxideElectrode"@en ;
    emmo:EMMO_967080e5_2f42_4eb2_a3a9_c58143e835f9 "electrode in which the active material is lithium nickel cobalt aluminium oxide"@en .

:electrochemistry_f1c7eacb_9f21_4100_925c_3974f266e06f a owl:Class ;
    rdfs:label "BilayerMembrane"@en ;
    rdfs:comment "an asymmetric membrane composed of two layers, typically with different chemical properties or functional roles"@en ;
    rdfs:subClassOf :electrochemistry_b2d11f0d_c1b0_4476_8d17_03b73d31e01f ;
    skos:prefLabel "BilayerMembrane"@en ;
    emmo:EMMO_967080e5_2f42_4eb2_a3a9_c58143e835f9 "an asymmetric membrane composed of two layers, typically with different chemical properties or functional roles"@en .

:electrochemistry_f2251de5_0a7d_4887_8bd1_c906db84abee a owl:Class ;
    rdfs:label "R26700" ;
    rdfs:comment "a cylindrical case with a nominal diameter of 26 mm and height of 70 mm"@en ;
    rdfs:subClassOf :electrochemistry_b1cf9fee_2164_4f95_8204_90f717373a8a ;
    skos:altLabel "R26/70" ;
    skos:prefLabel "R26700" ;
    emmo:EMMO_967080e5_2f42_4eb2_a3a9_c58143e835f9 "a cylindrical case with a nominal diameter of 26 mm and height of 70 mm"@en .

:electrochemistry_f2cf71c1_f2d7_4131_82e0_2701cdecea55 a owl:Class ;
    rdfs:label "R1632" ;
    rdfs:comment "a coin case with a nominal diameter of 16.0 mm and a height of 3.2 mm"@en ;
    rdfs:subClassOf :electrochemistry_3979cd56_6256_414d_966c_7f723bf71e37 ;
    skos:prefLabel "R1632" ;
    emmo:EMMO_967080e5_2f42_4eb2_a3a9_c58143e835f9 "a coin case with a nominal diameter of 16.0 mm and a height of 3.2 mm"@en .

:electrochemistry_f49b84d4_e1f9_424c_bb22_8cea23c0a7d4 a owl:Class ;
    rdfs:label "ElectrochemicalMethod"@en ;
    rdfs:comment "a method used in electrochemistry"@en ;
    rdfs:subClassOf emmo:EMMO_bafc17b5_9be4_4823_8bbe_ab4e90b6738c ;
    owl:deprecated true ;
    skos:prefLabel "ElectrochemicalMethod"@en ;
    emmo:EMMO_967080e5_2f42_4eb2_a3a9_c58143e835f9 "a method used in electrochemistry"@en .

:electrochemistry_f4a6a682_fd7c_43df_bed2_df70848d6026 a owl:Class ;
    rdfs:label "P2714891" ;
    rdfs:comment "a prismatic case with a nominal length of 27 mm, width of 148 mm, and height of 91 mm"@en ;
    rdfs:subClassOf :electrochemistry_43cd6e14_dd43_41b5_b5b4_344d53841603 ;
    skos:altLabel "P27/148/91" ;
    skos:prefLabel "P2714891" ;
    emmo:EMMO_967080e5_2f42_4eb2_a3a9_c58143e835f9 "a prismatic case with a nominal length of 27 mm, width of 148 mm, and height of 91 mm"@en .

:electrochemistry_f54474fc_5d07_474b_97ae_f5d0349363b4 a owl:Class ;
    rdfs:label "HybridFlowCell"@en ;
    rdfs:comment "a flow cell that uses one or more electroactive components deposited as a solid layer"@en ;
    rdfs:subClassOf :electrochemistry_95e4aa95_b7e9_40d7_b78e_4d7dcc31093d ;
    skos:prefLabel "HybridFlowCell"@en ;
    emmo:EMMO_967080e5_2f42_4eb2_a3a9_c58143e835f9 "a flow cell that uses one or more electroactive components deposited as a solid layer"@en .

:electrochemistry_f57a7dac_2ec2_4d51_b697_01a844c4467f a owl:Class ;
    rdfs:label "TrasattiBuzzancaModel"@en ;
    rdfs:comment "considers the effects of specific adsorbed ions in the double layer"@en ;
    rdfs:subClassOf :electrochemistry_ac9723d1_bac0_4109_874e_32849de9299b ;
    skos:prefLabel "TrasattiBuzzancaModel"@en ;
    emmo:EMMO_967080e5_2f42_4eb2_a3a9_c58143e835f9 "considers the effects of specific adsorbed ions in the double layer"@en ;
    emmo:EMMO_c7b62dd7_063a_4c2a_8504_42f7264ba83f "proposed by Sergio Trasatti and Giovanni Buzzanca in 1971"@en .

:electrochemistry_f58476a9_f008_4502_ac94_2f1ebbce1fe3 a owl:Class ;
    rdfs:label "R38136" ;
    rdfs:comment "a cylindrical case with a nominal diameter of 38 mm and height of 136 mm"@en ;
    rdfs:subClassOf :electrochemistry_b1cf9fee_2164_4f95_8204_90f717373a8a ;
    skos:altLabel "R38/136" ;
    skos:prefLabel "R38136" ;
    emmo:EMMO_967080e5_2f42_4eb2_a3a9_c58143e835f9 "a cylindrical case with a nominal diameter of 38 mm and height of 136 mm"@en .

:electrochemistry_f6223121_7df5_42f8_902c_d26fa2fc4f04 a owl:Class ;
    rdfs:label "LeadOxideElectrode"@en ;
    rdfs:comment "electrode in which the active material is lead oxide"@en ;
    rdfs:subClassOf [ a owl:Restriction ;
            owl:onProperty :electrochemistry_860aa941_5ff9_4452_8a16_7856fad07bee ;
            owl:someValuesFrom chems:substance_4126ee09_b9c6_4694_bf33_0d8970e05f72 ],
        :electrochemistry_e4b6cb36_4dac_49e3_871d_40bcfca943a5 ;
    owl:deprecated true ;
    skos:altLabel "PbOElectrode"@en ;
    skos:prefLabel "LeadOxideElectrode"@en ;
    emmo:EMMO_967080e5_2f42_4eb2_a3a9_c58143e835f9 "electrode in which the active material is lead oxide"@en .

:electrochemistry_f6341d7d_7620_48f5_97b2_99b55c349169 a owl:Class ;
    rdfs:label "ParticleCracking"@en ;
    rdfs:comment "a degradation mechanism in electrochemical cells in which fractures in the particles degrade performance"@en ;
    rdfs:subClassOf [ a owl:Restriction ;
            owl:onProperty emmo:EMMO_ae2d1a96_bfa1_409a_a7d2_03d69e8a125a ;
            owl:someValuesFrom :electrochemistry_79d1b273_58cd_4be6_a250_434817f7c261 ],
        [ a owl:Restriction ;
            owl:onProperty emmo:EMMO_d67ee67e_4fac_4676_82c9_aec361dba698 ;
            owl:someValuesFrom :electrochemistry_e3d3d21c_cb9a_498c_bdb0_63c964f0d3c6 ],
        :electrochemistry_0a0de817_addc_46a5_8ba2_255d48cdf366 ;
    skos:prefLabel "ParticleCracking"@en ;
    skos:scopeNote "Often afflicts active material particles."@en ;
    emmo:EMMO_967080e5_2f42_4eb2_a3a9_c58143e835f9 "a degradation mechanism in electrochemical cells in which fractures in the particles degrade performance"@en .

:electrochemistry_f7e253da_b12e_40b0_ba51_8cb039839ab6 a owl:Class ;
    rdfs:label "R1225" ;
    rdfs:comment "a coin case with a nominal diameter of 12.05 mm and a height of 2.5 mm"@en ;
    rdfs:subClassOf :electrochemistry_3979cd56_6256_414d_966c_7f723bf71e37 ;
    skos:prefLabel "R1225" ;
    emmo:EMMO_967080e5_2f42_4eb2_a3a9_c58143e835f9 "a coin case with a nominal diameter of 12.05 mm and a height of 2.5 mm"@en .

:electrochemistry_f8e0d532_cf44_403c_9188_e00ee161a3c1 a owl:Class ;
    rdfs:label "CathodeElectrolyteInterphase"@en ;
    rdfs:comment "a type of solid electrolyte interface that forms on the surface of the electrode designated as the \"cathode\" or positive electrode"@en ;
    rdfs:subClassOf :electrochemistry_ecf136cb_2584_4cb1_98b7_2d2b3d22e40d ;
    owl:deprecated true ;
    skos:prefLabel "CathodeElectrolyteInterphase"@en ;
    emmo:EMMO_967080e5_2f42_4eb2_a3a9_c58143e835f9 "a type of solid electrolyte interface that forms on the surface of the electrode designated as the \"cathode\" or positive electrode"@en ;
    emmo:EMMO_c7b62dd7_063a_4c2a_8504_42f7264ba83f "used to distinguish the interphase on the cathode surface from that on the anode, which is typically called the solid electrolyte interphase (SEI)"@en .

:electrochemistry_f8f81b27_1d6c_42d8_a7e9_5a2534102562 a owl:Class ;
    rdfs:label "SodiumChromiumOxideElectrode"@en ;
    rdfs:comment "electrode in which the active material is sodium chromium oxide"@en ;
    rdfs:subClassOf [ a owl:Restriction ;
            owl:onProperty :electrochemistry_860aa941_5ff9_4452_8a16_7856fad07bee ;
            owl:someValuesFrom chems:substance_68f9b85e_340f_46ec_96da_ebb6bd62f5fd ],
        :electrochemistry_e4b6cb36_4dac_49e3_871d_40bcfca943a5 ;
    owl:deprecated true ;
    skos:prefLabel "SodiumChromiumOxideElectrode"@en ;
    emmo:EMMO_967080e5_2f42_4eb2_a3a9_c58143e835f9 "electrode in which the active material is sodium chromium oxide"@en .

:electrochemistry_f9e2e676_5cd1_4e22_a776_af45838d4027 a owl:Class ;
    rdfs:label "AmmoniaSolution"@en ;
    rdfs:comment "a solution of ammonia (NH3) dissolved in water (H2O)"@en ;
    rdfs:subClassOf :electrochemistry_615cff2a_be95_4e65_9471_98db23f4c878 ;
    owl:deprecated true ;
    skos:altLabel "AqueousAmmoniaSolution"@en ;
    skos:prefLabel "AmmoniaSolution"@en ;
    emmo:EMMO_967080e5_2f42_4eb2_a3a9_c58143e835f9 "a solution of ammonia (NH3) dissolved in water (H2O)"@en ;
    emmo:EMMO_c7b62dd7_063a_4c2a_8504_42f7264ba83f "the solution can also be made by dissolving ammonium hydroxide (NH4OH) in water"@en .

:electrochemistry_f9f056bb_a38b_43bd_a6bd_99d618431f4d a owl:Class ;
    rdfs:label "PalladiumBasedElectrode"@en ;
    rdfs:comment "an electrode in which the primary active material consists of palladium or palladium compounds"@en ;
    rdfs:subClassOf :electrochemistry_9a823d64_9d10_4a29_9cbd_9bbdad7985bc ;
    skos:prefLabel "PalladiumBasedElectrode"@en ;
    emmo:EMMO_967080e5_2f42_4eb2_a3a9_c58143e835f9 "an electrode in which the primary active material consists of palladium or palladium compounds"@en .

:electrochemistry_fa54f95d_b49e_43b5_84c3_35520d0fb2f6 a owl:Class ;
    rdfs:label "GouyChapmanModel"@en ;
    rdfs:comment "an extension of the Helmholtz model that describes the distribution of ions as a function of distance from the electrode surface to the bulk of the electroylte"@en ;
    rdfs:subClassOf :electrochemistry_ac9723d1_bac0_4109_874e_32849de9299b ;
    skos:prefLabel "GouyChapmanModel"@en ;
    emmo:EMMO_967080e5_2f42_4eb2_a3a9_c58143e835f9 "an extension of the Helmholtz model that describes the distribution of ions as a function of distance from the electrode surface to the bulk of the electroylte"@en ;
    emmo:EMMO_c7b62dd7_063a_4c2a_8504_42f7264ba83f "this model fails for highly charged double layers"@en .

:electrochemistry_fab4bd12_c4ed_417a_92a3_bcb109000d82 a owl:Class ;
    rdfs:label "R2040" ;
    rdfs:comment "a coin case with a nominal diameter of 20.0 mm and a height of 4.0 mm"@en ;
    rdfs:subClassOf :electrochemistry_3979cd56_6256_414d_966c_7f723bf71e37 ;
    skos:prefLabel "R2040" ;
    emmo:EMMO_967080e5_2f42_4eb2_a3a9_c58143e835f9 "a coin case with a nominal diameter of 20.0 mm and a height of 4.0 mm"@en .

:electrochemistry_fbf40756_3265_4468_bcdb_88d162afc539 a owl:Class ;
    rdfs:label "R2320" ;
    rdfs:comment "a coin case with a nominal diameter of 23.0 mm and a height of 2.0 mm"@en ;
    rdfs:subClassOf :electrochemistry_3979cd56_6256_414d_966c_7f723bf71e37 ;
    skos:prefLabel "R2320" ;
    emmo:EMMO_967080e5_2f42_4eb2_a3a9_c58143e835f9 "a coin case with a nominal diameter of 23.0 mm and a height of 2.0 mm"@en .

:electrochemistry_fc9e7ba3_5084_4c2a_b488_c6a96af99232 a owl:Class ;
    rdfs:label "R54215" ;
    rdfs:comment "a cylindrical case with a nominal diameter of 54 mm and height of 215 mm"@en ;
    rdfs:subClassOf :electrochemistry_b1cf9fee_2164_4f95_8204_90f717373a8a ;
    skos:altLabel "R54/215" ;
    skos:prefLabel "R54215" ;
    emmo:EMMO_967080e5_2f42_4eb2_a3a9_c58143e835f9 "a cylindrical case with a nominal diameter of 54 mm and height of 215 mm"@en .

:electrochemistry_fd7caf39_0a43_4fbf_958e_a62067aa9007 a owl:Class ;
    rdfs:label "LithiumCobaltOxideElectrode"@en ;
    rdfs:comment "electrode in which the active material is lithium cobalt oxide"@en ;
    rdfs:subClassOf [ a owl:Restriction ;
            owl:onProperty :electrochemistry_860aa941_5ff9_4452_8a16_7856fad07bee ;
            owl:someValuesFrom chems:substance_4c62d334_a124_40b3_9fd1_fe713d01a6af ],
        :electrochemistry_838c115b_6bc9_4ce8_9f8d_86a6bf67742a,
        :electrochemistry_e4b6cb36_4dac_49e3_871d_40bcfca943a5 ;
    owl:deprecated true ;
    skos:altLabel "LCOElectrode"@en ;
    skos:prefLabel "LithiumCobaltOxideElectrode"@en ;
    emmo:EMMO_967080e5_2f42_4eb2_a3a9_c58143e835f9 "electrode in which the active material is lithium cobalt oxide"@en .

:electrochemistry_fe054d02_41c7_40e9_8206_3440ab6a67b2 a owl:Class ;
    rdfs:label "R1154" ;
    rdfs:comment "a coin case with a nominal diameter of 11.6 mm and a height of 5.4 mm"@en ;
    rdfs:subClassOf :electrochemistry_3979cd56_6256_414d_966c_7f723bf71e37 ;
    skos:altLabel "R44" ;
    skos:prefLabel "R1154" ;
    emmo:EMMO_967080e5_2f42_4eb2_a3a9_c58143e835f9 "a coin case with a nominal diameter of 11.6 mm and a height of 5.4 mm"@en .

:electrochemistry_fe3a6c9a_85b8_4da6_aa4f_71c8de74939e a owl:Class ;
    rdfs:label "NernstEquation"@en ;
    rdfs:comment "An equation that relates the reduction potential of an electrochemical reaction (half-cell or full cell reaction) to the standard electrode potential, temperature, and activities (often approximated by concentrations) of the chemical species undergoing reduction and oxidation."@en ;
    rdfs:subClassOf :electrochemistry_3d805c2a_4801_440e_9e4d_0fa5585c76ae ;
    skos:prefLabel "NernstEquation"@en ;
    emmo:EMMO_26bf1bef_d192_4da6_b0eb_d2209698fb54 "https://www.wikidata.org/wiki/Q751124" ;
    emmo:EMMO_6dd685dd_1895_46e4_b227_be9f7d643c25 "https://dbpedia.org/page/Nernst_equation"@en ;
    emmo:EMMO_967080e5_2f42_4eb2_a3a9_c58143e835f9 "An equation that relates the reduction potential of an electrochemical reaction (half-cell or full cell reaction) to the standard electrode potential, temperature, and activities (often approximated by concentrations) of the chemical species undergoing reduction and oxidation."@en ;
    emmo:EMMO_c7b62dd7_063a_4c2a_8504_42f7264ba83f "E_{eq} = E^0 - (R*T/(z*F))*ln(Q)",
        "An expression of the Law of Mass Action."@en ;
    emmo:EMMO_c84c6752_6d64_48cc_9500_e54a3c34898d "https://en.wikipedia.org/wiki/Nernst_equation" .

:electrochemistry_fffc3dad_6946_4c32_a9d3_f5f311339881 a owl:Class ;
    rdfs:label "LithiumManganeseOxideLithiumIronPhosphateElectrode"@en ;
    rdfs:comment "an electrode with blended lithium manganese oxide (LMO) and lithium iron phosphate (LFP) active materials"@en ;
    rdfs:subClassOf [ a owl:Restriction ;
            owl:onProperty :electrochemistry_860aa941_5ff9_4452_8a16_7856fad07bee ;
            owl:someValuesFrom chems:substance_aa8e9cc4_5f66_4307_b1c8_26fac7653a90 ],
        [ a owl:Restriction ;
            owl:onProperty :electrochemistry_860aa941_5ff9_4452_8a16_7856fad07bee ;
            owl:someValuesFrom chems:substance_e8fafdc8_6cd3_4dd0_9630_10ca8e3f1827 ],
        :electrochemistry_4839708a_3864_47eb_b719_373ff8874c61 ;
    owl:deprecated true ;
    skos:altLabel "LMOLFPElectrode"@en ;
    skos:prefLabel "LithiumManganeseOxideLithiumIronPhosphateElectrode"@en ;
    emmo:EMMO_967080e5_2f42_4eb2_a3a9_c58143e835f9 "an electrode with blended lithium manganese oxide (LMO) and lithium iron phosphate (LFP) active materials"@en .

<https://w3id.org/emmo/domain/reference/electrochemistry-reference> a owl:Ontology ;
    dcterms:abstract "This reference module contains the core terms for the electrochmistry domain."@en ;
    dcterms:bibliographicCitation "https://doi.org/10.5281/zenodo.7693664" ;
    dcterms:contributor <https://orcid.org/0000-0001-8869-3718>,
        <https://orcid.org/0000-0002-1560-809X>,
        <https://orcid.org/0000-0002-2547-155X> ;
    dcterms:created "2022-11-25"^^xsd:date ;
    dcterms:creator <https://orcid.org/0000-0002-8758-6109>,
        <https://orcid.org/0000-0003-2954-1233> ;
    dcterms:issued "2025-02-12"^^xsd:date ;
    dcterms:license "https://creativecommons.org/licenses/by/4.0/legalcode" ;
    dcterms:modified "2025-02-12"^^xsd:date ;
    dcterms:publisher "EMMO" ;
    dcterms:source <https://doi.org/10.1109/IEEESTD.2016.7552407>,
        <https://doi.org/10.1351/goldbook>,
        <https://doi.org/10.1515/pac-2018-0109>,
        <https://www.electropedia.org> ;
    dcterms:title "Electrochemistry Domain Ontology"@en ;
    bibo:doi "10.5281/zenodo.7693664" ;
    bibo:status "unstable" ;
    vann:preferredNamespacePrefix "echem" ;
    vann:preferredNamespaceUri "https://w3id.org/emmo/domain/electrochemistry" ;
    owl:backwardCompatibleWith "0.26.0-beta" ;
    owl:imports <https://w3id.org/emmo/1.0.0>,
        <https://w3id.org/emmo/domain/characterisation-methodology/1.0.0/chameo>,
        <https://w3id.org/emmo/domain/chemical-substance/0.12.2-beta/chemical-substance>,
        <https://w3id.org/emmo/domain/electrochemistry/0.31.0/reference/electrochemistry-quantities> ;
    owl:priorVersion "0.26.0-beta" ;
    owl:versionIRI <https://w3id.org/emmo/domain/electrochemistry/0.31.0/reference/electrochemistry-reference> ;
    owl:versionInfo "0.31.0" ;
    foaf:logo "https://raw.githubusercontent.com/emmo-repo/domain-electrochemistry/gh-pages/assets/img/fig/png/domain-electrochemistry-logo.png" .

<https://orcid.org/0000-0001-8869-3718> a schema:Person ;
    rdfs:label "Francesca Lnstad Bleken" ;
    skos:prefLabel "Francesca Lnstad Bleken" ;
    schema:additionalName "Lnstad" ;
    schema:familyName "Bleken" ;
    schema:givenName "Francesca" ;
    schema:name "Francesca Lnstad Bleken" ;
    emmo:EMMO_c7b62dd7_063a_4c2a_8504_42f7264ba83f "" .

<https://orcid.org/0000-0002-1560-809X> a schema:Person ;
    rdfs:label "Jesper Friis" ;
    skos:prefLabel "Jesper Friis" ;
    schema:familyName "Friis" ;
    schema:givenName "Jesper" ;
    schema:name "Jesper Friis" ;
    emmo:EMMO_c7b62dd7_063a_4c2a_8504_42f7264ba83f "" .

<https://orcid.org/0000-0002-2547-155X> a schema:Person ;
    rdfs:label "Casper Welzel Andersen" ;
    skos:prefLabel "Casper Welzel Andersen" ;
    schema:additionalName "Welzel" ;
    schema:familyName "Andersen" ;
    schema:givenName "Casper" ;
    schema:name "Casper Welzel Andersen" ;
    emmo:EMMO_c7b62dd7_063a_4c2a_8504_42f7264ba83f "" .

<https://orcid.org/0000-0002-8758-6109> a schema:Person ;
    rdfs:label "Simon Clark" ;
    skos:prefLabel "Simon Clark" ;
    schema:familyName "Clark" ;
    schema:givenName "Simon" ;
    schema:name "Simon Clark" ;
    emmo:EMMO_c7b62dd7_063a_4c2a_8504_42f7264ba83f "" .

<https://orcid.org/0000-0003-2954-1233> a schema:Person ;
    rdfs:label "Eibar Flores" ;
    skos:prefLabel "Eibar Flores" ;
    schema:familyName "Flores" ;
    schema:givenName "Eibar" ;
    schema:name "Eibar Flores" ;
    emmo:EMMO_c7b62dd7_063a_4c2a_8504_42f7264ba83f "" .

emmo:EMMO_08bd340b_9d49_4d60_8ac5_b89f2f442169 a owl:ObjectProperty ;
    rdfs:label "hasProcessParameter"@en ;
    rdfs:comment "an object property linking a process to a process parameter"@en ;
    rdfs:range emmo:EMMO_cf80faa4_69d2_46d1_8a2b_f7f63ca244c1 ;
    rdfs:subPropertyOf emmo:EMMO_36e69413_8c59_4799_946c_10b05d266e22 ;
    skos:note "consider promoting to EMMO top or middle"@en ;
    skos:prefLabel "hasProcessParameter"@en ;
    emmo:EMMO_967080e5_2f42_4eb2_a3a9_c58143e835f9 "an object property linking a process to a process parameter"@en .

emmo:EMMO_2031516a_2be7_48e8_9af7_7e1270e308fe rdfs:subClassOf [ a owl:Restriction ;
            owl:onProperty :electrochemistry_808e94df_e002_4e64_a6db_182ed75078c6 ;
            owl:someValuesFrom emmo:EMMO_bc37743c_37c4_4ec7_9d58_d1aae5567352 ],
        [ a owl:Restriction ;
            owl:onProperty :electrochemistry_8784ef24_320b_4a3d_b200_654aec6c271c ;
            owl:someValuesFrom emmo:EMMO_bc37743c_37c4_4ec7_9d58_d1aae5567352 ] .

emmo:EMMO_35c29eb6_f57e_48d8_85af_854f9e926e77 a owl:InverseFunctionalProperty,
        owl:ObjectProperty .

emmo:EMMO_57d977ab_0036_4779_b59a_e47620afdb9c rdfs:subClassOf emmo:EMMO_38b579de_4331_40e0_803d_09efa298e726 .

emmo:EMMO_cf80faa4_69d2_46d1_8a2b_f7f63ca244c1 a owl:Class ;
    rdfs:label "ProcessParameter"@en ;
    rdfs:comment "A parameter that describes a process"@en ;
    rdfs:subClassOf emmo:EMMO_d1d436e7_72fc_49cd_863b_7bfb4ba5276a ;
    skos:note "consider promoting to EMMO top or middle"@en ;
    skos:prefLabel "ProcessParameter"@en ;
    emmo:EMMO_967080e5_2f42_4eb2_a3a9_c58143e835f9 "A parameter that describes a process"@en .

:electrochemistry_01260656_ac32_472e_9513_a607366538ec a owl:Class ;
    rdfs:label "ElectrodePassivation"@en ;
    rdfs:comment "formation of compounds that reduces the conductivity at the surface of an electrode"@en ;
    rdfs:subClassOf [ a owl:Restriction ;
            owl:onProperty emmo:EMMO_ae2d1a96_bfa1_409a_a7d2_03d69e8a125a ;
            owl:someValuesFrom :electrochemistry_0f007072_a8dd_4798_b865_1bf9363be627 ],
        [ a owl:Restriction ;
            owl:onProperty emmo:EMMO_ae2d1a96_bfa1_409a_a7d2_03d69e8a125a ;
            owl:someValuesFrom :electrochemistry_d16eec87_c646_4566_bda6_7d3357cda061 ],
        :electrochemistry_19abaccd_43be_4048_965c_e4fb63c5951b ;
    skos:altLabel "Passivation"@en ;
    skos:prefLabel "ElectrodePassivation"@en ;
    emmo:EMMO_26bf1bef_d192_4da6_b0eb_d2209698fb54 "https://www.wikidata.org/wiki/Q917260"@en ;
    emmo:EMMO_50c298c2_55a2_4068_b3ac_4e948c33181f "https://www.electropedia.org/iev/iev.nsf/display?openform&ievref=114-02-16"@en ;
    emmo:EMMO_967080e5_2f42_4eb2_a3a9_c58143e835f9 "formation of compounds that reduces the conductivity at the surface of an electrode"@en ;
    emmo:EMMO_c84c6752_6d64_48cc_9500_e54a3c34898d "https://en.wikipedia.org/wiki/Passivation_(chemistry)"@en .

:electrochemistry_0471ec77_91bc_4a78_be31_b6af613e5966 a owl:Class ;
    rdfs:label "Neutralisation"@en ;
    rdfs:comment "insertion or removal of electrons into or from ions to obtain particles having zero electric charge"@en ;
    rdfs:subClassOf emmo:EMMO_135ab8ea_e028_439e_be64_3e0f9734ea2b ;
    skos:altLabel "Neutralization"@en ;
    skos:prefLabel "Neutralisation"@en ;
    emmo:EMMO_50c298c2_55a2_4068_b3ac_4e948c33181f "https://www.electropedia.org/iev/iev.nsf/display?openform&ievref=114-01-11" ;
    emmo:EMMO_967080e5_2f42_4eb2_a3a9_c58143e835f9 "insertion or removal of electrons into or from ions to obtain particles having zero electric charge"@en .

:electrochemistry_0508a114_544a_4f54_a7de_9b947fb4b618 a owl:Class ;
    rdfs:label "SolidElectrolyte"@en ;
    rdfs:subClassOf :electrochemistry_fb0d9eef_92af_4628_8814_e065ca255d59 ;
    skos:altLabel "FastIonConductor"@en,
        "SolidStateElectrolyte"@en ;
    skos:example "NASICON (Na Super Ionic Conductor), which has the general formula Na1+xZr2P3-xSix O12 , 0 < x < 3."@en ;
    skos:prefLabel "SolidElectrolyte"@en ;
    emmo:EMMO_70fe84ff_99b6_4206_a9fc_9a8931836d84 "a solid electrolyte is a solid material where the predominant charge carriers are ions."@en ;
    emmo:EMMO_c84c6752_6d64_48cc_9500_e54a3c34898d "https://en.wikipedia.org/wiki/Fast_ion_conductor"@en .

:electrochemistry_0c9017b4_6efd_4e2b_8e24_48b60ebe9315 a owl:Class ;
    rdfs:label "GasDissolution"@en ;
    rdfs:comment "the dissolution of molecules from a gas into another phase"@en ;
    rdfs:subClassOf :electrochemistry_49263a32_eca6_4644_8144_0d3b14c26d0a ;
    skos:example "Absorption of CO into an alkaline electrolyte forming carbonate species."@en,
        "Hydrogen evolution during water electrolysis."@en ;
    skos:note "Often leads to efficiency loss or mechanical degradation in electrochemical devices."@en ;
    skos:prefLabel "GasDissolution"@en ;
    skos:related :electrochemistry_4288b145_ba79_4989_92f8_86086679b0fe ;
    emmo:EMMO_967080e5_2f42_4eb2_a3a9_c58143e835f9 "the dissolution of molecules from a gas into another phase"@en .

:electrochemistry_0ee59786_b090_444d_a46d_505797d07ca4 a owl:Class ;
    rdfs:label "VanadiumBasedElectrode"@en ;
    rdfs:comment "an electrode in which the primary active material consists of vanadium or vanadium compounds"@en ;
    rdfs:subClassOf :electrochemistry_9a823d64_9d10_4a29_9cbd_9bbdad7985bc ;
    skos:prefLabel "VanadiumBasedElectrode"@en ;
    emmo:EMMO_967080e5_2f42_4eb2_a3a9_c58143e835f9 "an electrode in which the primary active material consists of vanadium or vanadium compounds"@en ;
    emmo:EMMO_c7b62dd7_063a_4c2a_8504_42f7264ba83f "often represented in IEC cell designations by the letter V"@en,
        "this class is intended to enable designations based on IEC recommendations"@en .

:electrochemistry_0f827b54_370d_4c63_99a6_80f13b24e55e a owl:Class ;
    rdfs:label "GassingOfACell"@en ;
    rdfs:comment "evolution of gas resulting from electrolysis of the water in the electrolyte of a cell"@en ;
    rdfs:subClassOf [ a owl:Restriction ;
            owl:onProperty emmo:EMMO_d43af210_f854_4432_a891_ce3022e3b558 ;
            owl:someValuesFrom :electrochemistry_4288b145_ba79_4989_92f8_86086679b0fe ],
        :electrochemistry_19abaccd_43be_4048_965c_e4fb63c5951b ;
    skos:prefLabel "GassingOfACell"@en ;
    emmo:EMMO_50c298c2_55a2_4068_b3ac_4e948c33181f "https://www.electropedia.org/iev/iev.nsf/display?openform&ievref=482-05-51"@en ;
    emmo:EMMO_967080e5_2f42_4eb2_a3a9_c58143e835f9 "evolution of gas resulting from electrolysis of the water in the electrolyte of a cell"@en .

:electrochemistry_113e0469_8ae0_407f_892d_4b988f8d8a08 a owl:Class ;
    rdfs:label "ThermogalvanicCell"@en ;
    rdfs:comment "electrochemical cell that has two half-cells separated by a wall permeable to ions, both containing the same electrolyte differing only in their temperatures."@en ;
    rdfs:subClassOf :electrochemistry_0acd0fc2_1048_4604_8e90_bf4e84bd87df ;
    skos:altLabel "Thermocell"@en ;
    skos:prefLabel "ThermogalvanicCell"@en ;
    emmo:EMMO_26bf1bef_d192_4da6_b0eb_d2209698fb54 "https://www.wikidata.org/wiki/Q25304247" ;
    emmo:EMMO_50c298c2_55a2_4068_b3ac_4e948c33181f "https://www.electropedia.org/iev/iev.nsf/display?openform&ievref=114-03-09"@en ;
    emmo:EMMO_967080e5_2f42_4eb2_a3a9_c58143e835f9 "electrochemical cell that has two half-cells separated by a wall permeable to ions, both containing the same electrolyte differing only in their temperatures."@en ;
    emmo:EMMO_c84c6752_6d64_48cc_9500_e54a3c34898d "https://en.wikipedia.org/wiki/Thermogalvanic_cell"@en .

:electrochemistry_1152ae6b_8b57_4d99_912e_40c6a29342fb a owl:Class ;
    rdfs:label "FaradaysFirstLawOfElectrolysis"@en ;
    rdfs:comment "mass m of electrochemically-transformed substance is proportional to the charge Q passed, m  Q."@en ;
    rdfs:subClassOf emmo:EMMO_9c32fd69_f480_4130_83b3_fb25d9face14 ;
    skos:altLabel "FaradaysLaw"@en,
        "FaradaysLawOfElectrolysis"@en ;
    skos:prefLabel "FaradaysFirstLawOfElectrolysis"@en ;
    emmo:EMMO_967080e5_2f42_4eb2_a3a9_c58143e835f9 "mass m of electrochemically-transformed substance is proportional to the charge Q passed, m  Q."@en ;
    emmo:EMMO_c84c6752_6d64_48cc_9500_e54a3c34898d "https://en.wikipedia.org/wiki/Faraday%27s_laws_of_electrolysis#First_law"@en .

:electrochemistry_15325775_6d4c_4192_82f1_e4feca9de426 a owl:Class ;
    rdfs:label "IonExchangeMembrane"@en ;
    rdfs:comment "A membrane having ion-exchange groups:"@en ;
    rdfs:subClassOf :electrochemistry_331e6cca_f260_4bf8_af55_35304fe1bbe0 ;
    skos:prefLabel "IonExchangeMembrane"@en ;
    emmo:EMMO_26bf1bef_d192_4da6_b0eb_d2209698fb54 "https://www.wikidata.org/wiki/Q21082486" ;
    emmo:EMMO_967080e5_2f42_4eb2_a3a9_c58143e835f9 "A membrane having ion-exchange groups:"@en ;
    emmo:EMMO_c7b62dd7_063a_4c2a_8504_42f7264ba83f "a selective barrier that permits the passage of ions of one sign while preventing the passage of ions of opposite sign."@en ;
    emmo:EMMO_c84c6752_6d64_48cc_9500_e54a3c34898d "https://en.wikipedia.org/wiki/Ion-exchange_membrane" ;
    emmo:EMMO_fe015383_afb3_44a6_ae86_043628697aa2 "https://doi.org/10.1351/goldbook.IT07155"@en .

:electrochemistry_1784d824_15bd_4eff_9e40_61e23be6f979 a owl:ObjectProperty ;
    rdfs:label "hasElectrochemicalCell"@en ;
    rdfs:domain :electrochemistry_0acd0fc2_1048_4604_8e90_bf4e84bd87df ;
    rdfs:range :electrochemistry_6f2c88c9_5c04_4953_a298_032cc3ab9b77 ;
    rdfs:subPropertyOf emmo:EMMO_3c7f239f_e833_4a2b_98a1_c88831770c1b ;
    skos:prefLabel "hasElectrochemicalCell"@en .

:electrochemistry_187326b9_1089_4122_8e7e_1a0bcba210a1 a owl:Class ;
    rdfs:label "CathodicPolarisation"@en ;
    rdfs:comment "electrode polarization associated with a cathodic reaction"@en ;
    rdfs:subClassOf :electrochemistry_2e6933aa_4522_4f16_a437_37110e6cbd0d ;
    skos:altLabel "CathodicPolarization"@en ;
    skos:prefLabel "CathodicPolarisation"@en ;
    emmo:EMMO_50c298c2_55a2_4068_b3ac_4e948c33181f "https://www.electropedia.org/iev/iev.nsf/display?openform&ievref=114-02-18"@en ;
    emmo:EMMO_967080e5_2f42_4eb2_a3a9_c58143e835f9 "electrode polarization associated with a cathodic reaction"@en .

:electrochemistry_1a2eb6db_c927_4039_aea0_8dfab060fd27 a owl:Class ;
    rdfs:label "Mudrib"@en ;
    rdfs:comment "ridges in the bottom of the case which support the plate pack (electrode stack) and thus create a space which allows the active material detached from the plates (electrodes) to settle without causing a short-circuit between the plates (electrodes)"@en ;
    rdfs:subClassOf emmo:EMMO_f76884f7_964e_488e_9bb7_1b2453e9e817 ;
    skos:prefLabel "Mudrib"@en ;
    emmo:EMMO_50c298c2_55a2_4068_b3ac_4e948c33181f "https://www.electropedia.org/iev/iev.nsf/display?openform&ievref=482-05-18" ;
    emmo:EMMO_967080e5_2f42_4eb2_a3a9_c58143e835f9 "ridges in the bottom of the case which support the plate pack (electrode stack) and thus create a space which allows the active material detached from the plates (electrodes) to settle without causing a short-circuit between the plates (electrodes)"@en .

:electrochemistry_1e72986e_e19f_4c24_8663_cadd4318bd72 a owl:Class ;
    rdfs:label "StoichiometricEquation"@en ;
    rdfs:comment "the symbolic representation of a chemical reaction in the form of symbols and formulae, wherein the reactant entities are given on the left-hand side and the product entities on the right-hand side"@en ;
    rdfs:subClassOf emmo:EMMO_54ee6b5e_5261_44a8_86eb_5717e7fdb9d0,
        emmo:EMMO_bd8db028_aec2_4a44_ad93_1a9f8270f72c ;
    skos:altLabel "ChemicalEquation"@en,
        "ChemicalReactionEquation"@en ;
    skos:prefLabel "StoichiometricEquation"@en ;
    emmo:EMMO_26bf1bef_d192_4da6_b0eb_d2209698fb54 "https://www.wikidata.org/wiki/Q182527" ;
    emmo:EMMO_6dd685dd_1895_46e4_b227_be9f7d643c25 "https://dbpedia.org/page/Chemical_equation"@en ;
    emmo:EMMO_967080e5_2f42_4eb2_a3a9_c58143e835f9 "the symbolic representation of a chemical reaction in the form of symbols and formulae, wherein the reactant entities are given on the left-hand side and the product entities on the right-hand side"@en ;
    emmo:EMMO_c84c6752_6d64_48cc_9500_e54a3c34898d "https://en.wikipedia.org/wiki/Chemical_equation"@en ;
    emmo:EMMO_fe015383_afb3_44a6_ae86_043628697aa2 "https://doi.org/10.1351/goldbook.C01034"@en .

:electrochemistry_1f2d401c_eede_4178_9ff5_e5392bc2cb92 a owl:DatatypeProperty ;
    rdfs:label "hasIECCode"@en ;
    skos:prefLabel "hasIECCode"@en .

:electrochemistry_1fc5642c_b7b2_43bf_ad20_f96001db8800 a owl:Class ;
    rdfs:label "SupportingElectrolyte"@en ;
    rdfs:comment "electrolyte solution, the ions of which are electroinactive in the range of applied potential being studied, and whose ionic strength (and, therefore, contribution to the overall conductivity) is usually much greater than the concentration of an electroactive substance to be dissolved in it."@en ;
    rdfs:subClassOf :electrochemistry_fa22874b_76a9_4043_8b8f_6086c88746de ;
    skos:altLabel "BaseElectrolyte"@en,
        "IndifferentElectrolyte"@en,
        "InertElectrolyte"@en ;
    skos:prefLabel "SupportingElectrolyte"@en ;
    emmo:EMMO_967080e5_2f42_4eb2_a3a9_c58143e835f9 "electrolyte solution, the ions of which are electroinactive in the range of applied potential being studied, and whose ionic strength (and, therefore, contribution to the overall conductivity) is usually much greater than the concentration of an electroactive substance to be dissolved in it."@en ;
    emmo:EMMO_c84c6752_6d64_48cc_9500_e54a3c34898d "https://en.wikipedia.org/wiki/Supporting_electrolyte"@en ;
    emmo:EMMO_fe015383_afb3_44a6_ae86_043628697aa2 "https://goldbook.iupac.org/terms/view/S06149"@en .

:electrochemistry_26b19a7c_59ca_4e1b_8fb9_ba061c22531e a owl:Class ;
    rdfs:label "CopperBasedElectrode"@en ;
    rdfs:comment "an electrode in which the primary active material consists of copper or copper compounds"@en ;
    rdfs:subClassOf :electrochemistry_9a823d64_9d10_4a29_9cbd_9bbdad7985bc ;
    skos:prefLabel "CopperBasedElectrode"@en ;
    emmo:EMMO_967080e5_2f42_4eb2_a3a9_c58143e835f9 "an electrode in which the primary active material consists of copper or copper compounds"@en .

:electrochemistry_27662d03_1bcf_4393_a239_32e31b760839 a owl:Class ;
    rdfs:label "ElectrodeStack"@en ;
    rdfs:comment "finished assembly of the positive and negative plate (electrode) groups with interleaved separators and terminals or intercell connectors"@en ;
    rdfs:subClassOf emmo:EMMO_52bbaaee_1145_4be3_8a5c_b366851ea1b9 ;
    skos:altLabel "PlatePack"@en ;
    skos:prefLabel "ElectrodeStack"@en ;
    emmo:EMMO_50c298c2_55a2_4068_b3ac_4e948c33181f "https://www.electropedia.org/iev/iev.nsf/display?openform&ievref=482-02-08" ;
    emmo:EMMO_967080e5_2f42_4eb2_a3a9_c58143e835f9 "finished assembly of the positive and negative plate (electrode) groups with interleaved separators and terminals or intercell connectors"@en .

:electrochemistry_27a81a51_e8d7_42fb_834f_0d068fa45d89 a owl:Class ;
    rdfs:label "SaturatedSolution"@en ;
    rdfs:comment "solution which has the same concentration of a solute as one that is in equilibrium with undissolved solute at specified values of the temperature and pressure" ;
    rdfs:subClassOf emmo:EMMO_2031516a_2be7_48e8_9af7_7e1270e308fe ;
    skos:prefLabel "SaturatedSolution"@en ;
    emmo:EMMO_50c298c2_55a2_4068_b3ac_4e948c33181f "https://www.electropedia.org/iev/iev.nsf/display?openform&ievref=114-01-14" ;
    emmo:EMMO_967080e5_2f42_4eb2_a3a9_c58143e835f9 "solution which has the same concentration of a solute as one that is in equilibrium with undissolved solute at specified values of the temperature and pressure" ;
    emmo:EMMO_fe015383_afb3_44a6_ae86_043628697aa2 "https://doi.org/10.1351/goldbook.S05471"@en .

:electrochemistry_28213033_4c74_441c_81c4_a0cad05f9eb6 a owl:Class ;
    rdfs:label "AnodicPolarisation"@en ;
    rdfs:comment "electrode polarization associated with an anodic reaction"@en ;
    rdfs:subClassOf :electrochemistry_2e6933aa_4522_4f16_a437_37110e6cbd0d ;
    skos:altLabel "AnodicPolarization"@en ;
    skos:prefLabel "AnodicPolarisation"@en ;
    emmo:EMMO_50c298c2_55a2_4068_b3ac_4e948c33181f "https://www.electropedia.org/iev/iev.nsf/display?openform&ievref=114-02-17"@en ;
    emmo:EMMO_967080e5_2f42_4eb2_a3a9_c58143e835f9 "electrode polarization associated with an anodic reaction"@en .

:electrochemistry_2a40b878_7d09_49db_91b2_d0ee30192284 a owl:Class ;
    rdfs:label "StandardHydrogenElectrode"@en ;
    rdfs:comment "for solutions in protic solvents, the universal reference electrode for which, under standard conditions, the standard electrode potential (H+ / H2) is zero at all temperatures"@en ;
    rdfs:subClassOf :electrochemistry_7729c34e_1ae9_403d_b933_1765885e7f29 ;
    skos:altLabel "SHE"@en ;
    skos:prefLabel "StandardHydrogenElectrode"@en ;
    emmo:EMMO_26bf1bef_d192_4da6_b0eb_d2209698fb54 "https://www.wikidata.org/wiki/Q898559" ;
    emmo:EMMO_967080e5_2f42_4eb2_a3a9_c58143e835f9 "for solutions in protic solvents, the universal reference electrode for which, under standard conditions, the standard electrode potential (H+ / H2) is zero at all temperatures"@en ;
    emmo:EMMO_c7b62dd7_063a_4c2a_8504_42f7264ba83f "Potential of a platinum electrode in a theoretical ideal solution (the current standard for zero potential for all temperatures)"@en ;
    emmo:EMMO_c84c6752_6d64_48cc_9500_e54a3c34898d "https://en.wikipedia.org/wiki/Standard_hydrogen_electrode"@en ;
    emmo:EMMO_fe015383_afb3_44a6_ae86_043628697aa2 "https://goldbook.iupac.org/terms/view/S05917"@en .

:electrochemistry_2b50cdac_581f_48b9_87ca_bad5138ab58d a owl:Class ;
    rdfs:label "DoubleLayer"@en ;
    rdfs:comment "a double layer of charges exists at the interface between two conducting media: One side carries a positive excess charge, which is balanced by a negative excess of equal magnitude on the other side."@en ;
    rdfs:subClassOf :electrochemistry_f78e3c87_01c6_4cc2_b047_30322262e22d ;
    skos:altLabel "DL"@en,
        "EDL"@en,
        "ElectricalDoubleLayer"@en ;
    skos:prefLabel "DoubleLayer"@en ;
    emmo:EMMO_26bf1bef_d192_4da6_b0eb_d2209698fb54 "https://www.wikidata.org/wiki/Q904857" ;
    emmo:EMMO_967080e5_2f42_4eb2_a3a9_c58143e835f9 "a double layer of charges exists at the interface between two conducting media: One side carries a positive excess charge, which is balanced by a negative excess of equal magnitude on the other side."@en ;
    emmo:EMMO_c84c6752_6d64_48cc_9500_e54a3c34898d "https://en.wikipedia.org/wiki/Double_layer_(surface_science)"@en .

:electrochemistry_2d32a81a_2148_41bd_84fb_467aa8de4a8f a owl:Class ;
    rdfs:label "PlatinumElectrode"@en ;
    rdfs:comment "foil, wire, disc, or mesh electrode made of platinum, which is the most commonly used metallic working electrode in electrochemistry"@en ;
    rdfs:subClassOf [ a owl:Restriction ;
            owl:onProperty :electrochemistry_860aa941_5ff9_4452_8a16_7856fad07bee ;
            owl:someValuesFrom chems:substance_25f6ff4c_53ad_4837_97c4_aa6f06099bb5 ],
        :electrochemistry_d8a9a88e_d437_4fef_bc3c_65a1fe627061 ;
    skos:altLabel "PtElectrode"@en ;
    skos:prefLabel "PlatinumElectrode"@en ;
    emmo:EMMO_26bf1bef_d192_4da6_b0eb_d2209698fb54 "https://www.wikidata.org/wiki/Q20851363" ;
    emmo:EMMO_967080e5_2f42_4eb2_a3a9_c58143e835f9 "foil, wire, disc, or mesh electrode made of platinum, which is the most commonly used metallic working electrode in electrochemistry"@en ;
    emmo:EMMO_c7b62dd7_063a_4c2a_8504_42f7264ba83f "Pt has a very small overpotential for hydrogen evolution, which determines the negative potential limit in protic solvents. Pt adsorbs hydrogen, resulting in hydrogen adsorption/desorption waves. However, the positive potential limit in polar aprotic solvents free of oxygen and water is higher than that for any other commonly used electrode materials. In the presence of water and/or oxygen, Pt forms a film of oxide (and/or chemisorbed oxygen), resulting in potentially interfering waves or peaks."@en .

:electrochemistry_34bc54e3_de4c_41f8_8d3a_d77c951ee23a a owl:Class ;
    rdfs:label "Dendrite"@en ;
    rdfs:comment "needle-like or tree-like formation of crystalline growth formed during deposition of a material"@en ;
    rdfs:subClassOf emmo:EMMO_4f226cf3_6d02_4d35_8566_a9e641bc6ff3 ;
    skos:prefLabel "Dendrite"@en ;
    emmo:EMMO_26bf1bef_d192_4da6_b0eb_d2209698fb54 "https://www.wikidata.org/wiki/Q190136" ;
    emmo:EMMO_50c298c2_55a2_4068_b3ac_4e948c33181f "https://www.electropedia.org/iev/iev.nsf/display?openform&ievref=114-04-07" ;
    emmo:EMMO_967080e5_2f42_4eb2_a3a9_c58143e835f9 "needle-like or tree-like formation of crystalline growth formed during deposition of a material"@en ;
    emmo:EMMO_c84c6752_6d64_48cc_9500_e54a3c34898d "https://en.wikipedia.org/wiki/Dendrite_(crystal)"@en ;
    emmo:EMMO_fe015383_afb3_44a6_ae86_043628697aa2 "https://doi.org/10.1351/goldbook.D01588"@en .

:electrochemistry_3a77b5e7_9646_4154_bf8f_5f798989e5f3 a owl:Class ;
    rdfs:label "AnnularWorkingElectrode"@en ;
    rdfs:comment "a working electrode in the shape of a ring used in a rotating ring disk electrode (RRDE)."@en ;
    rdfs:subClassOf :electrochemistry_fb988878_ee54_4350_9ee9_228c00c3ad35 ;
    skos:altLabel "RingElectrode"@en ;
    skos:prefLabel "AnnularWorkingElectrode"@en ;
    emmo:EMMO_967080e5_2f42_4eb2_a3a9_c58143e835f9 "a working electrode in the shape of a ring used in a rotating ring disk electrode (RRDE)."@en .

:electrochemistry_3dcfe33d_6825_43c0_a798_68e871a68d39 a owl:ObjectProperty ;
    rdfs:label "hasCase"@en ;
    rdfs:comment "relates a device or assembly to the outer enclosure or housing that provides mechanical protection and containment"@en ;
    rdfs:domain :electrochemistry_0acd0fc2_1048_4604_8e90_bf4e84bd87df ;
    rdfs:range :electrochemistry_1aec4cc0_82d5_4042_a657_ed7fe291c3d8 ;
    rdfs:subPropertyOf emmo:EMMO_3c7f239f_e833_4a2b_98a1_c88831770c1b ;
    skos:prefLabel "hasCase"@en ;
    emmo:EMMO_967080e5_2f42_4eb2_a3a9_c58143e835f9 "relates a device or assembly to the outer enclosure or housing that provides mechanical protection and containment"@en .

:electrochemistry_403c300e_09b9_400b_943b_04e82a3cfb56 a owl:Class ;
    rdfs:label "ElectrodeCoating"@en ;
    rdfs:comment "a coating layer that is part of an electrode and contains one or more active chemical substances together with auxiliary components"@en ;
    rdfs:subClassOf [ a owl:Restriction ;
            owl:onProperty emmo:EMMO_e1097637_70d2_4895_973f_2396f04fa204 ;
            owl:someValuesFrom emmo:EMMO_3a6578ac_aee0_43b9_9bc6_1eb208c8c9a9 ],
        [ a owl:Restriction ;
            owl:onProperty emmo:EMMO_e1097637_70d2_4895_973f_2396f04fa204 ;
            owl:someValuesFrom emmo:EMMO_43003c86_9d15_433b_9789_ee2940920656 ],
        [ a owl:Restriction ;
            owl:onProperty :electrochemistry_056a5fab_3d99_46bd_8eb1_6e89a368e1a7 ;
            owl:someValuesFrom emmo:EMMO_df96cbb6_b5ee_4222_8eab_b3675df24bea ],
        [ a owl:Restriction ;
            owl:onProperty :electrochemistry_7df82c48_b599_4b02_bef0_9facc9c39410 ;
            owl:someValuesFrom emmo:EMMO_df96cbb6_b5ee_4222_8eab_b3675df24bea ],
        [ a owl:Restriction ;
            owl:onProperty :electrochemistry_860aa941_5ff9_4452_8a16_7856fad07bee ;
            owl:someValuesFrom emmo:EMMO_df96cbb6_b5ee_4222_8eab_b3675df24bea ],
        :electrochemistry_09a7f560_9ddf_4c32_b067_b213eca5b0a1 ;
    skos:example "A LiFePO4 cathode coating comprising LFP powder (active), PVDF (binder), and carbon black (conductive additive)"@en ;
    skos:prefLabel "ElectrodeCoating"@en ;
    skos:related :electrochemistry_0a399f3f_b873_41f5_be1f_9b6df75cc30a,
        :electrochemistry_68eb5e35_5bd8_47b1_9b7f_f67224fa291e,
        :electrochemistry_92147e31_d015_4889_a092_04fbab033f15 ;
    emmo:EMMO_967080e5_2f42_4eb2_a3a9_c58143e835f9 "a coating layer that is part of an electrode and contains one or more active chemical substances together with auxiliary components"@en .

:electrochemistry_444992e5_43f8_44a1_9767_b408dbe54330 a owl:Class ;
    rdfs:label "SelfDischarging"@en ;
    rdfs:comment "phenomenon by which a cell or battery loses energy in other ways than by discharge into an external circuit"@en ;
    rdfs:seeAlso "ChargeRetention"@en ;
    rdfs:subClassOf :electrochemistry_e3d3d21c_cb9a_498c_bdb0_63c964f0d3c6 ;
    skos:prefLabel "SelfDischarging"@en ;
    emmo:EMMO_26bf1bef_d192_4da6_b0eb_d2209698fb54 "https://www.wikidata.org/wiki/Q1418367" ;
    emmo:EMMO_50c298c2_55a2_4068_b3ac_4e948c33181f "https://www.electropedia.org/iev/iev.nsf/display?openform&ievref=482-03-27" ;
    emmo:EMMO_967080e5_2f42_4eb2_a3a9_c58143e835f9 "phenomenon by which a cell or battery loses energy in other ways than by discharge into an external circuit"@en ;
    emmo:EMMO_c84c6752_6d64_48cc_9500_e54a3c34898d "https://en.wikipedia.org/wiki/Self-discharge"@en .

:electrochemistry_457a8f92_0a19_4773_8114_a42edff32248 a owl:Class ;
    rdfs:label "PlateGroup"@en ;
    rdfs:comment "assembly of plates of the same polarity electrically connected together"@en ;
    rdfs:subClassOf [ a owl:Restriction ;
            owl:onProperty emmo:EMMO_dba27ca1_33c9_4443_a912_1519ce4c39ec ;
            owl:someValuesFrom :electrochemistry_92147e31_d015_4889_a092_04fbab033f15 ],
        emmo:EMMO_52bbaaee_1145_4be3_8a5c_b366851ea1b9 ;
    skos:prefLabel "PlateGroup"@en ;
    emmo:EMMO_50c298c2_55a2_4068_b3ac_4e948c33181f "https://www.electropedia.org/iev/iev.nsf/display?openform&ievref=482-02-04" ;
    emmo:EMMO_967080e5_2f42_4eb2_a3a9_c58143e835f9 "assembly of plates of the same polarity electrically connected together"@en .

:electrochemistry_47346d85_b9be_4480_8993_6307b1c58fcd a owl:Class ;
    rdfs:label "LithiumBasedElectrode"@en ;
    rdfs:comment "an electrode in which the primary active material consists of lithium or lithium compounds"@en ;
    rdfs:subClassOf :electrochemistry_9a823d64_9d10_4a29_9cbd_9bbdad7985bc ;
    skos:prefLabel "LithiumBasedElectrode"@en ;
    emmo:EMMO_967080e5_2f42_4eb2_a3a9_c58143e835f9 "an electrode in which the primary active material consists of lithium or lithium compounds"@en .

:electrochemistry_49909cd1_44f4_41b4_877a_82a52845a5cb a owl:Class ;
    rdfs:label "Spacer"@en ;
    rdfs:comment "component of a cell made of insulating material intended to maintain the spacing between plates of opposite polarity or between the plate pack and the case"@en ;
    rdfs:subClassOf emmo:EMMO_f76884f7_964e_488e_9bb7_1b2453e9e817 ;
    skos:prefLabel "Spacer"@en ;
    emmo:EMMO_50c298c2_55a2_4068_b3ac_4e948c33181f "https://www.electropedia.org/iev/iev.nsf/display?openform&ievref=482-02-10" ;
    emmo:EMMO_967080e5_2f42_4eb2_a3a9_c58143e835f9 "component of a cell made of insulating material intended to maintain the spacing between plates of opposite polarity or between the plate pack and the case"@en .

:electrochemistry_4d6f7f50_b343_4bd6_8612_2b8521a99c9b a owl:Class ;
    rdfs:label "Electrocatalysis"@en ;
    rdfs:comment "increasing the rate of an electrode reaction by adding specific material to the electrode."@en ;
    rdfs:subClassOf [ a owl:Restriction ;
            owl:onProperty emmo:EMMO_ae2d1a96_bfa1_409a_a7d2_03d69e8a125a ;
            owl:someValuesFrom :electrochemistry_a3b53904_22b1_42a9_a515_c8a3aed7e841 ],
        :electrochemistry_19abaccd_43be_4048_965c_e4fb63c5951b ;
    skos:prefLabel "Electrocatalysis"@en ;
    emmo:EMMO_26bf1bef_d192_4da6_b0eb_d2209698fb54 "https://www.wikidata.org/wiki/Q100318565" ;
    emmo:EMMO_50c298c2_55a2_4068_b3ac_4e948c33181f "https://www.electropedia.org/iev/iev.nsf/display?openform&ievref=114-04-15" ;
    emmo:EMMO_967080e5_2f42_4eb2_a3a9_c58143e835f9 "increasing the rate of an electrode reaction by adding specific material to the electrode."@en .

:electrochemistry_4df9926d_d4f2_4955_93f3_a03c5edc5383 a owl:ObjectProperty ;
    rdfs:label "hasCoating"@en ;
    rdfs:comment "relates a component to a coating that covers its surface to provide protective, functional, or structural properties"@en ;
    rdfs:range :electrochemistry_09a7f560_9ddf_4c32_b067_b213eca5b0a1 ;
    rdfs:subPropertyOf emmo:EMMO_dba27ca1_33c9_4443_a912_1519ce4c39ec ;
    skos:prefLabel "hasCoating"@en ;
    emmo:EMMO_967080e5_2f42_4eb2_a3a9_c58143e835f9 "relates a component to a coating that covers its surface to provide protective, functional, or structural properties"@en .

:electrochemistry_4e02d727_07fe_41fd_886c_041317342086 a owl:Class ;
    rdfs:label "BinaryElectrolyte"@en ;
    rdfs:comment "an electrolyte consisting of anions and cations with equal absolute charge numbers."@en ;
    rdfs:subClassOf :electrochemistry_fb0d9eef_92af_4628_8814_e065ca255d59 ;
    skos:example "KCl (1:1), MgSO4 (2:2)" ;
    skos:prefLabel "BinaryElectrolyte"@en ;
    emmo:EMMO_967080e5_2f42_4eb2_a3a9_c58143e835f9 "an electrolyte consisting of anions and cations with equal absolute charge numbers."@en .

:electrochemistry_52547692_f773_4e3f_8c8b_1d9d39bc3c8c a owl:Class ;
    rdfs:label "GoldBasedElectrode"@en ;
    rdfs:comment "an electrode in which the primary active material consists of gold or gold compounds"@en ;
    rdfs:subClassOf :electrochemistry_9a823d64_9d10_4a29_9cbd_9bbdad7985bc ;
    skos:prefLabel "GoldBasedElectrode"@en ;
    emmo:EMMO_967080e5_2f42_4eb2_a3a9_c58143e835f9 "an electrode in which the primary active material consists of gold or gold compounds"@en .

:electrochemistry_54e0c2bd_1bb2_4f9c_9b55_5b6cc34651ec a owl:Class ;
    rdfs:label "Interphase"@en ;
    rdfs:comment "a spatial region at the interface between two bulk phases in contact, which is different chemically and physically from both phases in contact"@en ;
    rdfs:seeAlso "https://doi.org/10.1002/admi.202101865"@en ;
    rdfs:subClassOf :electrochemistry_f78e3c87_01c6_4cc2_b047_30322262e22d ;
    skos:altLabel "InterfacialLayer"@en,
        "InterfacialRegion"@en ;
    skos:example "SEI"@en ;
    skos:prefLabel "Interphase"@en ;
    emmo:EMMO_157fdf31_6387_42be_8e72_10530519214a "https://raw.githubusercontent.com/emmo-repo/domain-electrochemistry/dev/docs/assets/img/fig/png/Interphase.png" ;
    emmo:EMMO_967080e5_2f42_4eb2_a3a9_c58143e835f9 "a spatial region at the interface between two bulk phases in contact, which is different chemically and physically from both phases in contact"@en ;
    emmo:EMMO_fe015383_afb3_44a6_ae86_043628697aa2 "https://goldbook.iupac.org/terms/view/I03085" .

:electrochemistry_5641910f_6e69_4ce4_be84_4b1bf14b8916 a owl:Class ;
    rdfs:label "Electroosmosis"@en ;
    rdfs:comment "movement of a fluid through a diaphragm, produced by application of an electric field"@en ;
    rdfs:subClassOf :electrochemistry_19abaccd_43be_4048_965c_e4fb63c5951b ;
    skos:prefLabel "Electroosmosis"@en ;
    emmo:EMMO_26bf1bef_d192_4da6_b0eb_d2209698fb54 "https://www.wikidata.org/wiki/Q241065" ;
    emmo:EMMO_50c298c2_55a2_4068_b3ac_4e948c33181f "https://www.electropedia.org/iev/iev.nsf/display?openform&ievref=114-04-01"@en ;
    emmo:EMMO_967080e5_2f42_4eb2_a3a9_c58143e835f9 "movement of a fluid through a diaphragm, produced by application of an electric field"@en ;
    emmo:EMMO_c84c6752_6d64_48cc_9500_e54a3c34898d "https://en.wikipedia.org/wiki/Electro-osmosis"@en .

:electrochemistry_5cb5548f_f774_4668_ad02_f0742581f2f1 a owl:Class ;
    rdfs:label "Electrocapillarity"@en ;
    rdfs:comment "change of the mechanical stress at the surface separating two bodies due to the presence of electric charges at the interface"@en ;
    rdfs:subClassOf :electrochemistry_19abaccd_43be_4048_965c_e4fb63c5951b ;
    skos:prefLabel "Electrocapillarity"@en ;
    emmo:EMMO_26bf1bef_d192_4da6_b0eb_d2209698fb54 "https://www.wikidata.org/wiki/Q9252431"@en ;
    emmo:EMMO_50c298c2_55a2_4068_b3ac_4e948c33181f "https://www.electropedia.org/iev/iev.nsf/display?openform&ievref=114-04-02"@en ;
    emmo:EMMO_967080e5_2f42_4eb2_a3a9_c58143e835f9 "change of the mechanical stress at the surface separating two bodies due to the presence of electric charges at the interface"@en ;
    emmo:EMMO_c84c6752_6d64_48cc_9500_e54a3c34898d "https://en.wikipedia.org/wiki/Electrocapillarity"@en .

:electrochemistry_5e1136d3_df00_40f7_a4bc_8259341053a1 a owl:Class ;
    rdfs:label "IronBasedElectrode"@en ;
    rdfs:comment "an electrode which contains mostly materials based on iron"@en ;
    rdfs:subClassOf :electrochemistry_9a823d64_9d10_4a29_9cbd_9bbdad7985bc ;
    skos:prefLabel "IronBasedElectrode"@en ;
    emmo:EMMO_967080e5_2f42_4eb2_a3a9_c58143e835f9 "an electrode which contains mostly materials based on iron"@en ;
    emmo:EMMO_c7b62dd7_063a_4c2a_8504_42f7264ba83f "often represented in cell designations by the letter F"@en,
        "this class is intended to enable designations based on IEC recommendations"@en .

:electrochemistry_5eb197ea_0c3e_4ea2_8392_81152ee91515 a owl:ObjectProperty ;
    rdfs:label "hasReferenceElectrode"@en ;
    rdfs:comment "relates an electrochemical cell or measurement setup to the electrode that provides a stable reference potential"@en ;
    rdfs:range :electrochemistry_0f007072_a8dd_4798_b865_1bf9363be627 ;
    rdfs:subPropertyOf :electrochemistry_578c41e9_ee01_4840_9c8c_04ab6e4e6241 ;
    skos:prefLabel "hasReferenceElectrode"@en ;
    emmo:EMMO_967080e5_2f42_4eb2_a3a9_c58143e835f9 "relates an electrochemical cell or measurement setup to the electrode that provides a stable reference potential"@en .

:electrochemistry_60bc27f0_8290_4113_8c3b_011433a733c7 a owl:Class ;
    rdfs:label "TerminalProtector"@en ;
    rdfs:comment "cover of insulating material used to avoid electric contact with the cell or battery terminal"@en ;
    rdfs:subClassOf emmo:EMMO_f76884f7_964e_488e_9bb7_1b2453e9e817 ;
    skos:altLabel "TerminalCover"@en ;
    skos:prefLabel "TerminalProtector"@en ;
    emmo:EMMO_50c298c2_55a2_4068_b3ac_4e948c33181f "https://www.electropedia.org/iev/iev.nsf/display?openform&ievref=482-02-23" ;
    emmo:EMMO_967080e5_2f42_4eb2_a3a9_c58143e835f9 "cover of insulating material used to avoid electric contact with the cell or battery terminal"@en .

:electrochemistry_60c5b2e5_164a_4ce6_8409_f386f5e50c03 a owl:Class ;
    rdfs:label "FaradaysSecondLawOfElectrolysis"@en ;
    rdfs:comment "when the same electric charge (quantity of electricity) Q is passed through several electrolytes, the mass, m_i, of the substances deposited are proportional to their respective chemical equivalent molar mass, M_i/z_i."@en ;
    rdfs:subClassOf emmo:EMMO_9c32fd69_f480_4130_83b3_fb25d9face14 ;
    skos:prefLabel "FaradaysSecondLawOfElectrolysis"@en ;
    emmo:EMMO_967080e5_2f42_4eb2_a3a9_c58143e835f9 "when the same electric charge (quantity of electricity) Q is passed through several electrolytes, the mass, m_i, of the substances deposited are proportional to their respective chemical equivalent molar mass, M_i/z_i."@en ;
    emmo:EMMO_c7b62dd7_063a_4c2a_8504_42f7264ba83f "m_1/m_2 = (M_1/z_1) / (M_2/z_2)" ;
    emmo:EMMO_c84c6752_6d64_48cc_9500_e54a3c34898d "https://en.wikipedia.org/wiki/Faraday%27s_laws_of_electrolysis#Second_law"@en .

:electrochemistry_637c576e_a50e_47ae_8c74_2024ce4c6d0f a owl:Class ;
    rdfs:label "SaltBridge"@en ;
    rdfs:comment "means of making electrolytic connection between two half cells without introducing a significant liquid junction potential."@en ;
    rdfs:subClassOf :electrochemistry_b5ea31c9_bb10_4276_980e_c3eceb1efc82 ;
    skos:prefLabel "SaltBridge"@en ;
    emmo:EMMO_26bf1bef_d192_4da6_b0eb_d2209698fb54 "https://www.wikidata.org/wiki/Q899119" ;
    emmo:EMMO_6dd685dd_1895_46e4_b227_be9f7d643c25 "https://dbpedia.org/page/Salt_bridge"@en ;
    emmo:EMMO_967080e5_2f42_4eb2_a3a9_c58143e835f9 "means of making electrolytic connection between two half cells without introducing a significant liquid junction potential."@en ;
    emmo:EMMO_c7b62dd7_063a_4c2a_8504_42f7264ba83f "A typical construction is a tube of an inert material (e.g. agar agar) filled with a solution containing an electrolyte with approximately equal ion mobilities of the cation and the anion (e.g., KNO3, KCl), with the ends of the tube immersed in the electrolyte solution of the half cells."@en ;
    emmo:EMMO_c84c6752_6d64_48cc_9500_e54a3c34898d "https://en.wikipedia.org/wiki/Salt_bridge"@en .

:electrochemistry_63ea1c9b_0bda_4a69_9745_efb08e6be685 a owl:Class ;
    rdfs:label "ElectrochemicalMigration"@en ;
    rdfs:comment "transport of ions in an electrolyte due to an electric field"@en ;
    rdfs:subClassOf :electrochemistry_19abaccd_43be_4048_965c_e4fb63c5951b ;
    skos:prefLabel "ElectrochemicalMigration"@en ;
    emmo:EMMO_26bf1bef_d192_4da6_b0eb_d2209698fb54 "https://www.wikidata.org/wiki/Q30587730"@en ;
    emmo:EMMO_50c298c2_55a2_4068_b3ac_4e948c33181f "https://www.electropedia.org/iev/iev.nsf/display?openform&ievref=114-04-06"@en ;
    emmo:EMMO_967080e5_2f42_4eb2_a3a9_c58143e835f9 "transport of ions in an electrolyte due to an electric field"@en ;
    emmo:EMMO_c84c6752_6d64_48cc_9500_e54a3c34898d "https://en.wikipedia.org/wiki/Electrochemical_migration"@en .

:electrochemistry_6559c04d_75bc_41ea_8ed8_8d3c09dae6b0 a owl:Class ;
    rdfs:label "LidSealingCompound"@en ;
    rdfs:comment "material used to seal the cell lid to the case or to the terminals of a cell"@en ;
    rdfs:subClassOf emmo:EMMO_57d977ab_0036_4779_b59a_e47620afdb9c ;
    skos:prefLabel "LidSealingCompound"@en ;
    emmo:EMMO_50c298c2_55a2_4068_b3ac_4e948c33181f "https://www.electropedia.org/iev/iev.nsf/display?openform&ievref=482-02-16" ;
    emmo:EMMO_967080e5_2f42_4eb2_a3a9_c58143e835f9 "material used to seal the cell lid to the case or to the terminals of a cell"@en .

:electrochemistry_65c90d8d_9712_4f3f_b830_d8163ec4cfcc a owl:Class ;
    rdfs:label "SolidAmalgamElectrode"@en ;
    rdfs:comment "electrode made of a solid amalgam of an appropriate metal"@en ;
    rdfs:subClassOf [ a owl:Restriction ;
            owl:onProperty :electrochemistry_860aa941_5ff9_4452_8a16_7856fad07bee ;
            owl:someValuesFrom chems:substance_dc5fb846_1824_40f8_9834_81f118aa1c2d ],
        :electrochemistry_5adb91e0_ffe1_41f3_b779_c6966f65fb0e ;
    skos:altLabel "SAE"@en ;
    skos:prefLabel "SolidAmalgamElectrode"@en ;
    emmo:EMMO_967080e5_2f42_4eb2_a3a9_c58143e835f9 "electrode made of a solid amalgam of an appropriate metal"@en ;
    emmo:EMMO_c7b62dd7_063a_4c2a_8504_42f7264ba83f "Liquid and paste amalgams can also be used."@en,
        "Solid amalgam electrodes are electrochemically similar to the hanging mercury drop electrode. Their main advantages are high hydrogen overpotential (similar to liquid mercury); a wide working potential range; the simple mechanical, chemical, and electrochemical regeneration of the surface; a long lifetime; low toxicity of material (comparable with that of dental amalgams); applicability for field measurements; compatibility with flow-through systems; simple construction, without mobile parts; and easy miniaturization."@en .

:electrochemistry_68eb5e35_5bd8_47b1_9b7f_f67224fa291e a owl:Class ;
    rdfs:label "Binder"@en ;
    rdfs:comment "material or substance that holds or draws other materials together to form a cohesive whole"@en ;
    rdfs:subClassOf :electrochemistry_b5ea31c9_bb10_4276_980e_c3eceb1efc82 ;
    skos:altLabel "ElectrodeBinder"@en ;
    skos:example "CMC, PVDF"@en ;
    skos:prefLabel "Binder"@en ;
    emmo:EMMO_26bf1bef_d192_4da6_b0eb_d2209698fb54 "https://www.wikidata.org/wiki/Q863583" ;
    emmo:EMMO_967080e5_2f42_4eb2_a3a9_c58143e835f9 "material or substance that holds or draws other materials together to form a cohesive whole"@en ;
    emmo:EMMO_c84c6752_6d64_48cc_9500_e54a3c34898d "https://en.wikipedia.org/wiki/Binder_(material)"@en .

:electrochemistry_6b1f594f_2c0a_46a0_8805_d6ab08baa75e a owl:Class ;
    rdfs:label "TubularPlate"@en ;
    rdfs:comment "positive plate (electrode) which is either composed of an assembly of porous tube of perforated metal or tissue either a gauntlet with or without a central current collector spine, the active material being placed within the tubes"@en ;
    rdfs:subClassOf :electrochemistry_aff732a9_238a_4734_977c_b2ba202af126 ;
    skos:prefLabel "TubularPlate"@en ;
    emmo:EMMO_50c298c2_55a2_4068_b3ac_4e948c33181f "https://www.electropedia.org/iev/iev.nsf/display?openform&ievref=482-02-07" ;
    emmo:EMMO_967080e5_2f42_4eb2_a3a9_c58143e835f9 "positive plate (electrode) which is either composed of an assembly of porous tube of perforated metal or tissue either a gauntlet with or without a central current collector spine, the active material being placed within the tubes"@en .

:electrochemistry_6fec8cc1_4e6c_428e_8343_6cf3c286a185 a owl:Class ;
    rdfs:label "GoldElectrode"@en ;
    rdfs:comment "foil, wire or disc electrode made of gold which is easily fabricated into a variety of electrode geometries"@en ;
    rdfs:subClassOf [ a owl:Restriction ;
            owl:onProperty :electrochemistry_860aa941_5ff9_4452_8a16_7856fad07bee ;
            owl:someValuesFrom chems:substance_b3815a7f_f64a_48f6_b0ce_d0032578c699 ],
        :electrochemistry_52547692_f773_4e3f_8c8b_1d9d39bc3c8c ;
    skos:altLabel "AuElectrode"@en ;
    skos:prefLabel "GoldElectrode"@en ;
    emmo:EMMO_967080e5_2f42_4eb2_a3a9_c58143e835f9 "foil, wire or disc electrode made of gold which is easily fabricated into a variety of electrode geometries"@en ;
    emmo:EMMO_c7b62dd7_063a_4c2a_8504_42f7264ba83f "At positive potentials, Au forms an oxide and/or chemisorbed oxygen layer, while in the presence of complexing anions, such as chloride or cyanide, it readily undergoes oxidation and dissolution, limiting its working potential range and its applications."@en .

:electrochemistry_76df6e7b_fc3b_4a1f_98b1_0ca9c0539e4c a owl:Class ;
    rdfs:label "OutputCable"@en ;
    rdfs:comment "cable used for the electrical connection of the battery terminals and the load and/or the charger"@en ;
    rdfs:subClassOf emmo:EMMO_f76884f7_964e_488e_9bb7_1b2453e9e817 ;
    skos:prefLabel "OutputCable"@en ;
    emmo:EMMO_50c298c2_55a2_4068_b3ac_4e948c33181f "https://www.electropedia.org/iev/iev.nsf/display?openform&ievref=482-02-36"@en ;
    emmo:EMMO_967080e5_2f42_4eb2_a3a9_c58143e835f9 "cable used for the electrical connection of the battery terminals and the load and/or the charger"@en .

:electrochemistry_7760b241_775f_4be1_b827_59f9bde9e5b2 a owl:Class ;
    rdfs:label "PhotoelectrolyticCell"@en ;
    rdfs:comment "electrolytic cell in which a chemical reaction is influenced by the absorption of light"@en ;
    rdfs:subClassOf :electrochemistry_e931087f_7681_4096_b200_5223bcc47eb4 ;
    skos:prefLabel "PhotoelectrolyticCell"@en ;
    emmo:EMMO_50c298c2_55a2_4068_b3ac_4e948c33181f "https://www.electropedia.org/iev/iev.nsf/display?openform&ievref=114-04-19"@en ;
    emmo:EMMO_967080e5_2f42_4eb2_a3a9_c58143e835f9 "electrolytic cell in which a chemical reaction is influenced by the absorption of light"@en .

:electrochemistry_7f4d74cd_d0a5_4908_9da9_7629fe419917 a owl:Class ;
    rdfs:label "RotatingRingDiskElectrode"@en ;
    rdfs:comment "a second annular working electrode positioned concentric with a rotating disc electrode to make a rotating ring-disc electrode (RRDE)"@en ;
    rdfs:subClassOf [ a owl:Restriction ;
            owl:onProperty emmo:EMMO_dba27ca1_33c9_4443_a912_1519ce4c39ec ;
            owl:someValuesFrom :electrochemistry_3a77b5e7_9646_4154_bf8f_5f798989e5f3 ],
        :electrochemistry_6c421175_477f_45e0_8b6c_c3464f5351c5 ;
    skos:altLabel "RRDE"@en ;
    skos:prefLabel "RotatingRingDiskElectrode"@en ;
    emmo:EMMO_26bf1bef_d192_4da6_b0eb_d2209698fb54 "https://www.wikidata.org/wiki/Q5829908"@en ;
    emmo:EMMO_967080e5_2f42_4eb2_a3a9_c58143e835f9 "a second annular working electrode positioned concentric with a rotating disc electrode to make a rotating ring-disc electrode (RRDE)"@en ;
    emmo:EMMO_c7b62dd7_063a_4c2a_8504_42f7264ba83f "This arrangement is largely used in mechanistic studies."@en ;
    emmo:EMMO_c84c6752_6d64_48cc_9500_e54a3c34898d "https://en.wikipedia.org/wiki/Rotating_ring-disk_electrode"@en .

:electrochemistry_81833d8a_b03d_4250_be84_6385415beb01 a owl:Class ;
    rdfs:label "ActiveMaterialMix"@en ;
    rdfs:comment "blend containing a material which reacts chemically to produce electrical energy with other constituents and additives"@en ;
    rdfs:subClassOf [ a owl:Restriction ;
            owl:onProperty emmo:EMMO_dba27ca1_33c9_4443_a912_1519ce4c39ec ;
            owl:someValuesFrom :electrochemistry_79d1b273_58cd_4be6_a250_434817f7c261 ],
        :electrochemistry_b5ea31c9_bb10_4276_980e_c3eceb1efc82 ;
    skos:prefLabel "ActiveMaterialMix"@en ;
    emmo:EMMO_50c298c2_55a2_4068_b3ac_4e948c33181f "https://www.electropedia.org/iev/iev.nsf/display?openform&ievref=482-02-34" ;
    emmo:EMMO_967080e5_2f42_4eb2_a3a9_c58143e835f9 "blend containing a material which reacts chemically to produce electrical energy with other constituents and additives"@en .

:electrochemistry_83d2c2d4_ffa9_42f4_9264_a0c59c657607 a owl:Class ;
    rdfs:label "PolarityReversal"@en ;
    rdfs:comment "reversing of the polarities of the electrodes of a cell, generally due to over-discharge of a low-capacity cell in a series arrangement"@en ;
    rdfs:subClassOf emmo:EMMO_bafc17b5_9be4_4823_8bbe_ab4e90b6738c ;
    skos:altLabel "CellReversal"@en ;
    skos:prefLabel "PolarityReversal"@en ;
    emmo:EMMO_50c298c2_55a2_4068_b3ac_4e948c33181f "https://www.electropedia.org/iev/iev.nsf/display?openform&ievref=482-03-03"@en ;
    emmo:EMMO_967080e5_2f42_4eb2_a3a9_c58143e835f9 "reversing of the polarities of the electrodes of a cell, generally due to over-discharge of a low-capacity cell in a series arrangement"@en .

:electrochemistry_86be0987_5e21_43ec_b975_8f679999d328 a owl:Class ;
    rdfs:label "BimetallicElectrode"@en ;
    rdfs:comment "electrode containing two different metals (e.g. platinum and ruthenium) on its surface (e.g. to modify its electrocatalytic properties)"@en ;
    rdfs:subClassOf :electrochemistry_5186239a_2af7_4dbf_92ca_22e8e583c528,
        :electrochemistry_5adb91e0_ffe1_41f3_b779_c6966f65fb0e ;
    skos:prefLabel "BimetallicElectrode"@en ;
    emmo:EMMO_967080e5_2f42_4eb2_a3a9_c58143e835f9 "electrode containing two different metals (e.g. platinum and ruthenium) on its surface (e.g. to modify its electrocatalytic properties)"@en .

:electrochemistry_88d2d4bc_4244_4419_a260_ad099a62d580 a owl:Class ;
    rdfs:label "SulfurBasedElectrode"@en ;
    rdfs:comment "an electrode in which the primary active material consists of sulfur or sulfur compounds"@en ;
    rdfs:subClassOf :electrochemistry_9a823d64_9d10_4a29_9cbd_9bbdad7985bc ;
    skos:prefLabel "SulfurBasedElectrode"@en ;
    emmo:EMMO_967080e5_2f42_4eb2_a3a9_c58143e835f9 "an electrode in which the primary active material consists of sulfur or sulfur compounds"@en .

:electrochemistry_8a5083b0_cd23_4f8c_99e8_b9ccd6f9f3a2 a owl:Class ;
    rdfs:label "ConcentrationCell"@en ;
    rdfs:comment "electrochemical cell that has two half-cells separated by a wall permeable to ions, both containing the same electrolyte differing only in their ion concentrations"@en ;
    rdfs:subClassOf :electrochemistry_0acd0fc2_1048_4604_8e90_bf4e84bd87df ;
    skos:prefLabel "ConcentrationCell"@en ;
    emmo:EMMO_157fdf31_6387_42be_8e72_10530519214a "https://raw.githubusercontent.com/emmo-repo/domain-electrochemistry/dev/docs/assets/img/fig/png/ConcentrationCell.png" ;
    emmo:EMMO_26bf1bef_d192_4da6_b0eb_d2209698fb54 "https://www.wikidata.org/wiki/Q903563" ;
    emmo:EMMO_50c298c2_55a2_4068_b3ac_4e948c33181f "https://www.electropedia.org/iev/iev.nsf/display?openform&ievref=114-03-08"@en ;
    emmo:EMMO_967080e5_2f42_4eb2_a3a9_c58143e835f9 "electrochemical cell that has two half-cells separated by a wall permeable to ions, both containing the same electrolyte differing only in their ion concentrations"@en ;
    emmo:EMMO_c7b62dd7_063a_4c2a_8504_42f7264ba83f "a concentration cell produces a voltage as it attempts to reach equilibrium, which will occur when the concentration in both cells is equal."@en ;
    emmo:EMMO_c84c6752_6d64_48cc_9500_e54a3c34898d "https://en.wikipedia.org/wiki/Concentration_cell"@en .

:electrochemistry_8ab1e656_38ff_48e6_ab09_293d76bc9044 a owl:Class ;
    rdfs:label "Catalyst"@en ;
    rdfs:comment "substance that increases chemical reaction speed, and which is conserved after the reaction"@en ;
    rdfs:subClassOf emmo:EMMO_2480b72b_db8d_460f_9a5f_c2912f979046 ;
    skos:prefLabel "Catalyst"@en ;
    emmo:EMMO_26bf1bef_d192_4da6_b0eb_d2209698fb54 "https://www.wikidata.org/wiki/Q12385831" ;
    emmo:EMMO_967080e5_2f42_4eb2_a3a9_c58143e835f9 "substance that increases chemical reaction speed, and which is conserved after the reaction"@en .

:electrochemistry_8c71739c_27c1_4d19_a0ff_02545296af43 a owl:Class ;
    rdfs:label "SeriesConnection"@en ;
    rdfs:comment "arrangement of cells or batteries wherein the positive terminal of each cell or battery is connected to the negative terminal of the next cell or battery in sequence."@en ;
    rdfs:subClassOf emmo:EMMO_52bbaaee_1145_4be3_8a5c_b366851ea1b9 ;
    skos:prefLabel "SeriesConnection"@en ;
    emmo:EMMO_50c298c2_55a2_4068_b3ac_4e948c33181f "https://www.electropedia.org/iev/iev.nsf/display?openform&ievref=482-03-41" ;
    emmo:EMMO_967080e5_2f42_4eb2_a3a9_c58143e835f9 "arrangement of cells or batteries wherein the positive terminal of each cell or battery is connected to the negative terminal of the next cell or battery in sequence."@en .

:electrochemistry_900d95fb_863d_4142_a96d_369fb39e2639 a owl:Class ;
    rdfs:label "ElectrolyticCapacitor"@en ;
    rdfs:comment "capacitor consisting of a metallic plate as first conductor, a very thin oxide film formed on the metal as the dielectric and an electrolyte as second conductor"@en ;
    rdfs:subClassOf :electrochemistry_0acd0fc2_1048_4604_8e90_bf4e84bd87df ;
    skos:prefLabel "ElectrolyticCapacitor"@en ;
    emmo:EMMO_26bf1bef_d192_4da6_b0eb_d2209698fb54 "https://www.wikidata.org/wiki/Q1326992" ;
    emmo:EMMO_50c298c2_55a2_4068_b3ac_4e948c33181f "https://www.electropedia.org/iev/iev.nsf/display?openform&ievref=114-03-04"@en ;
    emmo:EMMO_967080e5_2f42_4eb2_a3a9_c58143e835f9 "capacitor consisting of a metallic plate as first conductor, a very thin oxide film formed on the metal as the dielectric and an electrolyte as second conductor"@en ;
    emmo:EMMO_c84c6752_6d64_48cc_9500_e54a3c34898d "https://en.wikipedia.org/wiki/Electrolytic_capacitor"@en .

:electrochemistry_9317be62_e602_4343_a72d_02c87201b9f6 a owl:ObjectProperty ;
    rdfs:label "hasSeparator"@en ;
    rdfs:comment "relates a system to a separator that physically divides electrodes while allowing ionic transport"@en ;
    rdfs:range emmo:EMMO_38b579de_4331_40e0_803d_09efa298e726 ;
    rdfs:subPropertyOf emmo:EMMO_3c7f239f_e833_4a2b_98a1_c88831770c1b ;
    skos:prefLabel "hasSeparator"@en ;
    emmo:EMMO_967080e5_2f42_4eb2_a3a9_c58143e835f9 "relates a system to a separator that physically divides electrodes while allowing ionic transport"@en .

:electrochemistry_94d9d5e2_9e9b_4eb7_b3ce_f3d658b7ae64 a owl:Class ;
    rdfs:label "Interface"@en ;
    rdfs:comment "the plane ideally marking the boundary between two phases"@en ;
    rdfs:seeAlso "https://doi.org/10.1002/admi.202101865"@en ;
    rdfs:subClassOf emmo:EMMO_fcae603e_aa6e_4940_9fa1_9f0909cabf3b ;
    skos:prefLabel "Interface"@en ;
    emmo:EMMO_157fdf31_6387_42be_8e72_10530519214a "https://raw.githubusercontent.com/emmo-repo/domain-electrochemistry/dev/docs/assets/img/fig/png/Interface.png" ;
    emmo:EMMO_26bf1bef_d192_4da6_b0eb_d2209698fb54 "https://www.wikidata.org/wiki/Q901882" ;
    emmo:EMMO_967080e5_2f42_4eb2_a3a9_c58143e835f9 "the plane ideally marking the boundary between two phases"@en ;
    emmo:EMMO_c84c6752_6d64_48cc_9500_e54a3c34898d "https://en.wikipedia.org/wiki/Interface_(matter)" ;
    emmo:EMMO_fe015383_afb3_44a6_ae86_043628697aa2 "https://doi.org/10.1351/goldbook.I03082" .

:electrochemistry_95e4aa95_b7e9_40d7_b78e_4d7dcc31093d a owl:Class ;
    rdfs:label "FlowCell"@en ;
    rdfs:comment "an electrochemical device in which the active materials are flowed through the cell from an external source"@en ;
    rdfs:subClassOf :electrochemistry_0acd0fc2_1048_4604_8e90_bf4e84bd87df ;
    skos:altLabel "ElectrochemicalFlowCell"@en ;
    skos:prefLabel "FlowCell"@en ;
    emmo:EMMO_967080e5_2f42_4eb2_a3a9_c58143e835f9 "an electrochemical device in which the active materials are flowed through the cell from an external source"@en .

:electrochemistry_96309fa9_e157_48fe_9fda_41003860a3c0 a owl:Class ;
    rdfs:label "Electrochemiluminescence"@en ;
    rdfs:comment "chemiluminescence produced in electrode reactions"@en ;
    rdfs:subClassOf :electrochemistry_19abaccd_43be_4048_965c_e4fb63c5951b ;
    skos:altLabel "ECL"@en,
        "ElectrogeneratedChemiluminescence"@en ;
    skos:prefLabel "Electrochemiluminescence"@en ;
    emmo:EMMO_26bf1bef_d192_4da6_b0eb_d2209698fb54 "https://www.wikidata.org/wiki/Q755961" ;
    emmo:EMMO_50c298c2_55a2_4068_b3ac_4e948c33181f "https://www.electropedia.org/iev/iev.nsf/display?openform&ievref=114-04-18"@en ;
    emmo:EMMO_967080e5_2f42_4eb2_a3a9_c58143e835f9 "chemiluminescence produced in electrode reactions"@en ;
    emmo:EMMO_c84c6752_6d64_48cc_9500_e54a3c34898d "https://en.wikipedia.org/wiki/Electrochemiluminescence"@en .

:electrochemistry_9c73aff8_1c82_4116_a6be_78e21982b69d a owl:Class ;
    rdfs:label "ElectrodeElectrolyteInterface"@en ;
    rdfs:comment "interface between an electrolyte and an electrode where an electrode reaction takes place."@en ;
    rdfs:subClassOf :electrochemistry_50044b99_b858_433b_a32d_23d1e1cf88b2 ;
    skos:altLabel "ActiveSurfaceOfAnElectrode"@en ;
    skos:prefLabel "ElectrodeElectrolyteInterface"@en ;
    emmo:EMMO_50c298c2_55a2_4068_b3ac_4e948c33181f "https://www.electropedia.org/iev/iev.nsf/display?openform&ievref=114-02-05"@en,
        "https://www.electropedia.org/iev/iev.nsf/display?openform&ievref=482-02-26"@en ;
    emmo:EMMO_967080e5_2f42_4eb2_a3a9_c58143e835f9 "interface between an electrolyte and an electrode where an electrode reaction takes place."@en .

:electrochemistry_a462859d_d8bd_48ea_8bde_1576f1248a1e a owl:Class ;
    rdfs:label "SilverElectrode"@en ;
    rdfs:comment "electrode in the form of foil, mesh, wire, rod, tube, powder, pellets, or single crystal of silver"@en ;
    rdfs:subClassOf [ a owl:Restriction ;
            owl:onProperty :electrochemistry_860aa941_5ff9_4452_8a16_7856fad07bee ;
            owl:someValuesFrom chems:substance_e1e6ff98_0725_4d27_ab21_2ca5a95371f0 ],
        :electrochemistry_f897db90_afd6_42e7_8d1f_0fcba856e45a ;
    skos:altLabel "AgElectrode"@en ;
    skos:prefLabel "SilverElectrode"@en ;
    emmo:EMMO_26bf1bef_d192_4da6_b0eb_d2209698fb54 "https://www.wikidata.org/wiki/Q20851418" ;
    emmo:EMMO_967080e5_2f42_4eb2_a3a9_c58143e835f9 "electrode in the form of foil, mesh, wire, rod, tube, powder, pellets, or single crystal of silver"@en ;
    emmo:EMMO_c7b62dd7_063a_4c2a_8504_42f7264ba83f "Ag electrodes were first used in potentiometry for the determination of Cl, Br, I, as well as for Ag+ ions, to which they are sensitive."@en .

:electrochemistry_a8bfac4f_3f30_4e6d_8d8e_34b1eeecb614 a owl:Class ;
    rdfs:label "RoundElectrode"@en ;
    rdfs:comment "an electrode in the shape of a circle"@en ;
    rdfs:subClassOf :electrochemistry_0f007072_a8dd_4798_b865_1bf9363be627 ;
    skos:prefLabel "RoundElectrode"@en ;
    emmo:EMMO_967080e5_2f42_4eb2_a3a9_c58143e835f9 "an electrode in the shape of a circle"@en .

:electrochemistry_b3b3868f_6edd_4ce8_a984_08f9cf391f90 a owl:Class ;
    rdfs:label "Dissociation"@en ;
    rdfs:comment "process where molecules split up into ions due to being dissolved"@en ;
    rdfs:subClassOf :electrochemistry_8a1c9a7b_978c_4421_a9c1_d0b07b42aab9 ;
    skos:prefLabel "Dissociation"@en ;
    emmo:EMMO_26bf1bef_d192_4da6_b0eb_d2209698fb54 "https://www.wikidata.org/wiki/Q189673" ;
    emmo:EMMO_50c298c2_55a2_4068_b3ac_4e948c33181f "https://www.electropedia.org/iev/iev.nsf/display?openform&ievref=114-01-08" ;
    emmo:EMMO_967080e5_2f42_4eb2_a3a9_c58143e835f9 "process where molecules split up into ions due to being dissolved"@en ;
    emmo:EMMO_c84c6752_6d64_48cc_9500_e54a3c34898d "https://en.wikipedia.org/wiki/Dissociation_(chemistry)"@en .

:electrochemistry_b76a778f_253f_4210_a67f_fb6444d0de26 a owl:Class ;
    rdfs:label "DroppingMercuryElectrode"@en ;
    rdfs:comment "mercury electrode formed by sequence of mercury drops falling from a small aperture"@en ;
    rdfs:subClassOf :electrochemistry_df78745e_f9db_4830_88f0_8ce074fcb8ff ;
    skos:altLabel "DME"@en ;
    skos:prefLabel "DroppingMercuryElectrode"@en ;
    emmo:EMMO_26bf1bef_d192_4da6_b0eb_d2209698fb54 "https://www.wikidata.org/wiki/Q962292" ;
    emmo:EMMO_967080e5_2f42_4eb2_a3a9_c58143e835f9 "mercury electrode formed by sequence of mercury drops falling from a small aperture"@en ;
    emmo:EMMO_c7b62dd7_063a_4c2a_8504_42f7264ba83f "Other kinds of mercury drop electrodes are the static mercury drop electrode (SMDE), in which a drop is held at constant radius before being mechanically knocked off, and the hanging mercury drop elec- trode (HMDE), in which the whole experiment is performed on a single drop of mercury."@en,
        "The DME was introduced by Jaroslav Heyrovsk (1890  1967). A drop is renewed every few seconds. Many metals amalgamate with mercury so that in the analysis of metal ions in aqueous solution the DME maintains a fresh surface throughout."@en ;
    emmo:EMMO_c84c6752_6d64_48cc_9500_e54a3c34898d "https://en.wikipedia.org/wiki/Dropping_mercury_electrode"@en .

:electrochemistry_b91180e7_97ae_49e2_bf82_5bf720e7fa66 a owl:Class ;
    rdfs:label "ElectrochemicalDoubleLayerCapacitor"@en ;
    rdfs:comment "Device that stores electrical energy using a double layer in an electrochemical cell."@en ;
    rdfs:subClassOf :electrochemistry_dc6abae7_39b0_4d22_b52e_14d088a4bd5f ;
    skos:altLabel "DoubleLayerCapacitor"@en,
        "EDLC"@en,
        "ElectrochemicalCapacitor"@en ;
    skos:prefLabel "ElectrochemicalDoubleLayerCapacitor"@en ;
    emmo:EMMO_967080e5_2f42_4eb2_a3a9_c58143e835f9 "Device that stores electrical energy using a double layer in an electrochemical cell."@en ;
    emmo:EMMO_c7b62dd7_063a_4c2a_8504_42f7264ba83f "stores energy electrostatically in the Helmholtz Layer"@en .

:electrochemistry_b9bece97_a511_4cb9_88a2_b5bd5c5e5d74 a owl:Class ;
    rdfs:label "ThreeElectrodeElectrochemicalCell"@en ;
    rdfs:comment "electrochemical cell with a working electrode, reference electrode, and auxiliary electrode"@en ;
    rdfs:subClassOf :electrochemistry_6f2c88c9_5c04_4953_a298_032cc3ab9b77 ;
    skos:prefLabel "ThreeElectrodeElectrochemicalCell"@en ;
    skos:scopeNote "The working electrode is the site of interest where the electrochemical process occurs, the reference electrode provides a stable potential, and the auxiliary (counter) electrode completes the circuit."@en ;
    emmo:EMMO_5f7abc2a_5b50_41c3_8def_c8ba7c3b083e "A potentiostat can be used to maintain a potential difference between the working and reference electrodes."@en ;
    emmo:EMMO_967080e5_2f42_4eb2_a3a9_c58143e835f9 "electrochemical cell with a working electrode, reference electrode, and auxiliary electrode"@en ;
    emmo:EMMO_c7b62dd7_063a_4c2a_8504_42f7264ba83f "Electric current flows between the working and auxiliary electrodes. Electrode potential may be measured between the working and reference electrodes."@en .

:electrochemistry_bbc77932_643b_4603_a4e8_970ef06a76ad a owl:Class ;
    rdfs:label "EdgeInsulator"@en ;
    rdfs:comment "part which insures insulation between the plate (electrode) edges and adjacent plates (electrodes) and the container side walls"@en ;
    rdfs:subClassOf :electrochemistry_b5ea31c9_bb10_4276_980e_c3eceb1efc82 ;
    skos:prefLabel "EdgeInsulator"@en ;
    emmo:EMMO_50c298c2_55a2_4068_b3ac_4e948c33181f "https://www.electropedia.org/iev/iev.nsf/display?openform&ievref=482-02-19"@en ;
    emmo:EMMO_967080e5_2f42_4eb2_a3a9_c58143e835f9 "part which insures insulation between the plate (electrode) edges and adjacent plates (electrodes) and the container side walls"@en .

:electrochemistry_bed5b5f9_b89d_45e3_a8c2_81b70ae21847 a owl:Class ;
    rdfs:label "SeriesParallelConnection"@en ;
    rdfs:comment "arrangement of cells or batteries wherein in series connected cells or batteries are connected in parallel."@en ;
    rdfs:subClassOf emmo:EMMO_52bbaaee_1145_4be3_8a5c_b366851ea1b9 ;
    skos:prefLabel "SeriesParallelConnection"@en ;
    emmo:EMMO_50c298c2_55a2_4068_b3ac_4e948c33181f "https://www.electropedia.org/iev/iev.nsf/display?openform&ievref=482-03-42" ;
    emmo:EMMO_967080e5_2f42_4eb2_a3a9_c58143e835f9 "arrangement of cells or batteries wherein in series connected cells or batteries are connected in parallel."@en .

:electrochemistry_c05692eb_ae92_4e03_b355_f259f9089cb8 a owl:Class ;
    rdfs:label "ElectrolyteLevelIndicator"@en ;
    rdfs:comment "device used to assist in the measurement of the level of electrolyte in a cell"@en ;
    rdfs:subClassOf emmo:EMMO_494b372c_cfdf_47d3_a4de_5e037c540de8 ;
    skos:prefLabel "ElectrolyteLevelIndicator"@en ;
    emmo:EMMO_50c298c2_55a2_4068_b3ac_4e948c33181f "https://www.electropedia.org/iev/iev.nsf/display?openform&ievref=482-05-52" ;
    emmo:EMMO_967080e5_2f42_4eb2_a3a9_c58143e835f9 "device used to assist in the measurement of the level of electrolyte in a cell"@en .

:electrochemistry_c14ae9b3_e4ba_4129_a7b6_afd2d4571de6 a owl:Class ;
    rdfs:label "HermeticallySealedCell"@en ;
    rdfs:comment "permanently sealed gas tight cell without pressure release device"@en ;
    rdfs:subClassOf :electrochemistry_0acd0fc2_1048_4604_8e90_bf4e84bd87df ;
    skos:prefLabel "HermeticallySealedCell"@en ;
    emmo:EMMO_50c298c2_55a2_4068_b3ac_4e948c33181f "https://www.electropedia.org/iev/iev.nsf/display?openform&ievref=482-02-01" ;
    emmo:EMMO_967080e5_2f42_4eb2_a3a9_c58143e835f9 "permanently sealed gas tight cell without pressure release device"@en .

:electrochemistry_c2024587_3237_474e_8df9_91d10db2df47 a owl:Class ;
    rdfs:label "PolarizableElectrode"@en ;
    rdfs:comment "electrode whose potential changes with an applied potential"@en ;
    rdfs:subClassOf :electrochemistry_0f007072_a8dd_4798_b865_1bf9363be627 ;
    skos:prefLabel "PolarizableElectrode"@en ;
    emmo:EMMO_967080e5_2f42_4eb2_a3a9_c58143e835f9 "electrode whose potential changes with an applied potential"@en .

:electrochemistry_c3f4b34a_0e2c_46f3_baab_4ebd2682d26f a owl:Class ;
    rdfs:label "IonicLiquidElectrolyte"@en ;
    rdfs:comment "An ionic liquid is an electrolyte composed of a salt that is liquid below 100 C. Ionic liquids have found uses in electrochemical analysis, because their unconventional properties include a negligible vapor pressure, a high thermal and electrochemical stability, and exceptional dissolution properties for both organic and inorganic chemical species."@en ;
    rdfs:subClassOf :electrochemistry_5f9a9411_05f9_4576_acd3_81d7d41cfe98 ;
    skos:altLabel "IonicLiquid"@en ;
    skos:prefLabel "IonicLiquidElectrolyte"@en ;
    emmo:EMMO_6dd685dd_1895_46e4_b227_be9f7d643c25 "https://dbpedia.org/page/Ionic_liquid"@en ;
    emmo:EMMO_967080e5_2f42_4eb2_a3a9_c58143e835f9 "An ionic liquid is an electrolyte composed of a salt that is liquid below 100 C. Ionic liquids have found uses in electrochemical analysis, because their unconventional properties include a negligible vapor pressure, a high thermal and electrochemical stability, and exceptional dissolution properties for both organic and inorganic chemical species."@en ;
    emmo:EMMO_c84c6752_6d64_48cc_9500_e54a3c34898d "https://en.wikipedia.org/wiki/Ionic_liquid"@en .

:electrochemistry_c4a778c7_33da_4e1a_960e_402a210bfeff a owl:Class ;
    rdfs:label "HydrogenElectrode"@en ;
    rdfs:comment "platinized platinum electrode saturated by a stream of pure gaseous hydrogen"@en ;
    rdfs:subClassOf :electrochemistry_a0a619d7_da95_41f0_8bc3_9c19d636d543 ;
    skos:prefLabel "HydrogenElectrode"@en ;
    emmo:EMMO_50c298c2_55a2_4068_b3ac_4e948c33181f "https://www.electropedia.org/iev/iev.nsf/display?openform&ievref=114-03-16"@en ;
    emmo:EMMO_967080e5_2f42_4eb2_a3a9_c58143e835f9 "platinized platinum electrode saturated by a stream of pure gaseous hydrogen"@en ;
    emmo:EMMO_c7b62dd7_063a_4c2a_8504_42f7264ba83f "A platinized platinum electrode consists of a platinum rod covered by compact platinum powder called platinum black."@en .

:electrochemistry_c55ec02c_b727_4df1_97ce_91d7bb5d5e91 a owl:Class ;
    rdfs:label "Leakage"@en ;
    rdfs:comment "unplanned escape of electrolyte, gas or other material from a cell or battery"@en ;
    rdfs:subClassOf :electrochemistry_19abaccd_43be_4048_965c_e4fb63c5951b ;
    skos:prefLabel "Leakage"@en ;
    emmo:EMMO_50c298c2_55a2_4068_b3ac_4e948c33181f "https://www.electropedia.org/iev/iev.nsf/display?openform&ievref=482-02-32" ;
    emmo:EMMO_967080e5_2f42_4eb2_a3a9_c58143e835f9 "unplanned escape of electrolyte, gas or other material from a cell or battery"@en .

:electrochemistry_c76dbfeb_f3d9_44d4_9cbe_0946924f311f a owl:ObjectProperty ;
    rdfs:label "hasWorkingElectrode"@en ;
    rdfs:comment "relates an electrochemical cell or measurement setup to the electrode at which the primary reaction of interest occurs"@en ;
    rdfs:range :electrochemistry_0f007072_a8dd_4798_b865_1bf9363be627 ;
    rdfs:subPropertyOf :electrochemistry_578c41e9_ee01_4840_9c8c_04ab6e4e6241 ;
    skos:prefLabel "hasWorkingElectrode"@en ;
    emmo:EMMO_967080e5_2f42_4eb2_a3a9_c58143e835f9 "relates an electrochemical cell or measurement setup to the electrode at which the primary reaction of interest occurs"@en .

:electrochemistry_c936bfbe_7a0c_4185_a317_db1ce2c3c38c a owl:Class ;
    rdfs:label "CathodicProtection"@en ;
    rdfs:comment "electrochemical immunity produced by an appropriate cathodic polarization."@en ;
    rdfs:subClassOf emmo:EMMO_bafc17b5_9be4_4823_8bbe_ab4e90b6738c,
        :electrochemistry_4bc38e99_1978_4143_a766_fbb57f2cf46e ;
    skos:prefLabel "CathodicProtection"@en ;
    emmo:EMMO_26bf1bef_d192_4da6_b0eb_d2209698fb54 "https://www.wikidata.org/wiki/Q15152527" ;
    emmo:EMMO_50c298c2_55a2_4068_b3ac_4e948c33181f "https://www.electropedia.org/iev/iev.nsf/display?openform&ievref=114-04-05" ;
    emmo:EMMO_967080e5_2f42_4eb2_a3a9_c58143e835f9 "electrochemical immunity produced by an appropriate cathodic polarization."@en ;
    emmo:EMMO_c84c6752_6d64_48cc_9500_e54a3c34898d "https://en.wikipedia.org/wiki/Cathodic_protection"@en .

:electrochemistry_cc1f854a_ba6c_436e_bd18_c8b9159bbf52 a owl:Class ;
    rdfs:label "VentCap"@en ;
    rdfs:comment "component fitted into the filling hole of a cell with a provision of allowing the venting of electrolysis gas from the cell"@en ;
    rdfs:subClassOf emmo:EMMO_f76884f7_964e_488e_9bb7_1b2453e9e817 ;
    skos:prefLabel "VentCap"@en ;
    emmo:EMMO_50c298c2_55a2_4068_b3ac_4e948c33181f "https://www.electropedia.org/iev/iev.nsf/display?openform&ievref=482-05-23" ;
    emmo:EMMO_967080e5_2f42_4eb2_a3a9_c58143e835f9 "component fitted into the filling hole of a cell with a provision of allowing the venting of electrolysis gas from the cell"@en .

:electrochemistry_cc8c2c5d_cf3d_444d_a7e8_44ec4c06a88e a owl:ObjectProperty ;
    rdfs:label "hasCurrentCollector"@en ;
    rdfs:range emmo:EMMO_38b579de_4331_40e0_803d_09efa298e726 ;
    rdfs:subPropertyOf emmo:EMMO_3c7f239f_e833_4a2b_98a1_c88831770c1b ;
    skos:prefLabel "hasCurrentCollector"@en .

:electrochemistry_d0a26dc2_fde9_4a11_ac26_7c18499d28a5 a owl:Class ;
    rdfs:label "ZincBasedElectrode"@en ;
    rdfs:comment "an electrode in which the primary active material consists of zinc or zinc compounds"@en ;
    rdfs:subClassOf :electrochemistry_9a823d64_9d10_4a29_9cbd_9bbdad7985bc ;
    skos:prefLabel "ZincBasedElectrode"@en ;
    emmo:EMMO_967080e5_2f42_4eb2_a3a9_c58143e835f9 "an electrode in which the primary active material consists of zinc or zinc compounds"@en .

:electrochemistry_d5da9948_e95b_4f12_a2d2_10a48f390c52 a owl:Class ;
    rdfs:label "ParallelSeriesConnection"@en ;
    rdfs:comment "arrangement of cells or batteries wherein parallel connected cells or batteries are connected in series."@en ;
    rdfs:subClassOf emmo:EMMO_52bbaaee_1145_4be3_8a5c_b366851ea1b9 ;
    skos:prefLabel "ParallelSeriesConnection"@en ;
    emmo:EMMO_50c298c2_55a2_4068_b3ac_4e948c33181f "https://www.electropedia.org/iev/iev.nsf/display?openform&ievref=482-03-40" ;
    emmo:EMMO_967080e5_2f42_4eb2_a3a9_c58143e835f9 "arrangement of cells or batteries wherein parallel connected cells or batteries are connected in series."@en .

:electrochemistry_d8a9a88e_d437_4fef_bc3c_65a1fe627061 a owl:Class ;
    rdfs:label "PlatinumBasedElectrode"@en ;
    rdfs:comment "an electrode in which the primary active material consists of platinum or platinum compounds"@en ;
    rdfs:subClassOf :electrochemistry_9a823d64_9d10_4a29_9cbd_9bbdad7985bc ;
    skos:prefLabel "PlatinumBasedElectrode"@en ;
    emmo:EMMO_967080e5_2f42_4eb2_a3a9_c58143e835f9 "an electrode in which the primary active material consists of platinum or platinum compounds"@en .

:electrochemistry_d907805f_678b_4ab6_8b56_59631684f84b a owl:Class ;
    rdfs:label "ElectrodePair"@en ;
    rdfs:comment "assembly of one positive plate, one negative plate and the associated separator if any"@en ;
    rdfs:subClassOf emmo:EMMO_52bbaaee_1145_4be3_8a5c_b366851ea1b9 ;
    skos:altLabel "PlatePair"@en ;
    skos:prefLabel "ElectrodePair"@en ;
    emmo:EMMO_50c298c2_55a2_4068_b3ac_4e948c33181f "https://www.electropedia.org/iev/iev.nsf/display?openform&ievref=482-02-09" ;
    emmo:EMMO_967080e5_2f42_4eb2_a3a9_c58143e835f9 "assembly of one positive plate, one negative plate and the associated separator if any"@en .

:electrochemistry_e08d43cf_93e4_49c6_bcb6_472be52ae7fc a owl:ObjectProperty ;
    rdfs:label "hasCounterElectrode"@en ;
    rdfs:comment "relates an electrochemical cell or setup to the electrode that completes the electrical circuit and serves as a reference or counter to the working electrode"@en ;
    rdfs:range :electrochemistry_0f007072_a8dd_4798_b865_1bf9363be627 ;
    rdfs:subPropertyOf :electrochemistry_578c41e9_ee01_4840_9c8c_04ab6e4e6241 ;
    skos:prefLabel "hasCounterElectrode"@en ;
    emmo:EMMO_967080e5_2f42_4eb2_a3a9_c58143e835f9 "relates an electrochemical cell or setup to the electrode that completes the electrical circuit and serves as a reference or counter to the working electrode"@en .

:electrochemistry_e2a1dae1_05e4_4bd1_a39d_0eb10db482bc a owl:Class ;
    rdfs:label "Electrolysis"@en ;
    rdfs:comment "method of separating and neutralizing ions by an electric current in an electrolytic cell"@en ;
    rdfs:subClassOf :electrochemistry_19abaccd_43be_4048_965c_e4fb63c5951b ;
    skos:prefLabel "Electrolysis"@en ;
    emmo:EMMO_26bf1bef_d192_4da6_b0eb_d2209698fb54 "https://www.wikidata.org/wiki/Q64403" ;
    emmo:EMMO_50c298c2_55a2_4068_b3ac_4e948c33181f "https://www.electropedia.org/iev/iev.nsf/display?openform&ievref=114-04-09" ;
    emmo:EMMO_6dd685dd_1895_46e4_b227_be9f7d643c25 "https://dbpedia.org/page/Electrolysis"@en ;
    emmo:EMMO_705f27ae_954c_4f13_98aa_18473fc52b25 "From Greek elektron (electric) + lysis (loosening, dissolution): decomposition by electricity. Part of Faradays systematic terminology built to avoid theoretical commitments. Coined by Michael Faraday with support from William Whewell and Whitlock Nicholl."@en ;
    emmo:EMMO_967080e5_2f42_4eb2_a3a9_c58143e835f9 "method of separating and neutralizing ions by an electric current in an electrolytic cell"@en ;
    emmo:EMMO_c84c6752_6d64_48cc_9500_e54a3c34898d "https://en.wikipedia.org/wiki/Electrolysis"@en .

:electrochemistry_e94f6d42_35e4_4f9f_bb74_5e0628bbd454 a owl:Class ;
    rdfs:label "MonoblocContainer"@en ;
    rdfs:comment "case with multiple separate cell compartments"@en ;
    rdfs:subClassOf :electrochemistry_43cd6e14_dd43_41b5_b5b4_344d53841603 ;
    skos:prefLabel "MonoblocContainer"@en ;
    emmo:EMMO_50c298c2_55a2_4068_b3ac_4e948c33181f "https://www.electropedia.org/iev/iev.nsf/display?openform&ievref=482-02-18"@en ;
    emmo:EMMO_967080e5_2f42_4eb2_a3a9_c58143e835f9 "case with multiple separate cell compartments"@en .

:electrochemistry_eac15067_9594_4eab_a440_b537b0fd2075 a owl:DatatypeProperty ;
    rdfs:label "hasANSICode"@en ;
    skos:prefLabel "hasANSICode"@en .

:electrochemistry_ec1dce8b_bb46_41a9_b532_6bed381aa557 a owl:Class ;
    rdfs:label "VentedCell"@en ;
    rdfs:comment "secondary cell having a cover provided with an opening through which products of electrolysis and evaporation are allowed to escape freely from the cell to the atmosphere"@en ;
    rdfs:subClassOf :electrochemistry_0acd0fc2_1048_4604_8e90_bf4e84bd87df ;
    skos:prefLabel "VentedCell"@en ;
    emmo:EMMO_50c298c2_55a2_4068_b3ac_4e948c33181f "https://www.electropedia.org/iev/iev.nsf/display?openform&ievref=482-05-14" ;
    emmo:EMMO_967080e5_2f42_4eb2_a3a9_c58143e835f9 "secondary cell having a cover provided with an opening through which products of electrolysis and evaporation are allowed to escape freely from the cell to the atmosphere"@en .

:electrochemistry_ec6f3d6f_bdf5_418f_9314_3ef2ff528103 a owl:Class ;
    rdfs:label "CarbonInkElectrode"@en ;
    rdfs:comment "development of a carbon paste electrode that is screen printed using a carbon/polymer mixture of suitable composition"@en ;
    rdfs:subClassOf :electrochemistry_b0a0dddb_d942_4af2_b6a7_d7165f4253f1 ;
    skos:prefLabel "CarbonInkElectrode"@en ;
    emmo:EMMO_26bf1bef_d192_4da6_b0eb_d2209698fb54 "https://www.wikidata.org/wiki/Q120907443" ;
    emmo:EMMO_967080e5_2f42_4eb2_a3a9_c58143e835f9 "development of a carbon paste electrode that is screen printed using a carbon/polymer mixture of suitable composition"@en ;
    emmo:EMMO_c7b62dd7_063a_4c2a_8504_42f7264ba83f "These electrodes can easily be chemically modified by the incorporation of reagents (electrocatalysts, redox mediators, complexation agents, enzymes, etc.) and by the attachment of micro- or nanoparticles to prepare electrochemical sensors for analytical applications."@en,
        "Typical composition of a carbon ink expressed as mass fractions is graphite powder 60 % and polystyrene 40 %."@en .

:electrochemistry_ecf136cb_2584_4cb1_98b7_2d2b3d22e40d a owl:Class ;
    rdfs:label "SolidElectrolyteInterphase"@en ;
    rdfs:comment "an interfacial layer that forms between an electrode phase and and electrolyte phase, due to the decomposition of the electrolyte"@en ;
    rdfs:subClassOf :electrochemistry_d16eec87_c646_4566_bda6_7d3357cda061 ;
    owl:deprecated true ;
    skos:altLabel "SEI"@en ;
    skos:prefLabel "SolidElectrolyteInterphase"@en ;
    emmo:EMMO_967080e5_2f42_4eb2_a3a9_c58143e835f9 "an interfacial layer that forms between an electrode phase and and electrolyte phase, due to the decomposition of the electrolyte"@en ;
    emmo:EMMO_c7b62dd7_063a_4c2a_8504_42f7264ba83f "although the definition could apply to any electrode, it is conventionally used to describe interfacial layers that form on the anode of an electrochemical cell."@en .

:electrochemistry_efc4f7ab_850d_443c_a17f_184983021f96 a owl:Class ;
    rdfs:label "ParallelConnection"@en ;
    rdfs:comment "arrangement of cells or batteries wherein all the positive terminals and all the negative terminals, respectively, are connected together."@en ;
    rdfs:subClassOf emmo:EMMO_52bbaaee_1145_4be3_8a5c_b366851ea1b9 ;
    skos:prefLabel "ParallelConnection"@en ;
    emmo:EMMO_26bf1bef_d192_4da6_b0eb_d2209698fb54 "https://www.wikidata.org/wiki/Q302489" ;
    emmo:EMMO_50c298c2_55a2_4068_b3ac_4e948c33181f "https://www.electropedia.org/iev/iev.nsf/display?openform&ievref=482-03-39" ;
    emmo:EMMO_967080e5_2f42_4eb2_a3a9_c58143e835f9 "arrangement of cells or batteries wherein all the positive terminals and all the negative terminals, respectively, are connected together."@en .

:electrochemistry_f330680b_347e_45b3_9113_5ce09d18d60b a owl:Class ;
    rdfs:label "PressureReliefVent"@en ;
    rdfs:comment "vent of special design which allows to release gas from a cell in order to avoid excessive internal pressure and thereby to preclude rupture or explosion of the cell container"@en ;
    rdfs:subClassOf emmo:EMMO_f76884f7_964e_488e_9bb7_1b2453e9e817 ;
    skos:prefLabel "PressureReliefVent"@en ;
    emmo:EMMO_50c298c2_55a2_4068_b3ac_4e948c33181f "https://www.electropedia.org/iev/iev.nsf/display?openform&ievref=482-02-41" ;
    emmo:EMMO_967080e5_2f42_4eb2_a3a9_c58143e835f9 "vent of special design which allows to release gas from a cell in order to avoid excessive internal pressure and thereby to preclude rupture or explosion of the cell container"@en .

:electrochemistry_f6fcd255_248d_4603_b128_04dab960a676 a owl:Class ;
    rdfs:label "IndicatorElectrode"@en ;
    rdfs:comment "electrode that responds to one, or more than one, species in the solution being investigated, with no appreciable change of bulk solution composition during the measurement"@en ;
    rdfs:subClassOf :electrochemistry_0f007072_a8dd_4798_b865_1bf9363be627 ;
    skos:prefLabel "IndicatorElectrode"@en ;
    emmo:EMMO_26bf1bef_d192_4da6_b0eb_d2209698fb54 "https://www.wikidata.org/wiki/Q120907462" ;
    emmo:EMMO_967080e5_2f42_4eb2_a3a9_c58143e835f9 "electrode that responds to one, or more than one, species in the solution being investigated, with no appreciable change of bulk solution composition during the measurement"@en ;
    emmo:EMMO_c7b62dd7_063a_4c2a_8504_42f7264ba83f "If processes of interest occur both at the anode and the cathode of a cell (as in differential amperometry or controlled-current potentiometric titration with two indicator electrodes), the cell should be said to comprise two indicator or working electrodes."@en,
        "This term is typically used in potentiometry."@en ;
    emmo:EMMO_fe015383_afb3_44a6_ae86_043628697aa2 "https://goldbook.iupac.org/terms/view/I03006"@en .

:electrochemistry_f897db90_afd6_42e7_8d1f_0fcba856e45a a owl:Class ;
    rdfs:label "SilverBasedElectrode"@en ;
    rdfs:comment "an electrode in which the primary active material consists of silver or silver compounds"@en ;
    rdfs:subClassOf :electrochemistry_9a823d64_9d10_4a29_9cbd_9bbdad7985bc ;
    skos:prefLabel "SilverBasedElectrode"@en ;
    emmo:EMMO_967080e5_2f42_4eb2_a3a9_c58143e835f9 "an electrode in which the primary active material consists of silver or silver compounds"@en .

:electrochemistry_fd1fae29_a182_4692_98b8_919764b07b00 a owl:ObjectProperty ;
    rdfs:label "hasInsertedEntity"@en ;
    rdfs:domain :electrochemistry_757eae08_4d43_42d4_8b4e_8a0bfd2f9a1c ;
    rdfs:range emmo:EMMO_21205421_5783_4d3e_81e5_10c5d894a88a ;
    rdfs:subPropertyOf emmo:EMMO_dba27ca1_33c9_4443_a912_1519ce4c39ec ;
    skos:prefLabel "hasInsertedEntity"@en .

:electrochemistry_04f28ce3_251d_429e_aa85_ab3eb45bbcd2 a owl:Class ;
    rdfs:label "ThermalRunaway"@en ;
    rdfs:comment "unstable condition arising during constant voltage charge in which the rate of heat dissipation capability, causing a continuous temperature increase with resulting further charge current increase, which can lead to the destruction of the battery"@en ;
    rdfs:subClassOf :electrochemistry_19abaccd_43be_4048_965c_e4fb63c5951b ;
    skos:prefLabel "ThermalRunaway"@en ;
    emmo:EMMO_50c298c2_55a2_4068_b3ac_4e948c33181f "https://www.electropedia.org/iev/iev.nsf/display?openform&ievref=482-05-54" ;
    emmo:EMMO_967080e5_2f42_4eb2_a3a9_c58143e835f9 "unstable condition arising during constant voltage charge in which the rate of heat dissipation capability, causing a continuous temperature increase with resulting further charge current increase, which can lead to the destruction of the battery"@en ;
    emmo:EMMO_c7b62dd7_063a_4c2a_8504_42f7264ba83f "in lithium batteries thermal runaway may cause melting of lithium"@en .

:electrochemistry_056a5fab_3d99_46bd_8eb1_6e89a368e1a7 a owl:ObjectProperty ;
    rdfs:label "hasBinder"@en ;
    rdfs:comment "relates a composite material or coating to a binder that provides mechanical cohesion and adhesion between its constituents"@en ;
    rdfs:range emmo:EMMO_bc37743c_37c4_4ec7_9d58_d1aae5567352 ;
    rdfs:subPropertyOf emmo:EMMO_3c7f239f_e833_4a2b_98a1_c88831770c1b ;
    skos:prefLabel "hasBinder"@en ;
    emmo:EMMO_967080e5_2f42_4eb2_a3a9_c58143e835f9 "relates a composite material or coating to a binder that provides mechanical cohesion and adhesion between its constituents"@en .

:electrochemistry_09a7f560_9ddf_4c32_b067_b213eca5b0a1 a owl:Class ;
    rdfs:label "Coating"@en ;
    rdfs:comment "a covering on the surface of an object"@en ;
    rdfs:subClassOf [ a owl:Restriction ;
            owl:onProperty emmo:EMMO_e1097637_70d2_4895_973f_2396f04fa204 ;
            owl:someValuesFrom emmo:EMMO_3a6578ac_aee0_43b9_9bc6_1eb208c8c9a9 ],
        [ a owl:Restriction ;
            owl:onProperty emmo:EMMO_e1097637_70d2_4895_973f_2396f04fa204 ;
            owl:someValuesFrom emmo:EMMO_43003c86_9d15_433b_9789_ee2940920656 ],
        :electrochemistry_b5ea31c9_bb10_4276_980e_c3eceb1efc82 ;
    skos:prefLabel "Coating"@en ;
    emmo:EMMO_26bf1bef_d192_4da6_b0eb_d2209698fb54 "https://www.wikidata.org/wiki/Q1570182" ;
    emmo:EMMO_967080e5_2f42_4eb2_a3a9_c58143e835f9 "a covering on the surface of an object"@en ;
    emmo:EMMO_c84c6752_6d64_48cc_9500_e54a3c34898d "https://en.wikipedia.org/wiki/Coating"@en .

:electrochemistry_0a0de817_addc_46a5_8ba2_255d48cdf366 a owl:Class ;
    rdfs:label "ElectrochemicalDegradationPhenomenon"@en ;
    rdfs:comment "A phenomenon that causes an electrochemical device to deviate from its ideal behaviour."@en ;
    rdfs:subClassOf [ a owl:Restriction ;
            owl:onProperty emmo:EMMO_35c29eb6_f57e_48d8_85af_854f9e926e77 ;
            owl:someValuesFrom :electrochemistry_0acd0fc2_1048_4604_8e90_bf4e84bd87df ],
        :electrochemistry_19abaccd_43be_4048_965c_e4fb63c5951b ;
    skos:prefLabel "ElectrochemicalDegradationPhenomenon"@en ;
    emmo:EMMO_967080e5_2f42_4eb2_a3a9_c58143e835f9 "A phenomenon that causes an electrochemical device to deviate from its ideal behaviour."@en .

:electrochemistry_109a38d4_daaa_4748_a803_044fb7c97673 a owl:Class ;
    rdfs:label "Reduction"@en ;
    rdfs:comment "chemical reaction in which oxygen is removed from an oxide, implying a transfer of electrons from the oxygen atoms, or, more generally, in which a substance gains electrons"@en ;
    rdfs:subClassOf :electrochemistry_2d366f85_a644_4b3e_a641_fce81e72d158 ;
    skos:altLabel "ReductionReaction"@en ;
    skos:note "Electrons are generally transferred from another substance by an oxidation reaction."@en ;
    skos:prefLabel "Reduction"@en ;
    skos:related :electrochemistry_c6a35be8_7ce2_415b_be9e_3a5ff9a7f2ad ;
    emmo:EMMO_50c298c2_55a2_4068_b3ac_4e948c33181f "https://www.electropedia.org/iev/iev.nsf/display?openform&ievref=113-02-16" ;
    emmo:EMMO_967080e5_2f42_4eb2_a3a9_c58143e835f9 "chemical reaction in which oxygen is removed from an oxide, implying a transfer of electrons from the oxygen atoms, or, more generally, in which a substance gains electrons"@en ;
    emmo:EMMO_fe015383_afb3_44a6_ae86_043628697aa2 "https://goldbook.iupac.org/terms/view/R05222"@en .

:electrochemistry_15b852b5_19cc_49ab_849f_7df6175fb2be a owl:Class ;
    rdfs:label "Catholyte"@en ;
    rdfs:comment "electrolyte on the cathode side of an electrochemical cell that is divided into compartments."@en ;
    rdfs:subClassOf :electrochemistry_fb0d9eef_92af_4628_8814_e065ca255d59 ;
    skos:prefLabel "Catholyte"@en ;
    skos:related :electrochemistry_35c650ab_3b23_4938_b312_1b0dede2e6d5 ;
    emmo:EMMO_50c298c2_55a2_4068_b3ac_4e948c33181f "https://www.electropedia.org/iev/iev.nsf/display?openform&ievref=114-03-18"@en ;
    emmo:EMMO_705f27ae_954c_4f13_98aa_18473fc52b25 "From Greek kathodos ('way down') + lyts (, looser)"@en ;
    emmo:EMMO_967080e5_2f42_4eb2_a3a9_c58143e835f9 "electrolyte on the cathode side of an electrochemical cell that is divided into compartments."@en ;
    emmo:EMMO_c7b62dd7_063a_4c2a_8504_42f7264ba83f "Electrolyte solution in the cathodic compartment of an electrolysis cell or galvanic cell, i.e., in that part of the cell where the cathode is placed."@en .

:electrochemistry_212af058_3bbb_419f_a9c6_90ba9ebb3706 a owl:Class ;
    rdfs:label "CurrentCollector"@en ;
    rdfs:comment "A good electron conductor support designed to transfer electrons from the external circuit to the active materials of the cell."@en ;
    rdfs:subClassOf :electrochemistry_b5ea31c9_bb10_4276_980e_c3eceb1efc82 ;
    skos:altLabel "ElectrodeCurrentCollector"@en ;
    skos:example "Copper foil, Aluminum foil"@en ;
    skos:prefLabel "CurrentCollector"@en ;
    emmo:EMMO_26bf1bef_d192_4da6_b0eb_d2209698fb54 "https://www.wikidata.org/wiki/Q120907411" ;
    emmo:EMMO_50c298c2_55a2_4068_b3ac_4e948c33181f "https://www.electropedia.org/iev/iev.nsf/display?openform&ievref=485-06-07" ;
    emmo:EMMO_967080e5_2f42_4eb2_a3a9_c58143e835f9 "A good electron conductor support designed to transfer electrons from the external circuit to the active materials of the cell."@en .

:electrochemistry_328c6e36_3706_4d92_abae_432fa3adb2a0 a owl:Class ;
    rdfs:label "CellBaffle"@en ;
    rdfs:comment "internal component used to reduce the amount of electrolyte loss due to electrolyte spray being carried in the gas and/or by electrolyte movement"@en ;
    rdfs:subClassOf emmo:EMMO_f76884f7_964e_488e_9bb7_1b2453e9e817 ;
    skos:prefLabel "CellBaffle"@en ;
    emmo:EMMO_50c298c2_55a2_4068_b3ac_4e948c33181f "https://www.electropedia.org/iev/iev.nsf/display?openform&ievref=482-05-13" ;
    emmo:EMMO_967080e5_2f42_4eb2_a3a9_c58143e835f9 "internal component used to reduce the amount of electrolyte loss due to electrolyte spray being carried in the gas and/or by electrolyte movement"@en ;
    emmo:EMMO_c7b62dd7_063a_4c2a_8504_42f7264ba83f "a cell baffle has a second function in protecting the plate pack from damage by objects inserted through the filling hole"@en .

:electrochemistry_3663991d_9319_4f7a_922b_f0e428b58801 a owl:Class ;
    rdfs:label "PorousElectrode"@en ;
    rdfs:comment "porous electrodes consist of porous matrices of a single reactive electronic conductor or a mixture of solids that include essentially non-conducting, reactive materials in addition to electronic conductors. An electrolytic solution fills the void spaces of the porous matrix."@en ;
    rdfs:subClassOf [ a owl:Restriction ;
            owl:onProperty emmo:EMMO_e1097637_70d2_4895_973f_2396f04fa204 ;
            owl:someValuesFrom emmo:EMMO_3a6578ac_aee0_43b9_9bc6_1eb208c8c9a9 ],
        :electrochemistry_0f007072_a8dd_4798_b865_1bf9363be627 ;
    skos:prefLabel "PorousElectrode"@en ;
    emmo:EMMO_967080e5_2f42_4eb2_a3a9_c58143e835f9 "porous electrodes consist of porous matrices of a single reactive electronic conductor or a mixture of solids that include essentially non-conducting, reactive materials in addition to electronic conductors. An electrolytic solution fills the void spaces of the porous matrix."@en .

:electrochemistry_3f6c9e09_5f23_41cc_9f85_7de365cef089 a owl:Class ;
    rdfs:label "ElectrolyteCreep"@en ;
    rdfs:comment "gradual and slow spreading of an electrolyte film on the external surface of a cell or battery"@en ;
    rdfs:subClassOf :electrochemistry_19abaccd_43be_4048_965c_e4fb63c5951b ;
    skos:prefLabel "ElectrolyteCreep"@en ;
    emmo:EMMO_50c298c2_55a2_4068_b3ac_4e948c33181f "https://www.electropedia.org/iev/iev.nsf/display?openform&ievref=482-02-30" ;
    emmo:EMMO_967080e5_2f42_4eb2_a3a9_c58143e835f9 "gradual and slow spreading of an electrolyte film on the external surface of a cell or battery"@en ;
    emmo:EMMO_c7b62dd7_063a_4c2a_8504_42f7264ba83f "electrolyte creep is sometimes indicated by the presence of a visible solid deposit or wet spots"@en .

:electrochemistry_4288b145_ba79_4989_92f8_86086679b0fe a owl:Class ;
    rdfs:label "GasEvolution"@en ;
    rdfs:comment "process through which a gas is evolved"@en ;
    rdfs:subClassOf :electrochemistry_8a1c9a7b_978c_4421_a9c1_d0b07b42aab9 ;
    skos:altLabel "Gassing"@en ;
    skos:prefLabel "GasEvolution"@en ;
    skos:related :electrochemistry_0c9017b4_6efd_4e2b_8e24_48b60ebe9315 ;
    emmo:EMMO_26bf1bef_d192_4da6_b0eb_d2209698fb54 "https://www.wikidata.org/wiki/Q5526337" ;
    emmo:EMMO_967080e5_2f42_4eb2_a3a9_c58143e835f9 "process through which a gas is evolved"@en ;
    emmo:EMMO_c84c6752_6d64_48cc_9500_e54a3c34898d "https://en.wikipedia.org/wiki/Gas_evolution_reaction"@en .

:electrochemistry_4bc38e99_1978_4143_a766_fbb57f2cf46e a owl:Class ;
    rdfs:label "ElectrochemicalImmunity"@en ;
    rdfs:comment "situation in which a material in a given environment undergoes negligible electrochemical corrosion."@en ;
    rdfs:subClassOf :electrochemistry_19abaccd_43be_4048_965c_e4fb63c5951b ;
    skos:example "cathodic protection"@en ;
    skos:prefLabel "ElectrochemicalImmunity"@en ;
    emmo:EMMO_50c298c2_55a2_4068_b3ac_4e948c33181f "https://www.electropedia.org/iev/iev.nsf/display?openform&ievref=114-04-03" ;
    emmo:EMMO_967080e5_2f42_4eb2_a3a9_c58143e835f9 "situation in which a material in a given environment undergoes negligible electrochemical corrosion."@en .

:electrochemistry_4df84ec1_8a1a_4770_963f_bf48009bd043 a owl:Class ;
    rdfs:label "Electrodissolution"@en ;
    rdfs:comment "the electrochemical dissolution of a material to soluble species"@en ;
    rdfs:subClassOf :electrochemistry_49263a32_eca6_4644_8144_0d3b14c26d0a,
        :electrochemistry_a0580fa9_5073_44af_b33e_7adbc83892d0 ;
    skos:example "Dissolution of metallic copper as Zn^{2+} during corrosion or anodization."@en ;
    skos:note "It can be regarded as the reversal of electrodeposition."@en ;
    skos:prefLabel "Electrodissolution"@en ;
    skos:related :electrochemistry_f0c24970_4c14_4207_bd78_5f2181a67085 ;
    emmo:EMMO_967080e5_2f42_4eb2_a3a9_c58143e835f9 "the electrochemical dissolution of a material to soluble species"@en .

:electrochemistry_522f0c0b_cf33_4328_af71_12e38dae6798 a owl:Class ;
    rdfs:label "PositiveTerminal"@en ;
    rdfs:comment "accessible conductive part provided for the connection of an external electric circuit to the positive electrode of the cell"@en ;
    rdfs:subClassOf [ a owl:Restriction ;
            owl:onProperty emmo:EMMO_8785be5a_2493_4b12_8f39_31907ab11748 ;
            owl:someValuesFrom :electrochemistry_aff732a9_238a_4734_977c_b2ba202af126 ],
        :electrochemistry_3f70e5c5_67f0_483e_998b_b83b7739c4bc ;
    skos:prefLabel "PositiveTerminal"@en ;
    emmo:EMMO_50c298c2_55a2_4068_b3ac_4e948c33181f "https://www.electropedia.org/iev/iev.nsf/display?openform&ievref=482-02-25" ;
    emmo:EMMO_967080e5_2f42_4eb2_a3a9_c58143e835f9 "accessible conductive part provided for the connection of an external electric circuit to the positive electrode of the cell"@en .

:electrochemistry_5d299271_3f68_494f_ab96_3db9acdd3138 a owl:ObjectProperty ;
    rdfs:label "hasNegativeElectrode"@en ;
    rdfs:comment "relates an electrochemical cell to the electrode at which oxidation occurs during discharge"@en ;
    rdfs:range :electrochemistry_0f007072_a8dd_4798_b865_1bf9363be627 ;
    rdfs:subPropertyOf :electrochemistry_578c41e9_ee01_4840_9c8c_04ab6e4e6241 ;
    skos:prefLabel "hasNegativeElectrode"@en ;
    emmo:EMMO_967080e5_2f42_4eb2_a3a9_c58143e835f9 "relates an electrochemical cell to the electrode at which oxidation occurs during discharge"@en .

:electrochemistry_609b340f_3450_4a10_95c2_c457e3eb8a89 a owl:Class ;
    rdfs:label "LiquidElectrolyte"@en ;
    rdfs:comment "an electrolyte in the liquid phase."@en ;
    rdfs:subClassOf [ a owl:Restriction ;
            owl:onProperty emmo:EMMO_e1097637_70d2_4895_973f_2396f04fa204 ;
            owl:someValuesFrom emmo:EMMO_908da3d5_775e_425e_af96_33914618eb66 ],
        :electrochemistry_fb0d9eef_92af_4628_8814_e065ca255d59 ;
    skos:prefLabel "LiquidElectrolyte"@en ;
    emmo:EMMO_967080e5_2f42_4eb2_a3a9_c58143e835f9 "an electrolyte in the liquid phase."@en .

:electrochemistry_6592d8cc_4ce4_42ca_b010_6bfc4a8444d2 a owl:Class ;
    rdfs:label "AcidicElectrolyte"@en ;
    rdfs:comment "an aqueous electrolyte with a nominal pH values less than 7"@en ;
    rdfs:subClassOf :electrochemistry_b812e9d0_7c58_4455_b3e7_6847f10c8e8a ;
    skos:altLabel "AcidicAqueousElectrolyte"@en,
        "AcidicSolution"@en ;
    skos:example "HCl-H2O"@en ;
    skos:prefLabel "AcidicElectrolyte"@en ;
    emmo:EMMO_967080e5_2f42_4eb2_a3a9_c58143e835f9 "an aqueous electrolyte with a nominal pH values less than 7"@en ;
    emmo:EMMO_c7b62dd7_063a_4c2a_8504_42f7264ba83f "typical alkaline electrolytes have a pH in the range 0 < x < 4"@en .

:electrochemistry_6c421175_477f_45e0_8b6c_c3464f5351c5 a owl:Class ;
    rdfs:label "RotatingDiskElectrode"@en ;
    rdfs:comment "A disc electrode that is embedded in the centre of a cylinder which rotates in solution around the longitudinal cylinder axis."@en ;
    rdfs:subClassOf :electrochemistry_a8bfac4f_3f30_4e6d_8d8e_34b1eeecb614 ;
    skos:altLabel "RDE"@en ;
    skos:prefLabel "RotatingDiskElectrode"@en ;
    emmo:EMMO_26bf1bef_d192_4da6_b0eb_d2209698fb54 "https://www.wikidata.org/wiki/Q3587619" ;
    emmo:EMMO_967080e5_2f42_4eb2_a3a9_c58143e835f9 "A disc electrode that is embedded in the centre of a cylinder which rotates in solution around the longitudinal cylinder axis."@en ;
    emmo:EMMO_c7b62dd7_063a_4c2a_8504_42f7264ba83f "The current is directly proportional to the electrode area and the electrode is uniformly accessible."@en,
        "The limiting current is given by the Levich equation."@en ;
    emmo:EMMO_c84c6752_6d64_48cc_9500_e54a3c34898d "https://en.wikipedia.org/wiki/Rotating_disk_electrode"@en .

:electrochemistry_7df82c48_b599_4b02_bef0_9facc9c39410 a owl:ObjectProperty ;
    rdfs:label "hasAdditive"@en ;
    rdfs:comment "relates a component or mixture to an additive that is included in minor quantity to modify physical, chemical, or electrochemical properties"@en ;
    rdfs:range emmo:EMMO_bc37743c_37c4_4ec7_9d58_d1aae5567352 ;
    rdfs:subPropertyOf emmo:EMMO_3c7f239f_e833_4a2b_98a1_c88831770c1b ;
    skos:prefLabel "hasAdditive"@en ;
    emmo:EMMO_967080e5_2f42_4eb2_a3a9_c58143e835f9 "relates a component or mixture to an additive that is included in minor quantity to modify physical, chemical, or electrochemical properties"@en .

:electrochemistry_865a40fc_2187_4549_a7e1_37aa2458448f a owl:Class ;
    rdfs:label "Anolyte"@en ;
    rdfs:comment "electrolyte on the anode side of an electrochemical cell that is divided into compartments"@en ;
    rdfs:subClassOf :electrochemistry_fb0d9eef_92af_4628_8814_e065ca255d59 ;
    skos:prefLabel "Anolyte"@en ;
    skos:related :electrochemistry_b6319c74_d2ce_48c0_a75a_63156776b302 ;
    emmo:EMMO_50c298c2_55a2_4068_b3ac_4e948c33181f "https://www.electropedia.org/iev/iev.nsf/display?openform&ievref=114-03-19" ;
    emmo:EMMO_705f27ae_954c_4f13_98aa_18473fc52b25 "From Greek anodos ('way up') + lyts (, looser)"@en ;
    emmo:EMMO_967080e5_2f42_4eb2_a3a9_c58143e835f9 "electrolyte on the anode side of an electrochemical cell that is divided into compartments"@en ;
    emmo:EMMO_c7b62dd7_063a_4c2a_8504_42f7264ba83f "Electrolyte solution in the anodic compartment of an electrolysis cell or galvanic cell, i.e., in that part of the cell where the anode is placed."@en .

:electrochemistry_872b11e1_8bb3_4a2a_af90_bbaa0055d01e a owl:Class ;
    rdfs:label "Spring"@en ;
    rdfs:comment "an elastic device"@en ;
    rdfs:subClassOf emmo:EMMO_f76884f7_964e_488e_9bb7_1b2453e9e817 ;
    skos:prefLabel "Spring"@en ;
    emmo:EMMO_26bf1bef_d192_4da6_b0eb_d2209698fb54 "https://www.wikidata.org/wiki/Q102836" ;
    emmo:EMMO_967080e5_2f42_4eb2_a3a9_c58143e835f9 "an elastic device"@en ;
    emmo:EMMO_c84c6752_6d64_48cc_9500_e54a3c34898d "https://en.wikipedia.org/wiki/Spring_(device)"@en .

:electrochemistry_8d3bf304_78e4_4e99_abe1_6ab429e44ed1 a owl:Class ;
    rdfs:label "SealedCell"@en ;
    rdfs:comment "cell which remains closed and does not release either gas or liquid when operated within the limits specified by the manufacturer"@en ;
    rdfs:subClassOf :electrochemistry_0acd0fc2_1048_4604_8e90_bf4e84bd87df ;
    skos:prefLabel "SealedCell"@en ;
    emmo:EMMO_50c298c2_55a2_4068_b3ac_4e948c33181f "https://www.electropedia.org/iev/iev.nsf/display?openform&ievref=482-05-17"@en ;
    emmo:EMMO_967080e5_2f42_4eb2_a3a9_c58143e835f9 "cell which remains closed and does not release either gas or liquid when operated within the limits specified by the manufacturer"@en ;
    emmo:EMMO_c7b62dd7_063a_4c2a_8504_42f7264ba83f "a sealed cell may be equipped with a safety device to prevent a dangerously high internal pressure and is designed to operate during its life in its original sealed state"@en .

:electrochemistry_8e9cf965_9f92_46e8_b678_b50410ce3616 a owl:ObjectProperty ;
    rdfs:label "hasPositiveElectrode"@en ;
    rdfs:comment "relates an electrochemical cell to the electrode at which reduction occurs during discharge"@en ;
    rdfs:range :electrochemistry_0f007072_a8dd_4798_b865_1bf9363be627 ;
    rdfs:subPropertyOf :electrochemistry_578c41e9_ee01_4840_9c8c_04ab6e4e6241 ;
    skos:prefLabel "hasPositiveElectrode"@en ;
    emmo:EMMO_967080e5_2f42_4eb2_a3a9_c58143e835f9 "relates an electrochemical cell to the electrode at which reduction occurs during discharge"@en .

:electrochemistry_9f466223_e20a_474d_ac4d_6d4b6131c275 a owl:Class ;
    rdfs:label "NonPolarizableElectrode"@en ;
    rdfs:comment "an electrode that holds its potential essentially constant by efficiently allowing electric current to pass"@en ;
    rdfs:subClassOf :electrochemistry_0f007072_a8dd_4798_b865_1bf9363be627 ;
    skos:prefLabel "NonPolarizableElectrode"@en ;
    emmo:EMMO_967080e5_2f42_4eb2_a3a9_c58143e835f9 "an electrode that holds its potential essentially constant by efficiently allowing electric current to pass"@en ;
    emmo:EMMO_c7b62dd7_063a_4c2a_8504_42f7264ba83f "this is a desirable characteristic for a reference electrode"@en .

:electrochemistry_9fd49892_cf6d_482e_a6c3_5f763948ec29 a owl:Class ;
    rdfs:label "LiquidMetalElectrode"@en ;
    rdfs:comment "an electrode that uses a liquid metal"@en ;
    rdfs:subClassOf :electrochemistry_5adb91e0_ffe1_41f3_b779_c6966f65fb0e ;
    skos:prefLabel "LiquidMetalElectrode"@en ;
    emmo:EMMO_26bf1bef_d192_4da6_b0eb_d2209698fb54 "https://www.wikidata.org/wiki/Q6557456" ;
    emmo:EMMO_967080e5_2f42_4eb2_a3a9_c58143e835f9 "an electrode that uses a liquid metal"@en ;
    emmo:EMMO_c7b62dd7_063a_4c2a_8504_42f7264ba83f "they can be used in electrocapillarity, voltammetry, and impedance measurements"@en ;
    emmo:EMMO_c84c6752_6d64_48cc_9500_e54a3c34898d "https://en.wikipedia.org/wiki/Liquid_metal_electrode"@en .

:electrochemistry_a0fcb105_587f_45d8_a89a_46dc8f745069 a owl:Class ;
    rdfs:label "Jacket"@en ;
    rdfs:comment "partial or complete external covering of a cell"@en ;
    rdfs:subClassOf emmo:EMMO_f76884f7_964e_488e_9bb7_1b2453e9e817 ;
    skos:prefLabel "Jacket"@en ;
    emmo:EMMO_50c298c2_55a2_4068_b3ac_4e948c33181f "https://www.electropedia.org/iev/iev.nsf/display?openform&ievref=482-02-20"@en ;
    emmo:EMMO_967080e5_2f42_4eb2_a3a9_c58143e835f9 "partial or complete external covering of a cell"@en ;
    emmo:EMMO_c7b62dd7_063a_4c2a_8504_42f7264ba83f "a jacket may be made of metal (insulated from the cell terminals), plastic, paper or other suitable material"@en .

:electrochemistry_a2b92d2e_4431_411e_8da5_a4c08bac2c0e a owl:Class ;
    rdfs:label "Electroplating"@en ;
    rdfs:comment "process inside an electrolytic cell used to coat a conductive object with a layer of a material"@en ;
    rdfs:subClassOf :electrochemistry_f0c24970_4c14_4207_bd78_5f2181a67085 ;
    skos:altLabel "Galvanizing"@en ;
    skos:prefLabel "Electroplating"@en ;
    emmo:EMMO_50c298c2_55a2_4068_b3ac_4e948c33181f "https://www.electropedia.org/iev/iev.nsf/display?openform&ievref=114-04-17"@en ;
    emmo:EMMO_967080e5_2f42_4eb2_a3a9_c58143e835f9 "process inside an electrolytic cell used to coat a conductive object with a layer of a material"@en ;
    emmo:EMMO_c7b62dd7_063a_4c2a_8504_42f7264ba83f "The process of depositing a usually thin layer of metal upon a usually metallic substrate (or any other conductor, e.g. graphite), in order to improve the appearance, and/or to change the surface properties of the substrate."@en ;
    emmo:EMMO_c84c6752_6d64_48cc_9500_e54a3c34898d "https://en.wikipedia.org/wiki/Electroplating"@en .

:electrochemistry_a2f4dca3_829f_412b_9025_bd7581aad82a a owl:Class ;
    rdfs:label "Valve"@en ;
    rdfs:comment "component of a cell which permits the flow of gas in one direction only"@en ;
    rdfs:subClassOf emmo:EMMO_f76884f7_964e_488e_9bb7_1b2453e9e817 ;
    skos:prefLabel "Valve"@en ;
    emmo:EMMO_50c298c2_55a2_4068_b3ac_4e948c33181f "https://www.electropedia.org/iev/iev.nsf/display?openform&ievref=482-02-12" ;
    emmo:EMMO_967080e5_2f42_4eb2_a3a9_c58143e835f9 "component of a cell which permits the flow of gas in one direction only"@en ;
    emmo:EMMO_c7b62dd7_063a_4c2a_8504_42f7264ba83f "a valve has a characteristic venting or opening and closing pressure"@en .

:electrochemistry_ae56cce3_7a7c_4e53_bb58_31e0d642d47e a owl:Class ;
    rdfs:label "FlameArrestorVent"@en ;
    rdfs:comment "vent of special design which provides protection against the propagation of a flame front from or into the interior of a secondary cell"@en ;
    rdfs:subClassOf emmo:EMMO_f76884f7_964e_488e_9bb7_1b2453e9e817 ;
    skos:prefLabel "FlameArrestorVent"@en ;
    emmo:EMMO_50c298c2_55a2_4068_b3ac_4e948c33181f "https://www.electropedia.org/iev/iev.nsf/display?openform&ievref=482-05-11" ;
    emmo:EMMO_967080e5_2f42_4eb2_a3a9_c58143e835f9 "vent of special design which provides protection against the propagation of a flame front from or into the interior of a secondary cell"@en ;
    emmo:EMMO_c7b62dd7_063a_4c2a_8504_42f7264ba83f "this flame front may originate from a spark or an external naked flame igniting combustible electrolysis gas"@en .

:electrochemistry_b0a0dddb_d942_4af2_b6a7_d7165f4253f1 a owl:Class ;
    rdfs:label "CarbonPasteElectrode"@en ;
    rdfs:comment "Electrode of a composite of carbon powder and a pasting liquid (including mineral oil, Nujol, bromoform, bromonaphthalene)."@en ;
    rdfs:subClassOf :electrochemistry_a0a619d7_da95_41f0_8bc3_9c19d636d543 ;
    skos:altLabel "CPE"@en ;
    skos:prefLabel "CarbonPasteElectrode"@en ;
    emmo:EMMO_26bf1bef_d192_4da6_b0eb_d2209698fb54 "https://www.wikidata.org/wiki/Q5037987" ;
    emmo:EMMO_967080e5_2f42_4eb2_a3a9_c58143e835f9 "Electrode of a composite of carbon powder and a pasting liquid (including mineral oil, Nujol, bromoform, bromonaphthalene)."@en ;
    emmo:EMMO_c7b62dd7_063a_4c2a_8504_42f7264ba83f "The CPE was first described by Adams in 1958. A CPE is typically housed in a Teflon holder, contacted by a conductive wire (occasionally a piston is used to renew the surface by extrusion of the used paste). Problems are long-term stability of the paste and that the binder can influence its properties."@en,
        "These electrodes can easily be chemically modified by the incorporation of reagents (electrocatalysts, redox mediators, complexation agents, enzymes, etc.) and by the attachment of micro- or nanoparticles to prepare electrochemical sensors for analytical applications."@en ;
    emmo:EMMO_c84c6752_6d64_48cc_9500_e54a3c34898d "https://en.wikipedia.org/wiki/Carbon_paste_electrode"@en .

:electrochemistry_b2d11f0d_c1b0_4476_8d17_03b73d31e01f a owl:Class ;
    rdfs:label "AsymmetricMembrane"@en ;
    rdfs:comment "membrane constituted of two or more structural planes of non-identical morphologies"@en ;
    rdfs:subClassOf :electrochemistry_331e6cca_f260_4bf8_af55_35304fe1bbe0 ;
    skos:prefLabel "AsymmetricMembrane"@en ;
    emmo:EMMO_26bf1bef_d192_4da6_b0eb_d2209698fb54 "https://www.wikidata.org/wiki/Q120965018" ;
    emmo:EMMO_967080e5_2f42_4eb2_a3a9_c58143e835f9 "membrane constituted of two or more structural planes of non-identical morphologies"@en ;
    emmo:EMMO_fe015383_afb3_44a6_ae86_043628697aa2 "https://doi.org/10.1351/goldbook.AT06862" .

:electrochemistry_b79d4f9e_5727_4895_8d7f_5fc18d83eb90 a owl:Class ;
    rdfs:label "ParasiticReaction"@en ;
    rdfs:comment "an unwanted side reaction"@en ;
    rdfs:subClassOf :electrochemistry_f47611a2_e081_47f0_b287_3fda5f706154 ;
    skos:prefLabel "ParasiticReaction"@en ;
    skos:scopeNote "Parasitic reactions are a subset of side reactions specifically associated with unwanted charge transfer."@en ;
    emmo:EMMO_50c298c2_55a2_4068_b3ac_4e948c33181f "https://www.electropedia.org/iev/iev.nsf/display?openform&ievref=114-02-07",
        "https://www.electropedia.org/iev/iev.nsf/display?openform&ievref=482-03-13" ;
    emmo:EMMO_967080e5_2f42_4eb2_a3a9_c58143e835f9 "an unwanted side reaction"@en ;
    emmo:EMMO_c7b62dd7_063a_4c2a_8504_42f7264ba83f "in a galvanic cell, parasitic reactions may cause inefficiencies or loss of performance"@en .

:electrochemistry_b851c7e9_60bf_4d3d_abe1_8d08d3d85124 a owl:Class ;
    rdfs:label "NegativeTerminal"@en ;
    rdfs:comment "accessible conductive part provided for the connection of an external electric circuit to the negative electrode of the cell"@en ;
    rdfs:subClassOf [ a owl:Restriction ;
            owl:onProperty emmo:EMMO_8785be5a_2493_4b12_8f39_31907ab11748 ;
            owl:someValuesFrom :electrochemistry_c94c041b_8ea6_43e7_85cc_d2bce7785b4c ],
        :electrochemistry_3f70e5c5_67f0_483e_998b_b83b7739c4bc ;
    skos:prefLabel "NegativeTerminal"@en ;
    emmo:EMMO_50c298c2_55a2_4068_b3ac_4e948c33181f "https://www.electropedia.org/iev/iev.nsf/display?openform&ievref=482-02-24" ;
    emmo:EMMO_967080e5_2f42_4eb2_a3a9_c58143e835f9 "accessible conductive part provided for the connection of an external electric circuit to the negative electrode of the cell"@en .

:electrochemistry_c610d869_cc03_44f0_b40d_ca86e945b9c9 a owl:Class ;
    rdfs:label "NonSpillableCell"@en ;
    rdfs:comment "cell from which electrolyte cannot escape regardless of its orientation"@en ;
    rdfs:subClassOf :electrochemistry_0acd0fc2_1048_4604_8e90_bf4e84bd87df ;
    skos:prefLabel "NonSpillableCell"@en ;
    emmo:EMMO_50c298c2_55a2_4068_b3ac_4e948c33181f "https://www.electropedia.org/iev/iev.nsf/display?openform&ievref=482-05-16" ;
    emmo:EMMO_967080e5_2f42_4eb2_a3a9_c58143e835f9 "cell from which electrolyte cannot escape regardless of its orientation"@en ;
    emmo:EMMO_c7b62dd7_063a_4c2a_8504_42f7264ba83f "some vented cells or batteries are designed so as to be non-spillable when operated within the limits specified by the manufacturer"@en .

:electrochemistry_c6a35be8_7ce2_415b_be9e_3a5ff9a7f2ad a owl:Class ;
    rdfs:label "Oxidation"@en ;
    rdfs:comment "chemical reaction in which electrons are transferred from a substance to oxygen to form a compound of that substance or, more generally, in which substance loses electrons"@en ;
    rdfs:subClassOf :electrochemistry_2d366f85_a644_4b3e_a641_fce81e72d158 ;
    skos:altLabel "OxidationReaction"@en ;
    skos:note "Electrons are generally transferred to another substance by a reduction reaction."@en ;
    skos:prefLabel "Oxidation"@en ;
    skos:related :electrochemistry_109a38d4_daaa_4748_a803_044fb7c97673 ;
    emmo:EMMO_50c298c2_55a2_4068_b3ac_4e948c33181f "https://www.electropedia.org/iev/iev.nsf/display?openform&ievref=113-02-15"@en ;
    emmo:EMMO_967080e5_2f42_4eb2_a3a9_c58143e835f9 "chemical reaction in which electrons are transferred from a substance to oxygen to form a compound of that substance or, more generally, in which substance loses electrons"@en ;
    emmo:EMMO_fe015383_afb3_44a6_ae86_043628697aa2 "https://goldbook.iupac.org/terms/view/O04362"@en .

:electrochemistry_d16eec87_c646_4566_bda6_7d3357cda061 a owl:Class ;
    rdfs:label "PassivationLayer"@en ;
    rdfs:comment "an interfacial layer of an electrode surface, that causes the electrode to become passivated"@en ;
    rdfs:subClassOf :electrochemistry_f78e3c87_01c6_4cc2_b047_30322262e22d ;
    skos:prefLabel "PassivationLayer"@en ;
    emmo:EMMO_967080e5_2f42_4eb2_a3a9_c58143e835f9 "an interfacial layer of an electrode surface, that causes the electrode to become passivated"@en .

:electrochemistry_d54f6aac_7cd2_4d52_9bca_2f19bb1eaec4 a owl:Class ;
    rdfs:label "IronPhosphateBasedElectrode"@en ;
    rdfs:comment "an electrode in which the primary active material consists of iron phosphate or iron phosphate compounds"@en ;
    rdfs:subClassOf :electrochemistry_9a823d64_9d10_4a29_9cbd_9bbdad7985bc ;
    skos:prefLabel "IronPhosphateBasedElectrode"@en ;
    emmo:EMMO_967080e5_2f42_4eb2_a3a9_c58143e835f9 "an electrode in which the primary active material consists of iron phosphate or iron phosphate compounds"@en ;
    emmo:EMMO_c7b62dd7_063a_4c2a_8504_42f7264ba83f "represented in IEC cell designations by the letter code Fp"@en .

:electrochemistry_d8a78cd2_8107_46dd_a198_0b64676efc00 a owl:Class ;
    rdfs:label "Connector"@en ;
    rdfs:comment "conductor of electricity used for carrying current between components in an electric circuit"@en ;
    rdfs:subClassOf emmo:EMMO_f76884f7_964e_488e_9bb7_1b2453e9e817 ;
    skos:example "a connector electrically joins two cells, or a terminal of a cell to a terminal of the battery, or a terminal of the battery to an exterior circuit and also to auxiliary devices"@en ;
    skos:prefLabel "Connector"@en ;
    emmo:EMMO_50c298c2_55a2_4068_b3ac_4e948c33181f "https://www.electropedia.org/iev/iev.nsf/display?openform&ievref=482-02-37" ;
    emmo:EMMO_967080e5_2f42_4eb2_a3a9_c58143e835f9 "conductor of electricity used for carrying current between components in an electric circuit"@en .

:electrochemistry_dc6abae7_39b0_4d22_b52e_14d088a4bd5f a owl:Class ;
    rdfs:label "Supercapacitor"@en ;
    rdfs:comment "type of capacitor characterized by high capacitance, high specific and volumetric energy density, and low voltage limits"@en ;
    rdfs:subClassOf :electrochemistry_0acd0fc2_1048_4604_8e90_bf4e84bd87df ;
    skos:altLabel "Supercap"@en ;
    skos:prefLabel "Supercapacitor"@en ;
    emmo:EMMO_26bf1bef_d192_4da6_b0eb_d2209698fb54 "https://www.wikidata.org/wiki/Q754523" ;
    emmo:EMMO_50c298c2_55a2_4068_b3ac_4e948c33181f "https://www.electropedia.org/iev/iev.nsf/display?openform&ievref=114-03-03"@en ;
    emmo:EMMO_967080e5_2f42_4eb2_a3a9_c58143e835f9 "type of capacitor characterized by high capacitance, high specific and volumetric energy density, and low voltage limits"@en ;
    emmo:EMMO_c84c6752_6d64_48cc_9500_e54a3c34898d "https://en.wikipedia.org/wiki/Supercapacitor"@en .

:electrochemistry_df78745e_f9db_4830_88f0_8ce074fcb8ff a owl:Class ;
    rdfs:label "MercuryElectrode"@en ;
    rdfs:comment "liquid metal electrode used in polarography"@en ;
    rdfs:subClassOf [ a owl:Restriction ;
            owl:onProperty :electrochemistry_860aa941_5ff9_4452_8a16_7856fad07bee ;
            owl:someValuesFrom chems:substance_dc5fb846_1824_40f8_9834_81f118aa1c2d ],
        :electrochemistry_9fd49892_cf6d_482e_a6c3_5f763948ec29 ;
    skos:altLabel "HgElectrode"@en ;
    skos:prefLabel "MercuryElectrode"@en ;
    emmo:EMMO_967080e5_2f42_4eb2_a3a9_c58143e835f9 "liquid metal electrode used in polarography"@en ;
    emmo:EMMO_c7b62dd7_063a_4c2a_8504_42f7264ba83f "A mercury film electrode (MFE) or thin mercury film electrode (TMFE) is formed by coating a conducting substrate, usually glassy carbon, with a layer of mercury (thin film, amalgam, or array of microdrops), often by electrodeposition from a solution containing Hg(II). The electrode area is normally in the range of 0.1 to 0.5 cm2 and mercury film thickness typically ranges from 10 to 1000 nm, producing a film of large surface area-to-volume ratio that results in a high analyte pre-concentration during the deposition step of anodic stripping voltammetry. Compared to an HMDE, the MFE provides high sensitivity and resolution; however, it is somewhat less reproducible and more prone to interferences from intermetallic formation and surface-active substances."@en,
        "Liquid mercury is an ideal electrode material for negative potentials because of its high overpotential for hydrogen evolution (electrochemical reduction of hydroxonium cations from solution). However, mercury is readily oxidized, particularly in the presence of anions that form complexes or that pre- cipitate with Hg(I) or Hg(II) ions, and thus it is not suitable for use at positive potentials. The use of liquid mercury has largely been discontinued because of concerns about the toxicity of the element and its compounds."@en .

:electrochemistry_e3d3d21c_cb9a_498c_bdb0_63c964f0d3c6 a owl:Class ;
    rdfs:label "CapacityFade"@en ;
    rdfs:comment "a degradation phenomena in electrochemical devices in which the practicaclly achieveable capacity of the cell is less than the measured capacity at the beginning of life."@en ;
    rdfs:subClassOf [ a owl:Restriction ;
            owl:onProperty emmo:EMMO_ae2d1a96_bfa1_409a_a7d2_03d69e8a125a ;
            owl:someValuesFrom :electrochemistry_0acd0fc2_1048_4604_8e90_bf4e84bd87df ],
        :electrochemistry_0a0de817_addc_46a5_8ba2_255d48cdf366 ;
    skos:altLabel "CapacityLoss"@en ;
    skos:prefLabel "CapacityFade"@en ;
    emmo:EMMO_26bf1bef_d192_4da6_b0eb_d2209698fb54 "https://www.wikidata.org/wiki/Q16851742" ;
    emmo:EMMO_967080e5_2f42_4eb2_a3a9_c58143e835f9 "a degradation phenomena in electrochemical devices in which the practicaclly achieveable capacity of the cell is less than the measured capacity at the beginning of life."@en ;
    emmo:EMMO_c84c6752_6d64_48cc_9500_e54a3c34898d "https://en.wikipedia.org/wiki/Capacity_loss"@en .

:electrochemistry_eacb141f_6ab4_491f_8603_a3e025cefc82 a owl:Class ;
    rdfs:label "RoundCase"@en ;
    rdfs:comment "a case that is described by its diameter and height"@en ;
    rdfs:subClassOf [ a owl:Restriction ;
            owl:onProperty emmo:EMMO_dba27ca1_33c9_4443_a912_1519ce4c39ec ;
            owl:someValuesFrom :electrochemistry_1e33e37e_d7c9_4701_ba6d_a09456a13aaf ],
        [ a owl:Restriction ;
            owl:onProperty emmo:EMMO_dba27ca1_33c9_4443_a912_1519ce4c39ec ;
            owl:someValuesFrom :electrochemistry_4a5660bd_1c1a_40e5_8a41_463c720d3903 ],
        :electrochemistry_1aec4cc0_82d5_4042_a657_ed7fe291c3d8 ;
    skos:prefLabel "RoundCase"@en ;
    emmo:EMMO_967080e5_2f42_4eb2_a3a9_c58143e835f9 "a case that is described by its diameter and height"@en ;
    emmo:EMMO_c7b62dd7_063a_4c2a_8504_42f7264ba83f "often represented in cell designations by the letter R"@en .

:electrochemistry_ebdb68e9_c4b5_4d57_a042_c0f51d446755 a owl:Class ;
    rdfs:label "ElectrochemicalMaterial"@en ;
    rdfs:comment "a material that takes active part in an electrochemical reaction"@en ;
    rdfs:subClassOf emmo:EMMO_68390bfb_e307_479d_8f78_d66d8773cb1d ;
    skos:prefLabel "ElectrochemicalMaterial"@en ;
    emmo:EMMO_967080e5_2f42_4eb2_a3a9_c58143e835f9 "a material that takes active part in an electrochemical reaction"@en .

:electrochemistry_f47611a2_e081_47f0_b287_3fda5f706154 a owl:Class ;
    rdfs:label "SideReaction"@en ;
    rdfs:comment "chemical reaction which occurs in addition to the main process"@en ;
    rdfs:subClassOf :electrochemistry_8a1c9a7b_978c_4421_a9c1_d0b07b42aab9 ;
    skos:altLabel "SecondaryReaction"@en ;
    skos:prefLabel "SideReaction"@en ;
    emmo:EMMO_26bf1bef_d192_4da6_b0eb_d2209698fb54 "https://www.wikidata.org/wiki/Q22117434" ;
    emmo:EMMO_50c298c2_55a2_4068_b3ac_4e948c33181f "https://www.electropedia.org/iev/iev.nsf/display?openform&ievref=114-02-06",
        "https://www.electropedia.org/iev/iev.nsf/display?openform&ievref=482-03-13" ;
    emmo:EMMO_967080e5_2f42_4eb2_a3a9_c58143e835f9 "chemical reaction which occurs in addition to the main process"@en ;
    emmo:EMMO_b6730304_cabc_4104_b415_14218466445c "Side reactions can lead to degradation, gas formation, or loss of active material."@en ;
    emmo:EMMO_c84c6752_6d64_48cc_9500_e54a3c34898d "https://en.wikipedia.org/wiki/Side_reaction"@en .

emmo:EMMO_38b579de_4331_40e0_803d_09efa298e726 rdfs:subClassOf [ a owl:Restriction ;
            owl:onProperty emmo:EMMO_e1097637_70d2_4895_973f_2396f04fa204 ;
            owl:someValuesFrom emmo:EMMO_ed4af7ae_63a2_497e_bb88_2309619ea405 ],
        [ a owl:Restriction ;
            owl:onProperty emmo:EMMO_e1097637_70d2_4895_973f_2396f04fa204 ;
            owl:someValuesFrom emmo:EMMO_f1a51559_aa3d_43a0_9327_918039f0dfed ] .

:electrochemistry_0a399f3f_b873_41f5_be1f_9b6df75cc30a a owl:Class ;
    rdfs:label "Additive"@en ;
    rdfs:comment "a substance added to something in small quantities to alter its properties"@en ;
    rdfs:subClassOf :electrochemistry_b5ea31c9_bb10_4276_980e_c3eceb1efc82 ;
    skos:prefLabel "Additive"@en ;
    emmo:EMMO_26bf1bef_d192_4da6_b0eb_d2209698fb54 "https://www.wikidata.org/wiki/Q350176"@en ;
    emmo:EMMO_967080e5_2f42_4eb2_a3a9_c58143e835f9 "a substance added to something in small quantities to alter its properties"@en .

:electrochemistry_1e33e37e_d7c9_4701_ba6d_a09456a13aaf a owl:Class ;
    rdfs:label "CellLid"@en ;
    rdfs:comment "part used to close the case normally having holes for filling, topping-up, gas escape, terminals, etc."@en ;
    rdfs:subClassOf :electrochemistry_b5ea31c9_bb10_4276_980e_c3eceb1efc82 ;
    skos:prefLabel "CellLid"@en ;
    emmo:EMMO_50c298c2_55a2_4068_b3ac_4e948c33181f "https://www.electropedia.org/iev/iev.nsf/display?openform&ievref=482-02-15"@en ;
    emmo:EMMO_967080e5_2f42_4eb2_a3a9_c58143e835f9 "part used to close the case normally having holes for filling, topping-up, gas escape, terminals, etc."@en .

:electrochemistry_2d366f85_a644_4b3e_a641_fce81e72d158 a owl:Class ;
    rdfs:label "RedoxReaction"@en ;
    rdfs:comment "a chemical reaction involving a change in oxidation state of one or more atomic centers through electron transfer or an equivalent formal process"@en ;
    rdfs:subClassOf :electrochemistry_8a1c9a7b_978c_4421_a9c1_d0b07b42aab9 ;
    skos:altLabel "Redox"@en ;
    skos:prefLabel "RedoxReaction"@en ;
    skos:scopeNote "Redox reactions include both electrochemical and non-electrochemical processes; when the electron transfer occurs across an electrodeelectrolyte interface the reaction is electrochemical."@en ;
    emmo:EMMO_26bf1bef_d192_4da6_b0eb_d2209698fb54 "https://www.wikidata.org/wiki/Q82682"@en ;
    emmo:EMMO_967080e5_2f42_4eb2_a3a9_c58143e835f9 "a chemical reaction involving a change in oxidation state of one or more atomic centers through electron transfer or an equivalent formal process"@en ;
    emmo:EMMO_c84c6752_6d64_48cc_9500_e54a3c34898d "https://en.wikipedia.org/wiki/Redox"@en .

:electrochemistry_2e6933aa_4522_4f16_a437_37110e6cbd0d a owl:Class ;
    rdfs:label "ElectrodePolarisation"@en ;
    rdfs:comment "accumulation or depletion of electric charges at an electrode, resulting in a difference between the electrode potential with current flow, and the potential without current flow or equilibrium electrode potential"@en ;
    rdfs:subClassOf [ a owl:Restriction ;
            owl:onProperty emmo:EMMO_ae2d1a96_bfa1_409a_a7d2_03d69e8a125a ;
            owl:someValuesFrom :electrochemistry_0f007072_a8dd_4798_b865_1bf9363be627 ],
        :electrochemistry_19abaccd_43be_4048_965c_e4fb63c5951b ;
    skos:altLabel "ElectrodePolarization"@en,
        "Polarisation"@en,
        "Polarization"@en ;
    skos:prefLabel "ElectrodePolarisation"@en ;
    emmo:EMMO_26bf1bef_d192_4da6_b0eb_d2209698fb54 "https://www.wikidata.org/wiki/Q2698605" ;
    emmo:EMMO_50c298c2_55a2_4068_b3ac_4e948c33181f "https://www.electropedia.org/iev/iev.nsf/display?openform&ievref=114-02-15"@en ;
    emmo:EMMO_967080e5_2f42_4eb2_a3a9_c58143e835f9 "accumulation or depletion of electric charges at an electrode, resulting in a difference between the electrode potential with current flow, and the potential without current flow or equilibrium electrode potential"@en ;
    emmo:EMMO_c84c6752_6d64_48cc_9500_e54a3c34898d "https://en.wikipedia.org/wiki/Polarization_(electrochemistry)"@en .

:electrochemistry_3d805c2a_4801_440e_9e4d_0fa5585c76ae a owl:Class ;
    rdfs:label "ElectrochemicalRelation"@en ;
    rdfs:comment "A material relation in electrochemistry."@en ;
    rdfs:subClassOf emmo:EMMO_e5438930_04e7_4d42_ade5_3700d4a52ab7 ;
    skos:prefLabel "ElectrochemicalRelation"@en ;
    emmo:EMMO_967080e5_2f42_4eb2_a3a9_c58143e835f9 "A material relation in electrochemistry."@en .

:electrochemistry_3f70e5c5_67f0_483e_998b_b83b7739c4bc a owl:Class ;
    rdfs:label "Terminal"@en ;
    rdfs:comment "conductive part of a device, electric circuit or electric network, provided for connecting that device, electric circuit or electric network to one or more external conductors"@en ;
    rdfs:subClassOf emmo:EMMO_f76884f7_964e_488e_9bb7_1b2453e9e817 ;
    skos:prefLabel "Terminal"@en ;
    emmo:EMMO_50c298c2_55a2_4068_b3ac_4e948c33181f "https://www.electropedia.org/iev/iev.nsf/display?openform&ievref=482-02-22" ;
    emmo:EMMO_967080e5_2f42_4eb2_a3a9_c58143e835f9 "conductive part of a device, electric circuit or electric network, provided for connecting that device, electric circuit or electric network to one or more external conductors"@en .

:electrochemistry_468b3b63_b62a_4110_8c7e_40fffd5fdfd6 a owl:Class ;
    rdfs:label "ManganesePhosphateBasedElectrode"@en ;
    rdfs:comment "an electrode in which the primary active material consists of manganese phosphate or manganese phosphate compounds"@en ;
    rdfs:subClassOf :electrochemistry_9a823d64_9d10_4a29_9cbd_9bbdad7985bc ;
    skos:prefLabel "ManganesePhosphateBasedElectrode"@en ;
    emmo:EMMO_967080e5_2f42_4eb2_a3a9_c58143e835f9 "an electrode in which the primary active material consists of manganese phosphate or manganese phosphate compounds"@en ;
    emmo:EMMO_c7b62dd7_063a_4c2a_8504_42f7264ba83f "often represented in cell designations by the letter Mp"@en,
        "this class is intended to enable designations based on IEC recommendations"@en .

:electrochemistry_49263a32_eca6_4644_8144_0d3b14c26d0a a owl:Class ;
    rdfs:label "Dissolution"@en ;
    rdfs:comment "mixing of a substance into another substance with formation of one new homogeneous substance"@en ;
    rdfs:subClassOf :electrochemistry_8a1c9a7b_978c_4421_a9c1_d0b07b42aab9 ;
    skos:prefLabel "Dissolution"@en ;
    emmo:EMMO_50c298c2_55a2_4068_b3ac_4e948c33181f "https://www.electropedia.org/iev/iev.nsf/display?openform&ievref=114-01-04" ;
    emmo:EMMO_967080e5_2f42_4eb2_a3a9_c58143e835f9 "mixing of a substance into another substance with formation of one new homogeneous substance"@en ;
    emmo:EMMO_c7b62dd7_063a_4c2a_8504_42f7264ba83f "the result of the dissolution of one or more solutes into a solvent is a solution"@en .

:electrochemistry_4a5660bd_1c1a_40e5_8a41_463c720d3903 a owl:Class ;
    rdfs:label "CellCan"@en ;
    rdfs:comment "cell container which is usually metallic and typically, but not exclusively, cylindrical"@en ;
    rdfs:subClassOf :electrochemistry_b5ea31c9_bb10_4276_980e_c3eceb1efc82 ;
    skos:prefLabel "CellCan"@en ;
    emmo:EMMO_50c298c2_55a2_4068_b3ac_4e948c33181f "https://www.electropedia.org/iev/iev.nsf/display?openform&ievref=482-02-13" ;
    emmo:EMMO_967080e5_2f42_4eb2_a3a9_c58143e835f9 "cell container which is usually metallic and typically, but not exclusively, cylindrical"@en .

:electrochemistry_50044b99_b858_433b_a32d_23d1e1cf88b2 a owl:Class ;
    rdfs:label "ElectrochemicalInterface"@en ;
    rdfs:comment "the two-dimensional space comprising the boundary between two electrochemical constituents"@en ;
    rdfs:subClassOf :electrochemistry_94d9d5e2_9e9b_4eb7_b3ce_f3d658b7ae64 ;
    skos:prefLabel "ElectrochemicalInterface"@en ;
    emmo:EMMO_967080e5_2f42_4eb2_a3a9_c58143e835f9 "the two-dimensional space comprising the boundary between two electrochemical constituents"@en ;
    emmo:EMMO_c7b62dd7_063a_4c2a_8504_42f7264ba83f "The area where electrochemical reactions normally take place."@en .

:electrochemistry_5f9a9411_05f9_4576_acd3_81d7d41cfe98 a owl:Class ;
    rdfs:label "NonAqueousElectrolyte"@en ;
    rdfs:comment "an ion-transport medium that does not contain water."@en ;
    rdfs:subClassOf :electrochemistry_609b340f_3450_4a10_95c2_c457e3eb8a89 ;
    skos:altLabel "NonAqueousElectrolyticSolution"@en,
        "NonAqueousSolution"@en ;
    skos:prefLabel "NonAqueousElectrolyte"@en ;
    emmo:EMMO_967080e5_2f42_4eb2_a3a9_c58143e835f9 "an ion-transport medium that does not contain water."@en .

:electrochemistry_79d1b273_58cd_4be6_a250_434817f7c261 a owl:Class ;
    rdfs:label "ActiveMaterial"@en ;
    rdfs:comment "material that is oxidized or reduced at an electrode in an electrochemical cell"@en ;
    rdfs:subClassOf [ a owl:Restriction ;
            owl:onProperty emmo:EMMO_e1097637_70d2_4895_973f_2396f04fa204 ;
            owl:someValuesFrom :electrochemistry_1e3dc60d_dd6b_47d6_8161_70004fc5ee30 ],
        :electrochemistry_b5ea31c9_bb10_4276_980e_c3eceb1efc82,
        :electrochemistry_ebdb68e9_c4b5_4d57_a042_c0f51d446755 ;
    skos:altLabel "ActiveElectrochemicalMaterial"@en,
        "ElectrochemicallyActiveMaterial"@en ;
    skos:example "lithium iron phosphate"@en,
        "zinc"@en ;
    skos:prefLabel "ActiveMaterial"@en ;
    skos:related :electrochemistry_0f007072_a8dd_4798_b865_1bf9363be627 ;
    emmo:EMMO_26bf1bef_d192_4da6_b0eb_d2209698fb54 "https://www.wikidata.org/wiki/Q120907375" ;
    emmo:EMMO_50c298c2_55a2_4068_b3ac_4e948c33181f "https://www.electropedia.org/iev/iev.nsf/display?openform&ievref=482-02-33",
        "https://www.electropedia.org/iev/iev.nsf/display?openform&ievref=114-03-14"@en ;
    emmo:EMMO_967080e5_2f42_4eb2_a3a9_c58143e835f9 "material that is oxidized or reduced at an electrode in an electrochemical cell"@en .

:electrochemistry_838c115b_6bc9_4ce8_9f8d_86a6bf67742a a owl:Class ;
    rdfs:label "CobaltBasedElectrode"@en ;
    rdfs:comment "an electrode which contains mostly materials based on cobalt"@en ;
    rdfs:subClassOf :electrochemistry_9a823d64_9d10_4a29_9cbd_9bbdad7985bc ;
    skos:prefLabel "CobaltBasedElectrode"@en ;
    emmo:EMMO_967080e5_2f42_4eb2_a3a9_c58143e835f9 "an electrode which contains mostly materials based on cobalt"@en ;
    emmo:EMMO_c7b62dd7_063a_4c2a_8504_42f7264ba83f "often represented in IEC cell designations by the letter C"@en,
        "this class is intended to enable designations based on IEC recommendations"@en .

:electrochemistry_871bc4a4_2d17_4b88_9b0f_7ab85f14afea a owl:Class ;
    rdfs:label "CounterElectrode"@en ;
    rdfs:comment "electrode whose function is to carry the electric current flowing through the electrical circuit of an electrochemical cell, the electrochemical processes on its surface not being of interest"@en ;
    rdfs:subClassOf :electrochemistry_0f007072_a8dd_4798_b865_1bf9363be627 ;
    skos:altLabel "AuxiliaryElectrode"@en ;
    skos:prefLabel "CounterElectrode"@en ;
    skos:related :electrochemistry_7729c34e_1ae9_403d_b933_1765885e7f29,
        :electrochemistry_fb988878_ee54_4350_9ee9_228c00c3ad35 ;
    emmo:EMMO_26bf1bef_d192_4da6_b0eb_d2209698fb54 "https://www.wikidata.org/wiki/Q1768785" ;
    emmo:EMMO_967080e5_2f42_4eb2_a3a9_c58143e835f9 "electrode whose function is to carry the electric current flowing through the electrical circuit of an electrochemical cell, the electrochemical processes on its surface not being of interest"@en ;
    emmo:EMMO_c7b62dd7_063a_4c2a_8504_42f7264ba83f "An auxiliary electrode is used in any three-electrode cell, together with a working electrode and reference electrode."@en,
        "An auxiliary electrode must not add an excessive potential burden to the cell. It is chosen for the efficiency of the electrochemical reaction and usually has a greater surface area than the working electrode."@en ;
    emmo:EMMO_c84c6752_6d64_48cc_9500_e54a3c34898d "https://en.wikipedia.org/wiki/Auxiliary_electrode"@en ;
    emmo:EMMO_fe015383_afb3_44a6_ae86_043628697aa2 "https://goldbook.iupac.org/terms/view/A00535"@en .

:electrochemistry_e248373f_294f_4ca4_9edf_0ad6653bb64f a owl:Class ;
    rdfs:label "GalvanicCell"@en ;
    rdfs:comment "electrochemical cell in which chemical reactions occur spontaneously and chemical energy is converted into electrical energy."@en ;
    rdfs:subClassOf :electrochemistry_6f2c88c9_5c04_4953_a298_032cc3ab9b77 ;
    skos:prefLabel "GalvanicCell"@en ;
    emmo:EMMO_26bf1bef_d192_4da6_b0eb_d2209698fb54 "https://www.wikidata.org/wiki/Q209440" ;
    emmo:EMMO_50c298c2_55a2_4068_b3ac_4e948c33181f "https://www.electropedia.org/iev/iev.nsf/display?openform&ievref=114-03-02"@en ;
    emmo:EMMO_6dd685dd_1895_46e4_b227_be9f7d643c25 "https://dbpedia.org/page/Galvanic_cell"@en ;
    emmo:EMMO_967080e5_2f42_4eb2_a3a9_c58143e835f9 "electrochemical cell in which chemical reactions occur spontaneously and chemical energy is converted into electrical energy."@en ;
    emmo:EMMO_c7b62dd7_063a_4c2a_8504_42f7264ba83f "An electrochemical cell that spontaneously produces work."@en,
        "Electrochemical cell intended to produce electric energy."@en ;
    emmo:EMMO_c84c6752_6d64_48cc_9500_e54a3c34898d "https://en.wikipedia.org/wiki/Galvanic_cell"@en .

:electrochemistry_f0c24970_4c14_4207_bd78_5f2181a67085 a owl:Class ;
    rdfs:label "Electrodeposition"@en ;
    rdfs:comment "the process of forming a film or a bulk material using an electrochemical process where the electrons are supplied by an external power supply"@en ;
    rdfs:subClassOf emmo:EMMO_bafc17b5_9be4_4823_8bbe_ab4e90b6738c,
        :electrochemistry_f4a1323a_ce2b_4c1a_b89d_c80170110ed6 ;
    skos:example "Deposition of metallic zinc from Zn^{2+} ions in an electroplating bath."@en ;
    skos:prefLabel "Electrodeposition"@en ;
    skos:related :electrochemistry_4df84ec1_8a1a_4770_963f_bf48009bd043 ;
    skos:scopeNote "Used in manufacturing, coating, and electrorefining applications."@en ;
    emmo:EMMO_967080e5_2f42_4eb2_a3a9_c58143e835f9 "the process of forming a film or a bulk material using an electrochemical process where the electrons are supplied by an external power supply"@en .

:electrochemistry_f2c33088_224f_4fdb_857a_7cb62e3dddca a owl:Class ;
    rdfs:label "CarbonBasedElectrode"@en ;
    rdfs:comment "an electrode in which the primary active material consists of carbon or carbon compounds"@en ;
    rdfs:subClassOf :electrochemistry_0f007072_a8dd_4798_b865_1bf9363be627 ;
    skos:prefLabel "CarbonBasedElectrode"@en ;
    emmo:EMMO_967080e5_2f42_4eb2_a3a9_c58143e835f9 "an electrode in which the primary active material consists of carbon or carbon compounds"@en ;
    emmo:EMMO_c7b62dd7_063a_4c2a_8504_42f7264ba83f "often represented in IEC cell designations by the letter I"@en,
        "this class is intended to enable designations based on IEC recommendations"@en .

:electrochemistry_fa22874b_76a9_4043_8b8f_6086c88746de a owl:Class ;
    rdfs:label "ElectrolyteSolution"@en ;
    rdfs:comment "a liquid electrolyte that consists of solutes dissolved in a solvent"@en ;
    rdfs:subClassOf [ a owl:Restriction ;
            owl:onProperty :electrochemistry_808e94df_e002_4e64_a6db_182ed75078c6 ;
            owl:someValuesFrom chems:substance_0f2f65a7_5cc4_4c86_a4d0_676771c646f1 ],
        [ a owl:Restriction ;
            owl:onProperty :electrochemistry_8784ef24_320b_4a3d_b200_654aec6c271c ;
            owl:someValuesFrom chems:substance_3899a9c9_9b34_443e_8ce6_0257589bb38a ],
        emmo:EMMO_4b3e2374_52a1_4420_8e3f_3ae6b9bf7dff,
        :electrochemistry_609b340f_3450_4a10_95c2_c457e3eb8a89 ;
    skos:altLabel "ElectrolyticSolution"@en ;
    skos:prefLabel "ElectrolyteSolution"@en ;
    emmo:EMMO_967080e5_2f42_4eb2_a3a9_c58143e835f9 "a liquid electrolyte that consists of solutes dissolved in a solvent"@en .

:electrochemistry_057bb143_639c_472b_99ed_ffa1867f6e63 a owl:Class ;
    rdfs:label "GlassyCarbonElectrode"@en ;
    rdfs:comment "electrode made of glassy carbon material with an intertwined graphitic ribbon structure, formed by pyrolysis of a resol precursor at temperatures up to 3000 C"@en ;
    rdfs:subClassOf :electrochemistry_a0a619d7_da95_41f0_8bc3_9c19d636d543 ;
    skos:altLabel "GCE"@en ;
    skos:prefLabel "GlassyCarbonElectrode"@en ;
    emmo:EMMO_967080e5_2f42_4eb2_a3a9_c58143e835f9 "electrode made of glassy carbon material with an intertwined graphitic ribbon structure, formed by pyrolysis of a resol precursor at temperatures up to 3000 C"@en ;
    emmo:EMMO_c7b62dd7_063a_4c2a_8504_42f7264ba83f "extremely resistant to many chemicals, impermeable to gases and liquids, and has good electrical conductivity, high hardness and strength, and biocompatibility"@en,
        "glassy carbon combines glass-like mechanical characteristics with physical properties similar to graphite, owing to its graphene ribbon structure"@en,
        "one of the most frequently used working electrodes"@en .

:electrochemistry_2e3e14f9_4cb8_45b2_908e_47eec893dec8 a owl:Class ;
    rdfs:label "ElectrodeReaction"@en ;
    rdfs:comment "electrochemical reaction involving the transfer of electrons between electrolyte and electrode"@en ;
    rdfs:subClassOf :electrochemistry_a6a69e90_06b5_45b1_83cf_7c0bf39b2914 ;
    skos:prefLabel "ElectrodeReaction"@en ;
    emmo:EMMO_50c298c2_55a2_4068_b3ac_4e948c33181f "https://www.electropedia.org/iev/iev.nsf/display?openform&ievref=114-02-04"@en ;
    emmo:EMMO_967080e5_2f42_4eb2_a3a9_c58143e835f9 "electrochemical reaction involving the transfer of electrons between electrolyte and electrode"@en ;
    emmo:EMMO_c7b62dd7_063a_4c2a_8504_42f7264ba83f "An interfacial reaction that necessarily involves a charge-transfer step."@en,
        "The electrode (or interfacial) reaction involves all the processes (chemical reaction, structural reorganization, adsorption) accompanying the charge transfer step."@en ;
    emmo:EMMO_fe015383_afb3_44a6_ae86_043628697aa2 "https://doi.org/10.1351/goldbook.E01960"@en .

:electrochemistry_5186239a_2af7_4dbf_92ca_22e8e583c528 a owl:Class ;
    rdfs:label "BlendedActiveElectrode"@en ;
    rdfs:comment "an active electrode with a blend of two or more active materials"@en ;
    rdfs:subClassOf :electrochemistry_9a823d64_9d10_4a29_9cbd_9bbdad7985bc ;
    skos:prefLabel "BlendedActiveElectrode"@en ;
    emmo:EMMO_967080e5_2f42_4eb2_a3a9_c58143e835f9 "an active electrode with a blend of two or more active materials"@en .

:electrochemistry_5adb91e0_ffe1_41f3_b779_c6966f65fb0e a owl:Class ;
    rdfs:label "MetalElectrode"@en ;
    rdfs:comment "an electrode in which the actve electrochemical material is a metal"@en ;
    rdfs:subClassOf :electrochemistry_9a823d64_9d10_4a29_9cbd_9bbdad7985bc ;
    skos:prefLabel "MetalElectrode"@en ;
    emmo:EMMO_967080e5_2f42_4eb2_a3a9_c58143e835f9 "an electrode in which the actve electrochemical material is a metal"@en ;
    emmo:EMMO_c7b62dd7_063a_4c2a_8504_42f7264ba83f "the term metal is meant to loosely cover alkali metals, alkaline earth metals, transition metals, post-transition metals, and metalloids"@en .

:electrochemistry_615cff2a_be95_4e65_9471_98db23f4c878 a owl:Class ;
    rdfs:label "AlkalineElectrolyte"@en ;
    rdfs:comment "an aqueous electrolyte with a nominal pH greater than 7"@en ;
    rdfs:subClassOf :electrochemistry_b812e9d0_7c58_4455_b3e7_6847f10c8e8a ;
    skos:altLabel "AlkalineAqueousElectrolyte"@en,
        "AlkalineSolution"@en ;
    skos:example "KOH-H2O"@en ;
    skos:prefLabel "AlkalineElectrolyte"@en ;
    emmo:EMMO_967080e5_2f42_4eb2_a3a9_c58143e835f9 "an aqueous electrolyte with a nominal pH greater than 7"@en ;
    emmo:EMMO_c7b62dd7_063a_4c2a_8504_42f7264ba83f "typical alkaline electrolytes have a pH in the range 13 < x < 15"@en .

:electrochemistry_a0580fa9_5073_44af_b33e_7adbc83892d0 a owl:Class ;
    rdfs:label "AnodicReaction"@en ;
    rdfs:comment "electrode reaction in which oxidation occurs at the anode"@en ;
    rdfs:subClassOf :electrochemistry_2e3e14f9_4cb8_45b2_908e_47eec893dec8,
        :electrochemistry_c6a35be8_7ce2_415b_be9e_3a5ff9a7f2ad ;
    skos:altLabel "Electrooxidation"@en,
        "ElectrooxidationReaction"@en ;
    skos:prefLabel "AnodicReaction"@en ;
    skos:related :electrochemistry_b6319c74_d2ce_48c0_a75a_63156776b302,
        :electrochemistry_f4a1323a_ce2b_4c1a_b89d_c80170110ed6 ;
    emmo:EMMO_50c298c2_55a2_4068_b3ac_4e948c33181f "https://www.electropedia.org/iev/iev.nsf/display?openform&ievref=114-02-09"@en ;
    emmo:EMMO_967080e5_2f42_4eb2_a3a9_c58143e835f9 "electrode reaction in which oxidation occurs at the anode"@en .

:electrochemistry_a3b53904_22b1_42a9_a515_c8a3aed7e841 a owl:Class ;
    rdfs:label "Electrocatalyst"@en ;
    rdfs:comment "material that can cause electrocatalysis."@en ;
    rdfs:subClassOf :electrochemistry_8ab1e656_38ff_48e6_ab09_293d76bc9044 ;
    skos:prefLabel "Electrocatalyst"@en ;
    emmo:EMMO_26bf1bef_d192_4da6_b0eb_d2209698fb54 "https://www.wikidata.org/wiki/Q5357962" ;
    emmo:EMMO_50c298c2_55a2_4068_b3ac_4e948c33181f "https://www.electropedia.org/iev/iev.nsf/display?openform&ievref=114-04-16" ;
    emmo:EMMO_6dd685dd_1895_46e4_b227_be9f7d643c25 "https://dbpedia.org/page/Electrocatalyst"@en ;
    emmo:EMMO_967080e5_2f42_4eb2_a3a9_c58143e835f9 "material that can cause electrocatalysis."@en ;
    emmo:EMMO_c84c6752_6d64_48cc_9500_e54a3c34898d "https://en.wikipedia.org/wiki/Electrocatalyst"@en .

:electrochemistry_a6a69e90_06b5_45b1_83cf_7c0bf39b2914 a owl:Class ;
    rdfs:label "ElectrochemicalReaction"@en ;
    rdfs:comment "a chemical reaction in an electrolyte involving a transfer of electrons between chemical components or between chemical components and an electrode"@en ;
    rdfs:subClassOf :electrochemistry_19abaccd_43be_4048_965c_e4fb63c5951b,
        :electrochemistry_2d366f85_a644_4b3e_a641_fce81e72d158 ;
    skos:altLabel "ChargeTransferReaction"@en ;
    skos:note "electrochemical reactions occur at electrochemical interfaces"@en ;
    skos:prefLabel "ElectrochemicalReaction"@en ;
    emmo:EMMO_26bf1bef_d192_4da6_b0eb_d2209698fb54 "https://www.wikidata.org/wiki/Q120892494" ;
    emmo:EMMO_50c298c2_55a2_4068_b3ac_4e948c33181f "https://www.electropedia.org/iev/iev.nsf/display?openform&ievref=114-02-01",
        "https://www.electropedia.org/iev/iev.nsf/display?openform&ievref=482-03-01" ;
    emmo:EMMO_967080e5_2f42_4eb2_a3a9_c58143e835f9 "a chemical reaction in an electrolyte involving a transfer of electrons between chemical components or between chemical components and an electrode"@en ;
    emmo:EMMO_c7b62dd7_063a_4c2a_8504_42f7264ba83f "The electrode reaction can also involve other chemical reactions including subreactions on a cell electrode."@en,
        "any process either caused or accompanied by the passage of an electric current and involving in most cases the transfer of electrons between two substances"@en .

:electrochemistry_b1ac8d0c_a215_4e60_82b0_38272eff5131 a owl:Class ;
    rdfs:label "ManganeseBasedElectrode"@en ;
    rdfs:comment "an electrode in which the primary active material consists of manganese or manganese compounds"@en ;
    rdfs:subClassOf :electrochemistry_9a823d64_9d10_4a29_9cbd_9bbdad7985bc ;
    skos:prefLabel "ManganeseBasedElectrode"@en ;
    emmo:EMMO_967080e5_2f42_4eb2_a3a9_c58143e835f9 "an electrode in which the primary active material consists of manganese or manganese compounds"@en ;
    emmo:EMMO_c7b62dd7_063a_4c2a_8504_42f7264ba83f "often represented in cell designations by the letter M"@en,
        "this class is intended to enable designations based on IEC recommendations"@en .

:electrochemistry_b812e9d0_7c58_4455_b3e7_6847f10c8e8a a owl:Class ;
    rdfs:label "AqueousElectrolyte"@en ;
    rdfs:comment "an ion-transport medium, which may be immobilized, in which water is the solvent."@en ;
    rdfs:subClassOf emmo:EMMO_5cb107ba_7daa_46dd_8f9f_da22a6eac676,
        :electrochemistry_fa22874b_76a9_4043_8b8f_6086c88746de ;
    skos:altLabel "AqueousElectrolyticSolution"@en ;
    skos:prefLabel "AqueousElectrolyte"@en ;
    emmo:EMMO_26bf1bef_d192_4da6_b0eb_d2209698fb54 "https://www.wikidata.org/wiki/Q120906632" ;
    emmo:EMMO_6dd685dd_1895_46e4_b227_be9f7d643c25 "https://dbpedia.org/page/Aqueous_solution"@en ;
    emmo:EMMO_967080e5_2f42_4eb2_a3a9_c58143e835f9 "an ion-transport medium, which may be immobilized, in which water is the solvent."@en .

:electrochemistry_bbb1d95b_72d1_44f6_b07e_a3d7d41ac215 a owl:Class ;
    rdfs:label "GasDiffusionElectrode"@en ;
    rdfs:comment "a type of electrode specifically designed for gaseous reactants or products or both"@en ;
    rdfs:subClassOf [ a owl:Restriction ;
            owl:onProperty emmo:EMMO_dba27ca1_33c9_4443_a912_1519ce4c39ec ;
            owl:someValuesFrom :electrochemistry_a3b53904_22b1_42a9_a515_c8a3aed7e841 ],
        :electrochemistry_3663991d_9319_4f7a_922b_f0e428b58801,
        :electrochemistry_a0a619d7_da95_41f0_8bc3_9c19d636d543 ;
    skos:altLabel "GDE"@en ;
    skos:prefLabel "GasDiffusionElectrode"@en ;
    emmo:EMMO_26bf1bef_d192_4da6_b0eb_d2209698fb54 "https://www.wikidata.org/wiki/Q909759" ;
    emmo:EMMO_50c298c2_55a2_4068_b3ac_4e948c33181f "https://www.electropedia.org/iev/iev.nsf/display?openform&ievref=485-02-02" ;
    emmo:EMMO_967080e5_2f42_4eb2_a3a9_c58143e835f9 "a type of electrode specifically designed for gaseous reactants or products or both"@en ;
    emmo:EMMO_c7b62dd7_063a_4c2a_8504_42f7264ba83f "A gas diffusion electrode usually comprises one or more porous layers, like the gas diffusion layer and the catalyst layer."@en,
        "Gas diffusion electrodes can be gas diffusion anodes or gas diffusion cathodes."@en,
        "Gas diffusion electrodes can be used in batteries, fuel cells, and electrolyzers."@en ;
    emmo:EMMO_c84c6752_6d64_48cc_9500_e54a3c34898d "https://en.wikipedia.org/wiki/Gas_diffusion_electrode"@en .

:electrochemistry_dc205ac2_314e_415c_a2b6_b12e8359d54c a owl:Class ;
    rdfs:label "NearNeutralElectrolyte"@en ;
    rdfs:comment "an aqueous electrolyte with a nominal pH value between 4 and 10."@en ;
    rdfs:subClassOf :electrochemistry_b812e9d0_7c58_4455_b3e7_6847f10c8e8a ;
    skos:altLabel "NearNeutralAqueousElectrolyte"@en,
        "NearNeutralSolution"@en ;
    skos:prefLabel "NearNeutralElectrolyte"@en ;
    emmo:EMMO_967080e5_2f42_4eb2_a3a9_c58143e835f9 "an aqueous electrolyte with a nominal pH value between 4 and 10."@en ;
    emmo:EMMO_c7b62dd7_063a_4c2a_8504_42f7264ba83f "this covers the pH domain typically described as \"weakly acidic\", \"neutral\", and \"weakly alkaline\""@en .

:electrochemistry_e931087f_7681_4096_b200_5223bcc47eb4 a owl:Class ;
    rdfs:label "ElectrolyticCell"@en ;
    rdfs:comment "electrochemical cell intended to produce chemical reactions"@en ;
    rdfs:subClassOf :electrochemistry_6f2c88c9_5c04_4953_a298_032cc3ab9b77 ;
    skos:prefLabel "ElectrolyticCell"@en ;
    emmo:EMMO_26bf1bef_d192_4da6_b0eb_d2209698fb54 "https://www.wikidata.org/wiki/Q2608426" ;
    emmo:EMMO_50c298c2_55a2_4068_b3ac_4e948c33181f "https://www.electropedia.org/iev/iev.nsf/display?openform&ievref=114-03-06"@en ;
    emmo:EMMO_6dd685dd_1895_46e4_b227_be9f7d643c25 "https://dbpedia.org/page/Electrolytic_cell"@en ;
    emmo:EMMO_967080e5_2f42_4eb2_a3a9_c58143e835f9 "electrochemical cell intended to produce chemical reactions"@en ;
    emmo:EMMO_c7b62dd7_063a_4c2a_8504_42f7264ba83f "An electrochemical cell that requires input of work to drive the reaction."@en,
        "Electrochemical cell in which electrical energy is converted into chemical energy."@en ;
    emmo:EMMO_c84c6752_6d64_48cc_9500_e54a3c34898d "https://en.wikipedia.org/wiki/Electrolytic_cell"@en .

:electrochemistry_f78e3c87_01c6_4cc2_b047_30322262e22d a owl:Class ;
    rdfs:label "InterfacialRegion"@en ;
    rdfs:comment "a 3D spatial region at an interface with physical properties that are distinct from the bulk phases in contact"@en ;
    rdfs:seeAlso "https://doi.org/10.1002/admi.202101865"@en ;
    rdfs:subClassOf emmo:EMMO_fcae603e_aa6e_4940_9fa1_9f0909cabf3b ;
    skos:prefLabel "InterfacialRegion"@en ;
    emmo:EMMO_157fdf31_6387_42be_8e72_10530519214a "https://raw.githubusercontent.com/emmo-repo/domain-electrochemistry/dev/docs/assets/img/fig/png/InterfacialRegion.png" ;
    emmo:EMMO_967080e5_2f42_4eb2_a3a9_c58143e835f9 "a 3D spatial region at an interface with physical properties that are distinct from the bulk phases in contact"@en .

:electrochemistry_fb988878_ee54_4350_9ee9_228c00c3ad35 a owl:Class ;
    rdfs:label "WorkingElectrode"@en ;
    rdfs:comment "electrode at which one or more electroactive substances undergo reaction in the solution being investigated"@en ;
    rdfs:subClassOf :electrochemistry_0f007072_a8dd_4798_b865_1bf9363be627 ;
    skos:prefLabel "WorkingElectrode"@en ;
    skos:related :electrochemistry_7729c34e_1ae9_403d_b933_1765885e7f29,
        :electrochemistry_871bc4a4_2d17_4b88_9b0f_7ab85f14afea ;
    emmo:EMMO_26bf1bef_d192_4da6_b0eb_d2209698fb54 "https://www.wikidata.org/wiki/Q477099" ;
    emmo:EMMO_967080e5_2f42_4eb2_a3a9_c58143e835f9 "electrode at which one or more electroactive substances undergo reaction in the solution being investigated"@en ;
    emmo:EMMO_c7b62dd7_063a_4c2a_8504_42f7264ba83f "If processes of interest occur both at the anode and the cathode of a cell (as in differential amperometry or controlled-current potentiometric titration with two indicator electrodes), the cell should be said to comprise two indicator or working electrodes."@en,
        "Te potential of a working electrode is controlled with respect to the reference electrode."@en,
        "This term is typically used in voltammetry, polarography, amperometry, and coulometry."@en ;
    emmo:EMMO_c84c6752_6d64_48cc_9500_e54a3c34898d "https://en.wikipedia.org/wiki/Working_electrode"@en ;
    emmo:EMMO_fe015383_afb3_44a6_ae86_043628697aa2 "https://goldbook.iupac.org/terms/view/W06686"@en .

:electrochemistry_1586ef26_6d30_49e3_ae32_b4c9fc181941 a owl:Class ;
    rdfs:label "FormFactor"@en ;
    rdfs:comment "a sign that is used to indicate the shape of the case of an electrochemical device"@en ;
    rdfs:subClassOf emmo:EMMO_64c72d00_7582_44ea_a0b5_3a14e50acc36 ;
    skos:prefLabel "FormFactor"@en ;
    emmo:EMMO_967080e5_2f42_4eb2_a3a9_c58143e835f9 "a sign that is used to indicate the shape of the case of an electrochemical device"@en .

:electrochemistry_3bd08946_4e81_455d_9fca_dc7a5ead9315 a owl:ObjectProperty ;
    rdfs:label "hasElectrolyte"@en ;
    rdfs:comment "relates an electrochemical cell or system to the electrolyte that enables ionic conduction between electrodes"@en ;
    rdfs:domain :electrochemistry_6f2c88c9_5c04_4953_a298_032cc3ab9b77 ;
    rdfs:range emmo:EMMO_bc37743c_37c4_4ec7_9d58_d1aae5567352 ;
    rdfs:subPropertyOf emmo:EMMO_3c7f239f_e833_4a2b_98a1_c88831770c1b ;
    skos:prefLabel "hasElectrolyte"@en ;
    emmo:EMMO_967080e5_2f42_4eb2_a3a9_c58143e835f9 "relates an electrochemical cell or system to the electrolyte that enables ionic conduction between electrodes"@en .

:electrochemistry_4839708a_3864_47eb_b719_373ff8874c61 a owl:Class ;
    rdfs:label "BimetallicOxideElectrode"@en ;
    rdfs:comment "an electrode consisting of two metal oxide active materials"@en ;
    rdfs:subClassOf :electrochemistry_5186239a_2af7_4dbf_92ca_22e8e583c528,
        :electrochemistry_e4b6cb36_4dac_49e3_871d_40bcfca943a5 ;
    skos:prefLabel "BimetallicOxideElectrode"@en ;
    emmo:EMMO_967080e5_2f42_4eb2_a3a9_c58143e835f9 "an electrode consisting of two metal oxide active materials"@en .

:electrochemistry_9c557caa_61e2_4fa9_a517_4bad01a68122 a owl:Class ;
    rdfs:label "TitaniumBasedElectrode"@en ;
    rdfs:comment "an electrode in which the primary active material consists of titanium or titanium compounds"@en ;
    rdfs:subClassOf :electrochemistry_9a823d64_9d10_4a29_9cbd_9bbdad7985bc ;
    skos:prefLabel "TitaniumBasedElectrode"@en ;
    emmo:EMMO_967080e5_2f42_4eb2_a3a9_c58143e835f9 "an electrode in which the primary active material consists of titanium or titanium compounds"@en ;
    emmo:EMMO_c7b62dd7_063a_4c2a_8504_42f7264ba83f "often represented in cell designations by the letter T"@en,
        "this class is intended to enable designations based on IEC recommendations"@en .

:electrochemistry_a0a619d7_da95_41f0_8bc3_9c19d636d543 a owl:Class ;
    rdfs:label "InertElectrode"@en ;
    rdfs:comment "electrode that serves only as a source or sink for electrons without playing a chemical role in the electrode reaction"@en ;
    rdfs:subClassOf :electrochemistry_0f007072_a8dd_4798_b865_1bf9363be627 ;
    skos:prefLabel "InertElectrode"@en ;
    emmo:EMMO_26bf1bef_d192_4da6_b0eb_d2209698fb54 "https://www.wikidata.org/wiki/Q120907475" ;
    emmo:EMMO_50c298c2_55a2_4068_b3ac_4e948c33181f "https://www.electropedia.org/iev/iev.nsf/display?openform&ievref=114-02-08"@en ;
    emmo:EMMO_967080e5_2f42_4eb2_a3a9_c58143e835f9 "electrode that serves only as a source or sink for electrons without playing a chemical role in the electrode reaction"@en ;
    emmo:EMMO_c7b62dd7_063a_4c2a_8504_42f7264ba83f "Noble metals, mercury, and carbon are typically used as (nearly) inert electrodes."@en .

:electrochemistry_aff732a9_238a_4734_977c_b2ba202af126 a owl:Class ;
    rdfs:label "PositiveElectrode"@en ;
    rdfs:comment "for a device having two electrodes, that electrode having the higher electric potential"@en ;
    rdfs:subClassOf :electrochemistry_0f007072_a8dd_4798_b865_1bf9363be627 ;
    skos:altLabel "PositivePlate"@en ;
    skos:prefLabel "PositiveElectrode"@en ;
    skos:related :electrochemistry_35c650ab_3b23_4938_b312_1b0dede2e6d5,
        :electrochemistry_c94c041b_8ea6_43e7_85cc_d2bce7785b4c ;
    emmo:EMMO_0fa6566e_500f_4d24_baa9_b2b22c9a0b72 "The term \"cathode\" is often used interchangably with \"positive electrode\" even though it only applies while the cell is being discharged. When the cell is being charged the positive electrode becomes the anode."@en ;
    emmo:EMMO_26bf1bef_d192_4da6_b0eb_d2209698fb54 "https://www.wikidata.org/wiki/Q120907518" ;
    emmo:EMMO_50c298c2_55a2_4068_b3ac_4e948c33181f "https://www.electropedia.org/iev/iev.nsf/display?openform&ievref=151-13-05",
        "https://www.electropedia.org/iev/iev.nsf/display?openform&ievref=482-02-06" ;
    emmo:EMMO_967080e5_2f42_4eb2_a3a9_c58143e835f9 "for a device having two electrodes, that electrode having the higher electric potential"@en ;
    emmo:EMMO_c7b62dd7_063a_4c2a_8504_42f7264ba83f "by convention, a reduction reaction occurs during discharge"@en .

:electrochemistry_c94c041b_8ea6_43e7_85cc_d2bce7785b4c a owl:Class ;
    rdfs:label "NegativeElectrode"@en ;
    rdfs:comment "for a device having two electrodes, that electrode having the lower electric potential"@en ;
    rdfs:subClassOf :electrochemistry_0f007072_a8dd_4798_b865_1bf9363be627 ;
    skos:altLabel "NegativePlate"@en ;
    skos:note "by convention, an oxidation reaction occurs during discharge"@en ;
    skos:prefLabel "NegativeElectrode"@en ;
    skos:related :electrochemistry_aff732a9_238a_4734_977c_b2ba202af126,
        :electrochemistry_b6319c74_d2ce_48c0_a75a_63156776b302 ;
    emmo:EMMO_0fa6566e_500f_4d24_baa9_b2b22c9a0b72 "The term \"anode\" is often used interchangably with \"negative electrode\" even though it only applies while the cell is being discharged. When the cell is being charged the negatve electrode becomes the cathode."@en ;
    emmo:EMMO_26bf1bef_d192_4da6_b0eb_d2209698fb54 "https://www.wikidata.org/wiki/Q120907506" ;
    emmo:EMMO_50c298c2_55a2_4068_b3ac_4e948c33181f "https://www.electropedia.org/iev/iev.nsf/display?openform&ievref=151-13-04",
        "https://www.electropedia.org/iev/iev.nsf/display?openform&ievref=482-02-05" ;
    emmo:EMMO_967080e5_2f42_4eb2_a3a9_c58143e835f9 "for a device having two electrodes, that electrode having the lower electric potential"@en .

:electrochemistry_331e6cca_f260_4bf8_af55_35304fe1bbe0 a owl:Class ;
    rdfs:label "Separator"@en ;
    rdfs:comment "in an electrochemical cell, device made of insulating material permeable to the ions of the electrolyte and prohibiting totally or partially the mixing of the substances on both sides."@en ;
    rdfs:subClassOf [ a owl:Restriction ;
            owl:onProperty emmo:EMMO_e1097637_70d2_4895_973f_2396f04fa204 ;
            owl:someValuesFrom emmo:EMMO_3a6578ac_aee0_43b9_9bc6_1eb208c8c9a9 ],
        [ a owl:Restriction ;
            owl:onProperty emmo:EMMO_e1097637_70d2_4895_973f_2396f04fa204 ;
            owl:someValuesFrom emmo:EMMO_43003c86_9d15_433b_9789_ee2940920656 ],
        :electrochemistry_b5ea31c9_bb10_4276_980e_c3eceb1efc82 ;
    skos:altLabel "ElectrochemicalSeparator"@en ;
    skos:prefLabel "Separator"@en ;
    emmo:EMMO_26bf1bef_d192_4da6_b0eb_d2209698fb54 "https://www.wikidata.org/wiki/Q1718181" ;
    emmo:EMMO_50c298c2_55a2_4068_b3ac_4e948c33181f "https://www.electropedia.org/iev/iev.nsf/display?openform&ievref=482-02-11",
        "https://www.electropedia.org/iev/iev.nsf/display?openform&ievref=114-03-17"@en ;
    emmo:EMMO_967080e5_2f42_4eb2_a3a9_c58143e835f9 "in an electrochemical cell, device made of insulating material permeable to the ions of the electrolyte and prohibiting totally or partially the mixing of the substances on both sides."@en ;
    emmo:EMMO_c7b62dd7_063a_4c2a_8504_42f7264ba83f "Membranes and diaphragms are special forms of electrochemical separators."@en ;
    emmo:EMMO_c84c6752_6d64_48cc_9500_e54a3c34898d "https://en.wikipedia.org/wiki/Separator_(electricity)"@en .

:electrochemistry_35c650ab_3b23_4938_b312_1b0dede2e6d5 a owl:Class ;
    rdfs:label "Cathode"@en ;
    rdfs:comment "by convention, cell electrode at which, a reduction reaction occurs"@en ;
    rdfs:subClassOf :electrochemistry_0f007072_a8dd_4798_b865_1bf9363be627 ;
    skos:note "The cathode is the positive electrode during discharge and the negative electrode during charge."@en ;
    skos:prefLabel "Cathode"@en ;
    skos:related :electrochemistry_6f2c88c9_5c04_4953_a298_032cc3ab9b77,
        :electrochemistry_aff732a9_238a_4734_977c_b2ba202af126,
        :electrochemistry_b6319c74_d2ce_48c0_a75a_63156776b302,
        :electrochemistry_f4a1323a_ce2b_4c1a_b89d_c80170110ed6 ;
    emmo:EMMO_0fa6566e_500f_4d24_baa9_b2b22c9a0b72 "The term \"cathode\" is often used interchangably with \"positive electrode\" even though it only applies while the cell is being discharged. When the cell is being charged the negative electrode becomes the cathode."@en ;
    emmo:EMMO_26bf1bef_d192_4da6_b0eb_d2209698fb54 "https://www.wikidata.org/wiki/Q175233" ;
    emmo:EMMO_4c8480cf_56de_41da_8699_f12a9033313a "IEC and IUPAC recommend defining anode/cathode by oxidation/reduction rather than by polarity or charge sign."@en ;
    emmo:EMMO_50c298c2_55a2_4068_b3ac_4e948c33181f "https://www.electropedia.org/iev/iev.nsf/display?openform&ievref=151-13-03",
        "https://www.electropedia.org/iev/iev.nsf/display?openform&ievref=482-02-28" ;
    emmo:EMMO_6dd685dd_1895_46e4_b227_be9f7d643c25 "https://dbpedia.org/page/Cathode"@en ;
    emmo:EMMO_705f27ae_954c_4f13_98aa_18473fc52b25 "From Greek kathodos (way down). Intended to name the electrode on the downward path of current by convention; in modern usage the site of reduction. Coined by Michael Faraday with support from William Whewell and Whitlock Nicholl."@en ;
    emmo:EMMO_967080e5_2f42_4eb2_a3a9_c58143e835f9 "by convention, cell electrode at which, a reduction reaction occurs"@en ;
    emmo:EMMO_c84c6752_6d64_48cc_9500_e54a3c34898d "https://en.wikipedia.org/wiki/Cathode"@en ;
    emmo:EMMO_fe015383_afb3_44a6_ae86_043628697aa2 "https://goldbook.iupac.org/terms/view/C00905"@en .

:electrochemistry_8a1c9a7b_978c_4421_a9c1_d0b07b42aab9 a owl:Class ;
    rdfs:label "ChemicalReaction"@en ;
    rdfs:comment "a process that results in the interconversion of chemical species"@en ;
    rdfs:seeAlso :electrochemistry_d7f8cab9_b035_4ecd_be63_292672572526,
        :electrochemistry_e2514bf9_d012_4990_b68b_6f37443f18f6 ;
    rdfs:subClassOf [ a owl:Restriction ;
            owl:onProperty emmo:EMMO_36e69413_8c59_4799_946c_10b05d266e22 ;
            owl:someValuesFrom emmo:EMMO_cbcf8fe6_6da6_49e0_ab4d_00f737ea9689 ],
        [ a owl:Restriction ;
            owl:onProperty emmo:EMMO_c4bace1d_4db0_4cd3_87e9_18122bae2840 ;
            owl:someValuesFrom emmo:EMMO_cbcf8fe6_6da6_49e0_ab4d_00f737ea9689 ],
        emmo:EMMO_135ab8ea_e028_439e_be64_3e0f9734ea2b ;
    skos:prefLabel "ChemicalReaction"@en ;
    emmo:EMMO_26bf1bef_d192_4da6_b0eb_d2209698fb54 "https://www.wikidata.org/wiki/Q36534" ;
    emmo:EMMO_967080e5_2f42_4eb2_a3a9_c58143e835f9 "a process that results in the interconversion of chemical species"@en ;
    emmo:EMMO_c84c6752_6d64_48cc_9500_e54a3c34898d "https://en.wikipedia.org/wiki/Chemical_reaction"@en ;
    emmo:EMMO_fe015383_afb3_44a6_ae86_043628697aa2 "https://doi.org/10.1351/goldbook.C01033"@en .

:electrochemistry_92147e31_d015_4889_a092_04fbab033f15 a owl:Class ;
    rdfs:label "CoatedElectrode"@en ;
    rdfs:comment "cell electrode consisting of a current collector and active material"@en ;
    rdfs:subClassOf [ a owl:Restriction ;
            owl:onProperty :electrochemistry_4df9926d_d4f2_4955_93f3_a03c5edc5383 ;
            owl:someValuesFrom :electrochemistry_403c300e_09b9_400b_943b_04e82a3cfb56 ],
        [ a owl:Restriction ;
            owl:onProperty :electrochemistry_cc8c2c5d_cf3d_444d_a7e8_44ec4c06a88e ;
            owl:someValuesFrom :electrochemistry_212af058_3bbb_419f_a9c6_90ba9ebb3706 ],
        :electrochemistry_0f007072_a8dd_4798_b865_1bf9363be627 ;
    skos:altLabel "Plate"@en ;
    skos:prefLabel "CoatedElectrode"@en ;
    emmo:EMMO_157fdf31_6387_42be_8e72_10530519214a "https://raw.githubusercontent.com/emmo-repo/domain-electrochemistry/dev/docs/assets/img/fig/png/CoatedElectrode.png" ;
    emmo:EMMO_50c298c2_55a2_4068_b3ac_4e948c33181f "https://www.electropedia.org/iev/iev.nsf/display?openform&ievref=482-02-02"@en ;
    emmo:EMMO_967080e5_2f42_4eb2_a3a9_c58143e835f9 "cell electrode consisting of a current collector and active material"@en .

:electrochemistry_b6319c74_d2ce_48c0_a75a_63156776b302 a owl:Class ;
    rdfs:label "Anode"@en ;
    rdfs:comment "by convention, cell electrode at which an oxidation reaction occurs"@en ;
    rdfs:subClassOf :electrochemistry_0f007072_a8dd_4798_b865_1bf9363be627 ;
    skos:note "The anode is the negative electrode during discharge and the positive electrode during charge."@en ;
    skos:prefLabel "Anode"@en ;
    skos:related :electrochemistry_35c650ab_3b23_4938_b312_1b0dede2e6d5,
        :electrochemistry_6f2c88c9_5c04_4953_a298_032cc3ab9b77,
        :electrochemistry_a0580fa9_5073_44af_b33e_7adbc83892d0,
        :electrochemistry_c94c041b_8ea6_43e7_85cc_d2bce7785b4c ;
    emmo:EMMO_0fa6566e_500f_4d24_baa9_b2b22c9a0b72 "The term \"anode\" is often used interchangably with \"negative electrode\" even though it only applies while the cell is being discharged. When the cell is being charged the positive electrode becomes the anode."@en ;
    emmo:EMMO_26bf1bef_d192_4da6_b0eb_d2209698fb54 "https://www.wikidata.org/wiki/Q181232"@en ;
    emmo:EMMO_4c8480cf_56de_41da_8699_f12a9033313a "IEC and IUPAC recommend defining anode/cathode by oxidation/reduction rather than by polarity or charge sign."@en ;
    emmo:EMMO_50c298c2_55a2_4068_b3ac_4e948c33181f "https://www.electropedia.org/iev/iev.nsf/display?openform&ievref=482-02-27" ;
    emmo:EMMO_6dd685dd_1895_46e4_b227_be9f7d643c25 "https://dbpedia.org/page/Anode"@en ;
    emmo:EMMO_705f27ae_954c_4f13_98aa_18473fc52b25 "From Greek anodos (way up). Chosen to denote the electrode associated with the upward path of current by convention; later anchored by usage to the site of oxidation.Coined by Michael Faraday with guidance from William Whewell and Whitlock Nicholl."@en ;
    emmo:EMMO_967080e5_2f42_4eb2_a3a9_c58143e835f9 "by convention, cell electrode at which an oxidation reaction occurs"@en ;
    emmo:EMMO_c84c6752_6d64_48cc_9500_e54a3c34898d "https://en.wikipedia.org/wiki/Anode"@en ;
    emmo:EMMO_fe015383_afb3_44a6_ae86_043628697aa2 "https://goldbook.iupac.org/terms/view/A00370"@en .

:electrochemistry_f4a1323a_ce2b_4c1a_b89d_c80170110ed6 a owl:Class ;
    rdfs:label "CathodicReaction"@en ;
    rdfs:comment "electrode reaction in which reduction  occurs at the cathode"@en ;
    rdfs:subClassOf :electrochemistry_109a38d4_daaa_4748_a803_044fb7c97673,
        :electrochemistry_2e3e14f9_4cb8_45b2_908e_47eec893dec8 ;
    skos:altLabel "Electroreduction"@en,
        "ElectroreductionReaction"@en ;
    skos:prefLabel "CathodicReaction"@en ;
    skos:related :electrochemistry_35c650ab_3b23_4938_b312_1b0dede2e6d5,
        :electrochemistry_a0580fa9_5073_44af_b33e_7adbc83892d0 ;
    emmo:EMMO_50c298c2_55a2_4068_b3ac_4e948c33181f "https://www.electropedia.org/iev/iev.nsf/display?openform&ievref=482-03-12",
        "https://www.electropedia.org/iev/iev.nsf/display?openform&ievref=114-02-10"@en ;
    emmo:EMMO_967080e5_2f42_4eb2_a3a9_c58143e835f9 "electrode reaction in which reduction  occurs at the cathode"@en ;
    emmo:EMMO_c7b62dd7_063a_4c2a_8504_42f7264ba83f "electrode reaction involving an electrochemical reduction"@en,
        "electrode reaction, where the energy of electrons in the working electrode is higher than the LUMO orbital of the substrate"@en .

:electrochemistry_0d2aaaf4_1a8a_4a32_abd8_7d0fdf0ae9d2 a owl:Class ;
    rdfs:label "NickelBasedElectrode"@en ;
    rdfs:comment "an electrode in which the primary active material consists of nickel or nickel compounds"@en ;
    rdfs:subClassOf :electrochemistry_9a823d64_9d10_4a29_9cbd_9bbdad7985bc ;
    skos:prefLabel "NickelBasedElectrode"@en ;
    emmo:EMMO_967080e5_2f42_4eb2_a3a9_c58143e835f9 "an electrode in which the primary active material consists of nickel or nickel compounds"@en ;
    emmo:EMMO_c7b62dd7_063a_4c2a_8504_42f7264ba83f "often represented in IEC cell designations by the letter N"@en,
        "this class is intended to enable designations based on IEC recommendations"@en .

:electrochemistry_1aec4cc0_82d5_4042_a657_ed7fe291c3d8 a owl:Class ;
    rdfs:label "Case"@en ;
    rdfs:comment "container for the plate pack or packs and electrolyte of a cell or cells made of a material impervious to the electrolyte"@en ;
    rdfs:subClassOf :electrochemistry_b5ea31c9_bb10_4276_980e_c3eceb1efc82 ;
    skos:altLabel "Can"@en,
        "Container"@en,
        "Housing"@en ;
    skos:prefLabel "Case"@en ;
    emmo:EMMO_50c298c2_55a2_4068_b3ac_4e948c33181f "https://www.electropedia.org/iev/iev.nsf/display?openform&ievref=482-02-14" ;
    emmo:EMMO_967080e5_2f42_4eb2_a3a9_c58143e835f9 "container for the plate pack or packs and electrolyte of a cell or cells made of a material impervious to the electrolyte"@en .

:electrochemistry_578c41e9_ee01_4840_9c8c_04ab6e4e6241 a owl:ObjectProperty ;
    rdfs:label "hasElectrode"@en ;
    rdfs:comment "relates an electrochemical cell or subsystem to an electrode that participates in electron transfer reactions"@en ;
    rdfs:range :electrochemistry_0f007072_a8dd_4798_b865_1bf9363be627 ;
    rdfs:subPropertyOf emmo:EMMO_3c7f239f_e833_4a2b_98a1_c88831770c1b ;
    skos:prefLabel "hasElectrode"@en ;
    emmo:EMMO_967080e5_2f42_4eb2_a3a9_c58143e835f9 "relates an electrochemical cell or subsystem to an electrode that participates in electron transfer reactions"@en .

:electrochemistry_ac9723d1_bac0_4109_874e_32849de9299b a owl:Class ;
    rdfs:label "DoubleLayerModel"@en ;
    rdfs:comment "model representing the structure of an electrolyte at an electrode-electrolyte interface by a rigid layer formed by the charge carriers on the surface of the electrode and a diffuse layer formed by mobile ions in the electrolyte."@en ;
    rdfs:subClassOf emmo:EMMO_d7788d1a_020d_4c78_85a1_13563fcec168 ;
    skos:altLabel "ElectricalDoubleLayerModel"@en,
        "ElectricalPolarizationLayerModel"@en ;
    skos:prefLabel "DoubleLayerModel"@en ;
    emmo:EMMO_50c298c2_55a2_4068_b3ac_4e948c33181f "https://www.electropedia.org/iev/iev.nsf/display?openform&ievref=114-02-19" ;
    emmo:EMMO_967080e5_2f42_4eb2_a3a9_c58143e835f9 "model representing the structure of an electrolyte at an electrode-electrolyte interface by a rigid layer formed by the charge carriers on the surface of the electrode and a diffuse layer formed by mobile ions in the electrolyte."@en ;
    emmo:EMMO_c84c6752_6d64_48cc_9500_e54a3c34898d "https://en.wikipedia.org/wiki/Double_layer_(surface_science)"@en .

:electrochemistry_757eae08_4d43_42d4_8b4e_8a0bfd2f9a1c a owl:Class ;
    rdfs:label "InsertionElectrode"@en ;
    rdfs:comment "an electrode at which the predominant electrochemical reaction includes an insertion (intercalation) step"@en ;
    rdfs:subClassOf [ a owl:Restriction ;
            owl:onProperty :electrochemistry_fd1fae29_a182_4692_98b8_919764b07b00 ;
            owl:someValuesFrom emmo:EMMO_21205421_5783_4d3e_81e5_10c5d894a88a ],
        :electrochemistry_9a823d64_9d10_4a29_9cbd_9bbdad7985bc ;
    skos:altLabel "IntercalationElectrode"@en ;
    skos:prefLabel "InsertionElectrode"@en ;
    emmo:EMMO_967080e5_2f42_4eb2_a3a9_c58143e835f9 "an electrode at which the predominant electrochemical reaction includes an insertion (intercalation) step"@en .

:electrochemistry_7729c34e_1ae9_403d_b933_1765885e7f29 a owl:Class ;
    rdfs:label "ReferenceElectrode"@en ;
    rdfs:comment "Electrode with a well-defined and constant equilibrium potential with respect to which it is possible to measure or calculate electrode potentials of other electrodes by including them in an appropriate electrochemical cell."@en ;
    rdfs:subClassOf :electrochemistry_9f466223_e20a_474d_ac4d_6d4b6131c275 ;
    skos:example "The standard hydrogen electrode represents the primary standard in electrochemistry. Elec- trodes of the 2nd kind, such as Ag | AgCl, Hg | Hg2, Cl2, Hg | Hg2SO4, and Hg | HgO, can be used as reference electrodes in aqueous solutions containing ions Cl^{}, SO_4^{2}, and OH^{}, respectively."@en ;
    skos:prefLabel "ReferenceElectrode"@en ;
    skos:related :electrochemistry_871bc4a4_2d17_4b88_9b0f_7ab85f14afea,
        :electrochemistry_fb988878_ee54_4350_9ee9_228c00c3ad35 ;
    emmo:EMMO_26bf1bef_d192_4da6_b0eb_d2209698fb54 "https://www.wikidata.org/wiki/Q653954" ;
    emmo:EMMO_50c298c2_55a2_4068_b3ac_4e948c33181f "https://www.electropedia.org/iev/iev.nsf/display?openform&ievref=114-03-15"@en ;
    emmo:EMMO_967080e5_2f42_4eb2_a3a9_c58143e835f9 "Electrode with a well-defined and constant equilibrium potential with respect to which it is possible to measure or calculate electrode potentials of other electrodes by including them in an appropriate electrochemical cell."@en ;
    emmo:EMMO_c7b62dd7_063a_4c2a_8504_42f7264ba83f "Electrode that maintains an essentially constant potential under the conditions prevailing in an electrochemical measurement, and that serves for observation, measurement, or control of the potential of the indicator or working electrode."@en,
        "In potentiometry, under zero current condition, the essentially constant potential is achieved by ensuring a constant composition of solution in contact with the electrode forming a half-cell. Practical reference half-cells are generally non-polarizable electrodes of the 2nd kind (metal | insoluble salt | ion), constructed so that their electrolyte solutions serve as salt bridges to the solutions under investigation."@en,
        "Double junction reference electrodes are recommended when the reference electrolyte contains interfering components."@en ;
    emmo:EMMO_c84c6752_6d64_48cc_9500_e54a3c34898d "https://en.wikipedia.org/wiki/Reference_electrode"@en ;
    emmo:EMMO_fe015383_afb3_44a6_ae86_043628697aa2 "https://goldbook.iupac.org/terms/view/R05229"@en .

:electrochemistry_6f2c88c9_5c04_4953_a298_032cc3ab9b77 a owl:Class ;
    rdfs:label "ElectrochemicalCell"@en ;
    rdfs:comment "system containing two electrodes that allow transport of electrons, separated by an electrolyte that allows movement of ions but blocks movement of electrons"@en ;
    rdfs:seeAlso :electrochemistry_0acd0fc2_1048_4604_8e90_bf4e84bd87df ;
    rdfs:subClassOf [ a owl:Restriction ;
            owl:onProperty :electrochemistry_3bd08946_4e81_455d_9fca_dc7a5ead9315 ;
            owl:someValuesFrom emmo:EMMO_bc37743c_37c4_4ec7_9d58_d1aae5567352 ],
        [ a owl:Restriction ;
            owl:onProperty :electrochemistry_578c41e9_ee01_4840_9c8c_04ab6e4e6241 ;
            owl:someValuesFrom :electrochemistry_0f007072_a8dd_4798_b865_1bf9363be627 ],
        [ a owl:Restriction ;
            owl:onProperty :electrochemistry_5d299271_3f68_494f_ab96_3db9acdd3138 ;
            owl:someValuesFrom :electrochemistry_0f007072_a8dd_4798_b865_1bf9363be627 ],
        [ a owl:Restriction ;
            owl:onProperty :electrochemistry_5eb197ea_0c3e_4ea2_8392_81152ee91515 ;
            owl:someValuesFrom :electrochemistry_0f007072_a8dd_4798_b865_1bf9363be627 ],
        [ a owl:Restriction ;
            owl:onProperty :electrochemistry_8e9cf965_9f92_46e8_b678_b50410ce3616 ;
            owl:someValuesFrom :electrochemistry_0f007072_a8dd_4798_b865_1bf9363be627 ],
        [ a owl:Restriction ;
            owl:onProperty :electrochemistry_c76dbfeb_f3d9_44d4_9cbe_0946924f311f ;
            owl:someValuesFrom :electrochemistry_0f007072_a8dd_4798_b865_1bf9363be627 ],
        [ a owl:Restriction ;
            owl:onProperty :electrochemistry_e08d43cf_93e4_49c6_bcb6_472be52ae7fc ;
            owl:someValuesFrom :electrochemistry_0f007072_a8dd_4798_b865_1bf9363be627 ],
        [ a owl:Restriction ;
            owl:onProperty :electrochemistry_1f2d401c_eede_4178_9ff5_e5392bc2cb92 ;
            owl:someValuesFrom xsd:string ],
        [ a owl:Restriction ;
            owl:onProperty :electrochemistry_eac15067_9594_4eab_a440_b537b0fd2075 ;
            owl:someValuesFrom xsd:string ],
        emmo:EMMO_b9522e56_1fac_4766_97e6_428605fabd3e ;
    skos:note "composite system in which the supplied electric energy mainly produces chemical reactions or, conversely, in which the energy released by chemical reactions is mainly delivered by the system as electric energy"@en ;
    skos:prefLabel "ElectrochemicalCell"@en ;
    skos:related :electrochemistry_0acd0fc2_1048_4604_8e90_bf4e84bd87df,
        :electrochemistry_0f007072_a8dd_4798_b865_1bf9363be627,
        :electrochemistry_fb0d9eef_92af_4628_8814_e065ca255d59 ;
    skos:scopeNote "It is important to distinguish between the conceptual electrochemical cell and the electrochemical device used in practice."@en ;
    emmo:EMMO_0fa6566e_500f_4d24_baa9_b2b22c9a0b72 "Do not confuse the physical 'cell' with the manufactured 'device' that embeds it."@en ;
    emmo:EMMO_157fdf31_6387_42be_8e72_10530519214a "https://raw.githubusercontent.com/emmo-repo/domain-electrochemistry/dev/docs/assets/img/fig/png/ElectrochemicalCell.png" ;
    emmo:EMMO_26bf1bef_d192_4da6_b0eb_d2209698fb54 "https://www.wikidata.org/wiki/Q80097" ;
    emmo:EMMO_50c298c2_55a2_4068_b3ac_4e948c33181f "https://www.electropedia.org/iev/iev.nsf/display?openform&ievref=114-03-01"@en ;
    emmo:EMMO_5f7abc2a_5b50_41c3_8def_c8ba7c3b083e "Model each electrode, electrolyte, and interface explicitly to represent charge transport correctly in simulations or ontological mappings."@en ;
    emmo:EMMO_6dd685dd_1895_46e4_b227_be9f7d643c25 "http://dbpedia.org:8891/page/Electrochemical_cell" ;
    emmo:EMMO_967080e5_2f42_4eb2_a3a9_c58143e835f9 "system containing two electrodes that allow transport of electrons, separated by an electrolyte that allows movement of ions but blocks movement of electrons"@en ;
    emmo:EMMO_b6730304_cabc_4104_b415_14218466445c "Terminology varies across disciplines; in some contexts 'cell' may refer to the assembled device rather than the electrochemical unit of reaction."@en ;
    emmo:EMMO_c84c6752_6d64_48cc_9500_e54a3c34898d "https://en.wikipedia.org/wiki/Electrochemical_cell"@en .

:electrochemistry_b1cf9fee_2164_4f95_8204_90f717373a8a a owl:Class ;
    rdfs:label "CylindricalCase"@en ;
    rdfs:comment "a round-type case with a height that is greater than or equal to the diameter"@en ;
    rdfs:subClassOf :electrochemistry_eacb141f_6ab4_491f_8603_a3e025cefc82 ;
    skos:prefLabel "CylindricalCase"@en ;
    emmo:EMMO_967080e5_2f42_4eb2_a3a9_c58143e835f9 "a round-type case with a height that is greater than or equal to the diameter"@en .

:electrochemistry_fb0d9eef_92af_4628_8814_e065ca255d59 a owl:Class ;
    rdfs:label "Electrolyte"@en ;
    rdfs:comment "a material in which the mobile species are ions and free movement of electrons is blocked."@en ;
    rdfs:subClassOf [ a owl:Restriction ;
            owl:onProperty emmo:EMMO_e1097637_70d2_4895_973f_2396f04fa204 ;
            owl:someValuesFrom :electrochemistry_25dabdc2_68bf_4a38_8cbe_11be017358bc ],
        :electrochemistry_b5ea31c9_bb10_4276_980e_c3eceb1efc82,
        :electrochemistry_ebdb68e9_c4b5_4d57_a042_c0f51d446755 ;
    skos:prefLabel "Electrolyte"@en ;
    emmo:EMMO_26bf1bef_d192_4da6_b0eb_d2209698fb54 "https://www.wikidata.org/wiki/Q162908" ;
    emmo:EMMO_50c298c2_55a2_4068_b3ac_4e948c33181f "https://www.electropedia.org/iev/iev.nsf/display?openform&ievref=114-01-02",
        "https://www.electropedia.org/iev/iev.nsf/display?openform&ievref=482-02-29" ;
    emmo:EMMO_6dd685dd_1895_46e4_b227_be9f7d643c25 "https://dbpedia.org/page/Electrolyte"@en ;
    emmo:EMMO_705f27ae_954c_4f13_98aa_18473fc52b25 "From Greek elektron ('electric') + lyts (, looser): that which is set free or made to pass by electricity; adopted to denote the conducting medium undergoing electrolysis. Coined by Michael Faraday with support from William Whewell and Whitlock Nicholl."@en ;
    emmo:EMMO_967080e5_2f42_4eb2_a3a9_c58143e835f9 "a material in which the mobile species are ions and free movement of electrons is blocked."@en ;
    emmo:EMMO_c7b62dd7_063a_4c2a_8504_42f7264ba83f "A solid electrolyte is a solid material where the predominant charge carriers are ions. For example: NASICON (Na Super Ionic Conductor), which has the general formula Na1+xZr2P3-xSix O12 , 0 < x < 3."@en,
        "An ionic liquid is an electrolyte composed of a salt that is liquid below 100 C. Ionic liquids have found uses in electrochemical analysis, because their unconventional properties include a negligible vapor pressure, a high thermal and electrochemical stability, and exceptional dissolution properties for both organic and inorganic chemical species."@en,
        "conducting medium in which the flow of electric current is accompanied by the movement of ions"@en,
        "liquid or solid substance containing mobile ions that render it conductive"@en,
        "substance that provides ions on dissolution in a solvent or on melting"@en ;
    emmo:EMMO_c84c6752_6d64_48cc_9500_e54a3c34898d "https://en.wikipedia.org/wiki/Electrolyte"@en .

:electrochemistry_19abaccd_43be_4048_965c_e4fb63c5951b a owl:Class ;
    rdfs:label "ElectrochemicalPhenomenon"@en ;
    rdfs:comment "a chemical phenomenon that is accompanied by the flow of electric current"@en ;
    rdfs:subClassOf emmo:EMMO_135ab8ea_e028_439e_be64_3e0f9734ea2b ;
    skos:prefLabel "ElectrochemicalPhenomenon"@en ;
    emmo:EMMO_967080e5_2f42_4eb2_a3a9_c58143e835f9 "a chemical phenomenon that is accompanied by the flow of electric current"@en .

:electrochemistry_b5ea31c9_bb10_4276_980e_c3eceb1efc82 a owl:Class ;
    rdfs:label "ElectrochemicalComponent"@en ;
    rdfs:comment "A component in an electrochemical system."@en ;
    rdfs:subClassOf emmo:EMMO_f76884f7_964e_488e_9bb7_1b2453e9e817 ;
    skos:prefLabel "ElectrochemicalComponent"@en ;
    emmo:EMMO_967080e5_2f42_4eb2_a3a9_c58143e835f9 "A component in an electrochemical system."@en .

:electrochemistry_0acd0fc2_1048_4604_8e90_bf4e84bd87df a owl:Class ;
    rdfs:label "ElectrochemicalDevice"@en ;
    rdfs:comment "a device whose primary function is facilitating the conversion between chemical and electrical energy."@en ;
    rdfs:seeAlso :electrochemistry_6f2c88c9_5c04_4953_a298_032cc3ab9b77 ;
    rdfs:subClassOf [ a owl:Restriction ;
            owl:onProperty emmo:EMMO_dba27ca1_33c9_4443_a912_1519ce4c39ec ;
            owl:someValuesFrom :electrochemistry_522f0c0b_cf33_4328_af71_12e38dae6798 ],
        [ a owl:Restriction ;
            owl:onProperty emmo:EMMO_dba27ca1_33c9_4443_a912_1519ce4c39ec ;
            owl:someValuesFrom :electrochemistry_b851c7e9_60bf_4d3d_abe1_8d08d3d85124 ],
        [ a owl:Restriction ;
            owl:onProperty emmo:EMMO_e1097637_70d2_4895_973f_2396f04fa204 ;
            owl:someValuesFrom emmo:EMMO_e218c625_6a39_47a9_8d08_a2ef41c152a9 ],
        [ a owl:Restriction ;
            owl:onProperty emmo:EMMO_e1097637_70d2_4895_973f_2396f04fa204 ;
            owl:someValuesFrom :electrochemistry_0ddfd57a_d338_4690_be45_b26884ed6302 ],
        [ a owl:Restriction ;
            owl:onProperty emmo:EMMO_e1097637_70d2_4895_973f_2396f04fa204 ;
            owl:someValuesFrom :electrochemistry_0ea4d188_9701_4699_a5ca_812a98a9afa7 ],
        [ a owl:Restriction ;
            owl:onProperty emmo:EMMO_e1097637_70d2_4895_973f_2396f04fa204 ;
            owl:someValuesFrom :electrochemistry_2a1de79f_e927_45a2_9619_3799a0d61e9b ],
        [ a owl:Restriction ;
            owl:onProperty emmo:EMMO_e1097637_70d2_4895_973f_2396f04fa204 ;
            owl:someValuesFrom :electrochemistry_4a354510_4dc2_4803_8845_f4024a1a7260 ],
        [ a owl:Restriction ;
            owl:onProperty emmo:EMMO_e1097637_70d2_4895_973f_2396f04fa204 ;
            owl:someValuesFrom :electrochemistry_4aa1b96e_44a0_4b1a_a0ac_723d0223d80b ],
        [ a owl:Restriction ;
            owl:onProperty emmo:EMMO_e1097637_70d2_4895_973f_2396f04fa204 ;
            owl:someValuesFrom :electrochemistry_639b844a_e801_436b_985d_28926129ead6 ],
        [ a owl:Restriction ;
            owl:onProperty emmo:EMMO_e1097637_70d2_4895_973f_2396f04fa204 ;
            owl:someValuesFrom :electrochemistry_b90b1ad7_b9a8_44df_ad45_bfd25aac2e49 ],
        [ a owl:Restriction ;
            owl:onProperty emmo:EMMO_e1097637_70d2_4895_973f_2396f04fa204 ;
            owl:someValuesFrom :electrochemistry_de612af2_a029_4a02_8090_4a75ab13271d ],
        [ a owl:Restriction ;
            owl:onProperty :electrochemistry_1784d824_15bd_4eff_9e40_61e23be6f979 ;
            owl:someValuesFrom :electrochemistry_6f2c88c9_5c04_4953_a298_032cc3ab9b77 ],
        [ a owl:Restriction ;
            owl:onProperty :electrochemistry_3bd08946_4e81_455d_9fca_dc7a5ead9315 ;
            owl:someValuesFrom :electrochemistry_fb0d9eef_92af_4628_8814_e065ca255d59 ],
        [ a owl:Restriction ;
            owl:onProperty :electrochemistry_3dcfe33d_6825_43c0_a798_68e871a68d39 ;
            owl:someValuesFrom :electrochemistry_1aec4cc0_82d5_4042_a657_ed7fe291c3d8 ],
        [ a owl:Restriction ;
            owl:onProperty :electrochemistry_5d299271_3f68_494f_ab96_3db9acdd3138 ;
            owl:someValuesFrom :electrochemistry_0f007072_a8dd_4798_b865_1bf9363be627 ],
        [ a owl:Restriction ;
            owl:onProperty :electrochemistry_8e9cf965_9f92_46e8_b678_b50410ce3616 ;
            owl:someValuesFrom :electrochemistry_0f007072_a8dd_4798_b865_1bf9363be627 ],
        [ a owl:Restriction ;
            owl:onProperty :electrochemistry_9317be62_e602_4343_a72d_02c87201b9f6 ;
            owl:someValuesFrom :electrochemistry_331e6cca_f260_4bf8_af55_35304fe1bbe0 ],
        emmo:EMMO_494b372c_cfdf_47d3_a4de_5e037c540de8 ;
    skos:prefLabel "ElectrochemicalDevice"@en ;
    skos:scopeNote "The term refers to the engineered assembly; it must not be conflated with the electrochemical cell itself."@en ;
    emmo:EMMO_157fdf31_6387_42be_8e72_10530519214a "https://raw.githubusercontent.com/emmo-repo/domain-electrochemistry/dev/docs/assets/img/fig/png/ElectrochemicalDevice.png" ;
    emmo:EMMO_4c8480cf_56de_41da_8699_f12a9033313a "Electrochemical devices typically include safety and control subsystems that are not part of the electrochemical cell (e.g. pressure relief, BMS, valves, current collectors)."@en ;
    emmo:EMMO_5f7abc2a_5b50_41c3_8def_c8ba7c3b083e "When documenting a device, identify the number and arrangement of cells and the presence of auxiliary components such as separators, membranes, and power electronics."@en ;
    emmo:EMMO_967080e5_2f42_4eb2_a3a9_c58143e835f9 "a device whose primary function is facilitating the conversion between chemical and electrical energy."@en ;
    emmo:EMMO_c7b62dd7_063a_4c2a_8504_42f7264ba83f "an electrochemical device contains at least one electrochemical cell plus the apparati required to make it work as a practical device (e.g. terminals, container, etc.)"@en .

:electrochemistry_43cd6e14_dd43_41b5_b5b4_344d53841603 a owl:Class ;
    rdfs:label "PrismaticCase"@en ;
    rdfs:comment "a rigid prismatic case that is described by characteristic length, width, and height"@en ;
    rdfs:subClassOf [ a owl:Restriction ;
            owl:onProperty emmo:EMMO_dba27ca1_33c9_4443_a912_1519ce4c39ec ;
            owl:someValuesFrom :electrochemistry_1e33e37e_d7c9_4701_ba6d_a09456a13aaf ],
        [ a owl:Restriction ;
            owl:onProperty emmo:EMMO_dba27ca1_33c9_4443_a912_1519ce4c39ec ;
            owl:someValuesFrom :electrochemistry_4a5660bd_1c1a_40e5_8a41_463c720d3903 ],
        :electrochemistry_1aec4cc0_82d5_4042_a657_ed7fe291c3d8 ;
    skos:prefLabel "PrismaticCase"@en ;
    emmo:EMMO_967080e5_2f42_4eb2_a3a9_c58143e835f9 "a rigid prismatic case that is described by characteristic length, width, and height"@en ;
    emmo:EMMO_c7b62dd7_063a_4c2a_8504_42f7264ba83f "often represented in cell designations by the letter P"@en .

:electrochemistry_e4b6cb36_4dac_49e3_871d_40bcfca943a5 a owl:Class ;
    rdfs:label "MetalOxideElectrode"@en ;
    rdfs:comment "electrode in which the active material is a metal oxide"@en ;
    rdfs:subClassOf :electrochemistry_9a823d64_9d10_4a29_9cbd_9bbdad7985bc ;
    skos:prefLabel "MetalOxideElectrode"@en ;
    emmo:EMMO_967080e5_2f42_4eb2_a3a9_c58143e835f9 "electrode in which the active material is a metal oxide"@en .

:electrochemistry_0f007072_a8dd_4798_b865_1bf9363be627 a owl:Class ;
    rdfs:label "Electrode"@en ;
    rdfs:comment "electronically conductive part in electric contact with a medium of lower electronic conductivity and intended to perform one or more of the functions of emitting charge carriers to or receiving charge carriers from that medium or to establish an electric field in that medium"@en ;
    rdfs:subClassOf [ a owl:Restriction ;
            owl:onProperty emmo:EMMO_8785be5a_2493_4b12_8f39_31907ab11748 ;
            owl:someValuesFrom :electrochemistry_fb0d9eef_92af_4628_8814_e065ca255d59 ],
        [ a owl:Restriction ;
            owl:onProperty emmo:EMMO_dba27ca1_33c9_4443_a912_1519ce4c39ec ;
            owl:someValuesFrom :electrochemistry_50044b99_b858_433b_a32d_23d1e1cf88b2 ],
        [ a owl:Restriction ;
            owl:onProperty emmo:EMMO_e1097637_70d2_4895_973f_2396f04fa204 ;
            owl:someValuesFrom emmo:EMMO_43003c86_9d15_433b_9789_ee2940920656 ],
        [ a owl:Restriction ;
            owl:onProperty emmo:EMMO_e1097637_70d2_4895_973f_2396f04fa204 ;
            owl:someValuesFrom :electrochemistry_791c1915_a791_4450_acd8_7f94764743b5 ],
        [ a owl:Restriction ;
            owl:onProperty emmo:EMMO_e1097637_70d2_4895_973f_2396f04fa204 ;
            owl:someValuesFrom :electrochemistry_7fc10197_41d9_4c1e_a107_928f03eb2d36 ],
        [ a owl:Restriction ;
            owl:onProperty :electrochemistry_056a5fab_3d99_46bd_8eb1_6e89a368e1a7 ;
            owl:someValuesFrom emmo:EMMO_bc37743c_37c4_4ec7_9d58_d1aae5567352 ],
        [ a owl:Restriction ;
            owl:onProperty :electrochemistry_860aa941_5ff9_4452_8a16_7856fad07bee ;
            owl:someValuesFrom emmo:EMMO_bc37743c_37c4_4ec7_9d58_d1aae5567352 ],
        :electrochemistry_b5ea31c9_bb10_4276_980e_c3eceb1efc82 ;
    skos:prefLabel "Electrode"@en ;
    emmo:EMMO_26bf1bef_d192_4da6_b0eb_d2209698fb54 "https://www.wikidata.org/wiki/Q176140" ;
    emmo:EMMO_50c298c2_55a2_4068_b3ac_4e948c33181f "https://www.electropedia.org/iev/iev.nsf/display?openform&ievref=482-02-21",
        "https://www.electropedia.org/iev/iev.nsf/display?openform&ievref=114-02-03"@en ;
    emmo:EMMO_6dd685dd_1895_46e4_b227_be9f7d643c25 "https://dbpedia.org/page/Electrode"@en ;
    emmo:EMMO_705f27ae_954c_4f13_98aa_18473fc52b25 "From Greek elektron (amber, electricity) + hodos (way): the way of electricity. Proposed to replace vague poles/plates with a neutral, process-descriptive term. Introduced by Michael Faraday, with support from William Whewell and Whitlock Nicholl."@en ;
    emmo:EMMO_967080e5_2f42_4eb2_a3a9_c58143e835f9 "electronically conductive part in electric contact with a medium of lower electronic conductivity and intended to perform one or more of the functions of emitting charge carriers to or receiving charge carriers from that medium or to establish an electric field in that medium"@en ;
    emmo:EMMO_c7b62dd7_063a_4c2a_8504_42f7264ba83f "Alternative definition: Half-cell consisting of at least one electron conductor and at least one ionic conductor (electrolyte). - Terminology of electrochemical methods of analysis (IUPAC Recommendations 2019)"@en,
        "Electron conductor in an electrochemical cell connected to the external circuit."@en,
        "In some electroanalytical techniques (conductometry and differential potentiometry), two indicator electrodes are used. For many analytical measurements in cells with current flow, a three-electrode cell is used."@en,
        "Many types of electrodes are used. These may be classified into groups according to their composition, form and size, and according to their operating mode. See section 4."@en,
        "The current flow through electrochemical cells may be zero or non-zero. An electrochemical cell with current flow can operate either as a galvanic cell or an electrolytic cell."@en ;
    emmo:EMMO_c84c6752_6d64_48cc_9500_e54a3c34898d "https://en.wikipedia.org/wiki/Electrode"@en .

:electrochemistry_9a823d64_9d10_4a29_9cbd_9bbdad7985bc a owl:Class ;
    rdfs:label "ActiveElectrode"@en ;
    rdfs:comment "an electrode which is chemically altered by the electrode reaction"@en ;
    rdfs:subClassOf [ a owl:Restriction ;
            owl:onProperty emmo:EMMO_dba27ca1_33c9_4443_a912_1519ce4c39ec ;
            owl:someValuesFrom emmo:EMMO_df96cbb6_b5ee_4222_8eab_b3675df24bea ],
        :electrochemistry_0f007072_a8dd_4798_b865_1bf9363be627 ;
    skos:altLabel "NonInertElectrode"@en,
        "ReactiveElectrode"@en ;
    skos:prefLabel "ActiveElectrode"@en ;
    emmo:EMMO_967080e5_2f42_4eb2_a3a9_c58143e835f9 "an electrode which is chemically altered by the electrode reaction"@en ;
    emmo:EMMO_c7b62dd7_063a_4c2a_8504_42f7264ba83f "the opposite of an inert electrode"@en .

:electrochemistry_860aa941_5ff9_4452_8a16_7856fad07bee a owl:ObjectProperty ;
    rdfs:label "hasActiveMaterial"@en ;
    rdfs:comment "relates an electrode or other functional component to the material that participates directly in the primary electrochemical reaction"@en ;
    rdfs:range emmo:EMMO_bc37743c_37c4_4ec7_9d58_d1aae5567352 ;
    rdfs:subPropertyOf emmo:EMMO_3c7f239f_e833_4a2b_98a1_c88831770c1b ;
    skos:prefLabel "hasActiveMaterial"@en ;
    emmo:EMMO_967080e5_2f42_4eb2_a3a9_c58143e835f9 "relates an electrode or other functional component to the material that participates directly in the primary electrochemical reaction"@en .

:electrochemistry_3979cd56_6256_414d_966c_7f723bf71e37 a owl:Class ;
    rdfs:label "CoinCase"@en ;
    rdfs:comment "a round-type case with a height that is less than the diameter"@en ;
    rdfs:subClassOf :electrochemistry_eacb141f_6ab4_491f_8603_a3e025cefc82 ;
    skos:altLabel "ButtonCase"@en ;
    skos:prefLabel "CoinCase"@en ;
    emmo:EMMO_967080e5_2f42_4eb2_a3a9_c58143e835f9 "a round-type case with a height that is less than the diameter"@en .

[] a owl:Axiom ;
    dcterms:source "International Electrotechnical Commission (IEC), IEC 60050 - International Electrotechnical Vocabulary, retrieved from: https://www.electropedia.org" ;
    owl:annotatedProperty emmo:EMMO_967080e5_2f42_4eb2_a3a9_c58143e835f9 ;
    owl:annotatedSource :electrochemistry_444992e5_43f8_44a1_9767_b408dbe54330 ;
    owl:annotatedTarget "phenomenon by which a cell or battery loses energy in other ways than by discharge into an external circuit"@en .

[] a owl:Axiom ;
    dcterms:source "International Electrotechnical Commission (IEC), IEC 60050 - International Electrotechnical Vocabulary, retrieved from: https://www.electropedia.org" ;
    owl:annotatedProperty emmo:EMMO_967080e5_2f42_4eb2_a3a9_c58143e835f9 ;
    owl:annotatedSource :electrochemistry_457a8f92_0a19_4773_8114_a42edff32248 ;
    owl:annotatedTarget "assembly of plates of the same polarity electrically connected together"@en .

[] a owl:Axiom ;
    dcterms:source "International Electrotechnical Commission (IEC), IEC 60050 - International Electrotechnical Vocabulary, retrieved from: https://www.electropedia.org" ;
    owl:annotatedProperty emmo:EMMO_967080e5_2f42_4eb2_a3a9_c58143e835f9 ;
    owl:annotatedSource :electrochemistry_49263a32_eca6_4644_8144_0d3b14c26d0a ;
    owl:annotatedTarget "mixing of a substance into another substance with formation of one new homogeneous substance"@en .

[] a owl:Axiom ;
    dcterms:source "International Electrotechnical Commission (IEC), IEC 60050 - International Electrotechnical Vocabulary, retrieved from: https://www.electropedia.org" ;
    owl:annotatedProperty emmo:EMMO_967080e5_2f42_4eb2_a3a9_c58143e835f9 ;
    owl:annotatedSource :electrochemistry_49909cd1_44f4_41b4_877a_82a52845a5cb ;
    owl:annotatedTarget "component of a cell made of insulating material intended to maintain the spacing between plates of opposite polarity or between the plate pack and the case"@en .

[] a owl:Axiom ;
    dcterms:source "International Electrotechnical Commission (IEC), IEC 60050 - International Electrotechnical Vocabulary, retrieved from: https://www.electropedia.org" ;
    owl:annotatedProperty emmo:EMMO_967080e5_2f42_4eb2_a3a9_c58143e835f9 ;
    owl:annotatedSource :electrochemistry_4a5660bd_1c1a_40e5_8a41_463c720d3903 ;
    owl:annotatedTarget "cell container which is usually metallic and typically, but not exclusively, cylindrical"@en .

[] a owl:Axiom ;
    dcterms:source "International Electrotechnical Commission (IEC), IEC 60050 - International Electrotechnical Vocabulary, retrieved from: https://www.electropedia.org" ;
    owl:annotatedProperty emmo:EMMO_967080e5_2f42_4eb2_a3a9_c58143e835f9 ;
    owl:annotatedSource :electrochemistry_4bc38e99_1978_4143_a766_fbb57f2cf46e ;
    owl:annotatedTarget "situation in which a material in a given environment undergoes negligible electrochemical corrosion."@en .

[] a owl:Axiom ;
    dcterms:source "International Electrotechnical Commission (IEC), IEC 60050 - International Electrotechnical Vocabulary, retrieved from: https://www.electropedia.org" ;
    owl:annotatedProperty emmo:EMMO_967080e5_2f42_4eb2_a3a9_c58143e835f9 ;
    owl:annotatedSource :electrochemistry_4d6f7f50_b343_4bd6_8612_2b8521a99c9b ;
    owl:annotatedTarget "increasing the rate of an electrode reaction by adding specific material to the electrode."@en .

[] a owl:Axiom ;
    dcterms:source "A. J. Bard, G. Inzelt, and F. Scholz, Eds., Electrochemical Dictionary, 2nd Edition. Berlin: Springer-Verlag, 2012. DOI: https://doi.org/10.1007/978-3-642-29551-5" ;
    owl:annotatedProperty emmo:EMMO_967080e5_2f42_4eb2_a3a9_c58143e835f9 ;
    owl:annotatedSource :electrochemistry_4df84ec1_8a1a_4770_963f_bf48009bd043 ;
    owl:annotatedTarget "the electrochemical dissolution of a material to soluble species"@en .

[] a owl:Axiom ;
    dcterms:source "A. J. Bard, G. Inzelt, and F. Scholz, Eds., Electrochemical Dictionary, 2nd Edition. Berlin: Springer-Verlag, 2012. DOI: https://doi.org/10.1007/978-3-642-29551-5" ;
    owl:annotatedProperty emmo:EMMO_967080e5_2f42_4eb2_a3a9_c58143e835f9 ;
    owl:annotatedSource :electrochemistry_4e02d727_07fe_41fd_886c_041317342086 ;
    owl:annotatedTarget "an electrolyte consisting of anions and cations with equal absolute charge numbers."@en .

[] a owl:Axiom ;
    dcterms:source "International Electrotechnical Commission (IEC), IEC 60050 - International Electrotechnical Vocabulary, retrieved from: https://www.electropedia.org" ;
    owl:annotatedProperty emmo:EMMO_967080e5_2f42_4eb2_a3a9_c58143e835f9 ;
    owl:annotatedSource :electrochemistry_522f0c0b_cf33_4328_af71_12e38dae6798 ;
    owl:annotatedTarget "accessible conductive part provided for the connection of an external electric circuit to the positive electrode of the cell"@en .

[] a owl:Axiom ;
    dcterms:source "A. J. Bard, G. Inzelt, and F. Scholz, Eds., Electrochemical Dictionary, 2nd Edition. Berlin: Springer-Verlag, 2012. DOI: https://doi.org/10.1007/978-3-642-29551-5" ;
    owl:annotatedProperty emmo:EMMO_967080e5_2f42_4eb2_a3a9_c58143e835f9 ;
    owl:annotatedSource :electrochemistry_54e0c2bd_1bb2_4f9c_9b55_5b6cc34651ec ;
    owl:annotatedTarget "a spatial region at the interface between two bulk phases in contact, which is different chemically and physically from both phases in contact"@en .

[] a owl:Axiom ;
    dcterms:source "International Electrotechnical Commission (IEC), IEC 60050 - International Electrotechnical Vocabulary, retrieved from: https://www.electropedia.org" ;
    owl:annotatedProperty emmo:EMMO_967080e5_2f42_4eb2_a3a9_c58143e835f9 ;
    owl:annotatedSource :electrochemistry_5641910f_6e69_4ce4_be84_4b1bf14b8916 ;
    owl:annotatedTarget "movement of a fluid through a diaphragm, produced by application of an electric field"@en .

[] a owl:Axiom ;
    dcterms:source "International Electrotechnical Commission (IEC), IEC 60050 - International Electrotechnical Vocabulary, retrieved from: https://www.electropedia.org" ;
    owl:annotatedProperty emmo:EMMO_967080e5_2f42_4eb2_a3a9_c58143e835f9 ;
    owl:annotatedSource :electrochemistry_5cb5548f_f774_4668_ad02_f0742581f2f1 ;
    owl:annotatedTarget "change of the mechanical stress at the surface separating two bodies due to the presence of electric charges at the interface"@en .

[] a owl:Axiom ;
    dcterms:source "IEEE Standard Glossary of Stationary Battery Terminology (2016), https://doi.org/10.1109/IEEESTD.2016.7552407" ;
    owl:annotatedProperty emmo:EMMO_967080e5_2f42_4eb2_a3a9_c58143e835f9 ;
    owl:annotatedSource :electrochemistry_5f9a9411_05f9_4576_acd3_81d7d41cfe98 ;
    owl:annotatedTarget "an ion-transport medium that does not contain water."@en .

[] a owl:Axiom ;
    dcterms:source "International Electrotechnical Commission (IEC), IEC 60050 - International Electrotechnical Vocabulary, retrieved from: https://www.electropedia.org" ;
    owl:annotatedProperty emmo:EMMO_967080e5_2f42_4eb2_a3a9_c58143e835f9 ;
    owl:annotatedSource :electrochemistry_60bc27f0_8290_4113_8c3b_011433a733c7 ;
    owl:annotatedTarget "cover of insulating material used to avoid electric contact with the cell or battery terminal"@en .

[] a owl:Axiom ;
    dcterms:source "J. M. Pingarrn et al., Terminology of electrochemical methods of analysis (IUPAC Recommendations 2019), Pure and Applied Chemistry, 4, 92, 2020, 641-694. https://doi.org/10.1515/pac-2018-0109" ;
    owl:annotatedProperty emmo:EMMO_967080e5_2f42_4eb2_a3a9_c58143e835f9 ;
    owl:annotatedSource :electrochemistry_60c5b2e5_164a_4ce6_8409_f386f5e50c03 ;
    owl:annotatedTarget "when the same electric charge (quantity of electricity) Q is passed through several electrolytes, the mass, m_i, of the substances deposited are proportional to their respective chemical equivalent molar mass, M_i/z_i."@en .

[] a owl:Axiom ;
    dcterms:source "J. M. Pingarrn et al., Terminology of electrochemical methods of analysis (IUPAC Recommendations 2019), Pure and Applied Chemistry, 4, 92, 2020, 641-694. https://doi.org/10.1515/pac-2018-0109" ;
    owl:annotatedProperty emmo:EMMO_967080e5_2f42_4eb2_a3a9_c58143e835f9 ;
    owl:annotatedSource :electrochemistry_637c576e_a50e_47ae_8c74_2024ce4c6d0f ;
    owl:annotatedTarget "means of making electrolytic connection between two half cells without introducing a significant liquid junction potential."@en .

[] a owl:Axiom ;
    dcterms:source "International Electrotechnical Commission (IEC), IEC 60050 - International Electrotechnical Vocabulary, retrieved from: https://www.electropedia.org" ;
    owl:annotatedProperty emmo:EMMO_967080e5_2f42_4eb2_a3a9_c58143e835f9 ;
    owl:annotatedSource :electrochemistry_63ea1c9b_0bda_4a69_9745_efb08e6be685 ;
    owl:annotatedTarget "transport of ions in an electrolyte due to an electric field"@en .

[] a owl:Axiom ;
    dcterms:source "International Electrotechnical Commission (IEC), IEC 60050 - International Electrotechnical Vocabulary, retrieved from: https://www.electropedia.org" ;
    owl:annotatedProperty emmo:EMMO_967080e5_2f42_4eb2_a3a9_c58143e835f9 ;
    owl:annotatedSource :electrochemistry_6559c04d_75bc_41ea_8ed8_8d3c09dae6b0 ;
    owl:annotatedTarget "material used to seal the cell lid to the case or to the terminals of a cell"@en .

[] a owl:Axiom ;
    dcterms:source "J. M. Pingarrn et al., Terminology of electrochemical methods of analysis (IUPAC Recommendations 2019), Pure and Applied Chemistry, 4, 92, 2020, 641-694. https://doi.org/10.1515/pac-2018-0109" ;
    owl:annotatedProperty emmo:EMMO_967080e5_2f42_4eb2_a3a9_c58143e835f9 ;
    owl:annotatedSource :electrochemistry_65c90d8d_9712_4f3f_b830_d8163ec4cfcc ;
    owl:annotatedTarget "electrode made of a solid amalgam of an appropriate metal"@en .

[] a owl:Axiom ;
    dcterms:source "International Electrotechnical Commission (IEC), IEC 60050 - International Electrotechnical Vocabulary, retrieved from: https://www.electropedia.org" ;
    owl:annotatedProperty emmo:EMMO_967080e5_2f42_4eb2_a3a9_c58143e835f9 ;
    owl:annotatedSource :electrochemistry_6b1f594f_2c0a_46a0_8805_d6ab08baa75e ;
    owl:annotatedTarget "positive plate (electrode) which is either composed of an assembly of porous tube of perforated metal or tissue either a gauntlet with or without a central current collector spine, the active material being placed within the tubes"@en .

[] a owl:Axiom ;
    dcterms:source "J. M. Pingarrn et al., Terminology of electrochemical methods of analysis (IUPAC Recommendations 2019), Pure and Applied Chemistry, 4, 92, 2020, 641-694. https://doi.org/10.1515/pac-2018-0109" ;
    owl:annotatedProperty emmo:EMMO_967080e5_2f42_4eb2_a3a9_c58143e835f9 ;
    owl:annotatedSource :electrochemistry_6c421175_477f_45e0_8b6c_c3464f5351c5 ;
    owl:annotatedTarget "A disc electrode that is embedded in the centre of a cylinder which rotates in solution around the longitudinal cylinder axis."@en .

[] a owl:Axiom ;
    dcterms:source "International Electrotechnical Commission (IEC), IEC 60050 - International Electrotechnical Vocabulary, retrieved from: https://www.electropedia.org" ;
    owl:annotatedProperty emmo:EMMO_967080e5_2f42_4eb2_a3a9_c58143e835f9 ;
    owl:annotatedSource :electrochemistry_01260656_ac32_472e_9513_a607366538ec ;
    owl:annotatedTarget "formation of compounds that reduces the conductivity at the surface of an electrode"@en .

[] a owl:Axiom ;
    dcterms:source "International Electrotechnical Commission (IEC), IEC 60050 - International Electrotechnical Vocabulary, retrieved from: https://www.electropedia.org" ;
    owl:annotatedProperty skos:note ;
    owl:annotatedSource :electrochemistry_6f2c88c9_5c04_4953_a298_032cc3ab9b77 ;
    owl:annotatedTarget "composite system in which the supplied electric energy mainly produces chemical reactions or, conversely, in which the energy released by chemical reactions is mainly delivered by the system as electric energy"@en .

[] a owl:Axiom ;
    dcterms:source "J. Newman and K. E. Thmoas-Alyea, Electrochemical Systems, 3rd ed. Hoboken, New Jersey: John Wiley & Sons, 2004." ;
    owl:annotatedProperty emmo:EMMO_967080e5_2f42_4eb2_a3a9_c58143e835f9 ;
    owl:annotatedSource :electrochemistry_6f2c88c9_5c04_4953_a298_032cc3ab9b77 ;
    owl:annotatedTarget "system containing two electrodes that allow transport of electrons, separated by an electrolyte that allows movement of ions but blocks movement of electrons"@en .

[] a owl:Axiom ;
    dcterms:source "J. M. Pingarrn et al., Terminology of electrochemical methods of analysis (IUPAC Recommendations 2019), Pure and Applied Chemistry, 4, 92, 2020, 641-694. https://doi.org/10.1515/pac-2018-0109" ;
    owl:annotatedProperty emmo:EMMO_967080e5_2f42_4eb2_a3a9_c58143e835f9 ;
    owl:annotatedSource :electrochemistry_6fec8cc1_4e6c_428e_8343_6cf3c286a185 ;
    owl:annotatedTarget "foil, wire or disc electrode made of gold which is easily fabricated into a variety of electrode geometries"@en .

[] a owl:Axiom ;
    dcterms:source "International Electrotechnical Commission (IEC), IEC 60050 - International Electrotechnical Vocabulary, retrieved from: https://www.electropedia.org" ;
    owl:annotatedProperty emmo:EMMO_967080e5_2f42_4eb2_a3a9_c58143e835f9 ;
    owl:annotatedSource :electrochemistry_76df6e7b_fc3b_4a1f_98b1_0ca9c0539e4c ;
    owl:annotatedTarget "cable used for the electrical connection of the battery terminals and the load and/or the charger"@en .

[] a owl:Axiom ;
    dcterms:source "International Electrotechnical Commission (IEC), IEC 60050 - International Electrotechnical Vocabulary, retrieved from: https://www.electropedia.org" ;
    owl:annotatedProperty emmo:EMMO_967080e5_2f42_4eb2_a3a9_c58143e835f9 ;
    owl:annotatedSource :electrochemistry_0471ec77_91bc_4a78_be31_b6af613e5966 ;
    owl:annotatedTarget "insertion or removal of electrons into or from ions to obtain particles having zero electric charge"@en .

[] a owl:Axiom ;
    dcterms:source "International Electrotechnical Commission (IEC), IEC 60050 - International Electrotechnical Vocabulary, retrieved from: https://www.electropedia.org" ;
    owl:annotatedProperty emmo:EMMO_967080e5_2f42_4eb2_a3a9_c58143e835f9 ;
    owl:annotatedSource :electrochemistry_7729c34e_1ae9_403d_b933_1765885e7f29 ;
    owl:annotatedTarget "Electrode with a well-defined and constant equilibrium potential with respect to which it is possible to measure or calculate electrode potentials of other electrodes by including them in an appropriate electrochemical cell."@en .

[] a owl:Axiom ;
    dcterms:source "J. M. Pingarrn et al., Terminology of electrochemical methods of analysis (IUPAC Recommendations 2019), Pure and Applied Chemistry, 4, 92, 2020, 641-694. https://doi.org/10.1515/pac-2018-0109" ;
    owl:annotatedProperty emmo:EMMO_c7b62dd7_063a_4c2a_8504_42f7264ba83f ;
    owl:annotatedSource :electrochemistry_7729c34e_1ae9_403d_b933_1765885e7f29 ;
    owl:annotatedTarget "Electrode that maintains an essentially constant potential under the conditions prevailing in an electrochemical measurement, and that serves for observation, measurement, or control of the potential of the indicator or working electrode."@en .

[] a owl:Axiom ;
    dcterms:source "International Electrotechnical Commission (IEC), IEC 60050 - International Electrotechnical Vocabulary, retrieved from: https://www.electropedia.org" ;
    owl:annotatedProperty emmo:EMMO_967080e5_2f42_4eb2_a3a9_c58143e835f9 ;
    owl:annotatedSource :electrochemistry_7760b241_775f_4be1_b827_59f9bde9e5b2 ;
    owl:annotatedTarget "electrolytic cell in which a chemical reaction is influenced by the absorption of light"@en .

[] a owl:Axiom ;
    dcterms:source "International Electrotechnical Commission (IEC), IEC 60050 - International Electrotechnical Vocabulary, retrieved from: https://www.electropedia.org" ;
    owl:annotatedProperty emmo:EMMO_967080e5_2f42_4eb2_a3a9_c58143e835f9 ;
    owl:annotatedSource :electrochemistry_79d1b273_58cd_4be6_a250_434817f7c261 ;
    owl:annotatedTarget "material that is oxidized or reduced at an electrode in an electrochemical cell"@en .

[] a owl:Axiom ;
    dcterms:source "J. M. Pingarrn et al., Terminology of electrochemical methods of analysis (IUPAC Recommendations 2019), Pure and Applied Chemistry, 4, 92, 2020, 641-694. https://doi.org/10.1515/pac-2018-0109" ;
    owl:annotatedProperty emmo:EMMO_967080e5_2f42_4eb2_a3a9_c58143e835f9 ;
    owl:annotatedSource :electrochemistry_7f4d74cd_d0a5_4908_9da9_7629fe419917 ;
    owl:annotatedTarget "a second annular working electrode positioned concentric with a rotating disc electrode to make a rotating ring-disc electrode (RRDE)"@en .

[] a owl:Axiom ;
    dcterms:source "International Electrotechnical Commission (IEC), IEC 60050 - International Electrotechnical Vocabulary, retrieved from: https://www.electropedia.org" ;
    owl:annotatedProperty emmo:EMMO_967080e5_2f42_4eb2_a3a9_c58143e835f9 ;
    owl:annotatedSource :electrochemistry_04f28ce3_251d_429e_aa85_ab3eb45bbcd2 ;
    owl:annotatedTarget "unstable condition arising during constant voltage charge in which the rate of heat dissipation capability, causing a continuous temperature increase with resulting further charge current increase, which can lead to the destruction of the battery"@en .

[] a owl:Axiom ;
    dcterms:source "International Electrotechnical Commission (IEC), IEC 60050 - International Electrotechnical Vocabulary, retrieved from: https://www.electropedia.org" ;
    owl:annotatedProperty emmo:EMMO_967080e5_2f42_4eb2_a3a9_c58143e835f9 ;
    owl:annotatedSource :electrochemistry_81833d8a_b03d_4250_be84_6385415beb01 ;
    owl:annotatedTarget "blend containing a material which reacts chemically to produce electrical energy with other constituents and additives"@en .

[] a owl:Axiom ;
    dcterms:source "International Electrotechnical Commission (IEC), IEC 60050 - International Electrotechnical Vocabulary, retrieved from: https://www.electropedia.org" ;
    owl:annotatedProperty emmo:EMMO_967080e5_2f42_4eb2_a3a9_c58143e835f9 ;
    owl:annotatedSource :electrochemistry_83d2c2d4_ffa9_42f4_9264_a0c59c657607 ;
    owl:annotatedTarget "reversing of the polarities of the electrodes of a cell, generally due to over-discharge of a low-capacity cell in a series arrangement"@en .

[] a owl:Axiom ;
    dcterms:source "International Electrotechnical Commission (IEC), IEC 60050 - International Electrotechnical Vocabulary, retrieved from: https://www.electropedia.org" ;
    owl:annotatedProperty emmo:EMMO_967080e5_2f42_4eb2_a3a9_c58143e835f9 ;
    owl:annotatedSource :electrochemistry_865a40fc_2187_4549_a7e1_37aa2458448f ;
    owl:annotatedTarget "electrolyte on the anode side of an electrochemical cell that is divided into compartments"@en .

[] a owl:Axiom ;
    dcterms:source "A. J. Bard, G. Inzelt, and F. Scholz, Eds., Electrochemical Dictionary, 2nd Edition. Berlin: Springer-Verlag, 2012. DOI: https://doi.org/10.1007/978-3-642-29551-5" ;
    owl:annotatedProperty emmo:EMMO_c7b62dd7_063a_4c2a_8504_42f7264ba83f ;
    owl:annotatedSource :electrochemistry_865a40fc_2187_4549_a7e1_37aa2458448f ;
    owl:annotatedTarget "Electrolyte solution in the anodic compartment of an electrolysis cell or galvanic cell, i.e., in that part of the cell where the anode is placed."@en .

[] a owl:Axiom ;
    dcterms:source "J. M. Pingarrn et al., Terminology of electrochemical methods of analysis (IUPAC Recommendations 2019), Pure and Applied Chemistry, 4, 92, 2020, 641-694. https://doi.org/10.1515/pac-2018-0109" ;
    owl:annotatedProperty emmo:EMMO_967080e5_2f42_4eb2_a3a9_c58143e835f9 ;
    owl:annotatedSource :electrochemistry_86be0987_5e21_43ec_b975_8f679999d328 ;
    owl:annotatedTarget "electrode containing two different metals (e.g. platinum and ruthenium) on its surface (e.g. to modify its electrocatalytic properties)"@en .

[] a owl:Axiom ;
    dcterms:source "J. M. Pingarrn et al., Terminology of electrochemical methods of analysis (IUPAC Recommendations 2019), Pure and Applied Chemistry, 4, 92, 2020, 641-694. https://doi.org/10.1515/pac-2018-0109" ;
    owl:annotatedProperty emmo:EMMO_967080e5_2f42_4eb2_a3a9_c58143e835f9 ;
    owl:annotatedSource :electrochemistry_871bc4a4_2d17_4b88_9b0f_7ab85f14afea ;
    owl:annotatedTarget "electrode whose function is to carry the electric current flowing through the electrical circuit of an electrochemical cell, the electrochemical processes on its surface not being of interest"@en .

[] a owl:Axiom ;
    dcterms:source "PAC, 1994, 66, 1077. (Glossary of terms used in physical organic chemistry (IUPAC Recommendations 1994)) on page 1096" ;
    owl:annotatedProperty emmo:EMMO_967080e5_2f42_4eb2_a3a9_c58143e835f9 ;
    owl:annotatedSource :electrochemistry_8a1c9a7b_978c_4421_a9c1_d0b07b42aab9 ;
    owl:annotatedTarget "a process that results in the interconversion of chemical species"@en .

[] a owl:Axiom ;
    dcterms:source "International Electrotechnical Commission (IEC), IEC 60050 - International Electrotechnical Vocabulary, retrieved from: https://www.electropedia.org" ;
    owl:annotatedProperty emmo:EMMO_c7b62dd7_063a_4c2a_8504_42f7264ba83f ;
    owl:annotatedSource :electrochemistry_04f28ce3_251d_429e_aa85_ab3eb45bbcd2 ;
    owl:annotatedTarget "in lithium batteries thermal runaway may cause melting of lithium"@en .

[] a owl:Axiom ;
    dcterms:source "International Electrotechnical Commission (IEC), IEC 60050 - International Electrotechnical Vocabulary, retrieved from: https://www.electropedia.org" ;
    owl:annotatedProperty emmo:EMMO_967080e5_2f42_4eb2_a3a9_c58143e835f9 ;
    owl:annotatedSource :electrochemistry_8a5083b0_cd23_4f8c_99e8_b9ccd6f9f3a2 ;
    owl:annotatedTarget "electrochemical cell that has two half-cells separated by a wall permeable to ions, both containing the same electrolyte differing only in their ion concentrations"@en .

[] a owl:Axiom ;
    dcterms:source "International Electrotechnical Commission (IEC), IEC 60050 - International Electrotechnical Vocabulary, retrieved from: https://www.electropedia.org" ;
    owl:annotatedProperty emmo:EMMO_967080e5_2f42_4eb2_a3a9_c58143e835f9 ;
    owl:annotatedSource :electrochemistry_8c71739c_27c1_4d19_a0ff_02545296af43 ;
    owl:annotatedTarget "arrangement of cells or batteries wherein the positive terminal of each cell or battery is connected to the negative terminal of the next cell or battery in sequence."@en .

[] a owl:Axiom ;
    dcterms:source "International Electrotechnical Commission (IEC), IEC 60050 - International Electrotechnical Vocabulary, retrieved from: https://www.electropedia.org" ;
    owl:annotatedProperty emmo:EMMO_967080e5_2f42_4eb2_a3a9_c58143e835f9 ;
    owl:annotatedSource :electrochemistry_8d3bf304_78e4_4e99_abe1_6ab429e44ed1 ;
    owl:annotatedTarget "cell which remains closed and does not release either gas or liquid when operated within the limits specified by the manufacturer"@en .

[] a owl:Axiom ;
    dcterms:source "International Electrotechnical Commission (IEC), IEC 60050 - International Electrotechnical Vocabulary, retrieved from: https://www.electropedia.org" ;
    owl:annotatedProperty emmo:EMMO_c7b62dd7_063a_4c2a_8504_42f7264ba83f ;
    owl:annotatedSource :electrochemistry_8d3bf304_78e4_4e99_abe1_6ab429e44ed1 ;
    owl:annotatedTarget "a sealed cell may be equipped with a safety device to prevent a dangerously high internal pressure and is designed to operate during its life in its original sealed state"@en .

[] a owl:Axiom ;
    dcterms:source "International Electrotechnical Commission (IEC), IEC 60050 - International Electrotechnical Vocabulary, retrieved from: https://www.electropedia.org" ;
    owl:annotatedProperty emmo:EMMO_967080e5_2f42_4eb2_a3a9_c58143e835f9 ;
    owl:annotatedSource :electrochemistry_900d95fb_863d_4142_a96d_369fb39e2639 ;
    owl:annotatedTarget "capacitor consisting of a metallic plate as first conductor, a very thin oxide film formed on the metal as the dielectric and an electrolyte as second conductor"@en .

[] a owl:Axiom ;
    dcterms:source "International Electrotechnical Commission (IEC), IEC 60050 - International Electrotechnical Vocabulary, retrieved from: https://www.electropedia.org" ;
    owl:annotatedProperty emmo:EMMO_967080e5_2f42_4eb2_a3a9_c58143e835f9 ;
    owl:annotatedSource :electrochemistry_92147e31_d015_4889_a092_04fbab033f15 ;
    owl:annotatedTarget "cell electrode consisting of a current collector and active material"@en .

[] a owl:Axiom ;
    dcterms:source "International Electrotechnical Commission (IEC), IEC 60050 - International Electrotechnical Vocabulary, retrieved from: https://www.electropedia.org" ;
    owl:annotatedProperty emmo:EMMO_967080e5_2f42_4eb2_a3a9_c58143e835f9 ;
    owl:annotatedSource :electrochemistry_96309fa9_e157_48fe_9fda_41003860a3c0 ;
    owl:annotatedTarget "chemiluminescence produced in electrode reactions"@en .

[] a owl:Axiom ;
    dcterms:source "J. M. Pingarrn et al., Terminology of electrochemical methods of analysis (IUPAC Recommendations 2019), Pure and Applied Chemistry, 4, 92, 2020, 641-694. https://doi.org/10.1515/pac-2018-0109" ;
    owl:annotatedProperty emmo:EMMO_70fe84ff_99b6_4206_a9fc_9a8931836d84 ;
    owl:annotatedSource :electrochemistry_0508a114_544a_4f54_a7de_9b947fb4b618 ;
    owl:annotatedTarget "a solid electrolyte is a solid material where the predominant charge carriers are ions."@en .

[] a owl:Axiom ;
    dcterms:source "International Electrotechnical Commission (IEC), IEC 60050 - International Electrotechnical Vocabulary, retrieved from: https://www.electropedia.org" ;
    owl:annotatedProperty emmo:EMMO_967080e5_2f42_4eb2_a3a9_c58143e835f9 ;
    owl:annotatedSource :electrochemistry_9c73aff8_1c82_4116_a6be_78e21982b69d ;
    owl:annotatedTarget "interface between an electrolyte and an electrode where an electrode reaction takes place."@en .

[] a owl:Axiom ;
    dcterms:source "J. M. Pingarrn et al., Terminology of electrochemical methods of analysis (IUPAC Recommendations 2019), Pure and Applied Chemistry, 4, 92, 2020, 641-694. https://doi.org/10.1515/pac-2018-0109" ;
    owl:annotatedProperty emmo:EMMO_967080e5_2f42_4eb2_a3a9_c58143e835f9 ;
    owl:annotatedSource :electrochemistry_9f466223_e20a_474d_ac4d_6d4b6131c275 ;
    owl:annotatedTarget "an electrode that holds its potential essentially constant by efficiently allowing electric current to pass"@en .

[] a owl:Axiom ;
    dcterms:source "International Electrotechnical Commission (IEC), IEC 60050 - International Electrotechnical Vocabulary, retrieved from: https://www.electropedia.org" ;
    owl:annotatedProperty emmo:EMMO_967080e5_2f42_4eb2_a3a9_c58143e835f9 ;
    owl:annotatedSource :electrochemistry_a0580fa9_5073_44af_b33e_7adbc83892d0 ;
    owl:annotatedTarget "electrode reaction in which oxidation occurs at the anode"@en .

[] a owl:Axiom ;
    dcterms:source "International Electrotechnical Commission (IEC), IEC 60050 - International Electrotechnical Vocabulary, retrieved from: https://www.electropedia.org" ;
    owl:annotatedProperty emmo:EMMO_967080e5_2f42_4eb2_a3a9_c58143e835f9 ;
    owl:annotatedSource :electrochemistry_a0a619d7_da95_41f0_8bc3_9c19d636d543 ;
    owl:annotatedTarget "electrode that serves only as a source or sink for electrons without playing a chemical role in the electrode reaction"@en .

[] a owl:Axiom ;
    dcterms:source "International Electrotechnical Commission (IEC), IEC 60050 - International Electrotechnical Vocabulary, retrieved from: https://www.electropedia.org" ;
    owl:annotatedProperty emmo:EMMO_967080e5_2f42_4eb2_a3a9_c58143e835f9 ;
    owl:annotatedSource :electrochemistry_a0fcb105_587f_45d8_a89a_46dc8f745069 ;
    owl:annotatedTarget "partial or complete external covering of a cell"@en .

[] a owl:Axiom ;
    dcterms:source "J. M. Pingarrn et al., Terminology of electrochemical methods of analysis (IUPAC Recommendations 2019), Pure and Applied Chemistry, 4, 92, 2020, 641-694. https://doi.org/10.1515/pac-2018-0109" ;
    owl:annotatedProperty emmo:EMMO_967080e5_2f42_4eb2_a3a9_c58143e835f9 ;
    owl:annotatedSource :electrochemistry_057bb143_639c_472b_99ed_ffa1867f6e63 ;
    owl:annotatedTarget "electrode made of glassy carbon material with an intertwined graphitic ribbon structure, formed by pyrolysis of a resol precursor at temperatures up to 3000 C"@en .

[] a owl:Axiom ;
    dcterms:source "International Electrotechnical Commission (IEC), IEC 60050 - International Electrotechnical Vocabulary, retrieved from: https://www.electropedia.org" ;
    owl:annotatedProperty emmo:EMMO_c7b62dd7_063a_4c2a_8504_42f7264ba83f ;
    owl:annotatedSource :electrochemistry_a0fcb105_587f_45d8_a89a_46dc8f745069 ;
    owl:annotatedTarget "a jacket may be made of metal (insulated from the cell terminals), plastic, paper or other suitable material"@en .

[] a owl:Axiom ;
    dcterms:source "International Electrotechnical Commission (IEC), IEC 60050 - International Electrotechnical Vocabulary, retrieved from: https://www.electropedia.org" ;
    owl:annotatedProperty emmo:EMMO_967080e5_2f42_4eb2_a3a9_c58143e835f9 ;
    owl:annotatedSource :electrochemistry_a2b92d2e_4431_411e_8da5_a4c08bac2c0e ;
    owl:annotatedTarget "process inside an electrolytic cell used to coat a conductive object with a layer of a material"@en .

[] a owl:Axiom ;
    dcterms:source "A. J. Bard, G. Inzelt, and F. Scholz, Eds., Electrochemical Dictionary, 2nd Edition. Berlin: Springer-Verlag, 2012. DOI: https://doi.org/10.1007/978-3-642-29551-5" ;
    owl:annotatedProperty emmo:EMMO_c7b62dd7_063a_4c2a_8504_42f7264ba83f ;
    owl:annotatedSource :electrochemistry_a2b92d2e_4431_411e_8da5_a4c08bac2c0e ;
    owl:annotatedTarget "The process of depositing a usually thin layer of metal upon a usually metallic substrate (or any other conductor, e.g. graphite), in order to improve the appearance, and/or to change the surface properties of the substrate."@en .

[] a owl:Axiom ;
    dcterms:source "International Electrotechnical Commission (IEC), IEC 60050 - International Electrotechnical Vocabulary, retrieved from: https://www.electropedia.org" ;
    owl:annotatedProperty emmo:EMMO_967080e5_2f42_4eb2_a3a9_c58143e835f9 ;
    owl:annotatedSource :electrochemistry_a2f4dca3_829f_412b_9025_bd7581aad82a ;
    owl:annotatedTarget "component of a cell which permits the flow of gas in one direction only"@en .

[] a owl:Axiom ;
    dcterms:source "International Electrotechnical Commission (IEC), IEC 60050 - International Electrotechnical Vocabulary, retrieved from: https://www.electropedia.org" ;
    owl:annotatedProperty emmo:EMMO_c7b62dd7_063a_4c2a_8504_42f7264ba83f ;
    owl:annotatedSource :electrochemistry_a2f4dca3_829f_412b_9025_bd7581aad82a ;
    owl:annotatedTarget "a valve has a characteristic venting or opening and closing pressure"@en .

[] a owl:Axiom ;
    dcterms:source "International Electrotechnical Commission (IEC), IEC 60050 - International Electrotechnical Vocabulary, retrieved from: https://www.electropedia.org" ;
    owl:annotatedProperty emmo:EMMO_967080e5_2f42_4eb2_a3a9_c58143e835f9 ;
    owl:annotatedSource :electrochemistry_a3b53904_22b1_42a9_a515_c8a3aed7e841 ;
    owl:annotatedTarget "material that can cause electrocatalysis."@en .

[] a owl:Axiom ;
    dcterms:source "J. M. Pingarrn et al., Terminology of electrochemical methods of analysis (IUPAC Recommendations 2019), Pure and Applied Chemistry, 4, 92, 2020, 641-694. https://doi.org/10.1515/pac-2018-0109" ;
    owl:annotatedProperty emmo:EMMO_967080e5_2f42_4eb2_a3a9_c58143e835f9 ;
    owl:annotatedSource :electrochemistry_a462859d_d8bd_48ea_8bde_1576f1248a1e ;
    owl:annotatedTarget "electrode in the form of foil, mesh, wire, rod, tube, powder, pellets, or single crystal of silver"@en .

[] a owl:Axiom ;
    dcterms:source "International Electrotechnical Commission (IEC), IEC 60050 - International Electrotechnical Vocabulary, retrieved from: https://www.electropedia.org" ;
    owl:annotatedProperty emmo:EMMO_967080e5_2f42_4eb2_a3a9_c58143e835f9 ;
    owl:annotatedSource :electrochemistry_a6a69e90_06b5_45b1_83cf_7c0bf39b2914 ;
    owl:annotatedTarget "a chemical reaction in an electrolyte involving a transfer of electrons between chemical components or between chemical components and an electrode"@en .

[] a owl:Axiom ;
    dcterms:source "J. M. Pingarrn et al., Terminology of electrochemical methods of analysis (IUPAC Recommendations 2019), Pure and Applied Chemistry, 4, 92, 2020, 641-694. https://doi.org/10.1515/pac-2018-0109" ;
    owl:annotatedProperty emmo:EMMO_c7b62dd7_063a_4c2a_8504_42f7264ba83f ;
    owl:annotatedSource :electrochemistry_057bb143_639c_472b_99ed_ffa1867f6e63 ;
    owl:annotatedTarget "extremely resistant to many chemicals, impermeable to gases and liquids, and has good electrical conductivity, high hardness and strength, and biocompatibility"@en .

[] a owl:Axiom ;
    dcterms:source "International Electrotechnical Commission (IEC), IEC 60050 - International Electrotechnical Vocabulary, retrieved from: https://www.electropedia.org" ;
    owl:annotatedProperty emmo:EMMO_c7b62dd7_063a_4c2a_8504_42f7264ba83f ;
    owl:annotatedSource :electrochemistry_a6a69e90_06b5_45b1_83cf_7c0bf39b2914 ;
    owl:annotatedTarget "The electrode reaction can also involve other chemical reactions including subreactions on a cell electrode."@en .

[] a owl:Axiom ;
    dcterms:source "Bockris, J. O'M. and Despi, . Aleksandar R. (2011, December 15). Electrochemical reaction. Encyclopedia Britannica. https://www.britannica.com/science/electrochemical-reaction" ;
    owl:annotatedProperty emmo:EMMO_c7b62dd7_063a_4c2a_8504_42f7264ba83f ;
    owl:annotatedSource :electrochemistry_a6a69e90_06b5_45b1_83cf_7c0bf39b2914 ;
    owl:annotatedTarget "any process either caused or accompanied by the passage of an electric current and involving in most cases the transfer of electrons between two substances"@en .

[] a owl:Axiom ;
    dcterms:source "International Electrotechnical Commission (IEC), IEC 60050 - International Electrotechnical Vocabulary, retrieved from: https://www.electropedia.org" ;
    owl:annotatedProperty emmo:EMMO_967080e5_2f42_4eb2_a3a9_c58143e835f9 ;
    owl:annotatedSource :electrochemistry_ac9723d1_bac0_4109_874e_32849de9299b ;
    owl:annotatedTarget "model representing the structure of an electrolyte at an electrode-electrolyte interface by a rigid layer formed by the charge carriers on the surface of the electrode and a diffuse layer formed by mobile ions in the electrolyte."@en .

[] a owl:Axiom ;
    dcterms:source "International Electrotechnical Commission (IEC), IEC 60050 - International Electrotechnical Vocabulary, retrieved from: https://www.electropedia.org" ;
    owl:annotatedProperty emmo:EMMO_967080e5_2f42_4eb2_a3a9_c58143e835f9 ;
    owl:annotatedSource :electrochemistry_ae56cce3_7a7c_4e53_bb58_31e0d642d47e ;
    owl:annotatedTarget "vent of special design which provides protection against the propagation of a flame front from or into the interior of a secondary cell"@en .

[] a owl:Axiom ;
    dcterms:source "International Electrotechnical Commission (IEC), IEC 60050 - International Electrotechnical Vocabulary, retrieved from: https://www.electropedia.org" ;
    owl:annotatedProperty emmo:EMMO_c7b62dd7_063a_4c2a_8504_42f7264ba83f ;
    owl:annotatedSource :electrochemistry_ae56cce3_7a7c_4e53_bb58_31e0d642d47e ;
    owl:annotatedTarget "this flame front may originate from a spark or an external naked flame igniting combustible electrolysis gas"@en .

[] a owl:Axiom ;
    dcterms:source "International Electrotechnical Commission (IEC), IEC 60050 - International Electrotechnical Vocabulary, retrieved from: https://www.electropedia.org" ;
    owl:annotatedProperty emmo:EMMO_c7b62dd7_063a_4c2a_8504_42f7264ba83f ;
    owl:annotatedSource :electrochemistry_aff732a9_238a_4734_977c_b2ba202af126 ;
    owl:annotatedTarget "by convention, a reduction reaction occurs during discharge"@en .

[] a owl:Axiom ;
    dcterms:source "J. M. Pingarrn et al., Terminology of electrochemical methods of analysis (IUPAC Recommendations 2019), Pure and Applied Chemistry, 4, 92, 2020, 641-694. https://doi.org/10.1515/pac-2018-0109" ;
    owl:annotatedProperty emmo:EMMO_967080e5_2f42_4eb2_a3a9_c58143e835f9 ;
    owl:annotatedSource :electrochemistry_b0a0dddb_d942_4af2_b6a7_d7165f4253f1 ;
    owl:annotatedTarget "Electrode of a composite of carbon powder and a pasting liquid (including mineral oil, Nujol, bromoform, bromonaphthalene)."@en .

[] a owl:Axiom ;
    dcterms:source "IUPAC. Compendium of Chemical Terminology, 2nd ed. (the \"Gold Book\"). Compiled by A. D. McNaught and A. Wilkinson. Blackwell Scientific Publications, Oxford (1997). Online version (2019-) created by S. J. Chalk. ISBN 0-9678550-9-8. https://doi.org/10.1351/goldbook." ;
    owl:annotatedProperty emmo:EMMO_967080e5_2f42_4eb2_a3a9_c58143e835f9 ;
    owl:annotatedSource :electrochemistry_b2d11f0d_c1b0_4476_8d17_03b73d31e01f ;
    owl:annotatedTarget "membrane constituted of two or more structural planes of non-identical morphologies"@en .

[] a owl:Axiom ;
    dcterms:source "International Electrotechnical Commission (IEC), IEC 60050 - International Electrotechnical Vocabulary, retrieved from: https://www.electropedia.org" ;
    owl:annotatedProperty emmo:EMMO_967080e5_2f42_4eb2_a3a9_c58143e835f9 ;
    owl:annotatedSource :electrochemistry_b3b3868f_6edd_4ce8_a984_08f9cf391f90 ;
    owl:annotatedTarget "process where molecules split up into ions due to being dissolved"@en .

[] a owl:Axiom ;
    dcterms:source "J. M. Pingarrn et al., Terminology of electrochemical methods of analysis (IUPAC Recommendations 2019), Pure and Applied Chemistry, 4, 92, 2020, 641-694. https://doi.org/10.1515/pac-2018-0109" ;
    owl:annotatedProperty emmo:EMMO_c7b62dd7_063a_4c2a_8504_42f7264ba83f ;
    owl:annotatedSource :electrochemistry_057bb143_639c_472b_99ed_ffa1867f6e63 ;
    owl:annotatedTarget "glassy carbon combines glass-like mechanical characteristics with physical properties similar to graphite, owing to its graphene ribbon structure"@en .

[] a owl:Axiom ;
    dcterms:source "International Electrotechnical Commission (IEC), IEC 60050 - International Electrotechnical Vocabulary, retrieved from: https://www.electropedia.org" ;
    owl:annotatedProperty skos:note ;
    owl:annotatedSource :electrochemistry_b6319c74_d2ce_48c0_a75a_63156776b302 ;
    owl:annotatedTarget "The anode is the negative electrode during discharge and the positive electrode during charge."@en .

[] a owl:Axiom ;
    dcterms:source "International Electrotechnical Commission (IEC), IEC 60050 - International Electrotechnical Vocabulary, retrieved from: https://www.electropedia.org" ;
    owl:annotatedProperty emmo:EMMO_967080e5_2f42_4eb2_a3a9_c58143e835f9 ;
    owl:annotatedSource :electrochemistry_b6319c74_d2ce_48c0_a75a_63156776b302 ;
    owl:annotatedTarget "by convention, cell electrode at which an oxidation reaction occurs"@en .

[] a owl:Axiom ;
    dcterms:source "J. M. Pingarrn et al., Terminology of electrochemical methods of analysis (IUPAC Recommendations 2019), Pure and Applied Chemistry, 4, 92, 2020, 641-694. https://doi.org/10.1515/pac-2018-0109" ;
    owl:annotatedProperty emmo:EMMO_967080e5_2f42_4eb2_a3a9_c58143e835f9 ;
    owl:annotatedSource :electrochemistry_b76a778f_253f_4210_a67f_fb6444d0de26 ;
    owl:annotatedTarget "mercury electrode formed by sequence of mercury drops falling from a small aperture"@en .

[] a owl:Axiom ;
    dcterms:source "International Electrotechnical Commission (IEC), IEC 60050 - International Electrotechnical Vocabulary, retrieved from: https://www.electropedia.org" ;
    owl:annotatedProperty emmo:EMMO_967080e5_2f42_4eb2_a3a9_c58143e835f9 ;
    owl:annotatedSource :electrochemistry_b79d4f9e_5727_4895_8d7f_5fc18d83eb90 ;
    owl:annotatedTarget "an unwanted side reaction"@en .

[] a owl:Axiom ;
    dcterms:source "International Electrotechnical Commission (IEC), IEC 60050 - International Electrotechnical Vocabulary, retrieved from: https://www.electropedia.org" ;
    owl:annotatedProperty emmo:EMMO_c7b62dd7_063a_4c2a_8504_42f7264ba83f ;
    owl:annotatedSource :electrochemistry_b79d4f9e_5727_4895_8d7f_5fc18d83eb90 ;
    owl:annotatedTarget "in a galvanic cell, parasitic reactions may cause inefficiencies or loss of performance"@en .

[] a owl:Axiom ;
    dcterms:source "IEEE Standard Glossary of Stationary Battery Terminology (2016), https://doi.org/10.1109/IEEESTD.2016.7552407" ;
    owl:annotatedProperty emmo:EMMO_967080e5_2f42_4eb2_a3a9_c58143e835f9 ;
    owl:annotatedSource :electrochemistry_b812e9d0_7c58_4455_b3e7_6847f10c8e8a ;
    owl:annotatedTarget "an ion-transport medium, which may be immobilized, in which water is the solvent."@en .

[] a owl:Axiom ;
    dcterms:source "International Electrotechnical Commission (IEC), IEC 60050 - International Electrotechnical Vocabulary, retrieved from: https://www.electropedia.org" ;
    owl:annotatedProperty emmo:EMMO_967080e5_2f42_4eb2_a3a9_c58143e835f9 ;
    owl:annotatedSource :electrochemistry_b851c7e9_60bf_4d3d_abe1_8d08d3d85124 ;
    owl:annotatedTarget "accessible conductive part provided for the connection of an external electric circuit to the negative electrode of the cell"@en .

[] a owl:Axiom ;
    dcterms:source "International Electrotechnical Commission (IEC), IEC 60050 - International Electrotechnical Vocabulary, retrieved from: https://www.electropedia.org" ;
    owl:annotatedProperty emmo:EMMO_967080e5_2f42_4eb2_a3a9_c58143e835f9 ;
    owl:annotatedSource :electrochemistry_b91180e7_97ae_49e2_bf82_5bf720e7fa66 ;
    owl:annotatedTarget "Device that stores electrical energy using a double layer in an electrochemical cell."@en .

[] a owl:Axiom ;
    dcterms:source "J. M. Pingarrn et al., Terminology of electrochemical methods of analysis (IUPAC Recommendations 2019), Pure and Applied Chemistry, 4, 92, 2020, 641-694. https://doi.org/10.1515/pac-2018-0109" ;
    owl:annotatedProperty emmo:EMMO_c7b62dd7_063a_4c2a_8504_42f7264ba83f ;
    owl:annotatedSource :electrochemistry_057bb143_639c_472b_99ed_ffa1867f6e63 ;
    owl:annotatedTarget "one of the most frequently used working electrodes"@en .

[] a owl:Axiom ;
    dcterms:source "J. M. Pingarrn et al., Terminology of electrochemical methods of analysis (IUPAC Recommendations 2019), Pure and Applied Chemistry, 4, 92, 2020, 641-694. https://doi.org/10.1515/pac-2018-0109" ;
    owl:annotatedProperty emmo:EMMO_967080e5_2f42_4eb2_a3a9_c58143e835f9 ;
    owl:annotatedSource :electrochemistry_b9bece97_a511_4cb9_88a2_b5bd5c5e5d74 ;
    owl:annotatedTarget "electrochemical cell with a working electrode, reference electrode, and auxiliary electrode"@en .

[] a owl:Axiom ;
    dcterms:source "International Electrotechnical Commission (IEC), IEC 60050 - International Electrotechnical Vocabulary, retrieved from: https://www.electropedia.org" ;
    owl:annotatedProperty emmo:EMMO_967080e5_2f42_4eb2_a3a9_c58143e835f9 ;
    owl:annotatedSource :electrochemistry_bbb1d95b_72d1_44f6_b07e_a3d7d41ac215 ;
    owl:annotatedTarget "a type of electrode specifically designed for gaseous reactants or products or both"@en .

[] a owl:Axiom ;
    dcterms:source "International Electrotechnical Commission (IEC), IEC 60050 - International Electrotechnical Vocabulary, retrieved from: https://www.electropedia.org" ;
    owl:annotatedProperty emmo:EMMO_967080e5_2f42_4eb2_a3a9_c58143e835f9 ;
    owl:annotatedSource :electrochemistry_bbc77932_643b_4603_a4e8_970ef06a76ad ;
    owl:annotatedTarget "part which insures insulation between the plate (electrode) edges and adjacent plates (electrodes) and the container side walls"@en .

[] a owl:Axiom ;
    dcterms:source "International Electrotechnical Commission (IEC), IEC 60050 - International Electrotechnical Vocabulary, retrieved from: https://www.electropedia.org" ;
    owl:annotatedProperty emmo:EMMO_967080e5_2f42_4eb2_a3a9_c58143e835f9 ;
    owl:annotatedSource :electrochemistry_bed5b5f9_b89d_45e3_a8c2_81b70ae21847 ;
    owl:annotatedTarget "arrangement of cells or batteries wherein in series connected cells or batteries are connected in parallel."@en .

[] a owl:Axiom ;
    dcterms:source "International Electrotechnical Commission (IEC), IEC 60050 - International Electrotechnical Vocabulary, retrieved from: https://www.electropedia.org" ;
    owl:annotatedProperty emmo:EMMO_967080e5_2f42_4eb2_a3a9_c58143e835f9 ;
    owl:annotatedSource :electrochemistry_c05692eb_ae92_4e03_b355_f259f9089cb8 ;
    owl:annotatedTarget "device used to assist in the measurement of the level of electrolyte in a cell"@en .

[] a owl:Axiom ;
    dcterms:source "International Electrotechnical Commission (IEC), IEC 60050 - International Electrotechnical Vocabulary, retrieved from: https://www.electropedia.org" ;
    owl:annotatedProperty emmo:EMMO_967080e5_2f42_4eb2_a3a9_c58143e835f9 ;
    owl:annotatedSource :electrochemistry_c14ae9b3_e4ba_4129_a7b6_afd2d4571de6 ;
    owl:annotatedTarget "permanently sealed gas tight cell without pressure release device"@en .

[] a owl:Axiom ;
    dcterms:source "J. M. Pingarrn et al., Terminology of electrochemical methods of analysis (IUPAC Recommendations 2019), Pure and Applied Chemistry, 4, 92, 2020, 641-694. https://doi.org/10.1515/pac-2018-0109" ;
    owl:annotatedProperty emmo:EMMO_967080e5_2f42_4eb2_a3a9_c58143e835f9 ;
    owl:annotatedSource :electrochemistry_c2024587_3237_474e_8df9_91d10db2df47 ;
    owl:annotatedTarget "electrode whose potential changes with an applied potential"@en .

[] a owl:Axiom ;
    dcterms:source "J. M. Pingarrn et al., Terminology of electrochemical methods of analysis (IUPAC Recommendations 2019), Pure and Applied Chemistry, 4, 92, 2020, 641-694. https://doi.org/10.1515/pac-2018-0109" ;
    owl:annotatedProperty emmo:EMMO_967080e5_2f42_4eb2_a3a9_c58143e835f9 ;
    owl:annotatedSource :electrochemistry_c3f4b34a_0e2c_46f3_baab_4ebd2682d26f ;
    owl:annotatedTarget "An ionic liquid is an electrolyte composed of a salt that is liquid below 100 C. Ionic liquids have found uses in electrochemical analysis, because their unconventional properties include a negligible vapor pressure, a high thermal and electrochemical stability, and exceptional dissolution properties for both organic and inorganic chemical species."@en .

[] a owl:Axiom ;
    dcterms:source "International Electrotechnical Commission (IEC), IEC 60050 - International Electrotechnical Vocabulary, retrieved from: https://www.electropedia.org" ;
    owl:annotatedProperty emmo:EMMO_967080e5_2f42_4eb2_a3a9_c58143e835f9 ;
    owl:annotatedSource :electrochemistry_c4a778c7_33da_4e1a_960e_402a210bfeff ;
    owl:annotatedTarget "platinized platinum electrode saturated by a stream of pure gaseous hydrogen"@en .

[] a owl:Axiom ;
    dcterms:source "International Electrotechnical Commission (IEC), IEC 60050 - International Electrotechnical Vocabulary, retrieved from: https://www.electropedia.org" ;
    owl:annotatedProperty emmo:EMMO_967080e5_2f42_4eb2_a3a9_c58143e835f9 ;
    owl:annotatedSource :electrochemistry_c55ec02c_b727_4df1_97ce_91d7bb5d5e91 ;
    owl:annotatedTarget "unplanned escape of electrolyte, gas or other material from a cell or battery"@en .

[] a owl:Axiom ;
    dcterms:source "International Electrotechnical Commission (IEC), IEC 60050 - International Electrotechnical Vocabulary, retrieved from: https://www.electropedia.org" ;
    owl:annotatedProperty emmo:EMMO_967080e5_2f42_4eb2_a3a9_c58143e835f9 ;
    owl:annotatedSource :electrochemistry_c610d869_cc03_44f0_b40d_ca86e945b9c9 ;
    owl:annotatedTarget "cell from which electrolyte cannot escape regardless of its orientation"@en .

[] a owl:Axiom ;
    dcterms:source "International Electrotechnical Commission (IEC), IEC 60050 - International Electrotechnical Vocabulary, retrieved from: https://www.electropedia.org" ;
    owl:annotatedProperty emmo:EMMO_c7b62dd7_063a_4c2a_8504_42f7264ba83f ;
    owl:annotatedSource :electrochemistry_c610d869_cc03_44f0_b40d_ca86e945b9c9 ;
    owl:annotatedTarget "some vented cells or batteries are designed so as to be non-spillable when operated within the limits specified by the manufacturer"@en .

[] a owl:Axiom ;
    dcterms:source "International Electrotechnical Commission (IEC), IEC 60050 - International Electrotechnical Vocabulary, retrieved from: https://www.electropedia.org" ;
    owl:annotatedProperty emmo:EMMO_967080e5_2f42_4eb2_a3a9_c58143e835f9 ;
    owl:annotatedSource :electrochemistry_c936bfbe_7a0c_4185_a317_db1ce2c3c38c ;
    owl:annotatedTarget "electrochemical immunity produced by an appropriate cathodic polarization."@en .

[] a owl:Axiom ;
    dcterms:source "International Electrotechnical Commission (IEC), IEC 60050 - International Electrotechnical Vocabulary, retrieved from: https://www.electropedia.org" ;
    owl:annotatedProperty skos:note ;
    owl:annotatedSource :electrochemistry_c94c041b_8ea6_43e7_85cc_d2bce7785b4c ;
    owl:annotatedTarget "by convention, an oxidation reaction occurs during discharge"@en .

[] a owl:Axiom ;
    dcterms:source "International Electrotechnical Commission (IEC), IEC 60050 - International Electrotechnical Vocabulary, retrieved from: https://www.electropedia.org" ;
    owl:annotatedProperty emmo:EMMO_967080e5_2f42_4eb2_a3a9_c58143e835f9 ;
    owl:annotatedSource :electrochemistry_c94c041b_8ea6_43e7_85cc_d2bce7785b4c ;
    owl:annotatedTarget "for a device having two electrodes, that electrode having the lower electric potential"@en .

[] a owl:Axiom ;
    dcterms:source "International Electrotechnical Commission (IEC), IEC 60050 - International Electrotechnical Vocabulary, retrieved from: https://www.electropedia.org" ;
    owl:annotatedProperty emmo:EMMO_967080e5_2f42_4eb2_a3a9_c58143e835f9 ;
    owl:annotatedSource :electrochemistry_cc1f854a_ba6c_436e_bd18_c8b9159bbf52 ;
    owl:annotatedTarget "component fitted into the filling hole of a cell with a provision of allowing the venting of electrolysis gas from the cell"@en .

[] a owl:Axiom ;
    dcterms:source "International Electrotechnical Commission (IEC), IEC 60050 - International Electrotechnical Vocabulary, retrieved from: https://www.electropedia.org" ;
    owl:annotatedProperty emmo:EMMO_967080e5_2f42_4eb2_a3a9_c58143e835f9 ;
    owl:annotatedSource :electrochemistry_d5da9948_e95b_4f12_a2d2_10a48f390c52 ;
    owl:annotatedTarget "arrangement of cells or batteries wherein parallel connected cells or batteries are connected in series."@en .

[] a owl:Axiom ;
    dcterms:source "International Electrotechnical Commission (IEC), IEC 60050 - International Electrotechnical Vocabulary, retrieved from: https://www.electropedia.org" ;
    owl:annotatedProperty skos:example ;
    owl:annotatedSource :electrochemistry_d8a78cd2_8107_46dd_a198_0b64676efc00 ;
    owl:annotatedTarget "a connector electrically joins two cells, or a terminal of a cell to a terminal of the battery, or a terminal of the battery to an exterior circuit and also to auxiliary devices"@en .

[] a owl:Axiom ;
    dcterms:source "International Electrotechnical Commission (IEC), IEC 60050 - International Electrotechnical Vocabulary, retrieved from: https://www.electropedia.org" ;
    owl:annotatedProperty emmo:EMMO_967080e5_2f42_4eb2_a3a9_c58143e835f9 ;
    owl:annotatedSource :electrochemistry_d8a78cd2_8107_46dd_a198_0b64676efc00 ;
    owl:annotatedTarget "conductor of electricity used for carrying current between components in an electric circuit"@en .

[] a owl:Axiom ;
    dcterms:source "International Electrotechnical Commission (IEC), IEC 60050 - International Electrotechnical Vocabulary, retrieved from: https://www.electropedia.org" ;
    owl:annotatedProperty emmo:EMMO_967080e5_2f42_4eb2_a3a9_c58143e835f9 ;
    owl:annotatedSource :electrochemistry_d907805f_678b_4ab6_8b56_59631684f84b ;
    owl:annotatedTarget "assembly of one positive plate, one negative plate and the associated separator if any"@en .

[] a owl:Axiom ;
    dcterms:source "J. M. Pingarrn et al., Terminology of electrochemical methods of analysis (IUPAC Recommendations 2019), Pure and Applied Chemistry, 4, 92, 2020, 641-694. https://doi.org/10.1515/pac-2018-0109" ;
    owl:annotatedProperty emmo:EMMO_967080e5_2f42_4eb2_a3a9_c58143e835f9 ;
    owl:annotatedSource :electrochemistry_df78745e_f9db_4830_88f0_8ce074fcb8ff ;
    owl:annotatedTarget "liquid metal electrode used in polarography"@en .

[] a owl:Axiom ;
    dcterms:source "J. M. Pingarrn et al., Terminology of electrochemical methods of analysis (IUPAC Recommendations 2019), Pure and Applied Chemistry, 4, 92, 2020, 641-694. https://doi.org/10.1515/pac-2018-0109" ;
    owl:annotatedProperty emmo:EMMO_967080e5_2f42_4eb2_a3a9_c58143e835f9 ;
    owl:annotatedSource :electrochemistry_e248373f_294f_4ca4_9edf_0ad6653bb64f ;
    owl:annotatedTarget "electrochemical cell in which chemical reactions occur spontaneously and chemical energy is converted into electrical energy."@en .

[] a owl:Axiom ;
    dcterms:references "J. Newman and K. E. Thmoas-Alyea, Electrochemical Systems, 3rd ed. Hoboken, New Jersey: John Wiley & Sons, 2004." ;
    owl:annotatedProperty emmo:EMMO_c7b62dd7_063a_4c2a_8504_42f7264ba83f ;
    owl:annotatedSource :electrochemistry_e248373f_294f_4ca4_9edf_0ad6653bb64f ;
    owl:annotatedTarget "An electrochemical cell that spontaneously produces work."@en .

[] a owl:Axiom ;
    dcterms:source "International Electrotechnical Commission (IEC), IEC 60050 - International Electrotechnical Vocabulary, retrieved from: https://www.electropedia.org" ;
    owl:annotatedProperty emmo:EMMO_c7b62dd7_063a_4c2a_8504_42f7264ba83f ;
    owl:annotatedSource :electrochemistry_e248373f_294f_4ca4_9edf_0ad6653bb64f ;
    owl:annotatedTarget "Electrochemical cell intended to produce electric energy."@en .

[] a owl:Axiom ;
    dcterms:source "International Electrotechnical Commission (IEC), IEC 60050 - International Electrotechnical Vocabulary, retrieved from: https://www.electropedia.org" ;
    owl:annotatedProperty emmo:EMMO_967080e5_2f42_4eb2_a3a9_c58143e835f9 ;
    owl:annotatedSource :electrochemistry_e2a1dae1_05e4_4bd1_a39d_0eb10db482bc ;
    owl:annotatedTarget "method of separating and neutralizing ions by an electric current in an electrolytic cell"@en .

[] a owl:Axiom ;
    dcterms:source "International Electrotechnical Commission (IEC), IEC 60050 - International Electrotechnical Vocabulary, retrieved from: https://www.electropedia.org" ;
    owl:annotatedProperty emmo:EMMO_967080e5_2f42_4eb2_a3a9_c58143e835f9 ;
    owl:annotatedSource :electrochemistry_e931087f_7681_4096_b200_5223bcc47eb4 ;
    owl:annotatedTarget "electrochemical cell intended to produce chemical reactions"@en .

[] a owl:Axiom ;
    dcterms:references "J. Newman and K. E. Thmoas-Alyea, Electrochemical Systems, 3rd ed. Hoboken, New Jersey: John Wiley & Sons, 2004." ;
    owl:annotatedProperty emmo:EMMO_c7b62dd7_063a_4c2a_8504_42f7264ba83f ;
    owl:annotatedSource :electrochemistry_e931087f_7681_4096_b200_5223bcc47eb4 ;
    owl:annotatedTarget "An electrochemical cell that requires input of work to drive the reaction."@en .

[] a owl:Axiom ;
    dcterms:source "J. M. Pingarrn et al., Terminology of electrochemical methods of analysis (IUPAC Recommendations 2019), Pure and Applied Chemistry, 4, 92, 2020, 641-694. https://doi.org/10.1515/pac-2018-0109" ;
    owl:annotatedProperty emmo:EMMO_c7b62dd7_063a_4c2a_8504_42f7264ba83f ;
    owl:annotatedSource :electrochemistry_e931087f_7681_4096_b200_5223bcc47eb4 ;
    owl:annotatedTarget "Electrochemical cell in which electrical energy is converted into chemical energy."@en .

[] a owl:Axiom ;
    dcterms:source "International Electrotechnical Commission (IEC), IEC 60050 - International Electrotechnical Vocabulary, retrieved from: https://www.electropedia.org" ;
    owl:annotatedProperty emmo:EMMO_967080e5_2f42_4eb2_a3a9_c58143e835f9 ;
    owl:annotatedSource :electrochemistry_e94f6d42_35e4_4f9f_bb74_5e0628bbd454 ;
    owl:annotatedTarget "case with multiple separate cell compartments"@en .

[] a owl:Axiom ;
    dcterms:source "International Electrotechnical Commission (IEC), IEC 60050 - International Electrotechnical Vocabulary, retrieved from: https://www.electropedia.org" ;
    owl:annotatedProperty emmo:EMMO_967080e5_2f42_4eb2_a3a9_c58143e835f9 ;
    owl:annotatedSource :electrochemistry_ec1dce8b_bb46_41a9_b532_6bed381aa557 ;
    owl:annotatedTarget "secondary cell having a cover provided with an opening through which products of electrolysis and evaporation are allowed to escape freely from the cell to the atmosphere"@en .

[] a owl:Axiom ;
    dcterms:source "J. M. Pingarrn et al., Terminology of electrochemical methods of analysis (IUPAC Recommendations 2019), Pure and Applied Chemistry, 4, 92, 2020, 641-694. https://doi.org/10.1515/pac-2018-0109" ;
    owl:annotatedProperty emmo:EMMO_967080e5_2f42_4eb2_a3a9_c58143e835f9 ;
    owl:annotatedSource :electrochemistry_ec6f3d6f_bdf5_418f_9314_3ef2ff528103 ;
    owl:annotatedTarget "development of a carbon paste electrode that is screen printed using a carbon/polymer mixture of suitable composition"@en .

[] a owl:Axiom ;
    dcterms:source "International Electrotechnical Commission (IEC), IEC 60050 - International Electrotechnical Vocabulary, retrieved from: https://www.electropedia.org" ;
    owl:annotatedProperty emmo:EMMO_967080e5_2f42_4eb2_a3a9_c58143e835f9 ;
    owl:annotatedSource :electrochemistry_efc4f7ab_850d_443c_a17f_184983021f96 ;
    owl:annotatedTarget "arrangement of cells or batteries wherein all the positive terminals and all the negative terminals, respectively, are connected together."@en .

[] a owl:Axiom ;
    dcterms:source "A. J. Bard, G. Inzelt, and F. Scholz, Eds., Electrochemical Dictionary, 2nd Edition. Berlin: Springer-Verlag, 2012. DOI: https://doi.org/10.1007/978-3-642-29551-5" ;
    owl:annotatedProperty emmo:EMMO_967080e5_2f42_4eb2_a3a9_c58143e835f9 ;
    owl:annotatedSource :electrochemistry_f0c24970_4c14_4207_bd78_5f2181a67085 ;
    owl:annotatedTarget "the process of forming a film or a bulk material using an electrochemical process where the electrons are supplied by an external power supply"@en .

[] a owl:Axiom ;
    dcterms:source "International Electrotechnical Commission (IEC), IEC 60050 - International Electrotechnical Vocabulary, retrieved from: https://www.electropedia.org" ;
    owl:annotatedProperty emmo:EMMO_967080e5_2f42_4eb2_a3a9_c58143e835f9 ;
    owl:annotatedSource :electrochemistry_f330680b_347e_45b3_9113_5ce09d18d60b ;
    owl:annotatedTarget "vent of special design which allows to release gas from a cell in order to avoid excessive internal pressure and thereby to preclude rupture or explosion of the cell container"@en .

[] a owl:Axiom ;
    dcterms:source "International Electrotechnical Commission (IEC), IEC 60050 - International Electrotechnical Vocabulary, retrieved from: https://www.electropedia.org" ;
    owl:annotatedProperty emmo:EMMO_967080e5_2f42_4eb2_a3a9_c58143e835f9 ;
    owl:annotatedSource :electrochemistry_f47611a2_e081_47f0_b287_3fda5f706154 ;
    owl:annotatedTarget "chemical reaction which occurs in addition to the main process"@en .

[] a owl:Axiom ;
    dcterms:source "International Electrotechnical Commission (IEC), IEC 60050 - International Electrotechnical Vocabulary, retrieved from: https://www.electropedia.org" ;
    owl:annotatedProperty emmo:EMMO_967080e5_2f42_4eb2_a3a9_c58143e835f9 ;
    owl:annotatedSource :electrochemistry_f4a1323a_ce2b_4c1a_b89d_c80170110ed6 ;
    owl:annotatedTarget "electrode reaction in which reduction  occurs at the cathode"@en .

[] a owl:Axiom ;
    dcterms:source "International Electrotechnical Commission (IEC), IEC 60050 - International Electrotechnical Vocabulary, retrieved from: https://www.electropedia.org" ;
    owl:annotatedProperty emmo:EMMO_c7b62dd7_063a_4c2a_8504_42f7264ba83f ;
    owl:annotatedSource :electrochemistry_f4a1323a_ce2b_4c1a_b89d_c80170110ed6 ;
    owl:annotatedTarget "electrode reaction involving an electrochemical reduction"@en .

[] a owl:Axiom ;
    dcterms:source "A. J. Bard, G. Inzelt, and F. Scholz, Eds., Electrochemical Dictionary, 2nd Edition. Berlin: Springer-Verlag, 2012. DOI: https://doi.org/10.1007/978-3-642-29551-5" ;
    owl:annotatedProperty emmo:EMMO_c7b62dd7_063a_4c2a_8504_42f7264ba83f ;
    owl:annotatedSource :electrochemistry_f4a1323a_ce2b_4c1a_b89d_c80170110ed6 ;
    owl:annotatedTarget "electrode reaction, where the energy of electrons in the working electrode is higher than the LUMO orbital of the substrate"@en .

[] a owl:Axiom ;
    dcterms:source "J. M. Pingarrn et al., Terminology of electrochemical methods of analysis (IUPAC Recommendations 2019), Pure and Applied Chemistry, 4, 92, 2020, 641-694. https://doi.org/10.1515/pac-2018-0109" ;
    owl:annotatedProperty emmo:EMMO_967080e5_2f42_4eb2_a3a9_c58143e835f9 ;
    owl:annotatedSource :electrochemistry_f6fcd255_248d_4603_b128_04dab960a676 ;
    owl:annotatedTarget "electrode that responds to one, or more than one, species in the solution being investigated, with no appreciable change of bulk solution composition during the measurement"@en .

[] a owl:Axiom ;
    dcterms:source "J. Newman and K. E. Thmoas-Alyea, Electrochemical Systems, 3rd ed. Hoboken, New Jersey: John Wiley & Sons, 2004." ;
    owl:annotatedProperty emmo:EMMO_967080e5_2f42_4eb2_a3a9_c58143e835f9 ;
    owl:annotatedSource :electrochemistry_fb0d9eef_92af_4628_8814_e065ca255d59 ;
    owl:annotatedTarget "a material in which the mobile species are ions and free movement of electrons is blocked."@en .

[] a owl:Axiom ;
    dcterms:source "J. M. Pingarrn et al., Terminology of electrochemical methods of analysis (IUPAC Recommendations 2019), Pure and Applied Chemistry, 4, 92, 2020, 641-694. https://doi.org/10.1515/pac-2018-0109" ;
    owl:annotatedProperty emmo:EMMO_c7b62dd7_063a_4c2a_8504_42f7264ba83f ;
    owl:annotatedSource :electrochemistry_fb0d9eef_92af_4628_8814_e065ca255d59 ;
    owl:annotatedTarget "conducting medium in which the flow of electric current is accompanied by the movement of ions"@en .

[] a owl:Axiom ;
    dcterms:source "International Electrotechnical Commission (IEC), IEC 60050 - International Electrotechnical Vocabulary, retrieved from: https://www.electropedia.org" ;
    owl:annotatedProperty emmo:EMMO_c7b62dd7_063a_4c2a_8504_42f7264ba83f ;
    owl:annotatedSource :electrochemistry_fb0d9eef_92af_4628_8814_e065ca255d59 ;
    owl:annotatedTarget "liquid or solid substance containing mobile ions that render it conductive"@en .

[] a owl:Axiom ;
    dcterms:source "J. M. Pingarrn et al., Terminology of electrochemical methods of analysis (IUPAC Recommendations 2019), Pure and Applied Chemistry, 4, 92, 2020, 641-694. https://doi.org/10.1515/pac-2018-0109" ;
    owl:annotatedProperty emmo:EMMO_c7b62dd7_063a_4c2a_8504_42f7264ba83f ;
    owl:annotatedSource :electrochemistry_fb0d9eef_92af_4628_8814_e065ca255d59 ;
    owl:annotatedTarget "substance that provides ions on dissolution in a solvent or on melting"@en .

[] a owl:Axiom ;
    dcterms:source "J. M. Pingarrn et al., Terminology of electrochemical methods of analysis (IUPAC Recommendations 2019), Pure and Applied Chemistry, 4, 92, 2020, 641-694. https://doi.org/10.1515/pac-2018-0109" ;
    owl:annotatedProperty emmo:EMMO_967080e5_2f42_4eb2_a3a9_c58143e835f9 ;
    owl:annotatedSource :electrochemistry_fb988878_ee54_4350_9ee9_228c00c3ad35 ;
    owl:annotatedTarget "electrode at which one or more electroactive substances undergo reaction in the solution being investigated"@en .

[] a owl:Axiom ;
    dcterms:source "International Electrotechnical Commission (IEC), IEC 60050 - International Electrotechnical Vocabulary, retrieved from: https://www.electropedia.org" ;
    owl:annotatedProperty emmo:EMMO_967080e5_2f42_4eb2_a3a9_c58143e835f9 ;
    owl:annotatedSource :electrochemistry_0f007072_a8dd_4798_b865_1bf9363be627 ;
    owl:annotatedTarget "electronically conductive part in electric contact with a medium of lower electronic conductivity and intended to perform one or more of the functions of emitting charge carriers to or receiving charge carriers from that medium or to establish an electric field in that medium"@en .

[] a owl:Axiom ;
    dcterms:source "J. M. Pingarrn et al., Terminology of electrochemical methods of analysis (IUPAC Recommendations 2019), Pure and Applied Chemistry, 4, 92, 2020, 641-694. https://doi.org/10.1515/pac-2018-0109" ;
    owl:annotatedProperty emmo:EMMO_c7b62dd7_063a_4c2a_8504_42f7264ba83f ;
    owl:annotatedSource :electrochemistry_0f007072_a8dd_4798_b865_1bf9363be627 ;
    owl:annotatedTarget "Electron conductor in an electrochemical cell connected to the external circuit."@en .

[] a owl:Axiom ;
    dcterms:source "International Electrotechnical Commission (IEC), IEC 60050 - International Electrotechnical Vocabulary, retrieved from: https://www.electropedia.org" ;
    owl:annotatedProperty emmo:EMMO_967080e5_2f42_4eb2_a3a9_c58143e835f9 ;
    owl:annotatedSource :electrochemistry_0f827b54_370d_4c63_99a6_80f13b24e55e ;
    owl:annotatedTarget "evolution of gas resulting from electrolysis of the water in the electrolyte of a cell"@en .

[] a owl:Axiom ;
    dcterms:source "International Electrotechnical Commission (IEC), IEC 60050 - International Electrotechnical Vocabulary, retrieved from: https://www.electropedia.org" ;
    owl:annotatedProperty emmo:EMMO_967080e5_2f42_4eb2_a3a9_c58143e835f9 ;
    owl:annotatedSource :electrochemistry_113e0469_8ae0_407f_892d_4b988f8d8a08 ;
    owl:annotatedTarget "electrochemical cell that has two half-cells separated by a wall permeable to ions, both containing the same electrolyte differing only in their temperatures."@en .

[] a owl:Axiom ;
    dcterms:source "J. M. Pingarrn et al., Terminology of electrochemical methods of analysis (IUPAC Recommendations 2019), Pure and Applied Chemistry, 4, 92, 2020, 641-694. https://doi.org/10.1515/pac-2018-0109" ;
    owl:annotatedProperty emmo:EMMO_967080e5_2f42_4eb2_a3a9_c58143e835f9 ;
    owl:annotatedSource :electrochemistry_1152ae6b_8b57_4d99_912e_40c6a29342fb ;
    owl:annotatedTarget "mass m of electrochemically-transformed substance is proportional to the charge Q passed, m  Q."@en .

[] a owl:Axiom ;
    dcterms:source "IUPAC. Compendium of Chemical Terminology, 2nd ed. (the \"Gold Book\"). Compiled by A. D. McNaught and A. Wilkinson. Blackwell Scientific Publications, Oxford (1997). Online version (2019-) created by S. J. Chalk. ISBN 0-9678550-9-8. https://doi.org/10.1351/goldbook." ;
    owl:annotatedProperty emmo:EMMO_967080e5_2f42_4eb2_a3a9_c58143e835f9 ;
    owl:annotatedSource :electrochemistry_15325775_6d4c_4192_82f1_e4feca9de426 ;
    owl:annotatedTarget "A membrane having ion-exchange groups:"@en .

[] a owl:Axiom ;
    dcterms:source "International Electrotechnical Commission (IEC), IEC 60050 - International Electrotechnical Vocabulary, retrieved from: https://www.electropedia.org" ;
    owl:annotatedProperty emmo:EMMO_967080e5_2f42_4eb2_a3a9_c58143e835f9 ;
    owl:annotatedSource :electrochemistry_15b852b5_19cc_49ab_849f_7df6175fb2be ;
    owl:annotatedTarget "electrolyte on the cathode side of an electrochemical cell that is divided into compartments."@en .

[] a owl:Axiom ;
    dcterms:source "A. J. Bard, G. Inzelt, and F. Scholz, Eds., Electrochemical Dictionary, 2nd Edition. Berlin: Springer-Verlag, 2012. DOI: https://doi.org/10.1007/978-3-642-29551-5" ;
    owl:annotatedProperty emmo:EMMO_c7b62dd7_063a_4c2a_8504_42f7264ba83f ;
    owl:annotatedSource :electrochemistry_15b852b5_19cc_49ab_849f_7df6175fb2be ;
    owl:annotatedTarget "Electrolyte solution in the cathodic compartment of an electrolysis cell or galvanic cell, i.e., in that part of the cell where the cathode is placed."@en .

[] a owl:Axiom ;
    dcterms:source "International Electrotechnical Commission (IEC), IEC 60050 - International Electrotechnical Vocabulary, retrieved from: https://www.electropedia.org" ;
    owl:annotatedProperty emmo:EMMO_967080e5_2f42_4eb2_a3a9_c58143e835f9 ;
    owl:annotatedSource :electrochemistry_187326b9_1089_4122_8e7e_1a0bcba210a1 ;
    owl:annotatedTarget "electrode polarization associated with a cathodic reaction"@en .

[] a owl:Axiom ;
    dcterms:source "International Electrotechnical Commission (IEC), IEC 60050 - International Electrotechnical Vocabulary, retrieved from: https://www.electropedia.org" ;
    owl:annotatedProperty emmo:EMMO_967080e5_2f42_4eb2_a3a9_c58143e835f9 ;
    owl:annotatedSource :electrochemistry_1a2eb6db_c927_4039_aea0_8dfab060fd27 ;
    owl:annotatedTarget "ridges in the bottom of the case which support the plate pack (electrode stack) and thus create a space which allows the active material detached from the plates (electrodes) to settle without causing a short-circuit between the plates (electrodes)"@en .

[] a owl:Axiom ;
    dcterms:source "International Electrotechnical Commission (IEC), IEC 60050 - International Electrotechnical Vocabulary, retrieved from: https://www.electropedia.org" ;
    owl:annotatedProperty emmo:EMMO_967080e5_2f42_4eb2_a3a9_c58143e835f9 ;
    owl:annotatedSource :electrochemistry_1aec4cc0_82d5_4042_a657_ed7fe291c3d8 ;
    owl:annotatedTarget "container for the plate pack or packs and electrolyte of a cell or cells made of a material impervious to the electrolyte"@en .

[] a owl:Axiom ;
    dcterms:source "International Electrotechnical Commission (IEC), IEC 60050 - International Electrotechnical Vocabulary, retrieved from: https://www.electropedia.org" ;
    owl:annotatedProperty emmo:EMMO_967080e5_2f42_4eb2_a3a9_c58143e835f9 ;
    owl:annotatedSource :electrochemistry_1e33e37e_d7c9_4701_ba6d_a09456a13aaf ;
    owl:annotatedTarget "part used to close the case normally having holes for filling, topping-up, gas escape, terminals, etc."@en .

[] a owl:Axiom ;
    dcterms:source "IUPAC. Compendium of Chemical Terminology, 2nd ed. (the \"Gold Book\"). Compiled by A. D. McNaught and A. Wilkinson. Blackwell Scientific Publications, Oxford (1997). Online version (2019-) created by S. J. Chalk. ISBN 0-9678550-9-8. https://doi.org/10.1351/goldbook." ;
    owl:annotatedProperty emmo:EMMO_967080e5_2f42_4eb2_a3a9_c58143e835f9 ;
    owl:annotatedSource :electrochemistry_1e72986e_e19f_4c24_8663_cadd4318bd72 ;
    owl:annotatedTarget "the symbolic representation of a chemical reaction in the form of symbols and formulae, wherein the reactant entities are given on the left-hand side and the product entities on the right-hand side"@en .

[] a owl:Axiom ;
    dcterms:source "J. M. Pingarrn et al., Terminology of electrochemical methods of analysis (IUPAC Recommendations 2019), Pure and Applied Chemistry, 4, 92, 2020, 641-694. https://doi.org/10.1515/pac-2018-0109" ;
    owl:annotatedProperty emmo:EMMO_967080e5_2f42_4eb2_a3a9_c58143e835f9 ;
    owl:annotatedSource :electrochemistry_1fc5642c_b7b2_43bf_ad20_f96001db8800 ;
    owl:annotatedTarget "electrolyte solution, the ions of which are electroinactive in the range of applied potential being studied, and whose ionic strength (and, therefore, contribution to the overall conductivity) is usually much greater than the concentration of an electroactive substance to be dissolved in it."@en .

[] a owl:Axiom ;
    dcterms:source "A. J. Bard, G. Inzelt, and F. Scholz, Eds., Electrochemical Dictionary, 2nd Edition. Berlin: Springer-Verlag, 2012. DOI: https://doi.org/10.1007/978-3-642-29551-5" ;
    owl:annotatedProperty emmo:EMMO_967080e5_2f42_4eb2_a3a9_c58143e835f9 ;
    owl:annotatedSource :electrochemistry_212af058_3bbb_419f_a9c6_90ba9ebb3706 ;
    owl:annotatedTarget "A good electron conductor support designed to transfer electrons from the external circuit to the active materials of the cell."@en .

[] a owl:Axiom ;
    dcterms:source "International Electrotechnical Commission (IEC), IEC 60050 - International Electrotechnical Vocabulary, retrieved from: https://www.electropedia.org" ;
    owl:annotatedProperty emmo:EMMO_967080e5_2f42_4eb2_a3a9_c58143e835f9 ;
    owl:annotatedSource :electrochemistry_27662d03_1bcf_4393_a239_32e31b760839 ;
    owl:annotatedTarget "finished assembly of the positive and negative plate (electrode) groups with interleaved separators and terminals or intercell connectors"@en .

[] a owl:Axiom ;
    dcterms:source "International Electrotechnical Commission (IEC), IEC 60050 - International Electrotechnical Vocabulary, retrieved from: https://www.electropedia.org" ;
    owl:annotatedProperty emmo:EMMO_967080e5_2f42_4eb2_a3a9_c58143e835f9 ;
    owl:annotatedSource :electrochemistry_27a81a51_e8d7_42fb_834f_0d068fa45d89 ;
    owl:annotatedTarget "solution which has the same concentration of a solute as one that is in equilibrium with undissolved solute at specified values of the temperature and pressure" .

[] a owl:Axiom ;
    dcterms:source "International Electrotechnical Commission (IEC), IEC 60050 - International Electrotechnical Vocabulary, retrieved from: https://www.electropedia.org" ;
    owl:annotatedProperty emmo:EMMO_967080e5_2f42_4eb2_a3a9_c58143e835f9 ;
    owl:annotatedSource :electrochemistry_28213033_4c74_441c_81c4_a0cad05f9eb6 ;
    owl:annotatedTarget "electrode polarization associated with an anodic reaction"@en .

[] a owl:Axiom ;
    dcterms:source "IUPAC. Compendium of Chemical Terminology, 2nd ed. (the \"Gold Book\"). Compiled by A. D. McNaught and A. Wilkinson. Blackwell Scientific Publications, Oxford (1997). Online version (2019-) created by S. J. Chalk. ISBN 0-9678550-9-8. https://doi.org/10.1351/goldbook." ;
    owl:annotatedProperty emmo:EMMO_967080e5_2f42_4eb2_a3a9_c58143e835f9 ;
    owl:annotatedSource :electrochemistry_2a40b878_7d09_49db_91b2_d0ee30192284 ;
    owl:annotatedTarget "for solutions in protic solvents, the universal reference electrode for which, under standard conditions, the standard electrode potential (H+ / H2) is zero at all temperatures"@en .

[] a owl:Axiom ;
    dcterms:source "A. J. Bard, G. Inzelt, and F. Scholz, Eds., Electrochemical Dictionary, 2nd Edition. Berlin: Springer-Verlag, 2012. DOI: https://doi.org/10.1007/978-3-642-29551-5" ;
    owl:annotatedProperty emmo:EMMO_967080e5_2f42_4eb2_a3a9_c58143e835f9 ;
    owl:annotatedSource :electrochemistry_2b50cdac_581f_48b9_87ca_bad5138ab58d ;
    owl:annotatedTarget "a double layer of charges exists at the interface between two conducting media: One side carries a positive excess charge, which is balanced by a negative excess of equal magnitude on the other side."@en .

[] a owl:Axiom ;
    dcterms:source "J. M. Pingarrn et al., Terminology of electrochemical methods of analysis (IUPAC Recommendations 2019), Pure and Applied Chemistry, 4, 92, 2020, 641-694. https://doi.org/10.1515/pac-2018-0109" ;
    owl:annotatedProperty emmo:EMMO_967080e5_2f42_4eb2_a3a9_c58143e835f9 ;
    owl:annotatedSource :electrochemistry_2d32a81a_2148_41bd_84fb_467aa8de4a8f ;
    owl:annotatedTarget "foil, wire, disc, or mesh electrode made of platinum, which is the most commonly used metallic working electrode in electrochemistry"@en .

[] a owl:Axiom ;
    dcterms:source "International Electrotechnical Commission (IEC), IEC 60050 - International Electrotechnical Vocabulary, retrieved from: https://www.electropedia.org" ;
    owl:annotatedProperty emmo:EMMO_967080e5_2f42_4eb2_a3a9_c58143e835f9 ;
    owl:annotatedSource :electrochemistry_2e3e14f9_4cb8_45b2_908e_47eec893dec8 ;
    owl:annotatedTarget "electrochemical reaction involving the transfer of electrons between electrolyte and electrode"@en .

[] a owl:Axiom ;
    dcterms:source "A. J. Bard, G. Inzelt, and F. Scholz, Eds., Electrochemical Dictionary, 2nd Edition. Berlin: Springer-Verlag, 2012. DOI: https://doi.org/10.1007/978-3-642-29551-5" ;
    owl:annotatedProperty emmo:EMMO_c7b62dd7_063a_4c2a_8504_42f7264ba83f ;
    owl:annotatedSource :electrochemistry_2e3e14f9_4cb8_45b2_908e_47eec893dec8 ;
    owl:annotatedTarget "An interfacial reaction that necessarily involves a charge-transfer step."@en .

[] a owl:Axiom ;
    dcterms:source "International Electrotechnical Commission (IEC), IEC 60050 - International Electrotechnical Vocabulary, retrieved from: https://www.electropedia.org" ;
    owl:annotatedProperty emmo:EMMO_967080e5_2f42_4eb2_a3a9_c58143e835f9 ;
    owl:annotatedSource :electrochemistry_2e6933aa_4522_4f16_a437_37110e6cbd0d ;
    owl:annotatedTarget "accumulation or depletion of electric charges at an electrode, resulting in a difference between the electrode potential with current flow, and the potential without current flow or equilibrium electrode potential"@en .

[] a owl:Axiom ;
    dcterms:source "International Electrotechnical Commission (IEC), IEC 60050 - International Electrotechnical Vocabulary, retrieved from: https://www.electropedia.org" ;
    owl:annotatedProperty emmo:EMMO_967080e5_2f42_4eb2_a3a9_c58143e835f9 ;
    owl:annotatedSource :electrochemistry_328c6e36_3706_4d92_abae_432fa3adb2a0 ;
    owl:annotatedTarget "internal component used to reduce the amount of electrolyte loss due to electrolyte spray being carried in the gas and/or by electrolyte movement"@en .

[] a owl:Axiom ;
    dcterms:source "International Electrotechnical Commission (IEC), IEC 60050 - International Electrotechnical Vocabulary, retrieved from: https://www.electropedia.org" ;
    owl:annotatedProperty emmo:EMMO_c7b62dd7_063a_4c2a_8504_42f7264ba83f ;
    owl:annotatedSource :electrochemistry_328c6e36_3706_4d92_abae_432fa3adb2a0 ;
    owl:annotatedTarget "a cell baffle has a second function in protecting the plate pack from damage by objects inserted through the filling hole"@en .

[] a owl:Axiom ;
    dcterms:source "International Electrotechnical Commission (IEC), IEC 60050 - International Electrotechnical Vocabulary, retrieved from: https://www.electropedia.org" ;
    owl:annotatedProperty emmo:EMMO_967080e5_2f42_4eb2_a3a9_c58143e835f9 ;
    owl:annotatedSource :electrochemistry_331e6cca_f260_4bf8_af55_35304fe1bbe0 ;
    owl:annotatedTarget "in an electrochemical cell, device made of insulating material permeable to the ions of the electrolyte and prohibiting totally or partially the mixing of the substances on both sides."@en .

[] a owl:Axiom ;
    dcterms:source "International Electrotechnical Commission (IEC), IEC 60050 - International Electrotechnical Vocabulary, retrieved from: https://www.electropedia.org" ;
    owl:annotatedProperty emmo:EMMO_967080e5_2f42_4eb2_a3a9_c58143e835f9 ;
    owl:annotatedSource :electrochemistry_34bc54e3_de4c_41f8_8d3a_d77c951ee23a ;
    owl:annotatedTarget "needle-like or tree-like formation of crystalline growth formed during deposition of a material"@en .

[] a owl:Axiom ;
    dcterms:source "International Electrotechnical Commission (IEC), IEC 60050 - International Electrotechnical Vocabulary, retrieved from: https://www.electropedia.org" ;
    owl:annotatedProperty skos:note ;
    owl:annotatedSource :electrochemistry_35c650ab_3b23_4938_b312_1b0dede2e6d5 ;
    owl:annotatedTarget "The cathode is the positive electrode during discharge and the negative electrode during charge."@en .

[] a owl:Axiom ;
    dcterms:source "International Electrotechnical Commission (IEC), IEC 60050 - International Electrotechnical Vocabulary, retrieved from: https://www.electropedia.org" ;
    owl:annotatedProperty emmo:EMMO_967080e5_2f42_4eb2_a3a9_c58143e835f9 ;
    owl:annotatedSource :electrochemistry_35c650ab_3b23_4938_b312_1b0dede2e6d5 ;
    owl:annotatedTarget "by convention, cell electrode at which, a reduction reaction occurs"@en .

[] a owl:Axiom ;
    dcterms:references "J. Newman and K. E. Thmoas-Alyea, Electrochemical Systems, 3rd ed. Hoboken, New Jersey: John Wiley & Sons, 2004." ;
    owl:annotatedProperty emmo:EMMO_967080e5_2f42_4eb2_a3a9_c58143e835f9 ;
    owl:annotatedSource :electrochemistry_3663991d_9319_4f7a_922b_f0e428b58801 ;
    owl:annotatedTarget "porous electrodes consist of porous matrices of a single reactive electronic conductor or a mixture of solids that include essentially non-conducting, reactive materials in addition to electronic conductors. An electrolytic solution fills the void spaces of the porous matrix."@en .

[] a owl:Axiom ;
    dcterms:source "International Electrotechnical Commission (IEC), IEC 60050 - International Electrotechnical Vocabulary, retrieved from: https://www.electropedia.org" ;
    owl:annotatedProperty emmo:EMMO_967080e5_2f42_4eb2_a3a9_c58143e835f9 ;
    owl:annotatedSource :electrochemistry_3f6c9e09_5f23_41cc_9f85_7de365cef089 ;
    owl:annotatedTarget "gradual and slow spreading of an electrolyte film on the external surface of a cell or battery"@en .

[] a owl:Axiom ;
    dcterms:source "International Electrotechnical Commission (IEC), IEC 60050 - International Electrotechnical Vocabulary, retrieved from: https://www.electropedia.org" ;
    owl:annotatedProperty emmo:EMMO_c7b62dd7_063a_4c2a_8504_42f7264ba83f ;
    owl:annotatedSource :electrochemistry_3f6c9e09_5f23_41cc_9f85_7de365cef089 ;
    owl:annotatedTarget "electrolyte creep is sometimes indicated by the presence of a visible solid deposit or wet spots"@en .

[] a owl:Axiom ;
    dcterms:source "International Electrotechnical Commission (IEC), IEC 60050 - International Electrotechnical Vocabulary, retrieved from: https://www.electropedia.org" ;
    owl:annotatedProperty emmo:EMMO_967080e5_2f42_4eb2_a3a9_c58143e835f9 ;
    owl:annotatedSource :electrochemistry_3f70e5c5_67f0_483e_998b_b83b7739c4bc ;
    owl:annotatedTarget "conductive part of a device, electric circuit or electric network, provided for connecting that device, electric circuit or electric network to one or more external conductors"@en .

